<?xml version="1.0" encoding="utf-8"?>
<rdf:RDF
  xmlns:rdfs="http://www.w3.org/2000/01/rdf-schema#"
  xmlns:dct="http://purl.org/dc/terms/"
  xmlns:dcat="http://www.w3.org/ns/dcat#"
  xmlns:adms="http://www.w3.org/ns/adms#"
  xmlns:dcatapit="http://dati.gov.it/onto/dcatapit#"
  xmlns:vcard="http://www.w3.org/2006/vcard/ns#"
  xmlns:xkos="http://rdf-vocabulary.ddialliance.org/xkos#"
  xmlns:foaf="http://xmlns.com/foaf/0.1/"
  xmlns:ndc="https://w3id.org/italia/onto/NDC/"
  xmlns:skos="http://www.w3.org/2004/02/skos/core#"
  xmlns:clvapit="https://w3id.org/italia/onto/CLV/"
  xmlns:l0="https://w3id.org/italia/onto/l0/"
  xmlns:indicator="https://w3id.org/italia/onto/Indicator/"
  xmlns:rdf="http://www.w3.org/1999/02/22-rdf-syntax-ns#"
>
  <rdfs:Property rdf:about="http://purl.org/dc/terms/license"/>
  <skos:ConceptScheme rdf:about="https://w3id.org/italia/controlled-vocabulary/classifications-for-indicators/indicator-types">
    <rdf:type rdf:resource="http://www.w3.org/ns/adms#Asset"/>
    <rdf:type rdf:resource="http://dati.gov.it/onto/dcatapit#Dataset"/>
    <dct:title xml:lang="en">Types of Indicators Controlled Vocabulary</dct:title>
    <dct:title xml:lang="it">Vocabolario Controllato dei tipi di indicatori</dct:title>
    <dct:description xml:lang="en">This is the Types of Indicators controlled vocabulary. Indicators in fact can be indicators of outcome, of process and so on.</dct:description>
    <dct:description xml:lang="it">Questo è il vocabolario controllato dei tipi di indicatori. GLi indicatori infatti possono essere di processo, di risultato o esito e così via.</dct:description>
    <rdfs:comment xml:lang="en">This is the Types of Indicators controlled vocabulary. Indicators in fact can be indicators of outcome, of process and so on.</rdfs:comment>
    <rdfs:comment xml:lang="it">Questo è il vocabolario controllato dei tipi di indicatori. GLi indicatori infatti possono essere di processo, di risultato o esito e così via.</rdfs:comment>
    <rdfs:label xml:lang="en">Types of Indicators Controlled Vocabulary</rdfs:label>
    <rdfs:label xml:lang="it">Vocabolario Controllato dei tipi di indicatori</rdfs:label>
    <dct:type rdf:resource="http://purl.org/adms/assettype/CodeList"/>
    <xkos:numberOfLevels>1</xkos:numberOfLevels>
    <ndc:keyConcept>indicator-types</ndc:keyConcept>
    <adms:representationTechnique rdf:resource="http://purl.org/adms/representationtechnique/SKOS"/>
    <dct:identifier>https://w3id.org/italia/controlled-vocabulary/classifications-for-indicators/indicator-types</dct:identifier>
    <dct:rightsHolder>
      <dcatapit:Agent rdf:about="https://w3id.org/italia/data/public-organization/MDS">
        <rdf:type rdf:resource="http://xmlns.com/foaf/0.1/Agent"/>
        <dct:identifier>MDS</dct:identifier>
        <foaf:name xml:lang="it">Ministero della Salute</foaf:name>
      </dcatapit:Agent>
    </dct:rightsHolder>
    <dct:creator>
      <dcatapit:Agent rdf:about="https://w3id.org/italia/data/public-organization/agid">
        <rdf:type rdf:resource="http://xmlns.com/foaf/0.1/Agent"/>
        <dct:identifier>agid</dct:identifier>
        <foaf:name xml:lang="it">Agenzia per l'Italia Digitale</foaf:name>
        <foaf:name xml:lang="en">Italian Digital Agency</foaf:name>
      </dcatapit:Agent>
    </dct:creator>
    <dct:creator>
      <dcatapit:Agent rdf:about="https://w3id.org/italia/data/department/dtd">
        <rdf:type rdf:resource="http://xmlns.com/foaf/0.1/Agent"/>
        <dct:identifier>PCM</dct:identifier>
        <foaf:name xml:lang="it">Presidenza del Consiglio dei Ministri - Dipartimento per la Trasformazione Digitale</foaf:name>
        <foaf:name xml:lang="en">Presidency of the Council of Ministers - Department of Digital Transformation</foaf:name>
      </dcatapit:Agent>
    </dct:creator>
    <dct:publisher rdf:resource="https://w3id.org/italia/data/public-organization/agid"/>
    <dcat:theme rdf:resource="http://publications.europa.eu/resource/authority/data-theme/HEAL"/>
    <dcat:theme rdf:resource="http://publications.europa.eu/resource/authority/data-theme/TECH"/>
    <dct:conformsTo>
      <dcatapit:Standard rdf:about="https://w3id.org/italia/data/standard/SKOS">
        <rdf:type rdf:resource="http://purl.org/dc/terms/Standard"/>
        <dct:identifier>SKOS</dct:identifier>
        <dct:title>Simple Knowledge Organization System - SKOS</dct:title>
        <dct:description>The Simple Knowledge Organization System (SKOS) is a common data model for sharing and linking knowledge organization systems via the Web</dct:description>
      </dcatapit:Standard>
    </dct:conformsTo>
    <dct:language rdf:resource="http://publications.europa.eu/resource/authority/language/ITA"/>
    <dct:accrualPeriodicity rdf:resource="http://publications.europa.eu/resource/authority/frequency/IRREG"/>
    <rdfs:isDefinedBy rdf:resource="https://w3id.org/italia/controlled-vocabulary/classifications-for-indicators/indicator-types"/>
    <dcat:keyword xml:lang="it">Indicatori</dcat:keyword>
    <dcat:keyword xml:lang="it">Tipi di indicatori</dcat:keyword>
    <dcat:distribution>
      <dcatapit:Distribution rdf:about="https://w3id.org/italia/data/distribution/INDTYPE_RDF_Turtle">
        <dct:title xml:lang="it">Distribuzione RDF/Turtle del vocabolario controllato sui tipi degli indicatori</dct:title>
        <dct:title xml:lang="en">RDF/Turtle distribution of the types of indicators</dct:title>
        <dct:description xml:lang="it">Questa è la distribuzione RDF/Turtle del dataset Linked Open Data del vocabolario controllato sui tipi degli indicatori</dct:description>
        <dct:description xml:lang="en">This is the distribution in RDF/turtle of the Linked Open Dataset of the types of indicators</dct:description>
        <dct:format rdf:resource="http://publications.europa.eu/resource/authority/file-type/RDF_TURTLE"/>
        <dct:license rdf:resource="https://w3id.org/italia/controlled-vocabulary/licences/A21_CCBY40"/>
        <dcat:downloadURL rdf:resource="https://raw.githubusercontent.com/italia/daf-ontologie-vocabolari-controllati/master/VocabolariControllati/classifications-for-indicators/indicator-types/indicator-types.ttl"/>
        <dcat:accessURL rdf:resource="https://github.com/italia/daf-ontologie-vocabolari-controllati/tree/master/VocabolariControllati/classifications-for-indicators/indicator-types"/>
      </dcatapit:Distribution>
    </dcat:distribution>
    <dcat:distribution>
      <dcatapit:Distribution rdf:about="https://w3id.org/italia/data/distribution/INDTYPE_RDF_XML">
        <dct:title xml:lang="it">Distribuzione RDF/XML del vocabolario controllato sui tipi degli indicatori</dct:title>
        <dct:title xml:lang="en">RDF/XML distribution of the types of indicators</dct:title>
        <dct:description xml:lang="it">Questa è la distribuzione RDF/XML del dataset Linked Open Data del vocabolario controllato sui tipi degli indicatori</dct:description>
        <dct:description xml:lang="en">This is the distribution in RDF/XML of the Linked Open Dataset of the types of indicators.</dct:description>
        <dct:format rdf:resource="http://publications.europa.eu/resource/authority/file-type/RDF_XML"/>
        <dct:license rdf:resource="https://w3id.org/italia/controlled-vocabulary/licences/A21_CCBY40"/>
        <dcat:downloadURL rdf:resource="https://raw.githubusercontent.com/italia/daf-ontologie-vocabolari-controllati/master/VocabolariControllati/classifications-for-indicators/indicator-types/indicator-types.rdf"/>
        <dcat:accessURL rdf:resource="https://github.com/italia/daf-ontologie-vocabolari-controllati/tree/master/VocabolariControllati/classifications-for-indicators/indicator-types"/>
      </dcatapit:Distribution>
    </dcat:distribution>
    <dcat:distribution>
      <dcatapit:Distribution rdf:about="https://w3id.org/italia/data/distribution/INDTYPE_JSON_LD">
        <dct:title xml:lang="it">Distribuzione JSON_LD del vocabolario controllato sui tipi degli indicatori</dct:title>
        <dct:title xml:lang="en">JSON_LD distribution of the types of indicators</dct:title>
        <dct:description xml:lang="it">Questa è la distribuzione JSON_LD del dataset Linked Open Data del vocabolario controllato sui tipi degli indicatori</dct:description>
        <dct:description xml:lang="en">This is the distribution in JSON_LD of the Linked Open Dataset of the types of indicators</dct:description>
        <dct:format rdf:resource="http://publications.europa.eu/resource/authority/file-type/JSON_LD"/>
        <dct:license rdf:resource="https://w3id.org/italia/controlled-vocabulary/licences/A21_CCBY40"/>
        <dcat:downloadURL rdf:resource="https://raw.githubusercontent.com/italia/daf-ontologie-vocabolari-controllati/master/VocabolariControllati/classifications-for-indicators/indicator-types/indicator-types.jsonld"/>
        <dcat:accessURL rdf:resource="https://github.com/italia/daf-ontologie-vocabolari-controllati/tree/master/VocabolariControllati/classifications-for-indicators/indicator-types"/>
      </dcatapit:Distribution>
    </dcat:distribution>
    <dcat:distribution>
      <dcatapit:Distribution rdf:about="https://w3id.org/italia/data/distribution/INDTYPE_CSV">
        <dct:title xml:lang="it">Distribuzione CSV del vocabolario controllato sui tipi degli indicatori</dct:title>
        <dct:title xml:lang="en">CSV distribution of the types of indicators</dct:title>
        <dct:description xml:lang="it">Questa è la distribuzione CSV del dataset Linked Open Data del vocabolario controllato sui tipi degli indicatori</dct:description>
        <dct:description xml:lang="en">This is the distribution in CSV of the Open Dataset of the types of indicators</dct:description>
        <dct:format rdf:resource="http://publications.europa.eu/resource/authority/file-type/CSV"/>
        <dct:license rdf:resource="https://w3id.org/italia/controlled-vocabulary/licences/A21_CCBY40"/>
        <dcat:downloadURL rdf:resource="https://raw.githubusercontent.com/italia/daf-ontologie-vocabolari-controllati/master/VocabolariControllati/classifications-for-indicators/indicator-types/indicator-types.csv"/>
        <dcat:accessURL rdf:resource="https://github.com/italia/daf-ontologie-vocabolari-controllati/tree/master/VocabolariControllati/classifications-for-indicators/indicator-types"/>
      </dcatapit:Distribution>
    </dcat:distribution>
    <dcat:distribution>
      <dcatapit:Distribution rdf:about="https://w3id.org/italia/data/distribution/INDTYPE_XLSX">
        <dct:title xml:lang="it">Distribuzione XLSX del vocabolario controllato sui tipi degli indicatori</dct:title>
        <dct:title xml:lang="en">XLSX distribution of the types of indicators</dct:title>
        <dct:description xml:lang="it">Questa è la distribuzione XLSX del dataset Linked Open Data del vocabolario controllato sui tipi degli indicatori</dct:description>
        <dct:description xml:lang="en">This is the distribution in XLSX of the Open Dataset of the types of indicators</dct:description>
        <dct:format rdf:resource="http://publications.europa.eu/resource/authority/file-type/XLSX"/>
        <dct:license rdf:resource="https://w3id.org/italia/controlled-vocabulary/licences/A21_CCBY40"/>
        <dcat:downloadURL rdf:resource="https://github.com/italia/daf-ontologie-vocabolari-controllati/raw/master/VocabolariControllati/classifications-for-indicators/indicator-types/indicator-types.xlsx"/>
        <dcat:accessURL rdf:resource="https://github.com/italia/daf-ontologie-vocabolari-controllati/tree/master/VocabolariControllati/classifications-for-indicators/indicator-types"/>
      </dcatapit:Distribution>
    </dcat:distribution>
    <dcat:contactPoint>
      <dcatapit:Organization rdf:about="https://w3id.org/italia/data/contact-point/voc_AgID">
        <rdf:type rdf:resource="http://www.w3.org/2006/vcard/ns#Organization"/>
        <rdf:type rdf:resource="http://www.w3.org/2006/vcard/ns#Kind"/>
        <vcard:fn>banche dati e open data</vcard:fn>
        <vcard:hasEmail rdf:resource="mailto:info@dati.gov.it"/>
      </dcatapit:Organization>
    </dcat:contactPoint>
    <dct:issued rdf:datatype="http://www.w3.org/2001/XMLSchema#date">2020-05-26</dct:issued>
    <dct:modified rdf:datatype="http://www.w3.org/2001/XMLSchema#date">2020-05-26</dct:modified>
    <skos:hasTopConcept>
      <indicator:IndicatorType rdf:about="https://w3id.org/italia/controlled-vocabulary/classifications-for-indicators/indicator-types/process">
        <rdf:type rdf:resource="http://www.w3.org/2004/02/skos/core#Concept"/>
        <skos:inScheme rdf:resource="https://w3id.org/italia/controlled-vocabulary/classifications-for-indicators/indicator-types"/>
        <l0:name xml:lang="it">Indicatore di processo</l0:name>
        <clvapit:hasRankOrder>1</clvapit:hasRankOrder>
        <xkos:depth rdf:datatype="http://www.w3.org/2001/XMLSchema#integer">1</xkos:depth>
        <skos:notation>process</skos:notation>
        <dct:identifier>process</dct:identifier>
        <skos:prefLabel xml:lang="it">Indicatore di processo</skos:prefLabel>
        <skos:prefLabel xml:lang="en">Process indicator</skos:prefLabel>
      </indicator:IndicatorType>
    </skos:hasTopConcept>
    <skos:hasTopConcept>
      <indicator:IndicatorType rdf:about="https://w3id.org/italia/controlled-vocabulary/classifications-for-indicators/indicator-types/outcome">
        <rdf:type rdf:resource="http://www.w3.org/2004/02/skos/core#Concept"/>
        <skos:inScheme rdf:resource="https://w3id.org/italia/controlled-vocabulary/classifications-for-indicators/indicator-types"/>
        <clvapit:hasRankOrder>1</clvapit:hasRankOrder>
        <xkos:depth rdf:datatype="http://www.w3.org/2001/XMLSchema#integer">1</xkos:depth>
        <l0:name xml:lang="it">Indicatore di risultato</l0:name>
        <skos:notation>outcome</skos:notation>
        <dct:identifier>outcome</dct:identifier>
        <skos:prefLabel xml:lang="it">Indicatore di risultato</skos:prefLabel>
        <skos:prefLabel xml:lang="en">Outcome indicator</skos:prefLabel>
      </indicator:IndicatorType>
    </skos:hasTopConcept>
    <skos:hasTopConcept>
      <indicator:IndicatorType rdf:about="https://w3id.org/italia/controlled-vocabulary/classifications-for-indicators/indicator-types/structure">
        <rdf:type rdf:resource="http://www.w3.org/2004/02/skos/core#Concept"/>
        <skos:inScheme rdf:resource="https://w3id.org/italia/controlled-vocabulary/classifications-for-indicators/indicator-types"/>
        <clvapit:hasRankOrder>1</clvapit:hasRankOrder>
        <xkos:depth rdf:datatype="http://www.w3.org/2001/XMLSchema#integer">1</xkos:depth>
        <l0:name xml:lang="it">Indicatore di risultato</l0:name>
        <skos:notation>structure</skos:notation>
        <dct:identifier>structure</dct:identifier>
        <skos:prefLabel xml:lang="it">Indicatore di struttura</skos:prefLabel>
        <skos:prefLabel xml:lang="en">Structure indicator</skos:prefLabel>
      </indicator:IndicatorType>
    </skos:hasTopConcept>
  </skos:ConceptScheme>
  <rdfs:Property rdf:about="https://w3id.org/italia/onto/NDC/keyConcept"/>
  <rdfs:Property rdf:about="http://purl.org/dc/terms/accrualPeriodicity"/>
  <rdfs:Property rdf:about="http://purl.org/dc/terms/type"/>
  <rdfs:Property rdf:about="http://purl.org/dc/terms/language"/>
  <rdfs:Property rdf:about="http://purl.org/dc/terms/format"/>
  <rdfs:Property rdf:about="http://www.w3.org/2006/vcard/ns#fn"/>
  <rdfs:Property rdf:about="http://www.w3.org/ns/dcat#distribution"/>
  <rdfs:Property rdf:about="http://www.w3.org/2004/02/skos/core#narrowerTransitive"/>
  <rdfs:Property rdf:about="http://purl.org/dc/terms/publisher"/>
  <rdfs:Property rdf:about="http://rdf-vocabulary.ddialliance.org/xkos#numberOfLevels"/>
  <rdfs:Property rdf:about="http://www.w3.org/2004/02/skos/core#definition"/>
  <rdfs:Property rdf:about="http://purl.org/dc/terms/description"/>
  <rdfs:Property rdf:about="http://purl.org/dc/terms/conformsTo"/>
  <rdfs:Property rdf:about="http://www.w3.org/2006/vcard/ns#hasEmail"/>
  <rdfs:Property rdf:about="http://rdf-vocabulary.ddialliance.org/xkos#depth"/>
  <rdfs:Property rdf:about="https://w3id.org/italia/onto/Indicator/isMetByIndicator"/>
  <rdfs:Property rdf:about="http://www.w3.org/2002/07/owl#versionInfo"/>
  <rdfs:Property rdf:about="http://xmlns.com/foaf/0.1/name"/>
  <rdfs:Property rdf:about="https://w3id.org/italia/onto/l0/name"/>
  <rdfs:Property rdf:about="http://www.w3.org/ns/dcat#contactPoint"/>
  <rdfs:Property rdf:about="http://www.w3.org/2004/02/skos/core#prefLabel"/>
  <rdfs:Property rdf:about="http://purl.org/dc/terms/issued"/>
  <rdfs:Class rdf:about="https://w3id.org/italia/onto/Indicator/Indicator"/>
  <rdfs:Property rdf:about="http://www.w3.org/2004/02/skos/core#notation"/>
  <rdfs:Property rdf:about="https://w3id.org/italia/onto/Indicator/meetsPurpose"/>
  <rdfs:Property rdf:about="http://www.w3.org/2004/02/skos/core#broaderTransitive"/>
  <rdfs:Property rdf:about="http://purl.org/dc/terms/identifier"/>
  <rdfs:Property rdf:about="http://purl.org/dc/terms/modified"/>
  <rdfs:Property rdf:about="https://w3id.org/italia/onto/CLV/hasRankOrder"/>
  <rdfs:Property rdf:about="http://www.w3.org/ns/dcat#accessURL"/>
  <rdfs:Property rdf:about="http://purl.org/dc/terms/rightsHolder"/>
  <rdfs:Property rdf:about="http://www.w3.org/ns/dcat#downloadURL"/>
  <rdfs:Property rdf:about="http://purl.org/dc/terms/creator"/>
  <rdfs:Property rdf:about="http://www.w3.org/2004/02/skos/core#inScheme"/>
  <rdfs:Property rdf:about="http://www.w3.org/ns/dcat#keyword"/>
  <rdfs:Property rdf:about="http://www.w3.org/ns/dcat#theme"/>
  <rdfs:Property rdf:about="http://purl.org/dc/terms/subject"/>
  <rdfs:Property rdf:about="http://www.w3.org/ns/adms#representationTechnique"/>
  <rdfs:Property rdf:about="https://w3id.org/italia/onto/Indicator/hasIndicatorType"/>
  <rdfs:Property rdf:about="http://www.w3.org/2004/02/skos/core#narrower"/>
  <rdfs:Property rdf:about="http://www.w3.org/2004/02/skos/core#broader"/>
  <rdfs:Property rdf:about="http://purl.org/dc/terms/title"/>
  <rdfs:Property rdf:about="https://w3id.org/italia/onto/Indicator/definedInLegislation"/>
  <rdfs:Property rdf:about="https://w3id.org/italia/onto/l0/description"/>
  <rdfs:Class rdf:about="http://www.w3.org/2006/vcard/ns#Kind"/>
  <rdfs:Class rdf:about="http://dati.gov.it/onto/dcatapit#Organization"/>
  <rdfs:Class rdf:about="http://dati.gov.it/onto/dcatapit#Distribution"/>
  <rdfs:Class rdf:about="http://dati.gov.it/onto/dcatapit#Dataset"/>
  <rdfs:Class rdf:about="http://www.w3.org/2004/02/skos/core#ConceptScheme"/>
  <rdfs:Class rdf:about="http://dati.gov.it/onto/dcatapit#Standard"/>
  <rdfs:Class rdf:about="http://www.w3.org/2006/vcard/ns#Organization"/>
  <rdfs:Class rdf:about="http://purl.org/dc/terms/Standard"/>
  <rdfs:Class rdf:about="http://xmlns.com/foaf/0.1/Agent"/>
  <rdfs:Class rdf:about="http://www.w3.org/2004/02/skos/core#Concept"/>
  <rdfs:Class rdf:about="http://dati.gov.it/onto/dcatapit#Agent"/>
</rdf:RDF>
