<?xml version="1.0" encoding="UTF-8"?>
<rdf:RDF
   xmlns:admsapit="https://w3id.org/italia/onto/ADMS/"
   xmlns:dcat="http://www.w3.org/ns/dcat#"
   xmlns:dct="http://purl.org/dc/terms/"
   xmlns:foaf="http://xmlns.com/foaf/0.1/"
   xmlns:l0="https://w3id.org/italia/onto/l0/"
   xmlns:owl="http://www.w3.org/2002/07/owl#"
   xmlns:prov="http://www.w3.org/ns/prov#"
   xmlns:rdf="http://www.w3.org/1999/02/22-rdf-syntax-ns#"
   xmlns:rdfs="http://www.w3.org/2000/01/rdf-schema#"
   xmlns:vcard="http://www.w3.org/2006/vcard/ns#"
>
  <rdf:Description rdf:about="https://w3id.org/italia/onto/IoT/hasObservationValue">
    <rdf:type rdf:resource="http://www.w3.org/2002/07/owl#ObjectProperty"/>
    <owl:inverseOf rdf:resource="https://w3id.org/italia/onto/IoT/isObservationValueOf"/>
    <rdfs:domain rdf:resource="https://w3id.org/italia/onto/IoT/Observation"/>
    <rdfs:range rdf:resource="https://w3id.org/italia/onto/IoT/ObservationValue"/>
    <rdfs:comment xml:lang="en">Property that links an Observation to its value.</rdfs:comment>
    <rdfs:comment xml:lang="it">Proprietà che lega un'osservazione al suo valore.</rdfs:comment>
    <rdfs:isDefinedBy rdf:resource="https://w3id.org/italia/onto/IoT"/>
    <rdfs:label xml:lang="it">ha valore dell'osservazione</rdfs:label>
    <rdfs:label xml:lang="en">has observation value</rdfs:label>
    <owl:versionInfo xml:lang="it">stabile</owl:versionInfo>
    <owl:versionInfo xml:lang="en">stable</owl:versionInfo>
  </rdf:Description>
  <rdf:Description rdf:about="https://w3id.org/italia/data/organization/public-organization/td">
    <rdf:type rdf:resource="http://www.w3.org/2002/07/owl#NamedIndividual"/>
    <rdf:type rdf:resource="http://dati.gov.it/onto/dcatapit#Agent"/>
    <rdf:type rdf:resource="http://xmlns.com/foaf/0.1/Agent"/>
    <dct:identifier>TD</dct:identifier>
    <foaf:name xml:lang="en">Digital Transformation Team</foaf:name>
    <foaf:name xml:lang="it">Team per la Trasformazione Digitale</foaf:name>
  </rdf:Description>
  <rdf:Description rdf:nodeID="n690e025d2eb648a3a4574298c2d1991cb10">
    <rdf:type rdf:resource="http://www.w3.org/2002/07/owl#Restriction"/>
    <owl:onProperty rdf:resource="https://w3id.org/italia/onto/IoT/usedMethod"/>
    <owl:allValuesFrom rdf:resource="https://w3id.org/italia/onto/IoT/Method"/>
  </rdf:Description>
  <rdf:Description rdf:about="https://w3id.org/italia/data/distribution/IOT-RDF-TURTLE">
    <rdf:type rdf:resource="http://www.w3.org/2002/07/owl#NamedIndividual"/>
    <rdf:type rdf:resource="https://w3id.org/italia/onto/ADMS/SemanticAssetDistribution"/>
    <dct:description xml:lang="it">Questa è la distribuzione RDF/Turtle dell'ontologia degli eventi IoT</dct:description>
    <dct:description xml:lang="en">This is the distribution in RDF/turtle of the IoT Events ontology</dct:description>
    <dct:format rdf:resource="http://publications.europa.eu/resource/authority/file-type/RDF_TURTLE"/>
    <dct:license rdf:resource="https://w3id.org/italia/controlled-vocabulary/licences/A21_CCBY40"/>
    <dct:title xml:lang="it">Distribuzione RDF/Turtle ontologia IoT-AP_IT</dct:title>
    <dct:title xml:lang="en">RDF/Turtle distribution of IoT-AP_IT Ontology</dct:title>
    <dcat:accessURL rdf:resource="https://raw.githubusercontent.com/italia/daf-ontologie-vocabolari-controllati/master/Ontologie/IoT/latest"/>
    <dcat:downloadURL rdf:resource="https://raw.githubusercontent.com/italia/daf-ontologie-vocabolari-controllati/master/Ontologie/IoT/latest/IoT-AP_IT.ttl"/>
  </rdf:Description>
  <rdf:Description rdf:about="https://w3id.org/italia/onto/l0/Collection">
    <rdf:type rdf:resource="http://www.w3.org/2002/07/owl#Class"/>
  </rdf:Description>
  <rdf:Description rdf:about="https://w3id.org/italia/onto/IoT/observationCollectionMadeBySensor">
    <rdf:type rdf:resource="http://www.w3.org/2002/07/owl#ObjectProperty"/>
    <rdfs:domain rdf:resource="https://w3id.org/italia/onto/IoT/ObservationCollection"/>
    <rdfs:range rdf:resource="https://w3id.org/italia/onto/IoT/Sensor"/>
    <rdfs:comment xml:lang="en">Inverse property of makes observation collection that links a collection of observation made by a sensor.</rdfs:comment>
    <rdfs:comment xml:lang="it">Proprietà inversa di fa collezioni di osservazioni che unisce una collezione di osservazioni a un sensore che le produce.</rdfs:comment>
    <rdfs:isDefinedBy rdf:resource="https://w3id.org/italia/onto/IoT"/>
    <rdfs:label xml:lang="it">collezione di osservazioni fatte da sensore</rdfs:label>
    <rdfs:label xml:lang="en">observation collection made by sensor</rdfs:label>
    <owl:versionInfo xml:lang="it">stabile</owl:versionInfo>
    <owl:versionInfo xml:lang="en">stable</owl:versionInfo>
  </rdf:Description>
  <rdf:Description rdf:about="https://w3id.org/italia/onto/IoT/isValueForObservationParameter">
    <rdf:type rdf:resource="http://www.w3.org/2002/07/owl#ObjectProperty"/>
    <rdfs:domain rdf:resource="https://w3id.org/italia/onto/IoT/ObservationValue"/>
    <rdfs:range rdf:resource="https://w3id.org/italia/onto/IoT/ObservationParameter"/>
    <rdfs:comment xml:lang="en">Inverse property of has value for observation parameter that links an observation value to the  observation parameter</rdfs:comment>
    <rdfs:comment xml:lang="it">Proprietà inversa di ha valore per il parametro di osservazione che lega un valore dell'osservazione al parametro dell'osservazione.</rdfs:comment>
    <rdfs:isDefinedBy rdf:resource="https://w3id.org/italia/onto/IoT"/>
    <rdfs:label xml:lang="en">is value for observation parameter</rdfs:label>
    <rdfs:label xml:lang="it">è valore per parametro osservazione</rdfs:label>
    <owl:versionInfo xml:lang="it">stabile</owl:versionInfo>
    <owl:versionInfo xml:lang="en">stable</owl:versionInfo>
  </rdf:Description>
  <rdf:Description rdf:about="https://w3id.org/italia/onto/IoT/Observation">
    <rdf:type rdf:resource="http://www.w3.org/2002/07/owl#Class"/>
    <rdfs:subClassOf rdf:resource="https://w3id.org/italia/onto/l0/Activity"/>
    <rdfs:subClassOf rdf:nodeID="n690e025d2eb648a3a4574298c2d1991cb7"/>
    <rdfs:subClassOf rdf:nodeID="n690e025d2eb648a3a4574298c2d1991cb8"/>
    <rdfs:subClassOf rdf:nodeID="n690e025d2eb648a3a4574298c2d1991cb9"/>
    <rdfs:subClassOf rdf:nodeID="n690e025d2eb648a3a4574298c2d1991cb10"/>
    <rdfs:subClassOf rdf:nodeID="n690e025d2eb648a3a4574298c2d1991cb11"/>
    <rdfs:subClassOf rdf:nodeID="n690e025d2eb648a3a4574298c2d1991cb12"/>
    <rdfs:subClassOf rdf:nodeID="n690e025d2eb648a3a4574298c2d1991cb13"/>
    <rdfs:subClassOf rdf:nodeID="n690e025d2eb648a3a4574298c2d1991cb14"/>
    <rdfs:subClassOf rdf:nodeID="n690e025d2eb648a3a4574298c2d1991cb15"/>
    <rdfs:subClassOf rdf:nodeID="n690e025d2eb648a3a4574298c2d1991cb16"/>
    <rdfs:subClassOf rdf:nodeID="n690e025d2eb648a3a4574298c2d1991cb17"/>
    <rdfs:subClassOf rdf:nodeID="n690e025d2eb648a3a4574298c2d1991cb18"/>
    <rdfs:subClassOf rdf:nodeID="n690e025d2eb648a3a4574298c2d1991cb19"/>
    <rdfs:subClassOf rdf:nodeID="n690e025d2eb648a3a4574298c2d1991cb20"/>
    <rdfs:subClassOf rdf:nodeID="n690e025d2eb648a3a4574298c2d1991cb21"/>
    <rdfs:comment xml:lang="en">Act of carrying out an Observation (which is an Event) to estimate or calculate a value of an attribute of a feature of interest.</rdfs:comment>
    <rdfs:comment xml:lang="it">L'atto di condurre un'osservazione (che è un evento) per stimare o calcolare un valore di un attributo di una caratteristica di interesse.</rdfs:comment>
    <rdfs:isDefinedBy rdf:resource="https://w3id.org/italia/onto/IoT"/>
    <rdfs:label xml:lang="en">Observation</rdfs:label>
    <rdfs:label xml:lang="it">Osservazione</rdfs:label>
    <owl:versionInfo xml:lang="it">stabile</owl:versionInfo>
    <owl:versionInfo xml:lang="en">stable</owl:versionInfo>
  </rdf:Description>
  <rdf:Description rdf:about="https://w3id.org/italia/onto/IoT/consistsOf">
    <rdf:type rdf:resource="http://www.w3.org/2002/07/owl#ObjectProperty"/>
    <owl:inverseOf rdf:resource="https://w3id.org/italia/onto/IoT/isPartOf"/>
    <rdfs:domain rdf:resource="https://w3id.org/italia/onto/IoT/ObservationCollection"/>
    <rdfs:range rdf:resource="https://w3id.org/italia/onto/IoT/Observation"/>
    <rdfs:comment xml:lang="en">Property that links a collection of observations with its observations.</rdfs:comment>
    <rdfs:comment xml:lang="it">Proprietà che collega una collezione di osservazioni con le sue osservazioni.</rdfs:comment>
    <rdfs:isDefinedBy rdf:resource="https://w3id.org/italia/onto/IoT"/>
    <rdfs:label xml:lang="it">consiste di</rdfs:label>
    <rdfs:label xml:lang="en">consists of</rdfs:label>
    <owl:versionInfo xml:lang="it">stabile</owl:versionInfo>
    <owl:versionInfo xml:lang="en">stable</owl:versionInfo>
  </rdf:Description>
  <rdf:Description rdf:about="https://w3id.org/italia/onto/IoT/Precision">
    <rdf:type rdf:resource="http://www.w3.org/2002/07/owl#Class"/>
    <rdfs:subClassOf rdf:resource="https://w3id.org/italia/onto/IoT/MeasurementQuality"/>
    <rdfs:comment xml:lang="en">It represents the Precision; i.e., the  degree of reproducibility of a measurement. In other words, if exactly the same values were measured a number of times, an ideal sensor would output exactly the same value every time.</rdfs:comment>
    <rdfs:comment xml:lang="it">Questa classe rappresenta la Precisione, ovvero il grado di riproducibilità di una misura. In altre parole, se esattamente gli stessi valori sono stati misurati un certo numero di volte, un sensor ideale produrrebbe come output esattamente lo stesso valore ogni volta.</rdfs:comment>
    <rdfs:isDefinedBy rdf:resource="https://w3id.org/italia/onto/IoT"/>
    <rdfs:label xml:lang="en">Precision</rdfs:label>
    <rdfs:label xml:lang="it">Precisione</rdfs:label>
    <owl:versionInfo xml:lang="it">instabile</owl:versionInfo>
    <owl:versionInfo xml:lang="en">unstable</owl:versionInfo>
  </rdf:Description>
  <rdf:Description rdf:about="https://w3id.org/italia/onto/IoT/MonitoringFacility">
    <rdf:type rdf:resource="http://www.w3.org/2002/07/owl#Class"/>
    <rdfs:subClassOf rdf:resource="https://w3id.org/italia/onto/l0/Object"/>
    <rdfs:subClassOf rdf:nodeID="n690e025d2eb648a3a4574298c2d1991cb5"/>
    <rdfs:subClassOf rdf:nodeID="n690e025d2eb648a3a4574298c2d1991cb6"/>
    <rdfs:comment xml:lang="it">Il termine è utilizzato nelle relative specifiche INSPIRE per definire degli strumenti di monitoraggio. Nel contesto di questa ontologia sono i sensori e gli attuatori.</rdfs:comment>
    <rdfs:comment xml:lang="en">The term refers to the related INSPIRE specifications for environmental monitoring facilties. In the context of this ontology, it consists of sensors and actuators</rdfs:comment>
    <rdfs:isDefinedBy rdf:resource="https://w3id.org/italia/onto/IoT"/>
    <rdfs:label xml:lang="en">Monitoring Facility</rdfs:label>
    <rdfs:label xml:lang="it">Strumento di monitoraggio</rdfs:label>
    <owl:versionInfo xml:lang="it">provvisorio - in attesa di validazione</owl:versionInfo>
    <owl:versionInfo xml:lang="en">unstable</owl:versionInfo>
  </rdf:Description>
  <rdf:Description rdf:about="https://w3id.org/italia/onto/IoT/usedMethod">
    <rdf:type rdf:resource="http://www.w3.org/2002/07/owl#ObjectProperty"/>
    <rdfs:domain rdf:resource="https://w3id.org/italia/onto/IoT/Observation"/>
    <rdfs:range rdf:resource="https://w3id.org/italia/onto/IoT/Method"/>
    <rdfs:comment xml:lang="en">Property that links the observation with the method used to derive it.</rdfs:comment>
    <rdfs:comment xml:lang="it">Proprietà che collega l'osservazione con il metodo utilizzato per rilevarla.</rdfs:comment>
    <rdfs:isDefinedBy rdf:resource="https://w3id.org/italia/onto/IoT"/>
    <rdfs:label xml:lang="it">metodo usato</rdfs:label>
    <rdfs:label xml:lang="en">used method</rdfs:label>
    <owl:versionInfo xml:lang="it">provvisorio - da validare</owl:versionInfo>
    <owl:versionInfo xml:lang="en">unstable</owl:versionInfo>
  </rdf:Description>
  <rdf:Description rdf:nodeID="n690e025d2eb648a3a4574298c2d1991cb4">
    <rdf:type rdf:resource="http://www.w3.org/2002/07/owl#Restriction"/>
    <owl:onProperty rdf:resource="https://w3id.org/italia/onto/IoT/isMeasurementQualityValueOf"/>
    <owl:someValuesFrom rdf:resource="https://w3id.org/italia/onto/IoT/MeasurementQuality"/>
  </rdf:Description>
  <rdf:Description rdf:nodeID="n690e025d2eb648a3a4574298c2d1991cb24">
    <rdf:type rdf:resource="http://www.w3.org/2002/07/owl#Restriction"/>
    <owl:onProperty rdf:resource="https://w3id.org/italia/onto/l0/identifier"/>
    <owl:cardinality rdf:datatype="http://www.w3.org/2001/XMLSchema#nonNegativeInteger">1</owl:cardinality>
  </rdf:Description>
  <rdf:Description rdf:about="https://w3id.org/italia/onto/IoT/Frequency">
    <rdf:type rdf:resource="http://www.w3.org/2002/07/owl#Class"/>
    <rdfs:subClassOf rdf:resource="https://w3id.org/italia/onto/IoT/MeasurementQuality"/>
    <rdfs:comment xml:lang="en">It represents the Frequency; that is, the smallest possible time between one observation and the next, under the defined conditions.</rdfs:comment>
    <rdfs:comment xml:lang="it">Questa classe rappresenta la frequenza ovvero il più piccolo tempo possibile tra un'osservazione e un'altra, in determinate condizioni.</rdfs:comment>
    <rdfs:isDefinedBy rdf:resource="https://w3id.org/italia/onto/IoT"/>
    <rdfs:label xml:lang="en">Frequency</rdfs:label>
    <rdfs:label xml:lang="en">Frequenza</rdfs:label>
    <owl:versionInfo xml:lang="it">instabile</owl:versionInfo>
    <owl:versionInfo xml:lang="en">unstable</owl:versionInfo>
  </rdf:Description>
  <rdf:Description rdf:nodeID="n690e025d2eb648a3a4574298c2d1991cb28">
    <rdf:type rdf:resource="http://www.w3.org/2002/07/owl#Restriction"/>
    <owl:onProperty rdf:resource="https://w3id.org/italia/onto/IoT/hasValueForObservationParameter"/>
    <owl:someValuesFrom rdf:resource="https://w3id.org/italia/onto/IoT/ObservationValue"/>
  </rdf:Description>
  <rdf:Description rdf:about="https://w3id.org/italia/onto/IoT/isFeatureOfInterestFor">
    <rdf:type rdf:resource="http://www.w3.org/2002/07/owl#ObjectProperty"/>
    <rdfs:domain rdf:resource="https://w3id.org/italia/onto/IoT/FeatureOfInterest"/>
    <rdfs:range rdf:resource="https://w3id.org/italia/onto/IoT/Observation"/>
    <rdfs:comment xml:lang="en">Inverse property of has feature of interest that links a feature of interest to an observation.</rdfs:comment>
    <rdfs:comment xml:lang="it">Proprietà inversa di ha caratteristica di interesse che lega una caratteristica di interesse a un'osservaizione.</rdfs:comment>
    <rdfs:isDefinedBy rdf:resource="https://w3id.org/italia/onto/IoT"/>
    <rdfs:label xml:lang="en">is feature of interest for</rdfs:label>
    <rdfs:label xml:lang="it">è caratteristica di interesse per</rdfs:label>
    <owl:versionInfo xml:lang="it">stabile</owl:versionInfo>
    <owl:versionInfo xml:lang="en">stable</owl:versionInfo>
  </rdf:Description>
  <rdf:Description rdf:about="https://w3id.org/italia/onto/IoT/Method">
    <rdf:type rdf:resource="http://www.w3.org/2002/07/owl#Class"/>
    <rdfs:subClassOf rdf:resource="https://w3id.org/italia/onto/l0/Description"/>
    <rdfs:comment xml:lang="en">A workflow, protocol, plan, algorithm, or computational method specifying how to make an observation. It is implemented by monitoring facilities</rdfs:comment>
    <rdfs:comment xml:lang="it">Un metodo di misurazione, una procedura, un protocollo che specifica come effetturare un'osservazione e che è implementato da uno strumento di monitoraggio.</rdfs:comment>
    <rdfs:isDefinedBy rdf:resource="https://w3id.org/italia/onto/IoT"/>
    <rdfs:label xml:lang="en">Method</rdfs:label>
    <rdfs:label xml:lang="it">Metodo</rdfs:label>
    <rdfs:label xml:lang="it">Procedura</rdfs:label>
    <rdfs:label xml:lang="it">Protocollo</rdfs:label>
    <owl:versionInfo xml:lang="it">provvisoria - da validare</owl:versionInfo>
    <owl:versionInfo xml:lang="en">unstable</owl:versionInfo>
  </rdf:Description>
  <rdf:Description rdf:about="https://w3id.org/italia/onto/IoT/MeasurementQuality">
    <rdf:type rdf:resource="http://www.w3.org/2002/07/owl#Class"/>
    <rdfs:subClassOf rdf:resource="https://w3id.org/italia/onto/l0/Characteristic"/>
    <rdfs:subClassOf rdf:nodeID="n690e025d2eb648a3a4574298c2d1991cb3"/>
    <rdfs:comment xml:lang="it">Questa classe rappresenta dei parametri di qualità o capacità di misurazione dell'osservazione. Esempi di parametri sono: Latenza, Accuratezza, Ripetibilità, ecc.</rdfs:comment>
    <rdfs:comment xml:lang="en">This class represents quality parameters or measurement capabilities/qualities of an observation. Examples include Latency, Accuracy, Repetability, etc.</rdfs:comment>
    <rdfs:isDefinedBy rdf:resource="https://w3id.org/italia/onto/IoT"/>
    <rdfs:label xml:lang="en">Measurement Quality</rdfs:label>
    <rdfs:label xml:lang="it">Qualità di Misurazione</rdfs:label>
    <owl:versionInfo xml:lang="it">instabile</owl:versionInfo>
    <owl:versionInfo xml:lang="en">unstable</owl:versionInfo>
  </rdf:Description>
  <rdf:Description rdf:nodeID="n690e025d2eb648a3a4574298c2d1991cb31">
    <rdf:type rdf:resource="http://www.w3.org/2002/07/owl#Restriction"/>
    <owl:onProperty rdf:resource="https://w3id.org/italia/onto/IoT/isObservationValueOf"/>
    <owl:someValuesFrom rdf:resource="https://w3id.org/italia/onto/IoT/Observation"/>
  </rdf:Description>
  <rdf:Description rdf:nodeID="n690e025d2eb648a3a4574298c2d1991cb32">
    <rdf:type rdf:resource="http://www.w3.org/2002/07/owl#Restriction"/>
    <owl:onProperty rdf:resource="https://w3id.org/italia/onto/IoT/isValueForObservationParameter"/>
    <owl:someValuesFrom rdf:resource="https://w3id.org/italia/onto/IoT/ObservationParameter"/>
  </rdf:Description>
  <rdf:Description rdf:about="https://w3id.org/italia/onto/IoT/ObservationParameter">
    <rdf:type rdf:resource="http://www.w3.org/2002/07/owl#Class"/>
    <rdfs:subClassOf rdf:nodeID="n690e025d2eb648a3a4574298c2d1991cb25"/>
    <rdfs:subClassOf rdf:nodeID="n690e025d2eb648a3a4574298c2d1991cb28"/>
    <rdfs:subClassOf rdf:nodeID="n690e025d2eb648a3a4574298c2d1991cb29"/>
    <rdfs:subClassOf rdf:nodeID="n690e025d2eb648a3a4574298c2d1991cb30"/>
    <rdfs:comment xml:lang="en">An observation parameter (property, characteristic) of a feature of interest. For instance, if we say that the temperature of the kitchen is 28 clesius degrees, the observed attribute is temperature.</rdfs:comment>
    <rdfs:comment xml:lang="it">Rappresenta un parametro (proprietà) dell'osservazione di una caratteristica di interesse. Per esempio, se diciamo che la temperatura della cucina è di 28 gradi celsius, la temperatura rappresenta l'attributo osservato.</rdfs:comment>
    <rdfs:isDefinedBy rdf:resource="https://w3id.org/italia/onto/IoT"/>
    <rdfs:label xml:lang="en">Observation Parameter</rdfs:label>
    <rdfs:label xml:lang="it">Parametro dell'Osservazione</rdfs:label>
    <owl:versionInfo xml:lang="it">stabile</owl:versionInfo>
    <owl:versionInfo xml:lang="en">stable</owl:versionInfo>
  </rdf:Description>
  <rdf:Description rdf:nodeID="n690e025d2eb648a3a4574298c2d1991cb6">
    <rdf:type rdf:resource="http://www.w3.org/2002/07/owl#Restriction"/>
    <owl:onProperty rdf:resource="https://w3id.org/italia/onto/IoT/isHostedByPlatform"/>
    <owl:allValuesFrom rdf:resource="https://w3id.org/italia/onto/IoT/Platform"/>
  </rdf:Description>
  <rdf:Description rdf:about="https://w3id.org/italia/onto/IoT/isObservationParameterFor">
    <rdf:type rdf:resource="http://www.w3.org/2002/07/owl#ObjectProperty"/>
    <rdfs:domain rdf:resource="https://w3id.org/italia/onto/IoT/ObservationParameter"/>
    <rdfs:range rdf:resource="https://w3id.org/italia/onto/IoT/Observation"/>
    <rdfs:comment xml:lang="en">Inverse property of hasObservationParameter that links a parameter to its related observation.</rdfs:comment>
    <rdfs:comment xml:lang="it">Proprietà inversa di ha attributo osservato che lega un attributo osservato alla sua relativa osservazione.</rdfs:comment>
    <rdfs:isDefinedBy rdf:resource="https://w3id.org/italia/onto/IoT"/>
    <rdfs:label xml:lang="en">is observation parameter for</rdfs:label>
    <rdfs:label xml:lang="it">è parametro dell'osservazione per</rdfs:label>
    <owl:versionInfo xml:lang="it">stabile</owl:versionInfo>
    <owl:versionInfo xml:lang="en">stable</owl:versionInfo>
  </rdf:Description>
  <rdf:Description rdf:about="https://w3id.org/italia/onto/IoT">
    <rdf:type rdf:resource="http://www.w3.org/2002/07/owl#Ontology"/>
    <rdf:type rdf:resource="http://www.w3.org/2002/07/owl#NamedIndividual"/>
    <rdf:type rdf:resource="https://w3id.org/italia/onto/ADMS/SemanticAsset"/>
    <owl:versionIRI rdf:resource="https://w3id.org/italia/onto/IoT/1.1"/>
    <owl:imports rdf:resource="https://w3id.org/italia/onto/CLV"/>
    <owl:imports rdf:resource="https://w3id.org/italia/onto/MU"/>
    <owl:imports rdf:resource="https://w3id.org/italia/onto/TI"/>
    <owl:imports rdf:resource="https://w3id.org/italia/onto/l0"/>
    <dct:accrualPeriodicity rdf:resource="http://publications.europa.eu/resource/authority/frequency/IRREG"/>
    <dct:creator rdf:resource="http://spcdata.digitpa.gov.it/Amministrazione/agid"/>
    <dct:creator rdf:resource="https://w3id.org/italia/data/organization/support-unit/cnr-Z6HZEH/stlab"/>
    <dct:description xml:lang="it">Questa è l'ontologia di eventi IoT. Essa può essere utilizzata per esempio per rappresentare serie temporali e misure di sensoristica di vario tipo. Attualmente l'ontologia include classi specializzate per la modellazione di flussi di traffico.</dct:description>
    <dct:description xml:lang="en">This is the ontology used to represent IoT events. It can be used to model temporal series and measures of sensors of different type. Currently the ontology is specialized for modelling traffic flows.</dct:description>
    <dct:issued rdf:datatype="http://www.w3.org/2001/XMLSchema#date">2017-05-15</dct:issued>
    <dct:language rdf:resource="http://publications.europa.eu/resource/authority/language/ENG"/>
    <dct:language rdf:resource="http://publications.europa.eu/resource/authority/language/ITA"/>
    <dct:modified rdf:datatype="http://www.w3.org/2001/XMLSchema#date">2020-06-09</dct:modified>
    <dct:publisher rdf:resource="http://spcdata.digitpa.gov.it/Amministrazione/agid"/>
    <dct:rightsHolder rdf:resource="http://spcdata.digitpa.gov.it/Amministrazione/agid"/>
    <dct:title xml:lang="en">IoT event Ontology - Italian Application Profile</dct:title>
    <dct:title xml:lang="it">Ontologia Eventi IoT - Profilo applicativo italiano</dct:title>
    <rdfs:comment xml:lang="it">Questa è l'ontologia di eventi IoT. Essa può essere utilizzata per esempio per rappresentare serie temporali e misure di sensoristica di vario tipo. Attualmente l'ontologia include classi specializzate per la modellazione di flussi di traffico.</rdfs:comment>
    <rdfs:comment xml:lang="en">This is the ontology used to represent IoT events. It can be used to model temporal series and measures of sensors of different types. Currently the ontology has been specialized for modelling traffic flows.</rdfs:comment>
    <rdfs:isDefinedBy rdf:resource="https://w3id.org/italia/onto/IoT"/>
    <rdfs:label xml:lang="en">IoT event Ontology</rdfs:label>
    <rdfs:label xml:lang="it">Ontologia Eventi IoT</rdfs:label>
    <owl:versionInfo xml:lang="en">Version 1.1 - June 9 2020 - modification of the alignments to l0 for Method, FeatureOfInterest, ObservationParameter classes</owl:versionInfo>
    <owl:versionInfo xml:lang="it">Versione 1.1 - Giugno 9 2020 - modificati gli allineamenti a l0 per le classi Metodo, Caratteristica di Interesse e Parametro dell'Osservazione.</owl:versionInfo>
    <dcat:contactPoint rdf:resource="https://w3id.org/italia/data/contact-point/onto-agid"/>
    <dcat:keyword xml:lang="it">Internet of Things</dcat:keyword>
    <dcat:keyword xml:lang="it">Misurazione</dcat:keyword>
    <dcat:keyword xml:lang="it">Osservazione</dcat:keyword>
    <dcat:keyword xml:lang="it">Sensore</dcat:keyword>
    <dcat:keyword xml:lang="it">flusso di traffico</dcat:keyword>
    <dcat:theme rdf:resource="http://publications.europa.eu/resource/authority/data-theme/TECH"/>
    <dcat:theme rdf:resource="http://publications.europa.eu/resource/authority/data-theme/TRAN"/>
    <prov:wasDerivedFrom rdf:resource="https://w3id.org/italia/onto/IoT/1.0"/>
    <admsapit:acronym>IoT-AP_IT</admsapit:acronym>
    <admsapit:hasContributor rdf:resource="https://w3id.org/italia/data/organization/public-organization/td"/>
    <admsapit:hasFormalityLevel rdf:resource="https://w3id.org/italia/onto/ADMS/Formal"/>
    <admsapit:hasKeyClass rdf:resource="https://w3id.org/italia/onto/IoT/Actuator"/>
    <admsapit:hasKeyClass rdf:resource="https://w3id.org/italia/onto/IoT/Observation"/>
    <admsapit:hasKeyClass rdf:resource="https://w3id.org/italia/onto/IoT/Sensor"/>
    <admsapit:hasOntologyLanguage rdf:resource="https://w3id.org/italia/onto/ADMS/OWL"/>
    <admsapit:hasSemanticAssetDistribution rdf:resource="https://w3id.org/italia/data/distribution/IOT-JSON-LD"/>
    <admsapit:hasSemanticAssetDistribution rdf:resource="https://w3id.org/italia/data/distribution/IOT-RDF-TURTLE"/>
    <admsapit:hasSemanticAssetDistribution rdf:resource="https://w3id.org/italia/data/distribution/IOT-RDF-XML"/>
    <admsapit:hasTask rdf:resource="https://w3id.org/italia/onto/ADMS/AnnotationTask"/>
    <admsapit:hasTask rdf:resource="https://w3id.org/italia/onto/ADMS/QueryFormulationTask"/>
    <admsapit:hasTask rdf:resource="https://w3id.org/italia/onto/ADMS/SearchTask"/>
    <admsapit:last rdf:resource="https://w3id.org/italia/onto/IoT/1.0"/>
    <admsapit:officialURI rdf:datatype="http://www.w3.org/2001/XMLSchema#anyURI">https://w3id.org/italia/onto/IoT</admsapit:officialURI>
    <admsapit:prefix>iotapit</admsapit:prefix>
    <admsapit:semanticAssetInUse rdf:resource="https://w3id.org/italia/data/project/DAF"/>
    <admsapit:semanticAssetInUse rdf:resource="https://w3id.org/italia/data/project/OntoPiA"/>
    <admsapit:status>catalogued</admsapit:status>
    <admsapit:status>published</admsapit:status>
    <admsapit:target xml:lang="it">Cittadini</admsapit:target>
    <admsapit:target xml:lang="it">Imprese</admsapit:target>
    <admsapit:target xml:lang="it">Pubbliche Amministrazioni</admsapit:target>
    <admsapit:type rdf:resource="https://w3id.org/italia/onto/ADMS/ServiceOntology"/>
  </rdf:Description>
  <rdf:Description rdf:about="https://w3id.org/italia/onto/IoT/RoadSegment">
    <rdf:type rdf:resource="http://www.w3.org/2002/07/owl#Class"/>
    <rdfs:subClassOf rdf:resource="https://w3id.org/italia/onto/IoT/FeatureOfInterest"/>
    <rdfs:comment xml:lang="it">Classe che rappresenta un arco stradale. Se l'ontologia è utilizzata per rappresentare eventi IoT nell'ambito dei dati real time sul traffico, la classe è rilevante e connota l'arco stradale dell'osservazione.</rdfs:comment>
    <rdfs:comment xml:lang="en">This class represents the Road Segment  If the ontology is used to represent IoT events in the context of real time data traffic, the class is revelant and it represents the road segment of the observation.</rdfs:comment>
    <rdfs:isDefinedBy rdf:resource="https://w3id.org/italia/onto/IoT"/>
    <rdfs:label xml:lang="it">Arco Stradale</rdfs:label>
    <rdfs:label xml:lang="en">Road Segment</rdfs:label>
    <owl:versionInfo xml:lang="it">stabile</owl:versionInfo>
    <owl:versionInfo xml:lang="en">stable</owl:versionInfo>
  </rdf:Description>
  <rdf:Description rdf:about="https://w3id.org/italia/onto/IoT/Platform">
    <rdf:type rdf:resource="http://www.w3.org/2002/07/owl#Class"/>
    <rdfs:subClassOf rdf:resource="https://w3id.org/italia/onto/l0/Object"/>
    <rdfs:subClassOf rdf:nodeID="n690e025d2eb648a3a4574298c2d1991cb33"/>
    <rdfs:comment xml:lang="it">E' un oggetto che ospita strumenti di monitoraggio.  Può essere una boa, un cellulare, un sistema satellitare, una stazione meteo.</rdfs:comment>
    <rdfs:comment xml:lang="en">It is an object that hosts monitoring facilities. It can be a buoy, a mobile phone, a meteo station, a satellite</rdfs:comment>
    <rdfs:isDefinedBy rdf:resource="https://w3id.org/italia/onto/IoT"/>
    <rdfs:label xml:lang="it">Piattaforma</rdfs:label>
    <rdfs:label xml:lang="en">Platform</rdfs:label>
    <owl:versionInfo xml:lang="it">provvisorio - da validare</owl:versionInfo>
    <owl:versionInfo xml:lang="en">unstable</owl:versionInfo>
  </rdf:Description>
  <rdf:Description rdf:about="https://w3id.org/italia/onto/IoT/hasFeatureOfInterest">
    <rdf:type rdf:resource="http://www.w3.org/2002/07/owl#ObjectProperty"/>
    <owl:inverseOf rdf:resource="https://w3id.org/italia/onto/IoT/isFeatureOfInterestFor"/>
    <rdfs:domain rdf:resource="https://w3id.org/italia/onto/IoT/Observation"/>
    <rdfs:range rdf:resource="https://w3id.org/italia/onto/IoT/FeatureOfInterest"/>
    <rdfs:comment xml:lang="en">Property that links the Observation to a feature of interest.</rdfs:comment>
    <rdfs:comment xml:lang="it">Proprietà che lega un'osservazione a una caratteristica di interesse.</rdfs:comment>
    <rdfs:isDefinedBy rdf:resource="https://w3id.org/italia/onto/IoT"/>
    <rdfs:label xml:lang="it">ha caratteristica di interesse</rdfs:label>
    <rdfs:label xml:lang="en">has feature of interest</rdfs:label>
    <owl:versionInfo xml:lang="it">stabile</owl:versionInfo>
    <owl:versionInfo xml:lang="en">stable</owl:versionInfo>
  </rdf:Description>
  <rdf:Description rdf:about="https://w3id.org/italia/onto/IoT/implementsMethod">
    <rdf:type rdf:resource="http://www.w3.org/2002/07/owl#ObjectProperty"/>
    <rdfs:domain rdf:resource="https://w3id.org/italia/onto/IoT/MonitoringFacility"/>
    <rdfs:range rdf:resource="https://w3id.org/italia/onto/IoT/Method"/>
    <rdfs:isDefinedBy rdf:resource="https://w3id.org/italia/onto/IoT"/>
  </rdf:Description>
  <rdf:Description rdf:nodeID="n690e025d2eb648a3a4574298c2d1991cb7">
    <rdf:type rdf:resource="http://www.w3.org/2002/07/owl#Restriction"/>
    <owl:onProperty rdf:resource="https://w3id.org/italia/onto/IoT/hasObservationParameter"/>
    <owl:someValuesFrom rdf:resource="https://w3id.org/italia/onto/IoT/ObservationParameter"/>
  </rdf:Description>
  <rdf:Description rdf:about="https://w3id.org/italia/onto/CLV/Geometry">
    <rdf:type rdf:resource="http://www.w3.org/2002/07/owl#Class"/>
    <rdfs:isDefinedBy rdf:resource="https://w3id.org/italia/onto/CLV/"/>
  </rdf:Description>
  <rdf:Description rdf:nodeID="n690e025d2eb648a3a4574298c2d1991cb8">
    <rdf:type rdf:resource="http://www.w3.org/2002/07/owl#Restriction"/>
    <owl:onProperty rdf:resource="https://w3id.org/italia/onto/IoT/hasObservationValue"/>
    <owl:someValuesFrom rdf:resource="https://w3id.org/italia/onto/IoT/ObservationValue"/>
  </rdf:Description>
  <rdf:Description rdf:nodeID="n690e025d2eb648a3a4574298c2d1991cb23">
    <rdf:type rdf:resource="http://www.w3.org/2002/07/owl#Restriction"/>
    <owl:onProperty rdf:resource="https://w3id.org/italia/onto/IoT/observationCollectionMadeBySensor"/>
    <owl:qualifiedCardinality rdf:datatype="http://www.w3.org/2001/XMLSchema#nonNegativeInteger">1</owl:qualifiedCardinality>
    <owl:onClass rdf:resource="https://w3id.org/italia/onto/IoT/Sensor"/>
  </rdf:Description>
  <rdf:Description rdf:about="https://w3id.org/italia/data/distribution/IOT-RDF-XML">
    <rdf:type rdf:resource="http://www.w3.org/2002/07/owl#NamedIndividual"/>
    <rdf:type rdf:resource="https://w3id.org/italia/onto/ADMS/SemanticAssetDistribution"/>
    <dct:description xml:lang="it">Questa è la distribuzione RDF/XML dell'ontologia degli eventi IoT</dct:description>
    <dct:description xml:lang="en">This is the distribution in RDF/XML of the IoT Events ontology</dct:description>
    <dct:format rdf:resource="http://publications.europa.eu/resource/authority/file-type/RDF_XML"/>
    <dct:license rdf:resource="https://w3id.org/italia/controlled-vocabulary/licences/A21_CCBY40"/>
    <dct:title xml:lang="it">Distribuzione RDF/XML ontologia IoT-AP_IT</dct:title>
    <dct:title xml:lang="en">RDF/XML distribution of IoT-AP_IT Ontology</dct:title>
    <dcat:accessURL rdf:resource="https://raw.githubusercontent.com/italia/daf-ontologie-vocabolari-controllati/master/Ontologie/IoT/latest"/>
    <dcat:downloadURL rdf:resource="https://raw.githubusercontent.com/italia/daf-ontologie-vocabolari-controllati/master/Ontologie/IoT/latest/IoT-AP_IT.rdf"/>
  </rdf:Description>
  <rdf:Description rdf:about="https://w3id.org/italia/data/project/OntoPiA">
    <rdf:type rdf:resource="http://www.w3.org/2002/07/owl#NamedIndividual"/>
    <rdf:type rdf:resource="https://w3id.org/italia/onto/ADMS/Project"/>
    <l0:name xml:lang="it">OntoPiA - la rete di ontologie della pubblica amministrazione italiana</l0:name>
  </rdf:Description>
  <rdf:Description rdf:nodeID="n690e025d2eb648a3a4574298c2d1991cb27">
    <rdf:first rdf:resource="https://w3id.org/italia/onto/l0/Concept"/>
    <rdf:rest rdf:resource="http://www.w3.org/1999/02/22-rdf-syntax-ns#nil"/>
  </rdf:Description>
  <rdf:Description rdf:nodeID="n690e025d2eb648a3a4574298c2d1991cb11">
    <rdf:type rdf:resource="http://www.w3.org/2002/07/owl#Restriction"/>
    <owl:onProperty rdf:resource="https://w3id.org/italia/onto/IoT/hasFeatureOfInterest"/>
    <owl:qualifiedCardinality rdf:datatype="http://www.w3.org/2001/XMLSchema#nonNegativeInteger">1</owl:qualifiedCardinality>
    <owl:onClass rdf:resource="https://w3id.org/italia/onto/IoT/FeatureOfInterest"/>
  </rdf:Description>
  <rdf:Description rdf:about="https://w3id.org/italia/onto/IoT/generationTime">
    <rdf:type rdf:resource="http://www.w3.org/2002/07/owl#ObjectProperty"/>
    <rdfs:subPropertyOf rdf:resource="https://w3id.org/italia/onto/TI/atTime"/>
    <rdfs:domain rdf:resource="https://w3id.org/italia/onto/IoT/Observation"/>
    <rdfs:range rdf:resource="https://w3id.org/italia/onto/TI/TimeInterval"/>
    <rdfs:comment xml:lang="it">Questa proprietà è sottoproprietà di atTime e consente di modellare il tempo di generazione della osservazione.</rdfs:comment>
    <rdfs:comment xml:lang="en">This property is a subproperty of atTime and defines the generation time of the observation.</rdfs:comment>
    <rdfs:isDefinedBy rdf:resource="https://w3id.org/italia/onto/IoT"/>
    <rdfs:label xml:lang="en">generation time</rdfs:label>
    <rdfs:label xml:lang="it">tempo di generazione</rdfs:label>
    <owl:versionInfo xml:lang="it">stabile</owl:versionInfo>
    <owl:versionInfo xml:lang="en">stable</owl:versionInfo>
  </rdf:Description>
  <rdf:Description rdf:about="http://spcdata.digitpa.gov.it/Amministrazione/agid">
    <rdf:type rdf:resource="http://www.w3.org/2002/07/owl#NamedIndividual"/>
    <rdf:type rdf:resource="http://dati.gov.it/onto/dcatapit#Agent"/>
    <rdf:type rdf:resource="http://xmlns.com/foaf/0.1/Agent"/>
    <dct:identifier>agid</dct:identifier>
    <foaf:name xml:lang="it">Agenzia per l'Italia Digitale</foaf:name>
    <foaf:name xml:lang="en">Italian Digital Agency</foaf:name>
  </rdf:Description>
  <rdf:Description rdf:about="https://w3id.org/italia/onto/IoT/Accuracy">
    <rdf:type rdf:resource="http://www.w3.org/2002/07/owl#Class"/>
    <rdfs:subClassOf rdf:resource="https://w3id.org/italia/onto/IoT/MeasurementQuality"/>
    <rdfs:comment xml:lang="en">It represents the Accuracy; that is, the maximimum difference between the indicated value and the actual measurand being monitored, whilst taking into account all possible sources of error that are relevant to the application.</rdfs:comment>
    <rdfs:comment xml:lang="it">Questa classe rappresenta l'Accuratezza, cioè la differenza massima tra il valore indicato e il valore effettivo monitorato, tenuto conto di tutte le possibili fonti di errore rilevanti per l'applicazione.</rdfs:comment>
    <rdfs:isDefinedBy rdf:resource="https://w3id.org/italia/onto/IoT"/>
    <rdfs:label xml:lang="en">Accuracy</rdfs:label>
    <rdfs:label xml:lang="it">Accuratezza</rdfs:label>
    <owl:versionInfo xml:lang="it">instabile</owl:versionInfo>
    <owl:versionInfo xml:lang="en">unstable</owl:versionInfo>
  </rdf:Description>
  <rdf:Description rdf:about="https://w3id.org/italia/onto/IoT/ObservationCollection">
    <rdf:type rdf:resource="http://www.w3.org/2002/07/owl#Class"/>
    <rdfs:subClassOf rdf:resource="https://w3id.org/italia/onto/l0/Collection"/>
    <rdfs:subClassOf rdf:nodeID="n690e025d2eb648a3a4574298c2d1991cb22"/>
    <rdfs:subClassOf rdf:nodeID="n690e025d2eb648a3a4574298c2d1991cb23"/>
    <rdfs:subClassOf rdf:nodeID="n690e025d2eb648a3a4574298c2d1991cb24"/>
    <rdfs:comment xml:lang="it">Questa classe rappresenta una collezione di osservazioni fatte da un sensore. Potrebbe anche essere vista come uno stream di dati.</rdfs:comment>
    <rdfs:comment xml:lang="en">This class represents a collection of observations made by a sensor. It can also be thought of as a data stream.</rdfs:comment>
    <rdfs:isDefinedBy rdf:resource="https://w3id.org/italia/onto/IoT"/>
    <rdfs:label xml:lang="it">Collezione di Osservazioni</rdfs:label>
    <rdfs:label xml:lang="en">Observation Collection</rdfs:label>
    <owl:versionInfo xml:lang="it">instabile</owl:versionInfo>
    <owl:versionInfo xml:lang="en">unstable</owl:versionInfo>
  </rdf:Description>
  <rdf:Description rdf:about="https://w3id.org/italia/onto/IoT/makesObservation">
    <rdf:type rdf:resource="http://www.w3.org/2002/07/owl#ObjectProperty"/>
    <owl:inverseOf rdf:resource="https://w3id.org/italia/onto/IoT/observationMadeBySensor"/>
    <rdfs:domain rdf:resource="https://w3id.org/italia/onto/IoT/Sensor"/>
    <rdfs:range rdf:resource="https://w3id.org/italia/onto/IoT/Observation"/>
    <rdfs:comment xml:lang="en">Property that links a Sensor to the Observation.</rdfs:comment>
    <rdfs:comment xml:lang="it">Proprietà che collega un sensore all'osservazione fatta dal sensore.</rdfs:comment>
    <rdfs:isDefinedBy rdf:resource="https://w3id.org/italia/onto/IoT"/>
    <rdfs:label xml:lang="it">emette osservazione</rdfs:label>
    <rdfs:label xml:lang="it">fa osservazione</rdfs:label>
    <rdfs:label xml:lang="en">makes observation</rdfs:label>
    <rdfs:label xml:lang="it">produce osservazione</rdfs:label>
    <owl:versionInfo xml:lang="it">stabile</owl:versionInfo>
    <owl:versionInfo xml:lang="en">stable</owl:versionInfo>
  </rdf:Description>
  <rdf:Description rdf:about="https://w3id.org/italia/onto/IoT/phenomenonTime">
    <rdf:type rdf:resource="http://www.w3.org/2002/07/owl#ObjectProperty"/>
    <rdfs:subPropertyOf rdf:resource="https://w3id.org/italia/onto/TI/atTime"/>
    <rdfs:domain rdf:resource="https://w3id.org/italia/onto/IoT/Observation"/>
    <rdfs:range rdf:resource="https://w3id.org/italia/onto/TI/TimeInterval"/>
    <rdfs:comment xml:lang="it">Questa proprietà è sotto proprietà di atTime ed è utilizzata per modellare il tempo di validità dell'osservazione.</rdfs:comment>
    <rdfs:comment xml:lang="en">This property is subproperty of atTime and it is used to model the valididty time of an observation.</rdfs:comment>
    <rdfs:isDefinedBy rdf:resource="https://w3id.org/italia/onto/IoT"/>
    <rdfs:label xml:lang="en">phenomenon time</rdfs:label>
    <rdfs:label xml:lang="it">tempo di validità</rdfs:label>
    <rdfs:label xml:lang="it">tempo di validità del fenomeno</rdfs:label>
    <owl:versionInfo xml:lang="it">stabile</owl:versionInfo>
    <owl:versionInfo xml:lang="en">stable</owl:versionInfo>
  </rdf:Description>
  <rdf:Description rdf:about="https://w3id.org/italia/onto/IoT/comesFrom">
    <rdf:type rdf:resource="http://www.w3.org/2002/07/owl#ObjectProperty"/>
    <rdfs:domain rdf:resource="https://w3id.org/italia/onto/IoT/Observation"/>
    <rdfs:range rdf:resource="https://w3id.org/italia/onto/IoT/Platform"/>
    <rdfs:comment xml:lang="en">Property that links the observation with the platofrm where it comes from.</rdfs:comment>
    <rdfs:comment xml:lang="it">Proprietà che lega l'osservazione con la piattaforma da cui deriva.</rdfs:comment>
    <rdfs:isDefinedBy rdf:resource="https://w3id.org/italia/onto/IoT"/>
    <rdfs:label xml:lang="en">comes from</rdfs:label>
    <rdfs:label xml:lang="it">proviene da</rdfs:label>
    <owl:versionInfo xml:lang="it">provvisoria - da validare</owl:versionInfo>
    <owl:versionInfo xml:lang="en">unstable</owl:versionInfo>
  </rdf:Description>
  <rdf:Description rdf:about="https://w3id.org/italia/onto/IoT/makesObservationCollection">
    <rdf:type rdf:resource="http://www.w3.org/2002/07/owl#ObjectProperty"/>
    <owl:inverseOf rdf:resource="https://w3id.org/italia/onto/IoT/observationCollectionMadeBySensor"/>
    <rdfs:domain rdf:resource="https://w3id.org/italia/onto/IoT/Sensor"/>
    <rdfs:range rdf:resource="https://w3id.org/italia/onto/IoT/ObservationCollection"/>
    <rdfs:comment xml:lang="it">Questa proprietà collega un sensore a una collezione di osservazioni che esso fa.</rdfs:comment>
    <rdfs:comment xml:lang="en">The property links a sensor to the collection of observations that it makes.</rdfs:comment>
    <rdfs:isDefinedBy rdf:resource="https://w3id.org/italia/onto/IoT"/>
    <rdfs:label xml:lang="it">fa collezioni di osservazioni</rdfs:label>
    <rdfs:label xml:lang="en">makes observation collection</rdfs:label>
    <rdfs:label xml:lang="it">produce collezioni di osservazioni</rdfs:label>
    <owl:versionInfo xml:lang="it">stabile</owl:versionInfo>
    <owl:versionInfo xml:lang="en">stable</owl:versionInfo>
  </rdf:Description>
  <rdf:Description rdf:about="https://w3id.org/italia/onto/IoT/Latency">
    <rdf:type rdf:resource="http://www.w3.org/2002/07/owl#Class"/>
    <rdfs:subClassOf rdf:resource="https://w3id.org/italia/onto/IoT/MeasurementQuality"/>
    <rdfs:comment xml:lang="en">It represents the Latency; i.e., the time delay between the cause and the effect of some change in the system being observed</rdfs:comment>
    <rdfs:comment xml:lang="it">Questa classe rappresenta la Latenza, ovvero il ritardo di tempo tra la causa e l'effetto di qualche cambiamento nel sistema osservarto.</rdfs:comment>
    <rdfs:isDefinedBy rdf:resource="https://w3id.org/italia/onto/IoT"/>
    <rdfs:label xml:lang="en">Latency</rdfs:label>
    <rdfs:label xml:lang="it">Latenza</rdfs:label>
    <owl:versionInfo xml:lang="it">instabile</owl:versionInfo>
    <owl:versionInfo xml:lang="en">unstable</owl:versionInfo>
  </rdf:Description>
  <rdf:Description rdf:about="https://w3id.org/italia/data/project/DAF">
    <rdf:type rdf:resource="http://www.w3.org/2002/07/owl#NamedIndividual"/>
    <rdf:type rdf:resource="https://w3id.org/italia/onto/ADMS/Project"/>
    <foaf:name xml:lang="it">Data &amp; Analytics Framework</foaf:name>
  </rdf:Description>
  <rdf:Description rdf:nodeID="n690e025d2eb648a3a4574298c2d1991cb15">
    <rdf:type rdf:resource="http://www.w3.org/2002/07/owl#Restriction"/>
    <owl:onProperty rdf:resource="https://w3id.org/italia/onto/IoT/generationTime"/>
    <owl:maxQualifiedCardinality rdf:datatype="http://www.w3.org/2001/XMLSchema#nonNegativeInteger">1</owl:maxQualifiedCardinality>
    <owl:onClass rdf:resource="https://w3id.org/italia/onto/TI/TimeInterval"/>
  </rdf:Description>
  <rdf:Description rdf:about="http://purl.org/dc/terms/license">
    <rdf:type rdf:resource="http://www.w3.org/2002/07/owl#AnnotationProperty"/>
  </rdf:Description>
  <rdf:Description rdf:nodeID="n690e025d2eb648a3a4574298c2d1991cb17">
    <rdf:type rdf:resource="http://www.w3.org/2002/07/owl#Restriction"/>
    <owl:onProperty rdf:resource="https://w3id.org/italia/onto/TI/atTime"/>
    <owl:maxQualifiedCardinality rdf:datatype="http://www.w3.org/2001/XMLSchema#nonNegativeInteger">1</owl:maxQualifiedCardinality>
    <owl:onClass rdf:resource="https://w3id.org/italia/onto/TI/TimeInterval"/>
  </rdf:Description>
  <rdf:Description rdf:about="https://w3id.org/italia/onto/IoT/isObservationValueOf">
    <rdf:type rdf:resource="http://www.w3.org/2002/07/owl#ObjectProperty"/>
    <rdfs:domain rdf:resource="https://w3id.org/italia/onto/IoT/ObservationValue"/>
    <rdfs:range rdf:resource="https://w3id.org/italia/onto/IoT/Observation"/>
    <rdfs:comment xml:lang="en">Inverse property of hasObservedValue that links an ObservedValue to its related Observation.</rdfs:comment>
    <rdfs:comment xml:lang="it">Proprietà inversa di ha valore osservato che unisce un valore osservato alla relativa osservazione.</rdfs:comment>
    <rdfs:isDefinedBy rdf:resource="https://w3id.org/italia/onto/IoT"/>
    <rdfs:label xml:lang="en">is osbservation value of</rdfs:label>
    <rdfs:label xml:lang="it">è valore osservato di</rdfs:label>
    <owl:versionInfo xml:lang="it">stabile</owl:versionInfo>
    <owl:versionInfo xml:lang="en">stable</owl:versionInfo>
  </rdf:Description>
  <rdf:Description rdf:about="https://w3id.org/italia/onto/IoT/isMeasurementQualityValueOf">
    <rdf:type rdf:resource="http://www.w3.org/2002/07/owl#ObjectProperty"/>
    <rdfs:domain rdf:resource="https://w3id.org/italia/onto/IoT/MeasurementQualityValue"/>
    <rdfs:range rdf:resource="https://w3id.org/italia/onto/IoT/MeasurementQuality"/>
    <rdfs:comment xml:lang="en">Inverse property of has measurement quality value that links the measurement quality value to the measurment quality.</rdfs:comment>
    <rdfs:comment xml:lang="it">Proprietà inversa che lega un valore della qualità di misurazione con la qualità di misurazione.</rdfs:comment>
    <rdfs:isDefinedBy rdf:resource="https://w3id.org/italia/onto/IoT"/>
    <rdfs:label xml:lang="en">is measurement quality value of</rdfs:label>
    <rdfs:label xml:lang="it">è valore di qualità di misurazione di</rdfs:label>
    <owl:versionInfo xml:lang="it">stabile</owl:versionInfo>
    <owl:versionInfo xml:lang="en">stable</owl:versionInfo>
  </rdf:Description>
  <rdf:Description rdf:nodeID="n690e025d2eb648a3a4574298c2d1991cb34">
    <rdf:type rdf:resource="http://www.w3.org/2002/07/owl#Restriction"/>
    <owl:onProperty rdf:resource="https://w3id.org/italia/onto/IoT/makesObservation"/>
    <owl:allValuesFrom rdf:resource="https://w3id.org/italia/onto/IoT/Observation"/>
  </rdf:Description>
  <rdf:Description rdf:about="https://w3id.org/italia/onto/IoT/FeatureOfInterest">
    <rdf:type rdf:resource="http://www.w3.org/2002/07/owl#Class"/>
    <rdfs:subClassOf rdf:resource="https://w3id.org/italia/onto/l0/Entity"/>
    <rdfs:subClassOf rdf:nodeID="n690e025d2eb648a3a4574298c2d1991cb1"/>
    <rdfs:subClassOf rdf:nodeID="n690e025d2eb648a3a4574298c2d1991cb2"/>
    <rdfs:comment xml:lang="en">It represents the Feature whose Observed Attribute is being observed by a Sensor in order to get an Observed Value. For instance, if we say that the temperature of the kitchen is 28 celsius degrees, the Feature of Interest is the kitchen.</rdfs:comment>
    <rdfs:comment xml:lang="it">Rappresenta la caratteristica di interesse il cui attributo osservato è osservato da un sensor per ottenere un valore osservato. Per esempio, se diciamo che la temperatura della cucina è di 28 gradi celsius, la caratteristica di interesse è la cucina.</rdfs:comment>
    <rdfs:isDefinedBy rdf:resource="https://w3id.org/italia/onto/IoT"/>
    <rdfs:label xml:lang="it">Caratteristica di interesse</rdfs:label>
    <rdfs:label xml:lang="en">Feature of Interest</rdfs:label>
    <owl:versionInfo xml:lang="it">stabile</owl:versionInfo>
    <owl:versionInfo xml:lang="en">stable</owl:versionInfo>
  </rdf:Description>
  <rdf:Description rdf:about="https://w3id.org/italia/onto/IoT/hasQuality">
    <rdf:type rdf:resource="http://www.w3.org/2002/07/owl#ObjectProperty"/>
    <rdfs:domain rdf:resource="https://w3id.org/italia/onto/IoT/Observation"/>
    <rdfs:range rdf:resource="https://w3id.org/italia/onto/IoT/MeasurementQuality"/>
    <rdfs:comment xml:lang="en">Property that links an Observation to a number of measurement capabilities.</rdfs:comment>
    <rdfs:comment xml:lang="it">Proprietà che lega un'osservazione a una serie di parametri di qualità.</rdfs:comment>
    <rdfs:isDefinedBy rdf:resource="https://w3id.org/italia/onto/IoT"/>
    <rdfs:label xml:lang="it">ha qualità</rdfs:label>
    <rdfs:label xml:lang="en">has quality</rdfs:label>
    <owl:versionInfo xml:lang="it">stabile</owl:versionInfo>
    <owl:versionInfo xml:lang="en">stable</owl:versionInfo>
  </rdf:Description>
  <rdf:Description rdf:about="https://w3id.org/italia/onto/IoT/hasObservationParameter">
    <rdf:type rdf:resource="http://www.w3.org/2002/07/owl#ObjectProperty"/>
    <owl:inverseOf rdf:resource="https://w3id.org/italia/onto/IoT/isObservationParameterFor"/>
    <rdfs:domain rdf:resource="https://w3id.org/italia/onto/IoT/Observation"/>
    <rdfs:range rdf:resource="https://w3id.org/italia/onto/IoT/ObservationParameter"/>
    <rdfs:comment xml:lang="en">Property that links an observation to its parameter being observed.</rdfs:comment>
    <rdfs:comment xml:lang="it">Proprietà che collega un'osservazione al suo parametro osservato.</rdfs:comment>
    <rdfs:isDefinedBy rdf:resource="https://w3id.org/italia/onto/IoT"/>
    <rdfs:label xml:lang="it">ha parametro dell'osservazione</rdfs:label>
    <rdfs:label xml:lang="en">has observation parameter</rdfs:label>
    <owl:versionInfo xml:lang="it">stabile</owl:versionInfo>
    <owl:versionInfo xml:lang="en">stable</owl:versionInfo>
  </rdf:Description>
  <rdf:Description rdf:about="https://w3id.org/italia/onto/IoT/isHostedByPlatform">
    <rdf:type rdf:resource="http://www.w3.org/2002/07/owl#ObjectProperty"/>
    <rdfs:domain rdf:resource="https://w3id.org/italia/onto/IoT/MonitoringFacility"/>
    <rdfs:range rdf:resource="https://w3id.org/italia/onto/IoT/Platform"/>
    <rdfs:comment xml:lang="en">inverse property of "hosts monitoring facility" that connects moniotirng facilities with the platform that hosts them.</rdfs:comment>
    <rdfs:comment xml:lang="it">proprietà inversa di "ospita strumenti di monitoraggio" che collega gli strumenti di monitoraggio con la piattaforma che li ospitano</rdfs:comment>
    <rdfs:isDefinedBy rdf:resource="https://w3id.org/italia/onto/IoT"/>
    <rdfs:label xml:lang="en">is hosted by platform</rdfs:label>
    <rdfs:label xml:lang="it">è ospitato da piattaforma</rdfs:label>
    <owl:versionInfo xml:lang="it">provvisoria - da validare</owl:versionInfo>
    <owl:versionInfo xml:lang="en">unstable</owl:versionInfo>
  </rdf:Description>
  <rdf:Description rdf:about="http://purl.org/dc/elements/1.1/creator">
    <rdf:type rdf:resource="http://www.w3.org/2002/07/owl#AnnotationProperty"/>
  </rdf:Description>
  <rdf:Description rdf:about="https://w3id.org/italia/onto/IoT/Sensor">
    <rdf:type rdf:resource="http://www.w3.org/2002/07/owl#Class"/>
    <rdfs:subClassOf rdf:resource="https://w3id.org/italia/onto/IoT/MonitoringFacility"/>
    <rdfs:subClassOf rdf:nodeID="n690e025d2eb648a3a4574298c2d1991cb34"/>
    <rdfs:subClassOf rdf:nodeID="n690e025d2eb648a3a4574298c2d1991cb35"/>
    <rdfs:subClassOf rdf:nodeID="n690e025d2eb648a3a4574298c2d1991cb36"/>
    <rdfs:comment xml:lang="it">Questa classe rappresenta un sensore. Un sensore è uno strumento il cui scopo è quello di rilevare e rispondere a eventi o cambiamenti che avvengono nel proprio ambienti. L'informazione rilevata può essere  utilizzata e distribuita per successive elaborazioni.</rdfs:comment>
    <rdfs:comment xml:lang="en">This class represents a sensor. A sensor is a device whose purpose is to detect and respond to events or changes in its environment. The detected information can be used and disseminated for successive elaborations.</rdfs:comment>
    <rdfs:isDefinedBy rdf:resource="https://w3id.org/italia/onto/IoT"/>
    <rdfs:label xml:lang="en">Sensor</rdfs:label>
    <rdfs:label xml:lang="it">Sensore</rdfs:label>
    <owl:versionInfo xml:lang="it">stabile</owl:versionInfo>
    <owl:versionInfo xml:lang="en">stable</owl:versionInfo>
  </rdf:Description>
  <rdf:Description rdf:nodeID="n690e025d2eb648a3a4574298c2d1991cb20">
    <rdf:type rdf:resource="http://www.w3.org/2002/07/owl#Restriction"/>
    <owl:onProperty rdf:resource="https://w3id.org/italia/onto/TI/issued"/>
    <owl:maxQualifiedCardinality rdf:datatype="http://www.w3.org/2001/XMLSchema#nonNegativeInteger">1</owl:maxQualifiedCardinality>
    <owl:onDataRange rdf:resource="http://www.w3.org/2001/XMLSchema#dateTime"/>
  </rdf:Description>
  <rdf:Description rdf:nodeID="n690e025d2eb648a3a4574298c2d1991cb21">
    <rdf:type rdf:resource="http://www.w3.org/2002/07/owl#Restriction"/>
    <owl:onProperty rdf:resource="https://w3id.org/italia/onto/TI/modified"/>
    <owl:maxQualifiedCardinality rdf:datatype="http://www.w3.org/2001/XMLSchema#nonNegativeInteger">1</owl:maxQualifiedCardinality>
    <owl:onDataRange rdf:resource="http://www.w3.org/2001/XMLSchema#dateTime"/>
  </rdf:Description>
  <rdf:Description rdf:about="https://w3id.org/italia/onto/IoT/hasMeasurementQualityValue">
    <rdf:type rdf:resource="http://www.w3.org/2002/07/owl#ObjectProperty"/>
    <owl:inverseOf rdf:resource="https://w3id.org/italia/onto/IoT/isMeasurementQualityValueOf"/>
    <rdfs:domain rdf:resource="https://w3id.org/italia/onto/IoT/MeasurementQuality"/>
    <rdfs:range rdf:resource="https://w3id.org/italia/onto/IoT/MeasurementQualityValue"/>
    <rdfs:comment xml:lang="en">Property that links the Measrurement Quality with its value.</rdfs:comment>
    <rdfs:comment xml:lang="it">Proprietà che collega la Misurazione di qualità con il relativo valore.</rdfs:comment>
    <rdfs:isDefinedBy rdf:resource="https://w3id.org/italia/onto/IoT"/>
    <rdfs:label xml:lang="it">ha valore di qualità di misurazione</rdfs:label>
    <rdfs:label xml:lang="en">has measurement quality value</rdfs:label>
    <owl:versionInfo xml:lang="it">stabile</owl:versionInfo>
    <owl:versionInfo xml:lang="en">stable</owl:versionInfo>
  </rdf:Description>
  <rdf:Description rdf:about="https://w3id.org/italia/onto/IoT/hasValueForObservationParameter">
    <rdf:type rdf:resource="http://www.w3.org/2002/07/owl#ObjectProperty"/>
    <owl:inverseOf rdf:resource="https://w3id.org/italia/onto/IoT/isValueForObservationParameter"/>
    <rdfs:domain rdf:resource="https://w3id.org/italia/onto/IoT/ObservationParameter"/>
    <rdfs:range rdf:resource="https://w3id.org/italia/onto/IoT/ObservationValue"/>
    <rdfs:comment xml:lang="it">Questa proprietà connette l'attributo (parametro) dell'osservazione a rispettivo valore dell'osservazione.</rdfs:comment>
    <rdfs:comment xml:lang="en">This property links the Observation Parameter to the Observation Value.</rdfs:comment>
    <rdfs:isDefinedBy rdf:resource="https://w3id.org/italia/onto/IoT"/>
    <rdfs:label xml:lang="it">ha valore per parametro di osservazione</rdfs:label>
    <rdfs:label xml:lang="en">has value for observation parameter</rdfs:label>
    <owl:versionInfo xml:lang="it">stabile</owl:versionInfo>
    <owl:versionInfo xml:lang="en">stable</owl:versionInfo>
  </rdf:Description>
  <rdf:Description rdf:nodeID="n690e025d2eb648a3a4574298c2d1991cb1">
    <rdf:type rdf:resource="http://www.w3.org/2002/07/owl#Restriction"/>
    <owl:onProperty rdf:resource="https://w3id.org/italia/onto/IoT/isFeatureOfInterestFor"/>
    <owl:allValuesFrom rdf:resource="https://w3id.org/italia/onto/IoT/Observation"/>
  </rdf:Description>
  <rdf:Description rdf:about="https://w3id.org/italia/onto/IoT/ObservationValue">
    <rdf:type rdf:resource="http://www.w3.org/2002/07/owl#Class"/>
    <rdfs:subClassOf rdf:resource="https://w3id.org/italia/onto/MU/Value"/>
    <rdfs:subClassOf rdf:nodeID="n690e025d2eb648a3a4574298c2d1991cb31"/>
    <rdfs:subClassOf rdf:nodeID="n690e025d2eb648a3a4574298c2d1991cb32"/>
    <rdfs:comment xml:lang="en">It represents the value of the observation. For instance if we say that the temperature of the kitchen is 28 celsius degrees, the observed value is 28 celsius degrees.</rdfs:comment>
    <rdfs:comment xml:lang="it">Rappresenta il valore dell'osservazione. Per esempio se diciamo che la temperatura della cucina è di 28 gradi celsius, il valore osservato è 28 gradi celsius.</rdfs:comment>
    <rdfs:isDefinedBy rdf:resource="https://w3id.org/italia/onto/IoT"/>
    <rdfs:label xml:lang="en">Observation Value</rdfs:label>
    <rdfs:label xml:lang="it">Valore dell'Osservazione</rdfs:label>
    <owl:versionInfo xml:lang="it">stabile</owl:versionInfo>
    <owl:versionInfo xml:lang="en">stable</owl:versionInfo>
  </rdf:Description>
  <rdf:Description rdf:about="https://w3id.org/italia/data/contact-point/onto-agid">
    <rdf:type rdf:resource="http://www.w3.org/2002/07/owl#NamedIndividual"/>
    <rdf:type rdf:resource="http://dati.gov.it/onto/dcatapit#Organization"/>
    <rdf:type rdf:resource="http://www.w3.org/2006/vcard/ns#Kind"/>
    <rdf:type rdf:resource="http://www.w3.org/2006/vcard/ns#Organization"/>
    <vcard:fn>banche dati e open data</vcard:fn>
    <vcard:hasEmail rdf:resource="mailto:info@dati.gov.it"/>
  </rdf:Description>
  <rdf:Description rdf:about="https://w3id.org/italia/data/organization/support-unit/cnr-Z6HZEH/stlab">
    <rdf:type rdf:resource="http://www.w3.org/2002/07/owl#NamedIndividual"/>
    <rdf:type rdf:resource="http://dati.gov.it/onto/dcatapit#Agent"/>
    <dct:identifier>cnr - Z6HZEH - STLab</dct:identifier>
    <foaf:name xml:lang="en">Institute of Cognitive Sciences and Technologies of the Italian Research Council (CNR) - Semantic Technology Laboratory (STLab)</foaf:name>
    <foaf:name xml:lang="it">Istituto di Scienze e Tecnologie della Cognizione del CNR - Semantic Technology Lab (STLab)</foaf:name>
  </rdf:Description>
  <rdf:Description rdf:about="https://w3id.org/italia/onto/TI/modified">
    <rdf:type rdf:resource="http://www.w3.org/2002/07/owl#DatatypeProperty"/>
    <rdfs:isDefinedBy rdf:resource="https://w3id.org/italia/onto/TI/"/>
  </rdf:Description>
  <rdf:Description rdf:about="https://w3id.org/italia/onto/IoT/Repetability">
    <rdf:type rdf:resource="http://www.w3.org/2002/07/owl#Class"/>
    <rdfs:subClassOf rdf:resource="https://w3id.org/italia/onto/IoT/MeasurementQuality"/>
    <rdfs:comment xml:lang="en">It represents the Repetability; that is, the variation in measurements taken by the sensor on the same item, under the same conditions, and in a short period of time.</rdfs:comment>
    <rdfs:comment xml:lang="it">Questa classe rappresenta la ripetibilità ovvero la variazione nelle misurazioni fatte da un sensor sullo stesso oggetto, alle stesse condizioni e in un lasso breve di tempo.</rdfs:comment>
    <rdfs:isDefinedBy rdf:resource="https://w3id.org/italia/onto/IoT"/>
    <rdfs:label xml:lang="en">Repetability</rdfs:label>
    <rdfs:label xml:lang="it">Ripetibilità</rdfs:label>
    <owl:versionInfo xml:lang="it">instabile</owl:versionInfo>
    <owl:versionInfo xml:lang="en">unstable</owl:versionInfo>
  </rdf:Description>
  <rdf:Description rdf:about="https://w3id.org/italia/onto/IoT/TrafficFlow">
    <rdf:type rdf:resource="http://www.w3.org/2002/07/owl#Class"/>
    <rdfs:subClassOf rdf:resource="https://w3id.org/italia/onto/IoT/Observation"/>
    <rdfs:comment xml:lang="it">Questa classe rappresenta una specifica osservazione sui flussi di traffico</rdfs:comment>
    <rdfs:comment xml:lang="en">This class represents a specific observation on the traffic flows</rdfs:comment>
    <rdfs:isDefinedBy rdf:resource="https://w3id.org/italia/onto/IoT"/>
    <rdfs:label xml:lang="it">Flusso Traffico</rdfs:label>
    <rdfs:label xml:lang="en">Traffic Flow</rdfs:label>
    <owl:versionInfo xml:lang="it">instabile</owl:versionInfo>
    <owl:versionInfo xml:lang="en">unstable</owl:versionInfo>
  </rdf:Description>
  <rdf:Description rdf:nodeID="n690e025d2eb648a3a4574298c2d1991cb22">
    <rdf:type rdf:resource="http://www.w3.org/2002/07/owl#Restriction"/>
    <owl:onProperty rdf:resource="https://w3id.org/italia/onto/IoT/consistsOf"/>
    <owl:someValuesFrom rdf:resource="https://w3id.org/italia/onto/IoT/Observation"/>
  </rdf:Description>
  <rdf:Description rdf:about="https://w3id.org/italia/onto/IoT/isPartOf">
    <rdf:type rdf:resource="http://www.w3.org/2002/07/owl#ObjectProperty"/>
    <rdfs:domain rdf:resource="https://w3id.org/italia/onto/IoT/Observation"/>
    <rdfs:range rdf:resource="https://w3id.org/italia/onto/IoT/ObservationCollection"/>
    <rdfs:comment xml:lang="en">Inverse property of consistsOf that links an observation to its related collection.</rdfs:comment>
    <rdfs:comment xml:lang="it">Proprietà inversa di consiste di che lega un'osservazione alla sua relativa collezione.</rdfs:comment>
    <rdfs:isDefinedBy rdf:resource="https://w3id.org/italia/onto/IoT"/>
    <rdfs:label xml:lang="en">is part of</rdfs:label>
    <rdfs:label xml:lang="it">è parte di</rdfs:label>
    <owl:versionInfo xml:lang="it">stabile</owl:versionInfo>
    <owl:versionInfo xml:lang="en">stable</owl:versionInfo>
  </rdf:Description>
  <rdf:Description rdf:about="https://w3id.org/italia/onto/IoT/hostsMonitoringFacility">
    <rdf:type rdf:resource="http://www.w3.org/2002/07/owl#ObjectProperty"/>
    <owl:inverseOf rdf:resource="https://w3id.org/italia/onto/IoT/isHostedByPlatform"/>
    <rdfs:domain rdf:resource="https://w3id.org/italia/onto/IoT/Platform"/>
    <rdfs:range rdf:resource="https://w3id.org/italia/onto/IoT/MonitoringFacility"/>
    <rdfs:comment xml:lang="en">Property that links a platform with the monitoring facilities it hosts</rdfs:comment>
    <rdfs:comment xml:lang="it">Proprietà che collega la piattaforma agli strumenti di monitoraggio che ospita</rdfs:comment>
    <rdfs:isDefinedBy rdf:resource="https://w3id.org/italia/onto/IoT"/>
    <rdfs:label xml:lang="en">hosts monitoring facility</rdfs:label>
    <rdfs:label xml:lang="it">ospita strumenti di monitoraggio</rdfs:label>
    <owl:versionInfo xml:lang="it">provvisoria - da validare</owl:versionInfo>
    <owl:versionInfo xml:lang="en">unstable</owl:versionInfo>
  </rdf:Description>
  <rdf:Description rdf:about="https://w3id.org/italia/onto/l0/identifier">
    <rdf:type rdf:resource="http://www.w3.org/2002/07/owl#DatatypeProperty"/>
    <rdfs:isDefinedBy rdf:resource="https://w3id.org/italia/onto/l0/"/>
  </rdf:Description>
  <rdf:Description rdf:nodeID="n690e025d2eb648a3a4574298c2d1991cb5">
    <rdf:type rdf:resource="http://www.w3.org/2002/07/owl#Restriction"/>
    <owl:onProperty rdf:resource="https://w3id.org/italia/onto/IoT/implementsMethod"/>
    <owl:allValuesFrom rdf:resource="https://w3id.org/italia/onto/IoT/Method"/>
  </rdf:Description>
  <rdf:Description rdf:nodeID="n690e025d2eb648a3a4574298c2d1991cb36">
    <rdf:type rdf:resource="http://www.w3.org/2002/07/owl#Restriction"/>
    <owl:onProperty rdf:resource="https://w3id.org/italia/onto/l0/identifier"/>
    <owl:cardinality rdf:datatype="http://www.w3.org/2001/XMLSchema#nonNegativeInteger">1</owl:cardinality>
  </rdf:Description>
  <rdf:Description rdf:about="https://w3id.org/italia/onto/IoT/Offset">
    <rdf:type rdf:resource="http://www.w3.org/2002/07/owl#Class"/>
    <rdfs:subClassOf rdf:resource="https://w3id.org/italia/onto/IoT/MeasurementQuality"/>
    <rdfs:comment xml:lang="en">It represents the offset error; that is, the difference between the actual output value and the specified output value under some particular set of conditions.</rdfs:comment>
    <rdfs:comment xml:lang="it">Questa classe rappresenta l'errore di compensazione, ovvero  la differenza tra il valore reale di uscita e il valore di uscita specificato in alcune particolari condizioni.</rdfs:comment>
    <rdfs:isDefinedBy rdf:resource="https://w3id.org/italia/onto/IoT"/>
    <rdfs:label xml:lang="it">Compensazione</rdfs:label>
    <rdfs:label xml:lang="en">Offset</rdfs:label>
    <owl:versionInfo xml:lang="it">instabile</owl:versionInfo>
    <owl:versionInfo xml:lang="en">unstable</owl:versionInfo>
  </rdf:Description>
  <rdf:Description rdf:nodeID="n690e025d2eb648a3a4574298c2d1991cb14">
    <rdf:type rdf:resource="http://www.w3.org/2002/07/owl#Restriction"/>
    <owl:onProperty rdf:resource="https://w3id.org/italia/onto/CLV/hasGeometry"/>
    <owl:maxQualifiedCardinality rdf:datatype="http://www.w3.org/2001/XMLSchema#nonNegativeInteger">1</owl:maxQualifiedCardinality>
    <owl:onClass rdf:resource="https://w3id.org/italia/onto/CLV/Geometry"/>
  </rdf:Description>
  <rdf:Description rdf:nodeID="n690e025d2eb648a3a4574298c2d1991cb29">
    <rdf:type rdf:resource="http://www.w3.org/2002/07/owl#Restriction"/>
    <owl:onProperty rdf:resource="https://w3id.org/italia/onto/IoT/isObservationParameterFor"/>
    <owl:allValuesFrom rdf:resource="https://w3id.org/italia/onto/IoT/Observation"/>
  </rdf:Description>
  <rdf:Description rdf:about="https://w3id.org/italia/onto/IoT/observationMadeBySensor">
    <rdf:type rdf:resource="http://www.w3.org/2002/07/owl#ObjectProperty"/>
    <rdfs:domain rdf:resource="https://w3id.org/italia/onto/IoT/Observation"/>
    <rdfs:range rdf:resource="https://w3id.org/italia/onto/IoT/Sensor"/>
    <rdfs:comment xml:lang="it">Questa è la proprietù inversa che lega un'osservazione al sensore.</rdfs:comment>
    <rdfs:comment xml:lang="en">This is the inverse property of makesObservation and links an Observation to the Sensor.</rdfs:comment>
    <rdfs:isDefinedBy rdf:resource="https://w3id.org/italia/onto/IoT"/>
    <rdfs:label xml:lang="en">observation made by sensor</rdfs:label>
    <rdfs:label xml:lang="it">osservazione fatta dal sensore</rdfs:label>
    <owl:versionInfo xml:lang="it">stabile</owl:versionInfo>
    <owl:versionInfo xml:lang="en">stable</owl:versionInfo>
  </rdf:Description>
  <rdf:Description rdf:nodeID="n690e025d2eb648a3a4574298c2d1991cb18">
    <rdf:type rdf:resource="http://www.w3.org/2002/07/owl#Restriction"/>
    <owl:onProperty rdf:resource="https://w3id.org/italia/onto/l0/description"/>
    <owl:allValuesFrom rdf:resource="http://www.w3.org/2000/01/rdf-schema#Literal"/>
  </rdf:Description>
  <rdf:Description rdf:about="http://www.w3.org/ns/prov#wasDerivedFrom">
    <rdf:type rdf:resource="http://www.w3.org/2002/07/owl#AnnotationProperty"/>
  </rdf:Description>
  <rdf:Description rdf:nodeID="n690e025d2eb648a3a4574298c2d1991cb26">
    <rdf:first rdf:resource="https://w3id.org/italia/onto/l0/Characteristic"/>
    <rdf:rest rdf:nodeID="n690e025d2eb648a3a4574298c2d1991cb27"/>
  </rdf:Description>
  <rdf:Description rdf:nodeID="n690e025d2eb648a3a4574298c2d1991cb30">
    <rdf:type rdf:resource="http://www.w3.org/2002/07/owl#Restriction"/>
    <owl:onProperty rdf:resource="https://w3id.org/italia/onto/l0/name"/>
    <owl:someValuesFrom rdf:resource="http://www.w3.org/2000/01/rdf-schema#Literal"/>
  </rdf:Description>
  <rdf:Description rdf:nodeID="n690e025d2eb648a3a4574298c2d1991cb25">
    <rdf:type rdf:resource="http://www.w3.org/2002/07/owl#Class"/>
    <owl:unionOf rdf:nodeID="n690e025d2eb648a3a4574298c2d1991cb26"/>
  </rdf:Description>
  <rdf:Description rdf:about="https://w3id.org/italia/onto/IoT/Actuator">
    <rdf:type rdf:resource="http://www.w3.org/2002/07/owl#Class"/>
    <rdfs:subClassOf rdf:resource="https://w3id.org/italia/onto/IoT/MonitoringFacility"/>
    <rdfs:comment xml:lang="en">An actuator.</rdfs:comment>
    <rdfs:comment xml:lang="it">La classe che rappresenta un attuatore.</rdfs:comment>
    <rdfs:label xml:lang="en">Actuator</rdfs:label>
    <rdfs:label xml:lang="it">Attuatore</rdfs:label>
  </rdf:Description>
  <rdf:Description rdf:about="https://w3id.org/italia/onto/l0/Activity">
    <rdf:type rdf:resource="http://www.w3.org/2002/07/owl#Class"/>
  </rdf:Description>
  <rdf:Description rdf:about="https://w3id.org/italia/data/distribution/IOT-JSON-LD">
    <rdf:type rdf:resource="http://www.w3.org/2002/07/owl#NamedIndividual"/>
    <rdf:type rdf:resource="https://w3id.org/italia/onto/ADMS/SemanticAssetDistribution"/>
    <dct:description xml:lang="it">Questa è la distribuzione JSON-LD dell'ontologia degli eventi IoT</dct:description>
    <dct:description xml:lang="en">This is the distribution in JSON-LD of the IoT Events ontology</dct:description>
    <dct:format rdf:resource="http://publications.europa.eu/resource/authority/file-type/JSON_LD"/>
    <dct:license rdf:resource="https://w3id.org/italia/controlled-vocabulary/licences/A21_CCBY40"/>
    <dct:title xml:lang="it">Distribuzione JSON-LD ontologia IoT-AP_IT</dct:title>
    <dct:title xml:lang="en">JSON-LD distribution of IoT-AP_IT Ontology</dct:title>
    <dcat:accessURL rdf:resource="https://raw.githubusercontent.com/italia/daf-ontologie-vocabolari-controllati/master/Ontologie/IoT/latest"/>
    <dcat:downloadURL rdf:resource="https://raw.githubusercontent.com/italia/daf-ontologie-vocabolari-controllati/master/Ontologie/IoT/IoT-AP_IT.jsonld"/>
  </rdf:Description>
  <rdf:Description rdf:nodeID="n690e025d2eb648a3a4574298c2d1991cb3">
    <rdf:type rdf:resource="http://www.w3.org/2002/07/owl#Restriction"/>
    <owl:onProperty rdf:resource="https://w3id.org/italia/onto/IoT/hasMeasurementQualityValue"/>
    <owl:qualifiedCardinality rdf:datatype="http://www.w3.org/2001/XMLSchema#nonNegativeInteger">1</owl:qualifiedCardinality>
    <owl:onClass rdf:resource="https://w3id.org/italia/onto/IoT/MeasurementQualityValue"/>
  </rdf:Description>
  <rdf:Description rdf:about="https://w3id.org/italia/onto/l0/description">
    <rdf:type rdf:resource="http://www.w3.org/2002/07/owl#DatatypeProperty"/>
    <rdfs:isDefinedBy rdf:resource="https://w3id.org/italia/onto/l0/"/>
  </rdf:Description>
  <rdf:Description rdf:about="https://w3id.org/italia/onto/l0/Characteristic">
    <rdf:type rdf:resource="http://www.w3.org/2002/07/owl#Class"/>
  </rdf:Description>
  <rdf:Description rdf:nodeID="n690e025d2eb648a3a4574298c2d1991cb12">
    <rdf:type rdf:resource="http://www.w3.org/2002/07/owl#Restriction"/>
    <owl:onProperty rdf:resource="https://w3id.org/italia/onto/IoT/isPartOf"/>
    <owl:qualifiedCardinality rdf:datatype="http://www.w3.org/2001/XMLSchema#nonNegativeInteger">1</owl:qualifiedCardinality>
    <owl:onClass rdf:resource="https://w3id.org/italia/onto/IoT/ObservationCollection"/>
  </rdf:Description>
  <rdf:Description rdf:nodeID="n690e025d2eb648a3a4574298c2d1991cb33">
    <rdf:type rdf:resource="http://www.w3.org/2002/07/owl#Restriction"/>
    <owl:onProperty rdf:resource="https://w3id.org/italia/onto/IoT/hostsMonitoringFacility"/>
    <owl:allValuesFrom rdf:resource="https://w3id.org/italia/onto/IoT/MonitoringFacility"/>
  </rdf:Description>
  <rdf:Description rdf:nodeID="n690e025d2eb648a3a4574298c2d1991cb19">
    <rdf:type rdf:resource="http://www.w3.org/2002/07/owl#Restriction"/>
    <owl:onProperty rdf:resource="https://w3id.org/italia/onto/l0/identifier"/>
    <owl:cardinality rdf:datatype="http://www.w3.org/2001/XMLSchema#nonNegativeInteger">1</owl:cardinality>
  </rdf:Description>
  <rdf:Description rdf:nodeID="n690e025d2eb648a3a4574298c2d1991cb35">
    <rdf:type rdf:resource="http://www.w3.org/2002/07/owl#Restriction"/>
    <owl:onProperty rdf:resource="https://w3id.org/italia/onto/l0/description"/>
    <owl:allValuesFrom rdf:resource="http://www.w3.org/2000/01/rdf-schema#Literal"/>
  </rdf:Description>
  <rdf:Description rdf:about="https://w3id.org/italia/onto/CLV/hasGeometry">
    <rdf:type rdf:resource="http://www.w3.org/2002/07/owl#ObjectProperty"/>
    <rdfs:isDefinedBy rdf:resource="https://w3id.org/italia/onto/CLV/"/>
  </rdf:Description>
  <rdf:Description rdf:about="https://w3id.org/italia/onto/TI/atTime">
    <rdf:type rdf:resource="http://www.w3.org/2002/07/owl#ObjectProperty"/>
  </rdf:Description>
  <rdf:Description rdf:nodeID="n690e025d2eb648a3a4574298c2d1991cb13">
    <rdf:type rdf:resource="http://www.w3.org/2002/07/owl#Restriction"/>
    <owl:onProperty rdf:resource="https://w3id.org/italia/onto/IoT/observationMadeBySensor"/>
    <owl:qualifiedCardinality rdf:datatype="http://www.w3.org/2001/XMLSchema#nonNegativeInteger">1</owl:qualifiedCardinality>
    <owl:onClass rdf:resource="https://w3id.org/italia/onto/IoT/Sensor"/>
  </rdf:Description>
  <rdf:Description rdf:nodeID="n690e025d2eb648a3a4574298c2d1991cb2">
    <rdf:type rdf:resource="http://www.w3.org/2002/07/owl#Restriction"/>
    <owl:onProperty rdf:resource="https://w3id.org/italia/onto/l0/name"/>
    <owl:someValuesFrom rdf:resource="http://www.w3.org/2000/01/rdf-schema#Literal"/>
  </rdf:Description>
  <rdf:Description rdf:about="http://purl.org/dc/terms/modified">
    <rdf:type rdf:resource="http://www.w3.org/2002/07/owl#AnnotationProperty"/>
  </rdf:Description>
  <rdf:Description rdf:nodeID="n690e025d2eb648a3a4574298c2d1991cb16">
    <rdf:type rdf:resource="http://www.w3.org/2002/07/owl#Restriction"/>
    <owl:onProperty rdf:resource="https://w3id.org/italia/onto/IoT/phenomenonTime"/>
    <owl:maxQualifiedCardinality rdf:datatype="http://www.w3.org/2001/XMLSchema#nonNegativeInteger">1</owl:maxQualifiedCardinality>
    <owl:onClass rdf:resource="https://w3id.org/italia/onto/TI/TimeInterval"/>
  </rdf:Description>
  <rdf:Description rdf:about="https://w3id.org/italia/onto/IoT/MeasurementQualityValue">
    <rdf:type rdf:resource="http://www.w3.org/2002/07/owl#Class"/>
    <rdfs:subClassOf rdf:resource="https://w3id.org/italia/onto/MU/Value"/>
    <rdfs:subClassOf rdf:nodeID="n690e025d2eb648a3a4574298c2d1991cb4"/>
    <rdfs:isDefinedBy rdf:resource="https://w3id.org/italia/onto/IoT"/>
    <rdfs:label xml:lang="en">Measurement Quality Value</rdfs:label>
    <rdfs:label xml:lang="it">Valore Qualità di Misurazione</rdfs:label>
  </rdf:Description>
  <rdf:Description rdf:about="https://w3id.org/italia/onto/l0/name">
    <rdf:type rdf:resource="http://www.w3.org/2002/07/owl#DatatypeProperty"/>
    <rdfs:isDefinedBy rdf:resource="https://w3id.org/italia/onto/l0/"/>
  </rdf:Description>
  <rdf:Description rdf:nodeID="n690e025d2eb648a3a4574298c2d1991cb9">
    <rdf:type rdf:resource="http://www.w3.org/2002/07/owl#Restriction"/>
    <owl:onProperty rdf:resource="https://w3id.org/italia/onto/IoT/hasQuality"/>
    <owl:allValuesFrom rdf:resource="https://w3id.org/italia/onto/IoT/MeasurementQuality"/>
  </rdf:Description>
  <rdf:Description rdf:about="https://w3id.org/italia/onto/TI/issued">
    <rdf:type rdf:resource="http://www.w3.org/2002/07/owl#DatatypeProperty"/>
    <rdfs:isDefinedBy rdf:resource="https://w3id.org/italia/onto/TI/"/>
  </rdf:Description>
  <rdf:Description rdf:about="https://w3id.org/italia/onto/MU/Value">
    <rdf:type rdf:resource="http://www.w3.org/2002/07/owl#Class"/>
  </rdf:Description>
  <rdf:Description rdf:about="https://w3id.org/italia/onto/TI/TimeInterval">
    <rdf:type rdf:resource="http://www.w3.org/2002/07/owl#Class"/>
  </rdf:Description>
  <rdf:Description rdf:about="https://w3id.org/italia/onto/l0/Object">
    <rdf:type rdf:resource="http://www.w3.org/2002/07/owl#Class"/>
  </rdf:Description>
</rdf:RDF>
