<?xml version="1.0" encoding="UTF-8"?>
<rdf:RDF
   xmlns:admsapit="https://w3id.org/italia/onto/ADMS/"
   xmlns:dc="http://purl.org/dc/elements/1.1/"
   xmlns:dcat="http://www.w3.org/ns/dcat#"
   xmlns:dct="http://purl.org/dc/terms/"
   xmlns:foaf="http://xmlns.com/foaf/0.1/"
   xmlns:l0="https://w3id.org/italia/onto/l0/"
   xmlns:owl="http://www.w3.org/2002/07/owl#"
   xmlns:prov="http://www.w3.org/ns/prov#"
   xmlns:rdf="http://www.w3.org/1999/02/22-rdf-syntax-ns#"
   xmlns:rdfs="http://www.w3.org/2000/01/rdf-schema#"
   xmlns:vcard="http://www.w3.org/2006/vcard/ns#"
>
  <rdf:Description rdf:about="https://w3id.org/italia/onto/POT">
    <rdf:type rdf:resource="http://www.w3.org/2002/07/owl#Ontology"/>
    <rdf:type rdf:resource="http://www.w3.org/2002/07/owl#NamedIndividual"/>
    <rdf:type rdf:resource="https://w3id.org/italia/onto/ADMS/SemanticAsset"/>
    <owl:imports rdf:resource="https://w3id.org/italia/onto/MU"/>
    <owl:imports rdf:resource="https://w3id.org/italia/onto/TI"/>
    <owl:imports rdf:resource="https://w3id.org/italia/onto/l0"/>
    <owl:versionIRI rdf:resource="https://w3id.org/italia/onto/POT/0.3"/>
    <prov:wasDerivedFrom rdf:resource="http://dati.gov.it/onto/potapit/0.2"/>
    <admsapit:prefix>potapit</admsapit:prefix>
    <dct:creator rdf:resource="http://spcdata.digitpa.gov.it/Amministrazione/agid"/>
    <dct:creator rdf:resource="https://w3id.org/italia/data/organization/support-unit/cnr-Z6HZEH/stlab"/>
    <admsapit:target xml:lang="it">Cittadini</admsapit:target>
    <admsapit:target xml:lang="it">Pubbliche Amministrazioni</admsapit:target>
    <admsapit:target xml:lang="it">Imprese</admsapit:target>
    <dct:modified rdf:datatype="http://www.w3.org/2001/XMLSchema#date">2019-04-24</dct:modified>
    <admsapit:hasTask rdf:resource="https://w3id.org/italia/onto/ADMS/AnnotationTask"/>
    <admsapit:hasTask rdf:resource="https://w3id.org/italia/onto/ADMS/QueryFormulationTask"/>
    <admsapit:hasTask rdf:resource="https://w3id.org/italia/onto/ADMS/SearchTask"/>
    <admsapit:hasSemanticAssetDistribution rdf:resource="https://w3id.org/italia/data/distribution/POT-RDF-TURTLE"/>
    <admsapit:hasSemanticAssetDistribution rdf:resource="https://w3id.org/italia/data/distribution/POT-RDF-XML"/>
    <admsapit:hasSemanticAssetDistribution rdf:resource="https://w3id.org/italia/data/distribution/POT-JSON-LD"/>
    <rdfs:comment xml:lang="en">This is the ontology used to represent price , tickets and offers</rdfs:comment>
    <rdfs:comment xml:lang="it">Questa è l'ontologia del profilo applicativo italiano dei prezzi, offerte e biglietti</rdfs:comment>
    <admsapit:hasOntologyLanguage rdf:resource="https://w3id.org/italia/onto/ADMS/OWL"/>
    <admsapit:officialURI rdf:datatype="http://www.w3.org/2001/XMLSchema#anyURI">https://w3id.org/italia/onto/POT</admsapit:officialURI>
    <dcat:keyword xml:lang="it">prezzi</dcat:keyword>
    <dcat:keyword xml:lang="it">biglietto</dcat:keyword>
    <dcat:keyword xml:lang="it">offerta</dcat:keyword>
    <dct:language rdf:resource="http://publications.europa.eu/resource/authority/language/ENG"/>
    <dct:language rdf:resource="http://publications.europa.eu/resource/authority/language/ITA"/>
    <admsapit:hasFormalityLevel rdf:resource="https://w3id.org/italia/onto/ADMS/Formal"/>
    <admsapit:last rdf:resource="https://w3id.org/italia/onto/POT/0.3"/>
    <dct:title xml:lang="it">Ontologia dei Prezzi, Offerte e Biglietti - Profilo applicativo italiano</dct:title>
    <dct:title xml:lang="en">Price/Offer/Ticket ontology - Italian application profile</dct:title>
    <admsapit:hasKeyClass rdf:resource="https://w3id.org/italia/onto/POT/Ticket"/>
    <admsapit:hasKeyClass rdf:resource="https://w3id.org/italia/onto/POT/PriceSpecification"/>
    <admsapit:hasKeyClass rdf:resource="https://w3id.org/italia/onto/POT/Offer"/>
    <rdfs:isDefinedBy rdf:resource="https://w3id.org/italia/onto/POT"/>
    <dct:publisher rdf:resource="http://spcdata.digitpa.gov.it/Amministrazione/agid"/>
    <dct:rightsHolder rdf:resource="http://spcdata.digitpa.gov.it/Amministrazione/agid"/>
    <dct:description xml:lang="it">Questo il profilo applicativo italiano dell'ontologia dei prezzi, offerte e biglietti. L'ontologia può essere usata per rappresentare i dati relativi ai prezzi di un prodotto, le offerte e i biglietti, necessari per partecipare a eventi o aver accesso a determinati luoghi pubblici.</dct:description>
    <dct:description xml:lang="en">This is the Italian application profile of the price, offers and ticket ontologies.</dct:description>
    <owl:versionInfo xml:lang="it">Versione 0.3 - Modificata il 24 Aprile 2019 - Rifattorizzazione l0:Event in l0:EventOrSituation: Uso di w3id.org/italia/onto/POT come URI base</owl:versionInfo>
    <owl:versionInfo xml:lang="en">Version 0.3 - Modified on 24 April 2018 - Refactoring of l0:Event in l0:EventOrSituation; Use of w3id.org/italia/onto/POT/ as base URI</owl:versionInfo>
    <dcat:contactPoint rdf:resource="https://w3id.org/italia/data/contact-point/onto-agid"/>
    <admsapit:semanticAssetInUse rdf:resource="https://w3id.org/italia/data/project/DAF"/>
    <admsapit:semanticAssetInUse rdf:resource="https://w3id.org/italia/data/project/OntoPiA"/>
    <dct:accrualPeriodicity rdf:resource="http://publications.europa.eu/resource/authority/frequency/IRREG"/>
    <rdfs:label xml:lang="it">Ontologia dei prezzi, offerte e biglietti</rdfs:label>
    <rdfs:label xml:lang="en">Italian Price/Offer/Ticket ontology</rdfs:label>
    <dcat:theme rdf:resource="http://publications.europa.eu/resource/authority/data-theme/EDUC"/>
    <dcat:theme rdf:resource="http://publications.europa.eu/resource/authority/data-theme/SOCI"/>
    <dcat:theme rdf:resource="http://publications.europa.eu/resource/authority/data-theme/TRAN"/>
    <admsapit:acronym>POT-AP_IT</admsapit:acronym>
    <dct:issued rdf:datatype="http://www.w3.org/2001/XMLSchema#date">2017-11-17</dct:issued>
    <admsapit:hasContributor rdf:resource="https://w3id.org/italia/data/organization/public-organization/td"/>
    <admsapit:status>published</admsapit:status>
    <admsapit:status>catalogued</admsapit:status>
    <admsapit:type rdf:resource="https://w3id.org/italia/onto/ADMS/ServiceOntology"/>
  </rdf:Description>
  <rdf:Description rdf:about="https://w3id.org/italia/data/organization/public-organization/td">
    <rdf:type rdf:resource="http://www.w3.org/2002/07/owl#NamedIndividual"/>
    <rdf:type rdf:resource="http://dati.gov.it/onto/dcatapit#Agent"/>
    <rdf:type rdf:resource="http://xmlns.com/foaf/0.1/Agent"/>
    <dct:identifier>TD</dct:identifier>
    <foaf:name xml:lang="en">Digital Transformation Team</foaf:name>
    <foaf:name xml:lang="it">Team per la Trasformazione Digitale</foaf:name>
  </rdf:Description>
  <rdf:Description rdf:about="https://w3id.org/italia/onto/POT/UserType">
    <rdf:type rdf:resource="http://www.w3.org/2002/07/owl#Class"/>
    <rdfs:label xml:lang="en">User Type</rdfs:label>
    <rdfs:label xml:lang="it">Tipo di utente</rdfs:label>
    <rdfs:subClassOf rdf:resource="https://w3id.org/italia/onto/l0/Characteristic"/>
    <rdfs:subClassOf rdf:nodeID="n2282281da4664851aa816bdc565aff50b17"/>
    <rdfs:subClassOf rdf:nodeID="n2282281da4664851aa816bdc565aff50b18"/>
    <rdfs:comment xml:lang="en">It represents the identified type of users related to the tickets used to access an event or location. Examples include: people over 25 years old, people over 65 years old,  children, etc.</rdfs:comment>
    <rdfs:comment xml:lang="it">Rappresenta la tipologia di utenti relativa ai biglietti per accedere a un evento o a un luogo. Esempi includono:  "maggiorenni over 25", oppure "over 65", "bambini", ecc.</rdfs:comment>
    <owl:versionInfo xml:lang="en">stable</owl:versionInfo>
    <owl:versionInfo xml:lang="it">stabile</owl:versionInfo>
    <rdfs:isDefinedBy rdf:resource="https://w3id.org/italia/onto/POT"/>
  </rdf:Description>
  <rdf:Description rdf:nodeID="n2282281da4664851aa816bdc565aff50b18">
    <rdf:type rdf:resource="http://www.w3.org/2002/07/owl#Restriction"/>
    <owl:onProperty rdf:resource="https://w3id.org/italia/onto/l0/name"/>
    <owl:allValuesFrom rdf:resource="http://www.w3.org/2000/01/rdf-schema#Literal"/>
  </rdf:Description>
  <rdf:Description rdf:about="https://w3id.org/italia/onto/POT/hasCurrency">
    <rdf:type rdf:resource="http://www.w3.org/2002/07/owl#ObjectProperty"/>
    <rdfs:label xml:lang="en">has currency</rdfs:label>
    <rdfs:label xml:lang="it">ha valuta</rdfs:label>
    <rdfs:comment xml:lang="en">This property is used to connected the Price specification to Currency</rdfs:comment>
    <rdfs:comment xml:lang="it">Questa proprietà collega la specifica del prezzo con la classe currency.</rdfs:comment>
    <owl:versionInfo xml:lang="en">stable</owl:versionInfo>
    <owl:versionInfo xml:lang="it">stabile</owl:versionInfo>
    <rdfs:isDefinedBy rdf:resource="https://w3id.org/italia/onto/POT"/>
    <rdfs:range rdf:resource="https://w3id.org/italia/onto/POT/Currency"/>
    <rdfs:domain rdf:resource="https://w3id.org/italia/onto/POT/PriceSpecification"/>
  </rdf:Description>
  <rdf:Description rdf:about="http://spcdata.digitpa.gov.it/Amministrazione/agid">
    <rdf:type rdf:resource="http://www.w3.org/2002/07/owl#NamedIndividual"/>
    <rdf:type rdf:resource="http://dati.gov.it/onto/dcatapit#Agent"/>
    <rdf:type rdf:resource="http://xmlns.com/foaf/0.1/Agent"/>
    <dct:identifier>agid</dct:identifier>
    <foaf:name xml:lang="it">Agenzia per l'Italia Digitale</foaf:name>
    <foaf:name xml:lang="en">Italian Digital Agency</foaf:name>
  </rdf:Description>
  <rdf:Description rdf:about="https://w3id.org/italia/onto/POT/hasEligibleUser">
    <rdf:type rdf:resource="http://www.w3.org/2002/07/owl#ObjectProperty"/>
    <rdfs:label xml:lang="en">has eligible user</rdfs:label>
    <rdfs:label xml:lang="it">ha utente idoneo</rdfs:label>
    <rdfs:comment xml:lang="en">Property used to associate an offert for the access to an event or a locations with the type of user</rdfs:comment>
    <rdfs:comment xml:lang="it">Proprietà che consente di associare un'offerta per l'accesso a un evento o un luogo ad una tipologia di utente</rdfs:comment>
    <owl:versionInfo xml:lang="en">stable</owl:versionInfo>
    <owl:versionInfo xml:lang="it">stabile</owl:versionInfo>
    <rdfs:isDefinedBy rdf:resource="https://w3id.org/italia/onto/POT"/>
    <rdfs:domain rdf:resource="https://w3id.org/italia/onto/POT/Offer"/>
    <rdfs:range rdf:resource="https://w3id.org/italia/onto/POT/UserType"/>
  </rdf:Description>
  <rdf:Description rdf:about="https://w3id.org/italia/onto/POT/offers">
    <rdf:type rdf:resource="http://www.w3.org/2002/07/owl#ObjectProperty"/>
    <rdfs:label xml:lang="en">offers</rdfs:label>
    <rdfs:label xml:lang="it">offre</rdfs:label>
    <rdfs:comment xml:lang="en">Property used to associate an agent with an offer for accessing an event or a cultural institute or site</rdfs:comment>
    <rdfs:comment xml:lang="it">Proprietà che consente di associare un agente all'offerta per l'accesso a un evento o a un luogo della cultura.</rdfs:comment>
    <rdfs:isDefinedBy rdf:resource="https://w3id.org/italia/onto/POT"/>
    <rdfs:range rdf:resource="https://w3id.org/italia/onto/POT/Offer"/>
    <rdfs:domain rdf:resource="https://w3id.org/italia/onto/l0/Agent"/>
  </rdf:Description>
  <rdf:Description rdf:about="https://w3id.org/italia/onto/POT/Offer">
    <rdf:type rdf:resource="http://www.w3.org/2002/07/owl#Class"/>
    <rdfs:label xml:lang="en">Offer</rdfs:label>
    <rdfs:label xml:lang="it">Offerta</rdfs:label>
    <rdfs:subClassOf rdf:resource="https://w3id.org/italia/onto/l0/Description"/>
    <rdfs:subClassOf rdf:nodeID="n2282281da4664851aa816bdc565aff50b8"/>
    <rdfs:subClassOf rdf:nodeID="n2282281da4664851aa816bdc565aff50b9"/>
    <rdfs:subClassOf rdf:nodeID="n2282281da4664851aa816bdc565aff50b10"/>
    <rdfs:subClassOf rdf:nodeID="n2282281da4664851aa816bdc565aff50b11"/>
    <dc:description xml:lang="en">Any fare is expressed within the ontology by using instances of the class Offer.

It is possible to specify:
 * the type of user to whom the offer is applicable  (cf. object property cis:hasEligibleUser);
 * the information about the price (cf. object property hasPriceSpecification);
 * the information about the temporal validity of the offer (cf. object property hasValidity);
 * the association with a ticket (cf. object property includes).</dc:description>
    <rdfs:comment xml:lang="en">It represents an offer (reduction  for specific types of users or base price).</rdfs:comment>
    <rdfs:comment xml:lang="it">Concetto utilizzato per rappresentare  offerte (riduzioni per specifiche categorie di utenti o importo intero).</rdfs:comment>
    <owl:versionInfo xml:lang="en">stable</owl:versionInfo>
    <owl:versionInfo xml:lang="it">stabile</owl:versionInfo>
    <prov:wasDerivedFrom rdf:resource="http://purl.org/goodrelations/v1#Offering"/>
    <prov:wasDerivedFrom rdf:resource="http://schema.org/Offer"/>
    <rdfs:isDefinedBy rdf:resource="https://w3id.org/italia/onto/POT"/>
  </rdf:Description>
  <rdf:Description rdf:about="https://w3id.org/italia/onto/POT/PriceSpecification">
    <rdf:type rdf:resource="http://www.w3.org/2002/07/owl#Class"/>
    <rdfs:label xml:lang="en">Price Specification</rdfs:label>
    <rdfs:label xml:lang="it">Prezzo</rdfs:label>
    <rdfs:subClassOf rdf:resource="https://w3id.org/italia/onto/l0/Characteristic"/>
    <rdfs:subClassOf rdf:nodeID="n2282281da4664851aa816bdc565aff50b12"/>
    <rdfs:subClassOf rdf:nodeID="n2282281da4664851aa816bdc565aff50b13"/>
    <rdfs:subClassOf rdf:nodeID="n2282281da4664851aa816bdc565aff50b14"/>
    <dc:description xml:lang="en">A price specification provides the information about the cost of an offer.

It is associated to a currency (e.g., Euro) and a currency value (i.e., a quantity, e.g., 5).</dc:description>
    <dc:description rdf:resource="http://dati.beniculturali.it/cis/img/priceSpecification.png"/>
    <rdfs:comment xml:lang="en">It represents the price specification of the ticket</rdfs:comment>
    <rdfs:comment xml:lang="it">Rappresenta la specifica del prezzo del biglietto.</rdfs:comment>
    <owl:versionInfo xml:lang="en">stable</owl:versionInfo>
    <owl:versionInfo xml:lang="it">stabile</owl:versionInfo>
    <prov:wasDerivedFrom rdf:resource="http://purl.org/goodrelations/v1#PriceSpecification"/>
    <prov:wasDerivedFrom rdf:resource="http://schema.org/PriceSpecification"/>
    <rdfs:isDefinedBy rdf:resource="https://w3id.org/italia/onto/POT"/>
  </rdf:Description>
  <rdf:Description rdf:about="https://w3id.org/italia/data/distribution/POT-RDF-TURTLE">
    <rdf:type rdf:resource="http://www.w3.org/2002/07/owl#NamedIndividual"/>
    <rdf:type rdf:resource="https://w3id.org/italia/onto/ADMS/SemanticAssetDistribution"/>
    <dct:description xml:lang="it">Questa è la distribuzione RDF/Turtle dell'ontologia dei prezzi, offerte e biglietti</dct:description>
    <dct:description xml:lang="en">This is the distribution in RDF/turtle of the Price/Offer/Ticket ontology</dct:description>
    <dct:format rdf:resource="http://publications.europa.eu/resource/authority/file-type/RDF_TURTLE"/>
    <dct:license rdf:resource="https://w3id.org/italia/controlled-vocabulary/licences/A21_CCBY40"/>
    <dct:title xml:lang="it">Distribuzione RDF/Turtle ontologia POT-AP_IT</dct:title>
    <dct:title xml:lang="en">RDF/Turtle distribution of POT-AP_IT Ontology</dct:title>
    <dcat:accessURL rdf:resource="https://raw.githubusercontent.com/italia/daf-ontologie-vocabolari-controllati/master/Ontologie/POT/latest"/>
    <dcat:downloadURL rdf:resource="https://raw.githubusercontent.com/italia/daf-ontologie-vocabolari-controllati/master/Ontologie/POT/latest/POT-AP_IT.ttl"/>
  </rdf:Description>
  <rdf:Description rdf:about="https://w3id.org/italia/onto/POT/hasCurrencyValue">
    <rdf:type rdf:resource="http://www.w3.org/2002/07/owl#DatatypeProperty"/>
    <rdfs:label xml:lang="en">currency value</rdfs:label>
    <rdfs:label xml:lang="it">prezzo</rdfs:label>
    <rdfs:comment xml:lang="en">Property used to represent the price associated to a specific ticket or a general offer</rdfs:comment>
    <rdfs:comment xml:lang="it">Proprietà utilizzata per indicare il prezzo di un biglietto o di una generica offerta</rdfs:comment>
    <owl:versionInfo xml:lang="en">stable</owl:versionInfo>
    <owl:versionInfo xml:lang="it">stabile</owl:versionInfo>
    <rdfs:range rdf:resource="http://www.w3.org/2001/XMLSchema#double"/>
    <rdfs:isDefinedBy rdf:resource="https://w3id.org/italia/onto/POT"/>
    <rdfs:domain rdf:resource="https://w3id.org/italia/onto/POT/PriceSpecification"/>
  </rdf:Description>
  <rdf:Description rdf:nodeID="n2282281da4664851aa816bdc565aff50b15">
    <rdf:type rdf:resource="http://www.w3.org/2002/07/owl#Restriction"/>
    <owl:onProperty rdf:resource="https://w3id.org/italia/onto/POT/hasValidity"/>
    <owl:allValuesFrom rdf:resource="https://w3id.org/italia/onto/POT/Validity"/>
  </rdf:Description>
  <rdf:Description rdf:about="https://w3id.org/italia/data/contact-point/onto-agid">
    <rdf:type rdf:resource="http://www.w3.org/2002/07/owl#NamedIndividual"/>
    <rdf:type rdf:resource="http://dati.gov.it/onto/dcatapit#Organization"/>
    <rdf:type rdf:resource="http://www.w3.org/2006/vcard/ns#Kind"/>
    <rdf:type rdf:resource="http://www.w3.org/2006/vcard/ns#Organization"/>
    <vcard:fn>banche dati e open data</vcard:fn>
    <vcard:hasEmail rdf:resource="mailto:info@dati.gov.it"/>
  </rdf:Description>
  <rdf:Description rdf:about="https://w3id.org/italia/onto/POT/VAT">
    <rdf:type rdf:resource="http://www.w3.org/2002/07/owl#DatatypeProperty"/>
    <rdfs:label xml:lang="en">VAT</rdfs:label>
    <rdfs:label xml:lang="it">IVA</rdfs:label>
    <rdfs:comment xml:lang="en">This property represents the VAT applied to a price specification.</rdfs:comment>
    <rdfs:comment xml:lang="it">Questa proprietà rappresenta l'iva applicata alla specifica del prezzo.</rdfs:comment>
    <owl:versionInfo xml:lang="en">unstable</owl:versionInfo>
    <owl:versionInfo xml:lang="it">provvisoria</owl:versionInfo>
    <rdfs:range rdf:resource="http://www.w3.org/2000/01/rdf-schema#Literal"/>
    <rdfs:domain rdf:resource="https://w3id.org/italia/onto/POT/PriceSpecification"/>
  </rdf:Description>
  <rdf:Description rdf:about="https://w3id.org/italia/onto/POT/forAccessTo">
    <rdf:type rdf:resource="http://www.w3.org/2002/07/owl#ObjectProperty"/>
    <rdfs:label xml:lang="it">per l'accesso a</rdfs:label>
    <rdfs:label xml:lang="en">for access to</rdfs:label>
    <rdfs:comment xml:lang="en">Property used to associate a ticket to an event or location</rdfs:comment>
    <rdfs:comment xml:lang="it">Proprietà che consente di associare un biglietto a un evento o a un luogo</rdfs:comment>
    <owl:versionInfo xml:lang="en">stable</owl:versionInfo>
    <owl:versionInfo xml:lang="it">stabile</owl:versionInfo>
    <rdfs:isDefinedBy rdf:resource="https://w3id.org/italia/onto/POT"/>
    <rdfs:domain rdf:resource="https://w3id.org/italia/onto/POT/Ticket"/>
    <owl:inverseOf rdf:resource="https://w3id.org/italia/onto/POT/hasTicket"/>
    <rdfs:range rdf:nodeID="n2282281da4664851aa816bdc565aff50b1"/>
  </rdf:Description>
  <rdf:Description rdf:about="https://w3id.org/italia/onto/POT/Currency">
    <rdf:type rdf:resource="http://www.w3.org/2002/07/owl#Class"/>
    <rdfs:label xml:lang="en">Currency</rdfs:label>
    <rdfs:label xml:lang="it">Valuta</rdfs:label>
    <rdfs:subClassOf rdf:resource="https://w3id.org/italia/onto/l0/Object"/>
    <rdfs:subClassOf rdf:nodeID="n2282281da4664851aa816bdc565aff50b7"/>
    <dc:description xml:lang="en">Individuals of the this class represent currency instances (e.g., Euro, US Dollar, Pound, Australian Dollar, etc.); they are always associated with individuals of the class 'Price Specification'.

This allows modelling Price Specification as a a quantified value, where the value is expressed as an integer and it is quantified in terms of a currency</dc:description>
    <rdfs:comment xml:lang="en">This class represents a currency. In our domain currency is typically associated with Price Specification for tickets, and assumes specific values (e.g., Euro).</rdfs:comment>
    <rdfs:comment xml:lang="it">Questa classe rappresenta la valuta per i biglietti di ingresso agli eventi o luoghi della cultura. Nel nostro dominio è associata alla descrizione del prezzo per i biglietti. Assume valori specifici (e.g., Euro).</rdfs:comment>
    <owl:versionInfo xml:lang="en">stable</owl:versionInfo>
    <owl:versionInfo xml:lang="it">stabile</owl:versionInfo>
    <rdfs:isDefinedBy rdf:resource="https://w3id.org/italia/onto/POT"/>
  </rdf:Description>
  <rdf:Description rdf:about="https://w3id.org/italia/onto/POT/hasOffer">
    <rdf:type rdf:resource="http://www.w3.org/2002/07/owl#ObjectProperty"/>
    <rdfs:label xml:lang="en">has offer</rdfs:label>
    <rdfs:label xml:lang="it">ha offerta</rdfs:label>
    <rdfs:comment xml:lang="en">This property links anything to an offer</rdfs:comment>
    <rdfs:comment xml:lang="it">Questa proprietà collega un qualsiasi cosa a un'offerta</rdfs:comment>
    <owl:versionInfo xml:lang="en">stable</owl:versionInfo>
    <owl:versionInfo xml:lang="it">stabile</owl:versionInfo>
    <rdfs:domain rdf:resource="http://www.w3.org/2002/07/owl#Thing"/>
    <rdfs:isDefinedBy rdf:resource="https://w3id.org/italia/onto/POT"/>
    <rdfs:range rdf:resource="https://w3id.org/italia/onto/POT/Offer"/>
  </rdf:Description>
  <rdf:Description rdf:about="https://w3id.org/italia/onto/POT/Card">
    <rdf:type rdf:resource="http://www.w3.org/2002/07/owl#Class"/>
    <rdfs:label xml:lang="en">Card</rdfs:label>
    <rdfs:label xml:lang="it">Carta d'ingresso</rdfs:label>
    <rdfs:label xml:lang="it">Tessera d'ingresso</rdfs:label>
    <rdfs:subClassOf rdf:resource="https://w3id.org/italia/onto/POT/Ticket"/>
    <rdfs:comment xml:lang="en">This class represents a card.</rdfs:comment>
    <rdfs:comment xml:lang="it">Questa classe rappresenta una carta d'ingresso.</rdfs:comment>
    <owl:versionInfo xml:lang="en">stable</owl:versionInfo>
    <owl:versionInfo xml:lang="it">stabile</owl:versionInfo>
    <rdfs:isDefinedBy rdf:resource="https://w3id.org/italia/onto/POT"/>
  </rdf:Description>
  <rdf:Description rdf:nodeID="n2282281da4664851aa816bdc565aff50b20">
    <rdf:type rdf:resource="http://www.w3.org/2002/07/owl#Restriction"/>
    <owl:onProperty rdf:resource="https://w3id.org/italia/onto/TI/hasDuration"/>
    <owl:allValuesFrom rdf:nodeID="n2282281da4664851aa816bdc565aff50b21"/>
  </rdf:Description>
  <rdf:Description rdf:about="https://w3id.org/italia/onto/POT/Ticket">
    <rdf:type rdf:resource="http://www.w3.org/2002/07/owl#Class"/>
    <rdfs:label xml:lang="en">Ticket</rdfs:label>
    <rdfs:label xml:lang="it">Biglietto</rdfs:label>
    <rdfs:subClassOf rdf:resource="https://w3id.org/italia/onto/l0/Object"/>
    <rdfs:subClassOf rdf:nodeID="n2282281da4664851aa816bdc565aff50b15"/>
    <rdfs:subClassOf rdf:nodeID="n2282281da4664851aa816bdc565aff50b16"/>
    <rdfs:comment xml:lang="en">It represents an entrance ticket for a Cultural Institute or Site, if required, and for an event</rdfs:comment>
    <rdfs:comment xml:lang="it">Rappresenta il biglietto d'ingresso per l'Istitituto e Luogo della Cultura, qualora sia previsto, e per l'evento culturale.</rdfs:comment>
    <owl:versionInfo xml:lang="en">stable</owl:versionInfo>
    <owl:versionInfo xml:lang="it">stabile</owl:versionInfo>
    <rdfs:isDefinedBy rdf:resource="https://w3id.org/italia/onto/POT"/>
  </rdf:Description>
  <rdf:Description rdf:about="https://w3id.org/italia/data/project/OntoPiA">
    <rdf:type rdf:resource="http://www.w3.org/2002/07/owl#NamedIndividual"/>
    <rdf:type rdf:resource="https://w3id.org/italia/onto/ADMS/Project"/>
    <l0:name xml:lang="it">OntoPiA - la rete di ontologie della pubblica amministrazione italiana</l0:name>
  </rdf:Description>
  <rdf:Description rdf:about="https://w3id.org/italia/data/distribution/POT-RDF-XML">
    <rdf:type rdf:resource="http://www.w3.org/2002/07/owl#NamedIndividual"/>
    <rdf:type rdf:resource="https://w3id.org/italia/onto/ADMS/SemanticAssetDistribution"/>
    <dct:description xml:lang="it">Questa è la distribuzione RDF/XML dell'ontologia dei prezzi, offerte e biglietti</dct:description>
    <dct:description xml:lang="en">This is the distribution in RDF/XML of the Price/Offer/Ticket ontology</dct:description>
    <dct:format rdf:resource="http://publications.europa.eu/resource/authority/file-type/RDF_XML"/>
    <dct:license rdf:resource="https://w3id.org/italia/controlled-vocabulary/licences/A21_CCBY40"/>
    <dct:title xml:lang="it">Distribuzione RDF/XML ontologia POT-AP_IT</dct:title>
    <dct:title xml:lang="en">RDF/XML distribution of POT-AP_IT Ontology</dct:title>
    <dcat:accessURL rdf:resource="https://raw.githubusercontent.com/italia/daf-ontologie-vocabolari-controllati/master/Ontologie/POT/latest"/>
    <dcat:downloadURL rdf:resource="https://raw.githubusercontent.com/italia/daf-ontologie-vocabolari-controllati/master/Ontologie/POT/latest/POT-AP_IT.rdf"/>
  </rdf:Description>
  <rdf:Description rdf:nodeID="n2282281da4664851aa816bdc565aff50b13">
    <rdf:type rdf:resource="http://www.w3.org/2002/07/owl#Restriction"/>
    <owl:onProperty rdf:resource="https://w3id.org/italia/onto/POT/VAT"/>
    <owl:maxCardinality rdf:datatype="http://www.w3.org/2001/XMLSchema#nonNegativeInteger">1</owl:maxCardinality>
  </rdf:Description>
  <rdf:Description rdf:nodeID="n2282281da4664851aa816bdc565aff50b2">
    <rdf:first rdf:resource="https://w3id.org/italia/onto/l0/EventOrSituation"/>
    <rdf:rest rdf:nodeID="n2282281da4664851aa816bdc565aff50b3"/>
  </rdf:Description>
  <rdf:Description rdf:nodeID="n2282281da4664851aa816bdc565aff50b12">
    <rdf:type rdf:resource="http://www.w3.org/2002/07/owl#Restriction"/>
    <owl:onProperty rdf:resource="https://w3id.org/italia/onto/POT/hasCurrency"/>
    <owl:someValuesFrom rdf:resource="https://w3id.org/italia/onto/POT/Currency"/>
  </rdf:Description>
  <rdf:Description rdf:about="https://w3id.org/italia/onto/POT/hasPriceSpecification">
    <rdf:type rdf:resource="http://www.w3.org/2002/07/owl#ObjectProperty"/>
    <rdfs:label xml:lang="en">has price specification</rdfs:label>
    <rdfs:label xml:lang="it">ha specifica di prezzo</rdfs:label>
    <rdfs:label xml:lang="it">ha prezzo</rdfs:label>
    <rdfs:label xml:lang="it">ha costo</rdfs:label>
    <rdfs:comment xml:lang="en">This property is used to link an offer to its price specification.</rdfs:comment>
    <rdfs:comment xml:lang="it">Questa proprietà è utliizzata per collegare un offerta a una specifica del prezzo.</rdfs:comment>
    <owl:versionInfo xml:lang="en">stable</owl:versionInfo>
    <owl:versionInfo xml:lang="it">stabile</owl:versionInfo>
    <rdfs:isDefinedBy rdf:resource="https://w3id.org/italia/onto/POT"/>
    <rdfs:domain rdf:resource="https://w3id.org/italia/onto/POT/Offer"/>
    <rdfs:range rdf:resource="https://w3id.org/italia/onto/POT/PriceSpecification"/>
  </rdf:Description>
  <rdf:Description rdf:nodeID="n2282281da4664851aa816bdc565aff50b16">
    <rdf:type rdf:resource="http://www.w3.org/2002/07/owl#Restriction"/>
    <owl:onProperty rdf:resource="https://w3id.org/italia/onto/l0/description"/>
    <owl:allValuesFrom rdf:resource="http://www.w3.org/2000/01/rdf-schema#Literal"/>
  </rdf:Description>
  <rdf:Description rdf:about="https://w3id.org/italia/onto/POT/hasTicket">
    <rdf:type rdf:resource="http://www.w3.org/2002/07/owl#ObjectProperty"/>
    <rdfs:label xml:lang="en">has ticket</rdfs:label>
    <rdfs:label xml:lang="it">ha biglietto</rdfs:label>
    <rdfs:comment xml:lang="en">Property that associates a thing with a ticket.</rdfs:comment>
    <rdfs:comment xml:lang="it">Proprietà che associa una cosa ad un biglietto.</rdfs:comment>
    <rdfs:domain rdf:resource="http://www.w3.org/2002/07/owl#Thing"/>
    <rdfs:isDefinedBy rdf:resource="https://w3id.org/italia/onto/POT"/>
    <rdfs:range rdf:resource="https://w3id.org/italia/onto/POT/Ticket"/>
  </rdf:Description>
  <rdf:Description rdf:about="https://w3id.org/italia/data/project/DAF">
    <rdf:type rdf:resource="http://www.w3.org/2002/07/owl#NamedIndividual"/>
    <rdf:type rdf:resource="https://w3id.org/italia/onto/ADMS/Project"/>
    <foaf:name xml:lang="it">Data &amp; Analytics Framework</foaf:name>
  </rdf:Description>
  <rdf:Description rdf:nodeID="n2282281da4664851aa816bdc565aff50b8">
    <rdf:type rdf:resource="http://www.w3.org/2002/07/owl#Restriction"/>
    <owl:onProperty rdf:resource="https://w3id.org/italia/onto/l0/description"/>
    <owl:allValuesFrom rdf:resource="http://www.w3.org/2000/01/rdf-schema#Literal"/>
  </rdf:Description>
  <rdf:Description rdf:about="https://w3id.org/italia/onto/POT/hasValidity">
    <rdf:type rdf:resource="http://www.w3.org/2002/07/owl#ObjectProperty"/>
    <rdfs:label xml:lang="en">has validity</rdfs:label>
    <rdfs:label xml:lang="it">ha validità</rdfs:label>
    <rdfs:comment xml:lang="en">Property used to specify the validity of an offer or ticket.</rdfs:comment>
    <rdfs:comment xml:lang="it">Proprietà utilizzata per specificare una validità di un offerta o di un biglietto.</rdfs:comment>
    <owl:versionInfo xml:lang="it">stabile</owl:versionInfo>
    <owl:versionInfo xml:lang="it">stable</owl:versionInfo>
    <rdfs:isDefinedBy rdf:resource="https://w3id.org/italia/onto/POT"/>
    <rdfs:range rdf:resource="https://w3id.org/italia/onto/POT/Validity"/>
    <rdfs:domain rdf:nodeID="n2282281da4664851aa816bdc565aff50b4"/>
  </rdf:Description>
  <rdf:Description rdf:about="http://purl.org/dc/terms/license">
    <rdf:type rdf:resource="http://www.w3.org/2002/07/owl#AnnotationProperty"/>
  </rdf:Description>
  <rdf:Description rdf:about="https://w3id.org/italia/data/distribution/POT-JSON-LD">
    <rdf:type rdf:resource="http://www.w3.org/2002/07/owl#NamedIndividual"/>
    <rdf:type rdf:resource="https://w3id.org/italia/onto/ADMS/SemanticAssetDistribution"/>
    <dct:description xml:lang="it">Questa è la distribuzione JSON-LD dell'ontologia dei prezzi, offerte e biglietti</dct:description>
    <dct:description xml:lang="en">This is the distribution in JSON-LD of the Price/Offer/Ticket ontology</dct:description>
    <dct:format rdf:resource="http://publications.europa.eu/resource/authority/file-type/JSON_LD"/>
    <dct:license rdf:resource="https://w3id.org/italia/controlled-vocabulary/licences/A21_CCBY40"/>
    <dct:title xml:lang="it">Distribuzione JSON-LD ontologia POT-AP_IT</dct:title>
    <dct:title xml:lang="en">JSON-LD distribution of POT-AP_IT Ontology</dct:title>
    <dcat:accessURL rdf:resource="https://raw.githubusercontent.com/italia/daf-ontologie-vocabolari-controllati/master/Ontologie/POT/latest"/>
    <dcat:downloadURL rdf:resource="https://raw.githubusercontent.com/italia/daf-ontologie-vocabolari-controllati/master/Ontologie/POT/POT-AP_IT.jsonld"/>
  </rdf:Description>
  <rdf:Description rdf:nodeID="n2282281da4664851aa816bdc565aff50b21">
    <rdf:type rdf:resource="http://www.w3.org/2002/07/owl#Class"/>
    <owl:unionOf rdf:nodeID="n2282281da4664851aa816bdc565aff50b22"/>
  </rdf:Description>
  <rdf:Description rdf:nodeID="n2282281da4664851aa816bdc565aff50b6">
    <rdf:first rdf:resource="https://w3id.org/italia/onto/POT/Ticket"/>
    <rdf:rest rdf:resource="http://www.w3.org/1999/02/22-rdf-syntax-ns#nil"/>
  </rdf:Description>
  <rdf:Description rdf:nodeID="n2282281da4664851aa816bdc565aff50b14">
    <rdf:type rdf:resource="http://www.w3.org/2002/07/owl#Restriction"/>
    <owl:onProperty rdf:resource="https://w3id.org/italia/onto/POT/hasCurrencyValue"/>
    <owl:someValuesFrom rdf:resource="http://www.w3.org/2001/XMLSchema#double"/>
  </rdf:Description>
  <rdf:Description rdf:about="https://w3id.org/italia/onto/l0/Agent">
    <rdf:type rdf:resource="http://www.w3.org/2002/07/owl#Class"/>
  </rdf:Description>
  <rdf:Description rdf:nodeID="n2282281da4664851aa816bdc565aff50b3">
    <rdf:first rdf:resource="https://w3id.org/italia/onto/l0/Location"/>
    <rdf:rest rdf:resource="http://www.w3.org/1999/02/22-rdf-syntax-ns#nil"/>
  </rdf:Description>
  <rdf:Description rdf:nodeID="n2282281da4664851aa816bdc565aff50b11">
    <rdf:type rdf:resource="http://www.w3.org/2002/07/owl#Restriction"/>
    <owl:onProperty rdf:resource="https://w3id.org/italia/onto/POT/hasPriceSpecification"/>
    <owl:someValuesFrom rdf:resource="https://w3id.org/italia/onto/POT/PriceSpecification"/>
  </rdf:Description>
  <rdf:Description rdf:about="http://purl.org/dc/elements/1.1/description">
    <rdf:type rdf:resource="http://www.w3.org/2002/07/owl#AnnotationProperty"/>
  </rdf:Description>
  <rdf:Description rdf:nodeID="n2282281da4664851aa816bdc565aff50b9">
    <rdf:type rdf:resource="http://www.w3.org/2002/07/owl#Restriction"/>
    <owl:onProperty rdf:resource="https://w3id.org/italia/onto/POT/hasValidity"/>
    <owl:allValuesFrom rdf:resource="https://w3id.org/italia/onto/POT/Validity"/>
  </rdf:Description>
  <rdf:Description rdf:nodeID="n2282281da4664851aa816bdc565aff50b10">
    <rdf:type rdf:resource="http://www.w3.org/2002/07/owl#Restriction"/>
    <owl:onProperty rdf:resource="https://w3id.org/italia/onto/POT/includes"/>
    <owl:allValuesFrom rdf:resource="https://w3id.org/italia/onto/POT/Ticket"/>
  </rdf:Description>
  <rdf:Description rdf:nodeID="n2282281da4664851aa816bdc565aff50b4">
    <rdf:type rdf:resource="http://www.w3.org/2002/07/owl#Class"/>
    <owl:unionOf rdf:nodeID="n2282281da4664851aa816bdc565aff50b5"/>
  </rdf:Description>
  <rdf:Description rdf:about="https://w3id.org/italia/onto/l0/name">
    <rdf:type rdf:resource="http://www.w3.org/2002/07/owl#DatatypeProperty"/>
  </rdf:Description>
  <rdf:Description rdf:about="https://w3id.org/italia/onto/l0/Description">
    <rdf:type rdf:resource="http://www.w3.org/2002/07/owl#Class"/>
  </rdf:Description>
  <rdf:Description rdf:about="https://w3id.org/italia/onto/POT/Validity">
    <rdf:type rdf:resource="http://www.w3.org/2002/07/owl#Class"/>
    <rdfs:label xml:lang="en">Validity</rdfs:label>
    <rdfs:label xml:lang="it">Validità</rdfs:label>
    <rdfs:subClassOf rdf:resource="https://w3id.org/italia/onto/l0/EventOrSituation"/>
    <rdfs:subClassOf rdf:nodeID="n2282281da4664851aa816bdc565aff50b19"/>
    <rdfs:subClassOf rdf:nodeID="n2282281da4664851aa816bdc565aff50b20"/>
    <rdfs:comment xml:lang="en">This class represents the validity for the ticket and offering.</rdfs:comment>
    <rdfs:comment xml:lang="it">Questa classe rappresenta la validità di biglietti e di offerte.</rdfs:comment>
    <owl:versionInfo xml:lang="en">stable</owl:versionInfo>
    <owl:versionInfo xml:lang="it">stabile</owl:versionInfo>
    <rdfs:isDefinedBy rdf:resource="https://w3id.org/italia/onto/POT"/>
  </rdf:Description>
  <rdf:Description rdf:about="https://w3id.org/italia/data/organization/support-unit/cnr-Z6HZEH/stlab">
    <rdf:type rdf:resource="http://www.w3.org/2002/07/owl#NamedIndividual"/>
    <rdf:type rdf:resource="http://dati.gov.it/onto/dcatapit#Agent"/>
    <foaf:name xml:lang="en">Institute of Cognitive Sciences and Technologies of the Italian Research Council (CNR) - Semantic Technology Laboratory (STLab)</foaf:name>
    <foaf:name xml:lang="it">Istituto di Scienze e Tecnologie della Cognizione del CNR - Semantic Technology Lab (STLab)</foaf:name>
    <dct:identifier>cnr - Z6HZEH - STLab</dct:identifier>
  </rdf:Description>
  <rdf:Description rdf:nodeID="n2282281da4664851aa816bdc565aff50b17">
    <rdf:type rdf:resource="http://www.w3.org/2002/07/owl#Restriction"/>
    <owl:onProperty rdf:resource="https://w3id.org/italia/onto/l0/description"/>
    <owl:allValuesFrom rdf:resource="http://www.w3.org/2000/01/rdf-schema#Literal"/>
  </rdf:Description>
  <rdf:Description rdf:nodeID="n2282281da4664851aa816bdc565aff50b22">
    <rdf:first rdf:resource="https://w3id.org/italia/onto/MU/Value"/>
    <rdf:rest rdf:nodeID="n2282281da4664851aa816bdc565aff50b23"/>
  </rdf:Description>
  <rdf:Description rdf:nodeID="n2282281da4664851aa816bdc565aff50b23">
    <rdf:first rdf:resource="https://w3id.org/italia/onto/TI/TimeInterval"/>
    <rdf:rest rdf:resource="http://www.w3.org/1999/02/22-rdf-syntax-ns#nil"/>
  </rdf:Description>
  <rdf:Description rdf:nodeID="n2282281da4664851aa816bdc565aff50b5">
    <rdf:first rdf:resource="https://w3id.org/italia/onto/POT/Offer"/>
    <rdf:rest rdf:nodeID="n2282281da4664851aa816bdc565aff50b6"/>
  </rdf:Description>
  <rdf:Description rdf:about="https://w3id.org/italia/onto/POT/includes">
    <rdf:type rdf:resource="http://www.w3.org/2002/07/owl#ObjectProperty"/>
    <rdfs:label xml:lang="en">includes</rdfs:label>
    <rdfs:label xml:lang="it">include biglietto</rdfs:label>
    <rdfs:comment xml:lang="en">Property used to associate an offer with the relative ticket</rdfs:comment>
    <rdfs:comment xml:lang="it">Proprietà utilizzata per associare un'offerta al relativo biglietto.</rdfs:comment>
    <rdfs:isDefinedBy rdf:resource="https://w3id.org/italia/onto/POT"/>
    <rdfs:domain rdf:resource="https://w3id.org/italia/onto/POT/Offer"/>
    <rdfs:range rdf:resource="https://w3id.org/italia/onto/POT/Ticket"/>
  </rdf:Description>
  <rdf:Description rdf:nodeID="n2282281da4664851aa816bdc565aff50b19">
    <rdf:type rdf:resource="http://www.w3.org/2002/07/owl#Restriction"/>
    <owl:onProperty rdf:resource="https://w3id.org/italia/onto/l0/description"/>
    <owl:allValuesFrom rdf:resource="http://www.w3.org/2000/01/rdf-schema#Literal"/>
  </rdf:Description>
  <rdf:Description rdf:nodeID="n2282281da4664851aa816bdc565aff50b7">
    <rdf:type rdf:resource="http://www.w3.org/2002/07/owl#Restriction"/>
    <owl:onProperty rdf:resource="https://w3id.org/italia/onto/l0/name"/>
    <owl:someValuesFrom rdf:resource="http://www.w3.org/2000/01/rdf-schema#Literal"/>
  </rdf:Description>
  <rdf:Description rdf:about="http://www.w3.org/ns/prov#wasDerivedFrom">
    <rdf:type rdf:resource="http://www.w3.org/2002/07/owl#AnnotationProperty"/>
  </rdf:Description>
  <rdf:Description rdf:about="https://w3id.org/italia/onto/MU/Value">
    <rdf:type rdf:resource="http://www.w3.org/2002/07/owl#Class"/>
  </rdf:Description>
  <rdf:Description rdf:nodeID="n2282281da4664851aa816bdc565aff50b1">
    <rdf:type rdf:resource="http://www.w3.org/2002/07/owl#Class"/>
    <owl:unionOf rdf:nodeID="n2282281da4664851aa816bdc565aff50b2"/>
  </rdf:Description>
  <rdf:Description rdf:about="https://w3id.org/italia/onto/l0/Location">
    <rdf:type rdf:resource="http://www.w3.org/2002/07/owl#Class"/>
  </rdf:Description>
  <rdf:Description rdf:about="https://w3id.org/italia/onto/TI/hasDuration">
    <rdf:type rdf:resource="http://www.w3.org/2002/07/owl#ObjectProperty"/>
  </rdf:Description>
  <rdf:Description rdf:about="https://w3id.org/italia/onto/l0/description">
    <rdf:type rdf:resource="http://www.w3.org/2002/07/owl#DatatypeProperty"/>
  </rdf:Description>
  <rdf:Description rdf:about="https://w3id.org/italia/onto/l0/Characteristic">
    <rdf:type rdf:resource="http://www.w3.org/2002/07/owl#Class"/>
  </rdf:Description>
  <rdf:Description rdf:about="https://w3id.org/italia/onto/l0/EventOrSituation">
    <rdf:type rdf:resource="http://www.w3.org/2002/07/owl#Class"/>
  </rdf:Description>
  <rdf:Description rdf:about="https://w3id.org/italia/onto/TI/TimeInterval">
    <rdf:type rdf:resource="http://www.w3.org/2002/07/owl#Class"/>
  </rdf:Description>
  <rdf:Description rdf:about="https://w3id.org/italia/onto/l0/Object">
    <rdf:type rdf:resource="http://www.w3.org/2002/07/owl#Class"/>
  </rdf:Description>
</rdf:RDF>
