<?xml version="1.0" encoding="utf-8"?>
<rdf:RDF
  xmlns:rdfs="http://www.w3.org/2000/01/rdf-schema#"
  xmlns:dct="http://purl.org/dc/terms/"
  xmlns:dcat="http://www.w3.org/ns/dcat#"
  xmlns:adms="http://www.w3.org/ns/adms#"
  xmlns:dcatapit="http://dati.gov.it/onto/dcatapit#"
  xmlns:vcard="http://www.w3.org/2006/vcard/ns#"
  xmlns:foaf="http://xmlns.com/foaf/0.1/"
  xmlns:owl="http://www.w3.org/2002/07/owl#"
  xmlns:skos="http://www.w3.org/2004/02/skos/core#"
  xmlns:ndc="https://w3id.org/italia/onto/NDC/"
  xmlns:cpsvapit="https://w3id.org/italia/onto/CPSV/"
  xmlns:clvapit="https://w3id.org/italia/onto/CLV/"
  xmlns:xkos="http://rdf-vocabulary.ddialliance.org/xkos#"
  xmlns:rdf="http://www.w3.org/1999/02/22-rdf-syntax-ns#"
>
  <skos:ConceptScheme rdf:about="https://w3id.org/italia/controlled-vocabulary/classifications-for-public-services/authentication-type">
    <rdf:type rdf:resource="http://www.w3.org/ns/adms#Asset"/>
    <rdf:type rdf:resource="http://dati.gov.it/onto/dcatapit#Dataset"/>
    <rdfs:comment xml:lang="en">Controlled Vocabulary on the classification of the types of authentication. Currently, the vocabulary is used in the catalogue of public services. The translations in Germany were provided by Ivo Planoetscher of the Autonomous Province of Bolzano</rdfs:comment>
    <rdfs:comment xml:lang="it">Vocabolario controllato della classificazione dei tipi di autenticazione. Attualmente il vocabolario è utilizzato nell'ambito dello sviluppo del catalogo servizi pubblici. Le traduzioni in tedesco sono state fornite da Ivo Planoetscher della Pronvicia Autonoma di Bolzano</rdfs:comment>
    <dct:title xml:lang="en">Authentication Controlled Vocabulary</dct:title>
    <dct:title xml:lang="it">Vocabolario Controllato sui tipi di autenticazione</dct:title>
    <dct:description xml:lang="en">Controlled Vocabulary on the classification of the types of authentication. Currently, the vocabulary is used in the catalogue of public services. The translations in Germany were provided by Ivo Planoetscher of the Autonomous Province of Bolzano</dct:description>
    <dct:description xml:lang="it">Vocabolario controllato della classificazione dei tipi di autenticazione. Attualmente il vocabolario è utilizzato nell'ambito dello sviluppo del catalogo servizi pubblici. Le traduzioni in tedesco sono state fornite da Ivo Planoetscher della Pronvicia Autonoma di Bolzano</dct:description>
    <rdfs:label xml:lang="en">Authentication Controlled Vocabulary</rdfs:label>
    <rdfs:label xml:lang="it">Vocabolario Controllato sui tipi di autenticazione</rdfs:label>
    <xkos:numberOfLevels>2</xkos:numberOfLevels>
    <dct:type rdf:resource="http://purl.org/adms/assettype/Taxonomy"/>
    <adms:representationTechnique rdf:resource="http://purl.org/adms/representationtechnique/SKOS"/>
    <dct:identifier>agid:D.6</dct:identifier>
    <ndc:keyConcept>authentication-type</ndc:keyConcept>
    <dct:rightsHolder>
      <dcatapit:Agent rdf:about="http://spcdata.digitpa.gov.it/browse/page/Amministrazione/agid">
        <rdf:type rdf:resource="http://xmlns.com/foaf/0.1/Agent"/>
        <dct:identifier>agid</dct:identifier>
        <foaf:name xml:lang="it">Agenzia per l'Italia Digitale</foaf:name>
        <foaf:name xml:lang="en">Italian Digital Agency</foaf:name>
      </dcatapit:Agent>
    </dct:rightsHolder>
    <dct:creator rdf:resource="http://spcdata.digitpa.gov.it/browse/page/Amministrazione/agid"/>
    <dct:publisher rdf:resource="http://spcdata.digitpa.gov.it/browse/page/Amministrazione/agid"/>
    <dcat:theme rdf:resource="http://publications.europa.eu/resource/authority/data-theme/GOVE"/>
    <dct:subject rdf:resource="http://eurovoc.europa.eu/246051"/>
    <dct:subject rdf:resource="http://eurovoc.europa.eu/246146"/>
    <dct:subject rdf:resource="http://eurovoc.europa.eu/100169"/>
    <rdfs:isDefinedBy rdf:resource="https://w3id.org/italia/controlled-vocabulary/classifications-for-public-services/authentication-type"/>
    <dct:conformsTo>
      <dcatapit:Standard rdf:about="http://dati.gov.it/data/resource/Standard/SKOS">
        <rdf:type rdf:resource="http://purl.org/dc/terms/Standard"/>
        <dct:identifier>SKOS</dct:identifier>
        <dct:title>Simple Knowledge Organization System - SKOS</dct:title>
        <dct:description>The Simple Knowledge Organization System (SKOS) is a common data model for sharing and linking knowledge organization systems via the Web</dct:description>
      </dcatapit:Standard>
    </dct:conformsTo>
    <dct:language rdf:resource="http://publications.europa.eu/resource/authority/language/ITA"/>
    <dct:language rdf:resource="http://publications.europa.eu/resource/authority/language/ENG"/>
    <dct:language rdf:resource="http://publications.europa.eu/resource/authority/language/DEU"/>
    <dct:accrualPeriodicity rdf:resource="http://publications.europa.eu/resource/authority/frequency/IRREG"/>
    <dcat:keyword xml:lang="it">autenticazione</dcat:keyword>
    <dcat:keyword xml:lang="it">servizio pubblico</dcat:keyword>
    <dcat:keyword xml:lang="it">spid</dcat:keyword>
    <dcat:keyword xml:lang="it">password</dcat:keyword>
    <dcat:keyword xml:lang="it">carta nazionale servizi</dcat:keyword>
    <dcat:keyword xml:lang="en">authentication</dcat:keyword>
    <dcat:keyword xml:lang="en">public service</dcat:keyword>
    <dcat:keyword xml:lang="en">spid</dcat:keyword>
    <dcat:keyword xml:lang="en">password</dcat:keyword>
    <dcat:keyword xml:lang="en">national service card</dcat:keyword>
    <dcat:distribution>
      <dcatapit:Distribution rdf:about="http://dati.gov.it/data/resource/Distribution/Authentication_RDF_Turtle">
        <dct:title xml:lang="it">Distribuzione RDF/Turtle tipi autenticazione servizi pubblici</dct:title>
        <dct:title xml:lang="en">RDF/Turtle distribution types of authentication for public services</dct:title>
        <dct:description xml:lang="it">Questa è la distribuzione RDF/Turtle del dataset Linked Open Data del vocabolario controllato sulla classificazione dei tipi di autenticazione per i servizi pubblici</dct:description>
        <dct:description xml:lang="en">This is the distribution in RDF/Turtle of the Linked Open Dataset of the controlled vocabulary related to the types of authentication for public services</dct:description>
        <dct:format rdf:resource="http://publications.europa.eu/resource/authority/file-type/RDF_TURTLE"/>
        <dct:license rdf:resource="https://w3id.org/italia/controlled-vocabulary/licences/A21_CCBY40"/>
        <dcat:downloadURL rdf:resource="https://raw.githubusercontent.com/italia/daf-ontologie-vocabolari-controllati/master/VocabolariControllati/classifications-for-public-services/authentication-type/authentication-type.ttl"/>
        <dcat:accessURL rdf:resource="https://raw.githubusercontent.com/italia/daf-ontologie-vocabolari-controllati/master/VocabolariControllati/classifications-for-public-services/authentication-type"/>
      </dcatapit:Distribution>
    </dcat:distribution>
    <dcat:distribution>
      <dcatapit:Distribution rdf:about="http://dati.gov.it/data/resource/Distribution/Authentication_RDF_XML">
        <dct:title xml:lang="it">Distribuzione RDF/XML tipi autenticazione servizi pubblici</dct:title>
        <dct:title xml:lang="en">RDF/XML distribution types of authentication for public services</dct:title>
        <dct:description xml:lang="it">Questa è la distribuzione RDF/XML del dataset Linked Open Data del vocabolario controllato sulla classificazione dei tipi di autenticazione per i servizi pubblici</dct:description>
        <dct:description xml:lang="en">This is the distribution in RDF/XML of the Linked Open Dataset of the controlled vocabulary related to the types of authentication for public services</dct:description>
        <dct:format rdf:resource="http://publications.europa.eu/resource/authority/file-type/RDF_XML"/>
        <dct:license rdf:resource="https://w3id.org/italia/controlled-vocabulary/licences/A21_CCBY40"/>
        <dcat:downloadURL rdf:resource="https://raw.githubusercontent.com/italia/daf-ontologie-vocabolari-controllati/master/VocabolariControllati/classifications-for-public-services/authentication-type/authentication-type.rdf"/>
        <dcat:accessURL rdf:resource="https://raw.githubusercontent.com/italia/daf-ontologie-vocabolari-controllati/master/VocabolariControllati/classifications-for-public-services/authentication-type"/>
      </dcatapit:Distribution>
    </dcat:distribution>
    <dcat:distribution>
      <dcatapit:Distribution rdf:about="http://dati.gov.it/data/resource/Distribution/Authentication_JSON_LD">
        <dct:title xml:lang="it">Distribuzione JSON_LD tipi autenticazione servizi pubblici</dct:title>
        <dct:title xml:lang="en">JSON_LD distribution types of authentication for public services</dct:title>
        <dct:description xml:lang="it">Questa è la distribuzione JSON_LD del dataset Linked Open Data del vocabolario controllato sulla classificazione dei tipi di autenticazione per i servizi pubblici</dct:description>
        <dct:description xml:lang="en">This is the distribution in JSON_LD of the Linked Open Dataset of the controlled vocabulary related to the types of authentication for public services</dct:description>
        <dct:format rdf:resource="http://publications.europa.eu/resource/authority/file-type/JSON_LD"/>
        <dct:license rdf:resource="https://w3id.org/italia/controlled-vocabulary/licences/A21_CCBY40"/>
        <dcat:downloadURL rdf:resource="https://raw.githubusercontent.com/italia/daf-ontologie-vocabolari-controllati/master/VocabolariControllati/classifications-for-public-services/authentication-type/authentication-type.jsonld"/>
        <dcat:accessURL rdf:resource="https://raw.githubusercontent.com/italia/daf-ontologie-vocabolari-controllati/master/VocabolariControllati/classifications-for-public-services/authentication-type"/>
      </dcatapit:Distribution>
    </dcat:distribution>
    <dcat:distribution>
      <dcatapit:Distribution rdf:about="http://dati.gov.it/data/resource/Distribution/Authentication_CSV">
        <dct:title xml:lang="it">Distribuzione CSV tipi autenticazione servizi pubblici</dct:title>
        <dct:title xml:lang="en">CSV distribution types of authentication for public services</dct:title>
        <dct:description xml:lang="it">Questa è la distribuzione CSV del dataset Linked Open Data del vocabolario controllato sulla classificazione dei tipi di autenticazione per i servizi pubblici</dct:description>
        <dct:description xml:lang="en">This is the distribution in CSV of the Linked Open Dataset of the controlled vocabulary related to the types of authentication for public services</dct:description>
        <dct:format rdf:resource="http://publications.europa.eu/resource/authority/file-type/CSV"/>
        <dct:license rdf:resource="https://w3id.org/italia/controlled-vocabulary/licences/A21_CCBY40"/>
        <dcat:downloadURL rdf:resource="https://raw.githubusercontent.com/italia/daf-ontologie-vocabolari-controllati/master/VocabolariControllati/classifications-for-public-services/authentication-type/authentication-type.csv"/>
        <dcat:accessURL rdf:resource="https://raw.githubusercontent.com/italia/daf-ontologie-vocabolari-controllati/master/VocabolariControllati/classifications-for-public-services/authentication-type"/>
      </dcatapit:Distribution>
    </dcat:distribution>
    <dcat:distribution>
      <dcatapit:Distribution rdf:about="http://dati.gov.it/data/resource/Distribution/Authentication_XLSX">
        <dct:title xml:lang="it">Distribuzione XLSX tipi autenticazione servizi pubblici</dct:title>
        <dct:title xml:lang="en">XLSX distribution types of authentication for public services</dct:title>
        <dct:description xml:lang="it">Questa è la distribuzione XLSX del dataset Linked Open Data del vocabolario controllato sulla classificazione dei tipi di autenticazione per i servizi pubblici</dct:description>
        <dct:description xml:lang="en">This is the distribution in XLSX of the Linked Open Dataset of the controlled vocabulary related to the types of authentication for public services</dct:description>
        <dct:format rdf:resource="http://publications.europa.eu/resource/authority/file-type/XLSX"/>
        <dct:license rdf:resource="https://w3id.org/italia/controlled-vocabulary/licences/A21_CCBY40"/>
        <dcat:downloadURL rdf:resource="https://raw.githubusercontent.com/italia/daf-ontologie-vocabolari-controllati/master/VocabolariControllati/classifications-for-public-services/authentication-type/authentication-type.xlsx"/>
        <dcat:accessURL rdf:resource="https://raw.githubusercontent.com/italia/daf-ontologie-vocabolari-controllati/master/VocabolariControllati/classifications-for-public-services/authentication-type"/>
      </dcatapit:Distribution>
    </dcat:distribution>
    <dcat:contactPoint>
      <dcatapit:Organization rdf:about="http://dati.gov.it/data/resource/ContactPoint/voc_AgID">
        <rdf:type rdf:resource="http://www.w3.org/2006/vcard/ns#Organization"/>
        <rdf:type rdf:resource="http://www.w3.org/2006/vcard/ns#Kind"/>
        <vcard:fn>banche dati e open data</vcard:fn>
        <vcard:hasEmail rdf:resource="mailto:info@dati.gov.it"/>
      </dcatapit:Organization>
    </dcat:contactPoint>
    <skos:hasTopConcept>
      <skos:Concept rdf:about="https://w3id.org/italia/controlled-vocabulary/classifications-for-public-services/authentication-type/NONE">
        <rdf:type rdf:resource="https://w3id.org/italia/onto/CPSV/Authentication"/>
        <skos:inScheme rdf:resource="https://w3id.org/italia/controlled-vocabulary/classifications-for-public-services/authentication-type"/>
        <skos:notation>NONE</skos:notation>
        <dct:identifier>NONE</dct:identifier>
        <clvapit:hasRankOrder>1</clvapit:hasRankOrder>
        <skos:prefLabel xml:lang="it">Nessuna - accesso libero</skos:prefLabel>
        <skos:prefLabel xml:lang="de">Keine - freier Zugang</skos:prefLabel>
        <skos:prefLabel xml:lang="en">None - free access</skos:prefLabel>
      </skos:Concept>
    </skos:hasTopConcept>
    <skos:hasTopConcept>
      <skos:Concept rdf:about="https://w3id.org/italia/controlled-vocabulary/classifications-for-public-services/authentication-type/SFA">
        <rdf:type rdf:resource="https://w3id.org/italia/onto/CPSV/Authentication"/>
        <skos:inScheme rdf:resource="https://w3id.org/italia/controlled-vocabulary/classifications-for-public-services/authentication-type"/>
        <skos:notation>SFA</skos:notation>
        <dct:identifier>SFA</dct:identifier>
        <clvapit:hasRankOrder>1</clvapit:hasRankOrder>
        <skos:narrower rdf:resource="https://w3id.org/italia/controlled-vocabulary/classifications-for-public-services/authentication-type/IDPWD"/>
        <skos:narrower rdf:resource="https://w3id.org/italia/controlled-vocabulary/classifications-for-public-services/authentication-type/SPIDL1"/>
        <skos:prefLabel xml:lang="it">Autenticazione Singolo Fattore</skos:prefLabel>
        <skos:prefLabel xml:lang="de">Single-Faktor-Authentifizierung</skos:prefLabel>
        <skos:prefLabel xml:lang="en">Single Factor Authentication</skos:prefLabel>
      </skos:Concept>
    </skos:hasTopConcept>
    <skos:hasTopConcept>
      <skos:Concept rdf:about="https://w3id.org/italia/controlled-vocabulary/classifications-for-public-services/authentication-type/2FA">
        <rdf:type rdf:resource="https://w3id.org/italia/onto/CPSV/Authentication"/>
        <skos:inScheme rdf:resource="https://w3id.org/italia/controlled-vocabulary/classifications-for-public-services/authentication-type"/>
        <skos:notation>2FA</skos:notation>
        <dct:identifier>2FA</dct:identifier>
        <clvapit:hasRankOrder>1</clvapit:hasRankOrder>
        <skos:narrower rdf:resource="https://w3id.org/italia/controlled-vocabulary/classifications-for-public-services/authentication-type/SPIDL2"/>
        <skos:narrower rdf:resource="https://w3id.org/italia/controlled-vocabulary/classifications-for-public-services/authentication-type/IDOTP"/>
        <skos:prefLabel xml:lang="it">Autenticazione a due fattori</skos:prefLabel>
        <skos:prefLabel xml:lang="de">Zwei-Faktor-Authentifizierung</skos:prefLabel>
        <skos:prefLabel xml:lang="en">Two Factor authentication</skos:prefLabel>
      </skos:Concept>
    </skos:hasTopConcept>
    <skos:hasTopConcept rdf:resource="https://w3id.org/italia/controlled-vocabulary/classifications-for-public-services/authentication-type/22FAHW"/>
    <skos:hasTopConcept>
      <skos:Concept rdf:about="https://w3id.org/italia/controlled-vocabulary/classifications-for-public-services/authentication-type/MFA">
        <rdf:type rdf:resource="https://w3id.org/italia/onto/CPSV/Authentication"/>
        <skos:inScheme rdf:resource="https://w3id.org/italia/controlled-vocabulary/classifications-for-public-services/authentication-type"/>
        <skos:notation>MFA</skos:notation>
        <dct:identifier>MFA</dct:identifier>
        <clvapit:hasRankOrder>1</clvapit:hasRankOrder>
        <skos:narrower rdf:resource="https://w3id.org/italia/controlled-vocabulary/classifications-for-public-services/authentication-type/IDOTPBIO"/>
        <skos:prefLabel xml:lang="it">Autenticazione multi-fattore</skos:prefLabel>
        <skos:prefLabel xml:lang="de">Multi-Faktor-Authentifizierung</skos:prefLabel>
        <skos:prefLabel xml:lang="en">Multi-factor authentication</skos:prefLabel>
      </skos:Concept>
    </skos:hasTopConcept>
    <dct:issued rdf:datatype="http://www.w3.org/2001/XMLSchema#date">2017-10-20</dct:issued>
    <dct:modified rdf:datatype="http://www.w3.org/2001/XMLSchema#date">2018-03-14</dct:modified>
    <owl:versionInfo>0.1</owl:versionInfo>
  </skos:ConceptScheme>
  <rdfs:Property rdf:about="https://w3id.org/italia/onto/NDC/keyConcept"/>
  <rdfs:Property rdf:about="http://purl.org/dc/terms/accrualPeriodicity"/>
  <rdfs:Property rdf:about="http://purl.org/dc/terms/type"/>
  <rdfs:Property rdf:about="http://purl.org/dc/terms/format"/>
  <rdfs:Property rdf:about="http://www.w3.org/2006/vcard/ns#fn"/>
  <rdfs:Property rdf:about="http://purl.org/dc/terms/publisher"/>
  <rdfs:Property rdf:about="http://www.w3.org/2004/02/skos/core#definition"/>
  <rdfs:Property rdf:about="http://purl.org/dc/terms/description"/>
  <rdfs:Property rdf:about="http://www.w3.org/2002/07/owl#versionInfo"/>
  <rdfs:Property rdf:about="http://xmlns.com/foaf/0.1/name"/>
  <rdfs:Property rdf:about="http://www.w3.org/ns/dcat#contactPoint"/>
  <rdfs:Property rdf:about="http://purl.org/dc/terms/issued"/>
  <rdfs:Property rdf:about="http://www.w3.org/2004/02/skos/core#notation"/>
  <rdfs:Property rdf:about="https://w3id.org/italia/onto/CLV/hasRankOrder"/>
  <rdfs:Property rdf:about="http://www.w3.org/2004/02/skos/core#inScheme"/>
  <rdfs:Property rdf:about="http://www.w3.org/2004/02/skos/core#narrower"/>
  <rdfs:Property rdf:about="http://purl.org/dc/terms/title"/>
  <rdfs:Property rdf:about="http://purl.org/dc/terms/license"/>
  <rdfs:Property rdf:about="http://purl.org/dc/terms/language"/>
  <rdfs:Property rdf:about="http://www.w3.org/ns/dcat#distribution"/>
  <rdfs:Property rdf:about="http://rdf-vocabulary.ddialliance.org/xkos#numberOfLevels"/>
  <rdfs:Property rdf:about="http://purl.org/dc/terms/conformsTo"/>
  <rdfs:Property rdf:about="http://www.w3.org/2006/vcard/ns#hasEmail"/>
  <rdfs:Property rdf:about="http://www.w3.org/2004/02/skos/core#prefLabel"/>
  <rdfs:Property rdf:about="http://purl.org/dc/terms/identifier"/>
  <rdfs:Property rdf:about="http://purl.org/dc/terms/modified"/>
  <rdfs:Property rdf:about="http://www.w3.org/ns/dcat#accessURL"/>
  <rdfs:Property rdf:about="http://purl.org/dc/terms/rightsHolder"/>
  <rdfs:Property rdf:about="http://www.w3.org/ns/dcat#downloadURL"/>
  <rdfs:Property rdf:about="http://purl.org/dc/terms/creator"/>
  <rdfs:Property rdf:about="http://www.w3.org/ns/dcat#keyword"/>
  <rdfs:Property rdf:about="http://www.w3.org/ns/dcat#theme"/>
  <rdfs:Property rdf:about="http://purl.org/dc/terms/subject"/>
  <rdfs:Property rdf:about="http://www.w3.org/ns/adms#representationTechnique"/>
  <rdfs:Property rdf:about="http://www.w3.org/2004/02/skos/core#broader"/>
  <skos:Concept rdf:about="https://w3id.org/italia/controlled-vocabulary/classifications-for-public-services/authentication-type/CNS">
    <rdf:type rdf:resource="https://w3id.org/italia/onto/CPSV/Authentication"/>
    <skos:inScheme rdf:resource="https://w3id.org/italia/controlled-vocabulary/classifications-for-public-services/authentication-type"/>
    <skos:notation>CNS</skos:notation>
    <dct:identifier>CNS</dct:identifier>
    <clvapit:hasRankOrder>2</clvapit:hasRankOrder>
    <skos:broader>
      <skos:Concept rdf:about="https://w3id.org/italia/controlled-vocabulary/classifications-for-public-services/authentication-type/2FAHW">
        <rdf:type rdf:resource="https://w3id.org/italia/onto/CPSV/Authentication"/>
        <skos:inScheme rdf:resource="https://w3id.org/italia/controlled-vocabulary/classifications-for-public-services/authentication-type"/>
        <skos:notation>2FAHW</skos:notation>
        <dct:identifier>2FAHW</dct:identifier>
        <clvapit:hasRankOrder>1</clvapit:hasRankOrder>
        <skos:narrower rdf:resource="https://w3id.org/italia/controlled-vocabulary/classifications-for-public-services/authentication-type/SPIDL3"/>
        <skos:narrower rdf:resource="https://w3id.org/italia/controlled-vocabulary/classifications-for-public-services/authentication-type/CNS"/>
        <skos:narrower rdf:resource="https://w3id.org/italia/controlled-vocabulary/classifications-for-public-services/authentication-type/CIE"/>
        <skos:prefLabel xml:lang="it">Autenticazione a due fattori hardware</skos:prefLabel>
        <skos:prefLabel xml:lang="de">Zwei-Faktor-Hardware-Authentifizierung</skos:prefLabel>
        <skos:prefLabel xml:lang="en">Two Factor Authentication hardware</skos:prefLabel>
      </skos:Concept>
    </skos:broader>
    <skos:prefLabel xml:lang="it">Carta nazionale dei servizi (CNS)</skos:prefLabel>
    <skos:prefLabel xml:lang="de">Nationale Servicekarte</skos:prefLabel>
    <skos:prefLabel xml:lang="en">National service card</skos:prefLabel>
  </skos:Concept>
  <skos:Concept rdf:about="https://w3id.org/italia/controlled-vocabulary/classifications-for-public-services/authentication-type/CIE">
    <rdf:type rdf:resource="https://w3id.org/italia/onto/CPSV/Authentication"/>
    <skos:inScheme rdf:resource="https://w3id.org/italia/controlled-vocabulary/classifications-for-public-services/authentication-type"/>
    <skos:notation>CIE</skos:notation>
    <dct:identifier>CIE</dct:identifier>
    <clvapit:hasRankOrder>2</clvapit:hasRankOrder>
    <skos:broader rdf:resource="https://w3id.org/italia/controlled-vocabulary/classifications-for-public-services/authentication-type/2FAHW"/>
    <skos:prefLabel xml:lang="it">Carta d'identità elettronica (CIE)</skos:prefLabel>
    <skos:prefLabel xml:lang="de">Elektronischer Personalausweis (CIE)</skos:prefLabel>
    <skos:prefLabel xml:lang="en">Electronic identity card</skos:prefLabel>
  </skos:Concept>
  <skos:Concept rdf:about="https://w3id.org/italia/controlled-vocabulary/classifications-for-public-services/authentication-type/IDOTP">
    <rdf:type rdf:resource="https://w3id.org/italia/onto/CPSV/Authentication"/>
    <skos:inScheme rdf:resource="https://w3id.org/italia/controlled-vocabulary/classifications-for-public-services/authentication-type"/>
    <skos:notation>ID OTP</skos:notation>
    <dct:identifier>ID OTP</dct:identifier>
    <clvapit:hasRankOrder>2</clvapit:hasRankOrder>
    <skos:broader rdf:resource="https://w3id.org/italia/controlled-vocabulary/classifications-for-public-services/authentication-type/2FA"/>
    <skos:prefLabel xml:lang="it">User ID e One Time Password</skos:prefLabel>
    <skos:prefLabel xml:lang="de">Benutzer-ID und Einmal-Passwort</skos:prefLabel>
    <skos:prefLabel xml:lang="en">User ID and One Time Password</skos:prefLabel>
    <skos:definition xml:lang="it">Combinazione di due fattori: userid e one time password</skos:definition>
    <skos:definition xml:lang="en">Combination of two factors: userid and one time password</skos:definition>
  </skos:Concept>
  <rdfs:Class rdf:about="http://dati.gov.it/onto/dcatapit#Organization"/>
  <skos:Concept rdf:about="https://w3id.org/italia/controlled-vocabulary/classifications-for-public-services/authentication-type/SPIDL2">
    <rdf:type rdf:resource="https://w3id.org/italia/onto/CPSV/Authentication"/>
    <skos:inScheme rdf:resource="https://w3id.org/italia/controlled-vocabulary/classifications-for-public-services/authentication-type"/>
    <skos:notation>SPIDL2</skos:notation>
    <dct:identifier>SPIDL2</dct:identifier>
    <clvapit:hasRankOrder>2</clvapit:hasRankOrder>
    <skos:broader rdf:resource="https://w3id.org/italia/controlled-vocabulary/classifications-for-public-services/authentication-type/2FA"/>
    <skos:prefLabel xml:lang="it">SPID Livello 2</skos:prefLabel>
    <skos:prefLabel xml:lang="de">SPID (Nationales öffentliches System der e-ID) Stufe 2</skos:prefLabel>
    <skos:prefLabel xml:lang="en">SPID (National public system of e-ID) Level 2</skos:prefLabel>
  </skos:Concept>
  <skos:Concept rdf:about="https://w3id.org/italia/controlled-vocabulary/classifications-for-public-services/authentication-type/IDOTPBIO">
    <rdf:type rdf:resource="https://w3id.org/italia/onto/CPSV/Authentication"/>
    <skos:inScheme rdf:resource="https://w3id.org/italia/controlled-vocabulary/classifications-for-public-services/authentication-type"/>
    <skos:notation>USERID OTP BIO</skos:notation>
    <dct:identifier>USERID OTP BIO</dct:identifier>
    <clvapit:hasRankOrder>2</clvapit:hasRankOrder>
    <skos:broader rdf:resource="https://w3id.org/italia/controlled-vocabulary/classifications-for-public-services/authentication-type/MFA"/>
    <skos:prefLabel xml:lang="it">User ID, One Time Password e Biometria</skos:prefLabel>
    <skos:prefLabel xml:lang="en">User ID, One Time Password and Biometric</skos:prefLabel>
    <skos:prefLabel xml:lang="de">Benutzer-ID, Einmalpasswort und biometrische Daten</skos:prefLabel>
    <skos:definition xml:lang="it">Combinazione di più fattori: userid, one time password e strumenti di biometria</skos:definition>
    <skos:definition xml:lang="en">Combination of different factors: userid,  one time password and biometric mechanisms</skos:definition>
  </skos:Concept>
  <skos:Concept rdf:about="https://w3id.org/italia/controlled-vocabulary/classifications-for-public-services/authentication-type/SPIDL1">
    <rdf:type rdf:resource="https://w3id.org/italia/onto/CPSV/Authentication"/>
    <skos:inScheme rdf:resource="https://w3id.org/italia/controlled-vocabulary/classifications-for-public-services/authentication-type"/>
    <skos:broader rdf:resource="https://w3id.org/italia/controlled-vocabulary/classifications-for-public-services/authentication-type/SFA"/>
    <skos:notation>SPIDL1</skos:notation>
    <dct:identifier>SPIDL1</dct:identifier>
    <clvapit:hasRankOrder>2</clvapit:hasRankOrder>
    <skos:prefLabel xml:lang="it">Credenziale SPID Livello 1</skos:prefLabel>
    <skos:prefLabel xml:lang="de">SPID (Nationales öffentliches System der e-ID) Berechtigungsnachweis Stufe 1</skos:prefLabel>
    <skos:prefLabel xml:lang="en">SPID (National public system of e-ID) Credential Level 1</skos:prefLabel>
  </skos:Concept>
  <skos:Concept rdf:about="https://w3id.org/italia/controlled-vocabulary/classifications-for-public-services/authentication-type/SPIDL3">
    <rdf:type rdf:resource="https://w3id.org/italia/onto/CPSV/Authentication"/>
    <skos:inScheme rdf:resource="https://w3id.org/italia/controlled-vocabulary/classifications-for-public-services/authentication-type"/>
    <skos:notation>SPIDL3</skos:notation>
    <dct:identifier>SPIDL3</dct:identifier>
    <clvapit:hasRankOrder>2</clvapit:hasRankOrder>
    <skos:broader rdf:resource="https://w3id.org/italia/controlled-vocabulary/classifications-for-public-services/authentication-type/2FAHW"/>
    <skos:prefLabel xml:lang="it">SPID Livello 3</skos:prefLabel>
    <skos:prefLabel xml:lang="de">SPID (Nationales öffentliches System der e-ID) Stufe 3</skos:prefLabel>
    <skos:prefLabel xml:lang="en">SPID (National public system of e-ID) Level 3</skos:prefLabel>
  </skos:Concept>
  <rdfs:Class rdf:about="http://dati.gov.it/onto/dcatapit#Dataset"/>
  <rdfs:Class rdf:about="http://www.w3.org/2004/02/skos/core#ConceptScheme"/>
  <skos:Concept rdf:about="https://w3id.org/italia/controlled-vocabulary/classifications-for-public-services/authentication-type/IDPWD">
    <rdf:type rdf:resource="https://w3id.org/italia/onto/CPSV/Authentication"/>
    <skos:inScheme rdf:resource="https://w3id.org/italia/controlled-vocabulary/classifications-for-public-services/authentication-type"/>
    <skos:broader rdf:resource="https://w3id.org/italia/controlled-vocabulary/classifications-for-public-services/authentication-type/SFA"/>
    <skos:notation>IDPWD</skos:notation>
    <dct:identifier>IDPWD</dct:identifier>
    <clvapit:hasRankOrder>2</clvapit:hasRankOrder>
    <skos:prefLabel xml:lang="it">User ID e password</skos:prefLabel>
    <skos:prefLabel xml:lang="de">Benutzer-ID und Passwort</skos:prefLabel>
    <skos:prefLabel xml:lang="en">User ID and password</skos:prefLabel>
    <skos:definition xml:lang="it">Credenziale semplice basata sull'uso di username e password. Accesso tramite sistemi quali NoiPA, FiscoOnline e ogni altro sistema che richiede solo credenziali di tipo usernname e password ricadono in questa categoria</skos:definition>
    <skos:definition xml:lang="en">Simple credential consisting in username and password. Access to online Italian systems such as NoiPA and Fiscoonline and any other system that requires username and password fall into this category</skos:definition>
  </skos:Concept>
  <rdfs:Class rdf:about="http://dati.gov.it/onto/dcatapit#Standard"/>
  <rdfs:Class rdf:about="http://xmlns.com/foaf/0.1/Agent"/>
  <rdfs:Class rdf:about="http://www.w3.org/2004/02/skos/core#Concept"/>
  <rdfs:Class rdf:about="http://dati.gov.it/onto/dcatapit#Agent"/>
  <rdfs:Class rdf:about="http://www.w3.org/2006/vcard/ns#Kind"/>
  <rdfs:Class rdf:about="https://w3id.org/italia/onto/CPSV/Authentication"/>
  <rdfs:Class rdf:about="http://dati.gov.it/onto/dcatapit#Distribution"/>
  <rdfs:Class rdf:about="http://www.w3.org/2006/vcard/ns#Organization"/>
  <rdfs:Class rdf:about="http://purl.org/dc/terms/Standard"/>
</rdf:RDF>
