<?xml version="1.0"?>
<rdf:RDF xmlns="https://w3id.org/italia/onto/PublicContract/"
     xml:base="https://w3id.org/italia/onto/PublicContract/"
     xmlns:dc="http://purl.org/dc/elements/1.1/"
     xmlns:l0="https://w3id.org/italia/onto/l0/"
     xmlns:ti="https://w3id.org/italia/onto/TI/"
     xmlns:dct="http://purl.org/dc/terms/"
     xmlns:owl="http://www.w3.org/2002/07/owl#"
     xmlns:rdf="http://www.w3.org/1999/02/22-rdf-syntax-ns#"
     xmlns:xml="http://www.w3.org/XML/1998/namespace"
     xmlns:xsd="http://www.w3.org/2001/XMLSchema#"
     xmlns:dcat="http://www.w3.org/ns/dcat#"
     xmlns:foaf="http://xmlns.com/foaf/0.1/"
     xmlns:prov="http://www.w3.org/ns/prov#"
     xmlns:rdfs="http://www.w3.org/2000/01/rdf-schema#"
     xmlns:vcard="http://www.w3.org/2006/vcard/ns#"
     xmlns:schema="http://schema.org/"
     xmlns:covapit="https://w3id.org/italia/onto/COV/"
     xmlns:admsapit="https://w3id.org/italia/onto/ADMS/"
     xmlns:dcatapit="http://dati.gov.it/onto/dcatapit#">
    <owl:Ontology rdf:about="https://w3id.org/italia/onto/PublicContract">
        <owl:versionIRI rdf:resource="https://w3id.org/italia/onto/PublicContract/0.4"/>
        <owl:imports rdf:resource="https://w3id.org/italia/onto/RO"/>
        <owl:imports rdf:resource="https://w3id.org/italia/onto/l0"/>
        <dct:accrualPeriodicity rdf:resource="http://publications.europa.eu/resource/authority/frequency/IRREG"/>
        <dct:creator rdf:resource="http://spcdata.digitpa.gov.it/Amministrazione/agid"/>
        <dct:creator rdf:resource="http://spcdata.digitpa.gov.it/Amministrazione/csi_piem"/>
        <dct:creator rdf:resource="http://spcdata.digitpa.gov.it/Amministrazione/cvtiap"/>
        <dct:creator rdf:resource="https://w3id.org/italia/data/organization/private-organization/IT11491360019"/>
        <dct:description xml:lang="it">Questo il profilo applicativo italiano dell&apos;ontologia sui contratti pubblici</dct:description>
        <dct:description xml:lang="en">This is the Italian application profile of the public contract ontology</dct:description>
        <dct:issued rdf:datatype="http://www.w3.org/2001/XMLSchema#date">2018-04-27</dct:issued>
        <dct:language rdf:resource="http://publications.europa.eu/resource/authority/language/ENG"/>
        <dct:language rdf:resource="http://publications.europa.eu/resource/authority/language/ITA"/>
        <dct:modified rdf:datatype="http://www.w3.org/2001/XMLSchema#date">2019-04-23</dct:modified>
        <dct:publisher rdf:resource="http://spcdata.digitpa.gov.it/Amministrazione/agid"/>
        <dct:rightsHolder rdf:resource="http://spcdata.digitpa.gov.it/Amministrazione/cvtiap"/>
        <dct:title xml:lang="it">Ontologia dei Contratti Pubblici - Profilo applicativo italiano</dct:title>
        <dct:title xml:lang="en">Public Contracts ontology - Italian application profile</dct:title>
        <rdfs:comment xml:lang="it">Questa è l&apos;ontologia dei contratti pubblici italiani.</rdfs:comment>
        <rdfs:comment xml:lang="en">This is the ontology of the Italian public contracts.</rdfs:comment>
        <rdfs:isDefinedBy rdf:resource="https://w3id.org/italia/onto/PublicContract"/>
        <rdfs:label xml:lang="en">Italian public contracts ontology</rdfs:label>
        <rdfs:label xml:lang="it">Ontologia dei contratti pubblici italiani</rdfs:label>
        <owl:versionInfo xml:lang="en">Version 0.4- Modified on 23 April 2019 - Refactoring l0:Event in l0:EventOrSituation</owl:versionInfo>
        <owl:versionInfo xml:lang="it">Versione 0.4- Modificata il 23 Aprile 2019 - rifattorizzazione di l0:Event in l0:EventOrSituation</owl:versionInfo>
        <dcat:contactPoint rdf:resource="https://w3id.org/italia/data/contact-point/onto-agid"/>
        <dcat:keyword xml:lang="it">Appalto</dcat:keyword>
        <dcat:keyword xml:lang="it">Bando di gara</dcat:keyword>
        <dcat:keyword xml:lang="it">Contratto Pubblico</dcat:keyword>
        <dcat:keyword xml:lang="it">Gara</dcat:keyword>
        <dcat:keyword xml:lang="it">Procedura di realizzazione</dcat:keyword>
        <dcat:theme rdf:resource="http://publications.europa.eu/resource/authority/data-theme/GOVE"/>
        <admsapit:acronym>PC-AP_IT</admsapit:acronym>
        <admsapit:hasContributor rdf:resource="https://w3id.org/italia/data/organization/public-organization/td"/>
        <admsapit:hasContributor rdf:resource="https://w3id.org/italia/data/organization/support-unit/cnr-Z6HZEH/stlab"/>
        <admsapit:hasFormalityLevel rdf:resource="https://w3id.org/italia/onto/ADMS/Formal"/>
        <admsapit:hasKeyClass rdf:resource="https://w3id.org/italia/onto/PublicContract/Contract"/>
        <admsapit:hasKeyClass rdf:resource="https://w3id.org/italia/onto/PublicContract/Lot"/>
        <admsapit:hasKeyClass rdf:resource="https://w3id.org/italia/onto/PublicContract/Procedure"/>
        <admsapit:hasOntologyLanguage rdf:resource="https://w3id.org/italia/onto/ADMS/OWL"/>
        <admsapit:hasSemanticAssetDistribution rdf:resource="https://w3id.org/italia/data/distribution/PCAPIT-JSON-LD"/>
        <admsapit:hasSemanticAssetDistribution rdf:resource="https://w3id.org/italia/data/distribution/PCAPIT-RDF-TURTLE"/>
        <admsapit:hasSemanticAssetDistribution rdf:resource="https://w3id.org/italia/data/distribution/PCAPIT-RDF-XML"/>
        <admsapit:hasTask rdf:resource="https://w3id.org/italia/onto/ADMS/AnnotationTask"/>
        <admsapit:hasTask rdf:resource="https://w3id.org/italia/onto/ADMS/QueryFormulationTask"/>
        <admsapit:hasTask rdf:resource="https://w3id.org/italia/onto/ADMS/SearchTask"/>
        <admsapit:last rdf:resource="https://w3id.org/italia/onto/PublicContract/0.4"/>
        <admsapit:officialURI rdf:datatype="http://www.w3.org/2001/XMLSchema#anyURI">https://w3id.org/italia/onto/PublicContract</admsapit:officialURI>
        <admsapit:prefix>pcapit</admsapit:prefix>
        <admsapit:semanticAssetInUse rdf:resource="https://w3id.org/italia/data/project/DAF"/>
        <admsapit:semanticAssetInUse rdf:resource="https://w3id.org/italia/data/project/OntoPiA"/>
        <admsapit:status>final draft</admsapit:status>
        <admsapit:target xml:lang="it">Cittadini</admsapit:target>
        <admsapit:target xml:lang="it">Imprese</admsapit:target>
        <admsapit:target xml:lang="it">Pubbliche Amministrazioni</admsapit:target>
        <admsapit:type rdf:resource="https://w3id.org/italia/onto/ADMS/DomainOntology"/>
    </owl:Ontology>
    


    <!-- 
    ///////////////////////////////////////////////////////////////////////////////////////
    //
    // Annotation properties
    //
    ///////////////////////////////////////////////////////////////////////////////////////
     -->

    


    <!-- http://purl.org/dc/elements/1.1/contributor -->

    <owl:AnnotationProperty rdf:about="http://purl.org/dc/elements/1.1/contributor"/>
    


    <!-- http://www.w3.org/ns/prov#wasDerivedFrom -->

    <owl:AnnotationProperty rdf:about="http://www.w3.org/ns/prov#wasDerivedFrom"/>
    


    <!-- http://www.w3.org/ns/prov#wasInfluencedBy -->

    <owl:AnnotationProperty rdf:about="http://www.w3.org/ns/prov#wasInfluencedBy"/>
    


    <!-- https://w3id.org/italia/onto/l0/controlledVocabulary -->

    <owl:AnnotationProperty rdf:about="https://w3id.org/italia/onto/l0/controlledVocabulary"/>
    


    <!-- 
    ///////////////////////////////////////////////////////////////////////////////////////
    //
    // Datatypes
    //
    ///////////////////////////////////////////////////////////////////////////////////////
     -->

    


    <!-- http://www.w3.org/2001/XMLSchema#boolean -->

    <rdfs:Datatype rdf:about="http://www.w3.org/2001/XMLSchema#boolean"/>
    


    <!-- http://www.w3.org/2001/XMLSchema#date -->

    <rdfs:Datatype rdf:about="http://www.w3.org/2001/XMLSchema#date"/>
    


    <!-- http://www.w3.org/2001/XMLSchema#float -->

    <rdfs:Datatype rdf:about="http://www.w3.org/2001/XMLSchema#float"/>
    


    <!-- http://www.w3.org/2001/XMLSchema#string -->

    <rdfs:Datatype rdf:about="http://www.w3.org/2001/XMLSchema#string"/>
    


    <!-- 
    ///////////////////////////////////////////////////////////////////////////////////////
    //
    // Object Properties
    //
    ///////////////////////////////////////////////////////////////////////////////////////
     -->

    


    <!-- https://w3id.org/italia/onto/PublicContract/appliesToLot -->

    <owl:ObjectProperty rdf:about="https://w3id.org/italia/onto/PublicContract/appliesToLot">
        <rdfs:domain rdf:resource="https://w3id.org/italia/onto/PublicContract/Tender"/>
        <rdfs:range rdf:resource="https://w3id.org/italia/onto/PublicContract/Lot"/>
        <rdfs:comment xml:lang="it">Questa proprietà è utilizzata per rappresentare il legame tra l&apos;offerta e il lotto (l&apos;offerta si applica al lotto)</rdfs:comment>
        <rdfs:comment xml:lang="en">This property is used to represent the relationship between a tender to the lot (a tender applies to a lot)</rdfs:comment>
        <rdfs:isDefinedBy rdf:resource="https://w3id.org/italia/onto/PublicContract"/>
        <rdfs:label xml:lang="en">applies to lot</rdfs:label>
        <rdfs:label xml:lang="it">si applica a lotto</rdfs:label>
        <owl:versionInfo xml:lang="it">stabile</owl:versionInfo>
        <owl:versionInfo xml:lang="en">stable</owl:versionInfo>
    </owl:ObjectProperty>
    


    <!-- https://w3id.org/italia/onto/PublicContract/approvedInWPR -->

    <owl:ObjectProperty rdf:about="https://w3id.org/italia/onto/PublicContract/approvedInWPR">
        <owl:inverseOf rdf:resource="https://w3id.org/italia/onto/PublicContract/containsPaymentCertificate"/>
        <rdfs:domain rdf:resource="https://w3id.org/italia/onto/PublicContract/PaymentCertificate"/>
        <rdfs:range rdf:resource="https://w3id.org/italia/onto/PublicContract/WorkProgressReport"/>
        <rdfs:comment xml:lang="it">PEr i Lavori, la proprietà che collega il certificato di pagamento al SAL (Stato Avanzamento Lavori) documento che contiene la delibera al pagamento stesso.</rdfs:comment>
        <rdfs:comment xml:lang="en">The property that links the certificate of payment to the work progress report whereby the payment is approved.</rdfs:comment>
        <rdfs:isDefinedBy rdf:resource="https://w3id.org/italia/onto/PublicContract"/>
        <rdfs:label xml:lang="en">approved in work progress report</rdfs:label>
        <rdfs:label xml:lang="it">deliberato in Stato Avanzamento Lavori</rdfs:label>
        <owl:versionInfo xml:lang="it">stabile</owl:versionInfo>
        <owl:versionInfo xml:lang="en">stable</owl:versionInfo>
    </owl:ObjectProperty>
    


    <!-- https://w3id.org/italia/onto/PublicContract/attachesTenderDocument -->

    <owl:ObjectProperty rdf:about="https://w3id.org/italia/onto/PublicContract/attachesTenderDocument">
        <rdfs:domain rdf:resource="https://w3id.org/italia/onto/PublicContract/Tender"/>
        <rdfs:range rdf:resource="https://w3id.org/italia/onto/PublicContract/TenderDocument"/>
        <rdfs:comment xml:lang="en">Property that links the tender to the tender document</rdfs:comment>
        <rdfs:comment xml:lang="it">Proprietà che lega l&apos;intervento o la fase di presentazione dell&apos;offerta all&apos;offerta</rdfs:comment>
        <rdfs:isDefinedBy rdf:resource="https://w3id.org/italia/onto/PublicContract"/>
        <rdfs:label xml:lang="it">allega offerta</rdfs:label>
        <rdfs:label xml:lang="en">attaches tender document</rdfs:label>
        <owl:versionInfo xml:lang="it">stabile</owl:versionInfo>
        <owl:versionInfo xml:lang="en">stable</owl:versionInfo>
    </owl:ObjectProperty>
    


    <!-- https://w3id.org/italia/onto/PublicContract/changedByProcedureChangeEvent -->

    <owl:ObjectProperty rdf:about="https://w3id.org/italia/onto/PublicContract/changedByProcedureChangeEvent">
        <owl:inverseOf rdf:resource="https://w3id.org/italia/onto/PublicContract/hasOriginalSummary"/>
        <rdfs:domain rdf:resource="https://w3id.org/italia/onto/PublicContract/EconomicSummary"/>
        <rdfs:range rdf:resource="https://w3id.org/italia/onto/PublicContract/ProcedureChangeEvent"/>
        <rdfs:comment xml:lang="it">Questa proprietà è l&apos;inversa di &quot;prospetto economico di origine&quot; e indica un evento che ha contribuito al cambiamento di questo prospetto economico.</rdfs:comment>
        <rdfs:comment xml:lang="en">This property is the inverse of &quot;has original summary&quot; and determines the change event which resulted in a change to this economic summary.</rdfs:comment>
        <rdfs:isDefinedBy rdf:resource="https://w3id.org/italia/onto/PublicContract"/>
        <rdfs:label xml:lang="it">cambiato da evento di cambiamento procedura</rdfs:label>
        <rdfs:label xml:lang="en">changed by procedure change event</rdfs:label>
        <owl:versionInfo xml:lang="it">stabile</owl:versionInfo>
        <owl:versionInfo xml:lang="en">stable</owl:versionInfo>
    </owl:ObjectProperty>
    


    <!-- https://w3id.org/italia/onto/PublicContract/containsPaymentCertificate -->

    <owl:ObjectProperty rdf:about="https://w3id.org/italia/onto/PublicContract/containsPaymentCertificate">
        <rdfs:domain rdf:resource="https://w3id.org/italia/onto/PublicContract/WorkProgressReport"/>
        <rdfs:range rdf:resource="https://w3id.org/italia/onto/PublicContract/PaymentCertificate"/>
        <rdfs:comment xml:lang="en">Inverse property of approvedInWPR that links a work progress report to the payment certificate</rdfs:comment>
        <rdfs:comment xml:lang="it">Proprietà inversa di approvato in SAL che collega il SAL al certificato di pagamento</rdfs:comment>
        <rdfs:isDefinedBy rdf:resource="https://w3id.org/italia/onto/PublicContract"/>
        <rdfs:label xml:lang="en">contains payment certificate</rdfs:label>
        <rdfs:label xml:lang="it">contiene certificato di pagamento</rdfs:label>
        <owl:versionInfo xml:lang="it">stabile</owl:versionInfo>
        <owl:versionInfo xml:lang="en">stable</owl:versionInfo>
    </owl:ObjectProperty>
    


    <!-- https://w3id.org/italia/onto/PublicContract/hasAmendmentRationale -->

    <owl:ObjectProperty rdf:about="https://w3id.org/italia/onto/PublicContract/hasAmendmentRationale">
        <rdfs:domain rdf:resource="https://w3id.org/italia/onto/PublicContract/AmendmentDocument"/>
        <rdfs:range rdf:resource="https://w3id.org/italia/onto/PublicContract/AmendmentRationale"/>
        <rdfs:comment xml:lang="en">Property that links an Amendment document to the rationale behind the modifications</rdfs:comment>
        <rdfs:comment xml:lang="it">Proprietà che collega i documenti di modifca alle motivazioni che hanno portato alle modifiche</rdfs:comment>
        <rdfs:isDefinedBy rdf:resource="https://w3id.org/italia/onto/PublicContract"/>
        <rdfs:label xml:lang="it">ha motivazione della modifica</rdfs:label>
        <rdfs:label xml:lang="en">has amendment rationale</rdfs:label>
        <owl:versionInfo xml:lang="it">stabile</owl:versionInfo>
        <owl:versionInfo xml:lang="en">stable</owl:versionInfo>
    </owl:ObjectProperty>
    


    <!-- https://w3id.org/italia/onto/PublicContract/hasAwardCriterion -->

    <owl:ObjectProperty rdf:about="https://w3id.org/italia/onto/PublicContract/hasAwardCriterion">
        <rdfs:domain rdf:resource="https://w3id.org/italia/onto/PublicContract/Lot"/>
        <rdfs:range rdf:resource="https://w3id.org/italia/onto/PublicContract/AwardCriterion"/>
        <rdfs:comment xml:lang="it">La proprietà che determina il criterio di aggiudicazione del lotto. Tale proprietà fa riferimento a un vocabolario controllato.</rdfs:comment>
        <rdfs:comment xml:lang="en">The property that determines the award criteria of the lot. This property should be used in the case of procedures that include public calls followed by an awarding.</rdfs:comment>
        <rdfs:isDefinedBy rdf:resource="https://w3id.org/italia/onto/PublicContract"/>
        <rdfs:label xml:lang="it">ha criterio di aggiudicazione</rdfs:label>
        <rdfs:label xml:lang="en">has award criterion</rdfs:label>
        <owl:versionInfo xml:lang="it">stabile</owl:versionInfo>
        <owl:versionInfo xml:lang="en">stable</owl:versionInfo>
    </owl:ObjectProperty>
    


    <!-- https://w3id.org/italia/onto/PublicContract/hasAwardNotice -->

    <owl:ObjectProperty rdf:about="https://w3id.org/italia/onto/PublicContract/hasAwardNotice">
        <rdfs:subPropertyOf rdf:resource="https://w3id.org/italia/onto/PublicContract/hasNotice"/>
        <rdfs:domain rdf:resource="https://w3id.org/italia/onto/PublicContract/Lot"/>
        <rdfs:range rdf:resource="https://w3id.org/italia/onto/PublicContract/AwardNotice"/>
        <rdfs:comment xml:lang="it">La proprietà che collega il lotto all&apos;esito dell&apos;aggiudicazione dello stesso.</rdfs:comment>
        <rdfs:comment xml:lang="en">The property that links the lot to its award outcome.</rdfs:comment>
        <rdfs:isDefinedBy rdf:resource="https://w3id.org/italia/onto/PublicContract"/>
        <rdfs:label xml:lang="it">ha avviso di esito di procedura</rdfs:label>
        <rdfs:label xml:lang="en">has award notice</rdfs:label>
        <owl:versionInfo xml:lang="it">stabile</owl:versionInfo>
        <owl:versionInfo xml:lang="en">stable</owl:versionInfo>
    </owl:ObjectProperty>
    


    <!-- https://w3id.org/italia/onto/PublicContract/hasCPV -->

    <owl:ObjectProperty rdf:about="https://w3id.org/italia/onto/PublicContract/hasCPV">
        <rdfs:domain>
            <owl:Class>
                <owl:unionOf rdf:parseType="Collection">
                    <rdf:Description rdf:about="https://w3id.org/italia/onto/PublicContract/Contract"/>
                    <rdf:Description rdf:about="https://w3id.org/italia/onto/PublicContract/Lot"/>
                    <rdf:Description rdf:about="https://w3id.org/italia/onto/PublicContract/Notice"/>
                    <rdf:Description rdf:about="https://w3id.org/italia/onto/PublicContract/Procedure"/>
                </owl:unionOf>
            </owl:Class>
        </rdfs:domain>
        <rdfs:range rdf:resource="https://w3id.org/italia/onto/PublicContract/CPV"/>
        <rdfs:comment xml:lang="it">La proprietà che associa un bando, avviso, lotto o contratto a uno o più identificativi del vocabolario controllato dei CPV (Common Procurement Vocabulary), il sistema di classificazione per gli appalti pubblici. Tali identificativi identificano la categoria merceologica oggetto dell&apos;acquisto</rdfs:comment>
        <rdfs:comment xml:lang="en">The property that links a procedure, notice, lot or contract to the identifier within the controlled vocabulary of CPV (Common Procurement Vocabulary), a code describing the main object of a public procurement contract.</rdfs:comment>
        <rdfs:isDefinedBy rdf:resource="https://w3id.org/italia/onto/PublicContract"/>
        <rdfs:label xml:lang="it">ha CPV</rdfs:label>
        <rdfs:label xml:lang="en">has CPV</rdfs:label>
        <owl:versionInfo xml:lang="it">stabile</owl:versionInfo>
        <owl:versionInfo xml:lang="en">stable</owl:versionInfo>
    </owl:ObjectProperty>
    


    <!-- https://w3id.org/italia/onto/PublicContract/hasCallForCompetition -->

    <owl:ObjectProperty rdf:about="https://w3id.org/italia/onto/PublicContract/hasCallForCompetition">
        <rdfs:subPropertyOf rdf:resource="https://w3id.org/italia/onto/PublicContract/hasNotice"/>
        <rdfs:domain>
            <owl:Class>
                <owl:unionOf rdf:parseType="Collection">
                    <rdf:Description rdf:about="https://w3id.org/italia/onto/PublicContract/ProcurementProject"/>
                    <rdf:Description rdf:about="https://w3id.org/italia/onto/PublicContract/Publication"/>
                </owl:unionOf>
            </owl:Class>
        </rdfs:domain>
        <rdfs:range rdf:resource="https://w3id.org/italia/onto/PublicContract/CallForCompetition"/>
        <rdfs:comment xml:lang="it">La proprietà che indica il collegamento tra il la procedura o la fase di pubblicazione e un bando di gara. Diversi lotti possono fare riferimento ad un medesimo bando.</rdfs:comment>
        <rdfs:comment xml:lang="en">The property that links the procedure  or the publication phase to the related call for tender</rdfs:comment>
        <rdfs:isDefinedBy rdf:resource="https://w3id.org/italia/onto/PublicContract"/>
        <rdfs:label xml:lang="it">ha bando di gara</rdfs:label>
        <rdfs:label xml:lang="en">has call for competition</rdfs:label>
        <owl:versionInfo xml:lang="it">stabile</owl:versionInfo>
        <owl:versionInfo xml:lang="en">stable</owl:versionInfo>
    </owl:ObjectProperty>
    


    <!-- https://w3id.org/italia/onto/PublicContract/hasChangeDocument -->

    <owl:ObjectProperty rdf:about="https://w3id.org/italia/onto/PublicContract/hasChangeDocument">
        <rdfs:domain>
            <owl:Class>
                <owl:unionOf rdf:parseType="Collection">
                    <rdf:Description rdf:about="https://w3id.org/italia/onto/PublicContract/Contract"/>
                    <rdf:Description rdf:about="https://w3id.org/italia/onto/PublicContract/ProcurementProject"/>
                </owl:unionOf>
            </owl:Class>
        </rdfs:domain>
        <rdfs:range rdf:resource="https://w3id.org/italia/onto/PublicContract/AmendmentDocument"/>
        <rdfs:comment xml:lang="it">La proprietà che indica il documento che descrive una modifica alle caratteristiche di un Lotto o Contratto.</rdfs:comment>
        <rdfs:comment xml:lang="en">The property that determines the document describing a change to the characteristics of a lot or contract.</rdfs:comment>
        <rdfs:isDefinedBy rdf:resource="https://w3id.org/italia/onto/PublicContract"/>
        <rdfs:label xml:lang="it">ha documento di modifica</rdfs:label>
        <rdfs:label xml:lang="en">has change document</rdfs:label>
        <owl:versionInfo xml:lang="it">stabile</owl:versionInfo>
        <owl:versionInfo xml:lang="en">stable</owl:versionInfo>
    </owl:ObjectProperty>
    


    <!-- https://w3id.org/italia/onto/PublicContract/hasContract -->

    <owl:ObjectProperty rdf:about="https://w3id.org/italia/onto/PublicContract/hasContract">
        <rdfs:domain rdf:resource="https://w3id.org/italia/onto/PublicContract/Lot"/>
        <rdfs:range rdf:resource="https://w3id.org/italia/onto/PublicContract/Contract"/>
        <rdfs:comment xml:lang="it">La proprietà che determina il legame tra il lotto e il relativo contratto.</rdfs:comment>
        <rdfs:comment xml:lang="en">The property that determines the link between a contract and the relative lot.</rdfs:comment>
        <rdfs:isDefinedBy rdf:resource="https://w3id.org/italia/onto/PublicContract"/>
        <rdfs:label xml:lang="it">ha contratto</rdfs:label>
        <rdfs:label xml:lang="en">has contract</rdfs:label>
        <owl:versionInfo xml:lang="it">stabile</owl:versionInfo>
        <owl:versionInfo xml:lang="en">stable</owl:versionInfo>
    </owl:ObjectProperty>
    


    <!-- https://w3id.org/italia/onto/PublicContract/hasContractualResolution -->

    <owl:ObjectProperty rdf:about="https://w3id.org/italia/onto/PublicContract/hasContractualResolution">
        <rdfs:domain rdf:resource="https://w3id.org/italia/onto/PublicContract/Contract"/>
        <rdfs:range rdf:resource="https://w3id.org/italia/onto/PublicContract/Resolution"/>
        <rdfs:comment xml:lang="it">La proprietà che collega il contratto all&apos;evento che determina la risoluzione del contatto stesso</rdfs:comment>
        <rdfs:comment xml:lang="en">The property that links the contract to the event that determines its resolution.</rdfs:comment>
        <rdfs:isDefinedBy rdf:resource="https://w3id.org/italia/onto/PublicContract"/>
        <rdfs:label xml:lang="it">ha rescissione contrattuale</rdfs:label>
        <rdfs:label xml:lang="en">has contractual resolution</rdfs:label>
        <owl:versionInfo xml:lang="it">stabile</owl:versionInfo>
        <owl:versionInfo xml:lang="en">stable</owl:versionInfo>
    </owl:ObjectProperty>
    


    <!-- https://w3id.org/italia/onto/PublicContract/hasEconomicSummary -->

    <owl:ObjectProperty rdf:about="https://w3id.org/italia/onto/PublicContract/hasEconomicSummary">
        <rdfs:domain>
            <owl:Class>
                <owl:unionOf rdf:parseType="Collection">
                    <rdf:Description rdf:about="https://w3id.org/italia/onto/PublicContract/Contract"/>
                    <rdf:Description rdf:about="https://w3id.org/italia/onto/PublicContract/ProcurementProject"/>
                </owl:unionOf>
            </owl:Class>
        </rdfs:domain>
        <rdfs:range rdf:resource="https://w3id.org/italia/onto/PublicContract/EconomicSummary"/>
        <rdfs:comment xml:lang="it">Questa proprietà indica il prospetto economico di un lotto o contratto.</rdfs:comment>
        <rdfs:comment xml:lang="en">This property represents the economic summary of a lot or contract.</rdfs:comment>
        <rdfs:isDefinedBy rdf:resource="https://w3id.org/italia/onto/PublicContract"/>
        <rdfs:label xml:lang="it">ha prospetto economico</rdfs:label>
        <rdfs:label xml:lang="en">has economic summary</rdfs:label>
        <owl:versionInfo xml:lang="it">stabile</owl:versionInfo>
        <owl:versionInfo xml:lang="en">stable</owl:versionInfo>
    </owl:ObjectProperty>
    


    <!-- https://w3id.org/italia/onto/PublicContract/hasFrameworkAgreement -->

    <owl:ObjectProperty rdf:about="https://w3id.org/italia/onto/PublicContract/hasFrameworkAgreement">
        <rdfs:domain>
            <owl:Class>
                <owl:unionOf rdf:parseType="Collection">
                    <rdf:Description rdf:about="https://w3id.org/italia/onto/PublicContract/Contract"/>
                    <rdf:Description rdf:about="https://w3id.org/italia/onto/PublicContract/Procedure"/>
                </owl:unionOf>
            </owl:Class>
        </rdfs:domain>
        <rdfs:range rdf:resource="https://w3id.org/italia/onto/PublicContract/FrameworkAgreement"/>
        <rdfs:comment xml:lang="it">La proprietà che lega un&apos;istanza di procedura di realizzazione a un accordo quadro o convenzione.</rdfs:comment>
        <rdfs:comment xml:lang="en">The properties that links the procedure to its framework agreement.</rdfs:comment>
        <rdfs:isDefinedBy rdf:resource="https://w3id.org/italia/onto/PublicContract"/>
        <rdfs:label xml:lang="it">ha accordo quadro</rdfs:label>
        <rdfs:label xml:lang="en">has framework agreement</rdfs:label>
        <owl:versionInfo xml:lang="it">stabile</owl:versionInfo>
        <owl:versionInfo xml:lang="en">stable</owl:versionInfo>
    </owl:ObjectProperty>
    


    <!-- https://w3id.org/italia/onto/PublicContract/hasNotice -->

    <owl:ObjectProperty rdf:about="https://w3id.org/italia/onto/PublicContract/hasNotice">
        <rdfs:subPropertyOf rdf:resource="https://w3id.org/italia/onto/PublicContract/hasProcurementDocument"/>
        <rdfs:domain rdf:resource="https://w3id.org/italia/onto/PublicContract/ProcurementProject"/>
        <rdfs:range rdf:resource="https://w3id.org/italia/onto/PublicContract/Notice"/>
        <rdfs:comment xml:lang="en">Property that links a procedure or lot with a notice</rdfs:comment>
        <rdfs:comment xml:lang="it">Proprietà che lega una gara o lotto con un avviso</rdfs:comment>
        <rdfs:isDefinedBy rdf:resource="https://w3id.org/italia/onto/PublicContract"/>
        <rdfs:label xml:lang="it">ha avviso</rdfs:label>
        <rdfs:label xml:lang="en">has notice</rdfs:label>
        <owl:versionInfo xml:lang="it">stabile</owl:versionInfo>
        <owl:versionInfo xml:lang="en">stable</owl:versionInfo>
    </owl:ObjectProperty>
    


    <!-- https://w3id.org/italia/onto/PublicContract/hasNoticeType -->

    <owl:ObjectProperty rdf:about="https://w3id.org/italia/onto/PublicContract/hasNoticeType">
        <rdfs:domain rdf:resource="https://w3id.org/italia/onto/PublicContract/Notice"/>
        <rdfs:range rdf:resource="https://w3id.org/italia/onto/PublicContract/NoticeType"/>
        <rdfs:comment xml:lang="it">La proprietà che indica il tipo di bando.</rdfs:comment>
        <rdfs:comment xml:lang="en">The property that links a notice to its type.</rdfs:comment>
        <rdfs:isDefinedBy rdf:resource="https://w3id.org/italia/onto/PublicContract"/>
        <rdfs:label xml:lang="it">ha tipo di bando</rdfs:label>
        <rdfs:label xml:lang="en">has notice type</rdfs:label>
        <owl:versionInfo xml:lang="it">stabile</owl:versionInfo>
        <owl:versionInfo xml:lang="en">stable</owl:versionInfo>
    </owl:ObjectProperty>
    


    <!-- https://w3id.org/italia/onto/PublicContract/hasOriginalSummary -->

    <owl:ObjectProperty rdf:about="https://w3id.org/italia/onto/PublicContract/hasOriginalSummary">
        <rdfs:domain rdf:resource="https://w3id.org/italia/onto/PublicContract/ProcedureChangeEvent"/>
        <rdfs:range rdf:resource="https://w3id.org/italia/onto/PublicContract/EconomicSummary"/>
        <rdfs:comment xml:lang="it">Questa proprietà è l&apos;inversa di &quot;cambiata da&quot; e collega un evento di cambiamento al prospetto economico precedente al cambiamento stesso.</rdfs:comment>
        <rdfs:comment xml:lang="en">This property is the inverse of &quot;changed by&quot; and links a change event to the economic summary preceding the change event.</rdfs:comment>
        <rdfs:isDefinedBy rdf:resource="https://w3id.org/italia/onto/PublicContract"/>
        <rdfs:label xml:lang="it">ha prospetto economico di origine</rdfs:label>
        <rdfs:label xml:lang="en">has original summary</rdfs:label>
        <owl:versionInfo xml:lang="it">stabile</owl:versionInfo>
        <owl:versionInfo xml:lang="en">stable</owl:versionInfo>
    </owl:ObjectProperty>
    


    <!-- https://w3id.org/italia/onto/PublicContract/hasPaymentCertificate -->

    <owl:ObjectProperty rdf:about="https://w3id.org/italia/onto/PublicContract/hasPaymentCertificate">
        <rdfs:domain rdf:resource="https://w3id.org/italia/onto/PublicContract/Lot"/>
        <rdfs:range rdf:resource="https://w3id.org/italia/onto/PublicContract/PaymentCertificate"/>
        <rdfs:comment xml:lang="it">La proprietà che collega il lotto al certificato di pagamento. Per i lavori il certifcato di pagamento viene deliberato nel SAL.</rdfs:comment>
        <rdfs:comment xml:lang="en">The property that links the lot to the certificate of payment approved by the related progress of work report.</rdfs:comment>
        <rdfs:isDefinedBy rdf:resource="https://w3id.org/italia/onto/PublicContract"/>
        <rdfs:label xml:lang="it">ha certificato di pagamento</rdfs:label>
        <rdfs:label xml:lang="en">has certificate of payment</rdfs:label>
        <owl:versionInfo xml:lang="it">stabile</owl:versionInfo>
        <owl:versionInfo xml:lang="en">stable</owl:versionInfo>
    </owl:ObjectProperty>
    


    <!-- https://w3id.org/italia/onto/PublicContract/hasProcedureType -->

    <owl:ObjectProperty rdf:about="https://w3id.org/italia/onto/PublicContract/hasProcedureType">
        <rdfs:domain rdf:resource="https://w3id.org/italia/onto/PublicContract/Procedure"/>
        <rdfs:range rdf:resource="https://w3id.org/italia/onto/PublicContract/ProcedureType"/>
        <rdfs:comment xml:lang="it">La proprietà che specifica il tipo di procedura di affidamento di un lotto.</rdfs:comment>
        <rdfs:comment xml:lang="en">The property that links the procedure to its type.</rdfs:comment>
        <rdfs:isDefinedBy rdf:resource="https://w3id.org/italia/onto/PublicContract"/>
        <rdfs:label xml:lang="it">ha modalità di scelta contraente</rdfs:label>
        <rdfs:label xml:lang="en">has type of procedure</rdfs:label>
        <owl:versionInfo xml:lang="it">stabile</owl:versionInfo>
        <owl:versionInfo xml:lang="en">stable</owl:versionInfo>
    </owl:ObjectProperty>
    


    <!-- https://w3id.org/italia/onto/PublicContract/hasProcurementDocument -->

    <owl:ObjectProperty rdf:about="https://w3id.org/italia/onto/PublicContract/hasProcurementDocument">
        <rdfs:domain rdf:resource="https://w3id.org/italia/onto/PublicContract/ProcurementProject"/>
        <rdfs:range rdf:resource="https://w3id.org/italia/onto/PublicContract/ProcurementDocument"/>
        <rdfs:comment xml:lang="it">La proprietà che indica gli atti emessi dalla stazione appaltante nell&apos;espletamento di un progetto di approvigionamento.</rdfs:comment>
        <rdfs:comment xml:lang="en">The properties that links the procurement project to the documents issued by the contracting authority during the course of the procedure.</rdfs:comment>
        <rdfs:isDefinedBy rdf:resource="https://w3id.org/italia/onto/PublicContract"/>
        <rdfs:label xml:lang="it">ha atto di approvigionamento</rdfs:label>
        <rdfs:label xml:lang="it">has procurement document</rdfs:label>
        <owl:versionInfo xml:lang="it">stabile</owl:versionInfo>
        <owl:versionInfo xml:lang="en">stable</owl:versionInfo>
    </owl:ObjectProperty>
    


    <!-- https://w3id.org/italia/onto/PublicContract/hasProcuringEntity -->

    <owl:ObjectProperty rdf:about="https://w3id.org/italia/onto/PublicContract/hasProcuringEntity">
        <rdfs:domain rdf:resource="https://w3id.org/italia/onto/PublicContract/Procedure"/>
        <rdfs:range rdf:resource="https://w3id.org/italia/onto/l0/Agent"/>
        <rdfs:comment xml:lang="it">La proprietà che indica l&apos;istituzione che emette il contratto pubblico, riceve le offerte e sceglie il fornitore idoneo sulla base delle condizioni definite dal contratto.</rdfs:comment>
        <rdfs:comment xml:lang="en">The property that determines the institution which issues a public contract, receives tenders and chooses a suitable supplier on the base of the conditions given by the contract.</rdfs:comment>
        <rdfs:isDefinedBy rdf:resource="https://w3id.org/italia/onto/PublicContract"/>
        <rdfs:label xml:lang="it">ha stazione appaltante</rdfs:label>
        <rdfs:label xml:lang="en">has procuring entity</rdfs:label>
        <owl:versionInfo xml:lang="it">stabile</owl:versionInfo>
        <owl:versionInfo xml:lang="en">stable</owl:versionInfo>
    </owl:ObjectProperty>
    


    <!-- https://w3id.org/italia/onto/PublicContract/hasResolutionToContract -->

    <owl:ObjectProperty rdf:about="https://w3id.org/italia/onto/PublicContract/hasResolutionToContract">
        <rdfs:subPropertyOf rdf:resource="https://w3id.org/italia/onto/PublicContract/hasProcurementDocument"/>
        <rdfs:domain rdf:resource="https://w3id.org/italia/onto/PublicContract/Procedure"/>
        <rdfs:range rdf:resource="https://w3id.org/italia/onto/PublicContract/ResolutionToContract"/>
        <rdfs:comment xml:lang="it">La proprietà che determina il legame tra la procedura di realizzazione e una determina a contrarre relativa.</rdfs:comment>
        <rdfs:comment xml:lang="en">The property that links the procedure to the document whereby the contracting authority expresses its resoultion to contract.</rdfs:comment>
        <rdfs:isDefinedBy rdf:resource="https://w3id.org/italia/onto/PublicContract"/>
        <rdfs:label xml:lang="it">ha determina a contrarre</rdfs:label>
        <rdfs:label xml:lang="en">has decision to contract</rdfs:label>
        <owl:versionInfo xml:lang="it">stabile</owl:versionInfo>
        <owl:versionInfo xml:lang="en">stable</owl:versionInfo>
    </owl:ObjectProperty>
    


    <!-- https://w3id.org/italia/onto/PublicContract/hasResultingSummary -->

    <owl:ObjectProperty rdf:about="https://w3id.org/italia/onto/PublicContract/hasResultingSummary">
        <owl:inverseOf rdf:resource="https://w3id.org/italia/onto/PublicContract/resultedFrom"/>
        <rdfs:domain rdf:resource="https://w3id.org/italia/onto/PublicContract/ProcedureChangeEvent"/>
        <rdfs:range rdf:resource="https://w3id.org/italia/onto/PublicContract/EconomicSummary"/>
        <rdfs:comment xml:lang="it">Questa proprietà è l&apos;inversa di &quot;risultante da&quot; e indica un prospetto economico creato o ridefinito in seguito a un evento di cambiamento.</rdfs:comment>
        <rdfs:comment xml:lang="en">This property is the inverse of &quot;resulted from&quot; and determines the economic summary which was created or changed as a result of the change event.</rdfs:comment>
        <rdfs:isDefinedBy rdf:resource="https://w3id.org/italia/onto/PublicContract"/>
        <rdfs:label xml:lang="it">ha prospetto risultante</rdfs:label>
        <rdfs:label xml:lang="en">has resulting summary</rdfs:label>
        <owl:versionInfo xml:lang="it">stabile</owl:versionInfo>
        <owl:versionInfo xml:lang="en">stable</owl:versionInfo>
    </owl:ObjectProperty>
    


    <!-- https://w3id.org/italia/onto/PublicContract/hasWorkProgressReport -->

    <owl:ObjectProperty rdf:about="https://w3id.org/italia/onto/PublicContract/hasWorkProgressReport">
        <rdfs:domain rdf:resource="https://w3id.org/italia/onto/PublicContract/Lot"/>
        <rdfs:range rdf:resource="https://w3id.org/italia/onto/PublicContract/WorkProgressReport"/>
        <rdfs:comment xml:lang="it">La proprietà che collega il lotto al documento che ne certifica lo Stato di Avanzamento Lavori (SAL).</rdfs:comment>
        <rdfs:comment xml:lang="en">The property that links the lot to its work progress report.</rdfs:comment>
        <rdfs:isDefinedBy rdf:resource="https://w3id.org/italia/onto/PublicContract"/>
        <rdfs:label xml:lang="it">ha SAL (Stato Avanzamento Lavori)</rdfs:label>
        <rdfs:label xml:lang="en">has work progress report</rdfs:label>
        <owl:versionInfo xml:lang="it">stabile</owl:versionInfo>
        <owl:versionInfo xml:lang="en">stable</owl:versionInfo>
    </owl:ObjectProperty>
    


    <!-- https://w3id.org/italia/onto/PublicContract/includesLot -->

    <owl:ObjectProperty rdf:about="https://w3id.org/italia/onto/PublicContract/includesLot">
        <owl:inverseOf rdf:resource="https://w3id.org/italia/onto/PublicContract/isIncludedInProcedure"/>
        <rdfs:domain rdf:resource="https://w3id.org/italia/onto/PublicContract/Procedure"/>
        <rdfs:range rdf:resource="https://w3id.org/italia/onto/PublicContract/Lot"/>
        <rdfs:comment xml:lang="en">Property that links a procedure to the lot. A procedure has at least a lot</rdfs:comment>
        <rdfs:comment xml:lang="it">Proprietà che collega una procedura a un lotto. Una procedura ha almeno un lotto.</rdfs:comment>
        <rdfs:isDefinedBy rdf:resource="https://w3id.org/italia/onto/PublicContract"/>
        <rdfs:label xml:lang="it">include lotto</rdfs:label>
        <rdfs:label xml:lang="en">includes lot</rdfs:label>
        <owl:versionInfo xml:lang="it">stabile</owl:versionInfo>
        <owl:versionInfo xml:lang="en">stable</owl:versionInfo>
    </owl:ObjectProperty>
    


    <!-- https://w3id.org/italia/onto/PublicContract/isIncludedInProcedure -->

    <owl:ObjectProperty rdf:about="https://w3id.org/italia/onto/PublicContract/isIncludedInProcedure">
        <rdfs:domain rdf:resource="https://w3id.org/italia/onto/PublicContract/Lot"/>
        <rdfs:range rdf:resource="https://w3id.org/italia/onto/PublicContract/Procedure"/>
        <rdfs:comment xml:lang="en">Inverse property of &quot;includes lot&quot; that links a lot to its procedure</rdfs:comment>
        <rdfs:comment xml:lang="it">Proprietà inversa di &quot;include lotto&quot; che lega il lotto alla sua procedura</rdfs:comment>
        <rdfs:isDefinedBy rdf:resource="https://w3id.org/italia/onto/PublicContract"/>
        <rdfs:label xml:lang="en">is included in Procedure</rdfs:label>
        <rdfs:label xml:lang="it">è incluso in procedura</rdfs:label>
        <owl:versionInfo xml:lang="it">stabile</owl:versionInfo>
        <owl:versionInfo xml:lang="en">stable</owl:versionInfo>
    </owl:ObjectProperty>
    


    <!-- https://w3id.org/italia/onto/PublicContract/isPrimaryTopicOf -->

    <owl:ObjectProperty rdf:about="https://w3id.org/italia/onto/PublicContract/isPrimaryTopicOf">
        <rdfs:domain>
            <owl:Class>
                <owl:unionOf rdf:parseType="Collection">
                    <rdf:Description rdf:about="https://w3id.org/italia/onto/PublicContract/ProcedureChangeEvent"/>
                    <rdf:Description rdf:about="https://w3id.org/italia/onto/PublicContract/Resolution"/>
                </owl:unionOf>
            </owl:Class>
        </rdfs:domain>
        <rdfs:range rdf:resource="https://w3id.org/italia/onto/PublicContract/AmendmentDocument"/>
        <rdfs:comment xml:lang="it">La proprietà che collega un evento (per esempio un evento di cambiamento del propetto economico, oppure un evento di risoluzione di un contratto) al documento di modifica che ne descrive le caratteristiche.</rdfs:comment>
        <rdfs:comment xml:lang="en">The property that links an event (e.g., an event that modifies the economic summary of a procedure or the event that determines the resolution of a contract) to the document describing the characteristics of the event.</rdfs:comment>
        <rdfs:isDefinedBy rdf:resource="https://w3id.org/italia/onto/PublicContract"/>
        <rdfs:label xml:lang="en">is primary topic of</rdfs:label>
        <rdfs:label xml:lang="it">è argomento principale di</rdfs:label>
        <owl:versionInfo xml:lang="it">stabile</owl:versionInfo>
        <owl:versionInfo xml:lang="en">stable</owl:versionInfo>
    </owl:ObjectProperty>
    


    <!-- https://w3id.org/italia/onto/PublicContract/refersToTender -->

    <owl:ObjectProperty rdf:about="https://w3id.org/italia/onto/PublicContract/refersToTender">
        <rdfs:domain>
            <owl:Class>
                <owl:unionOf rdf:parseType="Collection">
                    <rdf:Description rdf:about="https://w3id.org/italia/onto/PublicContract/Contract"/>
                    <rdf:Description rdf:about="https://w3id.org/italia/onto/PublicContract/TenderDocument"/>
                </owl:unionOf>
            </owl:Class>
        </rdfs:domain>
        <rdfs:range rdf:resource="https://w3id.org/italia/onto/PublicContract/Tender"/>
        <rdfs:comment xml:lang="en">Property that links a tender document or contract to the tender</rdfs:comment>
        <rdfs:comment xml:lang="it">Proprietà che lega il documento di offerta o il contratto all&apos;offerta</rdfs:comment>
        <rdfs:isDefinedBy rdf:resource="https://w3id.org/italia/onto/PublicContract"/>
        <rdfs:label xml:lang="en">refers to tender</rdfs:label>
        <rdfs:label xml:lang="it">si riferisce all&apos;offerta</rdfs:label>
        <owl:versionInfo xml:lang="it">stabile</owl:versionInfo>
        <owl:versionInfo xml:lang="en">stable</owl:versionInfo>
    </owl:ObjectProperty>
    


    <!-- https://w3id.org/italia/onto/PublicContract/relatedToLot -->

    <owl:ObjectProperty rdf:about="https://w3id.org/italia/onto/PublicContract/relatedToLot">
        <rdfs:domain>
            <owl:Class>
                <owl:unionOf rdf:parseType="Collection">
                    <rdf:Description rdf:about="https://w3id.org/italia/onto/PublicContract/Inspection"/>
                    <rdf:Description rdf:about="https://w3id.org/italia/onto/PublicContract/Payment"/>
                </owl:unionOf>
            </owl:Class>
        </rdfs:domain>
        <rdfs:range rdf:resource="https://w3id.org/italia/onto/PublicContract/Lot"/>
        <rdfs:comment xml:lang="it">Property that links the inspection and payment phases to the lot</rdfs:comment>
        <rdfs:comment xml:lang="it">Proprietà che lega le fasi del collaudo e del pagamento a un lotto</rdfs:comment>
        <rdfs:isDefinedBy rdf:resource="https://w3id.org/italia/onto/PublicContract"/>
        <rdfs:label xml:lang="en">related to contract</rdfs:label>
        <rdfs:label xml:lang="it">relativo a contratto</rdfs:label>
        <owl:versionInfo xml:lang="it">stabile</owl:versionInfo>
        <owl:versionInfo xml:lang="en">stable</owl:versionInfo>
    </owl:ObjectProperty>
    


    <!-- https://w3id.org/italia/onto/PublicContract/resolutionReason -->

    <owl:ObjectProperty rdf:about="https://w3id.org/italia/onto/PublicContract/resolutionReason">
        <rdfs:subPropertyOf rdf:resource="https://w3id.org/italia/onto/PublicContract/hasAmendmentRationale"/>
        <rdfs:domain rdf:resource="https://w3id.org/italia/onto/PublicContract/ResolutionDocument"/>
        <rdfs:range rdf:resource="https://w3id.org/italia/onto/PublicContract/ResolutionReason"/>
        <rdfs:comment xml:lang="it">La proprietà che collega la risoluzione del contratto all&apos;identificativo nel vocabolario controllato delle motivazioni delle risoluzioni.</rdfs:comment>
        <rdfs:comment xml:lang="en">The property that links the resolution to the identifier within the controlled vocabulary of resolution reasons.</rdfs:comment>
        <rdfs:isDefinedBy rdf:resource="https://w3id.org/italia/onto/PublicContract"/>
        <rdfs:label xml:lang="it">ha motivazione della risoluzione</rdfs:label>
        <rdfs:label xml:lang="en">has resolution motivation</rdfs:label>
        <owl:versionInfo xml:lang="it">stabile</owl:versionInfo>
        <owl:versionInfo xml:lang="en">stable</owl:versionInfo>
    </owl:ObjectProperty>
    


    <!-- https://w3id.org/italia/onto/PublicContract/resultedFrom -->

    <owl:ObjectProperty rdf:about="https://w3id.org/italia/onto/PublicContract/resultedFrom">
        <rdfs:domain rdf:resource="https://w3id.org/italia/onto/PublicContract/EconomicSummary"/>
        <rdfs:range rdf:resource="https://w3id.org/italia/onto/PublicContract/ProcedureChangeEvent"/>
        <rdfs:comment xml:lang="it">Questa proprietà è l&apos;inversa di &quot;prospetto risultante&quot; e lega un prospetto economico all&apos;evento di cambiamento che lo ha ridefinito.</rdfs:comment>
        <rdfs:comment xml:lang="en">This property is the inverse of &quot;has resulting summary&quot; and links an economic summary to the change event that ridefined it.</rdfs:comment>
        <rdfs:isDefinedBy rdf:resource="https://w3id.org/italia/onto/PublicContract"/>
        <rdfs:label xml:lang="en">resulted from</rdfs:label>
        <rdfs:label xml:lang="it">risultante da</rdfs:label>
        <owl:versionInfo xml:lang="it">stabile</owl:versionInfo>
        <owl:versionInfo xml:lang="en">stable</owl:versionInfo>
    </owl:ObjectProperty>
    


    <!-- https://w3id.org/italia/onto/PublicContract/selectedTender -->

    <owl:ObjectProperty rdf:about="https://w3id.org/italia/onto/PublicContract/selectedTender">
        <rdfs:domain>
            <owl:Class>
                <owl:unionOf rdf:parseType="Collection">
                    <rdf:Description rdf:about="https://w3id.org/italia/onto/PublicContract/Award"/>
                    <rdf:Description rdf:about="https://w3id.org/italia/onto/PublicContract/AwardNotice"/>
                </owl:unionOf>
            </owl:Class>
        </rdfs:domain>
        <rdfs:range rdf:resource="https://w3id.org/italia/onto/PublicContract/Tender"/>
        <rdfs:comment xml:lang="it">La proprietà che indica l&apos;offerta selezionata, in seguito a un processo di aggiudicazione.</rdfs:comment>
        <rdfs:comment xml:lang="en">The property that determines the selected tender submitted by a tenderer.</rdfs:comment>
        <rdfs:isDefinedBy rdf:resource="https://w3id.org/italia/onto/PublicContract"/>
        <rdfs:label xml:lang="it">ha offerta selezionata</rdfs:label>
        <rdfs:label xml:lang="en">has selected tender</rdfs:label>
        <owl:versionInfo xml:lang="it">stabile</owl:versionInfo>
        <owl:versionInfo xml:lang="en">stable</owl:versionInfo>
    </owl:ObjectProperty>
    


    <!-- https://w3id.org/italia/onto/PublicContract/submittedDuring -->

    <owl:ObjectProperty rdf:about="https://w3id.org/italia/onto/PublicContract/submittedDuring">
        <rdfs:domain rdf:resource="https://w3id.org/italia/onto/PublicContract/Tender"/>
        <rdfs:range rdf:resource="https://w3id.org/italia/onto/PublicContract/TenderSubmission"/>
        <rdfs:comment xml:lang="en">Property that links the tender to the tender submission event/phase</rdfs:comment>
        <rdfs:comment xml:lang="it">Proprietà che collega una offerta alla fase (o evento) di presentazione dell&apos;offerta.</rdfs:comment>
        <rdfs:isDefinedBy rdf:resource="https://w3id.org/italia/onto/PublicContract"/>
        <rdfs:label xml:lang="it">presentata durante</rdfs:label>
        <rdfs:label xml:lang="en">submitted during</rdfs:label>
        <owl:versionInfo xml:lang="it">stabile</owl:versionInfo>
        <owl:versionInfo xml:lang="en">stable</owl:versionInfo>
    </owl:ObjectProperty>
    


    <!-- https://w3id.org/italia/onto/PublicContract/suspensionReason -->

    <owl:ObjectProperty rdf:about="https://w3id.org/italia/onto/PublicContract/suspensionReason">
        <rdfs:subPropertyOf rdf:resource="https://w3id.org/italia/onto/PublicContract/hasAmendmentRationale"/>
        <rdfs:domain rdf:resource="https://w3id.org/italia/onto/PublicContract/SuspensionDocument"/>
        <rdfs:range rdf:resource="https://w3id.org/italia/onto/PublicContract/SuspensionReason"/>
        <rdfs:comment xml:lang="it">La proprietà che collega la sospensione all&apos;dentificativo nel vocabolario controllato delle motivazioni delle sospensioni.</rdfs:comment>
        <rdfs:comment xml:lang="en">The property that links the suspension to the identifier within the controlled vocabulary of suspension reasons.</rdfs:comment>
        <rdfs:isDefinedBy rdf:resource="https://w3id.org/italia/onto/PublicContract"/>
        <rdfs:label xml:lang="it">ha motivazione della sospensione</rdfs:label>
        <rdfs:label xml:lang="en">has suspension reason</rdfs:label>
        <owl:versionInfo xml:lang="it">stabile</owl:versionInfo>
        <owl:versionInfo xml:lang="en">stable</owl:versionInfo>
    </owl:ObjectProperty>
    


    <!-- https://w3id.org/italia/onto/PublicContract/tenderer -->

    <owl:ObjectProperty rdf:about="https://w3id.org/italia/onto/PublicContract/tenderer">
        <rdfs:domain rdf:resource="https://w3id.org/italia/onto/PublicContract/Tender"/>
        <rdfs:range rdf:resource="https://w3id.org/italia/onto/l0/Agent"/>
        <rdfs:comment xml:lang="it">La proprietà che indica l&apos;organizzazione offerente di un&apos;offerta.</rdfs:comment>
        <rdfs:comment xml:lang="en">The property that links the tender to its tenderer.</rdfs:comment>
        <rdfs:isDefinedBy rdf:resource="https://w3id.org/italia/onto/PublicContract"/>
        <rdfs:label xml:lang="it">offerente</rdfs:label>
        <rdfs:label xml:lang="en">tenderer</rdfs:label>
        <owl:versionInfo xml:lang="it">stabile</owl:versionInfo>
        <owl:versionInfo xml:lang="en">stable</owl:versionInfo>
    </owl:ObjectProperty>
    


    <!-- https://w3id.org/italia/onto/PublicContract/variantReason -->

    <owl:ObjectProperty rdf:about="https://w3id.org/italia/onto/PublicContract/variantReason">
        <rdfs:subPropertyOf rdf:resource="https://w3id.org/italia/onto/PublicContract/hasAmendmentRationale"/>
        <rdfs:domain rdf:resource="https://w3id.org/italia/onto/PublicContract/VariantDocument"/>
        <rdfs:range rdf:resource="https://w3id.org/italia/onto/PublicContract/VariantReason"/>
        <rdfs:comment xml:lang="it">La proprietà che collega la variante all&apos;identificativo nel vocabolario controllato delle motivazioni delle varianti.</rdfs:comment>
        <rdfs:comment xml:lang="en">The property that links the variant to the identifier within the controlled vocabulary of variant reasons.</rdfs:comment>
        <rdfs:isDefinedBy rdf:resource="https://w3id.org/italia/onto/PublicContract"/>
        <rdfs:label xml:lang="it">ha motivazione della variante</rdfs:label>
        <rdfs:label xml:lang="en">has variant reason</rdfs:label>
        <owl:versionInfo xml:lang="it">stabile</owl:versionInfo>
        <owl:versionInfo xml:lang="en">stable</owl:versionInfo>
    </owl:ObjectProperty>
    


    <!-- https://w3id.org/italia/onto/PublicContract/winner -->

    <owl:ObjectProperty rdf:about="https://w3id.org/italia/onto/PublicContract/winner">
        <rdfs:domain>
            <owl:Class>
                <owl:unionOf rdf:parseType="Collection">
                    <rdf:Description rdf:about="https://w3id.org/italia/onto/PublicContract/AwardNotice"/>
                    <rdf:Description rdf:about="https://w3id.org/italia/onto/PublicContract/Contract"/>
                </owl:unionOf>
            </owl:Class>
        </rdfs:domain>
        <rdfs:range rdf:resource="https://w3id.org/italia/onto/l0/Agent"/>
        <rdfs:comment xml:lang="en">Property that identifies the winner and that links the award notice or contract  to the agent who won the tender</rdfs:comment>
        <rdfs:comment xml:lang="it">Proprietà che identifica il vincitore e che lega pertanto la notifica di ggiudicazione o il contratto con l&apos;agente (tipicamente organizzazione) che ha vinto la gara</rdfs:comment>
        <rdfs:isDefinedBy rdf:resource="https://w3id.org/italia/onto/PublicContract"/>
        <rdfs:label xml:lang="it">vincitore</rdfs:label>
        <rdfs:label xml:lang="en">winner</rdfs:label>
        <owl:versionInfo xml:lang="it">stabile</owl:versionInfo>
        <owl:versionInfo xml:lang="en">stable</owl:versionInfo>
    </owl:ObjectProperty>
    


    <!-- 
    ///////////////////////////////////////////////////////////////////////////////////////
    //
    // Data properties
    //
    ///////////////////////////////////////////////////////////////////////////////////////
     -->

    


    <!-- https://w3id.org/italia/onto/PublicContract/CIG -->

    <owl:DatatypeProperty rdf:about="https://w3id.org/italia/onto/PublicContract/CIG">
        <rdfs:subPropertyOf rdf:resource="https://w3id.org/italia/onto/l0/identifier"/>
        <rdfs:domain rdf:resource="https://w3id.org/italia/onto/PublicContract/Lot"/>
        <rdfs:range rdf:resource="http://www.w3.org/2001/XMLSchema#string"/>
        <rdfs:comment xml:lang="en">Property that identifies the unique code of the lot</rdfs:comment>
        <rdfs:comment xml:lang="it">Proprietà che identifica il CIG</rdfs:comment>
        <rdfs:isDefinedBy rdf:resource="https://w3id.org/italia/onto/PublicContract"/>
        <rdfs:label xml:lang="it">CIG (Codice Identificativo Gara)</rdfs:label>
        <rdfs:label xml:lang="en">Identifier of the Lot</rdfs:label>
        <owl:versionInfo xml:lang="it">stabile</owl:versionInfo>
        <owl:versionInfo xml:lang="en">stable</owl:versionInfo>
    </owl:DatatypeProperty>
    


    <!-- https://w3id.org/italia/onto/PublicContract/actualEndDate -->

    <owl:DatatypeProperty rdf:about="https://w3id.org/italia/onto/PublicContract/actualEndDate">
        <rdfs:subPropertyOf rdf:resource="https://w3id.org/italia/onto/TI/endTime"/>
        <rdfs:domain rdf:resource="https://w3id.org/italia/onto/PublicContract/Lot"/>
        <rdfs:range rdf:resource="http://www.w3.org/2001/XMLSchema#date"/>
        <rdfs:comment xml:lang="it">Questa proprietà indica la data effettiva in cui la prestazione relativa al lotto è terminata. Può essere dedotta dalle verifiche effettuate nel collaudo finale.</rdfs:comment>
        <rdfs:comment xml:lang="en">This property represents the actual end date of the lot, and it may be imported from the results of the testing stage.</rdfs:comment>
        <rdfs:isDefinedBy rdf:resource="https://w3id.org/italia/onto/PublicContract"/>
        <rdfs:label xml:lang="en">actual end date</rdfs:label>
        <rdfs:label xml:lang="it">data effettiva di fine prestazione</rdfs:label>
        <owl:versionInfo xml:lang="it">stabile</owl:versionInfo>
        <owl:versionInfo xml:lang="en">stable</owl:versionInfo>
    </owl:DatatypeProperty>
    


    <!-- https://w3id.org/italia/onto/PublicContract/actualStartDate -->

    <owl:DatatypeProperty rdf:about="https://w3id.org/italia/onto/PublicContract/actualStartDate">
        <rdfs:subPropertyOf rdf:resource="https://w3id.org/italia/onto/TI/startTime"/>
        <rdfs:domain rdf:resource="https://w3id.org/italia/onto/PublicContract/Lot"/>
        <rdfs:range rdf:resource="http://www.w3.org/2001/XMLSchema#date"/>
        <rdfs:comment xml:lang="it">Questa proprietà indica la data effettiva in cui la procedura è iniziata. Può essere dedotta dalle verifiche effettuate nel collaudo finale.</rdfs:comment>
        <rdfs:comment xml:lang="en">This property represents the actual start date of the procedure, and it may be imported from the results of the testing stage.</rdfs:comment>
        <rdfs:isDefinedBy rdf:resource="https://w3id.org/italia/onto/PublicContract"/>
        <rdfs:label xml:lang="en">actual start date</rdfs:label>
        <rdfs:label xml:lang="it">data di effettiva inizio prestazione</rdfs:label>
        <owl:versionInfo xml:lang="it">stabile</owl:versionInfo>
        <owl:versionInfo xml:lang="en">stable</owl:versionInfo>
    </owl:DatatypeProperty>
    


    <!-- https://w3id.org/italia/onto/PublicContract/additionalDay -->

    <owl:DatatypeProperty rdf:about="https://w3id.org/italia/onto/PublicContract/additionalDay">
        <rdfs:subPropertyOf rdf:resource="https://w3id.org/italia/onto/TI/duration"/>
        <rdfs:domain rdf:resource="https://w3id.org/italia/onto/PublicContract/VariantDocument"/>
        <rdfs:range rdf:resource="http://www.w3.org/2001/XMLSchema#float"/>
        <rdfs:comment xml:lang="it">Questa proprietà indica i giorni aggiuntivi necessari per il completamento dell&apos;intervento, indicati nel documento di variante.</rdfs:comment>
        <rdfs:comment xml:lang="en">The property that represents the additional days needed to complete the intervention, as reported by the variant document.</rdfs:comment>
        <rdfs:isDefinedBy rdf:resource="https://w3id.org/italia/onto/PublicContract"/>
        <rdfs:label xml:lang="en">additional day</rdfs:label>
        <rdfs:label xml:lang="it">giorni aggiuntivi</rdfs:label>
        <owl:versionInfo xml:lang="it">stabile</owl:versionInfo>
        <owl:versionInfo xml:lang="en">stable</owl:versionInfo>
    </owl:DatatypeProperty>
    


    <!-- https://w3id.org/italia/onto/PublicContract/agreedAmount -->

    <owl:DatatypeProperty rdf:about="https://w3id.org/italia/onto/PublicContract/agreedAmount">
        <rdfs:domain rdf:resource="https://w3id.org/italia/onto/PublicContract/AwardNotice"/>
        <rdfs:range rdf:resource="http://www.w3.org/2001/XMLSchema#float"/>
        <rdfs:comment xml:lang="it">La proprietà che determina il prezzo concordato (anche detto importo di aggiudicazione, nel caso di gare con bando) per la realizzazione del lotto.</rdfs:comment>
        <rdfs:comment xml:lang="en">The property that represents the agreed amount for the actualization of the lot.</rdfs:comment>
        <rdfs:isDefinedBy rdf:resource="https://w3id.org/italia/onto/PublicContract"/>
        <rdfs:label xml:lang="en">agreed amount</rdfs:label>
        <rdfs:label xml:lang="it">prezzo concordato</rdfs:label>
        <owl:versionInfo xml:lang="it">stabile</owl:versionInfo>
        <owl:versionInfo xml:lang="en">stable</owl:versionInfo>
    </owl:DatatypeProperty>
    


    <!-- https://w3id.org/italia/onto/PublicContract/auctionBaseAmount -->

    <owl:DatatypeProperty rdf:about="https://w3id.org/italia/onto/PublicContract/auctionBaseAmount">
        <rdfs:domain rdf:resource="https://w3id.org/italia/onto/PublicContract/ProcurementProject"/>
        <rdfs:range rdf:resource="http://www.w3.org/2001/XMLSchema#float"/>
        <rdfs:comment xml:lang="it">La proprietà che determina l&apos;importo base dell&apos;asta.</rdfs:comment>
        <rdfs:comment xml:lang="en">The property that determines the auction base amount.</rdfs:comment>
        <rdfs:isDefinedBy rdf:resource="https://w3id.org/italia/onto/PublicContract"/>
        <rdfs:label xml:lang="en">auction base amount</rdfs:label>
        <rdfs:label xml:lang="it">importo base asta</rdfs:label>
        <owl:versionInfo xml:lang="it">stabile</owl:versionInfo>
        <owl:versionInfo xml:lang="en">stable</owl:versionInfo>
    </owl:DatatypeProperty>
    


    <!-- https://w3id.org/italia/onto/PublicContract/availableAmount -->

    <owl:DatatypeProperty rdf:about="https://w3id.org/italia/onto/PublicContract/availableAmount">
        <rdfs:domain rdf:resource="https://w3id.org/italia/onto/PublicContract/EconomicSummary"/>
        <rdfs:range rdf:resource="http://www.w3.org/2001/XMLSchema#float"/>
        <rdfs:comment xml:lang="it">La proprietà che determina la somma a disposizione per il completamento di un lotto o contratto, nell&apos;ambito di una versione del prospetto economico.</rdfs:comment>
        <rdfs:comment xml:lang="en">The property that represents the amount available to complete a lot or contract. It is valid within a version of the economic summary.</rdfs:comment>
        <rdfs:isDefinedBy rdf:resource="https://w3id.org/italia/onto/PublicContract"/>
        <rdfs:label xml:lang="en">available amount</rdfs:label>
        <rdfs:label xml:lang="it">somma a disposizione</rdfs:label>
        <owl:versionInfo xml:lang="it">stabile</owl:versionInfo>
        <owl:versionInfo xml:lang="en">stable</owl:versionInfo>
    </owl:DatatypeProperty>
    


    <!-- https://w3id.org/italia/onto/PublicContract/currentAvailableAmount -->

    <owl:DatatypeProperty rdf:about="https://w3id.org/italia/onto/PublicContract/currentAvailableAmount">
        <rdfs:domain rdf:resource="https://w3id.org/italia/onto/PublicContract/Lot"/>
        <rdfs:range rdf:resource="http://www.w3.org/2001/XMLSchema#float"/>
        <rdfs:comment xml:lang="it">La proprietà che indica la somma attualmente a disposizione, riportata nell&apos;ultima versione del prospetto economico</rdfs:comment>
        <rdfs:comment xml:lang="en">The property that represents the amount currently available. The date is imported from the last economic summary related to the procedure.</rdfs:comment>
        <rdfs:isDefinedBy rdf:resource="https://w3id.org/italia/onto/PublicContract"/>
        <rdfs:label xml:lang="it">attuale somma a disposizione</rdfs:label>
        <rdfs:label xml:lang="en">current available amount</rdfs:label>
        <owl:versionInfo xml:lang="it">stabile</owl:versionInfo>
        <owl:versionInfo xml:lang="en">stable</owl:versionInfo>
    </owl:DatatypeProperty>
    


    <!-- https://w3id.org/italia/onto/PublicContract/currentEstimatedEndDate -->

    <owl:DatatypeProperty rdf:about="https://w3id.org/italia/onto/PublicContract/currentEstimatedEndDate">
        <rdfs:subPropertyOf rdf:resource="https://w3id.org/italia/onto/TI/endTime"/>
        <rdfs:domain rdf:resource="https://w3id.org/italia/onto/PublicContract/Lot"/>
        <rdfs:range rdf:resource="http://www.w3.org/2001/XMLSchema#date"/>
        <rdfs:comment xml:lang="it">La proprietà che indica la data entro la quale si prevede di portare a termine la prestazione. Si deduce tale data dall&apos;attuale prospetto economico del lotto, o comunque si intende che essa indica la più recente e valida previsione fatta.</rdfs:comment>
        <rdfs:comment xml:lang="en">The property that represents the estimated end date. The date is imported from the last economic summary related to the lot.</rdfs:comment>
        <rdfs:isDefinedBy rdf:resource="https://w3id.org/italia/onto/PublicContract"/>
        <rdfs:label xml:lang="it">attuale previsione di fine prestazione</rdfs:label>
        <rdfs:label xml:lang="en">current estimated end date</rdfs:label>
        <owl:versionInfo xml:lang="it">stabile</owl:versionInfo>
        <owl:versionInfo xml:lang="en">stable</owl:versionInfo>
    </owl:DatatypeProperty>
    


    <!-- https://w3id.org/italia/onto/PublicContract/currentPlanningAmount -->

    <owl:DatatypeProperty rdf:about="https://w3id.org/italia/onto/PublicContract/currentPlanningAmount">
        <rdfs:domain rdf:resource="https://w3id.org/italia/onto/PublicContract/Lot"/>
        <rdfs:range rdf:resource="http://www.w3.org/2001/XMLSchema#float"/>
        <rdfs:comment xml:lang="it">La proprietà che determina l&apos;importo attualmente previsto per la progettazione riportato nell&apos;ultima versione del prospetto economico</rdfs:comment>
        <rdfs:comment xml:lang="en">The property that represents the currently estimated planning amount. The date is imported from the last economic summary related to the procedure.</rdfs:comment>
        <rdfs:isDefinedBy rdf:resource="https://w3id.org/italia/onto/PublicContract"/>
        <rdfs:label xml:lang="it">attuale importo progettazione</rdfs:label>
        <rdfs:label xml:lang="en">current planning amount</rdfs:label>
        <owl:versionInfo xml:lang="it">stabile</owl:versionInfo>
        <owl:versionInfo xml:lang="en">stable</owl:versionInfo>
    </owl:DatatypeProperty>
    


    <!-- https://w3id.org/italia/onto/PublicContract/currentSafetyAmount -->

    <owl:DatatypeProperty rdf:about="https://w3id.org/italia/onto/PublicContract/currentSafetyAmount">
        <rdfs:domain rdf:resource="https://w3id.org/italia/onto/PublicContract/Lot"/>
        <rdfs:range rdf:resource="http://www.w3.org/2001/XMLSchema#float"/>
        <rdfs:comment xml:lang="it">La proprietà che determina l&apos;importo attualmente previsto per la sicurezza riportato nell&apos;ultima versione del prospetto economico</rdfs:comment>
        <rdfs:comment xml:lang="en">The property that represents the currently estimated safety amount needed for the completion of the procedure. The date is imported from the last economic summary related to the lot.</rdfs:comment>
        <rdfs:isDefinedBy rdf:resource="https://w3id.org/italia/onto/PublicContract"/>
        <rdfs:label xml:lang="it">attuale importo sicurezza</rdfs:label>
        <rdfs:label xml:lang="en">current safety amount</rdfs:label>
        <owl:versionInfo xml:lang="it">stabile</owl:versionInfo>
        <owl:versionInfo xml:lang="en">stable</owl:versionInfo>
    </owl:DatatypeProperty>
    


    <!-- https://w3id.org/italia/onto/PublicContract/currentServicesAmount -->

    <owl:DatatypeProperty rdf:about="https://w3id.org/italia/onto/PublicContract/currentServicesAmount">
        <rdfs:domain rdf:resource="https://w3id.org/italia/onto/PublicContract/Lot"/>
        <rdfs:range rdf:resource="http://www.w3.org/2001/XMLSchema#float"/>
        <rdfs:comment xml:lang="it">La proprietà che determina l&apos;importo attualmente stimato per i servizi, riportato nell&apos;ultima versione del prospetto economico.</rdfs:comment>
        <rdfs:comment xml:lang="en">The property that represents the currently estimated services amount. The date is imported from the last economic summary related to the lot.</rdfs:comment>
        <rdfs:isDefinedBy rdf:resource="https://w3id.org/italia/onto/PublicContract"/>
        <rdfs:label xml:lang="it">attuale importo servizi</rdfs:label>
        <rdfs:label xml:lang="en">current services amount</rdfs:label>
        <owl:versionInfo xml:lang="it">stabile</owl:versionInfo>
        <owl:versionInfo xml:lang="en">stable</owl:versionInfo>
    </owl:DatatypeProperty>
    


    <!-- https://w3id.org/italia/onto/PublicContract/currentSuppliesAmount -->

    <owl:DatatypeProperty rdf:about="https://w3id.org/italia/onto/PublicContract/currentSuppliesAmount">
        <rdfs:domain rdf:resource="https://w3id.org/italia/onto/PublicContract/Lot"/>
        <rdfs:range rdf:resource="http://www.w3.org/2001/XMLSchema#float"/>
        <rdfs:comment xml:lang="it">La proprietà che determina l&apos;importo attualmente stimato per le forniture, riportato nell&apos;ultima versione del prospetto economico.</rdfs:comment>
        <rdfs:comment xml:lang="en">The property that represents the currently estimated supplies amount. The date is imported from the last economic summary related to the lot.</rdfs:comment>
        <rdfs:isDefinedBy rdf:resource="https://w3id.org/italia/onto/PublicContract"/>
        <rdfs:label xml:lang="it">attuale importo forniture</rdfs:label>
        <rdfs:label xml:lang="en">current supplies amount</rdfs:label>
        <owl:versionInfo xml:lang="it">stabile</owl:versionInfo>
        <owl:versionInfo xml:lang="en">stable</owl:versionInfo>
    </owl:DatatypeProperty>
    


    <!-- https://w3id.org/italia/onto/PublicContract/currentTotalAmount -->

    <owl:DatatypeProperty rdf:about="https://w3id.org/italia/onto/PublicContract/currentTotalAmount">
        <rdfs:domain rdf:resource="https://w3id.org/italia/onto/PublicContract/Lot"/>
        <rdfs:range rdf:resource="http://www.w3.org/2001/XMLSchema#float"/>
        <rdfs:comment xml:lang="it">La proprietà che determina l&apos;importo totale attualmente previsto per il completamento della prestazione, così come è riportato nell&apos;ultima versione del prospetto economico.</rdfs:comment>
        <rdfs:comment xml:lang="en">The property that represents the currently estimated total amount needed for the completion of the lot. The date is imported from the last economic summary related to the lot.</rdfs:comment>
        <rdfs:isDefinedBy rdf:resource="https://w3id.org/italia/onto/PublicContract"/>
        <rdfs:label xml:lang="it">attuale importo totale</rdfs:label>
        <rdfs:label xml:lang="en">current total amount</rdfs:label>
        <owl:versionInfo xml:lang="it">stabile</owl:versionInfo>
        <owl:versionInfo xml:lang="en">stable</owl:versionInfo>
    </owl:DatatypeProperty>
    


    <!-- https://w3id.org/italia/onto/PublicContract/currentWorksAmount -->

    <owl:DatatypeProperty rdf:about="https://w3id.org/italia/onto/PublicContract/currentWorksAmount">
        <rdfs:domain rdf:resource="https://w3id.org/italia/onto/PublicContract/Lot"/>
        <rdfs:range rdf:resource="http://www.w3.org/2001/XMLSchema#float"/>
        <rdfs:comment xml:lang="it">La proprietà che determina l&apos;importo attualmente stimato per i lavori, riportato nell&apos;ultima versione del prospetto economico.</rdfs:comment>
        <rdfs:comment xml:lang="en">The property that represents the currently estimated works amount. The date is imported from the last economic summary related to the lot.</rdfs:comment>
        <rdfs:isDefinedBy rdf:resource="https://w3id.org/italia/onto/PublicContract"/>
        <rdfs:label xml:lang="it">attuale importo lavori</rdfs:label>
        <rdfs:label xml:lang="en">current works amount</rdfs:label>
        <owl:versionInfo xml:lang="it">stabile</owl:versionInfo>
        <owl:versionInfo xml:lang="en">stable</owl:versionInfo>
    </owl:DatatypeProperty>
    


    <!-- https://w3id.org/italia/onto/PublicContract/estimatedEndDate -->

    <owl:DatatypeProperty rdf:about="https://w3id.org/italia/onto/PublicContract/estimatedEndDate">
        <rdfs:subPropertyOf rdf:resource="https://w3id.org/italia/onto/TI/endTime"/>
        <rdfs:domain rdf:resource="https://w3id.org/italia/onto/PublicContract/EconomicSummary"/>
        <rdfs:range rdf:resource="http://www.w3.org/2001/XMLSchema#float"/>
        <rdfs:comment xml:lang="it">La proprietà che indica la data entro la quale si prevede di portare a termine un lotto o un contratto. La data è indicata nell&apos;ambito di una versione del prospetto economico, e può aggiornare (o essere aggiornata da) quella indicata nel prospetto economico precedente (o successivo).</rdfs:comment>
        <rdfs:comment xml:lang="en">The property that represents the estimated end date of a project, intervention, procedure or contract. The date is valid within a version of the economic summary, and may update (or be updated by) the date reported by the former (or next) economic summary</rdfs:comment>
        <rdfs:isDefinedBy rdf:resource="https://w3id.org/italia/onto/PublicContract"/>
        <rdfs:label xml:lang="en">estimated end date</rdfs:label>
        <rdfs:label xml:lang="it">previsione di fine prestazione</rdfs:label>
        <owl:versionInfo xml:lang="it">stabile</owl:versionInfo>
        <owl:versionInfo xml:lang="en">stable</owl:versionInfo>
    </owl:DatatypeProperty>
    


    <!-- https://w3id.org/italia/onto/PublicContract/expireDate -->

    <owl:DatatypeProperty rdf:about="https://w3id.org/italia/onto/PublicContract/expireDate">
        <rdfs:subPropertyOf rdf:resource="https://w3id.org/italia/onto/TI/endTime"/>
        <rdfs:domain rdf:resource="https://w3id.org/italia/onto/PublicContract/CallForCompetition"/>
        <rdfs:range rdf:resource="http://www.w3.org/2001/XMLSchema#date"/>
        <rdfs:comment xml:lang="it">Proprietà che determina la data di scadenza del bando.</rdfs:comment>
        <rdfs:comment xml:lang="en">The property that represents the expire date of the notice.</rdfs:comment>
        <rdfs:label xml:lang="it">data di scadenza</rdfs:label>
        <rdfs:label xml:lang="en">expire date</rdfs:label>
        <owl:versionInfo xml:lang="it">stabile</owl:versionInfo>
        <owl:versionInfo xml:lang="en">stable</owl:versionInfo>
    </owl:DatatypeProperty>
    


    <!-- https://w3id.org/italia/onto/PublicContract/increaseAmount -->

    <owl:DatatypeProperty rdf:about="https://w3id.org/italia/onto/PublicContract/increaseAmount">
        <rdfs:domain rdf:resource="https://w3id.org/italia/onto/PublicContract/VariantDocument"/>
        <rdfs:range rdf:resource="http://www.w3.org/2001/XMLSchema#float"/>
        <rdfs:comment xml:lang="it">Questa proprietà indica un aumento dell&apos;importo necessario per il completamento della prestazione indicata nel contratto. L&apos;importo è indicato nel documento di variante.</rdfs:comment>
        <rdfs:comment xml:lang="en">The property that represents the increase amount needed to complete the contract, as reported by the variant document.</rdfs:comment>
        <rdfs:isDefinedBy rdf:resource="https://w3id.org/italia/onto/PublicContract"/>
        <rdfs:label xml:lang="it">aumento importo</rdfs:label>
        <rdfs:label xml:lang="en">increase amount</rdfs:label>
        <owl:versionInfo xml:lang="it">stabile</owl:versionInfo>
        <owl:versionInfo xml:lang="en">stable</owl:versionInfo>
    </owl:DatatypeProperty>
    


    <!-- https://w3id.org/italia/onto/PublicContract/nonDiscountableSum -->

    <owl:DatatypeProperty rdf:about="https://w3id.org/italia/onto/PublicContract/nonDiscountableSum">
        <rdfs:domain rdf:resource="https://w3id.org/italia/onto/PublicContract/EconomicSummary"/>
        <rdfs:range rdf:resource="http://www.w3.org/2001/XMLSchema#float"/>
        <rdfs:comment xml:lang="it">La proprietà che determina la somma di denaro che non è ribassabile.</rdfs:comment>
        <rdfs:comment xml:lang="en">The property that determines the amount of the starting price that is not lowerable.</rdfs:comment>
        <rdfs:isDefinedBy rdf:resource="https://w3id.org/italia/onto/PublicContract"/>
        <rdfs:label xml:lang="it">somma non ribassabile</rdfs:label>
        <rdfs:label xml:lang="en">sum of non-discountable money</rdfs:label>
        <owl:versionInfo xml:lang="it">stabile</owl:versionInfo>
        <owl:versionInfo xml:lang="en">stable</owl:versionInfo>
    </owl:DatatypeProperty>
    


    <!-- https://w3id.org/italia/onto/PublicContract/outcomeDate -->

    <owl:DatatypeProperty rdf:about="https://w3id.org/italia/onto/PublicContract/outcomeDate">
        <rdfs:subPropertyOf rdf:resource="https://w3id.org/italia/onto/TI/date"/>
        <rdfs:domain rdf:resource="https://w3id.org/italia/onto/PublicContract/AwardNotice"/>
        <rdfs:range rdf:resource="http://www.w3.org/2001/XMLSchema#date"/>
        <rdfs:comment xml:lang="it">Proprietà che indica la data di aggiudicazione o affidamento a un offerente, o di adesione a un accordo quadro da parte di un offerente.</rdfs:comment>
        <rdfs:comment xml:lang="en">This property represents the date of the outcome of the procedure (e.g. the date of the award to a bidder, or the date of the framework agreement)</rdfs:comment>
        <rdfs:isDefinedBy rdf:resource="https://w3id.org/italia/onto/PublicContract"/>
        <rdfs:label xml:lang="it">data esito procedura</rdfs:label>
        <rdfs:label xml:lang="en">outcome date</rdfs:label>
        <owl:versionInfo xml:lang="it">stabile</owl:versionInfo>
        <owl:versionInfo xml:lang="en">stable</owl:versionInfo>
    </owl:DatatypeProperty>
    


    <!-- https://w3id.org/italia/onto/PublicContract/paymentAmount -->

    <owl:DatatypeProperty rdf:about="https://w3id.org/italia/onto/PublicContract/paymentAmount">
        <rdfs:domain rdf:resource="https://w3id.org/italia/onto/PublicContract/PaymentCertificate"/>
        <rdfs:range rdf:resource="http://www.w3.org/2001/XMLSchema#float"/>
        <rdfs:comment xml:lang="it">La proprietà che determina l&apos;importo del pagamento.</rdfs:comment>
        <rdfs:comment xml:lang="en">The property that represents the amount of the payment.</rdfs:comment>
        <rdfs:isDefinedBy rdf:resource="https://w3id.org/italia/onto/PublicContract"/>
        <rdfs:label xml:lang="en">amount of the payment</rdfs:label>
        <rdfs:label xml:lang="it">importo del pagamento</rdfs:label>
        <owl:versionInfo xml:lang="it">stabile</owl:versionInfo>
        <owl:versionInfo xml:lang="en">stable</owl:versionInfo>
    </owl:DatatypeProperty>
    


    <!-- https://w3id.org/italia/onto/PublicContract/paymentCetificateDate -->

    <owl:DatatypeProperty rdf:about="https://w3id.org/italia/onto/PublicContract/paymentCetificateDate">
        <rdfs:subPropertyOf rdf:resource="https://w3id.org/italia/onto/TI/date"/>
        <rdfs:domain rdf:resource="https://w3id.org/italia/onto/PublicContract/PaymentCertificate"/>
        <rdfs:range rdf:resource="http://www.w3.org/2001/XMLSchema#date"/>
        <rdfs:comment xml:lang="it">La proprietà che indica la data di emissione del certificato di pagamento da parte della stazione appaltante.</rdfs:comment>
        <rdfs:comment xml:lang="en">The property that represents the date of the certificate of the payment.</rdfs:comment>
        <rdfs:isDefinedBy rdf:resource="https://w3id.org/italia/onto/PublicContract"/>
        <rdfs:label xml:lang="it">data del certificato di pagamento</rdfs:label>
        <rdfs:label xml:lang="en">payment certificate date</rdfs:label>
        <owl:versionInfo xml:lang="it">stabile</owl:versionInfo>
        <owl:versionInfo xml:lang="en">stable</owl:versionInfo>
    </owl:DatatypeProperty>
    


    <!-- https://w3id.org/italia/onto/PublicContract/planningAmount -->

    <owl:DatatypeProperty rdf:about="https://w3id.org/italia/onto/PublicContract/planningAmount">
        <rdfs:domain rdf:resource="https://w3id.org/italia/onto/PublicContract/EconomicSummary"/>
        <rdfs:range rdf:resource="http://www.w3.org/2001/XMLSchema#float"/>
        <rdfs:comment xml:lang="it">La proprietà che determina l&apos;importo stimato per la progettazione, nell&apos;ambito di una versione del prospetto economico.</rdfs:comment>
        <rdfs:comment xml:lang="en">The property that represents the planning amount. It is valid within a version of the economic summary.</rdfs:comment>
        <rdfs:isDefinedBy rdf:resource="https://w3id.org/italia/onto/PublicContract"/>
        <rdfs:label xml:lang="it">importo progettazione</rdfs:label>
        <rdfs:label xml:lang="en">planning amount</rdfs:label>
        <owl:versionInfo xml:lang="it">stabile</owl:versionInfo>
        <owl:versionInfo xml:lang="en">stable</owl:versionInfo>
    </owl:DatatypeProperty>
    


    <!-- https://w3id.org/italia/onto/PublicContract/procedureTotalAmount -->

    <owl:DatatypeProperty rdf:about="https://w3id.org/italia/onto/PublicContract/procedureTotalAmount">
        <rdfs:domain rdf:resource="https://w3id.org/italia/onto/PublicContract/Procedure"/>
        <rdfs:range rdf:resource="http://www.w3.org/2001/XMLSchema#float"/>
        <rdfs:comment xml:lang="it">La proprietà che determina l&apos;importo totale della procedura</rdfs:comment>
        <rdfs:comment xml:lang="en">The property that represents the total amount for the procedure.</rdfs:comment>
        <rdfs:isDefinedBy rdf:resource="https://w3id.org/italia/onto/PublicContract"/>
        <rdfs:label xml:lang="it">importo complessivo gara</rdfs:label>
        <rdfs:label xml:lang="en">procedure total amount</rdfs:label>
        <owl:versionInfo xml:lang="it">stabile</owl:versionInfo>
        <owl:versionInfo xml:lang="en">stable</owl:versionInfo>
    </owl:DatatypeProperty>
    


    <!-- https://w3id.org/italia/onto/PublicContract/publicationDate -->

    <owl:DatatypeProperty rdf:about="https://w3id.org/italia/onto/PublicContract/publicationDate">
        <rdfs:subPropertyOf rdf:resource="https://w3id.org/italia/onto/TI/issued"/>
        <rdfs:domain>
            <owl:Class>
                <owl:unionOf rdf:parseType="Collection">
                    <rdf:Description rdf:about="https://w3id.org/italia/onto/PublicContract/CallForCompetition"/>
                    <rdf:Description rdf:about="https://w3id.org/italia/onto/PublicContract/Publication"/>
                </owl:unionOf>
            </owl:Class>
        </rdfs:domain>
        <rdfs:range rdf:resource="http://www.w3.org/2001/XMLSchema#date"/>
        <rdfs:comment xml:lang="it">La proprietà che indica la data di pubblicazione del bando o dell&apos;avviso.</rdfs:comment>
        <rdfs:comment xml:lang="en">The property that represents the publication date of the notice.</rdfs:comment>
        <rdfs:isDefinedBy rdf:resource="https://w3id.org/italia/onto/PublicContract"/>
        <rdfs:label xml:lang="it">data di pubblicazione</rdfs:label>
        <rdfs:label xml:lang="en">publication date</rdfs:label>
        <owl:versionInfo xml:lang="it">stabile</owl:versionInfo>
        <owl:versionInfo xml:lang="en">stable</owl:versionInfo>
    </owl:DatatypeProperty>
    


    <!-- https://w3id.org/italia/onto/PublicContract/reductionAmount -->

    <owl:DatatypeProperty rdf:about="https://w3id.org/italia/onto/PublicContract/reductionAmount">
        <rdfs:domain rdf:resource="https://w3id.org/italia/onto/PublicContract/VariantDocument"/>
        <rdfs:range rdf:resource="http://www.w3.org/2001/XMLSchema#float"/>
        <rdfs:comment xml:lang="it">Questa proprietà indica una diminuzione dell&apos;importo necessario per il completamento della prestazione indicata nel contratto, indicato nel documento di variante.</rdfs:comment>
        <rdfs:comment xml:lang="en">The property thath represents the reduction amount needed to complete the contract, as reported by the variant document.</rdfs:comment>
        <rdfs:isDefinedBy rdf:resource="https://w3id.org/italia/onto/PublicContract"/>
        <rdfs:label xml:lang="it">diminuzione importo</rdfs:label>
        <rdfs:label xml:lang="en">reduction amount</rdfs:label>
        <owl:versionInfo xml:lang="it">stabile</owl:versionInfo>
        <owl:versionInfo xml:lang="en">stable</owl:versionInfo>
    </owl:DatatypeProperty>
    


    <!-- https://w3id.org/italia/onto/PublicContract/reductionPercentage -->

    <owl:DatatypeProperty rdf:about="https://w3id.org/italia/onto/PublicContract/reductionPercentage">
        <rdfs:domain rdf:resource="https://w3id.org/italia/onto/PublicContract/AwardNotice"/>
        <rdfs:range rdf:resource="http://www.w3.org/2001/XMLSchema#float"/>
        <rdfs:comment xml:lang="it">La proprietà che determina la percentuale dichiarata di ribasso.</rdfs:comment>
        <rdfs:comment xml:lang="en">The property that determines the declared percentage of price cut.</rdfs:comment>
        <rdfs:isDefinedBy rdf:resource="https://w3id.org/italia/onto/PublicContract"/>
        <rdfs:label xml:lang="it">percentuale di ribasso</rdfs:label>
        <rdfs:label xml:lang="en">reduction percentage</rdfs:label>
        <owl:versionInfo xml:lang="it">stabile</owl:versionInfo>
        <owl:versionInfo xml:lang="en">stable</owl:versionInfo>
    </owl:DatatypeProperty>
    


    <!-- https://w3id.org/italia/onto/PublicContract/resumptionDate -->

    <owl:DatatypeProperty rdf:about="https://w3id.org/italia/onto/PublicContract/resumptionDate">
        <rdfs:subPropertyOf rdf:resource="https://w3id.org/italia/onto/TI/date"/>
        <rdfs:domain rdf:resource="https://w3id.org/italia/onto/PublicContract/SuspensionDocument"/>
        <rdfs:range rdf:resource="http://www.w3.org/2001/XMLSchema#date"/>
        <rdfs:comment xml:lang="it">Questa proprietà indica la data di inizio di ripresa del contratto.</rdfs:comment>
        <rdfs:comment xml:lang="en">The property that represents the starting date of the resumption of the contract.</rdfs:comment>
        <rdfs:isDefinedBy rdf:resource="https://w3id.org/italia/onto/PublicContract"/>
        <rdfs:label xml:lang="it">data ripresa</rdfs:label>
        <rdfs:label xml:lang="en">resumption date</rdfs:label>
        <owl:versionInfo xml:lang="it">stabile</owl:versionInfo>
        <owl:versionInfo xml:lang="en">stable</owl:versionInfo>
    </owl:DatatypeProperty>
    


    <!-- https://w3id.org/italia/onto/PublicContract/safetyAmount -->

    <owl:DatatypeProperty rdf:about="https://w3id.org/italia/onto/PublicContract/safetyAmount">
        <rdfs:domain rdf:resource="https://w3id.org/italia/onto/PublicContract/EconomicSummary"/>
        <rdfs:range rdf:resource="http://www.w3.org/2001/XMLSchema#float"/>
        <rdfs:comment xml:lang="it">La proprietà che determina l&apos;importo stimato per la sicurezza, nell&apos;ambito di una versione del prospetto economico.</rdfs:comment>
        <rdfs:comment xml:lang="en">The property that determines the amount of money to be spent for safety reason. It is valid within a version of the economic summary.</rdfs:comment>
        <rdfs:isDefinedBy rdf:resource="https://w3id.org/italia/onto/PublicContract"/>
        <rdfs:label xml:lang="it">importo di sicurezza</rdfs:label>
        <rdfs:label xml:lang="en">safety amount</rdfs:label>
        <owl:versionInfo xml:lang="it">stabile</owl:versionInfo>
        <owl:versionInfo xml:lang="en">stable</owl:versionInfo>
    </owl:DatatypeProperty>
    


    <!-- https://w3id.org/italia/onto/PublicContract/servicesAmount -->

    <owl:DatatypeProperty rdf:about="https://w3id.org/italia/onto/PublicContract/servicesAmount">
        <rdfs:domain rdf:resource="https://w3id.org/italia/onto/PublicContract/EconomicSummary"/>
        <rdfs:range rdf:resource="http://www.w3.org/2001/XMLSchema#float"/>
        <rdfs:comment xml:lang="it">La proprietà che determina l&apos;importo stimato per i servizi, nell&apos;ambito di una versione del prospetto economico.</rdfs:comment>
        <rdfs:comment xml:lang="en">The property that represents the services amount. It is valid within a version of the economic summary.</rdfs:comment>
        <rdfs:isDefinedBy rdf:resource="https://w3id.org/italia/onto/PublicContract"/>
        <rdfs:label xml:lang="it">importo servizi</rdfs:label>
        <rdfs:label xml:lang="en">services amount</rdfs:label>
        <owl:versionInfo xml:lang="it">stabile</owl:versionInfo>
        <owl:versionInfo xml:lang="en">stable</owl:versionInfo>
    </owl:DatatypeProperty>
    


    <!-- https://w3id.org/italia/onto/PublicContract/specialSector -->

    <owl:DatatypeProperty rdf:about="https://w3id.org/italia/onto/PublicContract/specialSector">
        <rdfs:domain rdf:resource="https://w3id.org/italia/onto/PublicContract/Lot"/>
        <rdfs:range rdf:resource="http://www.w3.org/2001/XMLSchema#boolean"/>
        <rdfs:comment xml:lang="it">La proprietà che determina se un lotto appartiene a uno dei settori speciali definiti dal DLGS 163/2006 Art3.</rdfs:comment>
        <rdfs:comment xml:lang="en">The property that determines if a lotto belongs to a special sector, according to the DLGS 163/2006 Art3.</rdfs:comment>
        <rdfs:isDefinedBy rdf:resource="https://w3id.org/italia/onto/PublicContract"/>
        <rdfs:label xml:lang="it">settore speciale</rdfs:label>
        <rdfs:label xml:lang="en">special sector</rdfs:label>
        <owl:versionInfo xml:lang="it">stabile</owl:versionInfo>
        <owl:versionInfo xml:lang="en">stable</owl:versionInfo>
    </owl:DatatypeProperty>
    


    <!-- https://w3id.org/italia/onto/PublicContract/suppliesAmount -->

    <owl:DatatypeProperty rdf:about="https://w3id.org/italia/onto/PublicContract/suppliesAmount">
        <rdfs:domain rdf:resource="https://w3id.org/italia/onto/PublicContract/EconomicSummary"/>
        <rdfs:range rdf:resource="http://www.w3.org/2001/XMLSchema#float"/>
        <rdfs:comment xml:lang="it">La proprietà che determina l&apos;importo stimato per le forniture, nell&apos;ambito di una versione del prospetto economico.</rdfs:comment>
        <rdfs:comment xml:lang="en">The property that represents the supplies amount. It is valid within a version of the economic summary.</rdfs:comment>
        <rdfs:isDefinedBy rdf:resource="https://w3id.org/italia/onto/PublicContract"/>
        <rdfs:label xml:lang="it">importo forniture</rdfs:label>
        <rdfs:label xml:lang="en">supplies amount</rdfs:label>
        <owl:versionInfo xml:lang="it">stabile</owl:versionInfo>
        <owl:versionInfo xml:lang="en">stable</owl:versionInfo>
    </owl:DatatypeProperty>
    


    <!-- https://w3id.org/italia/onto/PublicContract/suspensionDate -->

    <owl:DatatypeProperty rdf:about="https://w3id.org/italia/onto/PublicContract/suspensionDate">
        <rdfs:subPropertyOf rdf:resource="https://w3id.org/italia/onto/TI/date"/>
        <rdfs:domain rdf:resource="https://w3id.org/italia/onto/PublicContract/SuspensionDocument"/>
        <rdfs:range rdf:resource="http://www.w3.org/2001/XMLSchema#date"/>
        <rdfs:comment xml:lang="it">Questa proprietà indica la data di inizio della sospensione del contratto.</rdfs:comment>
        <rdfs:comment xml:lang="en">The property that represents the starting date of the suspension.</rdfs:comment>
        <rdfs:isDefinedBy rdf:resource="https://w3id.org/italia/onto/PublicContract"/>
        <rdfs:label xml:lang="it">data sospensione</rdfs:label>
        <rdfs:label xml:lang="en">suspension date</rdfs:label>
        <owl:versionInfo xml:lang="it">stabile</owl:versionInfo>
        <owl:versionInfo xml:lang="en">stable</owl:versionInfo>
    </owl:DatatypeProperty>
    


    <!-- https://w3id.org/italia/onto/PublicContract/totalAmount -->

    <owl:DatatypeProperty rdf:about="https://w3id.org/italia/onto/PublicContract/totalAmount">
        <rdfs:domain rdf:resource="https://w3id.org/italia/onto/PublicContract/EconomicSummary"/>
        <rdfs:range rdf:resource="http://www.w3.org/2001/XMLSchema#float"/>
        <rdfs:comment xml:lang="it">La proprietà che determina l&apos;importo totale previsto per il completamento di un lotto o contratto, nell&apos;ambito di una versione del prospetto economico.</rdfs:comment>
        <rdfs:comment xml:lang="en">The property that represents the total amount needed to complete a lot or contract. It is valid within a version of the economic summary.</rdfs:comment>
        <rdfs:isDefinedBy rdf:resource="https://w3id.org/italia/onto/PublicContract"/>
        <rdfs:label xml:lang="it">importo totale</rdfs:label>
        <rdfs:label xml:lang="en">total amount</rdfs:label>
        <owl:versionInfo xml:lang="it">stabile</owl:versionInfo>
        <owl:versionInfo xml:lang="en">stable</owl:versionInfo>
    </owl:DatatypeProperty>
    


    <!-- https://w3id.org/italia/onto/PublicContract/totalAmountPaid -->

    <owl:DatatypeProperty rdf:about="https://w3id.org/italia/onto/PublicContract/totalAmountPaid">
        <rdfs:domain rdf:resource="https://w3id.org/italia/onto/PublicContract/Lot"/>
        <rdfs:range rdf:resource="http://www.w3.org/2001/XMLSchema#float"/>
        <rdfs:comment xml:lang="it">La proprietà che indica l&apos;importo totale liquidato, che corrisponde alla sommatoria dei pagamenti effettuati.</rdfs:comment>
        <rdfs:comment xml:lang="en">The property that represents the total amount paid, that corresponds to the sum of the payments done.</rdfs:comment>
        <rdfs:isDefinedBy rdf:resource="https://w3id.org/italia/onto/PublicContract"/>
        <rdfs:label xml:lang="en">total amount paid</rdfs:label>
        <rdfs:label xml:lang="it">totale importo liquidato</rdfs:label>
        <owl:versionInfo xml:lang="it">stabile</owl:versionInfo>
        <owl:versionInfo xml:lang="en">stable</owl:versionInfo>
    </owl:DatatypeProperty>
    


    <!-- https://w3id.org/italia/onto/PublicContract/variantDate -->

    <owl:DatatypeProperty rdf:about="https://w3id.org/italia/onto/PublicContract/variantDate">
        <rdfs:subPropertyOf rdf:resource="https://w3id.org/italia/onto/TI/date"/>
        <rdfs:domain rdf:resource="https://w3id.org/italia/onto/PublicContract/VariantDocument"/>
        <rdfs:range rdf:resource="http://www.w3.org/2001/XMLSchema#date"/>
        <rdfs:comment xml:lang="it">La proprietà che determina la data di inizio della variante.</rdfs:comment>
        <rdfs:comment xml:lang="en">The property that represents the starting date of the variant.</rdfs:comment>
        <rdfs:isDefinedBy rdf:resource="https://w3id.org/italia/onto/PublicContract"/>
        <rdfs:label xml:lang="it">data variante</rdfs:label>
        <rdfs:label xml:lang="en">variant date</rdfs:label>
        <owl:versionInfo xml:lang="it">stabile</owl:versionInfo>
        <owl:versionInfo xml:lang="en">stable</owl:versionInfo>
    </owl:DatatypeProperty>
    


    <!-- https://w3id.org/italia/onto/PublicContract/variantType -->

    <owl:DatatypeProperty rdf:about="https://w3id.org/italia/onto/PublicContract/variantType">
        <rdfs:domain rdf:resource="https://w3id.org/italia/onto/PublicContract/VariantDocument"/>
        <rdfs:range rdf:resource="http://www.w3.org/2001/XMLSchema#string"/>
        <rdfs:comment xml:lang="it">La proprietà che determina il tipo di variante.</rdfs:comment>
        <rdfs:comment xml:lang="en">The property that represents the type of the variant.</rdfs:comment>
        <rdfs:isDefinedBy rdf:resource="https://w3id.org/italia/onto/PublicContract"/>
        <rdfs:label xml:lang="it">tipo variazione</rdfs:label>
        <rdfs:label xml:lang="en">variant type</rdfs:label>
        <owl:versionInfo xml:lang="it">stabile</owl:versionInfo>
        <owl:versionInfo xml:lang="en">stable</owl:versionInfo>
    </owl:DatatypeProperty>
    


    <!-- https://w3id.org/italia/onto/PublicContract/worksAmount -->

    <owl:DatatypeProperty rdf:about="https://w3id.org/italia/onto/PublicContract/worksAmount">
        <rdfs:domain rdf:resource="https://w3id.org/italia/onto/PublicContract/EconomicSummary"/>
        <rdfs:range rdf:resource="http://www.w3.org/2001/XMLSchema#float"/>
        <rdfs:comment xml:lang="it">La proprietà che determina l&apos;importo stimato per i lavori, nell&apos;ambito di una versione del prospetto economico.</rdfs:comment>
        <rdfs:comment xml:lang="en">The property that represents the works amount. It is valid within a version of the economic summary.</rdfs:comment>
        <rdfs:isDefinedBy rdf:resource="https://w3id.org/italia/onto/PublicContract"/>
        <rdfs:label xml:lang="it">importo lavori</rdfs:label>
        <rdfs:label xml:lang="en">works amount</rdfs:label>
        <owl:versionInfo xml:lang="it">stabile</owl:versionInfo>
        <owl:versionInfo xml:lang="en">stable</owl:versionInfo>
    </owl:DatatypeProperty>
    


    <!-- https://w3id.org/italia/onto/TI/date -->

    <owl:DatatypeProperty rdf:about="https://w3id.org/italia/onto/TI/date"/>
    


    <!-- https://w3id.org/italia/onto/TI/duration -->

    <owl:DatatypeProperty rdf:about="https://w3id.org/italia/onto/TI/duration"/>
    


    <!-- https://w3id.org/italia/onto/TI/endTime -->

    <owl:DatatypeProperty rdf:about="https://w3id.org/italia/onto/TI/endTime"/>
    


    <!-- https://w3id.org/italia/onto/TI/issued -->

    <owl:DatatypeProperty rdf:about="https://w3id.org/italia/onto/TI/issued"/>
    


    <!-- https://w3id.org/italia/onto/TI/startTime -->

    <owl:DatatypeProperty rdf:about="https://w3id.org/italia/onto/TI/startTime"/>
    


    <!-- https://w3id.org/italia/onto/l0/description -->

    <owl:DatatypeProperty rdf:about="https://w3id.org/italia/onto/l0/description"/>
    


    <!-- https://w3id.org/italia/onto/l0/identifier -->

    <owl:DatatypeProperty rdf:about="https://w3id.org/italia/onto/l0/identifier"/>
    


    <!-- https://w3id.org/italia/onto/l0/name -->

    <owl:DatatypeProperty rdf:about="https://w3id.org/italia/onto/l0/name"/>
    


    <!-- 
    ///////////////////////////////////////////////////////////////////////////////////////
    //
    // Classes
    //
    ///////////////////////////////////////////////////////////////////////////////////////
     -->

    


    <!-- https://w3id.org/italia/onto/PublicContract/AmendmentDocument -->

    <owl:Class rdf:about="https://w3id.org/italia/onto/PublicContract/AmendmentDocument">
        <rdfs:subClassOf rdf:resource="https://w3id.org/italia/onto/PublicContract/ProcurementDocument"/>
        <rdfs:comment xml:lang="it">La classe che rappresenta il documento che stabilisce una modifica nelle caratteristiche di un lotto o contratto.</rdfs:comment>
        <rdfs:comment xml:lang="en">The class that represents the document setting a change in the characteristics of a lot or contract.</rdfs:comment>
        <rdfs:isDefinedBy rdf:resource="https://w3id.org/italia/onto/PublicContract"/>
        <rdfs:label xml:lang="en">Amendement document</rdfs:label>
        <rdfs:label xml:lang="it">Documento di modifica</rdfs:label>
        <owl:versionInfo xml:lang="it">stabile</owl:versionInfo>
        <owl:versionInfo xml:lang="en">stable</owl:versionInfo>
        <prov:wasInfluencedBy rdf:resource="http://w3id.org/ocds/ns#Amendment"/>
    </owl:Class>
    


    <!-- https://w3id.org/italia/onto/PublicContract/AmendmentRationale -->

    <owl:Class rdf:about="https://w3id.org/italia/onto/PublicContract/AmendmentRationale">
        <rdfs:subClassOf rdf:resource="https://w3id.org/italia/onto/l0/Characteristic"/>
        <rdfs:comment xml:lang="en">Abstract class that groups the different types of reasons for the admendments.</rdfs:comment>
        <rdfs:comment xml:lang="it">Classe astratta che raggruppa i diversi tipi di  motivazioni per la modifica</rdfs:comment>
        <rdfs:isDefinedBy rdf:resource="https://w3id.org/italia/onto/PublicContract"/>
        <rdfs:label xml:lang="en">Amendment Rationale</rdfs:label>
        <rdfs:label xml:lang="it">Motivazione della Modifica</rdfs:label>
        <owl:versionInfo xml:lang="it">stabile</owl:versionInfo>
        <owl:versionInfo xml:lang="en">stable</owl:versionInfo>
    </owl:Class>
    


    <!-- https://w3id.org/italia/onto/PublicContract/Award -->

    <owl:Class rdf:about="https://w3id.org/italia/onto/PublicContract/Award">
        <rdfs:subClassOf rdf:resource="https://w3id.org/italia/onto/l0/EventOrSituation"/>
        <rdfs:isDefinedBy rdf:resource="https://w3id.org/italia/onto/PublicContract"/>
        <rdfs:label xml:lang="it">Aggiudicazione</rdfs:label>
        <rdfs:label xml:lang="en">Award</rdfs:label>
        <rdfs:label xml:lang="en">Selection</rdfs:label>
        <rdfs:label xml:lang="it">Selezione</rdfs:label>
        <owl:versionInfo xml:lang="it">provvisoria</owl:versionInfo>
        <owl:versionInfo xml:lang="en">unstable</owl:versionInfo>
        <prov:wasDerivedFrom rdf:resource="http://w3id.org/ocds/ns#Award"/>
    </owl:Class>
    


    <!-- https://w3id.org/italia/onto/PublicContract/AwardCriterion -->

    <owl:Class rdf:about="https://w3id.org/italia/onto/PublicContract/AwardCriterion">
        <rdfs:subClassOf rdf:resource="https://w3id.org/italia/onto/l0/Characteristic"/>
        <rdfs:comment xml:lang="it">Le istanze di questa classe rappresentano il criterio di aggiudicazione (tipicamente, il criterio dell&apos;offerta economicamente più vantaggiosa o del prezzo più basso) adottato nell&apos;ambito di una procedura di affidamento.</rdfs:comment>
        <rdfs:comment xml:lang="en">The class that represents the award criteria (e.g., &quot;most economically advantageous tender&quot; or &quot;lowest price&quot;) adopted for awarding. The instances of this class, at the moment are &quot;most economically advantageous tender&quot; and &quot;lowest price&quot;</rdfs:comment>
        <rdfs:isDefinedBy rdf:resource="https://w3id.org/italia/onto/PublicContract"/>
        <rdfs:label xml:lang="en">Award Criterion</rdfs:label>
        <rdfs:label xml:lang="it">Criterio di Aggiudicazione</rdfs:label>
        <rdfs:label xml:lang="it">Criterio di Selezione</rdfs:label>
        <rdfs:label xml:lang="en">Selection Criterion</rdfs:label>
        <owl:versionInfo xml:lang="it">stabile</owl:versionInfo>
        <owl:versionInfo xml:lang="en">stable</owl:versionInfo>
        <prov:wasDerivedFrom rdf:resource="http://w3id.org/ocds/ns#AwardCriteria"/>
        <prov:wasInfluencedBy rdf:resource="http://data.europa.eu/m8g/Criterion"/>
    </owl:Class>
    


    <!-- https://w3id.org/italia/onto/PublicContract/AwardNotice -->

    <owl:Class rdf:about="https://w3id.org/italia/onto/PublicContract/AwardNotice">
        <rdfs:subClassOf rdf:resource="https://w3id.org/italia/onto/PublicContract/Notice"/>
        <rdfs:subClassOf>
            <owl:Restriction>
                <owl:onProperty rdf:resource="https://w3id.org/italia/onto/PublicContract/winner"/>
                <owl:allValuesFrom rdf:resource="https://w3id.org/italia/onto/l0/Agent"/>
            </owl:Restriction>
        </rdfs:subClassOf>
        <rdfs:comment xml:lang="it">La classe che rappresenta l&apos;esito della procedura di affidamento, ovvero il documento che attesta l&apos;attribuzione di un lotto a un offerente. L&apos;attribuzione può avvenire tramite aggiudicazione, affidamento o adesione a un accordo quadro, a seconda della tipologia di procedura.</rdfs:comment>
        <rdfs:comment xml:lang="en">The class that represents the document that certifies the outcome of a procedure, namely the attribution of a lot to a bidder. Depending on the type of the procedure, the attribution can be an open award, a direct award, or a framework agreement.</rdfs:comment>
        <rdfs:isDefinedBy rdf:resource="https://w3id.org/italia/onto/PublicContract"/>
        <rdfs:label xml:lang="it">Avviso Esito di Procedura</rdfs:label>
        <rdfs:label xml:lang="en">Award Notice</rdfs:label>
        <owl:versionInfo xml:lang="it">stabile</owl:versionInfo>
        <owl:versionInfo xml:lang="en">stable</owl:versionInfo>
        <prov:wasInfluencedBy rdf:resource="http://contsem.unizar.es/def/sector-publico/pproc#ContractAwardNotice"/>
    </owl:Class>
    


    <!-- https://w3id.org/italia/onto/PublicContract/CPV -->

    <owl:Class rdf:about="https://w3id.org/italia/onto/PublicContract/CPV">
        <rdfs:subClassOf rdf:resource="https://w3id.org/italia/onto/l0/Characteristic"/>
        <rdfs:comment xml:lang="it">La Classe che rappresenta il CPV (Common Procurement Vocabular) con cui è classificata una procedura, un lotto o un contratto. Le istanze di questa classe possono essere rappresentate come concetti dello standard skos di un vocabolario controllato.</rdfs:comment>
        <rdfs:comment xml:lang="en">The class that represents the CPV (Common Procurement Vocabulary), code describing the main object of a procedure, lot or contract. The instances of this class can be represented as skos concepts of a controlled vocabulary.</rdfs:comment>
        <rdfs:isDefinedBy rdf:resource="https://w3id.org/italia/onto/PublicContract"/>
        <rdfs:label xml:lang="en">CPV (Common Procurement Vocabulary)</rdfs:label>
        <rdfs:label xml:lang="it">CPV (Vocabolario comune per gli appaltii)</rdfs:label>
        <owl:versionInfo xml:lang="it">stabile</owl:versionInfo>
        <owl:versionInfo xml:lang="en">stable</owl:versionInfo>
        <prov:wasDerivedFrom rdf:resource="http://www.w3.org/2004/02/skos/core#Concept"/>
    </owl:Class>
    


    <!-- https://w3id.org/italia/onto/PublicContract/CallForCompetition -->

    <owl:Class rdf:about="https://w3id.org/italia/onto/PublicContract/CallForCompetition">
        <rdfs:subClassOf rdf:resource="https://w3id.org/italia/onto/PublicContract/Notice"/>
        <rdfs:comment xml:lang="it">La classe che rappresenta un bando di gara pubblico.</rdfs:comment>
        <rdfs:comment xml:lang="en">This class represents a public call for tender.</rdfs:comment>
        <rdfs:isDefinedBy rdf:resource="https://w3id.org/italia/onto/PublicContract"/>
        <rdfs:label xml:lang="it">Bando di Gara</rdfs:label>
        <rdfs:label xml:lang="en">Call for Competition</rdfs:label>
        <owl:versionInfo xml:lang="it">stabile</owl:versionInfo>
        <owl:versionInfo xml:lang="en">stable</owl:versionInfo>
        <prov:wasDerivedFrom rdf:resource="http://data.europa.eu/eproc/ontology#CallForTender"/>
    </owl:Class>
    


    <!-- https://w3id.org/italia/onto/PublicContract/Concession -->

    <owl:Class rdf:about="https://w3id.org/italia/onto/PublicContract/Concession">
        <rdfs:subClassOf rdf:resource="https://w3id.org/italia/onto/PublicContract/Procedure"/>
        <rdfs:comment xml:lang="it">La classe che rappresenta la modalità di realizzazione di una gara tramite concessione.</rdfs:comment>
        <rdfs:comment xml:lang="en">The class that represents the implementation of a procedure through a concession.</rdfs:comment>
        <rdfs:isDefinedBy rdf:resource="https://w3id.org/italia/onto/PublicContract"/>
        <rdfs:label xml:lang="en">Concession</rdfs:label>
        <rdfs:label xml:lang="it">Concessione</rdfs:label>
        <owl:versionInfo xml:lang="it">stabile</owl:versionInfo>
        <owl:versionInfo xml:lang="en">stable</owl:versionInfo>
    </owl:Class>
    


    <!-- https://w3id.org/italia/onto/PublicContract/Contract -->

    <owl:Class rdf:about="https://w3id.org/italia/onto/PublicContract/Contract">
        <rdfs:subClassOf rdf:resource="https://w3id.org/italia/onto/PublicContract/Document"/>
        <rdfs:subClassOf>
            <owl:Restriction>
                <owl:onProperty rdf:resource="https://w3id.org/italia/onto/PublicContract/hasCPV"/>
                <owl:someValuesFrom rdf:resource="https://w3id.org/italia/onto/PublicContract/CPV"/>
            </owl:Restriction>
        </rdfs:subClassOf>
        <rdfs:subClassOf>
            <owl:Restriction>
                <owl:onProperty rdf:resource="https://w3id.org/italia/onto/PublicContract/refersToTender"/>
                <owl:someValuesFrom rdf:resource="https://w3id.org/italia/onto/PublicContract/Tender"/>
            </owl:Restriction>
        </rdfs:subClassOf>
        <rdfs:subClassOf>
            <owl:Restriction>
                <owl:onProperty rdf:resource="https://w3id.org/italia/onto/PublicContract/hasChangeDocument"/>
                <owl:allValuesFrom rdf:resource="https://w3id.org/italia/onto/PublicContract/AmendmentDocument"/>
            </owl:Restriction>
        </rdfs:subClassOf>
        <rdfs:subClassOf>
            <owl:Restriction>
                <owl:onProperty rdf:resource="https://w3id.org/italia/onto/PublicContract/hasContractualResolution"/>
                <owl:allValuesFrom rdf:resource="https://w3id.org/italia/onto/PublicContract/Resolution"/>
            </owl:Restriction>
        </rdfs:subClassOf>
        <rdfs:subClassOf>
            <owl:Restriction>
                <owl:onProperty rdf:resource="https://w3id.org/italia/onto/PublicContract/hasEconomicSummary"/>
                <owl:allValuesFrom rdf:resource="https://w3id.org/italia/onto/PublicContract/EconomicSummary"/>
            </owl:Restriction>
        </rdfs:subClassOf>
        <rdfs:subClassOf>
            <owl:Restriction>
                <owl:onProperty rdf:resource="https://w3id.org/italia/onto/PublicContract/winner"/>
                <owl:allValuesFrom rdf:resource="https://w3id.org/italia/onto/l0/Agent"/>
            </owl:Restriction>
        </rdfs:subClassOf>
        <rdfs:subClassOf>
            <owl:Restriction>
                <owl:onProperty rdf:resource="https://w3id.org/italia/onto/RO/holdsRoleInTime"/>
                <owl:allValuesFrom rdf:resource="https://w3id.org/italia/onto/RO/TimeIndexedRole"/>
            </owl:Restriction>
        </rdfs:subClassOf>
        <rdfs:subClassOf>
            <owl:Restriction>
                <owl:onProperty rdf:resource="https://w3id.org/italia/onto/PublicContract/hasFrameworkAgreement"/>
                <owl:maxQualifiedCardinality rdf:datatype="http://www.w3.org/2001/XMLSchema#nonNegativeInteger">1</owl:maxQualifiedCardinality>
                <owl:onClass rdf:resource="https://w3id.org/italia/onto/PublicContract/FrameworkAgreement"/>
            </owl:Restriction>
        </rdfs:subClassOf>
        <rdfs:comment xml:lang="en">An instance of this class is an abstract information entity about a realized contract between a contracting authority and their supplier.</rdfs:comment>
        <rdfs:comment xml:lang="it">Una istanza di questa classe rappresenta un contratto realizzato tra due o più agenti: ad esempio, tra una stazione appaltante ed un fornitore.</rdfs:comment>
        <rdfs:isDefinedBy rdf:resource="https://w3id.org/italia/onto/PublicContract"/>
        <rdfs:label xml:lang="en">Contract</rdfs:label>
        <rdfs:label xml:lang="it">Contratto</rdfs:label>
        <owl:versionInfo xml:lang="it">stabile</owl:versionInfo>
        <owl:versionInfo xml:lang="en">stable</owl:versionInfo>
        <prov:wasDerivedFrom rdf:resource="http://w3id.org/ocds/ns#Contract"/>
        <prov:wasDerivedFrom rdf:resource="http://www.omg.org/spec/EDMC-FIBO/FND/Agreements/Contracts/Contract"/>
    </owl:Class>
    


    <!-- https://w3id.org/italia/onto/PublicContract/DirectAdministration -->

    <owl:Class rdf:about="https://w3id.org/italia/onto/PublicContract/DirectAdministration">
        <rdfs:subClassOf rdf:resource="https://w3id.org/italia/onto/PublicContract/Procedure"/>
        <rdfs:comment xml:lang="it">La classe che rappresenta la modalità di realizzazione di una gara tramite amministrazione diretta.</rdfs:comment>
        <rdfs:comment xml:lang="en">The class that represents the implementation of a procedure through a direct administration.</rdfs:comment>
        <rdfs:isDefinedBy rdf:resource="https://w3id.org/italia/onto/PublicContract"/>
        <rdfs:label xml:lang="it">Amministrazione diretta</rdfs:label>
        <rdfs:label xml:lang="en">Direct administration</rdfs:label>
        <owl:versionInfo xml:lang="it">stabile</owl:versionInfo>
        <owl:versionInfo xml:lang="en">stable</owl:versionInfo>
    </owl:Class>
    


    <!-- https://w3id.org/italia/onto/PublicContract/Document -->

    <owl:Class rdf:about="https://w3id.org/italia/onto/PublicContract/Document">
        <rdfs:subClassOf rdf:resource="https://w3id.org/italia/onto/l0/Object"/>
        <rdfs:subClassOf>
            <owl:Restriction>
                <owl:onProperty rdf:resource="https://w3id.org/italia/onto/l0/identifier"/>
                <owl:cardinality rdf:datatype="http://www.w3.org/2001/XMLSchema#nonNegativeInteger">1</owl:cardinality>
            </owl:Restriction>
        </rdfs:subClassOf>
        <rdfs:comment xml:lang="it">La classe che rappresenta i vari documenti coinvolti in tutte le fasi di procurement</rdfs:comment>
        <rdfs:comment xml:lang="en">The class that represents all the various documents involved in the different procurement phases</rdfs:comment>
        <rdfs:isDefinedBy rdf:resource="https://w3id.org/italia/onto/PublicContract"/>
        <rdfs:label xml:lang="en">Document</rdfs:label>
        <rdfs:label xml:lang="it">Documento</rdfs:label>
        <owl:versionInfo xml:lang="it">provvisoria</owl:versionInfo>
        <owl:versionInfo xml:lang="en">unstable</owl:versionInfo>
        <prov:wasDerivedFrom rdf:resource="http://data.europa.eu/eproc/ontology#Document"/>
        <prov:wasDerivedFrom rdf:resource="http://w3id.org/ocds/ns#Document"/>
    </owl:Class>
    


    <!-- https://w3id.org/italia/onto/PublicContract/EconomicSummary -->

    <owl:Class rdf:about="https://w3id.org/italia/onto/PublicContract/EconomicSummary">
        <rdfs:subClassOf rdf:resource="https://w3id.org/italia/onto/l0/Characteristic"/>
        <rdfs:comment xml:lang="en">An instance of this class represents the economic summary of a lot or contract. Dates and amounts related to the economic summary are usually defined during the awarding and negotiation stages. Amounts may be imported from the &quot;economic framework&quot; that is periodically drawn up. The economic summary may be reshaped following a change event (e.g., a variant or a suspension). Such a modification creates a new economic summary which replaces the former and where dates and amounts are updated.</rdfs:comment>
        <rdfs:comment xml:lang="it">Un&apos;istanza di questa classe rappresenta il prospetto economico di un lotto o contratto. Date e ammontari contenuti nel prospetto sono generalmente definiti nelle fasi preliminari di aggiudicazione, affidamento, contrattazione e redazione del quadro economico. Il prospetto economico, così come il quadro economico che eventualmente lo alimenta in merito agli ammontari, può essere rimodulato in seguito a un evento di cambiamento (per esempio, una variante in corso d&apos;opera o una sospensione). Tale modifica genera un nuovo prospetto economico che sostituisce il precedente, e aggiorna i valori di date e ammontari in base a quanto stabilito nei documenti di modifica corrispondenti all&apos;evento di cambiamento stesso</rdfs:comment>
        <rdfs:isDefinedBy rdf:resource="https://w3id.org/italia/onto/PublicContract"/>
        <rdfs:label xml:lang="en">Economic summary</rdfs:label>
        <rdfs:label xml:lang="it">Prospetto economico</rdfs:label>
        <owl:versionInfo xml:lang="it">stabile</owl:versionInfo>
        <owl:versionInfo xml:lang="en">stable</owl:versionInfo>
    </owl:Class>
    


    <!-- https://w3id.org/italia/onto/PublicContract/FrameworkAgreement -->

    <owl:Class rdf:about="https://w3id.org/italia/onto/PublicContract/FrameworkAgreement">
        <rdfs:subClassOf rdf:resource="https://w3id.org/italia/onto/PublicContract/Procedure"/>
        <rdfs:comment xml:lang="it">La classe che rappresenta la modalità di realizzazione di una gara tramite un accordo quadro.</rdfs:comment>
        <rdfs:comment xml:lang="en">The class that represents the implementation of a procedure through a framework agreement.</rdfs:comment>
        <rdfs:isDefinedBy rdf:resource="https://w3id.org/italia/onto/PublicContract"/>
        <rdfs:label xml:lang="it">Accordo quadro</rdfs:label>
        <rdfs:label xml:lang="en">Framework agreement</rdfs:label>
        <owl:versionInfo xml:lang="it">stabile</owl:versionInfo>
        <owl:versionInfo xml:lang="en">stable</owl:versionInfo>
    </owl:Class>
    


    <!-- https://w3id.org/italia/onto/PublicContract/Inspection -->

    <owl:Class rdf:about="https://w3id.org/italia/onto/PublicContract/Inspection">
        <rdfs:subClassOf rdf:resource="https://w3id.org/italia/onto/l0/EventOrSituation"/>
        <rdfs:comment xml:lang="it">Le istanze di questa classe rappresentano i dati sulla fase di collaudo</rdfs:comment>
        <rdfs:comment xml:lang="en">The instances of this class represent the data regarding the inspection</rdfs:comment>
        <rdfs:isDefinedBy rdf:resource="https://w3id.org/italia/onto/PublicContract"/>
        <rdfs:label xml:lang="it">Collaudo</rdfs:label>
        <rdfs:label xml:lang="en">Inspection</rdfs:label>
        <owl:versionInfo xml:lang="it">provvisoria</owl:versionInfo>
        <owl:versionInfo xml:lang="en">unstable</owl:versionInfo>
    </owl:Class>
    


    <!-- https://w3id.org/italia/onto/PublicContract/Lot -->

    <owl:Class rdf:about="https://w3id.org/italia/onto/PublicContract/Lot">
        <rdfs:subClassOf rdf:resource="https://w3id.org/italia/onto/PublicContract/ProcurementProject"/>
        <rdfs:subClassOf>
            <owl:Restriction>
                <owl:onProperty rdf:resource="https://w3id.org/italia/onto/PublicContract/hasCPV"/>
                <owl:someValuesFrom rdf:resource="https://w3id.org/italia/onto/PublicContract/CPV"/>
            </owl:Restriction>
        </rdfs:subClassOf>
        <rdfs:subClassOf>
            <owl:Restriction>
                <owl:onProperty rdf:resource="https://w3id.org/italia/onto/PublicContract/hasContract"/>
                <owl:allValuesFrom rdf:resource="https://w3id.org/italia/onto/PublicContract/Contract"/>
            </owl:Restriction>
        </rdfs:subClassOf>
        <rdfs:subClassOf>
            <owl:Restriction>
                <owl:onProperty rdf:resource="https://w3id.org/italia/onto/PublicContract/isIncludedInProcedure"/>
                <owl:qualifiedCardinality rdf:datatype="http://www.w3.org/2001/XMLSchema#nonNegativeInteger">1</owl:qualifiedCardinality>
                <owl:onClass rdf:resource="https://w3id.org/italia/onto/PublicContract/Procedure"/>
            </owl:Restriction>
        </rdfs:subClassOf>
        <rdfs:subClassOf>
            <owl:Restriction>
                <owl:onProperty rdf:resource="https://w3id.org/italia/onto/PublicContract/CIG"/>
                <owl:cardinality rdf:datatype="http://www.w3.org/2001/XMLSchema#nonNegativeInteger">1</owl:cardinality>
            </owl:Restriction>
        </rdfs:subClassOf>
        <owl:disjointWith rdf:resource="https://w3id.org/italia/onto/PublicContract/Procedure"/>
        <rdfs:comment xml:lang="en">One of the parts of a procurement project that is being subdivided to allow the buyer to award different lots to different economic operators under different contracts.</rdfs:comment>
        <rdfs:comment xml:lang="it">Una delle parti in cui è suddiviso un progetto di procurement. La suddivisione in lotti ha lo scopo di consentire alla stazione appaltante di aggiudicare diversi lotti a diversi operatori economici tramite contratti distinti.</rdfs:comment>
        <rdfs:isDefinedBy rdf:resource="https://w3id.org/italia/onto/PublicContract"/>
        <rdfs:label xml:lang="en">Lot</rdfs:label>
        <rdfs:label xml:lang="it">Lotto</rdfs:label>
        <owl:versionInfo xml:lang="it">stabile</owl:versionInfo>
        <owl:versionInfo xml:lang="en">stable</owl:versionInfo>
    </owl:Class>
    


    <!-- https://w3id.org/italia/onto/PublicContract/Notice -->

    <owl:Class rdf:about="https://w3id.org/italia/onto/PublicContract/Notice">
        <rdfs:subClassOf rdf:resource="https://w3id.org/italia/onto/PublicContract/ProcurementDocument"/>
        <rdfs:subClassOf>
            <owl:Restriction>
                <owl:onProperty rdf:resource="https://w3id.org/italia/onto/PublicContract/hasCPV"/>
                <owl:someValuesFrom rdf:resource="https://w3id.org/italia/onto/PublicContract/CPV"/>
            </owl:Restriction>
        </rdfs:subClassOf>
        <rdfs:subClassOf>
            <owl:Restriction>
                <owl:onProperty rdf:resource="https://w3id.org/italia/onto/PublicContract/hasNoticeType"/>
                <owl:maxQualifiedCardinality rdf:datatype="http://www.w3.org/2001/XMLSchema#nonNegativeInteger">1</owl:maxQualifiedCardinality>
                <owl:onClass rdf:resource="https://w3id.org/italia/onto/PublicContract/NoticeType"/>
            </owl:Restriction>
        </rdfs:subClassOf>
        <rdfs:comment xml:lang="it">La classe che rappresenta qualunque tipo di annuncio o avviso relativo ad una procedura di affidamento. Tipicamente, un bando pubblico o un&apos;altra tipologia di avviso o invito.</rdfs:comment>
        <rdfs:comment xml:lang="en">This class represents any kind of notice or announcement related to a procedure of actualization of an intervention. Usually, it refers to a public call or any kind of notice or invitation.</rdfs:comment>
        <rdfs:isDefinedBy rdf:resource="https://w3id.org/italia/onto/PublicContract"/>
        <rdfs:label xml:lang="it">Avviso</rdfs:label>
        <rdfs:label xml:lang="en">Notice</rdfs:label>
        <owl:versionInfo xml:lang="it">stabile</owl:versionInfo>
        <owl:versionInfo xml:lang="en">stable</owl:versionInfo>
    </owl:Class>
    


    <!-- https://w3id.org/italia/onto/PublicContract/NoticeType -->

    <owl:Class rdf:about="https://w3id.org/italia/onto/PublicContract/NoticeType">
        <rdfs:subClassOf rdf:resource="https://w3id.org/italia/onto/l0/Characteristic"/>
        <rdfs:comment xml:lang="it">La classe che rappresenta il tipo di bando o avviso.</rdfs:comment>
        <rdfs:comment xml:lang="en">The class that represents the type of notice.</rdfs:comment>
        <rdfs:isDefinedBy rdf:resource="https://w3id.org/italia/onto/PublicContract"/>
        <rdfs:label xml:lang="en">Notice type</rdfs:label>
        <rdfs:label xml:lang="it">Tipologia dell&apos;avviso</rdfs:label>
        <owl:versionInfo xml:lang="it">provvisoria</owl:versionInfo>
        <owl:versionInfo xml:lang="en">unstable</owl:versionInfo>
        <prov:wasDerivedFrom rdf:resource="http://www.w3.org/2004/02/skos/core#Concept"/>
    </owl:Class>
    


    <!-- https://w3id.org/italia/onto/PublicContract/Payment -->

    <owl:Class rdf:about="https://w3id.org/italia/onto/PublicContract/Payment">
        <rdfs:subClassOf rdf:resource="https://w3id.org/italia/onto/l0/EventOrSituation"/>
        <rdfs:comment xml:lang="en">An instance of this class represents a payment made by the contracting authority.</rdfs:comment>
        <rdfs:comment xml:lang="it">La classe che rappresenta il pagamento effettuato dalla stazione appaltante.</rdfs:comment>
        <rdfs:isDefinedBy rdf:resource="https://w3id.org/italia/onto/PublicContract"/>
        <rdfs:label xml:lang="it">Pagamento</rdfs:label>
        <rdfs:label xml:lang="en">Payment</rdfs:label>
        <owl:versionInfo xml:lang="it">provvisoria</owl:versionInfo>
        <owl:versionInfo xml:lang="en">unstable</owl:versionInfo>
        <prov:wasInfluencedBy rdf:resource="http://data.europa.eu/eproc/ontology#Payment"/>
    </owl:Class>
    


    <!-- https://w3id.org/italia/onto/PublicContract/PaymentCertificate -->

    <owl:Class rdf:about="https://w3id.org/italia/onto/PublicContract/PaymentCertificate">
        <rdfs:subClassOf rdf:resource="https://w3id.org/italia/onto/PublicContract/Document"/>
        <rdfs:comment xml:lang="it">La classe che rappresenta il certificato di pagamento emesso dalla stazione appaltante, generalmente deliberato nell&apos;ambito di un SAL (Stato Avanzamento Lavori).</rdfs:comment>
        <rdfs:comment xml:lang="en">The class that represents the certificate of payment issued by the contracting authority, usually approved by the work progress report.</rdfs:comment>
        <rdfs:isDefinedBy rdf:resource="https://w3id.org/italia/onto/PublicContract"/>
        <rdfs:label xml:lang="it">Certificato di pagamento</rdfs:label>
        <rdfs:label xml:lang="en">Payment certificate</rdfs:label>
        <owl:versionInfo xml:lang="it">stabile</owl:versionInfo>
        <owl:versionInfo xml:lang="en">stable</owl:versionInfo>
    </owl:Class>
    


    <!-- https://w3id.org/italia/onto/PublicContract/Procedure -->

    <owl:Class rdf:about="https://w3id.org/italia/onto/PublicContract/Procedure">
        <rdfs:subClassOf rdf:resource="https://w3id.org/italia/onto/PublicContract/ProcurementProject"/>
        <rdfs:subClassOf>
            <owl:Restriction>
                <owl:onProperty rdf:resource="https://w3id.org/italia/onto/PublicContract/hasCPV"/>
                <owl:someValuesFrom rdf:resource="https://w3id.org/italia/onto/PublicContract/CPV"/>
            </owl:Restriction>
        </rdfs:subClassOf>
        <rdfs:subClassOf>
            <owl:Restriction>
                <owl:onProperty rdf:resource="https://w3id.org/italia/onto/PublicContract/hasProcurementDocument"/>
                <owl:someValuesFrom rdf:resource="https://w3id.org/italia/onto/PublicContract/ProcurementDocument"/>
            </owl:Restriction>
        </rdfs:subClassOf>
        <rdfs:subClassOf>
            <owl:Restriction>
                <owl:onProperty rdf:resource="https://w3id.org/italia/onto/PublicContract/includesLot"/>
                <owl:someValuesFrom rdf:resource="https://w3id.org/italia/onto/PublicContract/Lot"/>
            </owl:Restriction>
        </rdfs:subClassOf>
        <rdfs:subClassOf>
            <owl:Restriction>
                <owl:onProperty rdf:resource="https://w3id.org/italia/onto/RO/holdsRoleInTime"/>
                <owl:allValuesFrom rdf:resource="https://w3id.org/italia/onto/RO/TimeIndexedRole"/>
            </owl:Restriction>
        </rdfs:subClassOf>
        <rdfs:subClassOf>
            <owl:Restriction>
                <owl:onProperty rdf:resource="https://w3id.org/italia/onto/PublicContract/hasProcuringEntity"/>
                <owl:qualifiedCardinality rdf:datatype="http://www.w3.org/2001/XMLSchema#nonNegativeInteger">1</owl:qualifiedCardinality>
                <owl:onClass rdf:resource="https://w3id.org/italia/onto/l0/Agent"/>
            </owl:Restriction>
        </rdfs:subClassOf>
        <rdfs:subClassOf>
            <owl:Restriction>
                <owl:onProperty rdf:resource="https://w3id.org/italia/onto/l0/identifier"/>
                <owl:cardinality rdf:datatype="http://www.w3.org/2001/XMLSchema#nonNegativeInteger">1</owl:cardinality>
            </owl:Restriction>
        </rdfs:subClassOf>
        <rdfs:comment xml:lang="it">La classe che comprende le attività che una stazione appaltante mette in atto per realizzare un progetto di procurement, ad esempio le attività svolte tramite un contratto di appalto o di concessione, le attività realizzate attraverso amministrazione diretta,  parternariato pubblico/privato o adesione ad un accordo quadro. Le attività prevedono step procedurali che possono variare in relazione alla modalità di realizzazione.</rdfs:comment>
        <rdfs:comment xml:lang="en">The class that represents the activities that a contracting authority carries out in order to actualize a procurement project, such as those carried out through public procurement, concession, direct administration, public/private partnership or framework agreement. The steps of the procedure may vary according to the type of the procedure. Information.</rdfs:comment>
        <rdfs:isDefinedBy rdf:resource="https://w3id.org/italia/onto/PublicContract"/>
        <rdfs:label xml:lang="it">Gara</rdfs:label>
        <rdfs:label xml:lang="it">Modalità di realizzazione</rdfs:label>
        <rdfs:label xml:lang="it">Procedimento</rdfs:label>
        <rdfs:label xml:lang="it">Procedura di affidamento</rdfs:label>
        <rdfs:label xml:lang="en">Procedure</rdfs:label>
        <owl:versionInfo xml:lang="it">stabile</owl:versionInfo>
        <owl:versionInfo xml:lang="en">stable</owl:versionInfo>
    </owl:Class>
    


    <!-- https://w3id.org/italia/onto/PublicContract/ProcedureChangeEvent -->

    <owl:Class rdf:about="https://w3id.org/italia/onto/PublicContract/ProcedureChangeEvent">
        <rdfs:subClassOf rdf:resource="https://w3id.org/italia/onto/l0/EventOrSituation"/>
        <rdfs:comment xml:lang="en">An instance of this class represents an event of modification, for example an event leading to the reshaping of the economic summary.</rdfs:comment>
        <rdfs:comment xml:lang="it">Una istanza di questa classe rappresenta un evento di cambiamento, per esempio un evento che porta a una rimodulazione del prospetto economico di una procedura.</rdfs:comment>
        <rdfs:isDefinedBy rdf:resource="https://w3id.org/italia/onto/PublicContract"/>
        <rdfs:label xml:lang="it">Evento di cambiamento per il procedimento</rdfs:label>
        <rdfs:label xml:lang="en">Procedure Change eEvent</rdfs:label>
        <owl:versionInfo xml:lang="it">stabile</owl:versionInfo>
        <owl:versionInfo xml:lang="en">stable</owl:versionInfo>
        <prov:wasDerivedFrom rdf:resource="http://w3id.org/ocds/ns#Change"/>
    </owl:Class>
    


    <!-- https://w3id.org/italia/onto/PublicContract/ProcedureType -->

    <owl:Class rdf:about="https://w3id.org/italia/onto/PublicContract/ProcedureType">
        <rdfs:subClassOf rdf:resource="https://w3id.org/italia/onto/l0/Characteristic"/>
        <rdfs:comment xml:lang="it">La Classe che rappresenta la modalità di scelta del contraente (per esempio, secondo la procedura dell&apos;affidamento diretto, della procedura aperta o della procedura ristretta), che caratterizza la procedura di affidamento di un lotto, secondo le specifiche tecniche degli XML ex L.190/2012 previste da ANAC. La modalità di scelta del contraente va indicata in compatibilità con le diverse sotto-classi della procedura di affidamento, per cui ad ogni sotto-classe possono corrispondere solo alcune modalità. Le istanze di questa classe possono essere rappresentate come concetti dello standard skos di un vocabolario controllato. </rdfs:comment>
        <rdfs:comment xml:lang="en">The class that represents the type of procedure (e.g, direct award, open tender procedure, restricted tender procedure) as provided for by XML ex L.190/2012 technical requirements exploited by ANAC. The instances of this class can be represented as skos concepts of a controlled vocabulary.</rdfs:comment>
        <rdfs:isDefinedBy rdf:resource="https://w3id.org/italia/onto/PublicContract"/>
        <rdfs:label xml:lang="it">Procedura di Scelta del Contraente</rdfs:label>
        <rdfs:label xml:lang="en">Procedure type</rdfs:label>
        <owl:versionInfo xml:lang="it">stabile</owl:versionInfo>
        <owl:versionInfo xml:lang="en">stable</owl:versionInfo>
        <prov:wasDerivedFrom rdf:resource="http://www.w3.org/2004/02/skos/core#Concept"/>
        <prov:wasInfluencedBy rdf:resource="http://w3id.org/ocds/ns#Method"/>
    </owl:Class>
    


    <!-- https://w3id.org/italia/onto/PublicContract/ProcurementDocument -->

    <owl:Class rdf:about="https://w3id.org/italia/onto/PublicContract/ProcurementDocument">
        <rdfs:subClassOf rdf:resource="https://w3id.org/italia/onto/PublicContract/Document"/>
        <rdfs:comment xml:lang="it">La classe che rappresenta un documento emesso dalla stazione appaltante nel corso di una procedura di realizzazione.</rdfs:comment>
        <rdfs:comment xml:lang="en">The class that represents the document issued by the contracting authority during the course of a procedure.</rdfs:comment>
        <rdfs:isDefinedBy rdf:resource="https://w3id.org/italia/onto/PublicContract"/>
        <rdfs:label xml:lang="it">Documento dell&apos;approvvigionamento</rdfs:label>
        <rdfs:label xml:lang="en">Procurement Document</rdfs:label>
        <owl:versionInfo xml:lang="it">stabile</owl:versionInfo>
        <owl:versionInfo xml:lang="en">stable</owl:versionInfo>
    </owl:Class>
    


    <!-- https://w3id.org/italia/onto/PublicContract/ProcurementProject -->

    <owl:Class rdf:about="https://w3id.org/italia/onto/PublicContract/ProcurementProject">
        <rdfs:subClassOf rdf:resource="https://w3id.org/italia/onto/l0/Activity"/>
        <rdfs:subClassOf>
            <owl:Restriction>
                <owl:onProperty rdf:resource="https://w3id.org/italia/onto/PublicContract/hasChangeDocument"/>
                <owl:allValuesFrom rdf:resource="https://w3id.org/italia/onto/PublicContract/AmendmentDocument"/>
            </owl:Restriction>
        </rdfs:subClassOf>
        <rdfs:subClassOf>
            <owl:Restriction>
                <owl:onProperty rdf:resource="https://w3id.org/italia/onto/PublicContract/hasEconomicSummary"/>
                <owl:allValuesFrom rdf:resource="https://w3id.org/italia/onto/PublicContract/EconomicSummary"/>
            </owl:Restriction>
        </rdfs:subClassOf>
        <rdfs:subClassOf>
            <owl:Restriction>
                <owl:onProperty rdf:resource="https://w3id.org/italia/onto/l0/description"/>
                <owl:someValuesFrom rdf:resource="http://www.w3.org/2000/01/rdf-schema#Literal"/>
            </owl:Restriction>
        </rdfs:subClassOf>
        <rdfs:comment xml:lang="it">La classe che comprende i progetti atti a soddisfare un fabbisogno individuato dall&apos;amministrazione.</rdfs:comment>
        <rdfs:comment xml:lang="en">The class that includes projects aiming at meet the needs detected by a public administration.</rdfs:comment>
        <rdfs:isDefinedBy rdf:resource="https://w3id.org/italia/onto/PublicContract"/>
        <rdfs:label xml:lang="en">Procurement Project</rdfs:label>
        <rdfs:label xml:lang="it">Progetto di approvigionamento</rdfs:label>
        <owl:versionInfo xml:lang="it">provvisoria</owl:versionInfo>
        <owl:versionInfo xml:lang="en">unstable</owl:versionInfo>
    </owl:Class>
    


    <!-- https://w3id.org/italia/onto/PublicContract/PublicPrivatePartnership -->

    <owl:Class rdf:about="https://w3id.org/italia/onto/PublicContract/PublicPrivatePartnership">
        <rdfs:subClassOf rdf:resource="https://w3id.org/italia/onto/PublicContract/Procedure"/>
        <rdfs:comment xml:lang="it">La classe che rappresenta la modalità di realizzazione di una gara tramite un parternariato pubblico/privato.</rdfs:comment>
        <rdfs:comment xml:lang="en">The class that represents the implementation of a procedure through a public/private partnership.</rdfs:comment>
        <rdfs:isDefinedBy rdf:resource="https://w3id.org/italia/onto/PublicContract"/>
        <rdfs:label xml:lang="it">Parternariato Pubblico/Privato</rdfs:label>
        <rdfs:label xml:lang="en">Public/Private Partnership</rdfs:label>
        <owl:versionInfo xml:lang="it">stabile</owl:versionInfo>
        <owl:versionInfo xml:lang="en">stable</owl:versionInfo>
    </owl:Class>
    


    <!-- https://w3id.org/italia/onto/PublicContract/PublicProcurement -->

    <owl:Class rdf:about="https://w3id.org/italia/onto/PublicContract/PublicProcurement">
        <rdfs:subClassOf rdf:resource="https://w3id.org/italia/onto/PublicContract/Procedure"/>
        <rdfs:comment xml:lang="it">La classe che rappresenta la modalità di realizzazione di una gara tramite un contratto di appalto.</rdfs:comment>
        <rdfs:comment xml:lang="en">The class that represents the implementation of a procedure through a public procurement.</rdfs:comment>
        <rdfs:isDefinedBy rdf:resource="https://w3id.org/italia/onto/PublicContract"/>
        <rdfs:label xml:lang="it">Appalto</rdfs:label>
        <rdfs:label xml:lang="en">Public procurement</rdfs:label>
        <owl:versionInfo xml:lang="it">stabile</owl:versionInfo>
        <owl:versionInfo xml:lang="en">stable</owl:versionInfo>
    </owl:Class>
    


    <!-- https://w3id.org/italia/onto/PublicContract/Publication -->

    <owl:Class rdf:about="https://w3id.org/italia/onto/PublicContract/Publication">
        <rdfs:subClassOf rdf:resource="https://w3id.org/italia/onto/l0/EventOrSituation"/>
        <rdfs:comment xml:lang="it">Le istanze di questa classe rappresentano i dati sulla fase di pubblicazione di una gara</rdfs:comment>
        <rdfs:comment xml:lang="en">The instances of this class represent the data of the publication phase</rdfs:comment>
        <rdfs:isDefinedBy rdf:resource="https://w3id.org/italia/onto/PublicContract"/>
        <rdfs:label xml:lang="it">Pubblicazione</rdfs:label>
        <rdfs:label xml:lang="en">Publication</rdfs:label>
        <owl:versionInfo xml:lang="it">provvisoria</owl:versionInfo>
        <owl:versionInfo xml:lang="en">unstable</owl:versionInfo>
    </owl:Class>
    


    <!-- https://w3id.org/italia/onto/PublicContract/Resolution -->

    <owl:Class rdf:about="https://w3id.org/italia/onto/PublicContract/Resolution">
        <rdfs:subClassOf rdf:resource="https://w3id.org/italia/onto/l0/EventOrSituation"/>
        <rdfs:comment xml:lang="en">An instance of this class represents a resolution of contract.</rdfs:comment>
        <rdfs:comment xml:lang="it">Una istanza di questa classe rappresenta una risoluzione di un contratto.</rdfs:comment>
        <rdfs:isDefinedBy rdf:resource="https://w3id.org/italia/onto/PublicContract"/>
        <rdfs:label xml:lang="en">Resolution</rdfs:label>
        <rdfs:label xml:lang="it">Risoluzione</rdfs:label>
        <owl:versionInfo xml:lang="it">stabile</owl:versionInfo>
        <owl:versionInfo xml:lang="en">stable</owl:versionInfo>
    </owl:Class>
    


    <!-- https://w3id.org/italia/onto/PublicContract/ResolutionDocument -->

    <owl:Class rdf:about="https://w3id.org/italia/onto/PublicContract/ResolutionDocument">
        <rdfs:subClassOf rdf:resource="https://w3id.org/italia/onto/PublicContract/AmendmentDocument"/>
        <rdfs:comment xml:lang="it">La classe che rappresenta il documento che stabilisce la risoluzione di un contratto.</rdfs:comment>
        <rdfs:comment xml:lang="en">The class that represents the document setting the resolution of a contract.</rdfs:comment>
        <rdfs:isDefinedBy rdf:resource="https://w3id.org/italia/onto/PublicContract"/>
        <rdfs:label xml:lang="it">Documento di risoluzione</rdfs:label>
        <rdfs:label xml:lang="en">Resolution document</rdfs:label>
        <owl:versionInfo xml:lang="it">stabile</owl:versionInfo>
        <owl:versionInfo xml:lang="en">stable</owl:versionInfo>
    </owl:Class>
    


    <!-- https://w3id.org/italia/onto/PublicContract/ResolutionReason -->

    <owl:Class rdf:about="https://w3id.org/italia/onto/PublicContract/ResolutionReason">
        <rdfs:subClassOf rdf:resource="https://w3id.org/italia/onto/PublicContract/AmendmentRationale"/>
        <rdfs:comment xml:lang="it">La Classe che rappresenta la motivazione della risoluzione del contratto. Le istanze di questa classe possono essere rappresentate come concetti dello standard skos di un vocabolario controllato.</rdfs:comment>
        <rdfs:comment xml:lang="en">The class that represents the reason of the suspension. The instances of this class can be represented as skos concepts of a controlled vocabulary.</rdfs:comment>
        <rdfs:isDefinedBy rdf:resource="https://w3id.org/italia/onto/PublicContract"/>
        <rdfs:label xml:lang="it">Motivazione Risoluzione</rdfs:label>
        <rdfs:label xml:lang="en">Resolution reason</rdfs:label>
        <owl:versionInfo xml:lang="it">stabile</owl:versionInfo>
        <owl:versionInfo xml:lang="en">stable</owl:versionInfo>
        <prov:wasDerivedFrom rdf:resource="http://www.w3.org/2004/02/skos/core#Concept"/>
    </owl:Class>
    


    <!-- https://w3id.org/italia/onto/PublicContract/ResolutionToContract -->

    <owl:Class rdf:about="https://w3id.org/italia/onto/PublicContract/ResolutionToContract">
        <rdfs:subClassOf rdf:resource="https://w3id.org/italia/onto/PublicContract/Document"/>
        <rdfs:comment xml:lang="it">La classe che comprende gli atti con i quali la stazione appaltante manifesta la propria volontà di stipulare un contratto, individuando gli elementi essenziali del contratto e i criteri di selezione degli operatori economici e delle offerte.</rdfs:comment>
        <rdfs:comment xml:lang="en">The class that includes the documents by means of which the contracting authority expresses that it wants to conclude a contract.</rdfs:comment>
        <rdfs:isDefinedBy rdf:resource="https://w3id.org/italia/onto/PublicContract"/>
        <rdfs:label xml:lang="it">Determina a contrarre</rdfs:label>
        <rdfs:label xml:lang="en">Resolution to contract</rdfs:label>
        <owl:versionInfo xml:lang="it">stabile</owl:versionInfo>
        <owl:versionInfo xml:lang="en">stable</owl:versionInfo>
    </owl:Class>
    


    <!-- https://w3id.org/italia/onto/PublicContract/Suspension -->

    <owl:Class rdf:about="https://w3id.org/italia/onto/PublicContract/Suspension">
        <rdfs:subClassOf rdf:resource="https://w3id.org/italia/onto/PublicContract/ProcedureChangeEvent"/>
        <rdfs:comment xml:lang="en">An instance of this class represents a suspension.</rdfs:comment>
        <rdfs:comment xml:lang="it">Una istanza di questa classe rappresenta una sospensione.</rdfs:comment>
        <rdfs:isDefinedBy rdf:resource="https://w3id.org/italia/onto/PublicContract"/>
        <rdfs:label xml:lang="it">Sospensione</rdfs:label>
        <rdfs:label xml:lang="en">Suspension</rdfs:label>
        <owl:versionInfo xml:lang="it">stabile</owl:versionInfo>
        <owl:versionInfo xml:lang="en">stable</owl:versionInfo>
    </owl:Class>
    


    <!-- https://w3id.org/italia/onto/PublicContract/SuspensionDocument -->

    <owl:Class rdf:about="https://w3id.org/italia/onto/PublicContract/SuspensionDocument">
        <rdfs:subClassOf rdf:resource="https://w3id.org/italia/onto/PublicContract/AmendmentDocument"/>
        <rdfs:comment xml:lang="it">La classe che rappresenta il documento che stabilisce la sospensione di un contratto.</rdfs:comment>
        <rdfs:comment xml:lang="en">The class that represents the document setting the suspension.</rdfs:comment>
        <rdfs:isDefinedBy rdf:resource="https://w3id.org/italia/onto/PublicContract"/>
        <rdfs:label xml:lang="it">Documento di sospensione</rdfs:label>
        <rdfs:label xml:lang="en">Suspension Document</rdfs:label>
        <owl:versionInfo xml:lang="it">stabile</owl:versionInfo>
        <owl:versionInfo xml:lang="en">stable</owl:versionInfo>
    </owl:Class>
    


    <!-- https://w3id.org/italia/onto/PublicContract/SuspensionReason -->

    <owl:Class rdf:about="https://w3id.org/italia/onto/PublicContract/SuspensionReason">
        <rdfs:subClassOf rdf:resource="https://w3id.org/italia/onto/PublicContract/AmendmentRationale"/>
        <rdfs:comment xml:lang="it">La Classe che rappresenta la motivazione della sospensione. Le istanze di questa classe possono essere rappresentate come concetti dello standard skos di un vocabolario controllato</rdfs:comment>
        <rdfs:comment xml:lang="en">The class that represents the reason of the suspension. The instances of this class can be represented as skos concepts of a controlled vocabulary.</rdfs:comment>
        <rdfs:isDefinedBy rdf:resource="https://w3id.org/italia/onto/PublicContract"/>
        <rdfs:label xml:lang="it">Motivazione Sospensione</rdfs:label>
        <rdfs:label xml:lang="en">Suspension reason</rdfs:label>
        <owl:versionInfo xml:lang="it">stabile</owl:versionInfo>
        <owl:versionInfo xml:lang="en">stable</owl:versionInfo>
        <prov:wasDerivedFrom rdf:resource="http://www.w3.org/2004/02/skos/core#Concept"/>
    </owl:Class>
    


    <!-- https://w3id.org/italia/onto/PublicContract/Tender -->

    <owl:Class rdf:about="https://w3id.org/italia/onto/PublicContract/Tender">
        <rdfs:subClassOf rdf:resource="https://w3id.org/italia/onto/l0/Entity"/>
        <rdfs:subClassOf>
            <owl:Restriction>
                <owl:onProperty rdf:resource="https://w3id.org/italia/onto/PublicContract/appliesToLot"/>
                <owl:someValuesFrom rdf:resource="https://w3id.org/italia/onto/PublicContract/Lot"/>
            </owl:Restriction>
        </rdfs:subClassOf>
        <rdfs:subClassOf>
            <owl:Restriction>
                <owl:onProperty rdf:resource="https://w3id.org/italia/onto/PublicContract/attachesTenderDocument"/>
                <owl:someValuesFrom rdf:resource="https://w3id.org/italia/onto/PublicContract/TenderDocument"/>
            </owl:Restriction>
        </rdfs:subClassOf>
        <rdfs:subClassOf>
            <owl:Restriction>
                <owl:onProperty rdf:resource="https://w3id.org/italia/onto/PublicContract/tenderer"/>
                <owl:allValuesFrom rdf:resource="https://w3id.org/italia/onto/l0/Agent"/>
            </owl:Restriction>
        </rdfs:subClassOf>
        <rdfs:subClassOf>
            <owl:Restriction>
                <owl:onProperty rdf:resource="https://w3id.org/italia/onto/PublicContract/submittedDuring"/>
                <owl:qualifiedCardinality rdf:datatype="http://www.w3.org/2001/XMLSchema#nonNegativeInteger">1</owl:qualifiedCardinality>
                <owl:onClass rdf:resource="https://w3id.org/italia/onto/PublicContract/TenderSubmission"/>
            </owl:Restriction>
        </rdfs:subClassOf>
        <rdfs:comment xml:lang="it">Questa classe rappresenta un&apos;entità di offerta che si applica al lotto, a cui è attaccato un documento di offerta e che è presentata da un offerente durante la fase di presentazione delle offerte (rappresenta una relazione n-aria)</rdfs:comment>
        <rdfs:comment xml:lang="en">This class represents and entity related to the offer that applies to the lot, to which is attached a document and that it is presented during the tender submission phase (n-ary relationship)</rdfs:comment>
        <rdfs:isDefinedBy rdf:resource="https://w3id.org/italia/onto/PublicContract"/>
        <rdfs:label xml:lang="it">Offerta</rdfs:label>
        <rdfs:label xml:lang="en">Tender</rdfs:label>
        <owl:versionInfo xml:lang="it">stabile</owl:versionInfo>
        <owl:versionInfo xml:lang="en">stable</owl:versionInfo>
        <prov:wasInfluencedBy rdf:resource="http://w3id.org/ocds/ns#Tender"/>
    </owl:Class>
    


    <!-- https://w3id.org/italia/onto/PublicContract/TenderDocument -->

    <owl:Class rdf:about="https://w3id.org/italia/onto/PublicContract/TenderDocument">
        <rdfs:subClassOf rdf:resource="https://w3id.org/italia/onto/PublicContract/Document"/>
        <rdfs:subClassOf>
            <owl:Restriction>
                <owl:onProperty rdf:resource="https://w3id.org/italia/onto/PublicContract/refersToTender"/>
                <owl:maxQualifiedCardinality rdf:datatype="http://www.w3.org/2001/XMLSchema#nonNegativeInteger">1</owl:maxQualifiedCardinality>
                <owl:onClass rdf:resource="https://w3id.org/italia/onto/PublicContract/Tender"/>
            </owl:Restriction>
        </rdfs:subClassOf>
        <rdfs:comment xml:lang="it">Classe che rappresenta il documento con l&apos;offerta di un offerente in risposta a un bando di gara</rdfs:comment>
        <rdfs:comment xml:lang="en">It represents the document which includes the offer submitted as response to a call for tender</rdfs:comment>
        <rdfs:isDefinedBy rdf:resource="https://w3id.org/italia/onto/PublicContract"/>
        <rdfs:label xml:lang="it">Documento di Offerta</rdfs:label>
        <rdfs:label xml:lang="it">Tender Document</rdfs:label>
        <owl:versionInfo xml:lang="it">stabile</owl:versionInfo>
        <owl:versionInfo xml:lang="en">stable</owl:versionInfo>
        <prov:wasInfluencedBy rdf:resource="http://data.europa.eu/eproc/ontology#Tender"/>
    </owl:Class>
    


    <!-- https://w3id.org/italia/onto/PublicContract/TenderSubmission -->

    <owl:Class rdf:about="https://w3id.org/italia/onto/PublicContract/TenderSubmission">
        <rdfs:subClassOf rdf:resource="https://w3id.org/italia/onto/l0/EventOrSituation"/>
        <rdfs:comment xml:lang="en">An instance of this class rapresents the submission of a tender in a call for tenders or other procedure.</rdfs:comment>
        <rdfs:comment xml:lang="it">Una istanza di questa classe rappresenta una submission della tender relativa a una procedura di realizzazione.</rdfs:comment>
        <rdfs:isDefinedBy rdf:resource="https://w3id.org/italia/onto/PublicContract"/>
        <rdfs:label xml:lang="it">Presentazione Offerta</rdfs:label>
        <rdfs:label xml:lang="en">Tender submission</rdfs:label>
        <owl:versionInfo xml:lang="it">stabile</owl:versionInfo>
        <owl:versionInfo xml:lang="en">stable</owl:versionInfo>
    </owl:Class>
    


    <!-- https://w3id.org/italia/onto/PublicContract/Variant -->

    <owl:Class rdf:about="https://w3id.org/italia/onto/PublicContract/Variant">
        <rdfs:subClassOf rdf:resource="https://w3id.org/italia/onto/PublicContract/ProcedureChangeEvent"/>
        <rdfs:comment xml:lang="en">An instance of this class represents a variant.</rdfs:comment>
        <rdfs:comment xml:lang="it">Una istanza di questa classe rappresenta una variante in corso d&apos;opera.</rdfs:comment>
        <rdfs:isDefinedBy rdf:resource="https://w3id.org/italia/onto/PublicContract"/>
        <rdfs:label xml:lang="en">Variant</rdfs:label>
        <rdfs:label xml:lang="it">Variante</rdfs:label>
        <owl:versionInfo xml:lang="it">stabile</owl:versionInfo>
        <owl:versionInfo xml:lang="en">stable</owl:versionInfo>
    </owl:Class>
    


    <!-- https://w3id.org/italia/onto/PublicContract/VariantDocument -->

    <owl:Class rdf:about="https://w3id.org/italia/onto/PublicContract/VariantDocument">
        <rdfs:subClassOf rdf:resource="https://w3id.org/italia/onto/PublicContract/AmendmentDocument"/>
        <rdfs:comment xml:lang="it">La classe che rappresenta il documento che stabilisce la variante di un contratto.</rdfs:comment>
        <rdfs:comment xml:lang="en">The class that represents the document setting the variant.</rdfs:comment>
        <rdfs:isDefinedBy rdf:resource="https://w3id.org/italia/onto/PublicContract"/>
        <rdfs:label xml:lang="it">Documento di Variante</rdfs:label>
        <rdfs:label xml:lang="en">Variant Document</rdfs:label>
        <owl:versionInfo xml:lang="it">stabile</owl:versionInfo>
        <owl:versionInfo xml:lang="en">stable</owl:versionInfo>
    </owl:Class>
    


    <!-- https://w3id.org/italia/onto/PublicContract/VariantReason -->

    <owl:Class rdf:about="https://w3id.org/italia/onto/PublicContract/VariantReason">
        <rdfs:subClassOf rdf:resource="https://w3id.org/italia/onto/PublicContract/AmendmentRationale"/>
        <rdfs:comment xml:lang="it">La Classe che rappresenta la motivazione della variante in corso d&apos;opera. Le istanze di questa classe possono essere rappresentate come concetti dello standard skos di un vocabolario controllato</rdfs:comment>
        <rdfs:comment xml:lang="en">The class that represents the reason of the variant. The instances of this class can be represented as skos concepts of a controlled vocabulary.</rdfs:comment>
        <rdfs:isDefinedBy rdf:resource="https://w3id.org/italia/onto/PublicContract"/>
        <rdfs:label xml:lang="it">Motivazione Variante</rdfs:label>
        <rdfs:label xml:lang="en">Variant reason</rdfs:label>
        <owl:versionInfo xml:lang="it">stabile</owl:versionInfo>
        <owl:versionInfo xml:lang="en">stable</owl:versionInfo>
        <prov:wasDerivedFrom rdf:resource="http://www.w3.org/2004/02/skos/core#Concept"/>
    </owl:Class>
    


    <!-- https://w3id.org/italia/onto/PublicContract/WorkProgressReport -->

    <owl:Class rdf:about="https://w3id.org/italia/onto/PublicContract/WorkProgressReport">
        <rdfs:subClassOf rdf:resource="https://w3id.org/italia/onto/PublicContract/Document"/>
        <rdfs:comment xml:lang="it">La classe che comprende il documento che attesta lo stato di avanzamento dei lavori.</rdfs:comment>
        <rdfs:comment xml:lang="en">The class that represents the document reporting the progress of work.</rdfs:comment>
        <rdfs:isDefinedBy rdf:resource="https://w3id.org/italia/onto/PublicContract"/>
        <rdfs:label xml:lang="it">Stato avanzamento lavori</rdfs:label>
        <rdfs:label xml:lang="en">Work Progress Report</rdfs:label>
        <owl:versionInfo xml:lang="it">stabile</owl:versionInfo>
        <owl:versionInfo xml:lang="en">stable</owl:versionInfo>
    </owl:Class>
    


    <!-- https://w3id.org/italia/onto/l0/Activity -->

    <owl:Class rdf:about="https://w3id.org/italia/onto/l0/Activity"/>
    


    <!-- 
    ///////////////////////////////////////////////////////////////////////////////////////
    //
    // Individuals
    //
    ///////////////////////////////////////////////////////////////////////////////////////
     -->

    


    <!-- http://spcdata.digitpa.gov.it/Amministrazione/agid -->

    <owl:NamedIndividual rdf:about="http://spcdata.digitpa.gov.it/Amministrazione/agid">
        <rdf:type rdf:resource="http://dati.gov.it/onto/dcatapit#Agent"/>
        <rdf:type rdf:resource="http://xmlns.com/foaf/0.1/Agent"/>
        <dct:identifier>agid</dct:identifier>
        <foaf:name xml:lang="it">Agenzia per l&apos;Italia Digitale</foaf:name>
        <foaf:name xml:lang="en">Italian Digital Agency</foaf:name>
    </owl:NamedIndividual>
    


    <!-- http://spcdata.digitpa.gov.it/Amministrazione/csi_piem -->

    <owl:NamedIndividual rdf:about="http://spcdata.digitpa.gov.it/Amministrazione/csi_piem">
        <rdf:type rdf:resource="http://dati.gov.it/onto/dcatapit#Agent"/>
        <rdf:type rdf:resource="http://xmlns.com/foaf/0.1/Agent"/>
        <dct:identifier>csi_piem</dct:identifier>
        <foaf:name xml:lang="it">Consorzio per il sistema informativo CSI-Piemonte</foaf:name>
    </owl:NamedIndividual>
    


    <!-- http://spcdata.digitpa.gov.it/Amministrazione/cvtiap -->

    <owl:NamedIndividual rdf:about="http://spcdata.digitpa.gov.it/Amministrazione/cvtiap">
        <rdf:type rdf:resource="http://dati.gov.it/onto/dcatapit#Agent"/>
        <rdf:type rdf:resource="http://xmlns.com/foaf/0.1/Agent"/>
        <dct:identifier>cvtiap</dct:identifier>
        <foaf:name xml:lang="it">A.N.AC - Autorità Nazionale Anticorruzione</foaf:name>
    </owl:NamedIndividual>
    


    <!-- https://w3id.org/italia/data/contact-point/onto-agid -->

    <owl:NamedIndividual rdf:about="https://w3id.org/italia/data/contact-point/onto-agid">
        <rdf:type rdf:resource="http://dati.gov.it/onto/dcatapit#Organization"/>
        <rdf:type rdf:resource="http://www.w3.org/2006/vcard/ns#Kind"/>
        <rdf:type rdf:resource="http://www.w3.org/2006/vcard/ns#Organization"/>
        <vcard:fn>banche dati e open data</vcard:fn>
        <vcard:hasEmail rdf:resource="mailto:info@dati.gov.it"/>
    </owl:NamedIndividual>
    


    <!-- https://w3id.org/italia/data/distribution/PCAPIT-JSON-LD -->

    <owl:NamedIndividual rdf:about="https://w3id.org/italia/data/distribution/PCAPIT-JSON-LD">
        <rdf:type rdf:resource="https://w3id.org/italia/onto/ADMS/SemanticAssetDistribution"/>
        <dct:description xml:lang="it">Questa è la distribuzione JSON-LD dell&apos;ontologia dei contratti pubblici</dct:description>
        <dct:description xml:lang="en">This is the distribution in JSON-LD of the Public Contracts ontology</dct:description>
        <dct:format rdf:resource="http://publications.europa.eu/resource/authority/file-type/JSON_LD"/>
        <dct:license rdf:resource="https://w3id.org/italia/controlled-vocabulary/licences/A21_CCBY40"/>
        <dct:title xml:lang="it">Distribuzione JSON-LD ontologia PC-AP_IT</dct:title>
        <dct:title xml:lang="en">JSON-LD distribution of PC-AP_IT Ontology</dct:title>
        <dcat:accessURL rdf:resource="https://raw.githubusercontent.com/italia/daf-ontologie-vocabolari-controllati/master/Ontologie/PublicContract/latest"/>
        <dcat:downloadURL rdf:resource="https://raw.githubusercontent.com/italia/daf-ontologie-vocabolari-controllati/master/Ontologie/PublicContract/PublicContract-AP_IT.jsonld"/>
    </owl:NamedIndividual>
    


    <!-- https://w3id.org/italia/data/distribution/PCAPIT-RDF-TURTLE -->

    <owl:NamedIndividual rdf:about="https://w3id.org/italia/data/distribution/PCAPIT-RDF-TURTLE">
        <rdf:type rdf:resource="https://w3id.org/italia/onto/ADMS/SemanticAssetDistribution"/>
        <dct:description xml:lang="it">Questa è la distribuzione RDF/Turtle dell&apos;ontologia dei contratti pubblici</dct:description>
        <dct:description xml:lang="en">This is the distribution in RDF/turtle of the Public Contracts ontology</dct:description>
        <dct:format rdf:resource="http://publications.europa.eu/resource/authority/file-type/RDF_TURTLE"/>
        <dct:license rdf:resource="https://w3id.org/italia/controlled-vocabulary/licences/A21_CCBY40"/>
        <dct:title xml:lang="it">Distribuzione RDF/Turtle ontologia PC-AP_IT</dct:title>
        <dct:title xml:lang="en">RDF/Turtle distribution of PC-AP_IT Ontology</dct:title>
        <dcat:accessURL rdf:resource="https://raw.githubusercontent.com/italia/daf-ontologie-vocabolari-controllati/master/Ontologie/PublicContract/latest"/>
        <dcat:downloadURL rdf:resource="https://raw.githubusercontent.com/italia/daf-ontologie-vocabolari-controllati/master/Ontologie/PublicContract/latest/PubliContract-AP_IT.ttl"/>
    </owl:NamedIndividual>
    


    <!-- https://w3id.org/italia/data/distribution/PCAPIT-RDF-XML -->

    <owl:NamedIndividual rdf:about="https://w3id.org/italia/data/distribution/PCAPIT-RDF-XML">
        <rdf:type rdf:resource="https://w3id.org/italia/onto/ADMS/SemanticAssetDistribution"/>
        <dct:description xml:lang="it">Questa è la distribuzione RDF/XML dell&apos;ontologia dei contratti pubblici</dct:description>
        <dct:description xml:lang="en">This is the distribution in RDF/XML of the Public Contracts ontology</dct:description>
        <dct:format rdf:resource="http://publications.europa.eu/resource/authority/file-type/RDF_XML"/>
        <dct:license rdf:resource="https://w3id.org/italia/controlled-vocabulary/licences/A21_CCBY40"/>
        <dct:title xml:lang="it">Distribuzione RDF/XML ontologia PC-AP_IT</dct:title>
        <dct:title xml:lang="en">RDF/XML distribution of PC-AP_IT Ontology</dct:title>
        <dcat:accessURL rdf:resource="https://raw.githubusercontent.com/italia/daf-ontologie-vocabolari-controllati/master/Ontologie/PublicContract/latest"/>
        <dcat:downloadURL rdf:resource="https://raw.githubusercontent.com/italia/daf-ontologie-vocabolari-controllati/master/Ontologie/PublicContract/latest/PublicContract-AP_IT.rdf"/>
    </owl:NamedIndividual>
    


    <!-- https://w3id.org/italia/data/organization/private-organization/IT11491360019 -->

    <owl:NamedIndividual rdf:about="https://w3id.org/italia/data/organization/private-organization/IT11491360019">
        <rdf:type rdf:resource="http://dati.gov.it/onto/dcatapit#Agent"/>
        <rdf:type rdf:resource="http://xmlns.com/foaf/0.1/Agent"/>
        <dct:identifier>IT11491360019</dct:identifier>
        <foaf:name xml:lang="it">Synapta Srl</foaf:name>
    </owl:NamedIndividual>
    


    <!-- https://w3id.org/italia/data/organization/public-organization/td -->

    <owl:NamedIndividual rdf:about="https://w3id.org/italia/data/organization/public-organization/td">
        <rdf:type rdf:resource="http://dati.gov.it/onto/dcatapit#Agent"/>
        <rdf:type rdf:resource="http://xmlns.com/foaf/0.1/Agent"/>
        <dct:identifier>TD</dct:identifier>
        <foaf:name xml:lang="en">Digital Transformation Team</foaf:name>
        <foaf:name xml:lang="it">Team per la Trasformazione Digitale</foaf:name>
    </owl:NamedIndividual>
    


    <!-- https://w3id.org/italia/data/organization/support-unit/cnr-Z6HZEH/stlab -->

    <owl:NamedIndividual rdf:about="https://w3id.org/italia/data/organization/support-unit/cnr-Z6HZEH/stlab">
        <rdf:type rdf:resource="https://w3id.org/italia/onto/l0/Agent"/>
        <l0:name xml:lang="en">Institute of Cognitive Sciences and Technologies of the Italian Research Council (CNR) - Semantic Technology Laboratory (STLab)</l0:name>
        <l0:name xml:lang="it">Istituto di Scienze e Tecnologie della Cognizione del CNR - Semantic Technology Lab (STLab)</l0:name>
        <dct:identifier>cnr - Z6HZEH - STLab</dct:identifier>
    </owl:NamedIndividual>
    


    <!-- https://w3id.org/italia/data/project/DAF -->

    <owl:NamedIndividual rdf:about="https://w3id.org/italia/data/project/DAF">
        <rdf:type rdf:resource="https://w3id.org/italia/onto/ADMS/Project"/>
        <l0:name xml:lang="it">Data &amp; Analytics Framework</l0:name>
    </owl:NamedIndividual>
    


    <!-- https://w3id.org/italia/data/project/OntoPiA -->

    <owl:NamedIndividual rdf:about="https://w3id.org/italia/data/project/OntoPiA">
        <rdf:type rdf:resource="https://w3id.org/italia/onto/ADMS/Project"/>
        <l0:name xml:lang="it">OntoPiA - la rete di ontologie della pubblica amministrazione italiana</l0:name>
    </owl:NamedIndividual>
    


    <!-- https://w3id.org/italia/onto/PublicContract -->

    <owl:NamedIndividual rdf:about="https://w3id.org/italia/onto/PublicContract">
        <rdf:type rdf:resource="https://w3id.org/italia/onto/ADMS/SemanticAsset"/>
    </owl:NamedIndividual>
    


    <!-- https://w3id.org/italia/onto/PublicContract/LowestPrice -->

    <owl:NamedIndividual rdf:about="https://w3id.org/italia/onto/PublicContract/LowestPrice">
        <rdf:type rdf:resource="https://w3id.org/italia/onto/PublicContract/AwardCriterion"/>
        <rdfs:isDefinedBy rdf:resource="https://w3id.org/italia/onto/PublicContract"/>
        <rdfs:label xml:lang="en">Lowest Price</rdfs:label>
        <rdfs:label xml:lang="it">Prezzo più basso</rdfs:label>
        <owl:versionInfo xml:lang="it">stabile</owl:versionInfo>
        <owl:versionInfo xml:lang="en">stable</owl:versionInfo>
    </owl:NamedIndividual>
    


    <!-- https://w3id.org/italia/onto/PublicContract/MostEconomicallyAdvantageousTender -->

    <owl:NamedIndividual rdf:about="https://w3id.org/italia/onto/PublicContract/MostEconomicallyAdvantageousTender">
        <rdf:type rdf:resource="https://w3id.org/italia/onto/PublicContract/AwardCriterion"/>
        <rdfs:isDefinedBy rdf:resource="https://w3id.org/italia/onto/PublicContract"/>
        <rdfs:label xml:lang="en">Most economically advantageous offer</rdfs:label>
        <rdfs:label xml:lang="it">Offerta economicamente più vantaggiosa</rdfs:label>
        <owl:versionInfo xml:lang="it">stabile</owl:versionInfo>
        <owl:versionInfo xml:lang="en">stable</owl:versionInfo>
    </owl:NamedIndividual>
    


    <!-- 
    ///////////////////////////////////////////////////////////////////////////////////////
    //
    // Annotations
    //
    ///////////////////////////////////////////////////////////////////////////////////////
     -->

    <rdf:Description rdf:about="https://w3id.org/italia/onto/PublicContract/Good">
        <owl:versionInfo xml:lang="it">stabile</owl:versionInfo>
        <rdfs:comment xml:lang="it">Fornitura di prodotti</rdfs:comment>
        <owl:versionInfo xml:lang="en">stable</owl:versionInfo>
        <rdfs:label xml:lang="it">Fornitura di Prodotto</rdfs:label>
        <rdfs:isDefinedBy rdf:resource="https://w3id.org/italia/onto/PublicContract"/>
        <rdfs:comment xml:lang="en">The class that includes those interventions concerning the purchase of goods.</rdfs:comment>
        <rdfs:label xml:lang="it">Fornitura di Bene</rdfs:label>
        <rdfs:label xml:lang="en">Good supply</rdfs:label>
        <rdfs:comment xml:lang="it">La classe che comprende gli interventi che consistono nell&apos;acquisto di beni.</rdfs:comment>
    </rdf:Description>
    <rdf:Description rdf:about="https://w3id.org/italia/onto/PublicContract/ServiceIntervention">
        <rdfs:label xml:lang="en">Service Intervention</rdfs:label>
        <rdfs:isDefinedBy rdf:resource="https://w3id.org/italia/onto/PublicContract"/>
        <rdfs:label xml:lang="it">Fornitura di Servizio</rdfs:label>
        <rdfs:label xml:lang="en">Service supply</rdfs:label>
        <rdfs:comment xml:lang="it">La classe che comprende gli interventi che consistono nell&apos;acquisizione di servizi.</rdfs:comment>
        <owl:versionInfo xml:lang="it">stabile</owl:versionInfo>
        <rdfs:comment xml:lang="en">The class that includes those interventions concerning the acquisition of services.</rdfs:comment>
        <owl:versionInfo xml:lang="en">stable</owl:versionInfo>
    </rdf:Description>
    <rdf:Description rdf:about="https://w3id.org/italia/onto/PublicContract/Work">
        <owl:versionInfo xml:lang="it">stabile</owl:versionInfo>
        <rdfs:comment xml:lang="en">The class that includes those interventions concerning the actualization of public works.</rdfs:comment>
        <rdfs:comment xml:lang="it">La classe che comprende gli interventi che consistono nella realizzazione di lavori pubblici.</rdfs:comment>
        <rdfs:isDefinedBy rdf:resource="https://w3id.org/italia/onto/PublicContract"/>
        <owl:versionInfo xml:lang="en">stable</owl:versionInfo>
        <rdfs:label xml:lang="en">Work supply</rdfs:label>
        <rdfs:label xml:lang="it">Fornitura di lavori</rdfs:label>
    </rdf:Description>
</rdf:RDF>



<!-- Generated by the OWL API (version 4.5.9.2019-02-01T07:24:44Z) https://github.com/owlcs/owlapi -->

