<?xml version="1.0" encoding="UTF-8"?>
<rdf:RDF
   xmlns:ns1="https://w3id.org/italia/onto/ADMS/"
   xmlns:ns2="http://purl.org/dc/terms/"
   xmlns:ns3="http://www.w3.org/ns/dcat#"
   xmlns:ns4="https://w3id.org/italia/onto/l0/"
   xmlns:ns5="http://xmlns.com/foaf/0.1/"
   xmlns:ns6="http://www.w3.org/ns/prov#"
   xmlns:ns7="http://www.w3.org/2006/vcard/ns#"
   xmlns:owl="http://www.w3.org/2002/07/owl#"
   xmlns:rdf="http://www.w3.org/1999/02/22-rdf-syntax-ns#"
   xmlns:rdfs="http://www.w3.org/2000/01/rdf-schema#"
>
  <rdf:Description rdf:about="https://w3id.org/italia/onto/HER/pubmedId">
    <rdf:type rdf:resource="http://www.w3.org/2002/07/owl#DatatypeProperty"/>
    <rdfs:subPropertyOf rdf:resource="https://w3id.org/italia/onto/l0/identifier"/>
    <rdfs:domain rdf:resource="https://w3id.org/italia/onto/HER/Result"/>
    <rdfs:range rdf:resource="http://www.w3.org/2000/01/rdf-schema#Literal"/>
    <rdfs:comment xml:lang="it">Identificatore di una pubblicazione nel repository PubMed (https://pubmed.ncbi.nlm.nih.gov/)</rdfs:comment>
    <rdfs:comment xml:lang="en">Identifier of a publication in the PubMed repository (https://pubmed.ncbi.nlm.nih.gov/)</rdfs:comment>
    <rdfs:isDefinedBy rdf:resource="https://w3id.org/italia/onto/HER"/>
    <rdfs:label xml:lang="en">PubMed ID</rdfs:label>
    <rdfs:label xml:lang="it">identificatore PubMed</rdfs:label>
    <owl:versionInfo xml:lang="it">provvisoria</owl:versionInfo>
    <owl:versionInfo xml:lang="en">unstable</owl:versionInfo>
  </rdf:Description>
  <rdf:Description rdf:about="https://w3id.org/italia/onto/HER/AACTEligibility">
    <rdf:type rdf:resource="http://www.w3.org/2002/07/owl#Class"/>
    <rdfs:subClassOf rdf:resource="https://w3id.org/italia/onto/l0/Characteristic"/>
    <rdfs:subClassOf rdf:nodeID="n5bb3bff42afb4ca286d2c3fead9507ddb372"/>
    <rdfs:subClassOf rdf:nodeID="n5bb3bff42afb4ca286d2c3fead9507ddb373"/>
    <rdfs:subClassOf rdf:nodeID="n5bb3bff42afb4ca286d2c3fead9507ddb374"/>
    <rdfs:subClassOf rdf:nodeID="n5bb3bff42afb4ca286d2c3fead9507ddb375"/>
    <rdfs:comment xml:lang="it">I requisiti chiave che le persone che vogliono partecipare a uno studio clinico devono soddisfare o le caratteristiche che devono avere.</rdfs:comment>
    <rdfs:comment xml:lang="en">The key requirements that people who want to participate in a clinical study must meet or the characteristics they must have.</rdfs:comment>
    <rdfs:isDefinedBy rdf:resource="https://w3id.org/italia/onto/HER"/>
    <rdfs:label xml:lang="en">Eligibility</rdfs:label>
    <rdfs:label xml:lang="it">Idoneitá</rdfs:label>
    <owl:versionInfo xml:lang="it">stabile</owl:versionInfo>
    <owl:versionInfo xml:lang="en">stable</owl:versionInfo>
  </rdf:Description>
  <rdf:Description rdf:about="https://w3id.org/italia/onto/HER/AcademicDiscipline">
    <rdf:type rdf:resource="http://www.w3.org/2002/07/owl#Class"/>
    <rdfs:subClassOf rdf:resource="https://w3id.org/italia/onto/HER/HERClassification"/>
    <rdfs:subClassOf rdf:nodeID="n5bb3bff42afb4ca286d2c3fead9507ddb398"/>
    <rdfs:isDefinedBy rdf:resource="https://w3id.org/italia/onto/HER"/>
    <rdfs:label xml:lang="en">Classification of Academic Disciplines</rdfs:label>
    <rdfs:label xml:lang="it">Classificazione Settori Sicentifico Disciplinari</rdfs:label>
    <owl:versionInfo xml:lang="it">stabile</owl:versionInfo>
    <owl:versionInfo xml:lang="en">stable</owl:versionInfo>
    <ns6:wasDerivedFrom rdf:resource="http://www.w3.org/2004/02/skos/core#ConceptScheme"/>
    <ns4:controlledVocabulary rdf:resource="https://w3id.org/italia/controlled-vocabulary/classifications-for-universities/academic-disciplines"/>
  </rdf:Description>
  <rdf:Description rdf:about="https://w3id.org/italia/onto/HER/patentFamilyCode">
    <rdf:type rdf:resource="http://www.w3.org/2002/07/owl#DatatypeProperty"/>
    <rdfs:subPropertyOf rdf:resource="https://w3id.org/italia/onto/l0/identifier"/>
    <rdfs:domain rdf:resource="https://w3id.org/italia/onto/HER/Patent"/>
    <rdfs:range rdf:resource="http://www.w3.org/2000/01/rdf-schema#Literal"/>
    <rdfs:comment xml:lang="it">Il codice identificativo di una famiglia di brevetti.</rdfs:comment>
    <rdfs:comment xml:lang="en">The identification code of a patent family.</rdfs:comment>
    <rdfs:isDefinedBy rdf:resource="https://w3id.org/italia/onto/HER"/>
    <rdfs:label xml:lang="it">codice della famiglia di brevetti</rdfs:label>
    <rdfs:label xml:lang="en">patent family code</rdfs:label>
    <owl:versionInfo xml:lang="it">stabile</owl:versionInfo>
    <owl:versionInfo xml:lang="en">stable</owl:versionInfo>
  </rdf:Description>
  <rdf:Description rdf:about="https://w3id.org/italia/onto/HER/WIPOIPCSection">
    <rdf:type rdf:resource="http://www.w3.org/2002/07/owl#Class"/>
    <rdfs:subClassOf rdf:resource="https://w3id.org/italia/onto/HER/InternationalPatentClassification"/>
    <rdfs:comment xml:lang="it">La prima lettera di ogni simbolo di classificazione rappresenta la "sezione" costituita da una lettera da A ("Necessità umane") a H ("Elettricità").</rdfs:comment>
    <rdfs:comment xml:lang="en">The first letter of each classification symbol represents the "section" consisting of a letter from A ("Human Necessities") to H ("Electricity").</rdfs:comment>
    <rdfs:isDefinedBy rdf:resource="https://w3id.org/italia/onto/HER"/>
    <rdfs:label xml:lang="it">Sezione IPC WIPO</rdfs:label>
    <rdfs:label xml:lang="en">WIPO IPC Section</rdfs:label>
    <owl:versionInfo xml:lang="it">stabile</owl:versionInfo>
    <owl:versionInfo xml:lang="en">stable</owl:versionInfo>
    <ns6:wasDerivedFrom rdf:resource="http://www.w3.org/2004/02/skos/core#Concept"/>
  </rdf:Description>
  <rdf:Description rdf:about="https://w3id.org/italia/onto/HER/hasFundingScheme">
    <rdf:type rdf:resource="http://www.w3.org/2002/07/owl#ObjectProperty"/>
    <rdfs:domain rdf:nodeID="n5bb3bff42afb4ca286d2c3fead9507ddb64"/>
    <rdfs:range rdf:resource="https://w3id.org/italia/onto/HER/ECFundingScheme"/>
    <rdfs:comment xml:lang="it">Questa proprietà collega un progetto CE con il corrispondente schema di finanziamento</rdfs:comment>
    <rdfs:comment xml:lang="en">This property links an EC project with the corresponding funding scheme.</rdfs:comment>
    <rdfs:isDefinedBy rdf:resource="https://w3id.org/italia/onto/HER"/>
    <rdfs:label xml:lang="it">ha piano di finanziamento CE</rdfs:label>
    <rdfs:label xml:lang="en">has EC funding scheme</rdfs:label>
    <owl:versionInfo xml:lang="it">stabile</owl:versionInfo>
    <owl:versionInfo xml:lang="en">stable</owl:versionInfo>
  </rdf:Description>
  <rdf:Description rdf:nodeID="n5bb3bff42afb4ca286d2c3fead9507ddb46">
    <rdf:first rdf:resource="https://w3id.org/italia/onto/HER/ERCProject"/>
    <rdf:rest rdf:resource="http://www.w3.org/1999/02/22-rdf-syntax-ns#nil"/>
  </rdf:Description>
  <rdf:Description rdf:nodeID="n5bb3bff42afb4ca286d2c3fead9507ddb391">
    <rdf:type rdf:resource="http://www.w3.org/2002/07/owl#Restriction"/>
    <owl:onProperty rdf:resource="https://w3id.org/italia/onto/HER/resultsFirstSubmittedDate"/>
    <owl:maxQualifiedCardinality rdf:datatype="http://www.w3.org/2001/XMLSchema#nonNegativeInteger">1</owl:maxQualifiedCardinality>
    <owl:onDataRange rdf:resource="http://www.w3.org/2001/XMLSchema#date"/>
  </rdf:Description>
  <rdf:Description rdf:about="https://w3id.org/italia/onto/HER/ctnprinInitiativeCommittedCredit">
    <rdf:type rdf:resource="http://www.w3.org/2002/07/owl#DatatypeProperty"/>
    <rdfs:subPropertyOf rdf:resource="https://w3id.org/italia/onto/MU/value"/>
    <rdfs:domain rdf:resource="https://w3id.org/italia/onto/HER/CTNPRINInitiative"/>
    <rdfs:range rdf:resource="http://www.w3.org/2001/XMLSchema#decimal"/>
    <rdfs:comment xml:lang="en">Total credits committed by the Ministry on eligible costs following ex-ante evaluation (only for companies). Calculated as the sum of the homologous variable 'committedCredit' present at the lower aggregation level (committedCredit_operations).</rdfs:comment>
    <rdfs:comment xml:lang="it">Totale dei crediti impegnati dal Ministero sui costi ammessi a seguito di valutazione ex-ante (solo per imprese). Calcolati come somma dell'omologa variabile "committedCredit" presente a livello di aggregazione inferiore (committedCredit_operations).</rdfs:comment>
    <rdfs:isDefinedBy rdf:resource="https://w3id.org/italia/onto/HER"/>
    <rdfs:label xml:lang="en">committed credit of CTN/PRIN initiative</rdfs:label>
    <rdfs:label xml:lang="it">credito impegnato per iniziative CTN/PRIN</rdfs:label>
    <owl:versionInfo xml:lang="it">stabile</owl:versionInfo>
    <owl:versionInfo xml:lang="en">stable</owl:versionInfo>
  </rdf:Description>
  <rdf:Description rdf:about="https://w3id.org/italia/onto/HER/samplingMethod">
    <rdf:type rdf:resource="http://www.w3.org/2002/07/owl#DatatypeProperty"/>
    <rdfs:domain rdf:resource="https://w3id.org/italia/onto/HER/AACTEligibility"/>
    <rdfs:range rdf:nodeID="n5bb3bff42afb4ca286d2c3fead9507ddb271"/>
    <rdfs:comment xml:lang="en">Indicate the method used for the sampling approach and explain in the Detailed Description. Types are:
Probability Sample: Exclusively random process to guarantee that each participant or population has specified chance of selection, such as simple random sampling, systematic sampling, stratified random sampling, cluster sampling, and consecutive participant sampling
Non-Probability Sample: Any of a variety of other sampling processes, such as convenience sampling or invitation to volunteer
</rdfs:comment>
    <rdfs:comment xml:lang="it">Indicazioni e spiegazioni riguardo il metodo utilizzato per l'approccio di campionamento I tipi sono:
Campione di probabilità: Processo esclusivamente casuale per garantire che ogni partecipante o popolazione abbia specificato la possibilità di selezione, come il campionamento casuale semplice, il campionamento sistematico, il campionamento casuale stratificato, il campionamento a grappolo e il campionamento consecutivo dei partecipanti.
Campione di nonrobabilità: Qualsiasi di una varietà di altri processi di campionamento, come il campionamento di convenienza o l'invito al volontariato</rdfs:comment>
    <rdfs:isDefinedBy rdf:resource="https://w3id.org/italia/onto/HER"/>
    <rdfs:label xml:lang="it">Metodo di campionamento</rdfs:label>
    <rdfs:label xml:lang="en">sampling method</rdfs:label>
    <owl:versionInfo xml:lang="it">provvisoria - valutare l'uso di una classe per rappresentare un metodo</owl:versionInfo>
    <owl:versionInfo xml:lang="en">unstable - check the use of a class to represent a method</owl:versionInfo>
  </rdf:Description>
  <rdf:Description rdf:about="https://w3id.org/italia/onto/HER/lastUpdateSubmittedDate">
    <rdf:type rdf:resource="http://www.w3.org/2002/07/owl#DatatypeProperty"/>
    <rdfs:subPropertyOf rdf:resource="https://w3id.org/italia/onto/TI/modified"/>
    <rdfs:domain rdf:resource="https://w3id.org/italia/onto/HER/AACTStudy"/>
    <rdfs:range rdf:resource="http://www.w3.org/2001/XMLSchema#date"/>
    <rdfs:comment xml:lang="it">La data più recente in cui lo sponsor dello studio o lo sperimentatore ha presentato a ClinicalTrials.gov le modifiche al dossier dello studio. In genere c'è un ritardo di alcuni giorni tra la data dell'ultimo aggiornamento presentato e la data in cui le modifiche vengono pubblicate su ClinicalTrials.gov (la data dell'ultimo aggiornamento pubblicato).</rdfs:comment>
    <rdfs:comment xml:lang="en">The most recent date on which the study sponsor or investigator submitted changes to a study record to ClinicalTrials.gov. There is typically a delay of a few days between the last update submitted date and when the date changes are posted on ClinicalTrials.gov (the last update posted date).</rdfs:comment>
    <rdfs:isDefinedBy rdf:resource="https://w3id.org/italia/onto/HER"/>
    <rdfs:label xml:lang="it">data dell'ultimo aggiornamento presentato</rdfs:label>
    <rdfs:label xml:lang="en">last update submitted date</rdfs:label>
    <owl:versionInfo xml:lang="it">stabile</owl:versionInfo>
    <owl:versionInfo xml:lang="en">stable</owl:versionInfo>
  </rdf:Description>
  <rdf:Description rdf:about="https://w3id.org/italia/onto/HER/ctnprinAmountApprovedCost">
    <rdf:type rdf:resource="http://www.w3.org/2002/07/owl#DatatypeProperty"/>
    <rdfs:subPropertyOf rdf:resource="https://w3id.org/italia/onto/MU/value"/>
    <rdfs:domain rdf:resource="https://w3id.org/italia/onto/HER/CTNPRINAmount"/>
    <rdfs:range rdf:resource="http://www.w3.org/2001/XMLSchema#decimal"/>
    <rdfs:comment xml:lang="en">Approved cost per individual expense item after valuation in itinere compared to the cost reported by the beneficiary to which the operation relates.</rdfs:comment>
    <rdfs:comment xml:lang="it">Costo approvato per singola voce di spesa dopo valutazione in itinere rispetto al costo rendicontato dal beneficiario a cui fa capo l'operazione.</rdfs:comment>
    <rdfs:isDefinedBy rdf:resource="https://w3id.org/italia/onto/HER"/>
    <rdfs:label xml:lang="en">approved cost of CTN/PRIN amount</rdfs:label>
    <rdfs:label xml:lang="it">costo approvato dell'importo CTN/PRIN</rdfs:label>
    <owl:versionInfo xml:lang="it">stabile</owl:versionInfo>
    <owl:versionInfo xml:lang="en">stable</owl:versionInfo>
  </rdf:Description>
  <rdf:Description rdf:about="https://w3id.org/italia/onto/HER/USTATUniversityExpenseClass">
    <rdf:type rdf:resource="http://www.w3.org/2002/07/owl#Class"/>
    <rdfs:subClassOf rdf:resource="https://w3id.org/italia/onto/l0/Characteristic"/>
    <rdfs:comment xml:lang="en">Information on the expenditure for interventions in favor of students (student loans only) of the universities by type. Data are related to the financial year (T-1). The types of intervention are classified according to the following code/descriptions:
51 : SECTION 3 - LOANS PROVIDED BY CONVENTIONED CREDIT INSTITUTIONS - Amount of loans
52 : SECTION 3 - LOANS PROVIDED BY CONVENTIONED CREDIT INSTITUTIONS - Guarantee Fund
53 : section 3 - loans provided by conventioned credit institutions - amount of interest and/or capital contributions to be paid by the University</rdfs:comment>
    <rdfs:comment xml:lang="it">Informazioni sulla spesa per interventi a favore degli studenti (solo prestiti a studenti) degli atenei per tipologia. I dati sono relativi all'esercizio finanziario all'anno (T-1). Le tipologie di intervento sono classificate secondo i codici/descrizioni seguenti:
51    : SEZIONE 3 - PRESTITI EROGATI DA ISTITUTI DI CREDITO CONVENZIONATI - Ammontare dei prestiti
52    : SEZIONE 3 - PRESTITI EROGATI DA ISTITUTI DI CREDITO CONVENZIONATI - Fondo di garanzia
53    : SEZIONE 3 - PRESTITI EROGATI DA ISTITUTI DI CREDITO CONVENZIONATI - Ammontare contributi in conto interesse e/o conto capitale a carico dell'Ateneo</rdfs:comment>
    <rdfs:isDefinedBy rdf:resource="https://w3id.org/italia/onto/HER"/>
    <rdfs:label xml:lang="it">Classe di spese universitarie riportate da USTAT</rdfs:label>
    <rdfs:label xml:lang="en">USTAT Reported University Expense Class</rdfs:label>
    <owl:versionInfo xml:lang="it">stabile</owl:versionInfo>
    <owl:versionInfo xml:lang="en">stable</owl:versionInfo>
  </rdf:Description>
  <rdf:Description rdf:about="https://w3id.org/italia/onto/HER/hasUSTATUniversityInterventionType">
    <rdf:type rdf:resource="http://www.w3.org/2002/07/owl#ObjectProperty"/>
    <rdfs:domain rdf:resource="https://w3id.org/italia/onto/HER/USTATInterventionsForStudentsByUniversitiesAggregate"/>
    <rdfs:range rdf:resource="https://w3id.org/italia/onto/HER/USTATUniversityInterventionType"/>
    <rdfs:comment xml:lang="en">Property that links the aggregated data on the university intervention as defined by USTAT to the type of university intervention as defined by USTAT</rdfs:comment>
    <rdfs:comment xml:lang="it">Proprietà che collega i dati aggregati sui sugli interventi universitari come riportati da USTAT ai tipi di intervento universitari definiti nel contesto USTAT</rdfs:comment>
    <rdfs:isDefinedBy rdf:resource="https://w3id.org/italia/onto/HER"/>
    <rdfs:label xml:lang="en">has USTAT university intervention type</rdfs:label>
    <rdfs:label xml:lang="it">has tipo intervento universitario di USTAT</rdfs:label>
    <owl:versionInfo xml:lang="it">stabile</owl:versionInfo>
    <owl:versionInfo xml:lang="en">stable</owl:versionInfo>
  </rdf:Description>
  <rdf:Description rdf:about="https://w3id.org/italia/onto/HER/AACTResponsibleParty">
    <rdf:type rdf:resource="http://www.w3.org/2002/07/owl#Class"/>
    <rdfs:subClassOf rdf:resource="https://w3id.org/italia/onto/CPV/Person"/>
    <rdfs:comment xml:lang="it">La persona responsabile dell'invio di informazioni su uno studio clinico a ClinicalTrials.gov e dell'aggiornamento di tali informazioni. Di solito lo sponsor dello studio o lo sperimentatore.</rdfs:comment>
    <rdfs:comment xml:lang="en">The person responsible for submitting information about a clinical study to ClinicalTrials.gov and updating that information. Usually the study sponsor or investigator.</rdfs:comment>
    <rdfs:isDefinedBy rdf:resource="https://w3id.org/italia/onto/HER"/>
    <rdfs:label xml:lang="en">Responsible Party</rdfs:label>
    <rdfs:label xml:lang="it">parte responsabile</rdfs:label>
    <owl:versionInfo xml:lang="it">stabile</owl:versionInfo>
    <owl:versionInfo xml:lang="en">stable</owl:versionInfo>
  </rdf:Description>
  <rdf:Description rdf:about="https://w3id.org/italia/onto/HER/hasUSTATExonerationClass">
    <rdf:type rdf:resource="http://www.w3.org/2002/07/owl#ObjectProperty"/>
    <rdfs:domain rdf:nodeID="n5bb3bff42afb4ca286d2c3fead9507ddb93"/>
    <rdfs:range rdf:resource="https://w3id.org/italia/onto/HER/USTATExonerationType"/>
    <rdfs:comment xml:lang="it">Questa proprietà collega l'informazione sugli studenti esonerati (parzialmente o totalmente) alla classe di esonero corrispondente.</rdfs:comment>
    <rdfs:comment xml:lang="en">This property links information about exonerated students (partially or totally) to the corresponding exoneration class.</rdfs:comment>
    <rdfs:isDefinedBy rdf:resource="https://w3id.org/italia/onto/HER"/>
    <rdfs:label xml:lang="it">ha una classe di esonero</rdfs:label>
    <rdfs:label xml:lang="en">has exoneration class</rdfs:label>
    <owl:versionInfo xml:lang="it">stabile</owl:versionInfo>
    <owl:versionInfo xml:lang="en">stable</owl:versionInfo>
  </rdf:Description>
  <rdf:Description rdf:about="https://w3id.org/italia/onto/HER/numberOfRegisteredStudents">
    <rdf:type rdf:resource="http://www.w3.org/2002/07/owl#DatatypeProperty"/>
    <rdfs:domain rdf:nodeID="n5bb3bff42afb4ca286d2c3fead9507ddb218"/>
    <rdfs:range rdf:resource="http://www.w3.org/2001/XMLSchema#int"/>
    <rdfs:comment xml:lang="en">Number of students registered in the Italian education system.</rdfs:comment>
    <rdfs:comment xml:lang="it">Numero di studenti immatricolati al sistema educativo italiano.</rdfs:comment>
    <rdfs:isDefinedBy rdf:resource="https://w3id.org/italia/onto/HER"/>
    <rdfs:label xml:lang="en">number of registered students</rdfs:label>
    <rdfs:label xml:lang="it">numero di studenti immatricolati</rdfs:label>
    <owl:versionInfo xml:lang="it">stabile</owl:versionInfo>
    <owl:versionInfo xml:lang="en">stable</owl:versionInfo>
  </rdf:Description>
  <rdf:Description rdf:nodeID="n5bb3bff42afb4ca286d2c3fead9507ddb437">
    <rdf:type rdf:resource="http://www.w3.org/2002/07/owl#Restriction"/>
    <owl:onProperty rdf:resource="https://w3id.org/italia/onto/l0/identifier"/>
    <owl:cardinality rdf:datatype="http://www.w3.org/2001/XMLSchema#nonNegativeInteger">1</owl:cardinality>
  </rdf:Description>
  <rdf:Description rdf:about="https://w3id.org/italia/onto/HER/hasECActivityType">
    <rdf:type rdf:resource="http://www.w3.org/2002/07/owl#ObjectProperty"/>
    <rdfs:domain rdf:resource="https://w3id.org/italia/onto/HER/ECParticipant"/>
    <rdfs:range rdf:resource="https://w3id.org/italia/onto/HER/ECActivityType"/>
    <rdfs:comment xml:lang="it">Tipologia di organizzazione che partecipa ad un progetto CE. Le seguenti descrizioni e codici di convenzione sono utilizzati per distinguere tra i diversi tipi di organizzazioni: società private a scopo di lucro (PRC), enti pubblici (esclusi ricerca e istruzione) (PUB), organizzazioni di ricerca (esclusa l'istruzione) (REC), istituti di istruzione secondaria e superiore (HES) e altri enti (OTH).</rdfs:comment>
    <rdfs:comment xml:lang="en">Type of organisation participating in a EC project. The following descriptions and convention codes are used for distinguishing between different types of organisations: private for profit companies (PRC), public bodies (excluding research and education) (PUB), research organisations (excluding education) (REC), secondary and higher education establishments (HES), and other entities (OTH).</rdfs:comment>
    <rdfs:isDefinedBy rdf:resource="https://w3id.org/italia/onto/HER"/>
    <rdfs:label xml:lang="it">ha tipo di attivitá CE</rdfs:label>
    <rdfs:label xml:lang="en">has EC activity type</rdfs:label>
    <owl:versionInfo xml:lang="it">provvisoria</owl:versionInfo>
    <owl:versionInfo xml:lang="en">unstable</owl:versionInfo>
  </rdf:Description>
  <rdf:Description rdf:nodeID="n5bb3bff42afb4ca286d2c3fead9507ddb325">
    <rdf:first rdf:resource="https://w3id.org/italia/onto/HER/USTATPostgraduateAggregateOfRegistered"/>
    <rdf:rest rdf:nodeID="n5bb3bff42afb4ca286d2c3fead9507ddb326"/>
  </rdf:Description>
  <rdf:Description rdf:nodeID="n5bb3bff42afb4ca286d2c3fead9507ddb187">
    <rdf:type rdf:resource="http://www.w3.org/1999/02/22-rdf-syntax-ns#List"/>
    <rdf:first>Double</rdf:first>
    <rdf:rest rdf:nodeID="n5bb3bff42afb4ca286d2c3fead9507ddb188"/>
  </rdf:Description>
  <rdf:Description rdf:about="https://w3id.org/italia/onto/HER/totalInvestment">
    <rdf:type rdf:resource="http://www.w3.org/2002/07/owl#DatatypeProperty"/>
    <rdfs:subPropertyOf rdf:resource="https://w3id.org/italia/onto/MU/value"/>
    <rdfs:domain rdf:resource="https://w3id.org/italia/onto/HER/EUREKAProject"/>
    <rdfs:range rdf:resource="http://www.w3.org/2001/XMLSchema#decimal"/>
    <rdfs:comment xml:lang="en">Project total investment</rdfs:comment>
    <rdfs:comment xml:lang="it">Totale investimento del progetto</rdfs:comment>
    <rdfs:isDefinedBy rdf:resource="https://w3id.org/italia/onto/HER"/>
    <rdfs:label xml:lang="it">investimento totale</rdfs:label>
    <rdfs:label xml:lang="en">total investment</rdfs:label>
    <owl:versionInfo xml:lang="it">stabile</owl:versionInfo>
    <owl:versionInfo xml:lang="en">stable</owl:versionInfo>
  </rdf:Description>
  <rdf:Description rdf:nodeID="n5bb3bff42afb4ca286d2c3fead9507ddb346">
    <rdf:first rdf:resource="https://w3id.org/italia/onto/HER/USTATContributionByClass"/>
    <rdf:rest rdf:nodeID="n5bb3bff42afb4ca286d2c3fead9507ddb347"/>
  </rdf:Description>
  <rdf:Description rdf:nodeID="n5bb3bff42afb4ca286d2c3fead9507ddb263">
    <rdf:type rdf:resource="http://www.w3.org/1999/02/22-rdf-syntax-ns#List"/>
    <rdf:first>Supportive Care</rdf:first>
    <rdf:rest rdf:nodeID="n5bb3bff42afb4ca286d2c3fead9507ddb264"/>
  </rdf:Description>
  <rdf:Description rdf:about="https://w3id.org/italia/onto/HER/ctnprinAvailableBudget">
    <rdf:type rdf:resource="http://www.w3.org/2002/07/owl#DatatypeProperty"/>
    <rdf:type rdf:resource="http://www.w3.org/2002/07/owl#FunctionalProperty"/>
    <rdfs:domain rdf:resource="https://w3id.org/italia/onto/HER/CTNPRINFinancingFund"/>
    <rdfs:range rdf:resource="http://www.w3.org/2000/01/rdf-schema#Literal"/>
    <rdfs:comment xml:lang="en">Budget for the initiative available from the financing fund.</rdfs:comment>
    <rdfs:comment xml:lang="it">Budget per l'iniziativa in esame disponibile sul fondo di finanziamento.</rdfs:comment>
    <rdfs:isDefinedBy rdf:resource="https://w3id.org/italia/onto/HER"/>
    <rdfs:label xml:lang="en">available budget CTN/PRIN initiative's financing fund</rdfs:label>
    <rdfs:label xml:lang="it">budget fondo finanziamento iniziativa CTN/PRIN</rdfs:label>
    <owl:versionInfo xml:lang="it">stabile</owl:versionInfo>
    <owl:versionInfo xml:lang="en">stable</owl:versionInfo>
  </rdf:Description>
  <rdf:Description rdf:nodeID="n5bb3bff42afb4ca286d2c3fead9507ddb438">
    <rdf:type rdf:resource="http://www.w3.org/2002/07/owl#Restriction"/>
    <owl:onProperty rdf:resource="https://w3id.org/italia/onto/CLV/hasSpatialCoverage"/>
    <owl:allValuesFrom rdf:resource="https://w3id.org/italia/onto/CLV/Feature"/>
  </rdf:Description>
  <rdf:Description rdf:about="https://w3id.org/italia/onto/HER/isUnapprovedDevice">
    <rdf:type rdf:resource="http://www.w3.org/2002/07/owl#DatatypeProperty"/>
    <rdf:type rdf:resource="http://www.w3.org/2002/07/owl#FunctionalProperty"/>
    <rdfs:domain rdf:resource="https://w3id.org/italia/onto/HER/AACTStudy"/>
    <rdfs:range rdf:resource="http://www.w3.org/2001/XMLSchema#boolean"/>
    <rdfs:comment xml:lang="en">Indication that at least one device product studied in the clinical study has not been previously approved or cleared by the U.S. Food and Drug Administration (FDA) for one or more uses.</rdfs:comment>
    <rdfs:comment xml:lang="it">Indicazione che almeno un prodotto del dispositivo studiato nello studio clinico non è stato precedentemente approvato o approvato dalla Food and Drug Administration (FDA) degli Stati Uniti per uno o più usi.</rdfs:comment>
    <rdfs:isDefinedBy rdf:resource="https://w3id.org/italia/onto/HER"/>
    <rdfs:label xml:lang="en">is unapproved device?</rdfs:label>
    <rdfs:label xml:lang="it">è un dispositivo non regolamentato?</rdfs:label>
    <owl:versionInfo xml:lang="it">stabile</owl:versionInfo>
    <owl:versionInfo xml:lang="en">stable</owl:versionInfo>
  </rdf:Description>
  <rdf:Description rdf:about="https://w3id.org/italia/onto/HER/ItalianDiploma">
    <rdf:type rdf:resource="http://www.w3.org/2002/07/owl#Class"/>
    <rdfs:subClassOf rdf:resource="https://w3id.org/italia/onto/HER/Diploma"/>
    <rdfs:comment xml:lang="en">It is refers to the Italian maturity diploma that can be award upon successful completion of secondary education</rdfs:comment>
    <rdfs:comment xml:lang="it">Si riferisce al diploma di maturità italiano che può essere rilasciato al termine del ciclo di studi secondari.</rdfs:comment>
    <rdfs:isDefinedBy rdf:resource="https://w3id.org/italia/onto/HER"/>
    <rdfs:label xml:lang="it">Diploma italiano</rdfs:label>
    <rdfs:label xml:lang="en">Italian Diploma</rdfs:label>
    <owl:versionInfo xml:lang="it">stabile</owl:versionInfo>
    <owl:versionInfo xml:lang="en">stable</owl:versionInfo>
  </rdf:Description>
  <rdf:Description rdf:about="https://w3id.org/italia/onto/HER/masking">
    <rdf:type rdf:resource="http://www.w3.org/2002/07/owl#DatatypeProperty"/>
    <rdfs:domain rdf:resource="https://w3id.org/italia/onto/HER/AACTDesign"/>
    <rdfs:range rdf:nodeID="n5bb3bff42afb4ca286d2c3fead9507ddb186"/>
    <rdfs:comment xml:lang="it">Le parti coinvolte nello studio clinico che non possono conoscere gli interventi assegnati ai singoli partecipanti. I tipi di mascheramento comprendono: mascheramento aperto, mascheramento singolo cieco e mascheramento in doppio cieco.</rdfs:comment>
    <rdfs:comment xml:lang="en">The party or parties involved in the clinical trial who are prevented from having knowledge of the interventions assigned to individual participants. Types of masking include: open label, single blind masking, and double-blind masking.</rdfs:comment>
    <rdfs:isDefinedBy rdf:resource="https://w3id.org/italia/onto/HER"/>
    <rdfs:label xml:lang="it">mascheramento</rdfs:label>
    <rdfs:label xml:lang="en">masking</rdfs:label>
    <owl:versionInfo xml:lang="it">stabile</owl:versionInfo>
    <owl:versionInfo xml:lang="en">stable</owl:versionInfo>
  </rdf:Description>
  <rdf:Description rdf:nodeID="n5bb3bff42afb4ca286d2c3fead9507ddb224">
    <rdf:first rdf:resource="https://w3id.org/italia/onto/HER/MIURStudentsByDegreeDegreeClassAggregate"/>
    <rdf:rest rdf:nodeID="n5bb3bff42afb4ca286d2c3fead9507ddb225"/>
  </rdf:Description>
  <rdf:Description rdf:about="https://w3id.org/italia/onto/HER/primaryPurpose">
    <rdf:type rdf:resource="http://www.w3.org/2002/07/owl#DatatypeProperty"/>
    <rdfs:domain rdf:resource="https://w3id.org/italia/onto/HER/AACTDesign"/>
    <rdfs:range rdf:nodeID="n5bb3bff42afb4ca286d2c3fead9507ddb254"/>
    <rdfs:comment xml:lang="it">L'obiettivo principale degli interventi che vengono valutati dallo studio clinico. Gli scopi primari sono:
Trattamento: Uno o più interventi sono in fase di valutazione per il trattamento di una malattia, sindrome o condizione.
Prevenzione: Uno o più interventi sono in fase di valutazione per prevenire lo sviluppo di una specifica malattia o condizione di salute.
Diagnostica: Si stanno valutando uno o più interventi per identificare una malattia o una condizione di salute.
Cure di supporto: Uno o più interventi sono valutati per massimizzare il comfort, ridurre al minimo gli effetti collaterali o mitigare il declino della salute o della funzione del partecipante.
Screening: Uno o più interventi sono valutati o esaminati per identificare una condizione, o fattori di rischio per una condizione, in persone che non sono ancora note per avere la condizione o il fattore di rischio.
Ricerca sui servizi sanitari: Uno o più interventi per valutare la fornitura, i processi, la gestione, l'organizzazione o il finanziamento dell'assistenza sanitaria.
Scienza di base: Uno o più interventi per esaminare il meccanismo di base dell'azione (per esempio, la fisiologia o la biomeccanica di un intervento).
Fattibilità del dispositivo: Un intervento di un dispositivo viene valutato in un piccolo trial clinico (generalmente meno di 10 partecipanti) per determinare la fattibilità del prodotto; o un trial clinico per testare un prototipo di dispositivo per verificarne la fattibilità e non gli esiti sanitari. Tali studi sono condotti per confermare la progettazione e le specifiche operative di un dispositivo prima di iniziare una sperimentazione clinica completa.
Altro: Non si applica nessuna delle altre opzioni.</rdfs:comment>
    <rdfs:comment xml:lang="en">The main objective of the intervention(s) being evaluated by the clinical trial. Type os primary purpose are:
Treatment: One or more interventions are being evaluated for treating a disease, syndrome, or condition.
Prevention: One or more interventions are being assessed for preventing the development of a specific disease or health condition.
Diagnostic: One or more interventions are being evaluated for identifying a disease or health condition.
Supportive Care: One or more interventions are evaluated for maximizing comfort, minimizing side effects, or mitigating against a decline in the participant's health or function.
Screening: One or more interventions are assessed or examined for identifying a condition, or risk factors for a condition, in people who are not yet known to have the condition or risk factor.
Health Services Research: One or more interventions for evaluating the delivery, processes, management, organization, or financing of healthcare.
Basic Science: One or more interventions for examining the basic mechanism of action (for example, physiology or biomechanics of an intervention).
Device Feasibility: An intervention of a device product is being evaluated in a small clinical trial (generally fewer than 10 participants) to determine the feasibility of the product; or a clinical trial to test a prototype device for feasibility and not health outcomes. Such studies are conducted to confirm the design and operating specifications of a device before beginning a full clinical trial.
Other: None of the other options applies.
</rdfs:comment>
    <rdfs:isDefinedBy rdf:resource="https://w3id.org/italia/onto/HER"/>
    <rdfs:label xml:lang="it">Scopo primario</rdfs:label>
    <rdfs:label xml:lang="en">primary purpose</rdfs:label>
    <owl:versionInfo xml:lang="it">stabile</owl:versionInfo>
    <owl:versionInfo xml:lang="en">stable</owl:versionInfo>
  </rdf:Description>
  <rdf:Description rdf:about="https://w3id.org/italia/onto/HER/caregiverMasked">
    <rdf:type rdf:resource="http://www.w3.org/2002/07/owl#DatatypeProperty"/>
    <rdfs:domain rdf:resource="https://w3id.org/italia/onto/HER/AACTDesign"/>
    <rdfs:range rdf:resource="http://www.w3.org/2001/XMLSchema#boolean"/>
    <rdfs:comment xml:lang="en">Caregiver is the party or parties involved in the clinical trial who are prevented from having knowledge of the interventions assigned to individual participants. This property allows one to represent whether the caregiver is masked or not.</rdfs:comment>
    <rdfs:comment xml:lang="it">Il personale di assistenza sono le parti coinvolte nello studio clinico a cui viene impedito di conoscere gli interventi assegnati ai singoli partecipanti.</rdfs:comment>
    <rdfs:isDefinedBy rdf:resource="https://w3id.org/italia/onto/HER"/>
    <rdfs:label xml:lang="en">caregiver masked</rdfs:label>
    <rdfs:label xml:lang="it">parti coinvolte conoscono interventi</rdfs:label>
    <owl:versionInfo xml:lang="it">stabile</owl:versionInfo>
    <owl:versionInfo xml:lang="en">stable</owl:versionInfo>
  </rdf:Description>
  <rdf:Description rdf:nodeID="n5bb3bff42afb4ca286d2c3fead9507ddb405">
    <rdf:type rdf:resource="http://www.w3.org/2002/07/owl#Restriction"/>
    <owl:onProperty rdf:resource="https://w3id.org/italia/onto/HER/hasCHAFEAOutput"/>
    <owl:allValuesFrom rdf:resource="https://w3id.org/italia/onto/HER/CHAFEAOutput"/>
  </rdf:Description>
  <rdf:Description rdf:about="https://w3id.org/italia/data/project/OntoPiA">
    <rdf:type rdf:resource="http://www.w3.org/2002/07/owl#NamedIndividual"/>
    <rdf:type rdf:resource="https://w3id.org/italia/onto/ADMS/Project"/>
    <ns4:name xml:lang="it">OntoPiA - la rete di ontologie della pubblica amministrazione italiana</ns4:name>
    <rdfs:label xml:lang="it">OntoPiA - la rete di ontologie della pubblica amministrazione italiana</rdfs:label>
  </rdf:Description>
  <rdf:Description rdf:about="https://w3id.org/italia/onto/HER/hasArea">
    <rdf:type rdf:resource="http://www.w3.org/2002/07/owl#ObjectProperty"/>
    <rdfs:subPropertyOf rdf:resource="https://w3id.org/italia/onto/HER/hasAcademicDiscipline"/>
    <rdfs:domain rdf:nodeID="n5bb3bff42afb4ca286d2c3fead9507ddb35"/>
    <rdfs:range rdf:resource="https://w3id.org/italia/onto/HER/Area"/>
    <rdfs:comment xml:lang="en">Property that links some statistical aggregated data and the academic degree to the CUN area.</rdfs:comment>
    <rdfs:comment xml:lang="it">Proprietà che collega alcuni dati statistici e la laurea all'area CUN di riferimento della classificazione sulle discipline accademiche.</rdfs:comment>
    <rdfs:isDefinedBy rdf:resource="https://w3id.org/italia/onto/HER"/>
    <rdfs:label xml:lang="it">ha area CUN</rdfs:label>
    <rdfs:label xml:lang="en">has CUN area</rdfs:label>
    <owl:versionInfo xml:lang="it">stabile</owl:versionInfo>
    <owl:versionInfo xml:lang="en">stable</owl:versionInfo>
  </rdf:Description>
  <rdf:Description rdf:about="https://w3id.org/italia/onto/HER/hasEurekaCluster">
    <rdf:type rdf:resource="http://www.w3.org/2002/07/owl#ObjectProperty"/>
    <rdfs:domain rdf:resource="https://w3id.org/italia/onto/HER/EUREKAProject"/>
    <rdfs:range rdf:resource="https://w3id.org/italia/onto/HER/EUREKACluster"/>
    <rdfs:comment xml:lang="it">Questa proprietà collega un progetto EUREKA con il cluster corrispondente.</rdfs:comment>
    <rdfs:comment xml:lang="en">This property connects an EUREKA project with the corresponding cluster.</rdfs:comment>
    <rdfs:isDefinedBy rdf:resource="https://w3id.org/italia/onto/HER"/>
    <rdfs:label xml:lang="it">ha gruppo EUREKA</rdfs:label>
    <rdfs:label xml:lang="en">has EUREKA cluster</rdfs:label>
    <owl:versionInfo xml:lang="it">stabile</owl:versionInfo>
    <owl:versionInfo xml:lang="en">stable</owl:versionInfo>
  </rdf:Description>
  <rdf:Description rdf:nodeID="n5bb3bff42afb4ca286d2c3fead9507ddb444">
    <rdf:type rdf:resource="http://www.w3.org/2002/07/owl#Restriction"/>
    <owl:onProperty rdf:resource="https://w3id.org/italia/onto/HER/picNumber"/>
    <owl:maxCardinality rdf:datatype="http://www.w3.org/2001/XMLSchema#nonNegativeInteger">1</owl:maxCardinality>
  </rdf:Description>
  <rdf:Description rdf:about="https://w3id.org/italia/onto/HER/ErasmusPlusProjectResult">
    <rdf:type rdf:resource="http://www.w3.org/2002/07/owl#Class"/>
    <rdfs:subClassOf rdf:resource="https://w3id.org/italia/onto/HER/Result"/>
    <rdfs:subClassOf rdf:nodeID="n5bb3bff42afb4ca286d2c3fead9507ddb492"/>
    <rdfs:subClassOf rdf:nodeID="n5bb3bff42afb4ca286d2c3fead9507ddb493"/>
    <rdfs:comment xml:lang="en">It is used to address results for erasmus plus projects that have ended.</rdfs:comment>
    <rdfs:comment xml:lang="it">Viene utilizzato per indicare i risultati dei progetti erasmus plus che si sono conclusi.</rdfs:comment>
    <rdfs:isDefinedBy rdf:resource="https://w3id.org/italia/onto/HER"/>
    <rdfs:label xml:lang="en">Erasmus+ Project Result</rdfs:label>
    <rdfs:label xml:lang="it">Risultato progetto Erasmus+</rdfs:label>
    <owl:versionInfo xml:lang="it">stabile</owl:versionInfo>
    <owl:versionInfo xml:lang="en">stable</owl:versionInfo>
  </rdf:Description>
  <rdf:Description rdf:about="https://w3id.org/italia/onto/HER/patentPublicationNumber">
    <rdf:type rdf:resource="http://www.w3.org/2002/07/owl#DatatypeProperty"/>
    <rdfs:subPropertyOf rdf:resource="https://w3id.org/italia/onto/l0/identifier"/>
    <rdfs:domain rdf:resource="https://w3id.org/italia/onto/HER/PatentPublicationDetail"/>
    <rdfs:range rdf:resource="http://www.w3.org/2000/01/rdf-schema#Literal"/>
    <rdfs:comment xml:lang="it">Il numero di riferimento incrociato assegnato a una domanda di brevetto al momento della pubblicazione</rdfs:comment>
    <rdfs:comment xml:lang="en">The cross-reference number assigned to a patent application upon publication</rdfs:comment>
    <rdfs:isDefinedBy rdf:resource="https://w3id.org/italia/onto/HER"/>
    <rdfs:label xml:lang="it">numero pubblicazione brevetto</rdfs:label>
    <rdfs:label xml:lang="en">patent publication number</rdfs:label>
    <owl:versionInfo xml:lang="it">stabile</owl:versionInfo>
    <owl:versionInfo xml:lang="en">stable</owl:versionInfo>
  </rdf:Description>
  <rdf:Description rdf:about="https://w3id.org/italia/data/distribution/HERAPIT-JSON-LD">
    <rdf:type rdf:resource="http://www.w3.org/2002/07/owl#NamedIndividual"/>
    <rdf:type rdf:resource="https://w3id.org/italia/onto/ADMS/SemanticAssetDistribution"/>
    <ns2:description xml:lang="it">Questa è la distribuzione JSON-LD dell'ontologia della Ricerca Pubblica</ns2:description>
    <ns2:description xml:lang="en">This is the distribution in JSON-LD of the Public Research ontology</ns2:description>
    <ns2:format rdf:resource="http://publications.europa.eu/resource/authority/file-type/JSON_LD"/>
    <ns2:license rdf:resource="https://w3id.org/italia/controlled-vocabulary/licences/A21_CCBY40"/>
    <ns2:title xml:lang="it">Distribuzione JSON-LD ontologia PublicReseach-AP_IT</ns2:title>
    <ns2:title xml:lang="en">JSON-LD distribution of PublicReseach-AP_IT Ontology</ns2:title>
    <ns3:accessURL rdf:resource="https://raw.githubusercontent.com/italia/daf-ontologie-vocabolari-controllati/master/Ontologie/HER/latest"/>
    <ns3:downloadURL rdf:resource="https://raw.githubusercontent.com/italia/daf-ontologie-vocabolari-controllati/master/Ontologie/HER/latest/HER-AP_IT.jsonld"/>
  </rdf:Description>
  <rdf:Description rdf:about="https://w3id.org/italia/onto/HER/baselinePopulation">
    <rdf:type rdf:resource="http://www.w3.org/2002/07/owl#DatatypeProperty"/>
    <rdfs:domain rdf:resource="https://w3id.org/italia/onto/HER/AACTStudy"/>
    <rdfs:range rdf:resource="http://www.w3.org/2001/XMLSchema#int"/>
    <rdfs:comment xml:lang="en">Data collected at the beginning of a clinical study for all participants and for each arm or comparison group. These data include demographics, such as age, sex/gender, race and ethnicity, and study-specific measures (for example, systolic blood pressure, prior antidepressant treatment).</rdfs:comment>
    <rdfs:comment xml:lang="it">Dati raccolti all'inizio di uno studio clinico per tutti i partecipanti e per ogni braccio o gruppo di confronto. Questi dati includono dati demografici, come l'età, il sesso/genere, la razza e l'etnia, e misure specifiche dello studio (ad esempio, pressione sanguigna sistolica, trattamento antidepressivo preventivo).</rdfs:comment>
    <rdfs:isDefinedBy rdf:resource="https://w3id.org/italia/onto/HER"/>
    <rdfs:label xml:lang="en">baseline population</rdfs:label>
    <rdfs:label xml:lang="it">popolazione di base</rdfs:label>
    <owl:versionInfo xml:lang="it">stabile</owl:versionInfo>
    <owl:versionInfo xml:lang="en">stable</owl:versionInfo>
  </rdf:Description>
  <rdf:Description rdf:about="https://w3id.org/italia/onto/HER/sizeOfEntity">
    <rdf:type rdf:resource="http://www.w3.org/2002/07/owl#DatatypeProperty"/>
    <rdfs:domain rdf:resource="https://w3id.org/italia/onto/HER/CTNPRINEntity"/>
    <rdfs:range rdf:resource="http://www.w3.org/2000/01/rdf-schema#Literal"/>
    <rdfs:comment xml:lang="it">Dimensione dell'impresa secondo classificazione EU. N/A per soggetti pubblici. La proprietà deve essere valorizzata con le prefLabel di questo vocabolario controllato europeo: https://op.europa.eu/en/web/eu-vocabularies/at-concept-scheme/-/resource/authority/economic-operator-size/?target=Browse&amp;uri=http://publications.europa.eu/resource/authority/economic-operator-size</rdfs:comment>
    <rdfs:comment xml:lang="en">Enterprise size according to EU classification. N/A for public entities. The property should be valorized with the pref labels of the following EU controlled vocabulary: https://op.europa.eu/en/web/eu-vocabularies/at-concept-scheme/-/resource/authority/economic-operator-size/?target=Browse&amp;uri=http://publications.europa.eu/resource/authority/economic-operator-size</rdfs:comment>
    <rdfs:isDefinedBy rdf:resource="https://w3id.org/italia/onto/HER"/>
    <rdfs:label xml:lang="it">dimensione istituzione finanziata ctn/prin</rdfs:label>
    <rdfs:label xml:lang="en">size of ctn/prin funded institution</rdfs:label>
    <owl:versionInfo xml:lang="it">provvisoria - controllare come trasformare questa proprietà in una classe Concetto da allineare con skos:Concept così da utilizzare gli URI del vocabolario europeo https://op.europa.eu/en/web/eu-vocabularies/at-concept-scheme/-/resource/authority/economic-operator-size/?target=Browse&amp;uri=http://publications.europa.eu/resource/authority/economic-operator-size</owl:versionInfo>
    <owl:versionInfo xml:lang="en">unstable - investigate on how to transform this class in a Concept that is aligned with skos:Concept so that to reuse URis of the EU controlled vocabulary https://op.europa.eu/en/web/eu-vocabularies/at-concept-scheme/-/resource/authority/economic-operator-size/?target=Browse&amp;uri=http://publications.europa.eu/resource/authority/economic-operator-size</owl:versionInfo>
  </rdf:Description>
  <rdf:Description rdf:nodeID="n5bb3bff42afb4ca286d2c3fead9507ddb113">
    <rdf:first rdf:resource="https://w3id.org/italia/onto/HER/AcademicRole"/>
    <rdf:rest rdf:nodeID="n5bb3bff42afb4ca286d2c3fead9507ddb114"/>
  </rdf:Description>
  <rdf:Description rdf:about="https://w3id.org/italia/onto/HER/forChafeaProject">
    <rdf:type rdf:resource="http://www.w3.org/2002/07/owl#ObjectProperty"/>
    <rdfs:subPropertyOf rdf:resource="https://w3id.org/italia/onto/RO/forEntity"/>
    <rdfs:domain rdf:resource="https://w3id.org/italia/onto/HER/CHAFEAParticipant"/>
    <rdfs:range rdf:resource="https://w3id.org/italia/onto/HER/CHAFEAProject"/>
    <rdfs:comment xml:lang="it">Questa proprietà si collega ad una delle corrispondenti attività finanziate.</rdfs:comment>
    <rdfs:comment xml:lang="en">This property links to one of the corresponding funded activities.</rdfs:comment>
    <rdfs:isDefinedBy rdf:resource="https://w3id.org/italia/onto/HER"/>
    <rdfs:label xml:lang="it">ha un progetto chafea</rdfs:label>
    <rdfs:label xml:lang="en">has chafea project</rdfs:label>
    <owl:versionInfo xml:lang="it">prova</owl:versionInfo>
    <owl:versionInfo xml:lang="en">testing</owl:versionInfo>
  </rdf:Description>
  <rdf:Description rdf:about="https://w3id.org/italia/onto/HER/hasErasmusPlusParticipant">
    <rdf:type rdf:resource="http://www.w3.org/2002/07/owl#ObjectProperty"/>
    <rdfs:subPropertyOf rdf:resource="https://w3id.org/italia/onto/RO/hasRiT"/>
    <rdfs:domain rdf:resource="https://w3id.org/italia/onto/HER/ErasmusPlusProject"/>
    <rdfs:range rdf:resource="https://w3id.org/italia/onto/HER/ErasmusPlusParticipant"/>
    <rdfs:comment xml:lang="en">It is used to link Erasmus+ projects to the entities which partecipate in the project.</rdfs:comment>
    <rdfs:comment xml:lang="it">Viene utilizzato per collegare i progetti Erasmus+ alle entità che partecipano al progetto.</rdfs:comment>
    <rdfs:isDefinedBy rdf:resource="https://w3id.org/italia/onto/HER"/>
    <rdfs:label xml:lang="it">ha partecipante Erasmus+</rdfs:label>
    <rdfs:label xml:lang="en">has Erasmus+ participant</rdfs:label>
    <owl:versionInfo xml:lang="it">stabile</owl:versionInfo>
    <owl:versionInfo xml:lang="en">stable</owl:versionInfo>
  </rdf:Description>
  <rdf:Description rdf:about="https://w3id.org/italia/onto/HER/aactInterventionType">
    <rdf:type rdf:resource="http://www.w3.org/2002/07/owl#DatatypeProperty"/>
    <rdfs:domain rdf:resource="https://w3id.org/italia/onto/HER/AACTIntervention"/>
    <rdfs:range rdf:resource="http://www.w3.org/2000/01/rdf-schema#Literal"/>
    <rdfs:comment xml:lang="en">For each intervention studied in the clinical study, the general type of intervention. They are:
Drug: Including placebo
Device: Including sham
Biological/Vaccine
Procedure/Surgery
Radiation
Behavioral: For example, psychotherapy, lifestyle counseling
Genetic: Including gene transfer, stem cell and recombinant DNA
Dietary Supplement: For example, vitamins, minerals
Combination Product: Combining a drug and device, a biological product and device; a drug and biological product; or a drug, biological product, and device
Diagnostic Test: For example, imaging, in-vitro
Other
</rdfs:comment>
    <rdfs:comment xml:lang="it">Per ogni intervento studiato nello studio clinico, il tipo generale di intervento. Di seguito descritti:
Farmaci: Compreso il placebo
Dispositivo: Inclusa la finzione
Biologico/Vaccino
Procedimento/chirurgia
Radiazioni
Comportamentale: per esempio, psicoterapia, consulenza sullo stile di vita
Genetico: incluso il trasferimento di geni, cellule staminali e DNA ricombinante
Integratore alimentare: Per esempio, vitamine, minerali
Prodotto combinato: Combinazione di un farmaco e dispositivo, un prodotto e dispositivo biologico; un farmaco e prodotto biologico; o un farmaco, prodotto biologico e dispositivo
Test diagnostico: Per esempio, imaging, in vitro
Altro
</rdfs:comment>
    <rdfs:isDefinedBy rdf:resource="https://w3id.org/italia/onto/HER"/>
    <rdfs:label xml:lang="it">Tipo di intervento AACT</rdfs:label>
    <rdfs:label xml:lang="en">aact intervention type</rdfs:label>
    <owl:versionInfo xml:lang="it">provvisoria - valutare la possibilità di avere una classe specifica</owl:versionInfo>
    <owl:versionInfo xml:lang="en">unstable - evaluation of the possibility of having a specific class</owl:versionInfo>
  </rdf:Description>
  <rdf:Description rdf:about="https://w3id.org/italia/onto/HER/EUREKAProject">
    <rdf:type rdf:resource="http://www.w3.org/2002/07/owl#Class"/>
    <rdfs:subClassOf rdf:resource="https://w3id.org/italia/onto/Project/PublicResearchProject"/>
    <rdfs:subClassOf rdf:nodeID="n5bb3bff42afb4ca286d2c3fead9507ddb464"/>
    <rdfs:subClassOf rdf:nodeID="n5bb3bff42afb4ca286d2c3fead9507ddb465"/>
    <rdfs:subClassOf rdf:nodeID="n5bb3bff42afb4ca286d2c3fead9507ddb466"/>
    <rdfs:subClassOf rdf:nodeID="n5bb3bff42afb4ca286d2c3fead9507ddb467"/>
    <rdfs:subClassOf rdf:nodeID="n5bb3bff42afb4ca286d2c3fead9507ddb468"/>
    <rdfs:subClassOf rdf:nodeID="n5bb3bff42afb4ca286d2c3fead9507ddb469"/>
    <rdfs:subClassOf rdf:nodeID="n5bb3bff42afb4ca286d2c3fead9507ddb470"/>
    <rdfs:subClassOf rdf:nodeID="n5bb3bff42afb4ca286d2c3fead9507ddb471"/>
    <rdfs:subClassOf rdf:nodeID="n5bb3bff42afb4ca286d2c3fead9507ddb472"/>
    <rdfs:subClassOf rdf:nodeID="n5bb3bff42afb4ca286d2c3fead9507ddb473"/>
    <rdfs:comment xml:lang="en">Project funded by the EUREKA network.</rdfs:comment>
    <rdfs:comment xml:lang="it">Project funded by the EUREKA network.</rdfs:comment>
    <rdfs:isDefinedBy rdf:resource="https://w3id.org/italia/onto/HER"/>
    <rdfs:label xml:lang="en">EUREKA Project</rdfs:label>
    <rdfs:label xml:lang="it">Progetto EUREKA</rdfs:label>
    <owl:versionInfo xml:lang="it">stabile</owl:versionInfo>
    <owl:versionInfo xml:lang="en">stable</owl:versionInfo>
  </rdf:Description>
  <rdf:Description rdf:about="https://w3id.org/italia/onto/HER/resultsFirstSubmittedDate">
    <rdf:type rdf:resource="http://www.w3.org/2002/07/owl#DatatypeProperty"/>
    <rdfs:subPropertyOf rdf:resource="https://w3id.org/italia/onto/TI/date"/>
    <rdfs:domain rdf:resource="https://w3id.org/italia/onto/HER/AACTStudy"/>
    <rdfs:range rdf:resource="http://www.w3.org/2001/XMLSchema#date"/>
    <rdfs:comment xml:lang="en">Date on which first results were submited</rdfs:comment>
    <rdfs:comment xml:lang="it">La data in cui i primi risultati sono stati inviati.</rdfs:comment>
    <rdfs:isDefinedBy rdf:resource="https://w3id.org/italia/onto/HER"/>
    <rdfs:label xml:lang="en">results first submitted date</rdfs:label>
    <rdfs:label xml:lang="it">risultati prima data invio</rdfs:label>
    <owl:versionInfo xml:lang="it">stabile</owl:versionInfo>
    <owl:versionInfo xml:lang="en">stable</owl:versionInfo>
  </rdf:Description>
  <rdf:Description rdf:about="https://w3id.org/italia/onto/HER/hasFounderFaculty">
    <rdf:type rdf:resource="http://www.w3.org/2002/07/owl#ObjectProperty"/>
    <rdfs:domain rdf:resource="https://w3id.org/italia/onto/HER/Spinoff"/>
    <rdfs:range rdf:resource="https://w3id.org/italia/onto/COV/SupportUnit"/>
    <rdfs:comment xml:lang="en">Property used to link the spin-off to the faculty of the university of origin, or to a division of the research institution of origin.</rdfs:comment>
    <rdfs:comment xml:lang="en">Proprietà utilizzata per collegare lo spin-off alla facoltà dell'ateneo di origine, o a una divisione dell'ente di ricerca di origine.</rdfs:comment>
    <rdfs:isDefinedBy rdf:resource="https://w3id.org/italia/onto/HER"/>
    <rdfs:label xml:lang="it">has facoltà fondatrice</rdfs:label>
    <rdfs:label xml:lang="en">has founder faculty</rdfs:label>
    <owl:versionInfo xml:lang="it">prova</owl:versionInfo>
    <owl:versionInfo xml:lang="en">testing</owl:versionInfo>
  </rdf:Description>
  <rdf:Description rdf:about="https://w3id.org/italia/onto/HER/erasmusplusOrgType">
    <rdf:type rdf:resource="http://www.w3.org/2002/07/owl#DatatypeProperty"/>
    <rdfs:domain rdf:resource="https://w3id.org/italia/onto/HER/ErasmusPlusParticipant"/>
    <rdfs:range rdf:resource="http://www.w3.org/2000/01/rdf-schema#Literal"/>
    <rdfs:comment xml:lang="it">Quando disponibile, si riferisce al tipo di organizzazione che partecipa al progetto Erasmus+.</rdfs:comment>
    <rdfs:comment xml:lang="en">When available, it refers to the type of the organization participating in the Erasmus+ project.</rdfs:comment>
    <rdfs:isDefinedBy rdf:resource="https://w3id.org/italia/onto/HER"/>
    <rdfs:label xml:lang="en">erasmus+ organization type</rdfs:label>
    <rdfs:label xml:lang="it">tipologia di organizzazione erasmus+</rdfs:label>
    <owl:versionInfo xml:lang="it">provvisoria</owl:versionInfo>
    <owl:versionInfo xml:lang="en">unstable</owl:versionInfo>
  </rdf:Description>
  <rdf:Description rdf:about="https://w3id.org/italia/onto/HER/hasStartingDate">
    <rdf:type rdf:resource="http://www.w3.org/2002/07/owl#ObjectProperty"/>
    <rdfs:subPropertyOf rdf:resource="https://w3id.org/italia/onto/TI/hasTemporalEntity"/>
    <rdfs:domain rdf:nodeID="n5bb3bff42afb4ca286d2c3fead9507ddb86"/>
    <rdfs:range rdf:resource="https://w3id.org/italia/onto/TI#TimeInstant"/>
    <rdfs:comment xml:lang="it">Data di inizio di uno studio o di un'operazione.</rdfs:comment>
    <rdfs:comment xml:lang="en">Starting date of a study or operation.</rdfs:comment>
    <rdfs:isDefinedBy rdf:resource="https://w3id.org/italia/onto/HER"/>
    <rdfs:label xml:lang="it">ha data di inizio</rdfs:label>
    <rdfs:label xml:lang="en">has starting date</rdfs:label>
    <owl:versionInfo xml:lang="it">prova</owl:versionInfo>
    <owl:versionInfo xml:lang="en">testing</owl:versionInfo>
  </rdf:Description>
  <rdf:Description rdf:about="https://w3id.org/italia/onto/HER/MIURStudentsByDiplomaDegreeDegreeClassAggregate">
    <rdf:type rdf:resource="http://www.w3.org/2002/07/owl#Class"/>
    <rdfs:subClassOf rdf:resource="https://w3id.org/italia/onto/HER/StatisticalDataAggregation"/>
    <rdfs:comment xml:lang="en">Aggregated data on Italian students filed in the MIUR system, grouped by year, university, diploma, degree and degree class.</rdfs:comment>
    <rdfs:comment xml:lang="it">Dati aggregati sugli studenti italiani archiviati nel sistema MIUR, raggruppati per anno, università, diploma, laurea e classe di laurea.</rdfs:comment>
    <rdfs:isDefinedBy rdf:resource="https://w3id.org/italia/onto/HER"/>
    <rdfs:label xml:lang="en">Aggregate of Italian Students By Diploma, Degree and Degree Class</rdfs:label>
    <rdfs:label xml:lang="it">Aggregazione dei studenti italiani per diploma, laurea e classe di laurea</rdfs:label>
    <owl:versionInfo xml:lang="it">stabile</owl:versionInfo>
    <owl:versionInfo xml:lang="en">stable</owl:versionInfo>
  </rdf:Description>
  <rdf:Description rdf:nodeID="n5bb3bff42afb4ca286d2c3fead9507ddb412">
    <rdf:type rdf:resource="http://www.w3.org/2002/07/owl#Restriction"/>
    <owl:onProperty rdf:resource="https://w3id.org/italia/onto/l0/name"/>
    <owl:someValuesFrom rdf:resource="http://www.w3.org/2000/01/rdf-schema#Literal"/>
  </rdf:Description>
  <rdf:Description rdf:nodeID="n5bb3bff42afb4ca286d2c3fead9507ddb256">
    <rdf:type rdf:resource="http://www.w3.org/1999/02/22-rdf-syntax-ns#List"/>
    <rdf:first>Device Feasibility</rdf:first>
    <rdf:rest rdf:nodeID="n5bb3bff42afb4ca286d2c3fead9507ddb257"/>
  </rdf:Description>
  <rdf:Description rdf:about="https://w3id.org/italia/onto/HER/ErasmusPlusProject">
    <rdf:type rdf:resource="http://www.w3.org/2002/07/owl#Class"/>
    <rdfs:subClassOf rdf:resource="https://w3id.org/italia/onto/Project/PublicInvestmentProject"/>
    <rdfs:subClassOf rdf:nodeID="n5bb3bff42afb4ca286d2c3fead9507ddb482"/>
    <rdfs:subClassOf rdf:nodeID="n5bb3bff42afb4ca286d2c3fead9507ddb483"/>
    <rdfs:subClassOf rdf:nodeID="n5bb3bff42afb4ca286d2c3fead9507ddb484"/>
    <rdfs:subClassOf rdf:nodeID="n5bb3bff42afb4ca286d2c3fead9507ddb485"/>
    <rdfs:subClassOf rdf:nodeID="n5bb3bff42afb4ca286d2c3fead9507ddb486"/>
    <rdfs:subClassOf rdf:nodeID="n5bb3bff42afb4ca286d2c3fead9507ddb487"/>
    <rdfs:subClassOf rdf:nodeID="n5bb3bff42afb4ca286d2c3fead9507ddb488"/>
    <rdfs:subClassOf rdf:nodeID="n5bb3bff42afb4ca286d2c3fead9507ddb489"/>
    <rdfs:subClassOf rdf:nodeID="n5bb3bff42afb4ca286d2c3fead9507ddb490"/>
    <rdfs:subClassOf rdf:nodeID="n5bb3bff42afb4ca286d2c3fead9507ddb491"/>
    <rdfs:comment xml:lang="en">It refers to projects under the funding scheme "Erasmus+" from the European Union for education, training, youth and sport in Europe.</rdfs:comment>
    <rdfs:comment xml:lang="it">Si riferisce a progetti nell'ambito del programma di finanziamento "Erasmus+" dell'Unione Europea per l'istruzione, la formazione, la gioventù e lo sport in Europa.</rdfs:comment>
    <rdfs:isDefinedBy rdf:resource="https://w3id.org/italia/onto/HER"/>
    <rdfs:label xml:lang="en">Erasmus+ Project</rdfs:label>
    <rdfs:label xml:lang="it">Progetto Erasmus+</rdfs:label>
    <owl:versionInfo xml:lang="it">stabile</owl:versionInfo>
    <owl:versionInfo xml:lang="en">stable</owl:versionInfo>
  </rdf:Description>
  <rdf:Description rdf:about="https://w3id.org/italia/onto/HER/totalMale">
    <rdf:type rdf:resource="http://www.w3.org/2002/07/owl#DatatypeProperty"/>
    <rdfs:subPropertyOf rdf:resource="https://w3id.org/italia/onto/MU/value"/>
    <rdfs:domain rdf:nodeID="n5bb3bff42afb4ca286d2c3fead9507ddb339"/>
    <rdfs:range rdf:resource="http://www.w3.org/2000/01/rdf-schema#Literal"/>
    <rdfs:comment xml:lang="en">Total with respect to the male population of the sample considered.</rdfs:comment>
    <rdfs:comment xml:lang="it">Totale rispetto alla popolazione di sesso maschile del campione considerato.</rdfs:comment>
    <rdfs:isDefinedBy rdf:resource="https://w3id.org/italia/onto/HER"/>
    <rdfs:label xml:lang="en">total male</rdfs:label>
    <rdfs:label xml:lang="it">totale generemaschile</rdfs:label>
    <owl:versionInfo xml:lang="it">stabile</owl:versionInfo>
    <owl:versionInfo xml:lang="en">stable</owl:versionInfo>
  </rdf:Description>
  <rdf:Description rdf:about="https://w3id.org/italia/onto/HER/title">
    <rdf:type rdf:resource="http://www.w3.org/2002/07/owl#DatatypeProperty"/>
    <rdfs:domain rdf:resource="http://www.w3.org/2002/07/owl#Thing"/>
    <rdfs:range rdf:resource="http://www.w3.org/2000/01/rdf-schema#Literal"/>
    <rdfs:comment xml:lang="it">Testo del titolo di un progetto, risultato della ricerca, ecc.</rdfs:comment>
    <rdfs:comment xml:lang="en">Text of the title of a project, research output, etc.</rdfs:comment>
    <rdfs:isDefinedBy rdf:resource="https://w3id.org/italia/onto/HER"/>
    <rdfs:label xml:lang="en">title</rdfs:label>
    <rdfs:label xml:lang="it">titolo</rdfs:label>
    <owl:versionInfo xml:lang="it">stabile</owl:versionInfo>
    <owl:versionInfo xml:lang="en">stable</owl:versionInfo>
  </rdf:Description>
  <rdf:Description rdf:about="https://w3id.org/italia/onto/HER/totalMaleEnrolled">
    <rdf:type rdf:resource="http://www.w3.org/2002/07/owl#DatatypeProperty"/>
    <rdfs:subPropertyOf rdf:resource="https://w3id.org/italia/onto/MU/value"/>
    <rdfs:domain rdf:resource="https://w3id.org/italia/onto/HER/USTATStudentsBySexAggregate"/>
    <rdfs:range rdf:resource="http://www.w3.org/2000/01/rdf-schema#Literal"/>
    <rdfs:comment xml:lang="en">Number of registered male students corresponding to the selected combination of variables. In particular: number of male students who, with reference to a.a. (t) - (t+1), are enrolled on July 31st of the year (t+1). Notes: Students of levels 6 and 7 of ISCED 2011. For the year 2018-2019: elaborations on ANS data - extraction December 2019.</rdfs:comment>
    <rdfs:comment xml:lang="it">Numero di studenti di genere maschile iscritti, corrispondente alla combinazione di variabili selezionata. In particolare: numero di studenti di genere maschile che, con riferimento all' a.a. (t) - (t+1), risultano iscritti alla data del 31 luglio dell'anno (t+1). Note: Studenti dei livelli 6 e 7 della ISCED 2011. Per l'anno 2018-2019: elaborazioni su dati ANS - estrazione Dicembre 2019.</rdfs:comment>
    <rdfs:isDefinedBy rdf:resource="https://w3id.org/italia/onto/HER"/>
    <rdfs:label xml:lang="en">total male enrolled</rdfs:label>
    <rdfs:label xml:lang="it">totale di generemaschile iscritto</rdfs:label>
    <owl:versionInfo xml:lang="it">stabile</owl:versionInfo>
    <owl:versionInfo xml:lang="en">stable</owl:versionInfo>
  </rdf:Description>
  <rdf:Description rdf:about="https://w3id.org/italia/onto/HER/hasAACTMeshTerm">
    <rdf:type rdf:resource="http://www.w3.org/2002/07/owl#ObjectProperty"/>
    <rdfs:domain rdf:resource="https://w3id.org/italia/onto/HER/AACTStudy"/>
    <rdfs:range rdf:resource="https://w3id.org/italia/onto/HER/AACTMeshTerm"/>
    <rdfs:isDefinedBy rdf:resource="https://w3id.org/italia/onto/HER"/>
    <rdfs:label xml:lang="it">ha termine MeSH riportato da AACT</rdfs:label>
    <rdfs:label xml:lang="en">has AACT reported MeSH term</rdfs:label>
    <owl:versionInfo xml:lang="it">provvisoria</owl:versionInfo>
    <owl:versionInfo xml:lang="en">unstable</owl:versionInfo>
  </rdf:Description>
  <rdf:Description rdf:about="https://w3id.org/italia/onto/HER/ErasmusPlusProgramme">
    <rdf:type rdf:resource="http://www.w3.org/2002/07/owl#Class"/>
    <rdfs:subClassOf rdf:resource="https://w3id.org/italia/onto/HER/ErasmusPlusClassification"/>
    <rdfs:comment xml:lang="en">It refers to the funding programme (for example, Erasmus).</rdfs:comment>
    <rdfs:comment xml:lang="it">Si riferisce al programma di finanziamento (per esempio, Erasmus).</rdfs:comment>
    <rdfs:isDefinedBy rdf:resource="https://w3id.org/italia/onto/HER"/>
    <rdfs:label xml:lang="en">Erasmus+ Programme</rdfs:label>
    <rdfs:label xml:lang="it">Programma Erasmus+</rdfs:label>
    <owl:versionInfo xml:lang="it">stabile</owl:versionInfo>
    <owl:versionInfo xml:lang="en">stable</owl:versionInfo>
    <ns6:wasDerivedFrom rdf:resource="http://www.w3.org/2004/02/skos/core#Concept"/>
  </rdf:Description>
  <rdf:Description rdf:nodeID="n5bb3bff42afb4ca286d2c3fead9507ddb190">
    <rdf:type rdf:resource="http://www.w3.org/1999/02/22-rdf-syntax-ns#List"/>
    <rdf:first>Single</rdf:first>
    <rdf:rest rdf:nodeID="n5bb3bff42afb4ca286d2c3fead9507ddb191"/>
  </rdf:Description>
  <rdf:Description rdf:about="https://w3id.org/italia/onto/HER/total">
    <rdf:type rdf:resource="http://www.w3.org/2002/07/owl#DatatypeProperty"/>
    <rdfs:subPropertyOf rdf:resource="https://w3id.org/italia/onto/MU/value"/>
    <rdfs:domain rdf:nodeID="n5bb3bff42afb4ca286d2c3fead9507ddb297"/>
    <rdfs:range rdf:resource="http://www.w3.org/2001/XMLSchema#decimal"/>
    <rdfs:comment xml:lang="it">L'intero numero o importo.</rdfs:comment>
    <rdfs:comment xml:lang="en">The whole number or amount.</rdfs:comment>
    <rdfs:isDefinedBy rdf:resource="https://w3id.org/italia/onto/HER"/>
    <rdfs:label xml:lang="en">total</rdfs:label>
    <rdfs:label xml:lang="it">totale</rdfs:label>
    <owl:versionInfo xml:lang="it">provissoria - valutare un renaming della proprietà</owl:versionInfo>
    <owl:versionInfo xml:lang="en">unstable - check for a renaming of the property</owl:versionInfo>
  </rdf:Description>
  <rdf:Description rdf:about="https://w3id.org/italia/onto/HER/ERCPanel">
    <rdf:type rdf:resource="http://www.w3.org/2002/07/owl#Class"/>
    <rdfs:subClassOf rdf:resource="https://w3id.org/italia/onto/HER/ERCClassification"/>
    <rdfs:comment xml:lang="en">English Version: http://www.unipr.it/sites/default/files/allegatiparagrafo/01-08-2013/settori_erc.pdf</rdfs:comment>
    <rdfs:comment xml:lang="it">Versione in Italiano:
https://it.wikipedia.org/wiki/Settori_ERC</rdfs:comment>
    <rdfs:isDefinedBy rdf:resource="https://w3id.org/italia/onto/HER"/>
    <rdfs:label xml:lang="en">ERC Panel</rdfs:label>
    <rdfs:label xml:lang="it">Pannello ERC</rdfs:label>
    <owl:versionInfo xml:lang="it">stabile</owl:versionInfo>
    <owl:versionInfo xml:lang="en">stable</owl:versionInfo>
    <ns6:wasDerivedFrom rdf:resource="http://www.w3.org/2004/02/skos/core#Concept"/>
    <ns4:controlledVocabulary rdf:resource="https://w3id.org/italia/controlled-vocabulary/classifications-for-her/erc-panel-h2020-fp"/>
  </rdf:Description>
  <rdf:Description rdf:about="https://w3id.org/italia/onto/HER/ctnprinOperationGrantedContribution">
    <rdf:type rdf:resource="http://www.w3.org/2002/07/owl#DatatypeProperty"/>
    <rdfs:subPropertyOf rdf:resource="https://w3id.org/italia/onto/MU/value"/>
    <rdfs:domain rdf:resource="https://w3id.org/italia/onto/HER/CTNPRINOperation"/>
    <rdfs:range rdf:resource="http://www.w3.org/2001/XMLSchema#decimal"/>
    <rdfs:comment xml:lang="en">It represents the contributions disbursed in relation to the costs approved for the operation.</rdfs:comment>
    <rdfs:comment xml:lang="it">Rappresenta i contributi erogati rispetto ai costi approvati per l'operazione.</rdfs:comment>
    <rdfs:isDefinedBy rdf:resource="https://w3id.org/italia/onto/HER"/>
    <rdfs:label xml:lang="it">contributo erogato per operazioni CTN/PRIN</rdfs:label>
    <rdfs:label xml:lang="en">granted contribution of CTN/PRIN operation</rdfs:label>
    <owl:versionInfo xml:lang="it">stabile</owl:versionInfo>
    <owl:versionInfo xml:lang="en">stable</owl:versionInfo>
  </rdf:Description>
  <rdf:Description rdf:nodeID="n5bb3bff42afb4ca286d2c3fead9507ddb394">
    <rdf:type rdf:resource="http://www.w3.org/2002/07/owl#Restriction"/>
    <owl:onProperty rdf:resource="https://w3id.org/italia/onto/HER/studyFirstSubmittedQCDate"/>
    <owl:maxQualifiedCardinality rdf:datatype="http://www.w3.org/2001/XMLSchema#nonNegativeInteger">1</owl:maxQualifiedCardinality>
    <owl:onDataRange rdf:resource="http://www.w3.org/2001/XMLSchema#date"/>
  </rdf:Description>
  <rdf:Description rdf:nodeID="n5bb3bff42afb4ca286d2c3fead9507ddb24">
    <rdf:first rdf:resource="https://w3id.org/italia/onto/HER/MIURStudentsByCitizenshipDegreeDegreeClassAggregate"/>
    <rdf:rest rdf:nodeID="n5bb3bff42afb4ca286d2c3fead9507ddb25"/>
  </rdf:Description>
  <rdf:Description rdf:nodeID="n5bb3bff42afb4ca286d2c3fead9507ddb470">
    <rdf:type rdf:resource="http://www.w3.org/2002/07/owl#Restriction"/>
    <owl:onProperty rdf:resource="https://w3id.org/italia/onto/HER/eurekaProjectId"/>
    <owl:cardinality rdf:datatype="http://www.w3.org/2001/XMLSchema#nonNegativeInteger">1</owl:cardinality>
  </rdf:Description>
  <rdf:Description rdf:about="https://w3id.org/italia/onto/HER/WIPOIPCSubgroup">
    <rdf:type rdf:resource="http://www.w3.org/2002/07/owl#Class"/>
    <rdfs:subClassOf rdf:resource="https://w3id.org/italia/onto/HER/InternationalPatentClassification"/>
    <rdfs:comment xml:lang="it">La sottoclasse è seguita da un numero di "gruppo" composto da una a tre cifre, un tratto obliquo e un numero di almeno due cifre che rappresentano un "gruppo principale" o "sottogruppo".</rdfs:comment>
    <rdfs:comment xml:lang="en">The subclass is followed by a one-to-three-digit "group" number, an oblique stroke and a number of at least two digits representing a "main group" or "subgroup".</rdfs:comment>
    <rdfs:isDefinedBy rdf:resource="https://w3id.org/italia/onto/HER"/>
    <rdfs:label xml:lang="it">Sottogruppo WIPO IPC</rdfs:label>
    <rdfs:label xml:lang="en">WIPO IPC Subgroup</rdfs:label>
    <owl:versionInfo xml:lang="it">stabile</owl:versionInfo>
    <owl:versionInfo xml:lang="en">stable</owl:versionInfo>
    <ns6:wasDerivedFrom rdf:resource="http://www.w3.org/2004/02/skos/core#Concept"/>
  </rdf:Description>
  <rdf:Description rdf:about="https://w3id.org/italia/onto/HER/abstract">
    <rdf:type rdf:resource="http://www.w3.org/2002/07/owl#DatatypeProperty"/>
    <rdfs:subPropertyOf rdf:resource="https://w3id.org/italia/onto/l0/description"/>
    <rdfs:domain rdf:nodeID="n5bb3bff42afb4ca286d2c3fead9507ddb118"/>
    <rdfs:range rdf:resource="http://www.w3.org/2000/01/rdf-schema#Literal"/>
    <rdfs:comment xml:lang="it">Testo dell'abstract di un progetto, di un risultato della ricerca, di un'operazione.</rdfs:comment>
    <rdfs:comment xml:lang="en">Text of the abstract of a project, research output, accounting operation</rdfs:comment>
    <rdfs:isDefinedBy rdf:resource="https://w3id.org/italia/onto/HER"/>
    <rdfs:label xml:lang="en">abstract</rdfs:label>
    <rdfs:label xml:lang="it">riassunto</rdfs:label>
    <owl:versionInfo xml:lang="it">stabile</owl:versionInfo>
    <owl:versionInfo xml:lang="en">stable</owl:versionInfo>
  </rdf:Description>
  <rdf:Description rdf:nodeID="n5bb3bff42afb4ca286d2c3fead9507ddb2">
    <rdf:first rdf:resource="https://w3id.org/italia/onto/HER/ECProject"/>
    <rdf:rest rdf:nodeID="n5bb3bff42afb4ca286d2c3fead9507ddb3"/>
  </rdf:Description>
  <rdf:Description rdf:about="https://w3id.org/italia/onto/HER/AACTSponsor">
    <rdf:type rdf:resource="http://www.w3.org/2002/07/owl#Class"/>
    <rdfs:subClassOf rdf:resource="https://w3id.org/italia/onto/COV/PrivateOrganization"/>
    <rdfs:subClassOf rdf:nodeID="n5bb3bff42afb4ca286d2c3fead9507ddb380"/>
    <rdfs:comment xml:lang="it">L'organizzazione o la persona che avvia lo studio e che ha autorità e controllo sullo studio.</rdfs:comment>
    <rdfs:comment xml:lang="en">The organization or person who initiates the study and who has authority and control over the study.</rdfs:comment>
    <rdfs:isDefinedBy rdf:resource="https://w3id.org/italia/onto/HER"/>
    <rdfs:label xml:lang="en">Sponsor</rdfs:label>
    <rdfs:label xml:lang="it">sponsor</rdfs:label>
    <owl:versionInfo xml:lang="it">stabile</owl:versionInfo>
    <owl:versionInfo xml:lang="en">stable</owl:versionInfo>
  </rdf:Description>
  <rdf:Description rdf:about="https://w3id.org/italia/onto/HER/interventionModel">
    <rdf:type rdf:resource="http://www.w3.org/2002/07/owl#DatatypeProperty"/>
    <rdfs:domain rdf:resource="https://w3id.org/italia/onto/HER/AACTDesign"/>
    <rdfs:range rdf:resource="http://www.w3.org/2000/01/rdf-schema#Literal"/>
    <rdfs:comment xml:lang="it">Il disegno generale della strategia per l'assegnazione degli interventi ai partecipanti ad uno studio clinico. I tipi di modelli di intervento includono:
Gruppo singolo: Studi clinici in una sola branca
Parallelo: I partecipanti sono assegnati a uno dei due o più gruppi in parallelo per tutta la durata dello studio
Crossover: I partecipanti ricevono uno dei due (o più) interventi alternativi durante la fase iniziale dello studio e ricevono l'altro intervento durante la seconda fase dello studio
Fattoriale: Due o più interventi, ciascuno da solo e in combinazione, sono valutati in parallelo rispetto ad un gruppo di controllo
Sequenziale: I gruppi di partecipanti sono assegnati a ricevere gli interventi in base alle tappe precedenti che vengono raggiunte nello studio, come ad esempio in alcuni studi di escalation di dose e di progettazione adattiva


</rdfs:comment>
    <rdfs:comment xml:lang="en">The general design of the strategy for assigning interventions to participants in a clinical study. Types of intervention models include:
Single Group: Clinical trials with a single arm
Parallel: Participants are assigned to one of two or more groups in parallel for the duration of the study
Crossover: Participants receive one of two (or more) alternative interventions during the initial phase of the study and receive the other intervention during the second phase of the study
Factorial: Two or more interventions, each alone and in combination, are evaluated in parallel against a control group
Sequential: Groups of participants are assigned to receive interventions based on prior milestones being reached in the study, such as in some dose escalation and adaptive design studies
</rdfs:comment>
    <rdfs:isDefinedBy rdf:resource="https://w3id.org/italia/onto/HER"/>
    <rdfs:label xml:lang="it">Modello di Intervento</rdfs:label>
    <rdfs:label xml:lang="en">intervention model</rdfs:label>
    <owl:versionInfo xml:lang="it">provvisoria - controllare se sono previsti solo individui fissi</owl:versionInfo>
    <owl:versionInfo xml:lang="en">unstable - check whether there are fixed values only</owl:versionInfo>
  </rdf:Description>
  <rdf:Description rdf:about="https://w3id.org/italia/onto/HER/CHAFEAProject">
    <rdf:type rdf:resource="http://www.w3.org/2002/07/owl#Class"/>
    <rdfs:subClassOf rdf:resource="https://w3id.org/italia/onto/Project/PublicResearchProject"/>
    <rdfs:subClassOf rdf:nodeID="n5bb3bff42afb4ca286d2c3fead9507ddb404"/>
    <rdfs:subClassOf rdf:nodeID="n5bb3bff42afb4ca286d2c3fead9507ddb405"/>
    <rdfs:subClassOf rdf:nodeID="n5bb3bff42afb4ca286d2c3fead9507ddb406"/>
    <rdfs:subClassOf rdf:nodeID="n5bb3bff42afb4ca286d2c3fead9507ddb407"/>
    <rdfs:subClassOf rdf:nodeID="n5bb3bff42afb4ca286d2c3fead9507ddb408"/>
    <rdfs:subClassOf rdf:nodeID="n5bb3bff42afb4ca286d2c3fead9507ddb409"/>
    <rdfs:subClassOf rdf:nodeID="n5bb3bff42afb4ca286d2c3fead9507ddb410"/>
    <rdfs:subClassOf rdf:nodeID="n5bb3bff42afb4ca286d2c3fead9507ddb411"/>
    <rdfs:comment xml:lang="it">Attività finanziata pubblicata dall'Agenzia esecutiva per i consumatori, la salute, l'agricoltura e l'alimentazione (CHAFEA)</rdfs:comment>
    <rdfs:comment xml:lang="en">Funded activity published by the Consumers, Health, Agriculture and Food Executive Agency (CHAFEA)</rdfs:comment>
    <rdfs:isDefinedBy rdf:resource="https://w3id.org/italia/onto/HER"/>
    <rdfs:label xml:lang="en">CHAFEA Project</rdfs:label>
    <rdfs:label xml:lang="it">Progetto CHAFEA</rdfs:label>
    <owl:versionInfo xml:lang="it">stabile</owl:versionInfo>
    <owl:versionInfo xml:lang="en">stable</owl:versionInfo>
  </rdf:Description>
  <rdf:Description rdf:nodeID="n5bb3bff42afb4ca286d2c3fead9507ddb232">
    <rdf:type rdf:resource="http://www.w3.org/1999/02/22-rdf-syntax-ns#List"/>
    <rdf:first>Case Control</rdf:first>
    <rdf:rest rdf:nodeID="n5bb3bff42afb4ca286d2c3fead9507ddb233"/>
  </rdf:Description>
  <rdf:Description rdf:nodeID="n5bb3bff42afb4ca286d2c3fead9507ddb435">
    <rdf:type rdf:resource="http://www.w3.org/2002/07/owl#Restriction"/>
    <owl:onProperty rdf:resource="https://w3id.org/italia/onto/HER/removedCountry"/>
    <owl:maxQualifiedCardinality rdf:datatype="http://www.w3.org/2001/XMLSchema#nonNegativeInteger">1</owl:maxQualifiedCardinality>
    <owl:onDataRange rdf:resource="http://www.w3.org/2001/XMLSchema#boolean"/>
  </rdf:Description>
  <rdf:Description rdf:nodeID="n5bb3bff42afb4ca286d2c3fead9507ddb180">
    <rdf:type rdf:resource="http://www.w3.org/1999/02/22-rdf-syntax-ns#List"/>
    <rdf:first>Enrolling by invitation</rdf:first>
    <rdf:rest rdf:nodeID="n5bb3bff42afb4ca286d2c3fead9507ddb181"/>
  </rdf:Description>
  <rdf:Description rdf:about="https://w3id.org/italia/onto/HER/biospecDescription">
    <rdf:type rdf:resource="http://www.w3.org/2002/07/owl#DatatypeProperty"/>
    <rdfs:subPropertyOf rdf:resource="https://w3id.org/italia/onto/l0/description"/>
    <rdfs:domain rdf:resource="https://w3id.org/italia/onto/HER/AACTStudy"/>
    <rdfs:range rdf:resource="http://www.w3.org/2000/01/rdf-schema#Literal"/>
    <rdfs:comment xml:lang="en">Biological samples of material from study participants (e.g., whole blood, serum, white cells, urine, tissue).</rdfs:comment>
    <rdfs:comment xml:lang="it">Descrizione dei campioni biologici di materiale proveniente dai partecipanti allo studio (ad esempio, sangue intero, siero, globuli bianchi, urine, tessuti).</rdfs:comment>
    <rdfs:isDefinedBy rdf:resource="https://w3id.org/italia/onto/HER"/>
    <rdfs:label xml:lang="en">biospec description</rdfs:label>
    <rdfs:label xml:lang="it">descrizione biospec</rdfs:label>
    <owl:versionInfo xml:lang="it">stabile</owl:versionInfo>
    <owl:versionInfo xml:lang="en">stable</owl:versionInfo>
  </rdf:Description>
  <rdf:Description rdf:about="https://w3id.org/italia/onto/HER/numberOfArms">
    <rdf:type rdf:resource="http://www.w3.org/2002/07/owl#DatatypeProperty"/>
    <rdfs:domain rdf:resource="https://w3id.org/italia/onto/HER/AACTStudy"/>
    <rdfs:range rdf:resource="http://www.w3.org/2001/XMLSchema#int"/>
    <rdfs:comment xml:lang="en">number of pre-specified group or subgroup of participant(s) in a clinical trial assigned to receive specific intervention(s) (or no intervention) according to a protocol.</rdfs:comment>
    <rdfs:comment xml:lang="it">numero di gruppi o sottogruppi predefiniti di partecipanti ad uno studio clinico assegnati a ricevere uno o più interventi specifici (o nessun intervento) secondo un protocollo.</rdfs:comment>
    <rdfs:isDefinedBy rdf:resource="https://w3id.org/italia/onto/HER"/>
    <rdfs:label xml:lang="en">number of arms</rdfs:label>
    <rdfs:label xml:lang="it">numero di bracci</rdfs:label>
    <owl:versionInfo xml:lang="it">stabile</owl:versionInfo>
    <owl:versionInfo xml:lang="en">stable</owl:versionInfo>
  </rdf:Description>
  <rdf:Description rdf:about="https://w3id.org/italia/onto/HER/ctnprinOperationCommittedContribution">
    <rdf:type rdf:resource="http://www.w3.org/2002/07/owl#DatatypeProperty"/>
    <rdfs:subPropertyOf rdf:resource="https://w3id.org/italia/onto/MU/value"/>
    <rdfs:domain rdf:resource="https://w3id.org/italia/onto/HER/CTNPRINOperation"/>
    <rdfs:range rdf:resource="http://www.w3.org/2001/XMLSchema#decimal"/>
    <rdfs:comment xml:lang="it">Contributi impegnati dal Ministero sui costi ammessi a seguito di valutazione ex-ante. Calcolati come somma dell'omologa variabile "committedContribution" presente a livello di aggregazione inferiore (committedContribution_operations)</rdfs:comment>
    <rdfs:comment xml:lang="en">Contributions committed by the Ministry on eligible costs following ex-ante evaluation. Calculated as the sum of the corresponding 'committedContribution' variable at the lower aggregation level (committedContribution_operations).</rdfs:comment>
    <rdfs:isDefinedBy rdf:resource="https://w3id.org/italia/onto/HER"/>
    <rdfs:label xml:lang="en">committed contribution of CTN/PRIN operation</rdfs:label>
    <rdfs:label xml:lang="it">contributi impegnati per operazioni CTN/PRIN</rdfs:label>
    <owl:versionInfo xml:lang="it">stabile</owl:versionInfo>
    <owl:versionInfo xml:lang="en">stable</owl:versionInfo>
  </rdf:Description>
  <rdf:Description rdf:about="https://w3id.org/italia/onto/HER/studyFirstSubmittedDate">
    <rdf:type rdf:resource="http://www.w3.org/2002/07/owl#DatatypeProperty"/>
    <rdfs:subPropertyOf rdf:resource="https://w3id.org/italia/onto/TI/date"/>
    <rdfs:domain rdf:resource="https://w3id.org/italia/onto/HER/AACTStudy"/>
    <rdfs:range rdf:resource="http://www.w3.org/2001/XMLSchema#date"/>
    <rdfs:comment xml:lang="it">Il suffisso _submitted indica la data in cui il responsabile ha premuto il pulsante di rilascio nel sistema di invio dati di ClinicalTrials.gov, inviando così lo studio per la revisione prima della pubblicazione".</rdfs:comment>
    <rdfs:comment xml:lang="en">The _submitted suffix indicates the date that the responsible party pressed the release button in the ClinicalTrials.gov data submission system, thereby submitting the study for review prior to posting."</rdfs:comment>
    <rdfs:isDefinedBy rdf:resource="https://w3id.org/italia/onto/HER"/>
    <rdfs:label xml:lang="it">data presentazione primo studio</rdfs:label>
    <rdfs:label xml:lang="en">study first submitted date</rdfs:label>
    <owl:versionInfo xml:lang="it">stabile</owl:versionInfo>
    <owl:versionInfo xml:lang="en">stable</owl:versionInfo>
  </rdf:Description>
  <rdf:Description rdf:about="https://w3id.org/italia/onto/HER/MIURStudentsAggregate">
    <rdf:type rdf:resource="http://www.w3.org/2002/07/owl#Class"/>
    <rdfs:subClassOf rdf:resource="https://w3id.org/italia/onto/HER/StatisticalDataAggregation"/>
    <rdfs:comment xml:lang="en">Aggregated data on Italian students filed in the MIUR system, grouped by year and university.</rdfs:comment>
    <rdfs:comment xml:lang="it">Dati aggregati sugli studenti italiani archiviati nel sistema MIUR, raggruppati per anno e per università.</rdfs:comment>
    <rdfs:isDefinedBy rdf:resource="https://w3id.org/italia/onto/HER"/>
    <rdfs:label xml:lang="en">Aggregate of Italian Students</rdfs:label>
    <rdfs:label xml:lang="it">Aggregazione dei studenti italiani</rdfs:label>
    <owl:versionInfo xml:lang="it">stabile</owl:versionInfo>
    <owl:versionInfo xml:lang="en">stable</owl:versionInfo>
  </rdf:Description>
  <rdf:Description rdf:nodeID="n5bb3bff42afb4ca286d2c3fead9507ddb195">
    <rdf:first rdf:resource="https://w3id.org/italia/onto/HER/MIURStudentsByCitizenshipDegreeAggregate"/>
    <rdf:rest rdf:nodeID="n5bb3bff42afb4ca286d2c3fead9507ddb196"/>
  </rdf:Description>
  <rdf:Description rdf:about="https://w3id.org/italia/onto/HER/hasCompletionDate">
    <rdf:type rdf:resource="http://www.w3.org/2002/07/owl#ObjectProperty"/>
    <rdfs:subPropertyOf rdf:resource="https://w3id.org/italia/onto/TI/hasTemporalEntity"/>
    <rdfs:domain rdf:resource="https://w3id.org/italia/onto/HER/AACTStudy"/>
    <rdfs:range rdf:resource="https://w3id.org/italia/onto/TI#TimeInstant"/>
    <rdfs:comment xml:lang="it">La data in cui l'ultimo partecipante a uno studio clinico è stato esaminato o ha ricevuto un intervento/trattamento per raccogliere i dati finali per le misure di esito primario, le misure di esito secondario e gli eventi avversi (cioè l'ultima visita dell'ultimo partecipante). La data "stimata" di completamento dello studio è la data che i ricercatori ritengono essere la data di completamento dello studio.</rdfs:comment>
    <rdfs:comment xml:lang="en">The date on which the last participant in a clinical study was examined or received an intervention/treatment to collect final data for the primary outcome measures, secondary outcome measures, and adverse events (that is, the last participant's last visit). The "estimated" study completion date is the date that the researchers think will be the study completion date.</rdfs:comment>
    <rdfs:isDefinedBy rdf:resource="https://w3id.org/italia/onto/HER"/>
    <rdfs:label xml:lang="it">ha data di completamento</rdfs:label>
    <rdfs:label xml:lang="en">has completion date</rdfs:label>
    <owl:versionInfo xml:lang="it">prova</owl:versionInfo>
    <owl:versionInfo xml:lang="en">testing</owl:versionInfo>
  </rdf:Description>
  <rdf:Description rdf:nodeID="n5bb3bff42afb4ca286d2c3fead9507ddb453">
    <rdf:type rdf:resource="http://www.w3.org/2002/07/owl#Restriction"/>
    <owl:onProperty rdf:resource="https://w3id.org/italia/onto/HER/ecMaxContribution"/>
    <owl:qualifiedCardinality rdf:datatype="http://www.w3.org/2001/XMLSchema#nonNegativeInteger">1</owl:qualifiedCardinality>
    <owl:onDataRange rdf:resource="http://www.w3.org/2001/XMLSchema#decimal"/>
  </rdf:Description>
  <rdf:Description rdf:nodeID="n5bb3bff42afb4ca286d2c3fead9507ddb411">
    <rdf:type rdf:resource="http://www.w3.org/2002/07/owl#Restriction"/>
    <owl:onProperty rdf:resource="https://w3id.org/italia/onto/HER/endingYear"/>
    <owl:maxQualifiedCardinality rdf:datatype="http://www.w3.org/2001/XMLSchema#nonNegativeInteger">1</owl:maxQualifiedCardinality>
    <owl:onDataRange rdf:resource="http://www.w3.org/2001/XMLSchema#gYear"/>
  </rdf:Description>
  <rdf:Description rdf:about="https://w3id.org/italia/onto/HER/hasEurekaMarketArea">
    <rdf:type rdf:resource="http://www.w3.org/2002/07/owl#ObjectProperty"/>
    <rdfs:subPropertyOf rdf:resource="https://w3id.org/italia/onto/l0/hasTopic"/>
    <rdfs:domain rdf:resource="https://w3id.org/italia/onto/HER/EUREKAProject"/>
    <rdfs:range rdf:resource="https://w3id.org/italia/onto/HER/EUREKAMarketArea"/>
    <rdfs:comment xml:lang="it">Questa proprietà collega un progetto EUREKA con la corrispondente area di mercato.</rdfs:comment>
    <rdfs:comment xml:lang="en">This property connects an EUREKA projects with the corresponding market area.</rdfs:comment>
    <rdfs:isDefinedBy rdf:resource="https://w3id.org/italia/onto/HER"/>
    <rdfs:label xml:lang="it">ha area di mercato EUREKA</rdfs:label>
    <rdfs:label xml:lang="en">has EUREKA market area</rdfs:label>
    <owl:versionInfo xml:lang="it">stabile</owl:versionInfo>
    <owl:versionInfo xml:lang="en">stable</owl:versionInfo>
  </rdf:Description>
  <rdf:Description rdf:about="https://w3id.org/italia/onto/HER/hasAACTSponsor">
    <rdf:type rdf:resource="http://www.w3.org/2002/07/owl#ObjectProperty"/>
    <rdfs:domain rdf:resource="https://w3id.org/italia/onto/HER/AACTStudy"/>
    <rdfs:range rdf:resource="https://w3id.org/italia/onto/HER/AACTSponsor"/>
    <rdfs:comment xml:lang="it">L'organizzazione o la persona che avvia lo studio e che ha autorità e controllo sullo studio.</rdfs:comment>
    <rdfs:comment xml:lang="en">The organization or person who initiates the study and who has authority and control over the study.</rdfs:comment>
    <rdfs:isDefinedBy rdf:resource="https://w3id.org/italia/onto/HER"/>
    <rdfs:label xml:lang="it">ha sponsor AACT</rdfs:label>
    <rdfs:label xml:lang="en">has AACT sponsor</rdfs:label>
    <owl:versionInfo xml:lang="it">stabile</owl:versionInfo>
    <owl:versionInfo xml:lang="en">stable</owl:versionInfo>
  </rdf:Description>
  <rdf:Description rdf:nodeID="n5bb3bff42afb4ca286d2c3fead9507ddb400">
    <rdf:type rdf:resource="http://www.w3.org/2002/07/owl#Restriction"/>
    <owl:onProperty rdf:resource="https://w3id.org/italia/onto/HER/hasParticipationCountry"/>
    <owl:allValuesFrom rdf:resource="https://w3id.org/italia/onto/CLV/Country"/>
  </rdf:Description>
  <rdf:Description rdf:about="https://w3id.org/italia/onto/HER/ECTopic">
    <rdf:type rdf:resource="http://www.w3.org/2002/07/owl#Class"/>
    <rdfs:subClassOf rdf:resource="https://w3id.org/italia/onto/HER/ECClassification"/>
    <rdfs:comment xml:lang="en">Calls for proposals are subdivided into topics. A topic defines a specific subject or area for which applicants are invited to submit proposals. The description of a topic comprises its specific scope, the type of action, evaluation criteria and deadline for submission of proposals.</rdfs:comment>
    <rdfs:comment xml:lang="it">Gli inviti a presentare proposte sono suddivisi per argomenti. Un argomento definisce un argomento o un settore specifico per il quale i candidati sono invitati a presentare proposte. La descrizione di un argomento comprende il suo ambito specifico, il tipo di azione, i criteri di valutazione e la scadenza per la presentazione delle proposte.</rdfs:comment>
    <rdfs:isDefinedBy rdf:resource="https://w3id.org/italia/onto/HER"/>
    <rdfs:label xml:lang="it">Argomento di ricerca CE</rdfs:label>
    <rdfs:label xml:lang="en">EC Topic</rdfs:label>
    <owl:versionInfo xml:lang="it">stabile</owl:versionInfo>
    <owl:versionInfo xml:lang="en">stable</owl:versionInfo>
    <ns6:wasDerivedFrom rdf:resource="http://www.w3.org/2004/02/skos/core#Concept"/>
  </rdf:Description>
  <rdf:Description rdf:about="https://w3id.org/italia/onto/HER/proposalsCost">
    <rdf:type rdf:resource="http://www.w3.org/2002/07/owl#DatatypeProperty"/>
    <rdfs:domain rdf:resource="https://w3id.org/italia/onto/HER/CTNPRINInitiative"/>
    <rdfs:range rdf:resource="http://www.w3.org/2001/XMLSchema#decimal"/>
    <rdfs:comment xml:lang="it">Somma dei costi totali indicati dai proponenti nelle proposte presentate</rdfs:comment>
    <rdfs:comment xml:lang="en">Sum of the total costs indicated by the proposers in the submitted proposals</rdfs:comment>
    <rdfs:isDefinedBy rdf:resource="https://w3id.org/italia/onto/HER"/>
    <rdfs:label xml:lang="it">costo delle proposte</rdfs:label>
    <rdfs:label xml:lang="en">proposals cost</rdfs:label>
    <owl:versionInfo xml:lang="it">provvisoria - verificare il codominio</owl:versionInfo>
    <owl:versionInfo xml:lang="en">unstable - check the range</owl:versionInfo>
  </rdf:Description>
  <rdf:Description rdf:about="https://w3id.org/italia/onto/HER/ECActivityType">
    <rdf:type rdf:resource="http://www.w3.org/2002/07/owl#Class"/>
    <rdfs:subClassOf rdf:resource="https://w3id.org/italia/onto/HER/ECClassification"/>
    <rdfs:comment xml:lang="it">Tipologia di attività dell'organizzazione che partecipa a un progetto CE. Le seguenti descrizioni e codici di convenzione sono utilizzati per distinguere tra i diversi tipi di organizzazioni: società private a scopo di lucro (PRC), enti pubblici (esclusi ricerca e istruzione) (PUB), organizzazioni di ricerca (esclusa l'istruzione) (REC), istituti di istruzione secondaria e superiore (HES) e altri enti (OTH).</rdfs:comment>
    <rdfs:comment xml:lang="en">Type of activity performed by the organisation participating in a EC project. The following descriptions and convention codes are used for distinguishing between the different types of organisations according to their nature/activity: private for profit companies (PRC), public bodies (excluding research and education) (PUB), research organisations (excluding education) (REC), secondary and higher education establishments (HES), and other entities (OTH).</rdfs:comment>
    <rdfs:isDefinedBy rdf:resource="https://w3id.org/italia/onto/HER"/>
    <rdfs:label xml:lang="en">EC Activity Type of Organization</rdfs:label>
    <rdfs:label xml:lang="it">Tipologia CE di attivitá dell'organizzazione</rdfs:label>
    <owl:versionInfo xml:lang="it">stabile</owl:versionInfo>
    <owl:versionInfo xml:lang="en">stable</owl:versionInfo>
  </rdf:Description>
  <rdf:Description rdf:about="https://w3id.org/italia/onto/HER/ctnprinInitiativeAdmittedCost">
    <rdf:type rdf:resource="http://www.w3.org/2002/07/owl#DatatypeProperty"/>
    <rdfs:subPropertyOf rdf:resource="https://w3id.org/italia/onto/MU/value"/>
    <rdfs:domain rdf:resource="https://w3id.org/italia/onto/HER/CTNPRINInitiative"/>
    <rdfs:range rdf:resource="http://www.w3.org/2001/XMLSchema#decimal"/>
    <rdfs:comment xml:lang="en">Total admitted costs after evaluation of the costs indicated in the project proposals.  Calculated as the sum of the counterpart variable 'admittedCost' present at lower aggregation level (admittedCost_operations)</rdfs:comment>
    <rdfs:comment xml:lang="it">Totale dei costi ammessi dopo la valutazione dei costi indicati nelle proposte di progetto.  Calcolati come somma dell'omologa variabile "admittedCost" presente a livello di aggregazione inferiore (admittedCost_operations)</rdfs:comment>
    <rdfs:isDefinedBy rdf:resource="https://w3id.org/italia/onto/HER"/>
    <rdfs:label xml:lang="en">admitted cost of CTN/PRIN initiative</rdfs:label>
    <rdfs:label xml:lang="it">costi ammessi per iniziative CTN/PRIN</rdfs:label>
    <owl:versionInfo xml:lang="it">stabile</owl:versionInfo>
    <owl:versionInfo xml:lang="en">stable</owl:versionInfo>
  </rdf:Description>
  <rdf:Description rdf:about="https://w3id.org/italia/onto/HER/outcomesAssessorMasked">
    <rdf:type rdf:resource="http://www.w3.org/2002/07/owl#DatatypeProperty"/>
    <rdf:type rdf:resource="http://www.w3.org/2002/07/owl#FunctionalProperty"/>
    <rdfs:domain rdf:resource="https://w3id.org/italia/onto/HER/AACTDesign"/>
    <rdfs:range rdf:resource="http://www.w3.org/2001/XMLSchema#boolean"/>
    <rdfs:comment xml:lang="it">La persona che valuta gli esiti di interesse delle parti coinvolte nello studio clinico a cui viene impedito di avere conoscenza degli interventi assegnati ai singoli partecipanti.</rdfs:comment>
    <rdfs:comment xml:lang="en">The individual who evaluates the outcome(s) of interest is is the party or parties involved in the clinical trial who are prevented from having knowledge of the interventions assigned to individual participants.</rdfs:comment>
    <rdfs:isDefinedBy rdf:resource="https://w3id.org/italia/onto/HER"/>
    <rdfs:label xml:lang="en">outcomes assessor masked</rdfs:label>
    <rdfs:label xml:lang="it">risultato esaminatore mascherato</rdfs:label>
    <owl:versionInfo xml:lang="it">stabile</owl:versionInfo>
    <owl:versionInfo xml:lang="en">stable</owl:versionInfo>
  </rdf:Description>
  <rdf:Description rdf:about="https://w3id.org/italia/onto/HER/USTATStaffByGender">
    <rdf:type rdf:resource="http://www.w3.org/2002/07/owl#Class"/>
    <rdfs:subClassOf rdf:resource="https://w3id.org/italia/onto/HER/StatisticalDataAggregation"/>
    <rdfs:subClassOf rdf:nodeID="n5bb3bff42afb4ca286d2c3fead9507ddb539"/>
    <rdfs:subClassOf rdf:nodeID="n5bb3bff42afb4ca286d2c3fead9507ddb540"/>
    <rdfs:comment xml:lang="en">Data on the careers of teaching and research staff from a gender perspective. The data concern full professors, associate professors, researchers and research grant holders and are disaggregated by gender, age group, university, geographical area, field of research and development and grade. Data are available as of 2012. Whenever possible, the descriptions have been derived from the Record Sheet for the time series on university staff provided by USTAT - Open data.

Data at the 31/12 of the reference year.</rdfs:comment>
    <rdfs:comment xml:lang="it">Dati sulle carriere del personale docente e ricercatore in un'ottica di genere. I dati riguardano professori ordinari, professori associati, ricercatori e titolari di assegni di ricerca e sono disaggregati per genere, classe di età, ateneo, area geografica, field of research and development e grade. I dati sono disponibili a partire dal 2012. Quando possibile, le descrizioni sono state derivate dal Tracciato record per la serie storica sul personale universitario fornito dal USTAT - Open data.

Dati al 31/12 dell'anno di riferimento.</rdfs:comment>
    <rdfs:isDefinedBy rdf:resource="https://w3id.org/italia/onto/HER"/>
    <rdfs:label xml:lang="it">Aggrazione per genere dello Staff riportata da USTAT</rdfs:label>
    <rdfs:label xml:lang="en">USTAT Reported Aggregate of Staff By Sex</rdfs:label>
    <owl:versionInfo xml:lang="it">stabile</owl:versionInfo>
    <owl:versionInfo xml:lang="en">stable</owl:versionInfo>
  </rdf:Description>
  <rdf:Description rdf:about="https://w3id.org/italia/data/contact-point/onto-agid">
    <rdf:type rdf:resource="http://www.w3.org/2002/07/owl#NamedIndividual"/>
    <rdf:type rdf:resource="http://dati.gov.it/onto/dcatapit#Organization"/>
    <rdf:type rdf:resource="http://www.w3.org/2006/vcard/ns#Kind"/>
    <rdf:type rdf:resource="http://www.w3.org/2006/vcard/ns#Organization"/>
    <ns7:fn>banche dati e open data</ns7:fn>
    <ns7:hasEmail rdf:resource="mailto:info@dati.gov.it"/>
  </rdf:Description>
  <rdf:Description rdf:about="https://w3id.org/italia/onto/HER/ECFrameworkProgramme">
    <rdf:type rdf:resource="http://www.w3.org/2002/07/owl#Class"/>
    <rdfs:subClassOf rdf:resource="https://w3id.org/italia/onto/HER/ECClassification"/>
    <rdfs:comment xml:lang="it">I framework program, o in forma abbreviata dal FP1 a FP7 - "FP8" è stato chiamato "Horizon 2020" - sono programmi di finanziamento creati dall'Unione Europea e dalla Commissione Europea per sostenere e promuovere la ricerca nello Spazio Europeo della Ricerca (ERA).</rdfs:comment>
    <rdfs:comment xml:lang="en">The Framework Programmes, or abbreviated FP1 to FP7 with "FP8" being named "Horizon 2020", are funding programmes created by the European Union/European Commission to support and foster research in the European Research Area (ERA).</rdfs:comment>
    <rdfs:isDefinedBy rdf:resource="https://w3id.org/italia/onto/HER"/>
    <rdfs:label xml:lang="en">EC Framework Program</rdfs:label>
    <rdfs:label xml:lang="it">Programma quadro CE</rdfs:label>
    <owl:versionInfo xml:lang="it">stabile</owl:versionInfo>
    <owl:versionInfo xml:lang="en">stable</owl:versionInfo>
    <ns6:wasDerivedFrom rdf:resource="http://www.w3.org/2004/02/skos/core#Concept"/>
  </rdf:Description>
  <rdf:Description rdf:nodeID="n5bb3bff42afb4ca286d2c3fead9507ddb340">
    <rdf:first rdf:resource="https://w3id.org/italia/onto/HER/USTATPostgraduateAggregateOfEnrolled"/>
    <rdf:rest rdf:nodeID="n5bb3bff42afb4ca286d2c3fead9507ddb341"/>
  </rdf:Description>
  <rdf:Description rdf:about="https://w3id.org/italia/onto/HER/hasPatentPriorityDetail">
    <rdf:type rdf:resource="http://www.w3.org/2002/07/owl#ObjectProperty"/>
    <rdfs:domain rdf:resource="https://w3id.org/italia/onto/HER/Patent"/>
    <rdfs:range rdf:resource="https://w3id.org/italia/onto/HER/PatentPriorityDetail"/>
    <rdfs:isDefinedBy rdf:resource="https://w3id.org/italia/onto/HER"/>
    <rdfs:label xml:lang="it">ha dettagli prioritari pubblicazione brevetto</rdfs:label>
    <rdfs:label xml:lang="en">has patent priority details</rdfs:label>
    <owl:versionInfo xml:lang="it">stabile</owl:versionInfo>
    <owl:versionInfo xml:lang="en">stable</owl:versionInfo>
  </rdf:Description>
  <rdf:Description rdf:about="https://w3id.org/italia/onto/HER/InternationalPatentClassification">
    <rdf:type rdf:resource="http://www.w3.org/2002/07/owl#Class"/>
    <rdfs:subClassOf rdf:resource="https://w3id.org/italia/onto/l0/Topic"/>
    <rdfs:comment xml:lang="it">La classificazione internazionale dei brevetti (IPC), istituita dall'accordo di Strasburgo del 1971, prevede un sistema gerarchico di simboli indipendenti dal linguaggio per la classificazione dei brevetti e dei modelli di utilità in base alle diverse aree tecnologiche a cui si riferiscono.</rdfs:comment>
    <rdfs:comment xml:lang="en">The International Patent Classification (IPC), established by the Strasbourg Agreement 1971, provides for a hierarchical system of language independent symbols for the classification of patents and utility models according to the different areas of technology to which they pertain.</rdfs:comment>
    <rdfs:isDefinedBy rdf:resource="https://w3id.org/italia/onto/HER"/>
    <rdfs:label xml:lang="it">Classificazione internazionale dei brevetti</rdfs:label>
    <rdfs:label xml:lang="en">International Patent Classification</rdfs:label>
    <owl:versionInfo xml:lang="it">stabile</owl:versionInfo>
    <owl:versionInfo xml:lang="en">stable</owl:versionInfo>
    <ns6:wasDerivedFrom rdf:resource="http://www.w3.org/2004/02/skos/core#ConceptScheme"/>
  </rdf:Description>
  <rdf:Description rdf:about="https://w3id.org/italia/onto/HER/totalDoctorate">
    <rdf:type rdf:resource="http://www.w3.org/2002/07/owl#DatatypeProperty"/>
    <rdfs:subPropertyOf rdf:resource="https://w3id.org/italia/onto/MU/value"/>
    <rdfs:domain rdf:nodeID="n5bb3bff42afb4ca286d2c3fead9507ddb314"/>
    <rdfs:range rdf:resource="http://www.w3.org/2000/01/rdf-schema#Literal"/>
    <rdfs:comment xml:lang="en">Total with respect to students enrolled in PhD courses.</rdfs:comment>
    <rdfs:comment xml:lang="it">Totale rispetto agli iscritti a corsi di dottorato di ricerca.</rdfs:comment>
    <rdfs:isDefinedBy rdf:resource="https://w3id.org/italia/onto/HER"/>
    <rdfs:label xml:lang="en">total doctorate</rdfs:label>
    <rdfs:label xml:lang="it">totali dottorati</rdfs:label>
    <owl:versionInfo xml:lang="it">stabile</owl:versionInfo>
    <owl:versionInfo xml:lang="en">stable</owl:versionInfo>
  </rdf:Description>
  <rdf:Description rdf:about="https://w3id.org/italia/onto/HER/hasISCEDFClassification">
    <rdf:type rdf:resource="http://www.w3.org/2002/07/owl#ObjectProperty"/>
    <rdfs:subPropertyOf rdf:resource="https://w3id.org/italia/onto/l0/hasTopic"/>
    <rdfs:domain rdf:nodeID="n5bb3bff42afb4ca286d2c3fead9507ddb67"/>
    <rdfs:range rdf:resource="https://w3id.org/italia/onto/HER/ISCEDFClassification"/>
    <rdfs:comment xml:lang="it">Questa proprietà si collega alla classificazione internazionale standard dell'istruzione dell'UNESCO (ISCED).</rdfs:comment>
    <rdfs:comment xml:lang="en">This property links to the UNESCO's International Standard Classification of Education (ISCED).</rdfs:comment>
    <rdfs:isDefinedBy rdf:resource="https://w3id.org/italia/onto/HER"/>
    <rdfs:label xml:lang="it">ha classificazione ISCED-F</rdfs:label>
    <rdfs:label xml:lang="en">has ISCED-F classification</rdfs:label>
    <owl:versionInfo xml:lang="it">stabile</owl:versionInfo>
    <owl:versionInfo xml:lang="en">stable</owl:versionInfo>
  </rdf:Description>
  <rdf:Description rdf:about="https://w3id.org/italia/onto/HER/ECSubjectArea">
    <rdf:type rdf:resource="http://www.w3.org/2002/07/owl#Class"/>
    <rdfs:subClassOf rdf:resource="https://w3id.org/italia/onto/HER/ECClassification"/>
    <rdfs:comment xml:lang="it">Categorizzazione tematica utilizzata nel 7° Programma Quadro. Non disponibile in H2020.</rdfs:comment>
    <rdfs:comment xml:lang="en">Thematic categorisation used in the 7th Framework Programme. Not available in H2020.</rdfs:comment>
    <rdfs:isDefinedBy rdf:resource="https://w3id.org/italia/onto/HER"/>
    <rdfs:label xml:lang="it">Area tematica CE</rdfs:label>
    <rdfs:label xml:lang="en">EC Subject Area</rdfs:label>
    <owl:versionInfo xml:lang="it">stabile</owl:versionInfo>
    <owl:versionInfo xml:lang="en">stable</owl:versionInfo>
    <ns6:wasDerivedFrom rdf:resource="http://www.w3.org/2004/02/skos/core#Concept"/>
  </rdf:Description>
  <rdf:Description rdf:about="https://w3id.org/italia/onto/HER/expireDate">
    <rdf:type rdf:resource="http://www.w3.org/2002/07/owl#DatatypeProperty"/>
    <rdfs:subPropertyOf rdf:resource="https://w3id.org/italia/onto/TI/date"/>
    <rdfs:domain rdf:resource="https://w3id.org/italia/onto/HER/CTNPRINInitiative"/>
    <rdfs:range rdf:resource="http://www.w3.org/2001/XMLSchema#date"/>
    <rdfs:comment xml:lang="en">Final deadline for submission of project proposals for CTN/PRIN initiative</rdfs:comment>
    <rdfs:comment xml:lang="it">Ultima data di scadenza utile per la presentazione di proposte di progetto per l'iniziativa di tipo CTN/PRIN in esame</rdfs:comment>
    <rdfs:isDefinedBy rdf:resource="https://w3id.org/italia/onto/HER"/>
    <rdfs:label xml:lang="it">data scadenza</rdfs:label>
    <rdfs:label xml:lang="en">expiration date</rdfs:label>
    <owl:versionInfo xml:lang="it">stabile</owl:versionInfo>
    <owl:versionInfo xml:lang="en">stable</owl:versionInfo>
  </rdf:Description>
  <rdf:Description rdf:about="https://w3id.org/italia/onto/HER/AACTStudy">
    <rdf:type rdf:resource="http://www.w3.org/2002/07/owl#Class"/>
    <rdfs:subClassOf rdf:resource="https://w3id.org/italia/onto/l0/Activity"/>
    <rdfs:subClassOf rdf:nodeID="n5bb3bff42afb4ca286d2c3fead9507ddb381"/>
    <rdfs:subClassOf rdf:nodeID="n5bb3bff42afb4ca286d2c3fead9507ddb382"/>
    <rdfs:subClassOf rdf:nodeID="n5bb3bff42afb4ca286d2c3fead9507ddb383"/>
    <rdfs:subClassOf rdf:nodeID="n5bb3bff42afb4ca286d2c3fead9507ddb384"/>
    <rdfs:subClassOf rdf:nodeID="n5bb3bff42afb4ca286d2c3fead9507ddb385"/>
    <rdfs:subClassOf rdf:nodeID="n5bb3bff42afb4ca286d2c3fead9507ddb386"/>
    <rdfs:subClassOf rdf:nodeID="n5bb3bff42afb4ca286d2c3fead9507ddb387"/>
    <rdfs:subClassOf rdf:nodeID="n5bb3bff42afb4ca286d2c3fead9507ddb388"/>
    <rdfs:subClassOf rdf:nodeID="n5bb3bff42afb4ca286d2c3fead9507ddb389"/>
    <rdfs:subClassOf rdf:nodeID="n5bb3bff42afb4ca286d2c3fead9507ddb390"/>
    <rdfs:subClassOf rdf:nodeID="n5bb3bff42afb4ca286d2c3fead9507ddb391"/>
    <rdfs:subClassOf rdf:nodeID="n5bb3bff42afb4ca286d2c3fead9507ddb392"/>
    <rdfs:subClassOf rdf:nodeID="n5bb3bff42afb4ca286d2c3fead9507ddb393"/>
    <rdfs:subClassOf rdf:nodeID="n5bb3bff42afb4ca286d2c3fead9507ddb394"/>
    <rdfs:subClassOf rdf:nodeID="n5bb3bff42afb4ca286d2c3fead9507ddb395"/>
    <rdfs:subClassOf rdf:nodeID="n5bb3bff42afb4ca286d2c3fead9507ddb396"/>
    <rdfs:comment xml:lang="en">Clinical study</rdfs:comment>
    <rdfs:comment xml:lang="it">Studio clinico</rdfs:comment>
    <rdfs:isDefinedBy rdf:resource="https://w3id.org/italia/onto/HER"/>
    <rdfs:label xml:lang="it">Studio</rdfs:label>
    <rdfs:label xml:lang="en">Study</rdfs:label>
    <owl:versionInfo xml:lang="it">stabile</owl:versionInfo>
    <owl:versionInfo xml:lang="en">stable</owl:versionInfo>
  </rdf:Description>
  <rdf:Description rdf:about="https://w3id.org/italia/onto/HER/HES">
    <rdf:type rdf:resource="http://www.w3.org/2002/07/owl#NamedIndividual"/>
    <rdf:type rdf:resource="https://w3id.org/italia/onto/HER/ECActivityType"/>
    <rdfs:isDefinedBy rdf:resource="https://w3id.org/italia/onto/HER"/>
    <rdfs:label xml:lang="en">Higher or Secondary Education Establishments</rdfs:label>
    <owl:versionInfo xml:lang="it">stabile</owl:versionInfo>
    <owl:versionInfo xml:lang="en">stable</owl:versionInfo>
  </rdf:Description>
  <rdf:Description rdf:about="https://w3id.org/italia/onto/HER/AcademicDegree">
    <rdf:type rdf:resource="http://www.w3.org/2002/07/owl#Class"/>
    <rdfs:subClassOf rdf:resource="https://w3id.org/italia/onto/l0/Object"/>
    <rdfs:subClassOf rdf:nodeID="n5bb3bff42afb4ca286d2c3fead9507ddb397"/>
    <rdfs:comment xml:lang="it">Il principale titolo accademico post-secondario in Italia.</rdfs:comment>
    <rdfs:comment xml:lang="en">The main post-secondary academic degree in Italy.</rdfs:comment>
    <rdfs:isDefinedBy rdf:resource="https://w3id.org/italia/onto/HER"/>
    <rdfs:label xml:lang="en">Academic Degree</rdfs:label>
    <rdfs:label xml:lang="it">Laurea</rdfs:label>
    <owl:versionInfo xml:lang="it">stabile</owl:versionInfo>
    <owl:versionInfo xml:lang="en">stable</owl:versionInfo>
  </rdf:Description>
  <rdf:Description rdf:nodeID="n5bb3bff42afb4ca286d2c3fead9507ddb365">
    <rdf:first rdf:resource="https://w3id.org/italia/onto/HER/ECParticipant"/>
    <rdf:rest rdf:nodeID="n5bb3bff42afb4ca286d2c3fead9507ddb366"/>
  </rdf:Description>
  <rdf:Description rdf:nodeID="n5bb3bff42afb4ca286d2c3fead9507ddb336">
    <rdf:type rdf:resource="http://www.w3.org/2002/07/owl#Class"/>
    <owl:unionOf rdf:nodeID="n5bb3bff42afb4ca286d2c3fead9507ddb337"/>
  </rdf:Description>
  <rdf:Description rdf:about="https://w3id.org/italia/onto/HER/MIURStudentsByProvinceOfResidenceDegreeDegreeClassAggregate">
    <rdf:type rdf:resource="http://www.w3.org/2002/07/owl#Class"/>
    <rdfs:subClassOf rdf:resource="https://w3id.org/italia/onto/HER/StatisticalDataAggregation"/>
    <rdfs:subClassOf rdf:nodeID="n5bb3bff42afb4ca286d2c3fead9507ddb495"/>
    <rdfs:comment xml:lang="en">Aggregated data on Italian students filed in the MIUR system, grouped by year, university, Italian province of residence, degree and degree class.</rdfs:comment>
    <rdfs:comment xml:lang="it">Dati aggregati sugli studenti italiani archiviati nel sistema MIUR, raggruppati per anno, università, provincia di residenza italiana, laurea e classe di laurea.</rdfs:comment>
    <rdfs:isDefinedBy rdf:resource="https://w3id.org/italia/onto/HER"/>
    <rdfs:label xml:lang="en">Aggregate of Italian Students By Province of Residence, Degree and Degree Class</rdfs:label>
    <rdfs:label xml:lang="it">Aggregazione dei studenti italiani per provincia di residenza, laurea e classe di laurea</rdfs:label>
    <owl:versionInfo xml:lang="it">stabile</owl:versionInfo>
    <owl:versionInfo xml:lang="en">stable</owl:versionInfo>
  </rdf:Description>
  <rdf:Description rdf:about="https://w3id.org/italia/onto/HER/studiesFDARegulatedDrug">
    <rdf:type rdf:resource="http://www.w3.org/2002/07/owl#DatatypeProperty"/>
    <rdf:type rdf:resource="http://www.w3.org/2002/07/owl#FunctionalProperty"/>
    <rdfs:domain rdf:resource="https://w3id.org/italia/onto/HER/AACTStudy"/>
    <rdfs:range rdf:resource="http://www.w3.org/2001/XMLSchema#boolean"/>
    <rdfs:comment xml:lang="en">Indication that a clinical study is studying a drug product (including a biological product) subject to section 505 of the Federal Food, Drug, and Cosmetic Act or to section 351 of the Public Health Service Act. Select true/false</rdfs:comment>
    <rdfs:comment xml:lang="it">Indicazione che uno studio clinico sta studiando un prodotto farmaceutico (incluso un prodotto biologico) soggetto alla sezione 505 del Federal Food, Drug, and Cosmetic Act o alla sezione 351 del Public Health Service Act. Selezionare vero/falso.</rdfs:comment>
    <rdfs:isDefinedBy rdf:resource="https://w3id.org/italia/onto/HER"/>
    <rdfs:label xml:lang="it">studia  farmaco regolamentato dalla FDA</rdfs:label>
    <rdfs:label xml:lang="en">studies FDA regulated drug?</rdfs:label>
    <owl:versionInfo xml:lang="it">stabile</owl:versionInfo>
    <owl:versionInfo xml:lang="en">stable</owl:versionInfo>
  </rdf:Description>
  <rdf:Description rdf:about="https://w3id.org/italia/onto/HER/hasOperationalSpinoffAddress">
    <rdf:type rdf:resource="http://www.w3.org/2002/07/owl#ObjectProperty"/>
    <rdfs:subPropertyOf rdf:resource="https://w3id.org/italia/onto/CLV/hasAddress"/>
    <rdfs:domain rdf:resource="https://w3id.org/italia/onto/HER/Spinoff"/>
    <rdfs:range rdf:resource="https://w3id.org/italia/onto/CLV/Address"/>
    <rdfs:comment xml:lang="it">Collega lo spin-off alla sua sede operativa.</rdfs:comment>
    <rdfs:comment xml:lang="en">It connects the spin-off to its operational headquarters.</rdfs:comment>
    <rdfs:isDefinedBy rdf:resource="https://w3id.org/italia/onto/HER"/>
    <rdfs:label xml:lang="it">ha indirizzo operativo spinoff</rdfs:label>
    <rdfs:label xml:lang="en">has operational spinoff address</rdfs:label>
    <owl:versionInfo xml:lang="it">stabile</owl:versionInfo>
    <owl:versionInfo xml:lang="en">stable</owl:versionInfo>
  </rdf:Description>
  <rdf:Description rdf:about="https://w3id.org/italia/onto/HER/EUREKACluster">
    <rdf:type rdf:resource="http://www.w3.org/2002/07/owl#Class"/>
    <rdfs:subClassOf rdf:resource="https://w3id.org/italia/onto/l0/Concept"/>
    <rdfs:subClassOf rdf:nodeID="n5bb3bff42afb4ca286d2c3fead9507ddb460"/>
    <rdfs:comment xml:lang="en">EUREKA Clusters are strategic initiatives proposed and led by industry, developing generic technologies of key importance for European competitiveness</rdfs:comment>
    <rdfs:comment xml:lang="it">I Cluster EUREKA sono iniziative strategiche proposte e guidate dall'industria, che sviluppano tecnologie generiche di importanza fondamentale per la competitività europea</rdfs:comment>
    <rdfs:isDefinedBy rdf:resource="https://w3id.org/italia/onto/HER"/>
    <rdfs:label xml:lang="en">EUREKA Cluster</rdfs:label>
    <rdfs:label xml:lang="it">Gruppo EUREKA</rdfs:label>
    <owl:versionInfo xml:lang="it">stabile</owl:versionInfo>
    <owl:versionInfo xml:lang="en">stable</owl:versionInfo>
    <ns6:wasDerivedFrom rdf:resource="http://www.w3.org/2004/02/skos/core#Concept"/>
  </rdf:Description>
  <rdf:Description rdf:about="https://w3id.org/italia/onto/HER/lastKnownStatus">
    <rdf:type rdf:resource="http://www.w3.org/2002/07/owl#DatatypeProperty"/>
    <rdfs:domain rdf:resource="https://w3id.org/italia/onto/HER/AACTStudy"/>
    <rdfs:range rdf:nodeID="n5bb3bff42afb4ca286d2c3fead9507ddb178"/>
    <rdfs:comment xml:lang="en">Last registered study enrollment status. Enrollment status are: Not yet recruiting: The study has not started recruiting participants.
Recruiting: The study is currently recruiting participants.
Enrolling by invitation: The study is selecting its participants from a population, or group of people, decided on by the researchers in advance. These studies are not open to everyone who meets the eligibility criteria but only to people in that particular population, who are specifically invited to participate.
Active, not recruiting: The study is ongoing, and participants are receiving an intervention or being examined, but potential participants are not currently being recruited or enrolled.
Suspended: The study has stopped early but may start again.
Terminated: The study has stopped early and will not start again. Participants are no longer being examined or treated.
Completed: The study has ended normally, and participants are no longer being examined or treated (that is, the last participant's last visit has occurred).
Withdrawn: The study stopped early, before enrolling its first participant.
Unknown: A study on ClinicalTrials.gov whose last known status was recruiting; not yet recruiting; or active, not recruiting but that has passed its completion date, and the status has not been last verified within the past 2 years.</rdfs:comment>
    <rdfs:comment xml:lang="it">Ultimo stato di iscrizione allo studio registrato. Gli stati di iscrizione sono: Non ancora in fase di reclutamento: Lo studio non ha iniziato a reclutare partecipanti.
Reclutamento: Lo studio sta attualmente reclutando i partecipanti.
Iscrizione su invito: Lo studio sta selezionando i partecipanti da una popolazione, o gruppo di persone, decisa in anticipo dai ricercatori. Questi studi non sono aperti a tutti coloro che soddisfano i criteri di ammissibilità, ma solo alle persone di quella particolare popolazione, che sono specificamente invitate a partecipare.
Attivi, non reclutatori: Lo studio è in corso e i partecipanti ricevono un intervento o vengono esaminati, ma i potenziali partecipanti non sono attualmente reclutati o iscritti.
Sospeso: Lo studio è stato interrotto in anticipo ma potrebbe ricominciare.
Terminato: Lo studio si è interrotto anticipatamente e non inizierà di nuovo. I partecipanti non vengono più esaminati o trattati.
Completato: Lo studio è terminato normalmente e i partecipanti non vengono più esaminati o trattati (cioè si è verificata l'ultima visita dell'ultimo partecipante).
Ritirato: Lo studio si è interrotto anticipatamente, prima di iscrivere il primo partecipante.
Sconosciuto: Uno studio su ClinicalTrials.gov il cui ultimo stato conosciuto è stato il reclutamento; non ancora reclutamento; o attivo, non reclutamento ma che ha superato la data di completamento, e lo stato non è stato verificato per l'ultima volta negli ultimi 2 anni.</rdfs:comment>
    <rdfs:isDefinedBy rdf:resource="https://w3id.org/italia/onto/HER"/>
    <rdfs:label xml:lang="it">Ultimo stato conosciuto</rdfs:label>
    <rdfs:label xml:lang="en">last known status</rdfs:label>
    <owl:versionInfo xml:lang="it">stabile</owl:versionInfo>
    <owl:versionInfo xml:lang="en">stable</owl:versionInfo>
  </rdf:Description>
  <rdf:Description rdf:about="https://w3id.org/italia/onto/HER/MIURStudentsByProvinceOfResidenceAggregate">
    <rdf:type rdf:resource="http://www.w3.org/2002/07/owl#Class"/>
    <rdfs:subClassOf rdf:resource="https://w3id.org/italia/onto/HER/StatisticalDataAggregation"/>
    <rdfs:subClassOf rdf:nodeID="n5bb3bff42afb4ca286d2c3fead9507ddb494"/>
    <rdfs:comment xml:lang="en">Aggregated data on Italian students filed in the MIUR system, grouped by year, university and Italian province of residence.</rdfs:comment>
    <rdfs:comment xml:lang="it">Dati aggregati sugli studenti italiani archiviati nel sistema MIUR, raggruppati per anno, università e provincia di residenza italiana.</rdfs:comment>
    <rdfs:isDefinedBy rdf:resource="https://w3id.org/italia/onto/HER"/>
    <rdfs:label xml:lang="en">Aggregate of Italian Students By Province of Residence</rdfs:label>
    <rdfs:label xml:lang="it">Aggregazione dei studenti italiani per provincia di residenza</rdfs:label>
    <owl:versionInfo xml:lang="it">stabile</owl:versionInfo>
    <owl:versionInfo xml:lang="en">stable</owl:versionInfo>
  </rdf:Description>
  <rdf:Description rdf:about="https://w3id.org/italia/onto/HER/allocation">
    <rdf:type rdf:resource="http://www.w3.org/2002/07/owl#DatatypeProperty"/>
    <rdfs:domain rdf:resource="https://w3id.org/italia/onto/HER/AACTDesign"/>
    <rdfs:range rdf:nodeID="n5bb3bff42afb4ca286d2c3fead9507ddb132"/>
    <rdfs:comment xml:lang="en">A method used to assign participants to an arm of a clinical study. The types of allocation are:
Random sample. For a single-arm trial
Randomized: Participants are assigned to intervention groups by chance
Nonrandomized: Participants are expressly assigned to intervention groups through a non-random method, such as physician choice</rdfs:comment>
    <rdfs:comment xml:lang="it">Un metodo utilizzato per assegnare i partecipanti ad una branca di uno studio clinico. I tipi di assegnazione sono:
Campione casuale. Per uno studio su una singola branca
Casuale: I partecipanti sono assegnati a gruppi d'intervento per caso
Non casuale: I partecipanti sono espressamente assegnati ai gruppi di intervento attraverso un metodo non casuale, come la scelta del medico</rdfs:comment>
    <rdfs:isDefinedBy rdf:resource="https://w3id.org/italia/onto/HER"/>
    <rdfs:label xml:lang="en">allocation</rdfs:label>
    <rdfs:label xml:lang="it">assegnazione</rdfs:label>
    <owl:versionInfo xml:lang="it">stabile</owl:versionInfo>
    <owl:versionInfo xml:lang="en">stable</owl:versionInfo>
  </rdf:Description>
  <rdf:Description rdf:about="https://w3id.org/italia/onto/HER/PatentPublicationDetail">
    <rdf:type rdf:resource="http://www.w3.org/2002/07/owl#Class"/>
    <rdfs:subClassOf rdf:resource="https://w3id.org/italia/onto/l0/Description"/>
    <rdfs:subClassOf rdf:nodeID="n5bb3bff42afb4ca286d2c3fead9507ddb505"/>
    <rdfs:subClassOf rdf:nodeID="n5bb3bff42afb4ca286d2c3fead9507ddb506"/>
    <rdfs:subClassOf rdf:nodeID="n5bb3bff42afb4ca286d2c3fead9507ddb507"/>
    <rdfs:comment xml:lang="en">Details of the patent publication (e.g. publication number, year, etc.)</rdfs:comment>
    <rdfs:comment xml:lang="it">Dettagli della pubblicazione del brevetto (ad es. Numero di pubblicazione, anno, ecc.)</rdfs:comment>
    <rdfs:isDefinedBy rdf:resource="https://w3id.org/italia/onto/HER"/>
    <rdfs:label xml:lang="it">Dettagli della pubblicazione del brevetto</rdfs:label>
    <rdfs:label xml:lang="en">Patent Publication Details</rdfs:label>
    <owl:versionInfo xml:lang="it">stabile</owl:versionInfo>
    <owl:versionInfo xml:lang="en">stable</owl:versionInfo>
  </rdf:Description>
  <rdf:Description rdf:nodeID="n5bb3bff42afb4ca286d2c3fead9507ddb372">
    <rdf:type rdf:resource="http://www.w3.org/2002/07/owl#Restriction"/>
    <owl:onProperty rdf:resource="https://w3id.org/italia/onto/HER/aactCriterion"/>
    <owl:someValuesFrom rdf:resource="http://www.w3.org/2000/01/rdf-schema#Literal"/>
  </rdf:Description>
  <rdf:Description rdf:about="https://w3id.org/italia/onto/HER/hasInstrument">
    <rdf:type rdf:resource="http://www.w3.org/2002/07/owl#ObjectProperty"/>
    <rdfs:domain rdf:resource="https://w3id.org/italia/onto/HER/CHAFEAProject"/>
    <rdfs:range rdf:resource="https://w3id.org/italia/onto/HER/CHAFEAInstrument"/>
    <rdfs:comment xml:lang="it">Questa proprietà collega un progetto CHAFEA finanziato con lo strumento corrispondente.</rdfs:comment>
    <rdfs:comment xml:lang="en">This property connects a funded CHAFEA project with the corresponding instrument.</rdfs:comment>
    <rdfs:isDefinedBy rdf:resource="https://w3id.org/italia/onto/HER"/>
    <rdfs:label xml:lang="it">ha strumento CHAFEA</rdfs:label>
    <rdfs:label xml:lang="en">has CHAFEA instrument</rdfs:label>
    <owl:versionInfo xml:lang="it">stabile</owl:versionInfo>
    <owl:versionInfo xml:lang="en">stable</owl:versionInfo>
  </rdf:Description>
  <rdf:Description rdf:about="https://w3id.org/italia/data/distribution/HERAPIT-RDF-TURTLE">
    <rdf:type rdf:resource="http://www.w3.org/2002/07/owl#NamedIndividual"/>
    <rdf:type rdf:resource="https://w3id.org/italia/onto/ADMS/SemanticAssetDistribution"/>
    <ns2:description xml:lang="it">Questa è la distribuzione RDF/Turtle dell'ontologia della Ricerca Pubblica</ns2:description>
    <ns2:description xml:lang="en">This is the distribution in RDF/turtle of the Public Research ontology</ns2:description>
    <ns2:format rdf:resource="http://publications.europa.eu/resource/authority/file-type/RDF_TURTLE"/>
    <ns2:license rdf:resource="https://w3id.org/italia/controlled-vocabulary/licences/A21_CCBY40"/>
    <ns2:title xml:lang="it">Distribuzione RDF/Turtle ontologia PublicReseach-AP_IT</ns2:title>
    <ns2:title xml:lang="en">RDF/Turtle distribution of PublicReseach-AP_IT Ontology</ns2:title>
    <ns3:accessURL rdf:resource="https://raw.githubusercontent.com/italia/daf-ontologie-vocabolari-controllati/master/Ontologie/HER/latest"/>
    <ns3:downloadURL rdf:resource="https://raw.githubusercontent.com/italia/daf-ontologie-vocabolari-controllati/master/Ontologie/HER/latest/HER-AP_IT.ttl"/>
  </rdf:Description>
  <rdf:Description rdf:about="https://w3id.org/italia/onto/HER/hasAACTStudy">
    <rdf:type rdf:resource="http://www.w3.org/2002/07/owl#ObjectProperty"/>
    <rdfs:domain rdf:nodeID="n5bb3bff42afb4ca286d2c3fead9507ddb4"/>
    <rdfs:range rdf:resource="https://w3id.org/italia/onto/HER/AACTStudy"/>
    <rdfs:comment xml:lang="it">Questa proprietà si collega allo studio corrispondente.</rdfs:comment>
    <rdfs:comment xml:lang="en">This property links to the corresponding study.</rdfs:comment>
    <rdfs:isDefinedBy rdf:resource="https://w3id.org/italia/onto/HER"/>
    <rdfs:label xml:lang="it">ha studio AACT</rdfs:label>
    <rdfs:label xml:lang="en">has AACT study</rdfs:label>
    <owl:versionInfo xml:lang="it">stabile</owl:versionInfo>
    <owl:versionInfo xml:lang="en">stable</owl:versionInfo>
  </rdf:Description>
  <rdf:Description rdf:about="https://w3id.org/italia/onto/HER/totalFemaleDoctorateGraduated">
    <rdf:type rdf:resource="http://www.w3.org/2002/07/owl#DatatypeProperty"/>
    <rdfs:subPropertyOf rdf:resource="https://w3id.org/italia/onto/MU/value"/>
    <rdfs:domain rdf:resource="https://w3id.org/italia/onto/HER/USTATStudentsBySexAggregate"/>
    <rdfs:range rdf:resource="http://www.w3.org/2001/XMLSchema#decimal"/>
    <rdfs:comment xml:lang="en">Information on women PhDs, disaggregated by gender, university, geographical area, course type and field of education and training (ISCED-F 2013). Data available as of calendar year 2012.</rdfs:comment>
    <rdfs:comment xml:lang="it">Informazioni sui dottori di ricerca di genere femminile, disaggregate per genere, ateneo, area geografica, tipo di corso e field of education and training (ISCED-F 2013). Dati disponibili a partire dall’anno solare 2012.</rdfs:comment>
    <rdfs:isDefinedBy rdf:resource="https://w3id.org/italia/onto/HER"/>
    <rdfs:label xml:lang="en">total female doctorate graduated</rdfs:label>
    <rdfs:label xml:lang="it">totale di laurati ad un dottorato di genere famminile</rdfs:label>
    <owl:versionInfo xml:lang="it">stabile</owl:versionInfo>
    <owl:versionInfo xml:lang="en">stable</owl:versionInfo>
  </rdf:Description>
  <rdf:Description rdf:about="https://w3id.org/italia/data/project/toscana-open-research">
    <rdf:type rdf:resource="http://www.w3.org/2002/07/owl#NamedIndividual"/>
    <rdf:type rdf:resource="https://w3id.org/italia/onto/ADMS/Project"/>
    <ns4:name xml:lang="it">Toscana Open Research</ns4:name>
    <rdfs:label xml:lang="it">Toscana Open Research</rdfs:label>
  </rdf:Description>
  <rdf:Description rdf:about="https://w3id.org/italia/onto/HER/picNumber">
    <rdf:type rdf:resource="http://www.w3.org/2002/07/owl#DatatypeProperty"/>
    <rdfs:subPropertyOf rdf:resource="https://w3id.org/italia/onto/l0/identifier"/>
    <rdfs:domain rdf:nodeID="n5bb3bff42afb4ca286d2c3fead9507ddb247"/>
    <rdfs:range rdf:resource="http://www.w3.org/2000/01/rdf-schema#Literal"/>
    <rdfs:comment xml:lang="it">Numero di codice di identificazione del partecipante (PIC - Participant Identification Code). Si tratta di un numero a 9 cifre che serve come identificatore unico per le organizzazioni (soggetti giuridici) che partecipano a programmi di finanziamento / appalti dell'UE.</rdfs:comment>
    <rdfs:comment xml:lang="en">Participant Identification Code (PIC) number. It is a 9-digit number serving as a unique identifier for organisations (legal entities) participating in EU funding programmes / procurement.</rdfs:comment>
    <rdfs:isDefinedBy rdf:resource="https://w3id.org/italia/onto/HER"/>
    <rdfs:label xml:lang="it">codice identificativo partecipante</rdfs:label>
    <rdfs:label xml:lang="en">pic number</rdfs:label>
    <owl:versionInfo xml:lang="it">stabile</owl:versionInfo>
    <owl:versionInfo xml:lang="en">stable</owl:versionInfo>
  </rdf:Description>
  <rdf:Description rdf:nodeID="n5bb3bff42afb4ca286d2c3fead9507ddb138">
    <rdf:type rdf:resource="http://www.w3.org/1999/02/22-rdf-syntax-ns#List"/>
    <rdf:first>Sample With DNA</rdf:first>
    <rdf:rest rdf:nodeID="n5bb3bff42afb4ca286d2c3fead9507ddb139"/>
  </rdf:Description>
  <rdf:Description rdf:about="https://w3id.org/italia/onto/HER/USTATMealsProvidedAggregate">
    <rdf:type rdf:resource="http://www.w3.org/2002/07/owl#Class"/>
    <rdfs:subClassOf rdf:resource="https://w3id.org/italia/onto/HER/StatisticalDataAggregation"/>
    <rdfs:comment xml:lang="en">Meals provided and students who used the canteens in the calendar year of reference.</rdfs:comment>
    <rdfs:comment xml:lang="it">Pasti erogati e studenti che hanno usufruito delle mense nell'anno solare di riferimento.</rdfs:comment>
    <rdfs:isDefinedBy rdf:resource="https://w3id.org/italia/onto/HER"/>
    <rdfs:label xml:lang="it">Aggregazione dei pasti forniti riportati da USTAT</rdfs:label>
    <rdfs:label xml:lang="en">USTAT Aggregate of Meals Provided</rdfs:label>
    <owl:versionInfo xml:lang="it">stabile</owl:versionInfo>
    <owl:versionInfo xml:lang="en">stable</owl:versionInfo>
  </rdf:Description>
  <rdf:Description rdf:about="https://w3id.org/italia/onto/HER/ctnprinInitiativeGrantedContribution">
    <rdf:type rdf:resource="http://www.w3.org/2002/07/owl#DatatypeProperty"/>
    <rdfs:subPropertyOf rdf:resource="https://w3id.org/italia/onto/MU/value"/>
    <rdfs:domain rdf:resource="https://w3id.org/italia/onto/HER/CTNPRINInitiative"/>
    <rdfs:range rdf:resource="http://www.w3.org/2001/XMLSchema#decimal"/>
    <rdfs:comment xml:lang="en">Total contributions disbursed compared to approved costs. Calculated as the sum of the corresponding 'grantedContribution' variable at the lower aggregation level (grantedContribution_operations).</rdfs:comment>
    <rdfs:comment xml:lang="it">Totale dei contributi erogati rispetto ai costi approvati. Calcolati come somma dell'omologa variabile "grantedContribution" presente a livello di aggregazione inferiore (grantedContribution_operations).</rdfs:comment>
    <rdfs:isDefinedBy rdf:resource="https://w3id.org/italia/onto/HER"/>
    <rdfs:label xml:lang="it">contributo erogato per iniziative CTN/PRIN</rdfs:label>
    <rdfs:label xml:lang="en">granted contribution of CTN/PRIN initiative</rdfs:label>
    <owl:versionInfo xml:lang="it">stabile</owl:versionInfo>
    <owl:versionInfo xml:lang="en">stable</owl:versionInfo>
  </rdf:Description>
  <rdf:Description rdf:about="https://w3id.org/italia/onto/HER/innovative">
    <rdf:type rdf:resource="http://www.w3.org/2002/07/owl#DatatypeProperty"/>
    <rdf:type rdf:resource="http://www.w3.org/2002/07/owl#FunctionalProperty"/>
    <rdfs:domain rdf:resource="https://w3id.org/italia/onto/HER/Spinoff"/>
    <rdfs:range rdf:resource="http://www.w3.org/2001/XMLSchema#boolean"/>
    <rdfs:comment xml:lang="it">Indica se lo spin-off ha anche la qualifica di start-up innovativa ai sensi della L. 221/2012.</rdfs:comment>
    <rdfs:comment xml:lang="en">It indicates whether the spin-off also qualifies as an innovative start-up under Law 221/2012.</rdfs:comment>
    <rdfs:isDefinedBy rdf:resource="https://w3id.org/italia/onto/HER"/>
    <rdfs:label xml:lang="it">innovativa</rdfs:label>
    <rdfs:label xml:lang="en">innovative</rdfs:label>
    <owl:versionInfo xml:lang="it">stabile</owl:versionInfo>
    <owl:versionInfo xml:lang="en">stable</owl:versionInfo>
  </rdf:Description>
  <rdf:Description rdf:about="https://w3id.org/italia/onto/HER/founderPatent">
    <rdf:type rdf:resource="http://www.w3.org/2002/07/owl#DatatypeProperty"/>
    <rdf:type rdf:resource="http://www.w3.org/2002/07/owl#FunctionalProperty"/>
    <rdfs:domain rdf:resource="https://w3id.org/italia/onto/HER/Spinoff"/>
    <rdfs:range rdf:resource="http://www.w3.org/2001/XMLSchema#boolean"/>
    <rdfs:comment xml:lang="it">Indica se sono presenti o meno dei brevetti collegati allo spin-off.</rdfs:comment>
    <rdfs:comment xml:lang="en">It indicates whether there are or not any patents related to the spin-off.</rdfs:comment>
    <rdfs:isDefinedBy rdf:resource="https://w3id.org/italia/onto/HER"/>
    <rdfs:label xml:lang="it">brevetto fondatore</rdfs:label>
    <rdfs:label xml:lang="en">founder patent</rdfs:label>
    <owl:versionInfo xml:lang="it">stabile</owl:versionInfo>
    <owl:versionInfo xml:lang="en">stable</owl:versionInfo>
  </rdf:Description>
  <rdf:Description rdf:nodeID="n5bb3bff42afb4ca286d2c3fead9507ddb434">
    <rdf:type rdf:resource="http://www.w3.org/2002/07/owl#Restriction"/>
    <owl:onProperty rdf:resource="https://w3id.org/italia/onto/HER/withCountry"/>
    <owl:qualifiedCardinality rdf:datatype="http://www.w3.org/2001/XMLSchema#nonNegativeInteger">1</owl:qualifiedCardinality>
    <owl:onClass rdf:resource="https://w3id.org/italia/onto/CLV/Country"/>
  </rdf:Description>
  <rdf:Description rdf:about="https://w3id.org/italia/onto/HER/hasCoordinator">
    <rdf:type rdf:resource="http://www.w3.org/2002/07/owl#ObjectProperty"/>
    <owl:inverseOf rdf:resource="https://w3id.org/italia/onto/HER/isCoordinatorOf"/>
    <rdfs:domain rdf:resource="https://w3id.org/italia/onto/Project/PublicResearchProject"/>
    <rdfs:range rdf:resource="https://w3id.org/italia/onto/COV/Organization"/>
    <rdfs:comment xml:lang="it">Beneficiario principale in un gruppo di beneficiari. Punto di contatto principale per il progetto.</rdfs:comment>
    <rdfs:comment xml:lang="en">Lead beneficiary in a group of beneficiaries. Main contact point for the project.</rdfs:comment>
    <rdfs:isDefinedBy rdf:resource="https://w3id.org/italia/onto/HER"/>
    <rdfs:label xml:lang="it">ha coordinatore</rdfs:label>
    <rdfs:label xml:lang="en">has coordinator</rdfs:label>
    <owl:versionInfo xml:lang="it">provvisoria</owl:versionInfo>
    <owl:versionInfo xml:lang="en">unstable</owl:versionInfo>
  </rdf:Description>
  <rdf:Description rdf:about="https://w3id.org/italia/onto/HER/patentPriorityYear">
    <rdf:type rdf:resource="http://www.w3.org/2002/07/owl#DatatypeProperty"/>
    <rdfs:subPropertyOf rdf:resource="https://w3id.org/italia/onto/TI/year"/>
    <rdfs:domain rdf:resource="https://w3id.org/italia/onto/HER/PatentPriorityDetail"/>
    <rdfs:range rdf:resource="http://www.w3.org/2001/XMLSchema#gYear"/>
    <rdfs:comment xml:lang="it">L'anno della data di priorità della domanda corrispondente</rdfs:comment>
    <rdfs:comment xml:lang="en">The year of the priority date of the corresponding application</rdfs:comment>
    <rdfs:isDefinedBy rdf:resource="https://w3id.org/italia/onto/HER"/>
    <rdfs:label xml:lang="it">anno di prioritá</rdfs:label>
    <rdfs:label xml:lang="en">priority year</rdfs:label>
    <owl:versionInfo xml:lang="it">stabile</owl:versionInfo>
    <owl:versionInfo xml:lang="en">stable</owl:versionInfo>
  </rdf:Description>
  <rdf:Description rdf:about="https://w3id.org/italia/onto/HER/ctnprinOperationApprovedCost">
    <rdf:type rdf:resource="http://www.w3.org/2002/07/owl#DatatypeProperty"/>
    <rdfs:subPropertyOf rdf:resource="https://w3id.org/italia/onto/MU/value"/>
    <rdfs:domain rdf:resource="https://w3id.org/italia/onto/HER/CTNPRINOperation"/>
    <rdfs:range rdf:resource="http://www.w3.org/2001/XMLSchema#decimal"/>
    <rdfs:comment xml:lang="it">Costi approvati dopo valutazione in itinere rispetto ai costi rendicontati dal beneficiario a cui fa capo l'operazione. Calcolati come somma dell'omologa variabile "approvedCost" presente a livello di aggregazione inferiore (approvedCost_amounts)</rdfs:comment>
    <rdfs:comment xml:lang="en">Costs approved after evaluation in itinere compared to the costs reported by the beneficiary to which the operation belongs. Calculated as the sum of the approvedCost variable at the lower aggregation level (approvedCost_amounts).</rdfs:comment>
    <rdfs:isDefinedBy rdf:resource="https://w3id.org/italia/onto/HER"/>
    <rdfs:label xml:lang="en">approved cost of CTN/PRIN operation</rdfs:label>
    <rdfs:label xml:lang="it">costi approvati per operazioni CTN/PRIN</rdfs:label>
    <owl:versionInfo xml:lang="it">stabile</owl:versionInfo>
    <owl:versionInfo xml:lang="en">stable</owl:versionInfo>
  </rdf:Description>
  <rdf:Description rdf:about="https://w3id.org/italia/onto/HER/MIURStudentsByRegionOfResidenceDegreeDegreeClassAggregate">
    <rdf:type rdf:resource="http://www.w3.org/2002/07/owl#Class"/>
    <rdfs:subClassOf rdf:resource="https://w3id.org/italia/onto/HER/StatisticalDataAggregation"/>
    <rdfs:subClassOf rdf:nodeID="n5bb3bff42afb4ca286d2c3fead9507ddb497"/>
    <rdfs:comment xml:lang="en">Aggregated data on Italian students filed in the MIUR system, grouped by year, university, Italian region of residence, degree and degree class.</rdfs:comment>
    <rdfs:comment xml:lang="it">Dati aggregati sugli studenti italiani archiviati nel sistema MIUR, raggruppati per anno, università, regione di residenza italiana, laurea e classe di laurea.</rdfs:comment>
    <rdfs:isDefinedBy rdf:resource="https://w3id.org/italia/onto/HER"/>
    <rdfs:label xml:lang="en">Aggregate of Italian Students By Region of Residence, Degree and Degree Class</rdfs:label>
    <rdfs:label xml:lang="it">Aggregazione dei studenti italiani per regione di residenza, laurea e classe di laurea</rdfs:label>
    <owl:versionInfo xml:lang="it">stabile</owl:versionInfo>
    <owl:versionInfo xml:lang="en">stable</owl:versionInfo>
  </rdf:Description>
  <rdf:Description rdf:about="https://w3id.org/italia/onto/HER/WIPOIPCSubclass">
    <rdf:type rdf:resource="http://www.w3.org/2002/07/owl#Class"/>
    <rdfs:subClassOf rdf:resource="https://w3id.org/italia/onto/HER/InternationalPatentClassification"/>
    <rdfs:comment xml:lang="en">In each classification symbol, the letter following the class (two digit number after the initial letter) makes up the "subclass".</rdfs:comment>
    <rdfs:comment xml:lang="it">In ogni simbolo di classificazione, la lettera che segue la classe (numero di due cifre dopo la lettera iniziale) costituisce la "sottoclasse".</rdfs:comment>
    <rdfs:isDefinedBy rdf:resource="https://w3id.org/italia/onto/HER"/>
    <rdfs:label xml:lang="it">Sottoclasse WIPO IPC</rdfs:label>
    <rdfs:label xml:lang="en">WIPO IPC Subclass</rdfs:label>
    <owl:versionInfo xml:lang="it">stabile</owl:versionInfo>
    <owl:versionInfo xml:lang="en">stable</owl:versionInfo>
    <ns6:wasDerivedFrom rdf:resource="http://www.w3.org/2004/02/skos/core#Concept"/>
  </rdf:Description>
  <rdf:Description rdf:nodeID="n5bb3bff42afb4ca286d2c3fead9507ddb290">
    <rdf:type rdf:resource="http://www.w3.org/1999/02/22-rdf-syntax-ns#List"/>
    <rdf:first>Longitudinal, Prospective</rdf:first>
    <rdf:rest rdf:nodeID="n5bb3bff42afb4ca286d2c3fead9507ddb291"/>
  </rdf:Description>
  <rdf:Description rdf:about="https://w3id.org/italia/onto/HER/ECParticipant">
    <rdf:type rdf:resource="http://www.w3.org/2002/07/owl#Class"/>
    <rdfs:subClassOf rdf:resource="https://w3id.org/italia/onto/RO/TimeIndexedRole"/>
    <rdfs:subClassOf rdf:nodeID="n5bb3bff42afb4ca286d2c3fead9507ddb438"/>
    <rdfs:subClassOf rdf:nodeID="n5bb3bff42afb4ca286d2c3fead9507ddb439"/>
    <rdfs:subClassOf rdf:nodeID="n5bb3bff42afb4ca286d2c3fead9507ddb440"/>
    <rdfs:subClassOf rdf:nodeID="n5bb3bff42afb4ca286d2c3fead9507ddb441"/>
    <rdfs:subClassOf rdf:nodeID="n5bb3bff42afb4ca286d2c3fead9507ddb442"/>
    <rdfs:subClassOf rdf:nodeID="n5bb3bff42afb4ca286d2c3fead9507ddb443"/>
    <rdfs:subClassOf rdf:nodeID="n5bb3bff42afb4ca286d2c3fead9507ddb444"/>
    <rdfs:comment xml:lang="it">Partecipante ad un progetto CE. Questa classe è una reificazione del rapporto che coinvolge un progetto con un'organizzazione partecipante. Questa classe reificata memorizza informazioni aggiuntive come il finanziamento concesso dall'UE al partecipante specifico.</rdfs:comment>
    <rdfs:comment xml:lang="en">Participant in a EC project. This class is a reification of the relationship that involves a project with a participating organization. This reified class stores additional information such as the funding granted by the EU to the specific participant.</rdfs:comment>
    <rdfs:isDefinedBy rdf:resource="https://w3id.org/italia/onto/HER"/>
    <rdfs:label xml:lang="en">EC Participant</rdfs:label>
    <rdfs:label xml:lang="it">Partecipante CE</rdfs:label>
    <owl:versionInfo xml:lang="it">stabile</owl:versionInfo>
    <owl:versionInfo xml:lang="en">stable</owl:versionInfo>
  </rdf:Description>
  <rdf:Description rdf:about="https://w3id.org/italia/onto/HER/hasLastUpdatePostedDate">
    <rdf:type rdf:resource="http://www.w3.org/2002/07/owl#ObjectProperty"/>
    <rdfs:subPropertyOf rdf:resource="https://w3id.org/italia/onto/TI/hasTemporalEntity"/>
    <rdfs:domain rdf:resource="https://w3id.org/italia/onto/HER/AACTStudy"/>
    <rdfs:range rdf:resource="https://w3id.org/italia/onto/TI#TimeInstant"/>
    <rdfs:comment xml:lang="it">La data più recente in cui sono state rese disponibili su ClinicalTrials.gov. Ci può essere un ritardo tra la data in cui le modifiche sono state inviate a ClinicalTrials.gov dallo sponsor o dallo sperimentatore dello studio (la data dell'ultimo aggiornamento inviato) e la data dell'ultimo aggiornamento pubblicato.</rdfs:comment>
    <rdfs:comment xml:lang="en">The most recent date on which changes to a study record were made available on ClinicalTrials.gov. There may be a delay between when the changes were submitted to ClinicalTrials.gov by the study's sponsor or investigator (the last update submitted date) and the last update posted date</rdfs:comment>
    <rdfs:isDefinedBy rdf:resource="https://w3id.org/italia/onto/HER"/>
    <rdfs:label xml:lang="it">ha data ultimo aggiornamento pubblicato</rdfs:label>
    <rdfs:label xml:lang="en">has last update posted date</rdfs:label>
    <owl:versionInfo xml:lang="it">prova</owl:versionInfo>
    <owl:versionInfo xml:lang="en">testing</owl:versionInfo>
  </rdf:Description>
  <rdf:Description rdf:nodeID="n5bb3bff42afb4ca286d2c3fead9507ddb96">
    <rdf:type rdf:resource="http://www.w3.org/2002/07/owl#Class"/>
    <owl:unionOf rdf:nodeID="n5bb3bff42afb4ca286d2c3fead9507ddb97"/>
  </rdf:Description>
  <rdf:Description rdf:about="https://w3id.org/italia/onto/HER/publicationDate">
    <rdf:type rdf:resource="http://www.w3.org/2002/07/owl#DatatypeProperty"/>
    <rdfs:subPropertyOf rdf:resource="https://w3id.org/italia/onto/TI/date"/>
    <rdfs:domain rdf:nodeID="n5bb3bff42afb4ca286d2c3fead9507ddb265"/>
    <rdfs:range rdf:resource="http://www.w3.org/2001/XMLSchema#date"/>
    <rdfs:comment xml:lang="it">La data di pubblicazione di un risultato</rdfs:comment>
    <rdfs:comment xml:lang="en">The date of publication of a result</rdfs:comment>
    <rdfs:isDefinedBy rdf:resource="https://w3id.org/italia/onto/HER"/>
    <rdfs:label xml:lang="it">data pubblicazione</rdfs:label>
    <rdfs:label xml:lang="en">publication date</rdfs:label>
    <owl:versionInfo xml:lang="it">stabile</owl:versionInfo>
    <owl:versionInfo xml:lang="en">stable</owl:versionInfo>
  </rdf:Description>
  <rdf:Description rdf:about="https://w3id.org/italia/onto/HER/ErasmusPlusTopic">
    <rdf:type rdf:resource="http://www.w3.org/2002/07/owl#Class"/>
    <rdfs:subClassOf rdf:resource="https://w3id.org/italia/onto/HER/ErasmusPlusClassification"/>
    <rdfs:comment xml:lang="it">Quando disponibile, si riferisce all'argomento o agli argomenti principali del progetto.</rdfs:comment>
    <rdfs:comment xml:lang="en">When available, it refers to the main topic(s) of the project.</rdfs:comment>
    <rdfs:isDefinedBy rdf:resource="https://w3id.org/italia/onto/HER"/>
    <rdfs:label xml:lang="it">Argomento Erasmus+</rdfs:label>
    <rdfs:label xml:lang="en">Erasmus+ Topic</rdfs:label>
    <owl:versionInfo xml:lang="it">stabile</owl:versionInfo>
    <owl:versionInfo xml:lang="en">stable</owl:versionInfo>
    <ns6:wasDerivedFrom rdf:resource="http://www.w3.org/2004/02/skos/core#Concept"/>
  </rdf:Description>
  <rdf:Description rdf:about="https://w3id.org/italia/onto/HER/USTATInterventionsForStudentsByUniversitiesAggregate">
    <rdf:type rdf:resource="http://www.w3.org/2002/07/owl#Class"/>
    <rdfs:subClassOf rdf:resource="https://w3id.org/italia/onto/HER/StatisticalDataAggregation"/>
    <rdfs:subClassOf rdf:nodeID="n5bb3bff42afb4ca286d2c3fead9507ddb530"/>
    <rdfs:comment xml:lang="en">Data related to the number of interventions in favour of students (excluding the Right to Study by the regions) carried out by the universities.</rdfs:comment>
    <rdfs:comment xml:lang="it">Dati relativi al numero di interventi a favore degli studenti (escluso il Diritto allo Studio regionale) effettuati dagli atenei.</rdfs:comment>
    <rdfs:isDefinedBy rdf:resource="https://w3id.org/italia/onto/HER"/>
    <rdfs:label xml:lang="it">Aggregazione degli interventi universitari per gli studenti riportati da USTAT</rdfs:label>
    <rdfs:label xml:lang="en">USTAT Aggregate of University Interventions For Students</rdfs:label>
    <owl:versionInfo xml:lang="it">stabile</owl:versionInfo>
    <owl:versionInfo xml:lang="en">stable</owl:versionInfo>
  </rdf:Description>
  <rdf:Description rdf:about="https://w3id.org/italia/onto/HER/hasSSD">
    <rdf:type rdf:resource="http://www.w3.org/2002/07/owl#ObjectProperty"/>
    <rdfs:subPropertyOf rdf:resource="https://w3id.org/italia/onto/HER/hasAcademicDiscipline"/>
    <rdfs:domain rdf:resource="https://w3id.org/italia/onto/HER/ItalianPhDCourseByCycle"/>
    <rdfs:range rdf:resource="https://w3id.org/italia/onto/HER/ScientificDisciplinarySector"/>
    <rdfs:comment xml:lang="en">Property that links some statistical data to the scientific disciplinary sector of the academic disciplines classification.</rdfs:comment>
    <rdfs:comment xml:lang="it">Proprietà che collega alcuni dati statistici al settore scientifico disciplinare della classificazione sulle discipline accademiche.</rdfs:comment>
    <rdfs:isDefinedBy rdf:resource="https://w3id.org/italia/onto/HER"/>
    <rdfs:label xml:lang="it">ha settore scientifico disciplinare</rdfs:label>
    <rdfs:label xml:lang="en">has scientific disciplinary sector</rdfs:label>
    <owl:versionInfo xml:lang="it">stabile</owl:versionInfo>
    <owl:versionInfo xml:lang="en">stable</owl:versionInfo>
  </rdf:Description>
  <rdf:Description rdf:nodeID="n5bb3bff42afb4ca286d2c3fead9507ddb86">
    <rdf:type rdf:resource="http://www.w3.org/2002/07/owl#Class"/>
    <owl:unionOf rdf:nodeID="n5bb3bff42afb4ca286d2c3fead9507ddb87"/>
  </rdf:Description>
  <rdf:Description rdf:about="https://w3id.org/italia/onto/HER/totalMaleDoctorateStudents">
    <rdf:type rdf:resource="http://www.w3.org/2002/07/owl#DatatypeProperty"/>
    <rdfs:subPropertyOf rdf:resource="https://w3id.org/italia/onto/MU/value"/>
    <rdfs:domain rdf:resource="https://w3id.org/italia/onto/HER/USTATStudentsBySexAggregate"/>
    <rdfs:range rdf:resource="http://www.w3.org/2000/01/rdf-schema#Literal"/>
    <rdfs:comment xml:lang="en">Information on men enrolled in PhD courses, broken down by gender, university, geographical area, course type and field of education and training (ISCED-F 2013). Data available from the academic year 2012/2013. Students at ISCED Level 8 2011.
From 2015-2016 onwards, data are collected by the National Register of Students and Graduates (ANS_PL), which could lead to a discontinuity in the historical series.
Elaborations on ANS-PL data extracted on 2/10/2019.</rdfs:comment>
    <rdfs:comment xml:lang="it">Informazioni sugli uomini iscritti ai corsi di dottorato, disaggregate per genere, ateneo, area geografica, tipo di corso e field of education and training (ISCED-F 2013). Dati disponibili a partire dall’anno accademico 2012/2013. Studenti del livello 8 della ISCED 2011.
A partire dall'a.a. 2015-2016 i dati sono rilevati dall'Anagrafe Nazionale degli Studenti e dei Laureati (ANS_PL), ciò potrebbe determinare una discontinuità nella serie storica. Elaborazioni su dati ANS-PL estratti alla data del 2/10/2019.</rdfs:comment>
    <rdfs:isDefinedBy rdf:resource="https://w3id.org/italia/onto/HER"/>
    <rdfs:label xml:lang="en">total male doctorate students</rdfs:label>
    <rdfs:label xml:lang="it">totale degli studenti di dottorato di genere maschile</rdfs:label>
    <owl:versionInfo xml:lang="it">stabile</owl:versionInfo>
    <owl:versionInfo xml:lang="en">stable</owl:versionInfo>
  </rdf:Description>
  <rdf:Description rdf:about="https://w3id.org/italia/onto/HER/foundationProjectDescription">
    <rdf:type rdf:resource="http://www.w3.org/2002/07/owl#DatatypeProperty"/>
    <rdfs:subPropertyOf rdf:resource="https://w3id.org/italia/onto/l0/description"/>
    <rdfs:domain rdf:resource="https://w3id.org/italia/onto/HER/Spinoff"/>
    <rdfs:range rdf:resource="http://www.w3.org/2000/01/rdf-schema#Literal"/>
    <rdfs:comment xml:lang="it">Fornisce una descrizione del progetto alla base della fondazione dello spin-off.</rdfs:comment>
    <rdfs:comment xml:lang="en">It provides a description of the project behind the foundation of the spin-off.</rdfs:comment>
    <rdfs:isDefinedBy rdf:resource="https://w3id.org/italia/onto/HER"/>
    <rdfs:label xml:lang="it">descrizione progetto di fondazione</rdfs:label>
    <rdfs:label xml:lang="en">foundation project description</rdfs:label>
    <owl:versionInfo xml:lang="it">stabile</owl:versionInfo>
    <owl:versionInfo xml:lang="en">stable</owl:versionInfo>
  </rdf:Description>
  <rdf:Description rdf:about="https://w3id.org/italia/onto/HER/ERCResearchDomain">
    <rdf:type rdf:resource="http://www.w3.org/2002/07/owl#Class"/>
    <rdfs:subClassOf rdf:resource="https://w3id.org/italia/onto/HER/ERCClassification"/>
    <rdfs:comment xml:lang="en">Scientific domains to which the 25 ERC panels -used for the planning and operation of the evaluation of ERC grant proposals- are assigned to. They cover all fields of science, engineering and scholarship which, concretely: Social Sciences and Humanities (6 Panels, SH1–SH6), Physical Sciences and Engineering (10 Panels, PE1–PE10), Life Sciences (9 Panels, LS1–LS9).</rdfs:comment>
    <rdfs:comment xml:lang="it">Settori scientifici ai quali sono assegnati i 25 gruppi di esperti scientifici del CER - utilizzati per la pianificazione e il funzionamento della valutazione delle proposte di sovvenzione del CER -. Essi coprono tutti i campi della scienza, dell'ingegneria e delle borse di studio che, in concreto: Scienze sociali e umanistiche (6 gruppi, SH1-SH6), Scienze fisiche e ingegneria (10 gruppi, PE1-PE10), Scienze della vita (9 gruppi, LS1-LS9).</rdfs:comment>
    <rdfs:isDefinedBy rdf:resource="https://w3id.org/italia/onto/HER"/>
    <rdfs:label xml:lang="it">Dominio di ricerca ERC</rdfs:label>
    <rdfs:label xml:lang="en">ERC Research Domain</rdfs:label>
    <owl:versionInfo xml:lang="it">stabile</owl:versionInfo>
    <owl:versionInfo xml:lang="en">stable</owl:versionInfo>
    <ns6:wasDerivedFrom rdf:resource="http://www.w3.org/2004/02/skos/core#Concept"/>
    <ns4:controlledVocabulary rdf:resource="https://w3id.org/italia/controlled-vocabulary/classifications-for-her/erc-panel-h2020-fp"/>
  </rdf:Description>
  <rdf:Description rdf:about="https://w3id.org/italia/onto/HER/aactResponsiblePartyType">
    <rdf:type rdf:resource="http://www.w3.org/2002/07/owl#DatatypeProperty"/>
    <rdfs:domain rdf:resource="https://w3id.org/italia/onto/HER/AACTResponsibleParty"/>
    <rdfs:range rdf:resource="http://www.w3.org/2000/01/rdf-schema#Literal"/>
    <rdfs:comment xml:lang="en">Responsible Party type:
Sponsor: The entity (for example, corporation or agency) that initiates the study
Principal Investigator: The individual designated as responsible party by the sponsor (see Note)
Sponsor-Investigator: The individual who both initiates and conducts the study
</rdfs:comment>
    <rdfs:comment xml:lang="it">Tipologia di responsabile dello studio:
Sponsor: L'entità (per esempio, società o agenzia) che avvia lo studio
Investigatore principale: La persona designata come responsabile dallo sponsor (vedi nota)
Sponsor-Investigatore: L'individuo che inizia e conduce lo studio</rdfs:comment>
    <rdfs:isDefinedBy rdf:resource="https://w3id.org/italia/onto/HER"/>
    <rdfs:label xml:lang="en">responsible party type</rdfs:label>
    <rdfs:label xml:lang="it">tipo di parte reponsabile</rdfs:label>
    <owl:versionInfo xml:lang="it">provvisoria</owl:versionInfo>
    <owl:versionInfo xml:lang="en">unstable</owl:versionInfo>
  </rdf:Description>
  <rdf:Description rdf:about="https://w3id.org/italia/onto/COV/Office">
    <rdf:type rdf:resource="http://www.w3.org/2002/07/owl#Class"/>
  </rdf:Description>
  <rdf:Description rdf:about="https://w3id.org/italia/onto/HER/totalFemaleDoctorateStudents">
    <rdf:type rdf:resource="http://www.w3.org/2002/07/owl#DatatypeProperty"/>
    <rdfs:subPropertyOf rdf:resource="https://w3id.org/italia/onto/MU/value"/>
    <rdfs:domain rdf:resource="https://w3id.org/italia/onto/HER/USTATStudentsBySexAggregate"/>
    <rdfs:range rdf:resource="http://www.w3.org/2000/01/rdf-schema#Literal"/>
    <rdfs:comment xml:lang="en">Information on women enrolled in PhD courses, broken down by gender, university, geographical area, course type and field of education and training (ISCED-F 2013). Data available from the academic year 2012/2013. Students at ISCED Level 8 2011.
From 2015-2016 onwards, data are collected by the National Register of Students and Graduates (ANS_PL), which could lead to a discontinuity in the historical series.
Elaborations on ANS-PL data extracted on 2/10/2019.</rdfs:comment>
    <rdfs:comment xml:lang="it">Informazioni sulle donne iscritte ai corsi di dottorato, disaggregate per genere, ateneo, area geografica, tipo di corso e field of education and training (ISCED-F 2013). Dati disponibili a partire dall’anno accademico 2012/2013. Studenti del livello 8 della ISCED 2011.
A partire dall'a.a. 2015-2016 i dati sono rilevati dall'Anagrafe Nazionale degli Studenti e dei Laureati (ANS_PL), ciò potrebbe determinare una discontinuità nella serie storica.
Elaborazioni su dati ANS-PL estratti alla data del 2/10/2019.</rdfs:comment>
    <rdfs:isDefinedBy rdf:resource="https://w3id.org/italia/onto/HER"/>
    <rdfs:label xml:lang="en">total female doctorate students</rdfs:label>
    <rdfs:label xml:lang="it">totale degli studenti di dottorato di genere famminile</rdfs:label>
    <owl:versionInfo xml:lang="it">stabile</owl:versionInfo>
    <owl:versionInfo xml:lang="en">stable</owl:versionInfo>
  </rdf:Description>
  <rdf:Description rdf:about="https://w3id.org/italia/onto/HER/aactMaximumAge">
    <rdf:type rdf:resource="http://www.w3.org/2002/07/owl#DatatypeProperty"/>
    <rdfs:subPropertyOf rdf:resource="https://w3id.org/italia/onto/CPV/age"/>
    <rdfs:domain rdf:resource="https://w3id.org/italia/onto/HER/AACTEligibility"/>
    <rdfs:range rdf:resource="http://www.w3.org/2001/XMLSchema#integer"/>
    <rdfs:comment xml:lang="it">Il valore numerico, se presente, per l'età massima che un potenziale partecipante può avere per essere idoneo allo studio clinico.</rdfs:comment>
    <rdfs:comment xml:lang="en">The numerical value, if any, for the maximum age a potential participant can be to be eligible for the clinical study.</rdfs:comment>
    <rdfs:isDefinedBy rdf:resource="https://w3id.org/italia/onto/HER"/>
    <rdfs:label xml:lang="en">AACT maximum age</rdfs:label>
    <rdfs:label xml:lang="it">etá massima AACT</rdfs:label>
    <owl:versionInfo xml:lang="it">stabile</owl:versionInfo>
    <owl:versionInfo xml:lang="en">stable</owl:versionInfo>
  </rdf:Description>
  <rdf:Description rdf:about="https://w3id.org/italia/onto/HER/hasEligibleSex">
    <rdf:type rdf:resource="http://www.w3.org/2002/07/owl#ObjectProperty"/>
    <rdfs:domain rdf:resource="https://w3id.org/italia/onto/HER/AACTEligibility"/>
    <rdfs:range rdf:resource="https://w3id.org/italia/onto/CPV/Sex"/>
    <rdfs:comment xml:lang="en">Property that link the eligibility of clinical trials to the sex of a person. Since sex can be female and male, the property can be used to express when the eligible sex is female or when it is male, or both of the two. In this latter case, two occurences of this property can be used for the AACTEligibility class one for female, one for male, meaning that all possible sex options are accepted.</rdfs:comment>
    <rdfs:comment xml:lang="it">Proprietà che collega l'idoneità degli studi clinici al sesso di una persona. Poiché il sesso può essere femminile e maschile, la proprietà può essere usata per esprimere quando il sesso idoneo è femminile o quando è maschile, o entrambi. In quest'ultimo caso, due materializzazioni di questa proprietà possono essere utilizzate per la classe AACTEligibilità, una per il sesso femminile e una per il sesso maschile, il che significa che tutte le opzioni sul sesso sono accettate (nei dataset è l'equivalente dell'opzione "tutti)").</rdfs:comment>
    <rdfs:isDefinedBy rdf:resource="https://w3id.org/italia/onto/HER"/>
    <rdfs:label xml:lang="it">ha sesso idoneo</rdfs:label>
    <rdfs:label xml:lang="en">has eligible sex</rdfs:label>
    <owl:versionInfo xml:lang="it">stabile</owl:versionInfo>
    <owl:versionInfo xml:lang="en">stable</owl:versionInfo>
  </rdf:Description>
  <rdf:Description rdf:nodeID="n5bb3bff42afb4ca286d2c3fead9507ddb529">
    <rdf:type rdf:resource="http://www.w3.org/2002/07/owl#Restriction"/>
    <owl:onProperty rdf:resource="https://w3id.org/italia/onto/COV/hasOrganization"/>
    <owl:maxQualifiedCardinality rdf:datatype="http://www.w3.org/2001/XMLSchema#nonNegativeInteger">1</owl:maxQualifiedCardinality>
    <owl:onClass rdf:resource="https://w3id.org/italia/onto/COV/Organization"/>
  </rdf:Description>
  <rdf:Description rdf:about="https://w3id.org/italia/onto/HER/hasEurekaInstrument">
    <rdf:type rdf:resource="http://www.w3.org/2002/07/owl#ObjectProperty"/>
    <rdfs:domain rdf:resource="https://w3id.org/italia/onto/HER/EUREKAProject"/>
    <rdfs:range rdf:resource="https://w3id.org/italia/onto/HER/EUREKAInstrument"/>
    <rdfs:comment xml:lang="it">Questa proprietà collega un progetto EUREKA con lo strumento corrispondente.</rdfs:comment>
    <rdfs:comment xml:lang="en">This property connects an EUREKA project with the corresponding instrument.</rdfs:comment>
    <rdfs:isDefinedBy rdf:resource="https://w3id.org/italia/onto/HER"/>
    <rdfs:label xml:lang="it">ha strumento EUREKA</rdfs:label>
    <rdfs:label xml:lang="en">has EUREKA instrument</rdfs:label>
    <owl:versionInfo xml:lang="it">stabile</owl:versionInfo>
    <owl:versionInfo xml:lang="en">stable</owl:versionInfo>
  </rdf:Description>
  <rdf:Description rdf:nodeID="n5bb3bff42afb4ca286d2c3fead9507ddb163">
    <rdf:first rdf:resource="https://w3id.org/italia/onto/HER/ECProject"/>
    <rdf:rest rdf:nodeID="n5bb3bff42afb4ca286d2c3fead9507ddb164"/>
  </rdf:Description>
  <rdf:Description rdf:about="https://w3id.org/italia/onto/HER/hasCHAFEAParticipant">
    <rdf:type rdf:resource="http://www.w3.org/2002/07/owl#ObjectProperty"/>
    <rdfs:subPropertyOf rdf:resource="https://w3id.org/italia/onto/RO/hasRiT"/>
    <rdfs:domain rdf:resource="https://w3id.org/italia/onto/HER/CHAFEAProject"/>
    <rdfs:range rdf:resource="https://w3id.org/italia/onto/HER/CHAFEAParticipant"/>
    <rdfs:comment xml:lang="it">Questa proprietà collega un'attività finanziata con le istituzioni coinvolte.</rdfs:comment>
    <rdfs:comment xml:lang="en">This property connects a funded activity with the institutions involved.</rdfs:comment>
    <rdfs:isDefinedBy rdf:resource="https://w3id.org/italia/onto/HER"/>
    <rdfs:label xml:lang="it">ha partecipante CHAFEA</rdfs:label>
    <rdfs:label xml:lang="en">has CHAFEA participant</rdfs:label>
    <owl:versionInfo xml:lang="it">stabile</owl:versionInfo>
    <owl:versionInfo xml:lang="en">stable</owl:versionInfo>
  </rdf:Description>
  <rdf:Description rdf:about="https://w3id.org/italia/onto/HER/rcn">
    <rdf:type rdf:resource="http://www.w3.org/2002/07/owl#DatatypeProperty"/>
    <rdfs:subPropertyOf rdf:resource="https://w3id.org/italia/onto/l0/identifier"/>
    <rdfs:domain rdf:resource="https://w3id.org/italia/onto/HER/ECParticipant"/>
    <rdfs:range rdf:resource="http://www.w3.org/2000/01/rdf-schema#Literal"/>
    <rdfs:comment xml:lang="en">Record Control Number, used as a participant identifier in CORDIS.</rdfs:comment>
    <rdfs:comment xml:lang="it">Record Control Number, utilizzato come identificativo del partecipante in CORDIS.</rdfs:comment>
    <rdfs:isDefinedBy rdf:resource="https://w3id.org/italia/onto/HER"/>
    <rdfs:label xml:lang="it">numero record di controllo</rdfs:label>
    <rdfs:label xml:lang="en">record control number</rdfs:label>
    <owl:versionInfo xml:lang="it">stabile</owl:versionInfo>
    <owl:versionInfo xml:lang="en">stable</owl:versionInfo>
  </rdf:Description>
  <rdf:Description rdf:about="https://w3id.org/italia/onto/HER/studyFirstSubmittedQCDate">
    <rdf:type rdf:resource="http://www.w3.org/2002/07/owl#DatatypeProperty"/>
    <rdfs:subPropertyOf rdf:resource="https://w3id.org/italia/onto/TI/date"/>
    <rdfs:domain rdf:resource="https://w3id.org/italia/onto/HER/AACTStudy"/>
    <rdfs:range rdf:resource="http://www.w3.org/2001/XMLSchema#date"/>
    <rdfs:comment xml:lang="it">Il suffisso _submitted_qc indica la data di presentazione dello studio della versione del record che soddisfa i criteri di controllo di qualità. È comune che ci siano revisioni tra la prima presentazione dello studio e la presentazione che soddisfa i criteri qc. Si noti che questa non è la data in cui è stata completata la revisione qc".</rdfs:comment>
    <rdfs:comment xml:lang="en">The _submitted_qc suffix indicates the study submission date of the version of the record that met quality control criteria. It is common for there to be revisions between the first study submission and the submission that meets qc criteria. Note this is not the date that the qc review was completed."</rdfs:comment>
    <rdfs:isDefinedBy rdf:resource="https://w3id.org/italia/onto/HER"/>
    <rdfs:label xml:lang="it">data primo studio presentato QC</rdfs:label>
    <rdfs:label xml:lang="en">study first submitted QC date</rdfs:label>
    <owl:versionInfo xml:lang="it">stabile</owl:versionInfo>
    <owl:versionInfo xml:lang="en">stable</owl:versionInfo>
  </rdf:Description>
  <rdf:Description rdf:about="https://w3id.org/italia/onto/HER/USTATCanteenServiceClass">
    <rdf:type rdf:resource="http://www.w3.org/2002/07/owl#Class"/>
    <rdfs:subClassOf rdf:resource="https://w3id.org/italia/onto/l0/Characteristic"/>
    <rdfs:comment xml:lang="en">Information on accommodation and catering services at 1/11 of the reference year (T). In particular, the service provided is described through the identification code and description of the service: the possible values for codes and description are:
1 : Accommodation places in residences
2a: Accommodation in residences - of which assigned to eligible students (scholarship holders and non-scholarship holders)
4 : Accommodation in residences - of which allocated to non-eligible students
5 : Accommodation in residences - of which reserved for mobility students (e.g. Erasmus)
6 : Accommodation in residences - of which reserved for guest house use
7 : Directly managed canteens
8 : Seats in directly managed canteens
9 : Canteens under indirect management
10: Seats in indirectly managed canteens

When using the data take special care to avoid duplication, after carefully reading the code descriptions.
In particular, pay attention to the values indicated as ""of which..."", already included in the main entry.</rdfs:comment>
    <rdfs:comment xml:lang="it">Informazioni sui posti alloggio e servizi di ristorazione all'1/11 dell'anno di riferimento (T). In particolare, il servizio erogato viene descritto tramite il codice identificativo e la descrizione del servizio: i valori possibili per codici e descrizione sono:
1 : Posti alloggio in residenze
2a: Posti alloggio in residenze - di cui assegnati a studenti idonei (borsisti e non borsisti)
4 : Posti alloggio in residenze - di cui assegnati a studenti non idonei
5 : Posti alloggio in residenze - di cui riservati a studenti in mobilità (es. Erasmus)
6 : Posti alloggio in residenze - di cui riservati ad uso foresteria
7 : Mense attive a gestione diretta
8 : Posti a sedere in mense a gestione diretta
9 : Mense attive a gestione indiretta
10: Posti a sedere in mense a gestione indiretta

Nell'utilizzo dei dati porre particolare attenzione ad evitare duplicazioni, dopo aver letto accuratamente le descrizioni dei codici.
In particolare fare attenzione ai valori indicati come ""di cui…"", già ricompresi nella voce principale.

</rdfs:comment>
    <rdfs:isDefinedBy rdf:resource="https://w3id.org/italia/onto/HER"/>
    <rdfs:label xml:lang="it">Classe di servizio mensa riportata da USTAT</rdfs:label>
    <rdfs:label xml:lang="en">USTAT Reported Canteen Service Class</rdfs:label>
    <owl:versionInfo xml:lang="it">stabile</owl:versionInfo>
    <owl:versionInfo xml:lang="en">stable</owl:versionInfo>
  </rdf:Description>
  <rdf:Description rdf:about="https://w3id.org/italia/onto/HER/hasEnrollment">
    <rdf:type rdf:resource="http://www.w3.org/2002/07/owl#ObjectProperty"/>
    <rdfs:domain rdf:resource="https://w3id.org/italia/onto/HER/USTATEnrolledStudentsAggregate"/>
    <rdfs:range rdf:resource="https://w3id.org/italia/onto/HER/USTATEnrollment"/>
    <rdfs:comment xml:lang="it">Questa proprietà collega l'informazione sugli studenti iscritti degli atenei in regola con il pagamento delle tasse universitarie all'informazione sulle tipologie di iscrizione.</rdfs:comment>
    <rdfs:comment xml:lang="en">This property links information on enrolled students of universities in good standing with the payment of tuition fees to information on the types of enrollment.</rdfs:comment>
    <rdfs:isDefinedBy rdf:resource="https://w3id.org/italia/onto/HER"/>
    <rdfs:label xml:lang="it">ha  iscrizione</rdfs:label>
    <rdfs:label xml:lang="en">has enrollment</rdfs:label>
    <owl:versionInfo xml:lang="it">stabile</owl:versionInfo>
    <owl:versionInfo xml:lang="en">stable</owl:versionInfo>
  </rdf:Description>
  <rdf:Description rdf:nodeID="n5bb3bff42afb4ca286d2c3fead9507ddb282">
    <rdf:first rdf:resource="https://w3id.org/italia/onto/HER/EUREKAProject"/>
    <rdf:rest rdf:nodeID="n5bb3bff42afb4ca286d2c3fead9507ddb283"/>
  </rdf:Description>
  <rdf:Description rdf:nodeID="n5bb3bff42afb4ca286d2c3fead9507ddb109">
    <rdf:type rdf:resource="http://www.w3.org/2002/07/owl#Class"/>
    <owl:unionOf rdf:nodeID="n5bb3bff42afb4ca286d2c3fead9507ddb110"/>
  </rdf:Description>
  <rdf:Description rdf:about="https://w3id.org/italia/onto/HER/ageClass">
    <rdf:type rdf:resource="http://www.w3.org/2002/07/owl#DatatypeProperty"/>
    <rdfs:domain rdf:resource="https://w3id.org/italia/onto/HER/USTATStaffByGender"/>
    <rdfs:range rdf:resource="http://www.w3.org/2000/01/rdf-schema#Literal"/>
    <rdfs:comment xml:lang="en">Age classes of teaching/researcher staff. Currently can take the following values: &lt;35; 35 - 44; 45 -54; &gt;=55</rdfs:comment>
    <rdfs:comment xml:lang="it">Età in classi del personale docente/ricercatore. Attualmente può assumere i seguenti valori: &lt;35; 35 - 44; 45 -54; &gt;=55</rdfs:comment>
    <rdfs:isDefinedBy rdf:resource="https://w3id.org/italia/onto/HER"/>
    <rdfs:label xml:lang="en">age class</rdfs:label>
    <rdfs:label xml:lang="it">classe di etá</rdfs:label>
    <owl:versionInfo xml:lang="it">stabile</owl:versionInfo>
    <owl:versionInfo xml:lang="en">stable</owl:versionInfo>
  </rdf:Description>
  <rdf:Description rdf:nodeID="n5bb3bff42afb4ca286d2c3fead9507ddb308">
    <rdf:first rdf:resource="https://w3id.org/italia/onto/HER/USTATInterventionsForStudentsByUniversitiesAggregate"/>
    <rdf:rest rdf:nodeID="n5bb3bff42afb4ca286d2c3fead9507ddb309"/>
  </rdf:Description>
  <rdf:Description rdf:about="https://w3id.org/italia/onto/HER/numberOfBeneficiaries">
    <rdf:type rdf:resource="http://www.w3.org/2002/07/owl#DatatypeProperty"/>
    <rdfs:domain rdf:resource="https://w3id.org/italia/onto/HER/CTNPRINInitiative"/>
    <rdfs:range rdf:resource="http://www.w3.org/2001/XMLSchema#int"/>
    <rdfs:comment xml:lang="it">Numero totale di proponenti di proposte finanziate (beneficiari dei finanziamenti). NB: se un unico beneficiario è presente in più proposte finanziate viene contato tante volte quante sono le proposte in cui appare</rdfs:comment>
    <rdfs:comment xml:lang="en">Total number of proposers of funded proposals (beneficiaries of funding). NB: if a single beneficiary is present in several funded proposals it is counted as many times as the number of proposals in which it appears</rdfs:comment>
    <rdfs:isDefinedBy rdf:resource="https://w3id.org/italia/onto/HER"/>
    <rdfs:label xml:lang="en">number of beneficiaries</rdfs:label>
    <rdfs:label xml:lang="it">numero di beneficiari</rdfs:label>
    <owl:versionInfo xml:lang="it">stabile</owl:versionInfo>
    <owl:versionInfo xml:lang="en">stable</owl:versionInfo>
  </rdf:Description>
  <rdf:Description rdf:about="https://w3id.org/italia/onto/HER/ItalianPhDCourse">
    <rdf:type rdf:resource="http://www.w3.org/2002/07/owl#Class"/>
    <rdfs:subClassOf rdf:resource="https://w3id.org/italia/onto/HER/PhDCourse"/>
    <rdfs:comment xml:lang="en">A PhD courses provided by an Italian university.</rdfs:comment>
    <rdfs:comment xml:lang="it">Un corso di dottorato di ricerca previsot da un'universitá italiana.</rdfs:comment>
    <rdfs:isDefinedBy rdf:resource="https://w3id.org/italia/onto/HER"/>
    <rdfs:label xml:lang="it">Corso di Dottorato Italiano</rdfs:label>
    <rdfs:label xml:lang="en">Italian PhD Course</rdfs:label>
    <owl:versionInfo xml:lang="it">stabile</owl:versionInfo>
    <owl:versionInfo xml:lang="en">stable</owl:versionInfo>
  </rdf:Description>
  <rdf:Description rdf:about="https://w3id.org/italia/onto/HER/acceptsHealthyVolunteers">
    <rdf:type rdf:resource="http://www.w3.org/2002/07/owl#DatatypeProperty"/>
    <rdf:type rdf:resource="http://www.w3.org/2002/07/owl#FunctionalProperty"/>
    <rdfs:domain rdf:resource="https://w3id.org/italia/onto/HER/AACTEligibility"/>
    <rdfs:range rdf:resource="http://www.w3.org/2001/XMLSchema#boolean"/>
    <rdfs:comment xml:lang="it">I partecipanti che non hanno una malattia o una condizione, o condizioni o sintomi correlati</rdfs:comment>
    <rdfs:comment xml:lang="en">Participants do not have a disease or condition, or related conditions or symptoms</rdfs:comment>
    <rdfs:isDefinedBy rdf:resource="https://w3id.org/italia/onto/HER"/>
    <rdfs:label xml:lang="it">Volontari sani</rdfs:label>
    <rdfs:label xml:lang="en">healthy volunteers</rdfs:label>
    <owl:versionInfo xml:lang="it">provvisoria</owl:versionInfo>
    <owl:versionInfo xml:lang="en">unstable</owl:versionInfo>
  </rdf:Description>
  <rdf:Description rdf:nodeID="n5bb3bff42afb4ca286d2c3fead9507ddb211">
    <rdf:first rdf:resource="https://w3id.org/italia/onto/HER/MIURStudentsByDegreeDegreeClassAggregate"/>
    <rdf:rest rdf:nodeID="n5bb3bff42afb4ca286d2c3fead9507ddb212"/>
  </rdf:Description>
  <rdf:Description rdf:about="https://w3id.org/italia/onto/HER/USTATTAStaffByGender">
    <rdf:type rdf:resource="http://www.w3.org/2002/07/owl#Class"/>
    <rdfs:subClassOf rdf:resource="https://w3id.org/italia/onto/HER/StatisticalDataAggregation"/>
    <rdfs:comment xml:lang="en">Data on the careers of technical-administrative staff from a gender perspective. The data concern technical-administrative personnel with permanent and fixed-term contracts and are broken down by gender, university, geographical area, type of contract and functional area. The data are available from 2012.</rdfs:comment>
    <rdfs:comment xml:lang="it">Dati sulle carriere del personale tecnico-amministrativo in un'ottica di genere. I dati riguardano il personale tecnico-amministrativo con contratto a tempo indeterminato e determinato e sono disaggregati per genere, ateneo, area geografica, tipologia di contratto e area funzionale. I dati sono disponibili a partire dal 2012.</rdfs:comment>
    <rdfs:isDefinedBy rdf:resource="https://w3id.org/italia/onto/HER"/>
    <rdfs:label xml:lang="it">Aggregazione di Staff TA per genere riportato da USTAT</rdfs:label>
    <rdfs:label xml:lang="en">USTAT Reported Aggregate of TA Staff By Sex</rdfs:label>
    <owl:versionInfo xml:lang="it">stabile</owl:versionInfo>
    <owl:versionInfo xml:lang="en">stable</owl:versionInfo>
  </rdf:Description>
  <rdf:Description rdf:nodeID="n5bb3bff42afb4ca286d2c3fead9507ddb462">
    <rdf:type rdf:resource="http://www.w3.org/2002/07/owl#Restriction"/>
    <owl:onProperty rdf:resource="https://w3id.org/italia/onto/HER/eurekaOrgType"/>
    <owl:cardinality rdf:datatype="http://www.w3.org/2001/XMLSchema#nonNegativeInteger">1</owl:cardinality>
  </rdf:Description>
  <rdf:Description rdf:nodeID="n5bb3bff42afb4ca286d2c3fead9507ddb504">
    <rdf:type rdf:resource="http://www.w3.org/2002/07/owl#Restriction"/>
    <owl:onProperty rdf:resource="https://w3id.org/italia/onto/HER/patentPriorityNo"/>
    <owl:cardinality rdf:datatype="http://www.w3.org/2001/XMLSchema#nonNegativeInteger">1</owl:cardinality>
  </rdf:Description>
  <rdf:Description rdf:nodeID="n5bb3bff42afb4ca286d2c3fead9507ddb537">
    <rdf:type rdf:resource="http://www.w3.org/2002/07/owl#Restriction"/>
    <owl:onProperty rdf:resource="https://w3id.org/italia/onto/l0/description"/>
    <owl:someValuesFrom rdf:resource="http://www.w3.org/2000/01/rdf-schema#Literal"/>
  </rdf:Description>
  <rdf:Description rdf:nodeID="n5bb3bff42afb4ca286d2c3fead9507ddb111">
    <rdf:first rdf:resource="https://w3id.org/italia/onto/HER/USTATTemporaryStaff"/>
    <rdf:rest rdf:resource="http://www.w3.org/1999/02/22-rdf-syntax-ns#nil"/>
  </rdf:Description>
  <rdf:Description rdf:nodeID="n5bb3bff42afb4ca286d2c3fead9507ddb433">
    <rdf:type rdf:resource="http://www.w3.org/2002/07/owl#Restriction"/>
    <owl:onProperty rdf:resource="https://w3id.org/italia/onto/HER/hasAACTStudy"/>
    <owl:qualifiedCardinality rdf:datatype="http://www.w3.org/2001/XMLSchema#nonNegativeInteger">1</owl:qualifiedCardinality>
    <owl:onClass rdf:resource="https://w3id.org/italia/onto/HER/AACTStudy"/>
  </rdf:Description>
  <rdf:Description rdf:about="https://w3id.org/italia/onto/HER/hasParticipationCountry">
    <rdf:type rdf:resource="http://www.w3.org/2002/07/owl#ObjectProperty"/>
    <rdfs:domain rdf:nodeID="n5bb3bff42afb4ca286d2c3fead9507ddb76"/>
    <rdfs:range rdf:resource="https://w3id.org/italia/onto/CLV/Country"/>
    <rdfs:comment xml:lang="it">Questa proprietà si collega a un Paese.</rdfs:comment>
    <rdfs:comment xml:lang="en">This property links to a Country.</rdfs:comment>
    <rdfs:isDefinedBy rdf:resource="https://w3id.org/italia/onto/HER"/>
    <rdfs:label xml:lang="it">ha un pease</rdfs:label>
    <rdfs:label xml:lang="en">has country</rdfs:label>
    <owl:versionInfo xml:lang="it">provvisoria - da verificare</owl:versionInfo>
    <owl:versionInfo xml:lang="en">unstable</owl:versionInfo>
  </rdf:Description>
  <rdf:Description rdf:nodeID="n5bb3bff42afb4ca286d2c3fead9507ddb471">
    <rdf:type rdf:resource="http://www.w3.org/2002/07/owl#Restriction"/>
    <owl:onProperty rdf:resource="https://w3id.org/italia/onto/HER/startingYear"/>
    <owl:qualifiedCardinality rdf:datatype="http://www.w3.org/2001/XMLSchema#nonNegativeInteger">1</owl:qualifiedCardinality>
    <owl:onDataRange rdf:resource="http://www.w3.org/2001/XMLSchema#gYear"/>
  </rdf:Description>
  <rdf:Description rdf:about="https://w3id.org/italia/onto/HER/shortTitle">
    <rdf:type rdf:resource="http://www.w3.org/2002/07/owl#DatatypeProperty"/>
    <rdfs:domain rdf:resource="https://w3id.org/italia/onto/HER/AACTStudy"/>
    <rdfs:range rdf:resource="http://www.w3.org/2000/01/rdf-schema#Literal"/>
    <rdfs:comment xml:lang="en">A short title of the clinical study written in language intended for the lay public. The title should include, where possible, information on the participants, condition being evaluated, and intervention(s) studied.</rdfs:comment>
    <rdfs:comment xml:lang="it">Un breve titolo dello studio clinico scritto in un linguaggio destinato al pubblico laico. Il titolo dovrebbe includere, ove possibile, informazioni sui partecipanti, sulla condizione in corso di valutazione e sugli interventi studiati.</rdfs:comment>
    <rdfs:isDefinedBy rdf:resource="https://w3id.org/italia/onto/HER"/>
    <rdfs:label xml:lang="en">short title</rdfs:label>
    <rdfs:label xml:lang="it">titolo breve</rdfs:label>
    <owl:versionInfo xml:lang="it">stabile</owl:versionInfo>
    <owl:versionInfo xml:lang="en">stable</owl:versionInfo>
  </rdf:Description>
  <rdf:Description rdf:about="https://w3id.org/italia/onto/HER/ErasmusPlusParticipant">
    <rdf:type rdf:resource="http://www.w3.org/2002/07/owl#Class"/>
    <rdfs:subClassOf rdf:resource="https://w3id.org/italia/onto/RO/TimeIndexedRole"/>
    <rdfs:subClassOf rdf:nodeID="n5bb3bff42afb4ca286d2c3fead9507ddb477"/>
    <rdfs:subClassOf rdf:nodeID="n5bb3bff42afb4ca286d2c3fead9507ddb478"/>
    <rdfs:subClassOf rdf:nodeID="n5bb3bff42afb4ca286d2c3fead9507ddb479"/>
    <rdfs:subClassOf rdf:nodeID="n5bb3bff42afb4ca286d2c3fead9507ddb480"/>
    <rdfs:subClassOf rdf:nodeID="n5bb3bff42afb4ca286d2c3fead9507ddb481"/>
    <rdfs:comment xml:lang="en">It refers to the entities which are involved in the Erasmus+ projects.
The entities could be both universities and private organizations.</rdfs:comment>
    <rdfs:comment xml:lang="it">Si riferisce alle entità coinvolte nei progetti Erasmus+.
Le entità potrebbero essere sia università che organizzazioni private.</rdfs:comment>
    <rdfs:isDefinedBy rdf:resource="https://w3id.org/italia/onto/HER"/>
    <rdfs:label xml:lang="en">Erasmus+ Participant</rdfs:label>
    <rdfs:label xml:lang="it">Partecipante Erasmus+</rdfs:label>
    <owl:versionInfo xml:lang="it">stabile</owl:versionInfo>
    <owl:versionInfo xml:lang="en">stable</owl:versionInfo>
  </rdf:Description>
  <rdf:Description rdf:about="https://w3id.org/italia/onto/HER/hasCountryInvolvement">
    <rdf:type rdf:resource="http://www.w3.org/2002/07/owl#ObjectProperty"/>
    <rdfs:domain rdf:resource="https://w3id.org/italia/onto/HER/AACTStudy"/>
    <rdfs:range rdf:resource="https://w3id.org/italia/onto/HER/CountryInvolvement"/>
    <rdfs:comment xml:lang="en">Country where the facility conducting a clinical protocol is located</rdfs:comment>
    <rdfs:comment xml:lang="it">Paese in cui si trova la struttura che conduce un protocollo clinico</rdfs:comment>
    <rdfs:isDefinedBy rdf:resource="https://w3id.org/italia/onto/HER"/>
    <rdfs:label xml:lang="it">ha coinvolgimento del paese</rdfs:label>
    <rdfs:label xml:lang="en">has country involvement</rdfs:label>
    <owl:versionInfo xml:lang="it">stabile</owl:versionInfo>
    <owl:versionInfo xml:lang="en">stable</owl:versionInfo>
  </rdf:Description>
  <rdf:Description rdf:nodeID="n5bb3bff42afb4ca286d2c3fead9507ddb439">
    <rdf:type rdf:resource="http://www.w3.org/2002/07/owl#Restriction"/>
    <owl:onProperty rdf:resource="https://w3id.org/italia/onto/HER/hasParticipationCountry"/>
    <owl:allValuesFrom rdf:resource="https://w3id.org/italia/onto/CLV/Country"/>
  </rdf:Description>
  <rdf:Description rdf:about="https://w3id.org/italia/onto/HER/AACTIntervention">
    <rdf:type rdf:resource="http://www.w3.org/2002/07/owl#Class"/>
    <rdfs:subClassOf rdf:resource="https://w3id.org/italia/onto/l0/Activity"/>
    <rdfs:comment xml:lang="en">A process or action that is the focus of a clinical study. Interventions include drugs, medical devices, procedures, vaccines, and other products that are either investigational or already available. Interventions can also include noninvasive approaches, such as education or modifying diet and exercise.</rdfs:comment>
    <rdfs:comment xml:lang="it">Un processo o un'azione che è il fulcro di uno studio clinico. Gli interventi comprendono farmaci, dispositivi medici, procedure, vaccini e altri prodotti che sono in fase di sperimentazione o già disponibili. Gli interventi possono anche includere approcci non invasivi, come l'educazione o la modifica della dieta e dell'esercizio fisico.</rdfs:comment>
    <rdfs:isDefinedBy rdf:resource="https://w3id.org/italia/onto/HER"/>
    <rdfs:label xml:lang="en">AACT Intervention</rdfs:label>
    <rdfs:label xml:lang="it">Intervento AACT</rdfs:label>
    <owl:versionInfo xml:lang="it">stabile</owl:versionInfo>
    <owl:versionInfo xml:lang="en">stable</owl:versionInfo>
  </rdf:Description>
  <rdf:Description rdf:about="https://w3id.org/italia/data/private-organization/03033080213">
    <rdf:type rdf:resource="http://www.w3.org/2002/07/owl#NamedIndividual"/>
    <rdf:type rdf:resource="http://dati.gov.it/onto/dcatapit#Agent"/>
    <rdf:type rdf:resource="http://xmlns.com/foaf/0.1/Agent"/>
    <ns2:identifier>03033080213</ns2:identifier>
    <ns5:name xml:lang="en">ONTOPIC</ns5:name>
    <ns5:name xml:lang="it">ONTOPIC</ns5:name>
  </rdf:Description>
  <rdf:Description rdf:nodeID="n5bb3bff42afb4ca286d2c3fead9507ddb230">
    <rdf:first rdf:resource="https://w3id.org/italia/onto/HER/MIURStudentsByRegionOfResidenceDegreeDegreeClassAggregate"/>
    <rdf:rest rdf:resource="http://www.w3.org/1999/02/22-rdf-syntax-ns#nil"/>
  </rdf:Description>
  <rdf:Description rdf:about="https://w3id.org/italia/onto/HER/finalBalance">
    <rdf:type rdf:resource="http://www.w3.org/2002/07/owl#DatatypeProperty"/>
    <rdfs:subPropertyOf rdf:resource="https://w3id.org/italia/onto/MU/value"/>
    <rdfs:domain rdf:resource="https://w3id.org/italia/onto/HER/USTATContributionRevenue"/>
    <rdfs:range rdf:resource="http://www.w3.org/2001/XMLSchema#decimal"/>
    <rdfs:comment xml:lang="en">Amount of the final balance. The values are expressed in EURO. The final balance refers to the year (T-1).</rdfs:comment>
    <rdfs:comment xml:lang="it">Importo del conto consuntivo. I valori sono espressi in EURO. Il conto consuntivo fa riferimento all'anno (T-1).</rdfs:comment>
    <rdfs:isDefinedBy rdf:resource="https://w3id.org/italia/onto/HER"/>
    <rdfs:label xml:lang="it">bilancio finale</rdfs:label>
    <rdfs:label xml:lang="en">final balance</rdfs:label>
    <owl:versionInfo xml:lang="it">stabile</owl:versionInfo>
    <owl:versionInfo xml:lang="en">stable</owl:versionInfo>
  </rdf:Description>
  <rdf:Description rdf:about="https://w3id.org/italia/onto/HER/OTH">
    <rdf:type rdf:resource="http://www.w3.org/2002/07/owl#NamedIndividual"/>
    <rdf:type rdf:resource="https://w3id.org/italia/onto/HER/ECActivityType"/>
    <rdfs:isDefinedBy rdf:resource="https://w3id.org/italia/onto/HER"/>
    <rdfs:label xml:lang="en">Other</rdfs:label>
    <owl:versionInfo xml:lang="it">stabile</owl:versionInfo>
    <owl:versionInfo xml:lang="en">stable</owl:versionInfo>
  </rdf:Description>
  <rdf:Description rdf:nodeID="n5bb3bff42afb4ca286d2c3fead9507ddb215">
    <rdf:first rdf:resource="https://w3id.org/italia/onto/HER/MIURStudentsByProvinceOfResidenceDegreeDegreeClassAggregate"/>
    <rdf:rest rdf:nodeID="n5bb3bff42afb4ca286d2c3fead9507ddb216"/>
  </rdf:Description>
  <rdf:Description rdf:about="https://w3id.org/italia/onto/HER/revoked">
    <rdf:type rdf:resource="http://www.w3.org/2002/07/owl#DatatypeProperty"/>
    <rdf:type rdf:resource="http://www.w3.org/2002/07/owl#FunctionalProperty"/>
    <rdfs:domain rdf:resource="https://w3id.org/italia/onto/HER/CTNPRINOperation"/>
    <rdfs:range rdf:resource="http://www.w3.org/2001/XMLSchema#boolean"/>
    <rdfs:comment xml:lang="it">Questa proprietà è vera solo se il progetto è stato revocato e può assumere i valori "parzialmente" o "totalmente"</rdfs:comment>
    <rdfs:comment xml:lang="en">The value is true only if the project has been revoked and it can assume the values "partially" or "totally".</rdfs:comment>
    <rdfs:isDefinedBy rdf:resource="https://w3id.org/italia/onto/HER"/>
    <rdfs:label xml:lang="it">revocata</rdfs:label>
    <rdfs:label xml:lang="en">revoked</rdfs:label>
    <owl:versionInfo xml:lang="it">stabile</owl:versionInfo>
    <owl:versionInfo xml:lang="en">stable</owl:versionInfo>
  </rdf:Description>
  <rdf:Description rdf:nodeID="n5bb3bff42afb4ca286d2c3fead9507ddb301">
    <rdf:first rdf:resource="https://w3id.org/italia/onto/HER/USTATTemporaryStaff"/>
    <rdf:rest rdf:nodeID="n5bb3bff42afb4ca286d2c3fead9507ddb302"/>
  </rdf:Description>
  <rdf:Description rdf:nodeID="n5bb3bff42afb4ca286d2c3fead9507ddb196">
    <rdf:first rdf:resource="https://w3id.org/italia/onto/HER/MIURStudentsByCitizenshipDegreeClassAggregate"/>
    <rdf:rest rdf:nodeID="n5bb3bff42afb4ca286d2c3fead9507ddb197"/>
  </rdf:Description>
  <rdf:Description rdf:about="https://w3id.org/italia/onto/HER/hasFundingDSUOrg">
    <rdf:type rdf:resource="http://www.w3.org/2002/07/owl#ObjectProperty"/>
    <rdfs:domain rdf:resource="http://www.w3.org/2002/07/owl#Thing"/>
    <rdfs:range rdf:nodeID="n5bb3bff42afb4ca286d2c3fead9507ddb61"/>
    <rdfs:comment xml:lang="it">Questa proprietà collega qualunque cosa nel dominio inclusi gli interventi a favore degli studenti all'Ente o ufficio per il Diritto allo Studio Universitario (DSU) corrispondente.</rdfs:comment>
    <rdfs:comment xml:lang="en">This property links things including the interventions in favour of students to the corresponding Institution or Office for the Right to University Studies (DSU).</rdfs:comment>
    <rdfs:isDefinedBy rdf:resource="https://w3id.org/italia/onto/HER"/>
    <rdfs:label xml:lang="it">ha ente finanziatore di diritto allo studio</rdfs:label>
    <rdfs:label xml:lang="en">has funding DSU organisation</rdfs:label>
    <owl:versionInfo xml:lang="it">stabile</owl:versionInfo>
    <owl:versionInfo xml:lang="en">stable</owl:versionInfo>
  </rdf:Description>
  <rdf:Description rdf:nodeID="n5bb3bff42afb4ca286d2c3fead9507ddb200">
    <rdf:first rdf:resource="https://w3id.org/italia/onto/HER/MIURStudentsByDiplomaDegreeDegreeClassAggregate"/>
    <rdf:rest rdf:nodeID="n5bb3bff42afb4ca286d2c3fead9507ddb201"/>
  </rdf:Description>
  <rdf:Description rdf:about="https://w3id.org/italia/onto/HER/USTATReportedUniversityFacilityType">
    <rdf:type rdf:resource="http://www.w3.org/2002/07/owl#Class"/>
    <rdfs:subClassOf rdf:resource="https://w3id.org/italia/onto/l0/Characteristic"/>
    <rdfs:subClassOf rdf:nodeID="n5bb3bff42afb4ca286d2c3fead9507ddb537"/>
    <rdfs:subClassOf rdf:nodeID="n5bb3bff42afb4ca286d2c3fead9507ddb538"/>
    <rdfs:comment xml:lang="it">Strutture degli atenei: mense e posti alloggio direttamente gestiti dagli Atenei.</rdfs:comment>
    <rdfs:comment xml:lang="en">University structures: canteens and accommodation places directly managed by the universities.</rdfs:comment>
    <rdfs:isDefinedBy rdf:resource="https://w3id.org/italia/onto/HER"/>
    <rdfs:label xml:lang="it">Tipo struttura universitá riportata da USTAT</rdfs:label>
    <rdfs:label xml:lang="en">USTAT Reported Facility of University Type</rdfs:label>
    <owl:versionInfo xml:lang="it">stabile</owl:versionInfo>
    <owl:versionInfo xml:lang="en">stable</owl:versionInfo>
  </rdf:Description>
  <rdf:Description rdf:about="https://w3id.org/italia/onto/HER/founderShareholding">
    <rdf:type rdf:resource="http://www.w3.org/2002/07/owl#DatatypeProperty"/>
    <rdfs:domain rdf:resource="https://w3id.org/italia/onto/HER/Spinoff"/>
    <rdfs:range rdf:resource="http://www.w3.org/2001/XMLSchema#decimal"/>
    <rdfs:comment xml:lang="it">Indica la participazione azionaria  (in percentuale) dell'Università o dell'ente di ricerca di origine al momento della fondazione dello spin-off.</rdfs:comment>
    <rdfs:comment xml:lang="en">It indicates the shareholding (in percentage) of the university or research institution of origin at the time of the foundation of the spin-off.</rdfs:comment>
    <rdfs:isDefinedBy rdf:resource="https://w3id.org/italia/onto/HER"/>
    <rdfs:label xml:lang="en">founder shareholding</rdfs:label>
    <rdfs:label xml:lang="it">partecipazione azionaria fondatore</rdfs:label>
    <owl:versionInfo xml:lang="it">stabile</owl:versionInfo>
    <owl:versionInfo xml:lang="en">stable</owl:versionInfo>
  </rdf:Description>
  <rdf:Description rdf:about="https://w3id.org/italia/onto/l0/Activity">
    <rdf:type rdf:resource="http://www.w3.org/2002/07/owl#Class"/>
  </rdf:Description>
  <rdf:Description rdf:nodeID="n5bb3bff42afb4ca286d2c3fead9507ddb423">
    <rdf:type rdf:resource="http://www.w3.org/2002/07/owl#Restriction"/>
    <owl:onProperty rdf:resource="https://w3id.org/italia/onto/HER/hasCTNPRINAmount"/>
    <owl:allValuesFrom rdf:resource="https://w3id.org/italia/onto/HER/CTNPRINAmount"/>
  </rdf:Description>
  <rdf:Description rdf:nodeID="n5bb3bff42afb4ca286d2c3fead9507ddb475">
    <rdf:type rdf:resource="http://www.w3.org/2002/07/owl#Restriction"/>
    <owl:onProperty rdf:resource="https://w3id.org/italia/onto/l0/name"/>
    <owl:allValuesFrom rdf:resource="http://www.w3.org/2000/01/rdf-schema#Literal"/>
  </rdf:Description>
  <rdf:Description rdf:nodeID="n5bb3bff42afb4ca286d2c3fead9507ddb491">
    <rdf:type rdf:resource="http://www.w3.org/2002/07/owl#Restriction"/>
    <owl:onProperty rdf:resource="https://w3id.org/italia/onto/HER/totalGrant"/>
    <owl:maxQualifiedCardinality rdf:datatype="http://www.w3.org/2001/XMLSchema#nonNegativeInteger">1</owl:maxQualifiedCardinality>
    <owl:onDataRange rdf:resource="http://www.w3.org/2001/XMLSchema#decimal"/>
  </rdf:Description>
  <rdf:Description rdf:about="https://w3id.org/italia/onto/HER/hasUSTATExpenseClass">
    <rdf:type rdf:resource="http://www.w3.org/2002/07/owl#ObjectProperty"/>
    <rdfs:domain rdf:nodeID="n5bb3bff42afb4ca286d2c3fead9507ddb96"/>
    <rdfs:range rdf:nodeID="n5bb3bff42afb4ca286d2c3fead9507ddb99"/>
    <rdfs:comment xml:lang="it">Questa proprietà collega l'informazione sui dati relativi alla spesa per interventi a favore degli studenti degli atenei (solo prestiti a studenti) alla tipologia di spesa corrispondente.</rdfs:comment>
    <rdfs:comment xml:lang="en">This property links the information on expenses for interventions in favour of university students (student loans only) to the corresponding type of expenses.</rdfs:comment>
    <rdfs:isDefinedBy rdf:resource="https://w3id.org/italia/onto/HER"/>
    <rdfs:label xml:lang="it">ha una classe di spesa</rdfs:label>
    <rdfs:label xml:lang="en">has expense class</rdfs:label>
    <owl:versionInfo xml:lang="it">stabile</owl:versionInfo>
    <owl:versionInfo xml:lang="en">stable</owl:versionInfo>
  </rdf:Description>
  <rdf:Description rdf:nodeID="n5bb3bff42afb4ca286d2c3fead9507ddb288">
    <rdf:type rdf:resource="http://www.w3.org/1999/02/22-rdf-syntax-ns#List"/>
    <rdf:first>Cross-Sectional, Retrospective/Prospective</rdf:first>
    <rdf:rest rdf:nodeID="n5bb3bff42afb4ca286d2c3fead9507ddb289"/>
  </rdf:Description>
  <rdf:Description rdf:about="https://w3id.org/italia/onto/HER/planToShareIPD">
    <rdf:type rdf:resource="http://www.w3.org/2002/07/owl#DatatypeProperty"/>
    <rdfs:domain rdf:resource="https://w3id.org/italia/onto/HER/AACTStudy"/>
    <rdfs:range rdf:nodeID="n5bb3bff42afb4ca286d2c3fead9507ddb250"/>
    <rdfs:comment xml:lang="en">Define whether there is a plan to make individual participant data (IPD) collected in this study, including data dictionaries, available to other researchers (typically after the end of the study). Options are:
Yes: There is a plan to make IPD and related data dictionaries available.
No: There is not a plan to make IPD available.
Undecided: It is not yet known if there will be a plan to make IPD available.
</rdfs:comment>
    <rdfs:comment xml:lang="it">Definire se esiste un piano per mettere a disposizione di altri ricercatori (in genere dopo la fine dello studio) i dati dei singoli partecipanti (IPD) raccolti in questo studio, compresi i dizionari dei dati. Le opzioni sono:
Sì: esiste un piano per rendere disponibili i dizionari IPD e i relativi dizionari di dati.
No: non esiste un piano per rendere disponibile l'IPD.
Indeciso: Non si sa ancora se ci sarà un piano per rendere disponibile l'IPD.</rdfs:comment>
    <rdfs:isDefinedBy rdf:resource="https://w3id.org/italia/onto/HER"/>
    <rdfs:label xml:lang="it">piano per condivisione PDPI</rdfs:label>
    <rdfs:label xml:lang="en">plan to share IPD</rdfs:label>
    <owl:versionInfo xml:lang="it">stabile</owl:versionInfo>
    <owl:versionInfo xml:lang="en">stable</owl:versionInfo>
  </rdf:Description>
  <rdf:Description rdf:about="https://w3id.org/italia/onto/HER/patentPriorityNo">
    <rdf:type rdf:resource="http://www.w3.org/2002/07/owl#DatatypeProperty"/>
    <rdfs:subPropertyOf rdf:resource="https://w3id.org/italia/onto/l0/identifier"/>
    <rdfs:domain rdf:resource="https://w3id.org/italia/onto/HER/PatentPriorityDetail"/>
    <rdfs:range rdf:resource="http://www.w3.org/2000/01/rdf-schema#Literal"/>
    <rdfs:comment xml:lang="it">Il numero della domanda per la quale viene richiesta una data di priorità. È quindi uguale al numero di domanda del documento di priorità richiesto. Il numero di priorità è costituito da un codice paese (due lettere), l'anno di deposito (quattro cifre) e un numero seriale (variabile, sette cifre).</rdfs:comment>
    <rdfs:comment xml:lang="en">The number of the application for which a priority date is claimed. It is therefore the same as the application number of the claimed priority document. The priority number is made up of a country code (two letters), the year of filing (four digits) and a serial number (variable, seven digits).
</rdfs:comment>
    <rdfs:isDefinedBy rdf:resource="https://w3id.org/italia/onto/HER"/>
    <rdfs:label xml:lang="it">numero di prioritá brevetto</rdfs:label>
    <rdfs:label xml:lang="en">patent priority number</rdfs:label>
    <owl:versionInfo xml:lang="it">stabile</owl:versionInfo>
    <owl:versionInfo xml:lang="en">stable</owl:versionInfo>
  </rdf:Description>
  <rdf:Description rdf:nodeID="n5bb3bff42afb4ca286d2c3fead9507ddb493">
    <rdf:type rdf:resource="http://www.w3.org/2002/07/owl#Restriction"/>
    <owl:onProperty rdf:resource="https://w3id.org/italia/onto/l0/identifier"/>
    <owl:cardinality rdf:datatype="http://www.w3.org/2001/XMLSchema#nonNegativeInteger">1</owl:cardinality>
  </rdf:Description>
  <rdf:Description rdf:about="https://w3id.org/italia/onto/HER/hasResultsFirstPostedDate">
    <rdf:type rdf:resource="http://www.w3.org/2002/07/owl#ObjectProperty"/>
    <rdfs:subPropertyOf rdf:resource="https://w3id.org/italia/onto/TI/hasTemporalEntity"/>
    <rdfs:domain rdf:resource="https://w3id.org/italia/onto/HER/AACTStudy"/>
    <rdfs:range rdf:resource="https://w3id.org/italia/onto/TI#TimeInstant"/>
    <rdfs:comment xml:lang="it">Data in cui i risultati sono stati resi pubblici per la prima volta su ClinicalTrials.gov</rdfs:comment>
    <rdfs:comment xml:lang="en">Date on which results were first made public on ClinicalTrials.gov</rdfs:comment>
    <rdfs:isDefinedBy rdf:resource="https://w3id.org/italia/onto/HER"/>
    <rdfs:label xml:lang="it">ha risultati prima data pubblicazione</rdfs:label>
    <rdfs:label xml:lang="en">has results first posted date</rdfs:label>
    <owl:versionInfo xml:lang="it">prova</owl:versionInfo>
    <owl:versionInfo xml:lang="en">testing</owl:versionInfo>
  </rdf:Description>
  <rdf:Description rdf:nodeID="n5bb3bff42afb4ca286d2c3fead9507ddb463">
    <rdf:type rdf:resource="http://www.w3.org/2002/07/owl#Restriction"/>
    <owl:onProperty rdf:resource="https://w3id.org/italia/onto/HER/financialContribution"/>
    <owl:maxQualifiedCardinality rdf:datatype="http://www.w3.org/2001/XMLSchema#nonNegativeInteger">1</owl:maxQualifiedCardinality>
    <owl:onDataRange rdf:resource="http://www.w3.org/2001/XMLSchema#decimal"/>
  </rdf:Description>
  <rdf:Description rdf:about="https://w3id.org/italia/onto/HER/CTNPRINAmount">
    <rdf:type rdf:resource="http://www.w3.org/2002/07/owl#Class"/>
    <rdfs:subClassOf rdf:resource="https://w3id.org/italia/onto/MU/Value"/>
    <rdfs:subClassOf rdf:nodeID="n5bb3bff42afb4ca286d2c3fead9507ddb414"/>
    <rdfs:subClassOf rdf:nodeID="n5bb3bff42afb4ca286d2c3fead9507ddb415"/>
    <rdfs:comment xml:lang="it">Importi monetari allegati a un'operazione CTN/PRIN</rdfs:comment>
    <rdfs:comment xml:lang="en">Monetary amounts attached to a CTN/PRIN operation</rdfs:comment>
    <rdfs:isDefinedBy rdf:resource="https://w3id.org/italia/onto/HER"/>
    <rdfs:label xml:lang="it">Ammontare CTN/PRIN</rdfs:label>
    <rdfs:label xml:lang="en">CTN/PRIN Amount</rdfs:label>
    <owl:versionInfo xml:lang="it">stabile</owl:versionInfo>
    <owl:versionInfo xml:lang="en">stable</owl:versionInfo>
  </rdf:Description>
  <rdf:Description rdf:about="https://w3id.org/italia/onto/HER/totalFemaleEnrolled">
    <rdf:type rdf:resource="http://www.w3.org/2002/07/owl#DatatypeProperty"/>
    <rdfs:subPropertyOf rdf:resource="https://w3id.org/italia/onto/MU/value"/>
    <rdfs:domain rdf:resource="https://w3id.org/italia/onto/HER/USTATStudentsBySexAggregate"/>
    <rdfs:range rdf:resource="http://www.w3.org/2000/01/rdf-schema#Literal"/>
    <rdfs:comment xml:lang="en">Number of registered female students corresponding to the selected combination of variables. In particular: number of female students who, with reference to a.a. (t) - (t+1), are enrolled on July 31st of the year (t+1). Notes: Students of levels 6 and 7 of ISCED 2011. For the year 2018-2019: elaborations on ANS data - extraction December 2019.</rdfs:comment>
    <rdfs:comment xml:lang="it">Numero di studentesse di genere femminile iscritte corrispondente alla combinazione di variabili selezionata. In particolare: numero di studentesse che, con riferimento all' a.a. (t) - (t+1), risultano iscritte alla data del 31 luglio dell'anno (t+1). Note: Studentesse dei livelli 6 e 7 della ISCED 2011. Per l'anno 2018-2019: elaborazioni su dati ANS - estrazione Dicembre 2019.</rdfs:comment>
    <rdfs:isDefinedBy rdf:resource="https://w3id.org/italia/onto/HER"/>
    <rdfs:label xml:lang="en">total female enrolled</rdfs:label>
    <rdfs:label xml:lang="it">totale di genere femminile iscritto</rdfs:label>
    <owl:versionInfo xml:lang="it">stabile</owl:versionInfo>
    <owl:versionInfo xml:lang="en">stable</owl:versionInfo>
  </rdf:Description>
  <rdf:Description rdf:about="https://w3id.org/italia/onto/HER/ErasmusPlusFile">
    <rdf:type rdf:resource="http://www.w3.org/2002/07/owl#Class"/>
    <rdfs:subClassOf rdf:resource="https://w3id.org/italia/onto/l0/Object"/>
    <rdfs:subClassOf rdf:nodeID="n5bb3bff42afb4ca286d2c3fead9507ddb474"/>
    <rdfs:subClassOf rdf:nodeID="n5bb3bff42afb4ca286d2c3fead9507ddb475"/>
    <rdfs:subClassOf rdf:nodeID="n5bb3bff42afb4ca286d2c3fead9507ddb476"/>
    <rdfs:comment xml:lang="en">It refers to the output result file of an erasmus plus project.
The file tipycally is available by an url provided by the European Commission.</rdfs:comment>
    <rdfs:comment xml:lang="it">Si riferisce al file dei risultati di un progetto erasmus plus.
Il file è tipicamente disponibile tramite un url fornito dalla Commissione Europea.</rdfs:comment>
    <rdfs:isDefinedBy rdf:resource="https://w3id.org/italia/onto/HER"/>
    <rdfs:label xml:lang="en">Erasmus+ File</rdfs:label>
    <rdfs:label xml:lang="it">File Erasmus+</rdfs:label>
    <owl:versionInfo xml:lang="it">stabile</owl:versionInfo>
    <owl:versionInfo xml:lang="en">stable</owl:versionInfo>
  </rdf:Description>
  <rdf:Description rdf:nodeID="n5bb3bff42afb4ca286d2c3fead9507ddb430">
    <rdf:type rdf:resource="http://www.w3.org/2002/07/owl#Restriction"/>
    <owl:onProperty rdf:resource="https://w3id.org/italia/onto/HER/revocationDate"/>
    <owl:maxQualifiedCardinality rdf:datatype="http://www.w3.org/2001/XMLSchema#nonNegativeInteger">1</owl:maxQualifiedCardinality>
    <owl:onDataRange rdf:resource="http://www.w3.org/2001/XMLSchema#date"/>
  </rdf:Description>
  <rdf:Description rdf:about="https://w3id.org/italia/onto/HER/numberOfGroups">
    <rdf:type rdf:resource="http://www.w3.org/2002/07/owl#DatatypeProperty"/>
    <rdfs:domain rdf:resource="https://w3id.org/italia/onto/HER/AACTStudy"/>
    <rdfs:range rdf:resource="http://www.w3.org/2001/XMLSchema#int"/>
    <rdfs:comment xml:lang="en">number of Group/cohorts (group or subgroup of participants in an observational study that is assessed for biomedical or health outcomes).</rdfs:comment>
    <rdfs:comment xml:lang="it">numero di gruppi/coorte (gruppo o sottogruppo di partecipanti ad uno studio osservazionale che viene valutato per i risultati biomedici o sanitari).</rdfs:comment>
    <rdfs:isDefinedBy rdf:resource="https://w3id.org/italia/onto/HER"/>
    <rdfs:label xml:lang="en">number of groups</rdfs:label>
    <rdfs:label xml:lang="it">numero di gruppi</rdfs:label>
    <owl:versionInfo xml:lang="it">stabile</owl:versionInfo>
    <owl:versionInfo xml:lang="en">stable</owl:versionInfo>
  </rdf:Description>
  <rdf:Description rdf:about="https://w3id.org/italia/onto/HER/maskingDescription">
    <rdf:type rdf:resource="http://www.w3.org/2002/07/owl#DatatypeProperty"/>
    <rdfs:subPropertyOf rdf:resource="https://w3id.org/italia/onto/l0/description"/>
    <rdfs:domain rdf:resource="https://w3id.org/italia/onto/HER/AACTDesign"/>
    <rdfs:range rdf:resource="http://www.w3.org/2000/01/rdf-schema#Literal"/>
    <rdfs:comment xml:lang="it">Fornisce informazioni su altri soggetti che potrebbero essere oscurati nello studio clinico, se presenti.</rdfs:comment>
    <rdfs:comment xml:lang="en">Provide information about other parties who may be masked in the clinical trial, if any.</rdfs:comment>
    <rdfs:isDefinedBy rdf:resource="https://w3id.org/italia/onto/HER"/>
    <rdfs:label xml:lang="en">description of masking</rdfs:label>
    <rdfs:label xml:lang="it">descrizione mascheramento</rdfs:label>
    <owl:versionInfo xml:lang="it">stabile</owl:versionInfo>
    <owl:versionInfo xml:lang="en">stable</owl:versionInfo>
  </rdf:Description>
  <rdf:Description rdf:about="https://w3id.org/italia/onto/HER/hasPhdCourse">
    <rdf:type rdf:resource="http://www.w3.org/2002/07/owl#ObjectProperty"/>
    <rdfs:domain rdf:resource="https://w3id.org/italia/onto/HER/ItalianPhDCourseByCycle"/>
    <rdfs:range rdf:resource="https://w3id.org/italia/onto/HER/ItalianPhDCourse"/>
    <rdfs:comment xml:lang="it">Questa proprietà si collega ad un corso di dottorato di ricerca corrispondente.</rdfs:comment>
    <rdfs:comment xml:lang="en">This property links to a corresponding PhD course.</rdfs:comment>
    <rdfs:isDefinedBy rdf:resource="https://w3id.org/italia/onto/HER"/>
    <rdfs:label xml:lang="it">ha  corso di dottorato di ricerca</rdfs:label>
    <rdfs:label xml:lang="en">has phd course</rdfs:label>
    <owl:versionInfo xml:lang="it">stabile</owl:versionInfo>
    <owl:versionInfo xml:lang="en">stable</owl:versionInfo>
  </rdf:Description>
  <rdf:Description rdf:nodeID="n5bb3bff42afb4ca286d2c3fead9507ddb514">
    <rdf:type rdf:resource="http://www.w3.org/2002/07/owl#Restriction"/>
    <owl:onProperty rdf:resource="https://w3id.org/italia/onto/HER/hasOperationalSpinoffAddress"/>
    <owl:allValuesFrom rdf:resource="https://w3id.org/italia/onto/CLV/Address"/>
  </rdf:Description>
  <rdf:Description rdf:about="https://w3id.org/italia/onto/HER/USTATUniversityFacilitiesAggregate">
    <rdf:type rdf:resource="http://www.w3.org/2002/07/owl#Class"/>
    <rdfs:subClassOf rdf:resource="https://w3id.org/italia/onto/HER/StatisticalDataAggregation"/>
    <rdfs:subClassOf rdf:nodeID="n5bb3bff42afb4ca286d2c3fead9507ddb544"/>
    <rdfs:comment xml:lang="en">Data on the facilities of the universities: canteens and accommodation places directly managed by the universities.</rdfs:comment>
    <rdfs:comment xml:lang="it">Dati relativi alle strutture degli atenei: mense e posti alloggio direttamente gestiti dagli Atenei.</rdfs:comment>
    <rdfs:label xml:lang="it">Aggregato USTAT delle strutture universitarie</rdfs:label>
    <rdfs:label xml:lang="en">USTAT Aggregate of University Facilities</rdfs:label>
    <owl:versionInfo xml:lang="it">stabile</owl:versionInfo>
    <owl:versionInfo xml:lang="en">stable</owl:versionInfo>
  </rdf:Description>
  <rdf:Description rdf:about="https://w3id.org/italia/onto/HER/financialContribution">
    <rdf:type rdf:resource="http://www.w3.org/2002/07/owl#DatatypeProperty"/>
    <rdfs:domain rdf:resource="https://w3id.org/italia/onto/HER/EUREKAParticipant"/>
    <rdfs:range rdf:resource="http://www.w3.org/2001/XMLSchema#float"/>
    <rdfs:comment xml:lang="it">Il contributo finanziario per un partecipante a un progetto Eureka.</rdfs:comment>
    <rdfs:comment xml:lang="en">The financial contribution for a participant in an EUREKA project</rdfs:comment>
    <rdfs:isDefinedBy rdf:resource="https://w3id.org/italia/onto/HER"/>
    <rdfs:label xml:lang="it">contributo finanziario</rdfs:label>
    <rdfs:label xml:lang="en">financial contribution</rdfs:label>
    <owl:versionInfo xml:lang="it">stabile</owl:versionInfo>
    <owl:versionInfo xml:lang="en">stable</owl:versionInfo>
  </rdf:Description>
  <rdf:Description rdf:about="https://w3id.org/italia/onto/HER/dispositionFirstSubmittedDate">
    <rdf:type rdf:resource="http://www.w3.org/2002/07/owl#DatatypeProperty"/>
    <rdfs:subPropertyOf rdf:resource="https://w3id.org/italia/onto/TI/date"/>
    <rdfs:domain rdf:resource="https://w3id.org/italia/onto/HER/AACTStudy"/>
    <rdfs:range rdf:resource="http://www.w3.org/2001/XMLSchema#date"/>
    <rdfs:comment xml:lang="it">Data in cui uno sponsor indica che ritarderà la pubblicazione dei risultati (e sta certificando l'approvazione iniziale o il nuovo utilizzo), o quando richiede una proroga della scadenza. Il suffisso _submitted indica la data in cui il responsabile ha premuto il pulsante di rilascio nel sistema di invio dati di ClinicalTrials.gov, inviando così i dati per la revisione prima della pubblicazione.</rdfs:comment>
    <rdfs:comment xml:lang="en">Date when a sponsor indicates that they will be delaying posting of results (and are certifying initial approval or new use), or when they apply for an extension of the deadline. The _submitted suffix indicates the date that the responsible party pressed the release button in the ClinicalTrials.gov data submission system, thereby submitting the data for review prior to posting.</rdfs:comment>
    <rdfs:isDefinedBy rdf:resource="https://w3id.org/italia/onto/HER"/>
    <rdfs:label xml:lang="en">disposition first submitted date</rdfs:label>
    <rdfs:label xml:lang="it">disposizione prima data presentazione</rdfs:label>
    <owl:versionInfo xml:lang="it">stabile</owl:versionInfo>
    <owl:versionInfo xml:lang="en">stable</owl:versionInfo>
  </rdf:Description>
  <rdf:Description rdf:about="https://w3id.org/italia/onto/HER/totalDegreeExtraEU">
    <rdf:type rdf:resource="http://www.w3.org/2002/07/owl#DatatypeProperty"/>
    <rdfs:subPropertyOf rdf:resource="https://w3id.org/italia/onto/MU/value"/>
    <rdfs:domain rdf:nodeID="n5bb3bff42afb4ca286d2c3fead9507ddb311"/>
    <rdfs:range rdf:resource="http://www.w3.org/2000/01/rdf-schema#Literal"/>
    <rdfs:comment xml:lang="en">Total with respect to students from outside the European Union who are beneficiaries of interventions enrolled in degree courses, master's degree courses, courses of the old system. Students in good standing with the payment of tuition fees are considered.</rdfs:comment>
    <rdfs:comment xml:lang="it">Totale rispetto agli studenti di nazionalità extra Unione Europea beneficiari di interventi iscritti a corsi di laurea, corsi di laurea magistrale, corsi del vecchio ordinamento. Vengono considerati gli studenti in regola con il pagamento delle tasse universitarie.</rdfs:comment>
    <rdfs:isDefinedBy rdf:resource="https://w3id.org/italia/onto/HER"/>
    <rdfs:label xml:lang="en">total degree extra-EU</rdfs:label>
    <rdfs:label xml:lang="it">totale lauree extra-UE</rdfs:label>
    <owl:versionInfo xml:lang="it">stabile</owl:versionInfo>
    <owl:versionInfo xml:lang="en">stable</owl:versionInfo>
  </rdf:Description>
  <rdf:Description rdf:about="https://w3id.org/italia/onto/HER/hasAACTInterventionMeshTerm">
    <rdf:type rdf:resource="http://www.w3.org/2002/07/owl#ObjectProperty"/>
    <rdfs:subPropertyOf rdf:resource="https://w3id.org/italia/onto/HER/hasAACTMeshTerm"/>
    <rdfs:domain rdf:resource="https://w3id.org/italia/onto/HER/AACTStudy"/>
    <rdfs:range rdf:resource="https://w3id.org/italia/onto/HER/AACTInterventionMeshTerm"/>
    <rdfs:comment xml:lang="en">Clinical study intervention appropriate descriptors from NLM's Medical Subject Headings (MeSH)-controlled vocabulary thesaurus</rdfs:comment>
    <rdfs:comment xml:lang="it">interventi di studio clinico descritti da NLM's Medical Subject Headings (MeSH) - thesaurus del vocabolario controllato da NLM's Medical Subject Headings (MeSH) - thesaurus del vocabolario</rdfs:comment>
    <rdfs:isDefinedBy rdf:resource="https://w3id.org/italia/onto/HER"/>
    <rdfs:label xml:lang="it">ha termine MeSH di intervento AACT</rdfs:label>
    <rdfs:label xml:lang="en">has AACT intervention MeSH term</rdfs:label>
    <owl:versionInfo xml:lang="it">stabile</owl:versionInfo>
    <owl:versionInfo xml:lang="en">stable</owl:versionInfo>
  </rdf:Description>
  <rdf:Description rdf:about="https://w3id.org/italia/onto/HER/dispositionFirstSubmittedQCDate">
    <rdf:type rdf:resource="http://www.w3.org/2002/07/owl#DatatypeProperty"/>
    <rdfs:subPropertyOf rdf:resource="https://w3id.org/italia/onto/TI/date"/>
    <rdfs:domain rdf:resource="https://w3id.org/italia/onto/HER/AACTStudy"/>
    <rdfs:range rdf:resource="http://www.w3.org/2001/XMLSchema#date"/>
    <rdfs:comment xml:lang="it">Il suffisso _submitted_qc indica la data di presentazione della versione del record che soddisfa i criteri di controllo della qualità. È comune che ci siano revisioni tra la prima presentazione e la presentazione che soddisfa i criteri qc. Si noti che questa non è la data in cui è stata completata la revisione qc</rdfs:comment>
    <rdfs:comment xml:lang="en">The _submitted_qc suffix indicates the submission date of the version of the record that met quality control criteria. It is common for there to be revisions between the first submission and the submission that meets qc criteria. Note this is not the date that the qc review was completed."</rdfs:comment>
    <rdfs:isDefinedBy rdf:resource="https://w3id.org/italia/onto/HER"/>
    <rdfs:label xml:lang="en">disposition first submitted QC date</rdfs:label>
    <rdfs:label xml:lang="it">disposizione prima data presentazione QC</rdfs:label>
    <owl:versionInfo xml:lang="it">stabile</owl:versionInfo>
    <owl:versionInfo xml:lang="en">stable</owl:versionInfo>
  </rdf:Description>
  <rdf:Description rdf:nodeID="n5bb3bff42afb4ca286d2c3fead9507ddb293">
    <rdf:type rdf:resource="http://www.w3.org/1999/02/22-rdf-syntax-ns#List"/>
    <rdf:first>Other</rdf:first>
    <rdf:rest rdf:nodeID="n5bb3bff42afb4ca286d2c3fead9507ddb294"/>
  </rdf:Description>
  <rdf:Description rdf:about="https://w3id.org/italia/onto/HER/Area">
    <rdf:type rdf:resource="http://www.w3.org/2002/07/owl#Class"/>
    <rdfs:subClassOf rdf:resource="https://w3id.org/italia/onto/HER/AcademicDiscipline"/>
    <rdfs:comment xml:lang="en">It refers to the areas set up by the National University Council (CUN).
Currently, there are fourteen areas. (Gelmin Law 240/2010)
- Area 01 Mathematics and informatics
- Area 02 Physics
- Area 03 Chemistry
- Area 04 Earth Science
- Area 05 Biology
- Area 06 Medicine
- Area 07 Agricultural and veterinary science
- Area 08 Civil engineering and architecture
- Area 09 Industrial and information engineering
- Area 10 Antiquities, philology, literary studies, art history
- Area 11 History, philosophy, pedagogy and psychology
- Area 12 Law
- Area 13 Economics and statistics
- Area 14 Political and social science</rdfs:comment>
    <rdfs:comment xml:lang="it">Si riferisce alle aree istituite dal Consiglio Universitario Nazionale (CUN).
Attualmente le aree sono quattordici. (Legge Gelmin 240/2010)
- Area 01 Matematica e informatica
- Area 02 Fisica
- Area 03 Chimica
- Area 04 Scienze della Terra
- Area 05 Biologia
- Area 06 Medicina
- Area 07 Scienze agrarie e veterinarie
- Area 08 Ingegneria civile e architettura
- Area 09 Ingegneria industriale e dell'informazione
- Area 10 Antichità, filologia, studi letterari, storia dell'arte
- Area 11 Storia, filosofia, pedagogia e psicologia
- Area 12 Legge
- Area 13 Economia e statistica
- Area 14 Scienze politiche e sociali</rdfs:comment>
    <rdfs:isDefinedBy rdf:resource="https://w3id.org/italia/onto/HER"/>
    <rdfs:label xml:lang="it">Area CUN</rdfs:label>
    <rdfs:label xml:lang="en">CUN Area</rdfs:label>
    <owl:versionInfo xml:lang="it">stabile</owl:versionInfo>
    <owl:versionInfo xml:lang="en">stable</owl:versionInfo>
    <ns6:wasDerivedFrom rdf:resource="http://www.w3.org/2004/02/skos/core#Concept"/>
    <ns4:controlledVocabulary rdf:resource="https://w3id.org/italia/controlled-vocabulary/classifications-for-universities/academic-disciplines"/>
  </rdf:Description>
  <rdf:Description rdf:about="https://w3id.org/italia/onto/HER/hsUSTATStaffType">
    <rdf:type rdf:resource="http://www.w3.org/2002/07/owl#ObjectProperty"/>
    <rdfs:domain rdf:nodeID="n5bb3bff42afb4ca286d2c3fead9507ddb109"/>
    <rdfs:range rdf:resource="https://w3id.org/italia/onto/HER/USTATStaffType"/>
    <rdfs:comment xml:lang="it">Questa proprietà collega l'informazione sul personale relativo all'ente o Ufficio per il Diritto allo Studio Universitario (DSU) considerato alla tipologia di contratto di assunzione.</rdfs:comment>
    <rdfs:comment xml:lang="en">This property links the information on the personnel related to the institution or Office for the Right to University Studies (DSU) considered to the type of employment contract.</rdfs:comment>
    <rdfs:isDefinedBy rdf:resource="https://w3id.org/italia/onto/HER"/>
    <rdfs:label xml:lang="it">ha un ruolo di staff universitario italiano</rdfs:label>
    <rdfs:label xml:lang="en">has italian university staff role</rdfs:label>
    <owl:versionInfo xml:lang="it">provvisoria</owl:versionInfo>
    <owl:versionInfo xml:lang="en">unstable</owl:versionInfo>
  </rdf:Description>
  <rdf:Description rdf:nodeID="n5bb3bff42afb4ca286d2c3fead9507ddb208">
    <rdf:first rdf:resource="https://w3id.org/italia/onto/HER/MIURStudentsByCitizenshipDegreeAggregate"/>
    <rdf:rest rdf:nodeID="n5bb3bff42afb4ca286d2c3fead9507ddb209"/>
  </rdf:Description>
  <rdf:Description rdf:about="https://w3id.org/italia/onto/HER/CTNPRINEntity">
    <rdf:type rdf:resource="http://www.w3.org/2002/07/owl#Class"/>
    <rdfs:subClassOf rdf:resource="https://w3id.org/italia/onto/COV/Organization"/>
    <rdfs:comment xml:lang="it">Soggetti beneficiari dell'iniziativa. I dati integrati in ToscanaOpenResearch sono stati ottenuti nel contesto di un protocollo di intesa tra il Ministero dell'Istruzione, dell'Università e della Ricerca e la Regione toscana, e sono relativi a progetti aventi almeno un beneficiario con sede legale o operativa in Toscana.</rdfs:comment>
    <rdfs:comment xml:lang="en">Subjects that are beneficiaries of the initiative. The data integrated in ToscanaOpenResearch were obtained in the context of a memorandum of understanding between the Ministry of Education, University and Research and the Region of Tuscany, and are related to projects with at least one beneficiary with registered or operational headquarters in Tuscany.</rdfs:comment>
    <rdfs:isDefinedBy rdf:resource="https://w3id.org/italia/onto/HER"/>
    <rdfs:label xml:lang="en">CTN/PRIN Funded Institution</rdfs:label>
    <rdfs:label xml:lang="it">Istituzione finanziata da CTN/PRIN</rdfs:label>
    <owl:versionInfo xml:lang="it">stabile</owl:versionInfo>
    <owl:versionInfo xml:lang="en">stable</owl:versionInfo>
  </rdf:Description>
  <rdf:Description rdf:about="https://w3id.org/italia/onto/RO/Role">
    <rdf:type rdf:resource="http://www.w3.org/2002/07/owl#Class"/>
  </rdf:Description>
  <rdf:Description rdf:about="https://w3id.org/italia/onto/HER/totalFemaleGraduated">
    <rdf:type rdf:resource="http://www.w3.org/2002/07/owl#DatatypeProperty"/>
    <rdfs:subPropertyOf rdf:resource="https://w3id.org/italia/onto/MU/value"/>
    <rdfs:domain rdf:resource="https://w3id.org/italia/onto/HER/USTATStudentsBySexAggregate"/>
    <rdfs:range rdf:resource="http://www.w3.org/2000/01/rdf-schema#Literal"/>
    <rdfs:comment xml:lang="en">Number of female graduates corresponding to the selected combination of variables. In particular: Number of female students who graduated in the reference calendar year. Students of levels 6 and 7 of ISCED 2011.
For the year 2018: elaborations on ANS data - extraction December 2019.</rdfs:comment>
    <rdfs:comment xml:lang="it">Numero di laureate di genere femminile corrispondente alla combinazione di variabili selezionata. In particolare: Numero di studentesse che si sono laureate nell’anno solare di riferimento. Studentesse dei livelli 6 e 7 della ISCED 2011. Per l'anno 2018: elaborazioni su dati ANS - estrazione Dicembre 2019.</rdfs:comment>
    <rdfs:isDefinedBy rdf:resource="https://w3id.org/italia/onto/HER"/>
    <rdfs:label xml:lang="en">total female graduated</rdfs:label>
    <rdfs:label xml:lang="it">totale di genere femminile laureato</rdfs:label>
    <owl:versionInfo xml:lang="it">stabile</owl:versionInfo>
    <owl:versionInfo xml:lang="en">stable</owl:versionInfo>
  </rdf:Description>
  <rdf:Description rdf:about="https://w3id.org/italia/onto/HER/Result">
    <rdf:type rdf:resource="http://www.w3.org/2002/07/owl#Class"/>
    <rdfs:subClassOf rdf:resource="https://w3id.org/italia/onto/l0/Object"/>
    <rdfs:subClassOf rdf:nodeID="n5bb3bff42afb4ca286d2c3fead9507ddb509"/>
    <rdfs:subClassOf rdf:nodeID="n5bb3bff42afb4ca286d2c3fead9507ddb510"/>
    <rdfs:subClassOf rdf:nodeID="n5bb3bff42afb4ca286d2c3fead9507ddb511"/>
    <rdfs:subClassOf rdf:nodeID="n5bb3bff42afb4ca286d2c3fead9507ddb512"/>
    <rdfs:isDefinedBy rdf:resource="https://w3id.org/italia/onto/HER"/>
    <rdfs:label xml:lang="en">Result</rdfs:label>
    <rdfs:label xml:lang="it">Risultato (Output)</rdfs:label>
    <owl:versionInfo xml:lang="it">stabile</owl:versionInfo>
    <owl:versionInfo xml:lang="en">stable</owl:versionInfo>
  </rdf:Description>
  <rdf:Description rdf:about="https://w3id.org/italia/onto/HER/transmissionDate">
    <rdf:type rdf:resource="http://www.w3.org/2002/07/owl#DatatypeProperty"/>
    <rdfs:subPropertyOf rdf:resource="https://w3id.org/italia/onto/TI/date"/>
    <rdfs:domain rdf:resource="https://w3id.org/italia/onto/HER/CTNPRINOperation"/>
    <rdfs:range rdf:resource="http://www.w3.org/2001/XMLSchema#date"/>
    <rdfs:comment xml:lang="it">Data di presentazione della proposta progettuale associata all'operazione</rdfs:comment>
    <rdfs:comment xml:lang="en">Date of submission of the project proposal associated with the operation</rdfs:comment>
    <rdfs:isDefinedBy rdf:resource="https://w3id.org/italia/onto/HER"/>
    <rdfs:label xml:lang="it">data trasmissione</rdfs:label>
    <rdfs:label xml:lang="en">transmission date</rdfs:label>
    <owl:versionInfo xml:lang="it">stabile</owl:versionInfo>
    <owl:versionInfo xml:lang="en">stable</owl:versionInfo>
  </rdf:Description>
  <rdf:Description rdf:nodeID="n5bb3bff42afb4ca286d2c3fead9507ddb458">
    <rdf:type rdf:resource="http://www.w3.org/2002/07/owl#Restriction"/>
    <owl:onProperty rdf:resource="https://w3id.org/italia/onto/l0/identifier"/>
    <owl:cardinality rdf:datatype="http://www.w3.org/2001/XMLSchema#nonNegativeInteger">1</owl:cardinality>
  </rdf:Description>
  <rdf:Description rdf:about="https://w3id.org/italia/onto/HER/patentApplicationDate">
    <rdf:type rdf:resource="http://www.w3.org/2002/07/owl#DatatypeProperty"/>
    <rdfs:subPropertyOf rdf:resource="https://w3id.org/italia/onto/TI/date"/>
    <rdfs:domain rdf:resource="https://w3id.org/italia/onto/HER/Patent"/>
    <rdfs:range rdf:resource="http://www.w3.org/2001/XMLSchema#date"/>
    <rdfs:comment xml:lang="it">La data in cui è stata presentata la domanda di brevetto.</rdfs:comment>
    <rdfs:comment xml:lang="en">The data in which a patent's application was filled in.</rdfs:comment>
    <rdfs:isDefinedBy rdf:resource="https://w3id.org/italia/onto/HER"/>
    <rdfs:label xml:lang="it">data richiesta brevetto</rdfs:label>
    <rdfs:label xml:lang="en">patent application date</rdfs:label>
    <owl:versionInfo xml:lang="it">stabile</owl:versionInfo>
    <owl:versionInfo xml:lang="en">stable</owl:versionInfo>
  </rdf:Description>
  <rdf:Description rdf:about="https://w3id.org/italia/onto/Project/PublicResearchProject">
    <rdf:type rdf:resource="http://www.w3.org/2002/07/owl#Class"/>
    <rdfs:subClassOf rdf:nodeID="n5bb3bff42afb4ca286d2c3fead9507ddb548"/>
    <rdfs:subClassOf rdf:nodeID="n5bb3bff42afb4ca286d2c3fead9507ddb549"/>
  </rdf:Description>
  <rdf:Description rdf:nodeID="n5bb3bff42afb4ca286d2c3fead9507ddb146">
    <rdf:type rdf:resource="http://www.w3.org/1999/02/22-rdf-syntax-ns#List"/>
    <rdf:first>Formazione</rdf:first>
    <rdf:rest rdf:nodeID="n5bb3bff42afb4ca286d2c3fead9507ddb147"/>
  </rdf:Description>
  <rdf:Description rdf:about="https://w3id.org/italia/onto/COV/hasOrganization">
    <rdf:type rdf:resource="http://www.w3.org/2002/07/owl#ObjectProperty"/>
  </rdf:Description>
  <rdf:Description rdf:about="https://w3id.org/italia/onto/HER/patentApplicationYear">
    <rdf:type rdf:resource="http://www.w3.org/2002/07/owl#DatatypeProperty"/>
    <rdfs:subPropertyOf rdf:resource="https://w3id.org/italia/onto/TI/year"/>
    <rdfs:domain rdf:resource="https://w3id.org/italia/onto/HER/Result"/>
    <rdfs:range rdf:resource="http://www.w3.org/2001/XMLSchema#gYear"/>
    <rdfs:comment xml:lang="it">L'anno in cui è stata depositata la domanda di brevetto.</rdfs:comment>
    <rdfs:comment xml:lang="en">The year in which a patent application was filed.</rdfs:comment>
    <rdfs:isDefinedBy rdf:resource="https://w3id.org/italia/onto/HER"/>
    <rdfs:label xml:lang="it">anno della richiesta</rdfs:label>
    <rdfs:label xml:lang="en">application year</rdfs:label>
    <owl:versionInfo xml:lang="it">stabile</owl:versionInfo>
    <owl:versionInfo xml:lang="en">stable</owl:versionInfo>
  </rdf:Description>
  <rdf:Description rdf:about="https://w3id.org/italia/onto/HER/ctnprinInitiativeReportedCost">
    <rdf:type rdf:resource="http://www.w3.org/2002/07/owl#DatatypeProperty"/>
    <rdfs:subPropertyOf rdf:resource="https://w3id.org/italia/onto/MU/value"/>
    <rdfs:domain rdf:resource="https://w3id.org/italia/onto/HER/CTNPRINInitiative"/>
    <rdfs:range rdf:resource="http://www.w3.org/2001/XMLSchema#decimal"/>
    <rdfs:comment xml:lang="en">Total costs reported by beneficiaries compared to eligible costs. Calculated as the sum of the homologous variable 'reportedCost' present at the lower aggregation level (reportedCost_operations)</rdfs:comment>
    <rdfs:comment xml:lang="it">Totale dei costi rendicontati dai beneficiari rispetto ai costi ammessi. Calcolati come somma dell'omologa variabile "reportedCost" presente a livello di aggregazione inferiore (reportedCost_operations)</rdfs:comment>
    <rdfs:isDefinedBy rdf:resource="https://w3id.org/italia/onto/HER"/>
    <rdfs:label xml:lang="it">costi rendicontati per iniziative CTN/PRIN</rdfs:label>
    <rdfs:label xml:lang="en">reported cost of CTN/PRIN initiative</rdfs:label>
    <owl:versionInfo xml:lang="it">stabile</owl:versionInfo>
    <owl:versionInfo xml:lang="en">stable</owl:versionInfo>
  </rdf:Description>
  <rdf:Description rdf:nodeID="n5bb3bff42afb4ca286d2c3fead9507ddb83">
    <rdf:first rdf:resource="https://w3id.org/italia/onto/HER/MIURStudentsByCitizenshipDegreeAggregate"/>
    <rdf:rest rdf:nodeID="n5bb3bff42afb4ca286d2c3fead9507ddb84"/>
  </rdf:Description>
  <rdf:Description rdf:about="https://w3id.org/italia/onto/HER/ctnprinOperationAdmittedCost">
    <rdf:type rdf:resource="http://www.w3.org/2002/07/owl#DatatypeProperty"/>
    <rdfs:subPropertyOf rdf:resource="https://w3id.org/italia/onto/MU/value"/>
    <rdfs:domain rdf:resource="https://w3id.org/italia/onto/HER/CTNPRINOperation"/>
    <rdfs:range rdf:resource="http://www.w3.org/2001/XMLSchema#decimal"/>
    <rdfs:comment xml:lang="en">Admitted costs after evaluation of the costs indicated in the project proposal. Calculated as the sum of the counterpart variable 'admittedCost' present at lower aggregation level (admittedCost_amounts)</rdfs:comment>
    <rdfs:comment xml:lang="it">Costi ammessi dopo la valutazione dei costi indicati nella proposta di progetto. Calcolati come somma dell'omologa variabile "admittedCost" presente a livello di aggregazione inferiore (admittedCost_amounts)</rdfs:comment>
    <rdfs:isDefinedBy rdf:resource="https://w3id.org/italia/onto/HER"/>
    <rdfs:label xml:lang="en">admitted cost of CTN/PRIN operation</rdfs:label>
    <rdfs:label xml:lang="it">costi amessi per operazioni CTN/PRIN</rdfs:label>
    <owl:versionInfo xml:lang="it">stabile</owl:versionInfo>
    <owl:versionInfo xml:lang="en">stable</owl:versionInfo>
  </rdf:Description>
  <rdf:Description rdf:about="https://w3id.org/italia/onto/HER/allocatesFundsTo">
    <rdf:type rdf:resource="http://www.w3.org/2002/07/owl#ObjectProperty"/>
    <rdfs:domain rdf:resource="https://w3id.org/italia/onto/HER/CTNPRINOperation"/>
    <rdfs:range rdf:resource="https://w3id.org/italia/onto/HER/CTNPRINEntity"/>
    <rdfs:comment xml:lang="it">Indica i soggetti beneficiari dell'iniziativa.</rdfs:comment>
    <rdfs:comment xml:lang="en">Indicates the subjects benefiting from the initiative.</rdfs:comment>
    <rdfs:isDefinedBy rdf:resource="https://w3id.org/italia/onto/HER"/>
    <rdfs:label xml:lang="en">allocates funds to</rdfs:label>
    <rdfs:label xml:lang="it">fondi stanziati a</rdfs:label>
    <owl:versionInfo xml:lang="it">provvisoria</owl:versionInfo>
    <owl:versionInfo xml:lang="en">unstable</owl:versionInfo>
  </rdf:Description>
  <rdf:Description rdf:about="https://w3id.org/italia/onto/HER/verificationMonthYear">
    <rdf:type rdf:resource="http://www.w3.org/2002/07/owl#DatatypeProperty"/>
    <rdfs:subPropertyOf rdf:resource="https://w3id.org/italia/onto/TI/year"/>
    <rdfs:domain rdf:resource="https://w3id.org/italia/onto/HER/AACTStudy"/>
    <rdfs:range rdf:resource="http://www.w3.org/2001/XMLSchema#gYear"/>
    <rdfs:comment xml:lang="it">La data in cui lo studio è stato verificato per l'ultima volta in un formato di tipo data, in modo da poterlo utilizzare per trovare gli studi prima/dopo/conclusiva di una o più date. Per gli studi che forniscono solo mese/anno, viene utilizzato l'ultimo giorno del mese.</rdfs:comment>
    <rdfs:comment xml:lang="en">The date the study was last verified in a date-type format so that it can be used to find studies before/after/inclusive of a date or dates. For studies that only provide month/year, the last day of the month is used.</rdfs:comment>
    <rdfs:isDefinedBy rdf:resource="https://w3id.org/italia/onto/HER"/>
    <rdfs:label xml:lang="it">mese-anno di verifica</rdfs:label>
    <rdfs:label xml:lang="en">verification month-year</rdfs:label>
    <owl:versionInfo xml:lang="it">stabile</owl:versionInfo>
    <owl:versionInfo xml:lang="en">stable</owl:versionInfo>
  </rdf:Description>
  <rdf:Description rdf:about="https://w3id.org/italia/data/public-organization/r_toscan">
    <rdf:type rdf:resource="http://www.w3.org/2002/07/owl#NamedIndividual"/>
    <rdf:type rdf:resource="http://dati.gov.it/onto/dcatapit#Agent"/>
    <rdf:type rdf:resource="http://xmlns.com/foaf/0.1/Agent"/>
    <ns2:identifier>r_toscan</ns2:identifier>
    <ns5:name xml:lang="it">Regione Toscana</ns5:name>
    <ns5:name xml:lang="en">Toscany Region</ns5:name>
  </rdf:Description>
  <rdf:Description rdf:nodeID="n5bb3bff42afb4ca286d2c3fead9507ddb209">
    <rdf:first rdf:resource="https://w3id.org/italia/onto/HER/MIURStudentsByCitizenshipDegreeClassAggregate"/>
    <rdf:rest rdf:nodeID="n5bb3bff42afb4ca286d2c3fead9507ddb210"/>
  </rdf:Description>
  <rdf:Description rdf:about="https://w3id.org/italia/onto/HER/DegreeArea">
    <rdf:type rdf:resource="http://www.w3.org/2002/07/owl#Class"/>
    <rdfs:subClassOf rdf:resource="https://w3id.org/italia/onto/HER/HERClassification"/>
    <rdfs:comment xml:lang="en">According to http://anagrafe.miur.it/, the areas are the following:

- Sanitaria
- Scientifica
- Sociale
- Umanistica

Each faculty is gruped under one of the previous areas.</rdfs:comment>
    <rdfs:isDefinedBy rdf:resource="https://w3id.org/italia/onto/HER"/>
    <rdfs:label xml:lang="it">Area di laurea italiana</rdfs:label>
    <rdfs:label xml:lang="en">Italian Degree Area</rdfs:label>
    <owl:versionInfo xml:lang="it">stabile</owl:versionInfo>
    <owl:versionInfo xml:lang="en">stable</owl:versionInfo>
    <ns6:wasDerivedFrom rdf:resource="http://www.w3.org/2004/02/skos/core#Concept"/>
  </rdf:Description>
  <rdf:Description rdf:about="https://w3id.org/italia/onto/HER/totalFemale">
    <rdf:type rdf:resource="http://www.w3.org/2002/07/owl#DatatypeProperty"/>
    <rdfs:subPropertyOf rdf:resource="https://w3id.org/italia/onto/MU/value"/>
    <rdfs:domain rdf:nodeID="n5bb3bff42afb4ca286d2c3fead9507ddb322"/>
    <rdfs:range rdf:resource="http://www.w3.org/2001/XMLSchema#decimal"/>
    <rdfs:comment xml:lang="en">Total with respect to the female population of the sample considered.</rdfs:comment>
    <rdfs:comment xml:lang="it">Totale rispetto alla popolazione di sesso femminile del campione considerato.</rdfs:comment>
    <rdfs:isDefinedBy rdf:resource="https://w3id.org/italia/onto/HER"/>
    <rdfs:label xml:lang="en">total female</rdfs:label>
    <rdfs:label xml:lang="it">totale genere femminile</rdfs:label>
    <owl:versionInfo xml:lang="it">stabile</owl:versionInfo>
    <owl:versionInfo xml:lang="en">stable</owl:versionInfo>
  </rdf:Description>
  <rdf:Description rdf:about="https://w3id.org/italia/onto/HER/ReportedCitizenship">
    <rdf:type rdf:resource="http://www.w3.org/2002/07/owl#Class"/>
    <rdfs:subClassOf rdf:resource="https://w3id.org/italia/onto/l0/Characteristic"/>
    <rdfs:comment xml:lang="en">It refers to the citenzship of where a person was born. The possible values are:
- Italian
- Non italian</rdfs:comment>
    <rdfs:comment xml:lang="it">Si riferisce alla cittadinanza del luogo di nascita di una persona. I valori possibili sono:
- Italiano
- Non italiano</rdfs:comment>
    <rdfs:isDefinedBy rdf:resource="https://w3id.org/italia/onto/HER"/>
    <rdfs:label xml:lang="it">Cittadinanza riportata in sistemi nazionali scolastici</rdfs:label>
    <rdfs:label xml:lang="en">Reported Citizenship</rdfs:label>
    <owl:versionInfo xml:lang="it">provvisorio - da comprendere meglio con dati alla mano se possa essere sufficiente utilizzare la cittadinanza già definita nell'ontologia Core Person Vocabulary - Profilo Applicativo Italiano</owl:versionInfo>
    <owl:versionInfo xml:lang="en">unstable - to be investigated whether it is sufficient to use the citizenship already defined in CPV - Core Person Vocabulary - Italian Application Profile.</owl:versionInfo>
  </rdf:Description>
  <rdf:Description rdf:about="https://w3id.org/italia/onto/HER/overallStatus">
    <rdf:type rdf:resource="http://www.w3.org/2002/07/owl#DatatypeProperty"/>
    <rdfs:domain rdf:resource="https://w3id.org/italia/onto/HER/AACTStudy"/>
    <rdfs:range rdf:resource="http://www.w3.org/2000/01/rdf-schema#Literal"/>
    <rdfs:comment xml:lang="it">Indica lo stato di reclutamento attuale o lo stato di accesso ampliato.</rdfs:comment>
    <rdfs:comment xml:lang="en">Indicates the current recruitment status or the expanded access status.</rdfs:comment>
    <rdfs:isDefinedBy rdf:resource="https://w3id.org/italia/onto/HER"/>
    <rdfs:label xml:lang="en">overall status</rdfs:label>
    <rdfs:label xml:lang="it">stato complessivo</rdfs:label>
    <owl:versionInfo xml:lang="it">stabile</owl:versionInfo>
    <owl:versionInfo xml:lang="en">stable</owl:versionInfo>
  </rdf:Description>
  <rdf:Description rdf:about="https://w3id.org/italia/onto/HER/hasUSTATReportedHERInstitution">
    <rdf:type rdf:resource="http://www.w3.org/2002/07/owl#ObjectProperty"/>
    <rdfs:domain rdf:nodeID="n5bb3bff42afb4ca286d2c3fead9507ddb106"/>
    <rdfs:range rdf:resource="https://w3id.org/italia/onto/HER/USTATReportedHERInstitution"/>
    <rdfs:comment xml:lang="it">Questa proprietà collega l'informazione sui dati relativi agli interventi a favore degli studenti all'istituto per l'alta formazione (Ateneo, Istituto Alta Formazione Artistica e Musicale - AFAM, Scuola Superiore per Mediatori Linguistici, Altro) corrispondente.</rdfs:comment>
    <rdfs:comment xml:lang="en">This property links the information about the interventions in favour of the students to the corresponding Institute for Higher Education (Ateneo, Istituto Alta Formazione Artistica e Musicale - AFAM, Scuola Superiore per Mediatori Linguistici, Altro).</rdfs:comment>
    <rdfs:isDefinedBy rdf:resource="https://w3id.org/italia/onto/HER"/>
    <rdfs:label xml:lang="it">ha un'istituzione di HER riportata da USTAT</rdfs:label>
    <rdfs:label xml:lang="en">has USTAT reported HER institution</rdfs:label>
    <owl:versionInfo xml:lang="it">stabile</owl:versionInfo>
    <owl:versionInfo xml:lang="en">stable</owl:versionInfo>
  </rdf:Description>
  <rdf:Description rdf:about="https://w3id.org/italia/onto/HER/isUSExport">
    <rdf:type rdf:resource="http://www.w3.org/2002/07/owl#DatatypeProperty"/>
    <rdf:type rdf:resource="http://www.w3.org/2002/07/owl#FunctionalProperty"/>
    <rdfs:domain rdf:resource="https://w3id.org/italia/onto/HER/AACTStudy"/>
    <rdfs:range rdf:resource="http://www.w3.org/2001/XMLSchema#boolean"/>
    <rdfs:comment xml:lang="it">Se qualsiasi prodotto farmaceutico (incluso un prodotto biologico) o dispositivo studiato nello studio clinico viene fabbricato negli Stati Uniti o in uno dei suoi territori ed esportato per essere studiato in uno studio clinico in un altro paese. Richiesto se il farmaco regolamentato dalla FDA statunitense e/o il dispositivo regolamentato dalla FDA statunitense è "Sì", l'IND o l'IDE della FDA statunitense è "No", e le informazioni sulla struttura non includono almeno una sede negli Stati Uniti.</rdfs:comment>
    <rdfs:comment xml:lang="en">Whether any drug product (including a biological product) or device product studied in the clinical study is manufactured in the United States or one of its territories and exported for study in a clinical study in another country. Required if U.S. FDA-regulated Drug and/or U.S. FDA-regulated Device is "Yes," U.S. FDA IND or IDE is "No", and Facility Information does not include at least one U.S. location.</rdfs:comment>
    <rdfs:isDefinedBy rdf:resource="https://w3id.org/italia/onto/HER"/>
    <rdfs:label xml:lang="en">is US export</rdfs:label>
    <rdfs:label xml:lang="it">è esportato dagli US</rdfs:label>
    <owl:versionInfo xml:lang="it">stabile</owl:versionInfo>
    <owl:versionInfo xml:lang="en">stable</owl:versionInfo>
  </rdf:Description>
  <rdf:Description rdf:nodeID="n5bb3bff42afb4ca286d2c3fead9507ddb70">
    <rdf:type rdf:resource="http://www.w3.org/2002/07/owl#Class"/>
    <owl:unionOf rdf:nodeID="n5bb3bff42afb4ca286d2c3fead9507ddb71"/>
  </rdf:Description>
  <rdf:Description rdf:about="https://w3id.org/italia/onto/HER/verificationDate">
    <rdf:type rdf:resource="http://www.w3.org/2002/07/owl#DatatypeProperty"/>
    <rdfs:subPropertyOf rdf:resource="https://w3id.org/italia/onto/TI/date"/>
    <rdfs:domain rdf:resource="https://w3id.org/italia/onto/HER/AACTStudy"/>
    <rdfs:range rdf:resource="http://www.w3.org/2001/XMLSchema#date"/>
    <rdfs:comment xml:lang="it">Numero totale di partecipanti allo studio</rdfs:comment>
    <rdfs:comment xml:lang="en">The date the study was last verified in a date-type format so that it can be used to find studies before/after/inclusive of a date or dates. For studies that only provide month/year, the last day of the month is used.</rdfs:comment>
    <rdfs:isDefinedBy rdf:resource="https://w3id.org/italia/onto/HER"/>
    <rdfs:label xml:lang="it">data verifica</rdfs:label>
    <rdfs:label xml:lang="en">verification date</rdfs:label>
    <owl:versionInfo xml:lang="it">stabile</owl:versionInfo>
    <owl:versionInfo xml:lang="en">stable</owl:versionInfo>
  </rdf:Description>
  <rdf:Description rdf:nodeID="n5bb3bff42afb4ca286d2c3fead9507ddb399">
    <rdf:type rdf:resource="http://www.w3.org/2002/07/owl#Restriction"/>
    <owl:onProperty rdf:resource="https://w3id.org/italia/onto/HER/leaderName"/>
    <owl:someValuesFrom rdf:resource="http://www.w3.org/2000/01/rdf-schema#Literal"/>
  </rdf:Description>
  <rdf:Description rdf:nodeID="n5bb3bff42afb4ca286d2c3fead9507ddb388">
    <rdf:type rdf:resource="http://www.w3.org/2002/07/owl#Restriction"/>
    <owl:onProperty rdf:resource="https://w3id.org/italia/onto/HER/dispositionFirstSubmittedDate"/>
    <owl:maxQualifiedCardinality rdf:datatype="http://www.w3.org/2001/XMLSchema#nonNegativeInteger">1</owl:maxQualifiedCardinality>
    <owl:onDataRange rdf:resource="http://www.w3.org/2001/XMLSchema#date"/>
  </rdf:Description>
  <rdf:Description rdf:about="https://w3id.org/italia/onto/HER/USTATStaffType">
    <rdf:type rdf:resource="http://www.w3.org/2002/07/owl#Class"/>
    <rdfs:subClassOf rdf:resource="https://w3id.org/italia/onto/RO/Role"/>
    <rdfs:comment xml:lang="en">Information on the personnel in service in the Entities and Offices for the Right to University Studies - DSU, aggregated by Region. In particular:
- information on personnel on permanent service in the entities and offices for the DSU as of 31/12 of the year of reference, aggregated by Region;
- information on staff serving on a fixed-term contract in the entities and offices for the DSU in the reference year, aggregated by Region.

Please note that the individuals of this class are not the individuals of the defined controlled vocabulary on Italian Academic Roles. There are some elements of overlapping but they differ between each other.

One of the future work to be considered is to align the individuals of this specific class to one unique Italian academic roles controlled vocabulary to be applied at the national level.</rdfs:comment>
    <rdfs:comment xml:lang="it">Informazioni sul personale in servizio negli Enti e negli Uffici per il DSU, aggregato per Regione. In particolare:
- informazioni sul personale in servizio a tempo indeterminato negli Enti e negli Uffici per il DSU al 31/12 dell'anno di riferimento, aggregato per Regione;
- informazioni sul personale che ha prestato servizio a tempo determinato negli Enti e negli Uffici per il DSU nell'anno di riferimento, aggregato per Regione

Si noti che le istanze di questa classe potrebbero essere quelle del vocabolario controllato sui ruoli accademici italiani. Tuttavia, nei dati finora analizzati, questa classe ha istanze in parte differenti rispetto al vocabolario controllato creato.

Un possibile lavoro futuro è quello di eliminare questo elemento nel modello (per questo al momento è stato indicato come provvisorio) per consentire ai detentori di dati di uniformarsi a un vocabolario unico nazionale sui ruoli del personale universitario italiano.</rdfs:comment>
    <rdfs:isDefinedBy rdf:resource="https://w3id.org/italia/onto/HER"/>
    <rdfs:label xml:lang="en">Italian University Staff Role</rdfs:label>
    <rdfs:label xml:lang="it">Ruolo del personale universitario italiano</rdfs:label>
    <owl:versionInfo xml:lang="it">Provvisoria</owl:versionInfo>
    <owl:versionInfo xml:lang="en">Unstable</owl:versionInfo>
    <ns6:wasDerivedFrom rdf:resource="http://www.w3.org/2004/02/skos/core#Concept"/>
  </rdf:Description>
  <rdf:Description rdf:about="https://w3id.org/italia/onto/HER/DMCAvailable">
    <rdf:type rdf:resource="http://www.w3.org/2002/07/owl#DatatypeProperty"/>
    <rdfs:domain rdf:resource="https://w3id.org/italia/onto/HER/AACTStudy"/>
    <rdfs:range rdf:resource="http://www.w3.org/2001/XMLSchema#boolean"/>
    <rdfs:comment xml:lang="it">Lo studio dispone di un Comitato di monitoraggio dei dati (DMC) (un gruppo di scienziati indipendenti che monitorano la sicurezza e l'integrità scientifica di uno studio clinico. Il DMC può raccomandare allo sponsor di interrompere la sperimentazione se non è efficace, se danneggia i partecipanti o se è improbabile che serva al suo scopo scientifico. I membri sono scelti in base alle competenze e alle conoscenze scientifiche necessarie per monitorare lo specifico studio. Chiamato anche scheda di sicurezza e monitoraggio dei dati, o DSMB).

La proprietà indica se il comitato è presente o meno.</rdfs:comment>
    <rdfs:comment xml:lang="en">Study has a Data Monitoring Committee (DMC) (a group of independent scientists who monitor the safety and scientific integrity of a clinical trial. The DMC can recommend to the sponsor that the trial be stopped if it is not effective, is harming participants, or is unlikely to serve its scientific purpose. Members are chosen based on the scientific skills and knowledge needed to monitor the particular trial. Also called a data safety and monitoring board, or DSMB.)

The property indicates whether such a committee exists or not.</rdfs:comment>
    <rdfs:isDefinedBy rdf:resource="https://w3id.org/italia/onto/HER"/>
    <rdfs:label xml:lang="it">comitato di monitoraggio dati disponibile</rdfs:label>
    <rdfs:label xml:lang="en">data monitoring committee available</rdfs:label>
    <owl:versionInfo xml:lang="it">stabile</owl:versionInfo>
    <owl:versionInfo xml:lang="en">stable</owl:versionInfo>
  </rdf:Description>
  <rdf:Description rdf:about="https://w3id.org/italia/onto/HER/isCoordinatorOf">
    <rdf:type rdf:resource="http://www.w3.org/2002/07/owl#ObjectProperty"/>
    <rdfs:domain rdf:resource="https://w3id.org/italia/onto/COV/Organization"/>
    <rdfs:range rdf:resource="https://w3id.org/italia/onto/Project/PublicResearchProject"/>
    <rdfs:comment xml:lang="en">Inverse property of hasCoordinator</rdfs:comment>
    <rdfs:comment xml:lang="it">Proprietà inversa di ha coordinatore</rdfs:comment>
    <rdfs:isDefinedBy rdf:resource="https://w3id.org/italia/onto/HER"/>
    <rdfs:label xml:lang="en">is coordinator of</rdfs:label>
    <rdfs:label xml:lang="it">è coordinatore di</rdfs:label>
    <owl:versionInfo xml:lang="it">stabile</owl:versionInfo>
    <owl:versionInfo xml:lang="en">stable</owl:versionInfo>
  </rdf:Description>
  <rdf:Description rdf:nodeID="n5bb3bff42afb4ca286d2c3fead9507ddb535">
    <rdf:type rdf:resource="http://www.w3.org/2002/07/owl#Restriction"/>
    <owl:onProperty rdf:resource="https://w3id.org/italia/onto/COV/hasOrganization"/>
    <owl:maxQualifiedCardinality rdf:datatype="http://www.w3.org/2001/XMLSchema#nonNegativeInteger">1</owl:maxQualifiedCardinality>
    <owl:onClass rdf:resource="https://w3id.org/italia/onto/COV/Organization"/>
  </rdf:Description>
  <rdf:Description rdf:nodeID="n5bb3bff42afb4ca286d2c3fead9507ddb73">
    <rdf:type rdf:resource="http://www.w3.org/2002/07/owl#Class"/>
    <owl:unionOf rdf:nodeID="n5bb3bff42afb4ca286d2c3fead9507ddb74"/>
  </rdf:Description>
  <rdf:Description rdf:about="https://w3id.org/italia/onto/HER/expenseType">
    <rdf:type rdf:resource="http://www.w3.org/2002/07/owl#DatatypeProperty"/>
    <rdfs:domain rdf:resource="https://w3id.org/italia/onto/HER/CTNPRINAmount"/>
    <rdfs:range rdf:resource="http://www.w3.org/2000/01/rdf-schema#Literal"/>
    <rdfs:comment xml:lang="it">Tipologia di spesa tra quelle previste dall'iniziativa (bando, avviso, …): - Personale - Strumentazione - Fabbricati - ….</rdfs:comment>
    <rdfs:comment xml:lang="en">Type of expenditure among those foreseen by the initiative (call for proposals, notice, ...): - Personnel - Instrumentation - Buildings - ....</rdfs:comment>
    <rdfs:isDefinedBy rdf:resource="https://w3id.org/italia/onto/HER"/>
    <rdfs:label xml:lang="en">expense type</rdfs:label>
    <rdfs:label xml:lang="it">tipo di spese</rdfs:label>
    <owl:versionInfo xml:lang="it">stabile</owl:versionInfo>
    <owl:versionInfo xml:lang="en">stable</owl:versionInfo>
  </rdf:Description>
  <rdf:Description rdf:about="https://w3id.org/italia/onto/HER/ErasmusPlusActionType">
    <rdf:type rdf:resource="http://www.w3.org/2002/07/owl#Class"/>
    <rdfs:subClassOf rdf:resource="https://w3id.org/italia/onto/HER/ErasmusPlusClassification"/>
    <rdfs:comment xml:lang="en">It refers to the specific action type within each Key action.</rdfs:comment>
    <rdfs:comment xml:lang="it">Si riferisce al tipo di azione specifica all'interno di ogni azione chiave.</rdfs:comment>
    <rdfs:isDefinedBy rdf:resource="https://w3id.org/italia/onto/HER"/>
    <rdfs:label xml:lang="en">Erasmus+ Action Type</rdfs:label>
    <rdfs:label xml:lang="it">Tipo di azione Erasmus+</rdfs:label>
    <owl:versionInfo xml:lang="it">stabile</owl:versionInfo>
    <owl:versionInfo xml:lang="en">stable</owl:versionInfo>
    <ns6:wasDerivedFrom rdf:resource="http://www.w3.org/2004/02/skos/core#Concept"/>
  </rdf:Description>
  <rdf:Description rdf:about="https://w3id.org/italia/onto/HER/interventionModelDescription">
    <rdf:type rdf:resource="http://www.w3.org/2002/07/owl#DatatypeProperty"/>
    <rdfs:subPropertyOf rdf:resource="https://w3id.org/italia/onto/l0/description"/>
    <rdfs:domain rdf:resource="https://w3id.org/italia/onto/HER/AACTDesign"/>
    <rdfs:range rdf:resource="http://www.w3.org/2000/01/rdf-schema#Literal"/>
    <rdfs:comment xml:lang="it">Fornisce dettagli sul modello di studio utilizzato.</rdfs:comment>
    <rdfs:comment xml:lang="en">Provide details about the Interventional Study Model.</rdfs:comment>
    <rdfs:isDefinedBy rdf:resource="https://w3id.org/italia/onto/HER"/>
    <rdfs:label xml:lang="it">descrizione modello intervento</rdfs:label>
    <rdfs:label xml:lang="en">intervention model description</rdfs:label>
    <owl:versionInfo xml:lang="it">stabile</owl:versionInfo>
    <owl:versionInfo xml:lang="en">stable</owl:versionInfo>
  </rdf:Description>
  <rdf:Description rdf:about="https://w3id.org/italia/onto/HER/hasReportedCitizenship">
    <rdf:type rdf:resource="http://www.w3.org/2002/07/owl#ObjectProperty"/>
    <rdfs:domain rdf:nodeID="n5bb3bff42afb4ca286d2c3fead9507ddb81"/>
    <rdfs:range rdf:resource="https://w3id.org/italia/onto/HER/ReportedCitizenship"/>
    <rdfs:comment xml:lang="it">Questa proprietà si collega alla corrispondente cittadinanza segnalata dal sistema MIUR.</rdfs:comment>
    <rdfs:comment xml:lang="en">This property links to the corresponding citizenship reported by the MIUR system.</rdfs:comment>
    <rdfs:isDefinedBy rdf:resource="https://w3id.org/italia/onto/HER"/>
    <rdfs:label xml:lang="it">ha cittadinanza riportata</rdfs:label>
    <rdfs:label xml:lang="en">has reported citizenship</rdfs:label>
    <owl:versionInfo xml:lang="it">provvisoria</owl:versionInfo>
    <owl:versionInfo xml:lang="en">unstable</owl:versionInfo>
  </rdf:Description>
  <rdf:Description rdf:about="https://w3id.org/italia/onto/HER/admissionDate">
    <rdf:type rdf:resource="http://www.w3.org/2002/07/owl#DatatypeProperty"/>
    <rdfs:subPropertyOf rdf:resource="https://w3id.org/italia/onto/TI/date"/>
    <rdfs:domain rdf:resource="https://w3id.org/italia/onto/HER/CTNPRINOperation"/>
    <rdfs:range rdf:resource="http://www.w3.org/2001/XMLSchema#date"/>
    <rdfs:comment xml:lang="it">Data del decreto di ammissione al finanziamento del progetto associato all'operazione</rdfs:comment>
    <rdfs:comment xml:lang="en">Date of the decree of admission to the financing of the project associated with the operation</rdfs:comment>
    <rdfs:isDefinedBy rdf:resource="https://w3id.org/italia/onto/HER"/>
    <rdfs:label xml:lang="en">admission date</rdfs:label>
    <rdfs:label xml:lang="it">data di ammissione</rdfs:label>
    <owl:versionInfo xml:lang="it">stabile</owl:versionInfo>
    <owl:versionInfo xml:lang="en">stable</owl:versionInfo>
  </rdf:Description>
  <rdf:Description rdf:about="https://w3id.org/italia/onto/HER">
    <rdf:type rdf:resource="http://www.w3.org/2002/07/owl#Ontology"/>
    <rdf:type rdf:resource="http://www.w3.org/2002/07/owl#NamedIndividual"/>
    <rdf:type rdf:resource="https://w3id.org/italia/onto/ADMS/SemanticAsset"/>
    <owl:versionIRI rdf:resource="https://w3id.org/italia/onto/HER/0.4"/>
    <owl:imports rdf:resource="https://w3id.org/italia/onto/CPV"/>
    <owl:imports rdf:resource="https://w3id.org/italia/onto/Project"/>
    <owl:imports rdf:resource="https://w3id.org/italia/onto/l0"/>
    <ns2:accrualPeriodicity rdf:resource="http://publications.europa.eu/resource/authority/frequency/IRREG"/>
    <ns2:creator rdf:resource="https://w3id.org/italia/data/public-organization/agid"/>
    <ns2:creator rdf:resource="https://w3id.org/italia/data/public-organization/r_toscan"/>
    <ns2:creator rdf:resource="https://w3id.org/italia/datq/private-organization/siris"/>
    <ns2:creator rdf:resource="https://w3id.org/italia/datq/private-organization/03033080213"/>
    <ns2:description xml:lang="it">Questa è l'ontologia del profilo di italiano sull'alta formazione, ricerca e innovazione. Essa nasce come versione per OntoPiA dell'ontologia sviluppata nell'ambito del progetto Toscana Open Research (http://www.toscanaopenresearch.it/) disponibile in https://ontology-documentation-toscana-public.s3-eu-west-1.amazonaws.com/index.html#unics_miur_scholars</ns2:description>
    <ns2:description xml:lang="en">This is the ontology of the Italian application profile for Higher Education and Research. It is born as the OntoPiA's version of the ontology already developed in the context of Toscana Open Research Project (http://www.toscanaopenresearch.it/en/) and available in https://ontology-documentation-toscana-public.s3-eu-west-1.amazonaws.com/index.html#unics_miur_scholars</ns2:description>
    <ns2:issued rdf:datatype="http://www.w3.org/2001/XMLSchema#date">2020-04-02</ns2:issued>
    <ns2:language rdf:resource="http://publications.europa.eu/resource/authority/language/ENG"/>
    <ns2:language rdf:resource="http://publications.europa.eu/resource/authority/language/ITA"/>
    <ns2:modified xml:lang="en">2020-11-06</ns2:modified>
    <ns2:publisher rdf:resource="https://w3id.org/italia/data/public-organization/agid"/>
    <ns2:rightsHolder rdf:resource="https://w3id.org/italia/data/public-organization/r_toscan"/>
    <ns2:title xml:lang="en">Higher Education and Research Ontology</ns2:title>
    <ns2:title xml:lang="it">Ontologia sull'Alta Formazione, Ricerca e Innovazione</ns2:title>
    <rdfs:comment xml:lang="it">Questa è l'ontologia del profilo di italiano sull'alta formazione, ricerca e innovazione. Essa nasce come versione per OntoPiA dell'ontologia sviluppata nell'ambito del progetto Toscana Open Research (http://www.toscanaopenresearch.it/) disponibile in https://ontology-documentation-toscana-public.s3-eu-west-1.amazonaws.com/index.html#unics_miur_scholars</rdfs:comment>
    <rdfs:comment xml:lang="en">This is the ontology of the Italian application profile for Higher Education and Research. It is born as the OntoPiA's version of the ontology already developed in the context of Toscana Open Research Project (http://www.toscanaopenresearch.it/en/) and available in https://ontology-documentation-toscana-public.s3-eu-west-1.amazonaws.com/index.html#unics_miur_scholars</rdfs:comment>
    <rdfs:isDefinedBy rdf:resource="https://w3id.org/italia/onto/HER"/>
    <rdfs:label xml:lang="en">Higher Education and Research Ontology</rdfs:label>
    <rdfs:label xml:lang="it">Ontologia dell'Alta Formazione, Ricerca e Innovazione</rdfs:label>
    <owl:versionInfo xml:lang="en">Version 0.4 in OntoPiA</owl:versionInfo>
    <owl:versionInfo xml:lang="it">Versione 0.4 in OntoPiA</owl:versionInfo>
    <ns3:contactPoint rdf:resource="https://w3id.org/italia/data/contact-point/onto-agid"/>
    <ns3:keyword xml:lang="it">Peronale universitario</ns3:keyword>
    <ns3:keyword xml:lang="it">Progetti di ricerca</ns3:keyword>
    <ns3:keyword xml:lang="en">Public Research</ns3:keyword>
    <ns3:keyword xml:lang="en">Research Projects</ns3:keyword>
    <ns3:keyword xml:lang="it">Ricerca pubblica</ns3:keyword>
    <ns3:keyword xml:lang="en">Student</ns3:keyword>
    <ns3:keyword xml:lang="it">Studenti</ns3:keyword>
    <ns3:theme rdf:resource="http://publications.europa.eu/resource/authority/data-theme/EDUC"/>
    <ns6:wasDerivedFrom rdf:resource="https://w3id.org/italia/onto/HER/0.1"/>
    <ns1:acronym>HER-AP_IT</ns1:acronym>
    <ns1:hasFormalityLevel rdf:resource="https://w3id.org/italia/onto/ADMS/Formal"/>
    <ns1:hasKeyClass rdf:resource="https://w3id.org/italia/onto/HER/PublicResearchProject"/>
    <ns1:hasOntologyLanguage rdf:resource="https://w3id.org/italia/onto/ADMS/OWL"/>
    <ns1:hasSemanticAssetDistribution rdf:resource="https://w3id.org/italia/data/distribution/HERAPIT-JSON-LD"/>
    <ns1:hasSemanticAssetDistribution rdf:resource="https://w3id.org/italia/data/distribution/HERAPIT-RDF-TURTLE"/>
    <ns1:hasSemanticAssetDistribution rdf:resource="https://w3id.org/italia/data/distribution/HERAPIT-RDF-XML"/>
    <ns1:hasTask rdf:resource="https://w3id.org/italia/onto/ADMS/AnnotationTask"/>
    <ns1:hasTask rdf:resource="https://w3id.org/italia/onto/ADMS/QueryFormulationTask"/>
    <ns1:hasTask rdf:resource="https://w3id.org/italia/onto/ADMS/SearchTask"/>
    <ns1:last rdf:resource="https://w3id.org/italia/onto/CLV/1.0"/>
    <ns1:last rdf:resource="https://w3id.org/italia/onto/HER/0.3"/>
    <ns1:officialURI rdf:datatype="http://www.w3.org/2001/XMLSchema#anyURI">https://w3id.org/italia/onto/HER</ns1:officialURI>
    <ns1:prefix>herapit</ns1:prefix>
    <ns1:semanticAssetInUse rdf:resource="https://w3id.org/italia/data/project/OntoPiA"/>
    <ns1:semanticAssetInUse rdf:resource="https://w3id.org/italia/data/project/toscana-open-research"/>
    <ns1:status>draft</ns1:status>
    <ns1:target>Imprese</ns1:target>
    <ns1:target>Pubbliche Amministrazioni</ns1:target>
    <ns1:type rdf:resource="https://w3id.org/italia/onto/ADMS/DomainOntology"/>
  </rdf:Description>
  <rdf:Description rdf:nodeID="n5bb3bff42afb4ca286d2c3fead9507ddb452">
    <rdf:type rdf:resource="http://www.w3.org/2002/07/owl#Restriction"/>
    <owl:onProperty rdf:resource="https://w3id.org/italia/onto/HER/ecGrantAgreementNo"/>
    <owl:cardinality rdf:datatype="http://www.w3.org/2001/XMLSchema#nonNegativeInteger">1</owl:cardinality>
  </rdf:Description>
  <rdf:Description rdf:about="https://w3id.org/italia/onto/HER/ecMaxContribution">
    <rdf:type rdf:resource="http://www.w3.org/2002/07/owl#DatatypeProperty"/>
    <rdfs:subPropertyOf rdf:resource="https://w3id.org/italia/onto/MU/value"/>
    <rdfs:domain rdf:nodeID="n5bb3bff42afb4ca286d2c3fead9507ddb165"/>
    <rdfs:range rdf:resource="http://www.w3.org/2001/XMLSchema#decimal"/>
    <rdfs:comment xml:lang="it">La parte di costo di un progetto CE finanziata dall'Unione Europea. L'importo è espresso in euro.</rdfs:comment>
    <rdfs:comment xml:lang="en">The part of an EC project's cost that is funded by European Union. The amount is expressed in euros.</rdfs:comment>
    <rdfs:isDefinedBy rdf:resource="https://w3id.org/italia/onto/HER"/>
    <rdfs:label xml:lang="en">EC maximum contribution</rdfs:label>
    <rdfs:label xml:lang="it">massimo contributo CE</rdfs:label>
    <owl:versionInfo xml:lang="it">stabile</owl:versionInfo>
    <owl:versionInfo xml:lang="en">stable</owl:versionInfo>
  </rdf:Description>
  <rdf:Description rdf:nodeID="n5bb3bff42afb4ca286d2c3fead9507ddb389">
    <rdf:type rdf:resource="http://www.w3.org/2002/07/owl#Restriction"/>
    <owl:onProperty rdf:resource="https://w3id.org/italia/onto/HER/dispositionFirstSubmittedQCDate"/>
    <owl:maxQualifiedCardinality rdf:datatype="http://www.w3.org/2001/XMLSchema#nonNegativeInteger">1</owl:maxQualifiedCardinality>
    <owl:onDataRange rdf:resource="http://www.w3.org/2001/XMLSchema#date"/>
  </rdf:Description>
  <rdf:Description rdf:about="https://w3id.org/italia/onto/HER/USTATInterventionExpensesAggregate">
    <rdf:type rdf:resource="http://www.w3.org/2002/07/owl#Class"/>
    <rdfs:subClassOf rdf:resource="https://w3id.org/italia/onto/HER/StatisticalDataAggregation"/>
    <rdfs:comment xml:lang="en">Information on the expenditure committed for interventions granted to students for each University/Institute managed by each institution for the Right to University Studies (DSU)/Office, for the calendar year of reference.</rdfs:comment>
    <rdfs:comment xml:lang="it">Informazione sulla spesa impegnata per interventi concessi a studenti per ciascun Ateneo/Istituto gestito da ciascun ente per il DSU/ufficio, per l'anno solare di riferimento.</rdfs:comment>
    <rdfs:isDefinedBy rdf:resource="https://w3id.org/italia/onto/HER"/>
    <rdfs:label xml:lang="it">Aggregazione degli interventi di spese universitarie riportate da USTAT</rdfs:label>
    <rdfs:label xml:lang="en">USTAT Aggregate of University Intervention Expenses</rdfs:label>
    <owl:versionInfo xml:lang="it">stabile</owl:versionInfo>
    <owl:versionInfo xml:lang="en">stable</owl:versionInfo>
  </rdf:Description>
  <rdf:Description rdf:nodeID="n5bb3bff42afb4ca286d2c3fead9507ddb100">
    <rdf:first rdf:resource="https://w3id.org/italia/onto/HER/USTATExpenseClass"/>
    <rdf:rest rdf:nodeID="n5bb3bff42afb4ca286d2c3fead9507ddb101"/>
  </rdf:Description>
  <rdf:Description rdf:about="https://w3id.org/italia/onto/HER/numberOfFinancedProposals">
    <rdf:type rdf:resource="http://www.w3.org/2002/07/owl#DatatypeProperty"/>
    <rdfs:domain rdf:resource="https://w3id.org/italia/onto/HER/CTNPRINInitiative"/>
    <rdfs:range rdf:resource="http://www.w3.org/2001/XMLSchema#int"/>
    <rdfs:comment xml:lang="it">Numero totale delle proposte finanziate dall'iniziativa in esame</rdfs:comment>
    <rdfs:comment xml:lang="en">Total number of proposals financed by the initiative under consideration</rdfs:comment>
    <rdfs:isDefinedBy rdf:resource="https://w3id.org/italia/onto/HER"/>
    <rdfs:label xml:lang="en">number of financed proposals</rdfs:label>
    <rdfs:label xml:lang="it">numero di proposte finanziate</rdfs:label>
    <owl:versionInfo xml:lang="it">stabile</owl:versionInfo>
    <owl:versionInfo xml:lang="en">stable</owl:versionInfo>
  </rdf:Description>
  <rdf:Description rdf:about="https://w3id.org/italia/onto/HER/WIPOIPCMainGroup">
    <rdf:type rdf:resource="http://www.w3.org/2002/07/owl#Class"/>
    <rdfs:subClassOf rdf:resource="https://w3id.org/italia/onto/HER/InternationalPatentClassification"/>
    <rdfs:comment xml:lang="it">La sottoclasse è seguita da un numero di "gruppo" composto da una a tre cifre, un tratto obliquo e un numero di almeno due cifre che rappresentano un "gruppo principale" o "sottogruppo".</rdfs:comment>
    <rdfs:comment xml:lang="en">The subclass is followed by a one-to-three-digit "group" number, an oblique stroke and a number of at least two digits representing a "main group" or "subgroup".</rdfs:comment>
    <rdfs:isDefinedBy rdf:resource="https://w3id.org/italia/onto/HER"/>
    <rdfs:label xml:lang="it">Gruppo principale WIPO ipc</rdfs:label>
    <rdfs:label xml:lang="en">WIPO IPC Main Group</rdfs:label>
    <owl:versionInfo xml:lang="it">stabile</owl:versionInfo>
    <owl:versionInfo xml:lang="en">stable</owl:versionInfo>
    <ns6:wasDerivedFrom rdf:resource="http://www.w3.org/2004/02/skos/core#Concept"/>
  </rdf:Description>
  <rdf:Description rdf:about="https://w3id.org/italia/onto/HER/hasIPC">
    <rdf:type rdf:resource="http://www.w3.org/2002/07/owl#ObjectProperty"/>
    <rdfs:subPropertyOf rdf:resource="https://w3id.org/italia/onto/l0/hasTopic"/>
    <rdfs:domain rdf:resource="https://w3id.org/italia/onto/HER/Result"/>
    <rdfs:range rdf:resource="https://w3id.org/italia/onto/HER/InternationalPatentClassification"/>
    <rdfs:comment xml:lang="it">Questa proprietà collega un brevetto con le corrispondenti etichette di classificazione IPC.</rdfs:comment>
    <rdfs:comment xml:lang="en">This property connects a patent with the corresponding IPC classification labels.</rdfs:comment>
    <rdfs:isDefinedBy rdf:resource="https://w3id.org/italia/onto/HER"/>
    <rdfs:label xml:lang="it">ha una classificazione internazione dei brevetti</rdfs:label>
    <rdfs:label xml:lang="en">has International Patent Classification</rdfs:label>
    <owl:versionInfo xml:lang="it">stabile</owl:versionInfo>
    <owl:versionInfo xml:lang="en">stable</owl:versionInfo>
  </rdf:Description>
  <rdf:Description rdf:about="https://w3id.org/italia/onto/HER/departmentName">
    <rdf:type rdf:resource="http://www.w3.org/2002/07/owl#DatatypeProperty"/>
    <rdfs:subPropertyOf rdf:resource="https://w3id.org/italia/onto/l0/name"/>
    <rdfs:domain rdf:resource="https://w3id.org/italia/onto/HER/ItalianPhDCourseByCycle"/>
    <rdfs:range rdf:resource="http://www.w3.org/2000/01/rdf-schema#Literal"/>
    <rdfs:comment xml:lang="it">Il nome del dipartimento universitario corrispondente.</rdfs:comment>
    <rdfs:comment xml:lang="en">The corresponding university'a department name.</rdfs:comment>
    <rdfs:isDefinedBy rdf:resource="https://w3id.org/italia/onto/HER"/>
    <rdfs:label xml:lang="en">department name</rdfs:label>
    <rdfs:label xml:lang="it">nome dipartimento</rdfs:label>
    <owl:versionInfo xml:lang="it">provvisoria - valutare l'uso della classe organizzazione con il nome</owl:versionInfo>
    <owl:versionInfo xml:lang="en">unstable - evaluate the possiblity to reuse directly organisation class</owl:versionInfo>
  </rdf:Description>
  <rdf:Description rdf:nodeID="n5bb3bff42afb4ca286d2c3fead9507ddb309">
    <rdf:first rdf:resource="https://w3id.org/italia/onto/HER/USTATPartiallyExoneratedStudentsAggregate"/>
    <rdf:rest rdf:nodeID="n5bb3bff42afb4ca286d2c3fead9507ddb310"/>
  </rdf:Description>
  <rdf:Description rdf:about="https://w3id.org/italia/onto/HER/totalMaster">
    <rdf:type rdf:resource="http://www.w3.org/2002/07/owl#DatatypeProperty"/>
    <rdfs:subPropertyOf rdf:resource="https://w3id.org/italia/onto/MU/value"/>
    <rdfs:domain rdf:nodeID="n5bb3bff42afb4ca286d2c3fead9507ddb345"/>
    <rdfs:range rdf:resource="http://www.w3.org/2000/01/rdf-schema#Literal"/>
    <rdfs:comment xml:lang="en">Total with respect to students in good standing with the payment of tuition fees enrolled in Level I and Level II master's courses.</rdfs:comment>
    <rdfs:comment xml:lang="it">Totale rispetto agli studenti in regola con il pagamento delle tasse universitarie iscritti a corsi di master di I e II livello.</rdfs:comment>
    <rdfs:isDefinedBy rdf:resource="https://w3id.org/italia/onto/HER"/>
    <rdfs:label xml:lang="en">total master</rdfs:label>
    <rdfs:label xml:lang="it">totale lauree magistrali</rdfs:label>
    <owl:versionInfo xml:lang="it">stabile</owl:versionInfo>
    <owl:versionInfo xml:lang="en">stable</owl:versionInfo>
  </rdf:Description>
  <rdf:Description rdf:about="https://w3id.org/italia/onto/HER/revocationDate">
    <rdf:type rdf:resource="http://www.w3.org/2002/07/owl#DatatypeProperty"/>
    <rdfs:subPropertyOf rdf:resource="https://w3id.org/italia/onto/TI/date"/>
    <rdfs:domain rdf:resource="https://w3id.org/italia/onto/HER/CTNPRINOperation"/>
    <rdfs:range rdf:resource="http://www.w3.org/2001/XMLSchema#date"/>
    <rdfs:comment xml:lang="it">Data di revoca nel contesto delle operazioni PRIN. La proprietà è valorizzata solo se la relativa proprietà revoca è utilizzata.</rdfs:comment>
    <rdfs:comment xml:lang="en">Date of revocation of an operation in the context of PRIN. It is valorized only if the revoked property is used.</rdfs:comment>
    <rdfs:isDefinedBy rdf:resource="https://w3id.org/italia/onto/HER"/>
    <rdfs:label xml:lang="it">data revoca</rdfs:label>
    <rdfs:label xml:lang="en">revocation date</rdfs:label>
    <owl:versionInfo xml:lang="it">stabile</owl:versionInfo>
    <owl:versionInfo xml:lang="en">stable</owl:versionInfo>
  </rdf:Description>
  <rdf:Description rdf:about="https://w3id.org/italia/onto/HER/ERCClassification">
    <rdf:type rdf:resource="http://www.w3.org/2002/07/owl#Class"/>
    <rdfs:subClassOf rdf:resource="https://w3id.org/italia/onto/HER/ECClassification"/>
    <rdfs:isDefinedBy rdf:resource="https://w3id.org/italia/onto/HER"/>
    <rdfs:label xml:lang="it">Classificazione ERC</rdfs:label>
    <rdfs:label xml:lang="en">ERC Classification</rdfs:label>
    <owl:versionInfo xml:lang="it">stabile</owl:versionInfo>
    <owl:versionInfo xml:lang="en">stable</owl:versionInfo>
    <ns6:wasDerivedFrom rdf:resource="http://www.w3.org/2004/02/skos/core#ConceptScheme"/>
  </rdf:Description>
  <rdf:Description rdf:nodeID="n5bb3bff42afb4ca286d2c3fead9507ddb440">
    <rdf:type rdf:resource="http://www.w3.org/2002/07/owl#Restriction"/>
    <owl:onProperty rdf:resource="https://w3id.org/italia/onto/HER/hasECActivityType"/>
    <owl:qualifiedCardinality rdf:datatype="http://www.w3.org/2001/XMLSchema#nonNegativeInteger">1</owl:qualifiedCardinality>
    <owl:onClass rdf:resource="https://w3id.org/italia/onto/HER/ECActivityType"/>
  </rdf:Description>
  <rdf:Description rdf:about="https://w3id.org/italia/onto/HER/CHAFEAParticipant">
    <rdf:type rdf:resource="http://www.w3.org/2002/07/owl#Class"/>
    <rdfs:subClassOf rdf:resource="https://w3id.org/italia/onto/RO/TimeIndexedRole"/>
    <rdfs:subClassOf rdf:nodeID="n5bb3bff42afb4ca286d2c3fead9507ddb400"/>
    <rdfs:subClassOf rdf:nodeID="n5bb3bff42afb4ca286d2c3fead9507ddb401"/>
    <rdfs:subClassOf rdf:nodeID="n5bb3bff42afb4ca286d2c3fead9507ddb402"/>
    <rdfs:subClassOf rdf:nodeID="n5bb3bff42afb4ca286d2c3fead9507ddb403"/>
    <rdfs:comment xml:lang="en">Involved Institutions</rdfs:comment>
    <rdfs:comment xml:lang="it">Istituzioni coinvolte</rdfs:comment>
    <rdfs:isDefinedBy rdf:resource="https://w3id.org/italia/onto/HER"/>
    <rdfs:label xml:lang="en">CHAFEA Participant</rdfs:label>
    <rdfs:label xml:lang="it">Partecipanti CHAFEA</rdfs:label>
    <owl:versionInfo xml:lang="it">stabile</owl:versionInfo>
    <owl:versionInfo xml:lang="en">stable</owl:versionInfo>
  </rdf:Description>
  <rdf:Description rdf:nodeID="n5bb3bff42afb4ca286d2c3fead9507ddb447">
    <rdf:type rdf:resource="http://www.w3.org/2002/07/owl#Restriction"/>
    <owl:onProperty rdf:resource="https://w3id.org/italia/onto/HER/hasSubjectArea"/>
    <owl:allValuesFrom rdf:resource="https://w3id.org/italia/onto/HER/ECSubjectArea"/>
  </rdf:Description>
  <rdf:Description rdf:about="https://w3id.org/italia/onto/HER/grant">
    <rdf:type rdf:resource="http://www.w3.org/2002/07/owl#DatatypeProperty"/>
    <rdfs:domain rdf:resource="https://w3id.org/italia/onto/HER/EUREKAParticipant"/>
    <rdfs:range rdf:resource="http://www.w3.org/2001/XMLSchema#decimal"/>
    <rdfs:comment xml:lang="en">Property used to indicate the funding in euros received by the EUREKA participant</rdfs:comment>
    <rdfs:comment xml:lang="it">Proprietà usata per indicare il contributo in euro ricevuto dai  partecipanti EUREKA</rdfs:comment>
    <rdfs:isDefinedBy rdf:resource="https://w3id.org/italia/onto/HER"/>
    <rdfs:label xml:lang="it">contributo (per partecipanti EUREKA)</rdfs:label>
    <rdfs:label xml:lang="en">grant (for EUREKA participant)</rdfs:label>
    <owl:versionInfo xml:lang="it">stabile</owl:versionInfo>
    <owl:versionInfo xml:lang="en">stable</owl:versionInfo>
  </rdf:Description>
  <rdf:Description rdf:about="https://w3id.org/italia/onto/HER/hasAcademicDegree">
    <rdf:type rdf:resource="http://www.w3.org/2002/07/owl#ObjectProperty"/>
    <rdfs:domain rdf:nodeID="n5bb3bff42afb4ca286d2c3fead9507ddb10"/>
    <rdfs:range rdf:resource="https://w3id.org/italia/onto/HER/AcademicDegree"/>
    <rdfs:comment xml:lang="it">Questa proprietà è collegata a un titolo accademico.</rdfs:comment>
    <rdfs:comment xml:lang="en">This property links to an academic degree.</rdfs:comment>
    <rdfs:isDefinedBy rdf:resource="https://w3id.org/italia/onto/HER"/>
    <rdfs:label xml:lang="it">ha una laurea</rdfs:label>
    <rdfs:label xml:lang="en">has academic degree</rdfs:label>
    <owl:versionInfo xml:lang="it">stabile</owl:versionInfo>
    <owl:versionInfo xml:lang="en">stable</owl:versionInfo>
  </rdf:Description>
  <rdf:Description rdf:about="https://w3id.org/italia/onto/HER/ctnprinOperationCommittedCredit">
    <rdf:type rdf:resource="http://www.w3.org/2002/07/owl#DatatypeProperty"/>
    <rdfs:subPropertyOf rdf:resource="https://w3id.org/italia/onto/MU/value"/>
    <rdfs:domain rdf:resource="https://w3id.org/italia/onto/HER/CTNPRINOperation"/>
    <rdfs:range rdf:resource="http://www.w3.org/2001/XMLSchema#decimal"/>
    <rdfs:comment xml:lang="it">Crediti impegnati dal Ministero sui costi ammessi a seguito di valutazione ex-ante (solo per imprese). Calcolati come somma dell'omologa variabile "committedCredit" presente a livello di aggregazione inferiore (committedCredit_amounts)</rdfs:comment>
    <rdfs:comment xml:lang="en">Credits committed by the Ministry on eligible costs following ex-ante evaluation (only for companies). Calculated as the sum of the homologous variable 'committedCredit' present at the lower aggregation level (committedCredit_amounts)</rdfs:comment>
    <rdfs:isDefinedBy rdf:resource="https://w3id.org/italia/onto/HER"/>
    <rdfs:label xml:lang="en">committed credit of CTN/PRIN operation</rdfs:label>
    <rdfs:label xml:lang="it">credito impegnato per operazioni CTN/PRIN</rdfs:label>
    <owl:versionInfo xml:lang="it">stabile</owl:versionInfo>
    <owl:versionInfo xml:lang="en">stable</owl:versionInfo>
  </rdf:Description>
  <rdf:Description rdf:nodeID="n5bb3bff42afb4ca286d2c3fead9507ddb392">
    <rdf:type rdf:resource="http://www.w3.org/2002/07/owl#Restriction"/>
    <owl:onProperty rdf:resource="https://w3id.org/italia/onto/HER/resultsFirstSubmittedQCDate"/>
    <owl:maxQualifiedCardinality rdf:datatype="http://www.w3.org/2001/XMLSchema#nonNegativeInteger">1</owl:maxQualifiedCardinality>
    <owl:onDataRange rdf:resource="http://www.w3.org/2001/XMLSchema#date"/>
  </rdf:Description>
  <rdf:Description rdf:nodeID="n5bb3bff42afb4ca286d2c3fead9507ddb417">
    <rdf:type rdf:resource="http://www.w3.org/2002/07/owl#Restriction"/>
    <owl:onProperty rdf:resource="https://w3id.org/italia/onto/HER/decreeDate"/>
    <owl:qualifiedCardinality rdf:datatype="http://www.w3.org/2001/XMLSchema#nonNegativeInteger">1</owl:qualifiedCardinality>
    <owl:onDataRange rdf:resource="http://www.w3.org/2001/XMLSchema#date"/>
  </rdf:Description>
  <rdf:Description rdf:about="https://w3id.org/italia/onto/HER/ipdTimeFrame">
    <rdf:type rdf:resource="http://www.w3.org/2002/07/owl#DatatypeProperty"/>
    <rdfs:domain rdf:resource="https://w3id.org/italia/onto/HER/AACTStudy"/>
    <rdfs:range rdf:resource="http://www.w3.org/2000/01/rdf-schema#Literal"/>
    <rdfs:comment xml:lang="en">A description of when the IPD and any additional supporting information will become available and for how long, including the start and end dates or period of availability. This may be provided as an absolute date (for example, starting in January 2025) or as a date relative to the time when summary data are published or otherwise made available (for example, starting 6 months after publication).</rdfs:comment>
    <rdfs:comment xml:lang="it">Una descrizione di quando il DPI ed eventuali informazioni aggiuntive di supporto saranno disponibili e per quanto tempo, incluse le date di inizio e fine o il periodo di disponibilità. Questa può essere fornita come data assoluta (ad esempio, a partire da gennaio 2025) o come data relativa al momento in cui i dati sintetici sono pubblicati o resi disponibili in altro modo (ad esempio, a partire da 6 mesi dopo la pubblicazione).</rdfs:comment>
    <rdfs:isDefinedBy rdf:resource="https://w3id.org/italia/onto/HER"/>
    <rdfs:label xml:lang="en">IPD time frame</rdfs:label>
    <rdfs:label xml:lang="it">Intervallo di tempo IPD</rdfs:label>
    <owl:versionInfo xml:lang="it">provvisoria - valutazione della possibilità di usare la classe Intervallo Temporale in quanto periodo di tempo</owl:versionInfo>
    <owl:versionInfo xml:lang="en">unstable - evaluation of the possibility to use the class TimeInterval since it seems a period of time.</owl:versionInfo>
  </rdf:Description>
  <rdf:Description rdf:about="https://w3id.org/italia/onto/HER/whyStopped">
    <rdf:type rdf:resource="http://www.w3.org/2002/07/owl#DatatypeProperty"/>
    <rdfs:domain rdf:resource="https://w3id.org/italia/onto/HER/AACTStudy"/>
    <rdfs:range rdf:resource="http://www.w3.org/2000/01/rdf-schema#Literal"/>
    <rdfs:comment xml:lang="en">A brief explanation of the reason(s) why such clinical study was stopped (for a clinical study that is "Suspended," "Terminated," or "Withdrawn" prior to its planned completion as anticipated by the protocol).</rdfs:comment>
    <rdfs:comment xml:lang="it">Una breve spiegazione delle ragioni per cui tale studio clinico è stato interrotto (per uno studio clinico "Sospeso", "Terminato" o "Ritirato" prima del suo completamento previsto, come previsto dal protocollo).</rdfs:comment>
    <rdfs:isDefinedBy rdf:resource="https://w3id.org/italia/onto/HER"/>
    <rdfs:label xml:lang="it">perchè bloccato</rdfs:label>
    <rdfs:label xml:lang="en">why stopped</rdfs:label>
    <owl:versionInfo xml:lang="it">stabile</owl:versionInfo>
    <owl:versionInfo xml:lang="en">stable</owl:versionInfo>
  </rdf:Description>
  <rdf:Description rdf:about="https://w3id.org/italia/onto/HER/hasDSUInterventionType">
    <rdf:type rdf:resource="http://www.w3.org/2002/07/owl#ObjectProperty"/>
    <rdfs:domain rdf:resource="https://w3id.org/italia/onto/HER/DSURightToUniversityStudiesAggregate"/>
    <rdfs:range rdf:resource="https://w3id.org/italia/onto/HER/DSUInterventionType"/>
    <rdfs:comment xml:lang="it">Questa proprietà collega l'informazione sui dati relativi agli interventi a favore degli studenti alla tipologia di intervento corrispondente.</rdfs:comment>
    <rdfs:comment xml:lang="en">This property links the information on student intervention data to the corresponding type of intervention.</rdfs:comment>
    <rdfs:isDefinedBy rdf:resource="https://w3id.org/italia/onto/HER"/>
    <rdfs:label xml:lang="it">ha tipo/classe di intervento DSU</rdfs:label>
    <rdfs:label xml:lang="en">has DSU intervention type</rdfs:label>
    <owl:versionInfo xml:lang="it">stabile</owl:versionInfo>
    <owl:versionInfo xml:lang="en">stable</owl:versionInfo>
  </rdf:Description>
  <rdf:Description rdf:about="https://w3id.org/italia/onto/HER/expandedAccessType">
    <rdf:type rdf:resource="http://www.w3.org/2002/07/owl#DatatypeProperty"/>
    <rdfs:domain rdf:resource="https://w3id.org/italia/onto/HER/AACTStudy"/>
    <rdfs:range rdf:nodeID="n5bb3bff42afb4ca286d2c3fead9507ddb174"/>
    <rdfs:comment xml:lang="en">Property used to indicate the type of expanded access for the AACT study. (A way for patients with serious diseases or conditions who cannot participate in a clinical trial to gain access to a medical product that has not been approved by the U.S. Food and Drug Administration (FDA). Also called compassionate use.).
The type can be:
"Individual" -- it allows a single patient, with a serious disease or condition who cannot participate in a clinical trial, access to a drug or biological product that has not been approved by the FDA. This category also includes access in an emergency situation.);
"Intermediate" -- it allows more than one patient (but generally fewer patients than through a Treatment IND/Protocol) access to a drug or biological product that has not been approved by the FDA. This type of expanded access is used when multiple patients with the same disease or condition seek access to a specific drug or biological product that has not been approved by the FDA;
"Treatment" --it allows a large, widespread population access to a drug or biological product that has not been approved by the FDA. This type of expanded access can only be provided if the product is already being developed for marketing for the same use as the expanded access use.</rdfs:comment>
    <rdfs:comment xml:lang="it">Proprietà utilizzata per indicare il tipo di accesso esteso per lo studio AACT. (Un modo per i pazienti con malattie o condizioni gravi che non possono partecipare a uno studio clinico per ottenere l'accesso a un prodotto medico che non è stato approvato dalla Food and Drug Administration (FDA) degli Stati Uniti. Chiamato anche uso compassionevole).
Il tipo può essere:
"Individuale" -- permette a un singolo paziente, con una malattia o condizione grave che non può partecipare a una sperimentazione clinica, di accedere a un farmaco o a un prodotto biologico che non è stato approvato dalla FDA. Questa categoria comprende anche l'accesso in una situazione di emergenza);
"Intermedio" -- permette a più di un paziente (ma generalmente meno pazienti che attraverso un trattamento IND/Protocollo) l'accesso a un farmaco o prodotto biologico che non è stato approvato dalla FDA. Questo tipo di accesso esteso viene utilizzato quando più pazienti con la stessa malattia o condizione cercano di accedere a un farmaco o prodotto biologico specifico che non è stato approvato dalla FDA;
"Trattamento" -- permette a una vasta e diffusa popolazione di accedere a un farmaco o prodotto biologico che non è stato approvato dalla FDA. Questo tipo di accesso esteso può essere fornito solo se il prodotto è già in fase di sviluppo per la commercializzazione per lo stesso uso dell'accesso esteso.</rdfs:comment>
    <rdfs:isDefinedBy rdf:resource="https://w3id.org/italia/onto/HER"/>
    <rdfs:label xml:lang="en">expanded access type</rdfs:label>
    <rdfs:label xml:lang="it">tipo accesso esteso</rdfs:label>
    <owl:versionInfo xml:lang="it">stabile</owl:versionInfo>
    <owl:versionInfo xml:lang="en">stable</owl:versionInfo>
  </rdf:Description>
  <rdf:Description rdf:about="https://w3id.org/italia/onto/HER/numberOfSubmittedProposals">
    <rdf:type rdf:resource="http://www.w3.org/2002/07/owl#DatatypeProperty"/>
    <rdfs:domain rdf:resource="https://w3id.org/italia/onto/HER/CTNPRINInitiative"/>
    <rdfs:range rdf:resource="http://www.w3.org/2001/XMLSchema#int"/>
    <rdfs:comment xml:lang="it">Numero totale delle proposte presentate per l'iniziativa in esame</rdfs:comment>
    <rdfs:comment xml:lang="en">Total number of proposals submitted for the initiative under consideration</rdfs:comment>
    <rdfs:isDefinedBy rdf:resource="https://w3id.org/italia/onto/HER"/>
    <rdfs:label xml:lang="en">number of submitted proposals</rdfs:label>
    <rdfs:label xml:lang="it">numero di proposte inviate</rdfs:label>
    <owl:versionInfo xml:lang="it">stabile</owl:versionInfo>
    <owl:versionInfo xml:lang="en">stable</owl:versionInfo>
  </rdf:Description>
  <rdf:Description rdf:about="https://w3id.org/italia/onto/HER/planToShareIPDDescription">
    <rdf:type rdf:resource="http://www.w3.org/2002/07/owl#DatatypeProperty"/>
    <rdfs:subPropertyOf rdf:resource="https://w3id.org/italia/onto/l0/description"/>
    <rdfs:domain rdf:resource="https://w3id.org/italia/onto/HER/AACTStudy"/>
    <rdfs:range rdf:resource="http://www.w3.org/2000/01/rdf-schema#Literal"/>
    <rdfs:comment xml:lang="en">If Plan to Share IPD is "Yes," briefly describe what specific individual participant data sets are to be shared (for example, all collected IPD, all IPD that underlie results in a publication). If the Plan to Share IPD is "No" or "Undecided," an explanation may be provided for why IPD will not be shared or why it is not yet decided.</rdfs:comment>
    <rdfs:comment xml:lang="it">Se Plan to Share IPD è "Sì", descrive brevemente quali specifici set di dati dei singoli partecipanti devono essere condivisi (ad esempio, tutti gli IPD raccolti, tutti gli IPD che sono alla base di una pubblicazione). Se l'IPD del Piano di condivisione è "No" o "Indeciso", può essere fornita una spiegazione del perché l'IPD non sarà condiviso o perché non è ancora stato deciso.</rdfs:comment>
    <rdfs:isDefinedBy rdf:resource="https://w3id.org/italia/onto/HER"/>
    <rdfs:label xml:lang="en">description of plan to share IPD</rdfs:label>
    <rdfs:label xml:lang="it">descrizione del piano di condivisione del DPI</rdfs:label>
    <owl:versionInfo xml:lang="it">stabile</owl:versionInfo>
    <owl:versionInfo xml:lang="en">stable</owl:versionInfo>
  </rdf:Description>
  <rdf:Description rdf:about="https://w3id.org/italia/onto/COV/hasPublicOrganization">
    <rdf:type rdf:resource="http://www.w3.org/2002/07/owl#ObjectProperty"/>
  </rdf:Description>
  <rdf:Description rdf:nodeID="n5bb3bff42afb4ca286d2c3fead9507ddb49">
    <rdf:first rdf:resource="https://w3id.org/italia/onto/HER/ERCProject"/>
    <rdf:rest rdf:resource="http://www.w3.org/1999/02/22-rdf-syntax-ns#nil"/>
  </rdf:Description>
  <rdf:Description rdf:about="https://w3id.org/italia/onto/HER/ItalianAcademicRole">
    <rdf:type rdf:resource="http://www.w3.org/2002/07/owl#Class"/>
    <rdfs:subClassOf rdf:resource="https://w3id.org/italia/onto/HER/AcademicRole"/>
    <rdfs:comment xml:lang="en">It refers to the academic position held. In the Italian university system,
there are the following academic roles:
- Full professor (or first-tier professor) who is admitted after a competition;
- Associate professor (or second level professor) to whom access is granted following a competition;
- Adjunct professor;
- Temporary lecturer;
- Assistant Professor;
- Research fellow;
- Assistant Professor (tenure track);
- Postdoctoral Researcher
- Professor Emeritus</rdfs:comment>
    <rdfs:comment xml:lang="it">Si riferisce alla posizione accademica ricoperta. Nel sistema universitario italiano,
ci sono i seguenti ruoli accademici:
- Professore ordinario (o professore di primo livello) che viene ammesso dopo un concorso;
- Professore associato (o professore di secondo livello) al quale viene concesso l'accesso a seguito di un concorso;
- Professore aggiunto;
- Docente temporaneo;
- Professore assistente;
- Ricercatore;
- Professore assistente (cattedra di ruolo);
- Ricercatore post-dottorato
- Professore emerito</rdfs:comment>
    <rdfs:isDefinedBy rdf:resource="https://w3id.org/italia/onto/HER"/>
    <rdfs:label xml:lang="en">Italian Academic Role</rdfs:label>
    <rdfs:label xml:lang="it">Ruolo accademico italiano</rdfs:label>
    <owl:versionInfo xml:lang="it">stabile</owl:versionInfo>
    <owl:versionInfo xml:lang="en">stable</owl:versionInfo>
    <ns6:wasDerivedFrom rdf:resource="http://www.w3.org/2004/02/skos/core#Concept"/>
    <ns4:controlledVocabulary rdf:resource="https://w3id.org/italia/controlled-vocabulary/classifications-for-universitites/italian-academic-roles"/>
  </rdf:Description>
  <rdf:Description rdf:nodeID="n5bb3bff42afb4ca286d2c3fead9507ddb314">
    <rdf:type rdf:resource="http://www.w3.org/2002/07/owl#Class"/>
    <owl:unionOf rdf:nodeID="n5bb3bff42afb4ca286d2c3fead9507ddb315"/>
  </rdf:Description>
  <rdf:Description rdf:nodeID="n5bb3bff42afb4ca286d2c3fead9507ddb356">
    <rdf:type rdf:resource="http://www.w3.org/2002/07/owl#Class"/>
    <owl:unionOf rdf:nodeID="n5bb3bff42afb4ca286d2c3fead9507ddb357"/>
  </rdf:Description>
  <rdf:Description rdf:about="https://w3id.org/italia/onto/HER/ASJCSubjectArea">
    <rdf:type rdf:resource="http://www.w3.org/2002/07/owl#Class"/>
    <rdfs:subClassOf rdf:resource="https://w3id.org/italia/onto/HER/ASJC"/>
    <rdfs:comment xml:lang="en">The SCOPUS classification scheme contains 27 subject areas: Agricultural and Biological Sciences; Arts and Humanities; Biochemistry; Genetics and Molecular Biology; Business; Management and Accounting; Chemical Engineering; Chemistry; Computer Science; Decision Sciences; Dentistry; Earth and Planetary Science; Economics; Econometrics and Finance; Energy
Engineering; Environmental Science; Health Professions; Immunology and Microbiology; Materials Science; Mathematics; Medicine; Multidisciplinary; Neuroscience; Nursing; Pharmacology, Toxicology and Pharmaceutics; Physics and Astronomy; Psychology; Social Sciences; Veterinary

Attributes:
:name
:scopusSubjectAreaCode</rdfs:comment>
    <rdfs:isDefinedBy rdf:resource="https://w3id.org/italia/onto/HER"/>
    <owl:versionInfo xml:lang="it">stabile</owl:versionInfo>
    <owl:versionInfo xml:lang="en">stable</owl:versionInfo>
    <ns6:wasDerivedFrom rdf:resource="http://www.w3.org/2004/02/skos/core#Concept"/>
    <ns4:controlledVocabulary rdf:resource="https://w3id.org/italia/controlled-vocabulary/classifications-for-universities/all-science-journal"/>
  </rdf:Description>
  <rdf:Description rdf:nodeID="n5bb3bff42afb4ca286d2c3fead9507ddb465">
    <rdf:type rdf:resource="http://www.w3.org/2002/07/owl#Restriction"/>
    <owl:onProperty rdf:resource="https://w3id.org/italia/onto/HER/hasEurekaInstrument"/>
    <owl:qualifiedCardinality rdf:datatype="http://www.w3.org/2001/XMLSchema#nonNegativeInteger">1</owl:qualifiedCardinality>
    <owl:onClass rdf:resource="https://w3id.org/italia/onto/HER/EUREKAInstrument"/>
  </rdf:Description>
  <rdf:Description rdf:about="https://w3id.org/italia/onto/HER/hasUSTATPostgraduateCourse">
    <rdf:type rdf:resource="http://www.w3.org/2002/07/owl#ObjectProperty"/>
    <rdfs:domain rdf:nodeID="n5bb3bff42afb4ca286d2c3fead9507ddb102"/>
    <rdfs:range rdf:resource="https://w3id.org/italia/onto/HER/USTATReportedPostgraduateCourse"/>
    <rdfs:comment xml:lang="it">Questa proprietà collega l'informazione sulla popolazione di studenti o diplomati di corsi di formazione post-laurea al corso corrispondente.</rdfs:comment>
    <rdfs:comment xml:lang="en">This property links information about the population of students or graduates of postgraduate training courses to the corresponding course.</rdfs:comment>
    <rdfs:isDefinedBy rdf:resource="https://w3id.org/italia/onto/HER"/>
    <rdfs:label xml:lang="it">ha un corso di perfezionamento</rdfs:label>
    <rdfs:label xml:lang="en">has postgraduate course</rdfs:label>
    <owl:versionInfo xml:lang="it">stabile</owl:versionInfo>
    <owl:versionInfo xml:lang="en">stable</owl:versionInfo>
  </rdf:Description>
  <rdf:Description rdf:about="https://w3id.org/italia/onto/HER/aactMinimumAge">
    <rdf:type rdf:resource="http://www.w3.org/2002/07/owl#DatatypeProperty"/>
    <rdfs:subPropertyOf rdf:resource="https://w3id.org/italia/onto/CPV/age"/>
    <rdfs:domain rdf:resource="https://w3id.org/italia/onto/HER/AACTEligibility"/>
    <rdfs:range rdf:resource="http://www.w3.org/2001/XMLSchema#integer"/>
    <rdfs:comment xml:lang="it">L'eventuale valore numerico per l'età minima che un potenziale partecipante deve soddisfare per essere idoneo allo studio clinico.</rdfs:comment>
    <rdfs:comment xml:lang="en">The numerical value, if any, for the minimum age a potential participant must meet to be eligible for the clinical study.</rdfs:comment>
    <rdfs:isDefinedBy rdf:resource="https://w3id.org/italia/onto/HER"/>
    <rdfs:label xml:lang="en">AACT minimum age</rdfs:label>
    <rdfs:label xml:lang="it">etá minima AACT</rdfs:label>
    <owl:versionInfo xml:lang="it">stabile</owl:versionInfo>
    <owl:versionInfo xml:lang="en">stable</owl:versionInfo>
  </rdf:Description>
  <rdf:Description rdf:about="https://w3id.org/italia/onto/HER/ctnprinAmountAdmittedCost">
    <rdf:type rdf:resource="http://www.w3.org/2002/07/owl#DatatypeProperty"/>
    <rdfs:subPropertyOf rdf:resource="https://w3id.org/italia/onto/MU/value"/>
    <rdfs:domain rdf:resource="https://w3id.org/italia/onto/HER/CTNPRINAmount"/>
    <rdfs:range rdf:resource="http://www.w3.org/2001/XMLSchema#decimal"/>
    <rdfs:comment xml:lang="en">Cost admitted by decree after the evaluation of the costs indicated in the project proposal for each item of expenditure</rdfs:comment>
    <rdfs:comment xml:lang="it">Costo ammesso da decreto dopo la valutazione dei costo indicato nella proposta di progetto  per singola voce di spesa</rdfs:comment>
    <rdfs:isDefinedBy rdf:resource="https://w3id.org/italia/onto/HER"/>
    <rdfs:label xml:lang="en">admitted cost of CTN/PRIN amount</rdfs:label>
    <rdfs:label xml:lang="it">costo ammesso dell'importo CTN/PRIN</rdfs:label>
    <owl:versionInfo xml:lang="it">stabile</owl:versionInfo>
    <owl:versionInfo xml:lang="en">stable</owl:versionInfo>
  </rdf:Description>
  <rdf:Description rdf:about="https://w3id.org/italia/onto/HER/withAcademicRole">
    <rdf:type rdf:resource="http://www.w3.org/2002/07/owl#ObjectProperty"/>
    <rdfs:subPropertyOf rdf:resource="https://w3id.org/italia/onto/RO/withRole"/>
    <rdfs:domain rdf:resource="https://w3id.org/italia/onto/HER/AcademicAffiliation"/>
    <rdfs:range rdf:nodeID="n5bb3bff42afb4ca286d2c3fead9507ddb112"/>
    <rdfs:comment xml:lang="it">Questa proprietà collega un'affiliazione accademica con il ruolo accademico corrispondente.</rdfs:comment>
    <rdfs:comment xml:lang="en">This property connects an Academic Affiliation with the corresponding Academic Role.</rdfs:comment>
    <rdfs:isDefinedBy rdf:resource="https://w3id.org/italia/onto/HER"/>
    <rdfs:label xml:lang="it">con ruolo accademico</rdfs:label>
    <rdfs:label xml:lang="en">with academic role</rdfs:label>
    <owl:versionInfo xml:lang="it">stabile</owl:versionInfo>
    <owl:versionInfo xml:lang="en">stable</owl:versionInfo>
  </rdf:Description>
  <rdf:Description rdf:about="https://w3id.org/italia/onto/HER/MIURStudentsByCitizenshipDegreeAggregate">
    <rdf:type rdf:resource="http://www.w3.org/2002/07/owl#Class"/>
    <rdfs:subClassOf rdf:resource="https://w3id.org/italia/onto/HER/StatisticalDataAggregation"/>
    <rdfs:comment xml:lang="en">Aggregated data on Italian students filed in the MIUR system, grouped by year, university, citizenship and degree.</rdfs:comment>
    <rdfs:comment xml:lang="it">Dati aggregati sugli studenti italiani archiviati nel sistema MIUR, raggruppati per anno, università, cittadinanza e laurea.</rdfs:comment>
    <rdfs:isDefinedBy rdf:resource="https://w3id.org/italia/onto/HER"/>
    <rdfs:label xml:lang="en">Aggregate of Italian Students By Citizenship and Degree</rdfs:label>
    <rdfs:label xml:lang="it">Aggregazione dei studenti italiani per cittadinanza e laurea</rdfs:label>
    <owl:versionInfo xml:lang="it">stabile</owl:versionInfo>
    <owl:versionInfo xml:lang="en">stable</owl:versionInfo>
  </rdf:Description>
  <rdf:Description rdf:about="https://w3id.org/italia/onto/HER/documentationURL">
    <rdf:type rdf:resource="http://www.w3.org/2002/07/owl#DatatypeProperty"/>
    <rdfs:subPropertyOf rdf:resource="https://w3id.org/italia/onto/SM/URL"/>
    <rdfs:domain rdf:resource="https://w3id.org/italia/onto/HER/CTNPRINInitiative"/>
    <rdfs:range rdf:resource="http://www.w3.org/2001/XMLSchema#anyURI"/>
    <rdfs:comment xml:lang="it">Link a pagina web contenente il decreto del MIUR in cui è pubblicato il bando/avviso/... che prevede la concessione di finanziamenti per l'iniziativa in esame oltre ad eventuali allegati e decreti integrativi</rdfs:comment>
    <rdfs:comment xml:lang="en">Link to the web page containing the decree of the Ministry of Education, University and Research (MIUR) in which is published the call/announcement /... which provides for the granting of funding for the initiative in question, as well as any attachments and supplementary decrees.</rdfs:comment>
    <rdfs:isDefinedBy rdf:resource="https://w3id.org/italia/onto/HER"/>
    <rdfs:label xml:lang="it">URL documentazione</rdfs:label>
    <rdfs:label xml:lang="en">documentation URL</rdfs:label>
    <owl:versionInfo xml:lang="it">stabile</owl:versionInfo>
    <owl:versionInfo xml:lang="en">stable</owl:versionInfo>
  </rdf:Description>
  <rdf:Description rdf:nodeID="n5bb3bff42afb4ca286d2c3fead9507ddb54">
    <rdf:first rdf:resource="https://w3id.org/italia/onto/HER/CTNPRINOperation"/>
    <rdf:rest rdf:nodeID="n5bb3bff42afb4ca286d2c3fead9507ddb55"/>
  </rdf:Description>
  <rdf:Description rdf:about="https://w3id.org/italia/onto/HER/EUREKAMarketArea">
    <rdf:type rdf:resource="http://www.w3.org/2002/07/owl#Class"/>
    <rdfs:subClassOf rdf:resource="https://w3id.org/italia/onto/HER/HERClassification"/>
    <rdfs:comment xml:lang="it">Area di mercato EUREKA (Prodotti industriali / Produzione; Medicina / Salute; Trasporti; Consumer Related)</rdfs:comment>
    <rdfs:comment xml:lang="en">EUREKA Market area (Industrial Products / Manufacturing; Medical / Health Related; Transportation; Consumer Related)</rdfs:comment>
    <rdfs:isDefinedBy rdf:resource="https://w3id.org/italia/onto/HER"/>
    <rdfs:label xml:lang="it">Area di mercato EUREKA</rdfs:label>
    <rdfs:label xml:lang="en">EUREKA Market Area</rdfs:label>
    <owl:versionInfo xml:lang="it">stabile</owl:versionInfo>
    <owl:versionInfo xml:lang="en">stable</owl:versionInfo>
    <ns6:wasDerivedFrom rdf:resource="http://www.w3.org/2004/02/skos/core#Concept"/>
  </rdf:Description>
  <rdf:Description rdf:about="https://w3id.org/italia/onto/HER/hasUSTATMeasureOfMealsProvided">
    <rdf:type rdf:resource="http://www.w3.org/2002/07/owl#ObjectProperty"/>
    <rdfs:domain rdf:resource="https://w3id.org/italia/onto/HER/USTATMealsProvidedAggregate"/>
    <rdfs:range rdf:resource="https://w3id.org/italia/onto/HER/USTATMeasureOfMealsProvided"/>
    <rdfs:comment xml:lang="it">Questa proprietà collega l'informazione sui pasti erogati con la corrispondente tipologia.</rdfs:comment>
    <rdfs:comment xml:lang="en">This property links the information on the meals provided with the corresponding type.</rdfs:comment>
    <rdfs:isDefinedBy rdf:resource="https://w3id.org/italia/onto/HER"/>
    <rdfs:label xml:lang="en">measure of meals provided</rdfs:label>
    <rdfs:label xml:lang="it">misure dei pasti forniti</rdfs:label>
    <owl:versionInfo xml:lang="it">stabile</owl:versionInfo>
    <owl:versionInfo xml:lang="en">stable</owl:versionInfo>
  </rdf:Description>
  <rdf:Description rdf:nodeID="n5bb3bff42afb4ca286d2c3fead9507ddb145">
    <rdf:type rdf:resource="http://www.w3.org/1999/02/22-rdf-syntax-ns#List"/>
    <rdf:first>Development</rdf:first>
    <rdf:rest rdf:nodeID="n5bb3bff42afb4ca286d2c3fead9507ddb146"/>
  </rdf:Description>
  <rdf:Description rdf:nodeID="n5bb3bff42afb4ca286d2c3fead9507ddb88">
    <rdf:first rdf:resource="https://w3id.org/italia/onto/HER/CTNPRINOperation"/>
    <rdf:rest rdf:nodeID="n5bb3bff42afb4ca286d2c3fead9507ddb89"/>
  </rdf:Description>
  <rdf:Description rdf:about="https://w3id.org/italia/onto/HER/totalForeignFemale">
    <rdf:type rdf:resource="http://www.w3.org/2002/07/owl#DatatypeProperty"/>
    <rdfs:subPropertyOf rdf:resource="https://w3id.org/italia/onto/MU/value"/>
    <rdfs:domain rdf:nodeID="n5bb3bff42afb4ca286d2c3fead9507ddb328"/>
    <rdfs:range rdf:resource="http://www.w3.org/2000/01/rdf-schema#Literal"/>
    <rdfs:comment xml:lang="en">Total with respect to the population of women with foreign citizenship of the sample considered.</rdfs:comment>
    <rdfs:comment xml:lang="it">Totale rispetto alla popolazione di sesso femminile e con cittadinanza straniera del campione considerato.</rdfs:comment>
    <rdfs:isDefinedBy rdf:resource="https://w3id.org/italia/onto/HER"/>
    <rdfs:label xml:lang="en">total foreign female</rdfs:label>
    <rdfs:label xml:lang="it">totale di genere femminile straniero</rdfs:label>
    <owl:versionInfo xml:lang="it">stabile</owl:versionInfo>
    <owl:versionInfo xml:lang="en">stable</owl:versionInfo>
  </rdf:Description>
  <rdf:Description rdf:about="https://w3id.org/italia/onto/HER/startingYear">
    <rdf:type rdf:resource="http://www.w3.org/2002/07/owl#DatatypeProperty"/>
    <rdfs:subPropertyOf rdf:resource="https://w3id.org/italia/onto/TI/year"/>
    <rdfs:domain rdf:nodeID="n5bb3bff42afb4ca286d2c3fead9507ddb274"/>
    <rdfs:range rdf:resource="http://www.w3.org/2001/XMLSchema#gYear"/>
    <rdfs:comment xml:lang="en">Property used to model the starting year. Typically used for most of the Public Research Projects</rdfs:comment>
    <rdfs:comment xml:lang="it">Proprietà usata per modellare l'anno di inziio. Tipicamente utilizzata per la maggior parte dei progetti di ricerca pubblica.</rdfs:comment>
    <rdfs:isDefinedBy rdf:resource="https://w3id.org/italia/onto/HER"/>
    <rdfs:label xml:lang="it">anno inizio</rdfs:label>
    <rdfs:label xml:lang="en">starting year</rdfs:label>
    <owl:versionInfo xml:lang="it">stabile</owl:versionInfo>
    <owl:versionInfo xml:lang="en">stable</owl:versionInfo>
  </rdf:Description>
  <rdf:Description rdf:nodeID="n5bb3bff42afb4ca286d2c3fead9507ddb428">
    <rdf:type rdf:resource="http://www.w3.org/2002/07/owl#Restriction"/>
    <owl:onProperty rdf:resource="https://w3id.org/italia/onto/HER/ctnprinOperationIdentifier"/>
    <owl:cardinality rdf:datatype="http://www.w3.org/2001/XMLSchema#nonNegativeInteger">1</owl:cardinality>
  </rdf:Description>
  <rdf:Description rdf:nodeID="n5bb3bff42afb4ca286d2c3fead9507ddb42">
    <rdf:first rdf:resource="https://w3id.org/italia/onto/HER/ECProject"/>
    <rdf:rest rdf:nodeID="n5bb3bff42afb4ca286d2c3fead9507ddb43"/>
  </rdf:Description>
  <rdf:Description rdf:nodeID="n5bb3bff42afb4ca286d2c3fead9507ddb121">
    <rdf:first rdf:resource="https://w3id.org/italia/onto/Project/PublicResearchProject"/>
    <rdf:rest rdf:resource="http://www.w3.org/1999/02/22-rdf-syntax-ns#nil"/>
  </rdf:Description>
  <rdf:Description rdf:nodeID="n5bb3bff42afb4ca286d2c3fead9507ddb410">
    <rdf:type rdf:resource="http://www.w3.org/2002/07/owl#Restriction"/>
    <owl:onProperty rdf:resource="https://w3id.org/italia/onto/HER/startingYear"/>
    <owl:qualifiedCardinality rdf:datatype="http://www.w3.org/2001/XMLSchema#nonNegativeInteger">1</owl:qualifiedCardinality>
    <owl:onDataRange rdf:resource="http://www.w3.org/2001/XMLSchema#gYear"/>
  </rdf:Description>
  <rdf:Description rdf:nodeID="n5bb3bff42afb4ca286d2c3fead9507ddb248">
    <rdf:first rdf:resource="https://w3id.org/italia/onto/HER/ECParticipant"/>
    <rdf:rest rdf:nodeID="n5bb3bff42afb4ca286d2c3fead9507ddb249"/>
  </rdf:Description>
  <rdf:Description rdf:about="https://w3id.org/italia/onto/HER/hasEUREKAParticipant">
    <rdf:type rdf:resource="http://www.w3.org/2002/07/owl#ObjectProperty"/>
    <rdfs:subPropertyOf rdf:resource="https://w3id.org/italia/onto/RO/hasRiT"/>
    <rdfs:domain rdf:resource="https://w3id.org/italia/onto/HER/EUREKAProject"/>
    <rdfs:range rdf:resource="https://w3id.org/italia/onto/HER/EUREKAParticipant"/>
    <rdfs:comment xml:lang="it">Questa proprietà collega un progetto EUREKA con uno dei suoi partecipanti.</rdfs:comment>
    <rdfs:comment xml:lang="en">This property connects an EUREKA project with one of its participants.</rdfs:comment>
    <rdfs:isDefinedBy rdf:resource="https://w3id.org/italia/onto/HER"/>
    <rdfs:label xml:lang="it">ha partecipant EUREKA</rdfs:label>
    <rdfs:label xml:lang="en">has EUREKA participant</rdfs:label>
    <owl:versionInfo xml:lang="it">stabile</owl:versionInfo>
    <owl:versionInfo xml:lang="en">stable</owl:versionInfo>
  </rdf:Description>
  <rdf:Description rdf:nodeID="n5bb3bff42afb4ca286d2c3fead9507ddb530">
    <rdf:type rdf:resource="http://www.w3.org/2002/07/owl#Restriction"/>
    <owl:onProperty rdf:resource="https://w3id.org/italia/onto/COV/hasOrganization"/>
    <owl:maxQualifiedCardinality rdf:datatype="http://www.w3.org/2001/XMLSchema#nonNegativeInteger">1</owl:maxQualifiedCardinality>
    <owl:onClass rdf:resource="https://w3id.org/italia/onto/COV/Organization"/>
  </rdf:Description>
  <rdf:Description rdf:about="https://w3id.org/italia/onto/HER/hasAACTConditionMeshTerm">
    <rdf:type rdf:resource="http://www.w3.org/2002/07/owl#ObjectProperty"/>
    <rdfs:subPropertyOf rdf:resource="https://w3id.org/italia/onto/HER/hasAACTMeshTerm"/>
    <rdfs:domain rdf:resource="https://w3id.org/italia/onto/HER/AACTStudy"/>
    <rdfs:range rdf:resource="https://w3id.org/italia/onto/HER/AACTConditionMeshTerm"/>
    <rdfs:comment xml:lang="it">Il nome o i nomi della malattia o della condizione o delle condizioni studiate nello studio clinico, o il focus dello studio clinico descrittori appropriati da NLM's Medical Subject Headings (MeSH) - thesaurus vocabolario controllato da NLM's Medical Subject Headings (MeSH) - o termini da un altro vocabolario, come la Systematized Nomenclature of Medicine-Clinical Terms (SNOMED CT), che è stato mappato a MeSH all'interno del Metathesaurus Unified Medical Language System (UMLS).</rdfs:comment>
    <rdfs:comment xml:lang="en">The name(s) of the disease(s) or condition(s) studied in the clinical study, or the focus of the clinical study appropriate descriptors from NLM's Medical Subject Headings (MeSH)-controlled vocabulary thesaurus or terms from another vocabulary, such as the Systematized Nomenclature of Medicine—Clinical Terms (SNOMED CT), that has been mapped to MeSH within the Unified Medical Language System (UMLS) Metathesaurus.</rdfs:comment>
    <rdfs:isDefinedBy rdf:resource="https://w3id.org/italia/onto/HER"/>
    <rdfs:label xml:lang="it">ha termine MeSH di condizione AACT</rdfs:label>
    <rdfs:label xml:lang="en">has AACT condition MeSH term</rdfs:label>
    <owl:versionInfo xml:lang="it">stabile</owl:versionInfo>
    <owl:versionInfo xml:lang="en">stable</owl:versionInfo>
  </rdf:Description>
  <rdf:Description rdf:about="https://w3id.org/italia/onto/HER/USTATExpenseClass">
    <rdf:type rdf:resource="http://www.w3.org/2002/07/owl#Class"/>
    <rdfs:subClassOf rdf:resource="https://w3id.org/italia/onto/l0/Characteristic"/>
    <rdfs:comment xml:lang="it">Codice della spesa per tipologia di intervento. Corrispondono alle tipologie di intervento secondo le relazioni:
1 : Borse di studio - Spesa per borse concesse
2 : Borse di studio - Spesa per borse concesse - di cui Fondo Sociale Europeo
3 : Prestiti di onore e altri prestiti agevolati - Spesa per prestiti concessi
4 : Mobilità internazionale - Spesa per contributi concessi
5 : Interventi a favore di studenti in situazione di handicap - Spesa per interventi concessi
6 : Attività di collaborazione a tempo parziale - Spesa per attività di collaborazioni a tempo parziale
7 : Posti alloggio e contributi-alloggio - Spesa per contributi-alloggio assegnati
8 : Posti alloggio e contributi-alloggio - Spesa per contributi-alloggio assegnati - di cui spesa per contributi a borsisti (non beneficiari di alloggio)
9 : Posti alloggio e contributi-alloggio - Spesa per contributi-alloggio assegnati - di cui spesa per contributi a idonei non borsisti (non beneficiari di alloggio)
10 : Posti alloggio e contributi-alloggio - Spesa per contributi-alloggio assegnati - di cui spesa per contributi a studenti non idonei alla borsa
11 : Altri interventi di tipo finanziario - Spesa per premi per il conseguimento del titolo
12 : Altri interventi di tipo finanziario - Spesa per contributi finanziari per il trasporto
13 : Altri interventi di tipo finanziario - Spesa per contributi straordinari
14 : Altri interventi di tipo finanziario - Spesa per altri sussidi concessi</rdfs:comment>
    <rdfs:comment xml:lang="en">Spending code by type of intervention. They correspond to the types of intervention according to the reports:
1 : Scholarships - Expenditure for scholarships awarded
2 : Scholarships - Expenditure for grants - of which European Social Fund (Fondo Sociale Europeo)
3 : Honour loans and other subsidised loans - Expenditure on loans granted
4 : International mobility - Expenditure on granted contributions
5 : Interventions in favour of students with disabilities - Expenditure for interventions granted
6 : Part-time collaboration activities - Expenditure for part-time collaboration activities
7 : Accommodation places and accommodation contributions - Expenditure for allocated accommodation contributions
8 : Accommodation and accommodation grants - Expenditure for allocated accommodation grants - of which expenditure for grants to scholarship holders (not beneficiaries of accommodation)
9 : Accommodation and accommodation grants - Expenditure for allocated accommodation grants - of which expenditure for grants to eligible non-scholarship holders (non-beneficiaries of accommodation)
10 : Accommodation places and accommodation contributions - Expenditure for assigned accommodation contributions - of which expenditure for contributions to students not eligible for the grant
11 : Other financial measures - Expenditure on bonuses for obtaining the title
12 : Other financial interventions - Expenditure on financial contributions for transport
13 : Other financial interventions - Expenditure on extraordinary contributions
14 : Other financial interventions - Expenditure on other subsidies granted.
</rdfs:comment>
    <rdfs:isDefinedBy rdf:resource="https://w3id.org/italia/onto/HER"/>
    <rdfs:label xml:lang="it">Classe di spese riportata da USTAT</rdfs:label>
    <rdfs:label xml:lang="en">USTAT Reported Expense Class</rdfs:label>
    <owl:versionInfo xml:lang="it">stabile</owl:versionInfo>
    <owl:versionInfo xml:lang="en">stable</owl:versionInfo>
  </rdf:Description>
  <rdf:Description rdf:about="https://w3id.org/italia/onto/HER/totalGrant">
    <rdf:type rdf:resource="http://www.w3.org/2002/07/owl#DatatypeProperty"/>
    <rdfs:subPropertyOf rdf:resource="https://w3id.org/italia/onto/MU/value"/>
    <rdfs:domain rdf:nodeID="n5bb3bff42afb4ca286d2c3fead9507ddb336"/>
    <rdfs:range rdf:resource="http://www.w3.org/2001/XMLSchema#decimal"/>
    <rdfs:comment xml:lang="en">Project total grant</rdfs:comment>
    <rdfs:comment xml:lang="it">Totale contributo progetto</rdfs:comment>
    <rdfs:isDefinedBy rdf:resource="https://w3id.org/italia/onto/HER"/>
    <rdfs:label xml:lang="en">total grant</rdfs:label>
    <rdfs:label xml:lang="it">totale contributo</rdfs:label>
    <owl:versionInfo xml:lang="it">stabile</owl:versionInfo>
    <owl:versionInfo xml:lang="en">stable</owl:versionInfo>
  </rdf:Description>
  <rdf:Description rdf:about="https://w3id.org/italia/onto/HER/PHDCycle">
    <rdf:type rdf:resource="http://www.w3.org/2002/07/owl#DatatypeProperty"/>
    <rdfs:domain rdf:nodeID="n5bb3bff42afb4ca286d2c3fead9507ddb115"/>
    <rdfs:range rdf:resource="http://www.w3.org/2000/01/rdf-schema#Literal"/>
    <rdfs:comment xml:lang="it">Numero del ciclo del Dottorato di Ricerca. Valido solo per i corsi di Dottorato di Ricerca.</rdfs:comment>
    <rdfs:comment xml:lang="en">PhD cycle number. Only valid for PhD courses.</rdfs:comment>
    <rdfs:isDefinedBy rdf:resource="https://w3id.org/italia/onto/HER"/>
    <rdfs:label xml:lang="en">academic cycle</rdfs:label>
    <rdfs:label xml:lang="it">ciclo accademico</rdfs:label>
    <owl:versionInfo xml:lang="it">stabile</owl:versionInfo>
    <owl:versionInfo xml:lang="en">stable</owl:versionInfo>
  </rdf:Description>
  <rdf:Description rdf:about="https://w3id.org/italia/onto/HER/totalMaleGraduated">
    <rdf:type rdf:resource="http://www.w3.org/2002/07/owl#DatatypeProperty"/>
    <rdfs:subPropertyOf rdf:resource="https://w3id.org/italia/onto/MU/value"/>
    <rdfs:domain rdf:resource="https://w3id.org/italia/onto/HER/USTATStudentsBySexAggregate"/>
    <rdfs:range rdf:resource="http://www.w3.org/2000/01/rdf-schema#Literal"/>
    <rdfs:comment xml:lang="en">Number of male graduates corresponding to the selected combination of variables. In particular: Number of male students who graduated in the reference calendar year. Students of levels 6 and 7 of ISCED 2011.
For the year 2018: elaborations on ANS data - extraction December 2019.</rdfs:comment>
    <rdfs:comment xml:lang="it">Numero di laureati di genere maschile corrispondente alla combinazione di variabili selezionata. In particolare: Numero di studenti di genere maschile che si sono laureati nell’anno solare di riferimento. Studenti dei livelli 6 e 7 della ISCED 2011.
Per l'anno 2018: elaborazioni su dati ANS - estrazione Dicembre 2019.</rdfs:comment>
    <rdfs:isDefinedBy rdf:resource="https://w3id.org/italia/onto/HER"/>
    <rdfs:label xml:lang="en">total male graduated</rdfs:label>
    <rdfs:label xml:lang="it">totale di genere maschile laureato</rdfs:label>
    <owl:versionInfo xml:lang="it">stabile</owl:versionInfo>
    <owl:versionInfo xml:lang="en">stable</owl:versionInfo>
  </rdf:Description>
  <rdf:Description rdf:nodeID="n5bb3bff42afb4ca286d2c3fead9507ddb413">
    <rdf:type rdf:resource="http://www.w3.org/2002/07/owl#Restriction"/>
    <owl:onProperty rdf:resource="https://w3id.org/italia/onto/l0/identifier"/>
    <owl:cardinality rdf:datatype="http://www.w3.org/2001/XMLSchema#nonNegativeInteger">1</owl:cardinality>
  </rdf:Description>
  <rdf:Description rdf:nodeID="n5bb3bff42afb4ca286d2c3fead9507ddb272">
    <rdf:type rdf:resource="http://www.w3.org/1999/02/22-rdf-syntax-ns#List"/>
    <rdf:first>Non-Probability Sample</rdf:first>
    <rdf:rest rdf:nodeID="n5bb3bff42afb4ca286d2c3fead9507ddb273"/>
  </rdf:Description>
  <rdf:Description rdf:nodeID="n5bb3bff42afb4ca286d2c3fead9507ddb94">
    <rdf:first rdf:resource="https://w3id.org/italia/onto/HER/USTATPartiallyExoneratedStudentsAggregate"/>
    <rdf:rest rdf:nodeID="n5bb3bff42afb4ca286d2c3fead9507ddb95"/>
  </rdf:Description>
  <rdf:Description rdf:about="https://w3id.org/italia/onto/HER/phase">
    <rdf:type rdf:resource="http://www.w3.org/2002/07/owl#DatatypeProperty"/>
    <rdfs:domain rdf:resource="https://w3id.org/italia/onto/HER/AACTStudy"/>
    <rdfs:range rdf:resource="http://www.w3.org/2000/01/rdf-schema#Literal"/>
    <rdfs:comment xml:lang="it">La fase di uno studio clinico che studia un farmaco o un prodotto biologico, basato sulle definizioni sviluppate dalla Food and Drug Administration (FDA) degli Stati Uniti. La fase si basa sull'obiettivo dello studio, sul numero di partecipanti e su altre caratteristiche. Ci sono cinque fasi: Fase 1 iniziale (precedentemente elencata come Fase 0), Fase 1, Fase 2, Fase 3 e Fase 4. Non applicabile è utilizzato per descrivere studi senza fasi definite dall'FDA, compresi studi su dispositivi o interventi comportamentali.</rdfs:comment>
    <rdfs:comment xml:lang="en">The stage of a clinical trial studying a drug or biological product, based on definitions developed by the U.S. Food and Drug Administration (FDA). The phase is based on the study's objective, the number of participants, and other characteristics. There are five phases: Early Phase 1 (formerly listed as Phase 0), Phase 1, Phase 2, Phase 3, and Phase 4. Not Applicable is used to describe trials without FDA-defined phases, including trials of devices or behavioral interventions.</rdfs:comment>
    <rdfs:isDefinedBy rdf:resource="https://w3id.org/italia/onto/HER"/>
    <rdfs:label xml:lang="it">fase</rdfs:label>
    <rdfs:label xml:lang="en">phase</rdfs:label>
    <owl:versionInfo xml:lang="it">stabile</owl:versionInfo>
    <owl:versionInfo xml:lang="en">stable</owl:versionInfo>
  </rdf:Description>
  <rdf:Description rdf:about="https://w3id.org/italia/onto/HER/foundedBy">
    <rdf:type rdf:resource="http://www.w3.org/2002/07/owl#ObjectProperty"/>
    <rdfs:domain rdf:resource="https://w3id.org/italia/onto/HER/Spinoff"/>
    <rdfs:range rdf:resource="https://w3id.org/italia/onto/COV/Organization"/>
    <rdfs:comment xml:lang="en">It is used to link the spin-off to the research institution or university of origin, to which its foundation is linked.</rdfs:comment>
    <rdfs:comment xml:lang="it">Viene utilizzato per collegare lo spin-off all'ente di ricerca o ateneo di origine, a cui è collegata la sua fondazione.</rdfs:comment>
    <rdfs:isDefinedBy rdf:resource="https://w3id.org/italia/onto/HER"/>
    <rdfs:label xml:lang="it">fondata da</rdfs:label>
    <rdfs:label xml:lang="en">founded by</rdfs:label>
    <owl:versionInfo xml:lang="it">stabile</owl:versionInfo>
    <owl:versionInfo xml:lang="en">stable</owl:versionInfo>
  </rdf:Description>
  <rdf:Description rdf:nodeID="n5bb3bff42afb4ca286d2c3fead9507ddb312">
    <rdf:first rdf:resource="https://w3id.org/italia/onto/HER/DSURightToUniversityStudiesAggregate"/>
    <rdf:rest rdf:nodeID="n5bb3bff42afb4ca286d2c3fead9507ddb313"/>
  </rdf:Description>
  <rdf:Description rdf:about="https://w3id.org/italia/onto/HER/CountryInvolvement">
    <rdf:type rdf:resource="http://www.w3.org/2002/07/owl#Class"/>
    <rdfs:subClassOf rdf:resource="https://w3id.org/italia/onto/l0/EventOrSituation"/>
    <rdfs:subClassOf rdf:nodeID="n5bb3bff42afb4ca286d2c3fead9507ddb433"/>
    <rdfs:subClassOf rdf:nodeID="n5bb3bff42afb4ca286d2c3fead9507ddb434"/>
    <rdfs:subClassOf rdf:nodeID="n5bb3bff42afb4ca286d2c3fead9507ddb435"/>
    <rdfs:comment xml:lang="en">Country where the facility conducting a clinical protocol is located</rdfs:comment>
    <rdfs:comment xml:lang="it">Paese in cui si trova la struttura che conduce un protocollo clinico</rdfs:comment>
    <rdfs:isDefinedBy rdf:resource="https://w3id.org/italia/onto/HER"/>
    <rdfs:label xml:lang="it">Coinvolgimento del paese</rdfs:label>
    <rdfs:label xml:lang="en">Country Involvement</rdfs:label>
    <owl:versionInfo xml:lang="it">stabile</owl:versionInfo>
    <owl:versionInfo xml:lang="en">stable</owl:versionInfo>
  </rdf:Description>
  <rdf:Description rdf:about="https://w3id.org/italia/onto/HER/hasDispositionFirstPostedDate">
    <rdf:type rdf:resource="http://www.w3.org/2002/07/owl#ObjectProperty"/>
    <rdfs:subPropertyOf rdf:resource="https://w3id.org/italia/onto/TI/hasTemporalEntity"/>
    <rdfs:domain rdf:resource="https://w3id.org/italia/onto/HER/AACTStudy"/>
    <rdfs:range rdf:resource="https://w3id.org/italia/onto/TI#TimeInstant"/>
    <rdfs:comment xml:lang="it">Il suffisso _posted indica la data in cui una presentazione è stata resa pubblica su ClinicalTrials.gov. In genere, l'invio avviene il giorno lavorativo successivo al completamento della revisione del qc. Abbiamo iniziato a raccogliere le date di pubblicazione all'inizio del 2017. Le date precedenti a tale data sono estmate. Tutte le date pubblicate includono un attributo di tipo Actual o Estimate.</rdfs:comment>
    <rdfs:comment xml:lang="en">The _posted suffix indicates the date that a submission was made public on ClinicalTrials.gov. Typically, posting occurs the business day after qc review was successfully completed. We began collecting posted dates in early 2017. Dates from before then are estmates. All posted dates include a type attribute of Actual or Estimate.</rdfs:comment>
    <rdfs:isDefinedBy rdf:resource="https://w3id.org/italia/onto/HER"/>
    <rdfs:label xml:lang="it">ha disposizione prima data pubblicazione</rdfs:label>
    <rdfs:label xml:lang="en">has disposition first posted date</rdfs:label>
    <owl:versionInfo xml:lang="it">prova</owl:versionInfo>
    <owl:versionInfo xml:lang="en">testing</owl:versionInfo>
  </rdf:Description>
  <rdf:Description rdf:about="https://w3id.org/italia/onto/HER/PhDCourse">
    <rdf:type rdf:resource="http://www.w3.org/2002/07/owl#Class"/>
    <rdfs:subClassOf rdf:resource="https://w3id.org/italia/onto/l0/Object"/>
    <rdfs:comment xml:lang="en">A PhD course.</rdfs:comment>
    <rdfs:comment xml:lang="it">Un corso di dottorato di ricerca.</rdfs:comment>
    <rdfs:isDefinedBy rdf:resource="https://w3id.org/italia/onto/HER"/>
    <rdfs:label xml:lang="it">Corso di dottorato</rdfs:label>
    <rdfs:label xml:lang="en">PhD Course</rdfs:label>
    <owl:versionInfo xml:lang="it">stabile</owl:versionInfo>
    <owl:versionInfo xml:lang="en">stable</owl:versionInfo>
  </rdf:Description>
  <rdf:Description rdf:nodeID="n5bb3bff42afb4ca286d2c3fead9507ddb253">
    <rdf:type rdf:resource="http://www.w3.org/1999/02/22-rdf-syntax-ns#List"/>
    <rdf:first>Yes</rdf:first>
    <rdf:rest rdf:resource="http://www.w3.org/1999/02/22-rdf-syntax-ns#nil"/>
  </rdf:Description>
  <rdf:Description rdf:about="https://w3id.org/italia/onto/HER/DegreeClass">
    <rdf:type rdf:resource="http://www.w3.org/2002/07/owl#Class"/>
    <rdfs:subClassOf rdf:resource="https://w3id.org/italia/onto/HER/HERClassification"/>
    <rdfs:comment xml:lang="it">http://www.miur.it/0002Univer/0021Offert/index_cf2.htm

- Determinazione delle classi delle lauree universitarie (1-42)
http://www.miur.it/UserFiles/521.pdf

- Determinazione delle classi delle lauree specialistiche (1-104)</rdfs:comment>
    <rdfs:isDefinedBy rdf:resource="https://w3id.org/italia/onto/HER"/>
    <rdfs:label xml:lang="en">Italian Degree Class</rdfs:label>
    <rdfs:label xml:lang="it">Tipo di laurea italiana</rdfs:label>
    <owl:versionInfo xml:lang="it">stabile</owl:versionInfo>
    <owl:versionInfo xml:lang="en">stable</owl:versionInfo>
    <ns6:wasDerivedFrom rdf:resource="http://www.w3.org/2004/02/skos/core#Concept"/>
  </rdf:Description>
  <rdf:Description rdf:about="https://w3id.org/italia/onto/HER/patentKindCode">
    <rdf:type rdf:resource="http://www.w3.org/2002/07/owl#DatatypeProperty"/>
    <rdfs:subPropertyOf rdf:resource="https://w3id.org/italia/onto/l0/identifier"/>
    <rdfs:domain rdf:nodeID="n5bb3bff42afb4ca286d2c3fead9507ddb244"/>
    <rdfs:range rdf:resource="http://www.w3.org/2000/01/rdf-schema#Literal"/>
    <rdfs:comment xml:lang="it">I codici OMPI ST.16 standard (codici tipo) includono una lettera e, in molti casi, un numero, utilizzato per distinguere il tipo di documento di brevetto (ad esempio, pubblicazione di una domanda di brevetto di utilità (pubblicazione di una domanda di brevetto), brevetto, brevetto vegetale pubblicazione di domanda, brevetto di impianto o brevetto di progettazione) e il livello di pubblicazione (ad es. prima pubblicazione, seconda pubblicazione o pubblicazione corretta).</rdfs:comment>
    <rdfs:comment xml:lang="en">WIPO Standard ST.16 codes (kind codes) include a letter, and in many cases a number, used to distinguish the kind of patent document (e.g., publication of an application for a utility patent (patent application publication), patent, plant patent application publication, plant patent, or design patent) and the level of publication (e.g., first publication, second publication, or corrected publication).</rdfs:comment>
    <rdfs:isDefinedBy rdf:resource="https://w3id.org/italia/onto/HER"/>
    <rdfs:label xml:lang="it">codice tipologia brevetto</rdfs:label>
    <rdfs:label xml:lang="en">patent kind code</rdfs:label>
    <owl:versionInfo xml:lang="it">stabile</owl:versionInfo>
    <owl:versionInfo xml:lang="en">stable</owl:versionInfo>
  </rdf:Description>
  <rdf:Description rdf:about="https://w3id.org/italia/onto/HER/ASJCField">
    <rdf:type rdf:resource="http://www.w3.org/2002/07/owl#Class"/>
    <rdfs:subClassOf rdf:resource="https://w3id.org/italia/onto/HER/ASJC"/>
    <rdfs:comment xml:lang="en">Journals are assigned to 27 major thematic categories as well as to 313 specific subject categories according to Scopus® Classification.</rdfs:comment>
    <rdfs:isDefinedBy rdf:resource="https://w3id.org/italia/onto/HER"/>
    <owl:versionInfo xml:lang="it">stabile</owl:versionInfo>
    <owl:versionInfo xml:lang="en">stable</owl:versionInfo>
    <ns6:wasDerivedFrom rdf:resource="http://www.w3.org/2004/02/skos/core#Concept"/>
    <ns4:controlledVocabulary rdf:resource="https://w3id.org/italia/controlled-vocabulary/classifications-for-universities/all-science-journal"/>
  </rdf:Description>
  <rdf:Description rdf:nodeID="n5bb3bff42afb4ca286d2c3fead9507ddb56">
    <rdf:first rdf:resource="https://w3id.org/italia/onto/HER/ECProject"/>
    <rdf:rest rdf:nodeID="n5bb3bff42afb4ca286d2c3fead9507ddb57"/>
  </rdf:Description>
  <rdf:Description rdf:about="https://w3id.org/italia/onto/HER/ECProject">
    <rdf:type rdf:resource="http://www.w3.org/2002/07/owl#Class"/>
    <rdfs:subClassOf rdf:resource="https://w3id.org/italia/onto/Project/PublicResearchProject"/>
    <rdfs:subClassOf rdf:nodeID="n5bb3bff42afb4ca286d2c3fead9507ddb445"/>
    <rdfs:subClassOf rdf:nodeID="n5bb3bff42afb4ca286d2c3fead9507ddb446"/>
    <rdfs:subClassOf rdf:nodeID="n5bb3bff42afb4ca286d2c3fead9507ddb447"/>
    <rdfs:subClassOf rdf:nodeID="n5bb3bff42afb4ca286d2c3fead9507ddb448"/>
    <rdfs:subClassOf rdf:nodeID="n5bb3bff42afb4ca286d2c3fead9507ddb449"/>
    <rdfs:subClassOf rdf:nodeID="n5bb3bff42afb4ca286d2c3fead9507ddb450"/>
    <rdfs:subClassOf rdf:nodeID="n5bb3bff42afb4ca286d2c3fead9507ddb451"/>
    <rdfs:subClassOf rdf:nodeID="n5bb3bff42afb4ca286d2c3fead9507ddb452"/>
    <rdfs:subClassOf rdf:nodeID="n5bb3bff42afb4ca286d2c3fead9507ddb453"/>
    <rdfs:subClassOf rdf:nodeID="n5bb3bff42afb4ca286d2c3fead9507ddb454"/>
    <rdfs:subClassOf rdf:nodeID="n5bb3bff42afb4ca286d2c3fead9507ddb455"/>
    <rdfs:subClassOf rdf:nodeID="n5bb3bff42afb4ca286d2c3fead9507ddb456"/>
    <rdfs:comment xml:lang="it">Progetto finanziato dai programmi quadro dell'UE per la ricerca e l'innovazione (dal 1° PQ1 a Horizon 2020) e pubblicato dalla Commissione europea sul servizio comunitario di informazione per la ricerca e lo sviluppo (CORDIS).</rdfs:comment>
    <rdfs:comment xml:lang="en">Project funded by the EU's framework programmes for research and innovation (FP1 to Horizon 2020) and published by the European Comission on the Community Research and Development Information Service (CORDIS).</rdfs:comment>
    <rdfs:isDefinedBy rdf:resource="https://w3id.org/italia/onto/HER"/>
    <rdfs:label xml:lang="en">EC Project</rdfs:label>
    <rdfs:label xml:lang="it">Progetto CE</rdfs:label>
    <owl:versionInfo xml:lang="it">stabile</owl:versionInfo>
    <owl:versionInfo xml:lang="en">stable</owl:versionInfo>
  </rdf:Description>
  <rdf:Description rdf:about="https://w3id.org/italia/onto/HER/USTATStudentsBySexAggregate">
    <rdf:type rdf:resource="http://www.w3.org/2002/07/owl#Class"/>
    <rdfs:subClassOf rdf:resource="https://w3id.org/italia/onto/HER/StatisticalDataAggregation"/>
    <rdfs:subClassOf rdf:nodeID="n5bb3bff42afb4ca286d2c3fead9507ddb541"/>
    <rdfs:comment xml:lang="en">Data on the student population from a gender perspective. The data concern students, graduates, PhDs and PhDs. The data are available from the academic year 2012/2013. Where possible, the descriptions have been derived from the Record Sheet for the Student time Series provided by USTAT - Open data.</rdfs:comment>
    <rdfs:comment xml:lang="it">Dati sulla popolazione studentesca in un'ottica di genere. I dati riguardano student-i/-esse, laureat-i/-e, dottorand-i/-e e dottori di ricerca. I dati sono disponibili a partire dall'anno accademico 2012/2013. Quando possibile, le descrizioni sono state derivate dal Tracciato record per la serie storica sugli studenti fornito dal USTAT - Open data.</rdfs:comment>
    <rdfs:isDefinedBy rdf:resource="https://w3id.org/italia/onto/HER"/>
    <rdfs:label xml:lang="it">Aggregazione degli studenti per genere riportati da USTAT</rdfs:label>
    <rdfs:label xml:lang="en">USTAT Aggregate of Students By Sex</rdfs:label>
    <owl:versionInfo xml:lang="it">stabile</owl:versionInfo>
    <owl:versionInfo xml:lang="en">stable</owl:versionInfo>
  </rdf:Description>
  <rdf:Description rdf:about="https://w3id.org/italia/onto/HER/hasAACTResponsible">
    <rdf:type rdf:resource="http://www.w3.org/2002/07/owl#ObjectProperty"/>
    <rdfs:domain rdf:resource="https://w3id.org/italia/onto/HER/AACTStudy"/>
    <rdfs:range rdf:resource="https://w3id.org/italia/onto/CPV/Person"/>
    <rdfs:comment xml:lang="it">La persona responsabile dell'invio di informazioni su uno studio clinico a ClinicalTrials.gov e dell'aggiornamento di tali informazioni. Di solito lo sponsor dello studio o lo sperimentatore.</rdfs:comment>
    <rdfs:comment xml:lang="en">The person responsible for submitting information about a clinical study to ClinicalTrials.gov and updating that information. Usually the study sponsor or investigator.</rdfs:comment>
    <rdfs:isDefinedBy rdf:resource="https://w3id.org/italia/onto/HER"/>
    <rdfs:label xml:lang="it">ha responsabile AACT</rdfs:label>
    <rdfs:label xml:lang="en">has AACT responsible</rdfs:label>
    <owl:versionInfo xml:lang="it">stabile</owl:versionInfo>
    <owl:versionInfo xml:lang="en">stable</owl:versionInfo>
  </rdf:Description>
  <rdf:Description rdf:nodeID="n5bb3bff42afb4ca286d2c3fead9507ddb20">
    <rdf:first rdf:resource="https://w3id.org/italia/onto/HER/MIURStudentsAggregate"/>
    <rdf:rest rdf:nodeID="n5bb3bff42afb4ca286d2c3fead9507ddb21"/>
  </rdf:Description>
  <rdf:Description rdf:nodeID="n5bb3bff42afb4ca286d2c3fead9507ddb214">
    <rdf:first rdf:resource="https://w3id.org/italia/onto/HER/MIURStudentsByProvinceOfResidenceAggregate"/>
    <rdf:rest rdf:nodeID="n5bb3bff42afb4ca286d2c3fead9507ddb215"/>
  </rdf:Description>
  <rdf:Description rdf:about="https://w3id.org/italia/onto/HER/hasPatentInventor">
    <rdf:type rdf:resource="http://www.w3.org/2002/07/owl#ObjectProperty"/>
    <rdfs:domain rdf:resource="https://w3id.org/italia/onto/HER/Patent"/>
    <rdfs:range rdf:resource="https://w3id.org/italia/onto/CPV/Person"/>
    <rdfs:comment xml:lang="it">Questa proprietà collega un brevetto con le persone che lo hanno inventato.</rdfs:comment>
    <rdfs:comment xml:lang="en">This property connects a patent with the persons that invented it.</rdfs:comment>
    <rdfs:isDefinedBy rdf:resource="https://w3id.org/italia/onto/HER"/>
    <rdfs:label xml:lang="it">ha inventore</rdfs:label>
    <rdfs:label xml:lang="en">has inventor</rdfs:label>
    <owl:versionInfo xml:lang="it">stabile</owl:versionInfo>
    <owl:versionInfo xml:lang="en">stable</owl:versionInfo>
  </rdf:Description>
  <rdf:Description rdf:nodeID="n5bb3bff42afb4ca286d2c3fead9507ddb354">
    <rdf:first rdf:resource="https://w3id.org/italia/onto/HER/USTATPartiallyExoneratedStudentsAggregate"/>
    <rdf:rest rdf:nodeID="n5bb3bff42afb4ca286d2c3fead9507ddb355"/>
  </rdf:Description>
  <rdf:Description rdf:about="https://w3id.org/italia/onto/HER/status">
    <rdf:type rdf:resource="http://www.w3.org/2002/07/owl#DatatypeProperty"/>
    <rdfs:domain rdf:nodeID="n5bb3bff42afb4ca286d2c3fead9507ddb280"/>
    <rdfs:range rdf:resource="http://www.w3.org/2000/01/rdf-schema#Literal"/>
    <rdfs:comment xml:lang="it">Descrizione testuale dello stato di una struttura o progetto.</rdfs:comment>
    <rdfs:comment xml:lang="en">Textual description of the status of a facility or project.</rdfs:comment>
    <rdfs:isDefinedBy rdf:resource="https://w3id.org/italia/onto/HER"/>
    <rdfs:label xml:lang="it">stato</rdfs:label>
    <rdfs:label xml:lang="en">status</rdfs:label>
  </rdf:Description>
  <rdf:Description rdf:nodeID="n5bb3bff42afb4ca286d2c3fead9507ddb390">
    <rdf:type rdf:resource="http://www.w3.org/2002/07/owl#Restriction"/>
    <owl:onProperty rdf:resource="https://w3id.org/italia/onto/HER/ipdURL"/>
    <owl:maxQualifiedCardinality rdf:datatype="http://www.w3.org/2001/XMLSchema#nonNegativeInteger">1</owl:maxQualifiedCardinality>
    <owl:onDataRange rdf:resource="http://www.w3.org/2001/XMLSchema#anyURI"/>
  </rdf:Description>
  <rdf:Description rdf:about="https://w3id.org/italia/onto/HER/totalSpecialization">
    <rdf:type rdf:resource="http://www.w3.org/2002/07/owl#DatatypeProperty"/>
    <rdfs:subPropertyOf rdf:resource="https://w3id.org/italia/onto/MU/value"/>
    <rdfs:domain rdf:nodeID="n5bb3bff42afb4ca286d2c3fead9507ddb356"/>
    <rdfs:range rdf:resource="http://www.w3.org/2001/XMLSchema#int"/>
    <rdfs:comment xml:lang="en">Total with respect to students in good standing with the payment of tuition fees enrolled in specialized courses.</rdfs:comment>
    <rdfs:comment xml:lang="it">Totale rispetto agli studenti in regola con il pagamento delle tasse universitarie iscritti a corsi di specializzazione.</rdfs:comment>
    <rdfs:isDefinedBy rdf:resource="https://w3id.org/italia/onto/HER"/>
    <rdfs:label xml:lang="en">total specialization</rdfs:label>
    <rdfs:label xml:lang="it">totale specializzazioni</rdfs:label>
    <owl:versionInfo xml:lang="it">stabile</owl:versionInfo>
    <owl:versionInfo xml:lang="en">stable</owl:versionInfo>
  </rdf:Description>
  <rdf:Description rdf:nodeID="n5bb3bff42afb4ca286d2c3fead9507ddb298">
    <rdf:first rdf:resource="https://w3id.org/italia/onto/HER/DSUCanteenAndAccomodationsAggregate"/>
    <rdf:rest rdf:nodeID="n5bb3bff42afb4ca286d2c3fead9507ddb299"/>
  </rdf:Description>
  <rdf:Description rdf:about="https://w3id.org/italia/onto/HER/CPCClassification">
    <rdf:type rdf:resource="http://www.w3.org/2002/07/owl#Class"/>
    <rdfs:subClassOf rdf:resource="https://w3id.org/italia/onto/HER/HERClassification"/>
    <rdfs:subClassOf rdf:nodeID="n5bb3bff42afb4ca286d2c3fead9507ddb412"/>
    <rdfs:subClassOf rdf:nodeID="n5bb3bff42afb4ca286d2c3fead9507ddb413"/>
    <rdfs:isDefinedBy rdf:resource="https://w3id.org/italia/onto/HER"/>
    <rdfs:label xml:lang="it">Classificazione dei brevetti cooperativi</rdfs:label>
    <rdfs:label xml:lang="en">Cooperative Patent Classification</rdfs:label>
    <owl:versionInfo xml:lang="it">stabile</owl:versionInfo>
    <owl:versionInfo xml:lang="en">stable</owl:versionInfo>
    <ns6:wasDerivedFrom rdf:resource="http://www.w3.org/2004/02/skos/core#ConceptScheme"/>
  </rdf:Description>
  <rdf:Description rdf:about="https://w3id.org/italia/onto/HER/withCountry">
    <rdf:type rdf:resource="http://www.w3.org/2002/07/owl#ObjectProperty"/>
    <rdfs:domain rdf:resource="https://w3id.org/italia/onto/HER/CountryInvolvement"/>
    <rdfs:range rdf:resource="https://w3id.org/italia/onto/CLV/Country"/>
    <rdfs:comment xml:lang="it">Questa proprietà collega un coinvolgimento del paese con il paese corrispondente</rdfs:comment>
    <rdfs:comment xml:lang="en">This property connects a country involvement with the corresponding country</rdfs:comment>
    <rdfs:isDefinedBy rdf:resource="https://w3id.org/italia/onto/HER"/>
    <rdfs:label xml:lang="it">con paese</rdfs:label>
    <rdfs:label xml:lang="en">with country</rdfs:label>
    <owl:versionInfo xml:lang="it">stabile</owl:versionInfo>
    <owl:versionInfo xml:lang="en">stable</owl:versionInfo>
  </rdf:Description>
  <rdf:Description rdf:nodeID="n5bb3bff42afb4ca286d2c3fead9507ddb507">
    <rdf:type rdf:resource="http://www.w3.org/2002/07/owl#Restriction"/>
    <owl:onProperty rdf:resource="https://w3id.org/italia/onto/HER/publicationDate"/>
    <owl:qualifiedCardinality rdf:datatype="http://www.w3.org/2001/XMLSchema#nonNegativeInteger">1</owl:qualifiedCardinality>
    <owl:onDataRange rdf:resource="http://www.w3.org/2001/XMLSchema#date"/>
  </rdf:Description>
  <rdf:Description rdf:about="https://w3id.org/italia/onto/HER/hasUSTATContributionRevenueClass">
    <rdf:type rdf:resource="http://www.w3.org/2002/07/owl#ObjectProperty"/>
    <rdfs:domain rdf:resource="https://w3id.org/italia/onto/HER/USTATContributionRevenue"/>
    <rdfs:range rdf:resource="https://w3id.org/italia/onto/HER/USTATContributionRevenueClass"/>
    <rdfs:comment xml:lang="it">Questa proprietà collega l'informazione sui dati relativi al gettito dalla contribuzione studentesca degli atenei alle informazioni sulla fonte del gettito.</rdfs:comment>
    <rdfs:comment xml:lang="en">This property links information on revenue data from student contributions to information on the source of the revenue.</rdfs:comment>
    <rdfs:isDefinedBy rdf:resource="https://w3id.org/italia/onto/HER"/>
    <rdfs:label xml:lang="it">ha un classe di contributo ricavante</rdfs:label>
    <rdfs:label xml:lang="en">has contribution revenue class</rdfs:label>
    <owl:versionInfo xml:lang="it">stabile</owl:versionInfo>
    <owl:versionInfo xml:lang="en">stable</owl:versionInfo>
  </rdf:Description>
  <rdf:Description rdf:about="https://w3id.org/italia/onto/HER/CTNPRINFinancingFund">
    <rdf:type rdf:resource="http://www.w3.org/2002/07/owl#Class"/>
    <rdfs:subClassOf rdf:resource="https://w3id.org/italia/onto/l0/Object"/>
    <rdfs:subClassOf rdf:nodeID="n5bb3bff42afb4ca286d2c3fead9507ddb416"/>
    <rdfs:comment xml:lang="en">Financing fund from which the initiative draws its economic resources</rdfs:comment>
    <rdfs:comment xml:lang="it">Fondo di finanziamento da cui l'iniziativa attinge le sue risorse economiche</rdfs:comment>
    <rdfs:isDefinedBy rdf:resource="https://w3id.org/italia/onto/HER"/>
    <rdfs:label xml:lang="en">CTN/PRIN Financing Fund</rdfs:label>
    <rdfs:label xml:lang="it">Fondo di finanziamento CTN/PRIN</rdfs:label>
    <owl:versionInfo xml:lang="it">stabile</owl:versionInfo>
    <owl:versionInfo xml:lang="en">stable</owl:versionInfo>
  </rdf:Description>
  <rdf:Description rdf:about="https://w3id.org/italia/onto/HER/USTATUniversityInterventionType">
    <rdf:type rdf:resource="http://www.w3.org/2002/07/owl#Class"/>
    <rdfs:subClassOf rdf:resource="https://w3id.org/italia/onto/l0/Characteristic"/>
    <rdfs:subClassOf rdf:nodeID="n5bb3bff42afb4ca286d2c3fead9507ddb546"/>
    <rdfs:subClassOf rdf:nodeID="n5bb3bff42afb4ca286d2c3fead9507ddb547"/>
    <rdfs:comment xml:lang="it">Tipologia di intervento effettuato dall'ateneo. La tipologia è definita dai codici/descrizioni di seguito:
030 : Borse di studio - N. borse di studio concesse con fondi dell'ATENEO (escluse le borse post-laurea riportate nell'apposita sezione)
061 : Mobilità internazionale - N. iscritti nell'ateneo coinvolti in programmi di mobilità internazionale (studenti in uscita)
061c : Mobilità internazionale - N. iscritti nell'ateneo coinvolti in programmi di mobilità internazionale (studenti in uscita) - di cui studenti SENZA borsa
061m : Mobilità internazionale - N. iscritti nell'ateneo coinvolti in programmi di mobilità internazionale (studenti in uscita) - di cui studenti in mobilità extraeuropea
061p : Mobilità internazionale - N. iscritti nell'ateneo coinvolti in programmi di mobilità internazionale (studenti in uscita) - di cui dottorandi percettori di borsa che usufruiscono della maggiorazione del 50%
063 : Mobilità internazionale - N. iscritti in atenei esteri coinvolti in programmi di mobilità internazionale presso l'ateneo italiano (studenti in entrata)
063c : Mobilità internazionale - N. iscritti in atenei esteri coinvolti in programmi di mobilità internazionale presso l'ateneo italiano (studenti in entrata) - di cui studenti con borsa dell'Ateneo italiano
064 : Mobilità internazionale - N. iscritti in atenei esteri coinvolti in programmi di mobilità internazionale presso l'ateneo italiano (studenti in entrata) - di cui studenti provenienti da Paesi extraeuropei
073 : Interventi a favore di studenti in situazione di disabilità - N. contributi finanziari
074 : Interventi a favore di studenti in situazione di disabilità - N. interventi non finanziari
081 : Attività di collaborazione a tempo parziale - N. collaborazioni
091 : Posti alloggio e contributi-alloggio - N. domande posti alloggio
092 : Posti alloggio e contributi-alloggio - N. posti alloggio assegnati
092c : Posti alloggio e contributi-alloggio - N. posti alloggio assegnati - di cui assegnati in strutture convenzionate o private
093 : Posti alloggio e contributi-alloggio - N. domande contributi-alloggio
094 : Posti alloggio e contributi-alloggio - N. contributi-alloggio assegnati
101 : Altri interventi di tipo finanziario - N. prestiti agevolati concessi da istituti di credito convenzionati
101a : Altri interventi di tipo finanziario - N. prestiti agevolati concessi da istituti di credito convenzionati - di cui con contributo in conto interesse e/o in conto capitale a carico dell'Ateneo
104 : Altri interventi di tipo finanziario - N. altri sussidi erogati
111a : Borse di studio post-lauream - N. borse finanziate con fondi MIUR
111b : Borse di studio post-lauream - N. borse finanziate da altri Ministeri
112 : Borse di studio post-lauream - N. borse finanziate dall'Ateneo con fondi propri
113 : Borse di studio post-lauream - N. borse finanziate mediante convenzione con altri Atenei
114 : Borse di studio post-lauream - N. borse finanziate con fondi UE
115 : Borse di studio post-lauream - N. borse finanziate mediante convenzione con altri enti pubblici
116 : Borse di studio post-lauream - N. borse finanziate mediante convenzione con enti privati</rdfs:comment>
    <rdfs:comment xml:lang="en">Type of intervention carried out by the university. The typology is defined by the codes/descriptions below:
030 : Scholarships - No. of scholarships awarded with funds from the University (excluding post-graduate scholarships listed in the appropriate section)
061 : International mobility - No. of students enrolled at the university involved in international mobility programmes (outgoing students)
061c : International mobility - No. enrolled at the university involved in international mobility programmes (outgoing students) - of which students WITHOUT a grant
061m : International mobility - No. of students enrolled at the university involved in international mobility programmes (outgoing students) - of which students on mobility outside Europe
061p : International mobility - No. of students enrolled at the university involved in international mobility programmes (outgoing students) - of which PhD students who are grant recipients benefiting from the 50% surcharge
063 : International mobility - No. enrolled in foreign universities involved in international mobility programs at the Italian university (incoming students)
063c : International mobility - No. enrolled in foreign universities involved in international mobility programs at the Italian athenaeum (incoming students) - of which students with a scholarship from the Italian university
064 : International mobility - No. enrolled in foreign universities involved in international mobility programs at the Italian university (incoming students) - of which students from non-European countries
073 : Interventions in favour of students with disabilities - No. of financial contributions
074 : Interventions in favour of students with disabilities - No. of non-financial interventions
081 : Part-time collaboration activities - No. of collaborations
091 : Accommodation places and accommodation contributions - No. of applications for accommodation places
092 : Accommodation and accommodation contributions - No. of accommodation places allocated
092c : Accommodation places and accommodation contributions - No. of accommodation places allocated - of which allocated in contracted or private facilities
093 : Accommodation places and accommodation contributions - No. of accommodation contributions applications
094 : Accommodation and accommodation contributions - No. of accommodation contributions allocated
101 : Other financial measures - No. of subsidised loans granted by credit institutions under agreement
101a : Other financial measures - No. of subsidized loans granted by credit institutions - of which with an interest rate and/or capital contribution borne by the University
104 : Other financial interventions - No. of other subsidies granted
111a : Post-graduate scholarships - No. of scholarships financed by MIUR funds
111b : Post-graduate scholarships - No. of scholarships funded by other Ministries
112 : Post-graduate scholarships - No. of scholarships financed by the University from its own funds
113 : Post-graduate scholarships - No. of scholarships financed by agreement with other universities
114 : Post-graduate scholarships - No. of EU-funded scholarships
115 : Post-graduate scholarships - No. of grants financed by agreement with other public bodies
116 : Post-graduate scholarships - No. of scholarships financed by agreement with private bodies</rdfs:comment>
    <rdfs:isDefinedBy rdf:resource="https://w3id.org/italia/onto/HER"/>
    <rdfs:label xml:lang="it">Tipo (o classe) di interventi universitari riportati da USTAT</rdfs:label>
    <rdfs:label xml:lang="en">USTAT Reported University Intervention Class</rdfs:label>
    <owl:versionInfo xml:lang="it">stabile</owl:versionInfo>
    <owl:versionInfo xml:lang="en">stable</owl:versionInfo>
  </rdf:Description>
  <rdf:Description rdf:about="https://w3id.org/italia/onto/HER/USTATPermanentStaff">
    <rdf:type rdf:resource="http://www.w3.org/2002/07/owl#Class"/>
    <rdfs:subClassOf rdf:resource="https://w3id.org/italia/onto/COV/Group"/>
    <rdfs:subClassOf rdf:nodeID="n5bb3bff42afb4ca286d2c3fead9507ddb532"/>
    <rdfs:comment xml:lang="it">Personale in servizio a tempo indeterminato negli Enti e negli Uffici per il Diritto allo Studio Universitario - DSU al 31/12 dell'anno di riferimento, aggregato per Regione.</rdfs:comment>
    <rdfs:comment xml:lang="en">Personnel in permanent service in the Entities and Offices for the Right to University Studies - DSU at 31/12 of the year of reference, aggregated by Region.</rdfs:comment>
    <rdfs:isDefinedBy rdf:resource="https://w3id.org/italia/onto/HER"/>
    <rdfs:label xml:lang="en">Permanent Staff</rdfs:label>
    <rdfs:label xml:lang="it">Personale Indeterminato</rdfs:label>
    <owl:versionInfo xml:lang="it">stabile</owl:versionInfo>
    <owl:versionInfo xml:lang="en">stable</owl:versionInfo>
  </rdf:Description>
  <rdf:Description rdf:about="https://w3id.org/italia/onto/HER/enrollmentType">
    <rdf:type rdf:resource="http://www.w3.org/2002/07/owl#DatatypeProperty"/>
    <rdfs:domain rdf:resource="https://w3id.org/italia/onto/HER/AACTStudy"/>
    <rdfs:range rdf:resource="http://www.w3.org/2000/01/rdf-schema#Literal"/>
    <rdfs:comment xml:lang="it">Il numero totale di partecipanti da iscrivere. Essi sono: la stima (numero target) o il numero totale effettivo di partecipanti che vengono arruolati nello studio clinico.</rdfs:comment>
    <rdfs:comment xml:lang="en">The total number of participants to be enrolled. They are either: estimated (target number) or the actual total number of participants that are enrolled in the clinical study.</rdfs:comment>
    <rdfs:isDefinedBy rdf:resource="https://w3id.org/italia/onto/HER"/>
    <rdfs:label xml:lang="en">enrollment type</rdfs:label>
    <rdfs:label xml:lang="it">tipo di iscrizione</rdfs:label>
    <owl:versionInfo xml:lang="it">provvisoria - definizione necessita di revisione</owl:versionInfo>
    <owl:versionInfo xml:lang="en">unstable - definition need to be re-checked</owl:versionInfo>
  </rdf:Description>
  <rdf:Description rdf:about="https://w3id.org/italia/onto/HER/hasSubjectArea">
    <rdf:type rdf:resource="http://www.w3.org/2002/07/owl#ObjectProperty"/>
    <rdfs:subPropertyOf rdf:resource="https://w3id.org/italia/onto/l0/hasTopic"/>
    <rdfs:domain rdf:nodeID="n5bb3bff42afb4ca286d2c3fead9507ddb90"/>
    <rdfs:range rdf:resource="https://w3id.org/italia/onto/HER/ECSubjectArea"/>
    <rdfs:comment xml:lang="it">Questa proprietà collega un progetto CE con la corrispondente categorizzazione tematica. Questa categorizzazione è disponibile per il programma quadro FP7, ma non per H2020.</rdfs:comment>
    <rdfs:comment xml:lang="en">This property connects an EC project with the corresponding thematic categorisation. This categorisation is available for the FP7 framework programme, but not for H2020.</rdfs:comment>
    <rdfs:isDefinedBy rdf:resource="https://w3id.org/italia/onto/HER"/>
    <rdfs:label xml:lang="it">ha un'area tematica CE</rdfs:label>
    <rdfs:label xml:lang="en">has EC subject area</rdfs:label>
    <owl:versionInfo xml:lang="it">stabile</owl:versionInfo>
    <owl:versionInfo xml:lang="en">stable</owl:versionInfo>
  </rdf:Description>
  <rdf:Description rdf:about="https://w3id.org/italia/onto/HER/CHAFEATopic">
    <rdf:type rdf:resource="http://www.w3.org/2002/07/owl#Class"/>
    <rdfs:subClassOf rdf:resource="https://w3id.org/italia/onto/HER/HERClassification"/>
    <rdfs:comment xml:lang="en">Classification of funded activities published by the Consumers, Health, Agriculture and Food Executive Agency (CHAFEA)</rdfs:comment>
    <rdfs:comment xml:lang="it">Classificazione delle attività finanziate pubblicata dall'Agenzia esecutiva per i consumatori, la salute, l'agricoltura e l'alimentazione (CHAFEA)</rdfs:comment>
    <rdfs:isDefinedBy rdf:resource="https://w3id.org/italia/onto/HER"/>
    <rdfs:label xml:lang="it">Argomento CHAFEA</rdfs:label>
    <rdfs:label xml:lang="en">CHAFEA Topic</rdfs:label>
    <owl:versionInfo xml:lang="it">stabile</owl:versionInfo>
    <owl:versionInfo xml:lang="en">stable</owl:versionInfo>
    <ns6:wasDerivedFrom rdf:resource="http://www.w3.org/2004/02/skos/core#Concept"/>
  </rdf:Description>
  <rdf:Description rdf:nodeID="n5bb3bff42afb4ca286d2c3fead9507ddb179">
    <rdf:type rdf:resource="http://www.w3.org/1999/02/22-rdf-syntax-ns#List"/>
    <rdf:first>Active not recruiting</rdf:first>
    <rdf:rest rdf:nodeID="n5bb3bff42afb4ca286d2c3fead9507ddb180"/>
  </rdf:Description>
  <rdf:Description rdf:about="https://w3id.org/italia/onto/HER/hasAcademicOrg">
    <rdf:type rdf:resource="http://www.w3.org/2002/07/owl#ObjectProperty"/>
    <rdfs:subPropertyOf rdf:resource="https://w3id.org/italia/onto/COV/hasPublicOrganization"/>
    <rdfs:domain rdf:nodeID="n5bb3bff42afb4ca286d2c3fead9507ddb18"/>
    <rdfs:range rdf:resource="https://w3id.org/italia/onto/COV/PublicOrganization"/>
    <rdfs:comment xml:lang="it">Questa proprietà si collega diversi dati statistici a un'organizzazione accademica.</rdfs:comment>
    <rdfs:comment xml:lang="en">This property links different statistical data to an academic Organization.</rdfs:comment>
    <rdfs:isDefinedBy rdf:resource="https://w3id.org/italia/onto/HER"/>
    <rdfs:label xml:lang="it">ha organizzazione accademica</rdfs:label>
    <rdfs:label xml:lang="en">has academic organization</rdfs:label>
    <owl:versionInfo xml:lang="it">provvisoria</owl:versionInfo>
    <owl:versionInfo xml:lang="en">unstable</owl:versionInfo>
  </rdf:Description>
  <rdf:Description rdf:nodeID="n5bb3bff42afb4ca286d2c3fead9507ddb218">
    <rdf:type rdf:resource="http://www.w3.org/2002/07/owl#Class"/>
    <owl:unionOf rdf:nodeID="n5bb3bff42afb4ca286d2c3fead9507ddb219"/>
  </rdf:Description>
  <rdf:Description rdf:about="https://w3id.org/italia/onto/HER/Patent">
    <rdf:type rdf:resource="http://www.w3.org/2002/07/owl#Class"/>
    <rdfs:subClassOf rdf:resource="https://w3id.org/italia/onto/HER/Result"/>
    <rdfs:subClassOf rdf:nodeID="n5bb3bff42afb4ca286d2c3fead9507ddb498"/>
    <rdfs:subClassOf rdf:nodeID="n5bb3bff42afb4ca286d2c3fead9507ddb499"/>
    <rdfs:subClassOf rdf:nodeID="n5bb3bff42afb4ca286d2c3fead9507ddb500"/>
    <rdfs:subClassOf rdf:nodeID="n5bb3bff42afb4ca286d2c3fead9507ddb501"/>
    <rdfs:subClassOf rdf:nodeID="n5bb3bff42afb4ca286d2c3fead9507ddb502"/>
    <rdfs:comment xml:lang="en">A granted patent, i.e. an intellectual property right for the owner to exclude others from making, using, selling and importing an invention</rdfs:comment>
    <rdfs:comment xml:lang="it">Un brevetto concesso, ovvero un diritto di proprietà intellettuale per il proprietario di escludere altri dal fare, utilizzare, vendere e importare un'invenzione</rdfs:comment>
    <rdfs:isDefinedBy rdf:resource="https://w3id.org/italia/onto/HER"/>
    <rdfs:label xml:lang="it">Brevetto</rdfs:label>
    <rdfs:label xml:lang="en">Patent</rdfs:label>
    <owl:versionInfo xml:lang="it">stabile</owl:versionInfo>
    <owl:versionInfo xml:lang="en">stable</owl:versionInfo>
  </rdf:Description>
  <rdf:Description rdf:nodeID="n5bb3bff42afb4ca286d2c3fead9507ddb455">
    <rdf:type rdf:resource="http://www.w3.org/2002/07/owl#Restriction"/>
    <owl:onProperty rdf:resource="https://w3id.org/italia/onto/HER/endingYear"/>
    <owl:maxQualifiedCardinality rdf:datatype="http://www.w3.org/2001/XMLSchema#nonNegativeInteger">1</owl:maxQualifiedCardinality>
    <owl:onDataRange rdf:resource="http://www.w3.org/2001/XMLSchema#gYear"/>
  </rdf:Description>
  <rdf:Description rdf:nodeID="n5bb3bff42afb4ca286d2c3fead9507ddb401">
    <rdf:type rdf:resource="http://www.w3.org/2002/07/owl#Restriction"/>
    <owl:onProperty rdf:resource="https://w3id.org/italia/onto/l0/description"/>
    <owl:someValuesFrom rdf:resource="http://www.w3.org/2000/01/rdf-schema#Literal"/>
  </rdf:Description>
  <rdf:Description rdf:about="https://w3id.org/italia/onto/HER/totalDegree">
    <rdf:type rdf:resource="http://www.w3.org/2002/07/owl#DatatypeProperty"/>
    <rdfs:subPropertyOf rdf:resource="https://w3id.org/italia/onto/MU/value"/>
    <rdfs:domain rdf:nodeID="n5bb3bff42afb4ca286d2c3fead9507ddb303"/>
    <rdfs:range rdf:resource="http://www.w3.org/2000/01/rdf-schema#Literal"/>
    <rdfs:comment xml:lang="en">Total with respect to undergraduate students: in this case, undergraduate students are considered to be students in good standing with the payment of tuition fees enrolled in undergraduate courses, master's degree courses, courses of the old system.</rdfs:comment>
    <rdfs:comment xml:lang="it">Totale rispetto agli studenti di laurea: in questo caso, vengono considerati studenti di laurea gli studenti in regola con il pagamento delle tasse universitarie iscritti a corsi di laurea, corsi di laurea magistrale, corsi del vecchio ordinamento.</rdfs:comment>
    <rdfs:isDefinedBy rdf:resource="https://w3id.org/italia/onto/HER"/>
    <rdfs:label xml:lang="en">total degree</rdfs:label>
    <rdfs:label xml:lang="it">totale lauree</rdfs:label>
    <owl:versionInfo xml:lang="it">stabile</owl:versionInfo>
    <owl:versionInfo xml:lang="en">stable</owl:versionInfo>
  </rdf:Description>
  <rdf:Description rdf:about="https://w3id.org/italia/onto/HER/lastUpdateSubmittedQCDate">
    <rdf:type rdf:resource="http://www.w3.org/2002/07/owl#DatatypeProperty"/>
    <rdfs:subPropertyOf rdf:resource="https://w3id.org/italia/onto/TI/modified"/>
    <rdfs:domain rdf:resource="https://w3id.org/italia/onto/HER/AACTStudy"/>
    <rdfs:range rdf:resource="http://www.w3.org/2001/XMLSchema#date"/>
    <rdfs:comment xml:lang="it">La data più recente in cui lo sponsor dello studio o lo sperimentatore ha presentato modifiche al registro dello studio che sono coerenti con i criteri di revisione del controllo di qualità (QC) della National Library of Medicine (NLM). È responsabilità dello sponsor o dello sperimentatore assicurarsi che la documentazione dello studio sia coerente con i criteri di revisione del controllo di qualità della NLM.</rdfs:comment>
    <rdfs:comment xml:lang="en">The most recent date on which the study sponsor or investigator submitted changes to a study record that are consistent with National Library of Medicine (NLM) quality control (QC) review criteria. It is the responsibility of the sponsor or investigator to ensure that the study record is consistent with the NLM QC review criteria.</rdfs:comment>
    <rdfs:isDefinedBy rdf:resource="https://w3id.org/italia/onto/HER"/>
    <rdfs:label xml:lang="it">data dell'ultimo aggiornamento presentato QC</rdfs:label>
    <rdfs:label xml:lang="en">last update submitted QC date</rdfs:label>
    <owl:versionInfo xml:lang="it">stabile</owl:versionInfo>
    <owl:versionInfo xml:lang="en">stable</owl:versionInfo>
  </rdf:Description>
  <rdf:Description rdf:about="https://w3id.org/italia/onto/HER/USTATEnrollment">
    <rdf:type rdf:resource="http://www.w3.org/2002/07/owl#Class"/>
    <rdfs:subClassOf rdf:resource="https://w3id.org/italia/onto/HER/StatisticalDataAggregation"/>
    <rdfs:comment xml:lang="en">Information on the types of enrollment of the enrolled students of the universities in good standing with the payment of tuition fees. In particular, the identification/extended name shows the code/description of the type of enrollment, respectively and may consist of values:
T1: Total enrolled students
T1a: Total enrolled students - of which PhD students with financial support
T1b: Total enrolled students - of which students with partial coverage of fees from external bodies
T1c: Total number of enrolled students - of which students enrolled part-time</rdfs:comment>
    <rdfs:comment xml:lang="it">Informazioni sulle tipologie di iscrizione degli iscritti degli atenei in regola con il pagamento delle tasse universitarie. In particolare, l'identificativo/nome esteso riportano il codice/la descrizione della tipologia di iscrizione , rispettivamente, e possono essumere i valori:
T1: Totale iscritti
T1a: Totale iscritti - di cui dottorandi con supporto finanziario
T1b: Totale iscritti - di cui studenti con parziale copertura delle tasse da enti esterni
T1c: Totale iscritti - di cui studenti iscritti a tempo parziale</rdfs:comment>
    <rdfs:isDefinedBy rdf:resource="https://w3id.org/italia/onto/HER"/>
    <rdfs:label xml:lang="it">Iscrizioni riportate da USTAT</rdfs:label>
    <rdfs:label xml:lang="en">USTAT Reported Enrollment</rdfs:label>
    <owl:versionInfo xml:lang="it">stabile</owl:versionInfo>
    <owl:versionInfo xml:lang="en">stable</owl:versionInfo>
  </rdf:Description>
  <rdf:Description rdf:about="https://w3id.org/italia/onto/HER/USTATEnrolledStudentsAggregate">
    <rdf:type rdf:resource="http://www.w3.org/2002/07/owl#Class"/>
    <rdfs:subClassOf rdf:resource="https://w3id.org/italia/onto/HER/StatisticalDataAggregation"/>
    <rdfs:subClassOf rdf:nodeID="n5bb3bff42afb4ca286d2c3fead9507ddb529"/>
    <rdfs:comment xml:lang="en">Data on university students' enrolled at universities in good standing with the payment of tuition fees.</rdfs:comment>
    <rdfs:comment xml:lang="it">Dati relativi agli iscritti degli atenei in regola con il pagamento delle tasse universitarie.</rdfs:comment>
    <rdfs:isDefinedBy rdf:resource="https://w3id.org/italia/onto/HER"/>
    <rdfs:label xml:lang="it">Aggregazione degli studenti iscritt riportati da USTAT</rdfs:label>
    <rdfs:label xml:lang="en">USTAT Aggregate of Enrolled Students</rdfs:label>
    <owl:versionInfo xml:lang="it">stabile</owl:versionInfo>
    <owl:versionInfo xml:lang="en">stable</owl:versionInfo>
  </rdf:Description>
  <rdf:Description rdf:nodeID="n5bb3bff42afb4ca286d2c3fead9507ddb252">
    <rdf:type rdf:resource="http://www.w3.org/1999/02/22-rdf-syntax-ns#List"/>
    <rdf:first>Undecided</rdf:first>
    <rdf:rest rdf:nodeID="n5bb3bff42afb4ca286d2c3fead9507ddb253"/>
  </rdf:Description>
  <rdf:Description rdf:about="https://w3id.org/italia/onto/HER/ItalianStudentType">
    <rdf:type rdf:resource="http://www.w3.org/2002/07/owl#Class"/>
    <rdfs:subClassOf rdf:resource="https://w3id.org/italia/onto/RO/Role"/>
    <rdfs:comment xml:lang="it">Tipo di studente nel sistema accademico italiano (Immatricolato, Iscritto, Laureato, Dottorato, ...)</rdfs:comment>
    <rdfs:comment xml:lang="en">Type of student in the Italian academic system.</rdfs:comment>
    <rdfs:isDefinedBy rdf:resource="https://w3id.org/italia/onto/HER"/>
    <rdfs:label xml:lang="en">Italian Student Type</rdfs:label>
    <rdfs:label xml:lang="it">Tipo di studente italiano</rdfs:label>
    <owl:versionInfo xml:lang="it">stabile</owl:versionInfo>
    <owl:versionInfo xml:lang="en">stable</owl:versionInfo>
  </rdf:Description>
  <rdf:Description rdf:about="https://w3id.org/italia/onto/HER/resultType">
    <rdf:type rdf:resource="http://www.w3.org/2002/07/owl#DatatypeProperty"/>
    <rdfs:domain rdf:resource="https://w3id.org/italia/onto/HER/Result"/>
    <rdfs:range rdf:resource="http://www.w3.org/2000/01/rdf-schema#Literal"/>
    <rdfs:comment xml:lang="it">Testo che indica il tipo di risultato/prodotto corrispondente. I valori possibili sono: "Dimostratore, pilota, prototipo", "Documento, rapporti...", "Siti web, compilazione di brevetti, video ecc.</rdfs:comment>
    <rdfs:comment xml:lang="en">Text denoting the corresponding type of result. Possible values are: "Demonstrator, pilot, prototype", "Document, reports...", "Websites, patent filling, videos etc" and "Other".</rdfs:comment>
    <rdfs:isDefinedBy rdf:resource="https://w3id.org/italia/onto/HER"/>
    <rdfs:label xml:lang="en">result type</rdfs:label>
    <rdfs:label xml:lang="it">tipo di risultato</rdfs:label>
    <owl:versionInfo xml:lang="it">provvisoria - verificare la presenza di valori controllati</owl:versionInfo>
    <owl:versionInfo xml:lang="en">unstable - check if fixed values are applicable</owl:versionInfo>
  </rdf:Description>
  <rdf:Description rdf:nodeID="n5bb3bff42afb4ca286d2c3fead9507ddb226">
    <rdf:first rdf:resource="https://w3id.org/italia/onto/HER/MIURStudentsByDiplomaDegreeDegreeClassAggregate"/>
    <rdf:rest rdf:nodeID="n5bb3bff42afb4ca286d2c3fead9507ddb227"/>
  </rdf:Description>
  <rdf:Description rdf:nodeID="n5bb3bff42afb4ca286d2c3fead9507ddb233">
    <rdf:type rdf:resource="http://www.w3.org/1999/02/22-rdf-syntax-ns#List"/>
    <rdf:first>Case Control, Natural History</rdf:first>
    <rdf:rest rdf:nodeID="n5bb3bff42afb4ca286d2c3fead9507ddb234"/>
  </rdf:Description>
  <rdf:Description rdf:about="https://w3id.org/italia/onto/HER/ctnprinAmountCommittedCredit">
    <rdf:type rdf:resource="http://www.w3.org/2002/07/owl#DatatypeProperty"/>
    <rdfs:subPropertyOf rdf:resource="https://w3id.org/italia/onto/MU/value"/>
    <rdfs:domain rdf:resource="https://w3id.org/italia/onto/HER/CTNPRINAmount"/>
    <rdfs:range rdf:resource="http://www.w3.org/2001/XMLSchema#decimal"/>
    <rdfs:comment xml:lang="en">Credit committed by the Ministry on the eligible costs per single expense item following ex-ante evaluation
(for companies only).</rdfs:comment>
    <rdfs:comment xml:lang="it">Credito impegnato dal Ministero sui costi ammessi per singola voce di spesa a seguito di valutazione ex-ante
(solo per imprese).</rdfs:comment>
    <rdfs:isDefinedBy rdf:resource="https://w3id.org/italia/onto/HER"/>
    <rdfs:label xml:lang="en">committed credit of CTN/PRIN amount</rdfs:label>
    <rdfs:label xml:lang="it">credito impegnato dell'importo CTN/PRIN</rdfs:label>
    <owl:versionInfo xml:lang="it">stabile</owl:versionInfo>
    <owl:versionInfo xml:lang="en">stable</owl:versionInfo>
  </rdf:Description>
  <rdf:Description rdf:nodeID="n5bb3bff42afb4ca286d2c3fead9507ddb316">
    <rdf:first rdf:resource="https://w3id.org/italia/onto/HER/USTATContributionByClass"/>
    <rdf:rest rdf:nodeID="n5bb3bff42afb4ca286d2c3fead9507ddb317"/>
  </rdf:Description>
  <rdf:Description rdf:nodeID="n5bb3bff42afb4ca286d2c3fead9507ddb134">
    <rdf:type rdf:resource="http://www.w3.org/1999/02/22-rdf-syntax-ns#List"/>
    <rdf:first>Random Sample</rdf:first>
    <rdf:rest rdf:nodeID="n5bb3bff42afb4ca286d2c3fead9507ddb135"/>
  </rdf:Description>
  <rdf:Description rdf:about="https://w3id.org/italia/onto/HER/totalPerfectioningMaster">
    <rdf:type rdf:resource="http://www.w3.org/2002/07/owl#DatatypeProperty"/>
    <rdfs:subPropertyOf rdf:resource="https://w3id.org/italia/onto/MU/value"/>
    <rdfs:domain rdf:nodeID="n5bb3bff42afb4ca286d2c3fead9507ddb351"/>
    <rdfs:range rdf:resource="http://www.w3.org/2000/01/rdf-schema#Literal"/>
    <rdfs:comment xml:lang="en">Total with respect to students enrolled in 1st and 2nd level master's courses and perfectioning courses. Disaggregation criterion used for data from 2009 to 2013, both included.</rdfs:comment>
    <rdfs:comment xml:lang="it">Totale rispetto agli studenti iscritti a corsi di master di I e II livello e a corsi di perfezionamento. Criterio di disaggregazione utilizzato per dati dal 2009 al 2013, entrambi inclusi.</rdfs:comment>
    <rdfs:isDefinedBy rdf:resource="https://w3id.org/italia/onto/HER"/>
    <rdfs:label xml:lang="en">total perfectioning master</rdfs:label>
    <rdfs:label xml:lang="it">totale corsi di perfezionamento</rdfs:label>
    <owl:versionInfo xml:lang="it">stabile</owl:versionInfo>
    <owl:versionInfo xml:lang="en">stable</owl:versionInfo>
  </rdf:Description>
  <rdf:Description rdf:about="https://w3id.org/italia/onto/l0/Concept">
    <rdf:type rdf:resource="http://www.w3.org/2002/07/owl#Class"/>
  </rdf:Description>
  <rdf:Description rdf:about="https://w3id.org/italia/onto/HER/requiredContribution">
    <rdf:type rdf:resource="http://www.w3.org/2002/07/owl#DatatypeProperty"/>
    <rdfs:domain rdf:resource="https://w3id.org/italia/onto/HER/CTNPRINInitiative"/>
    <rdfs:range rdf:resource="http://www.w3.org/2001/XMLSchema#decimal"/>
    <rdfs:comment xml:lang="en">Total contributions requested in the project proposals</rdfs:comment>
    <rdfs:comment xml:lang="it">Totale dei contributi totali richiesti nelle proposte di progetto</rdfs:comment>
    <rdfs:isDefinedBy rdf:resource="https://w3id.org/italia/onto/HER"/>
    <rdfs:label xml:lang="it">contributi richiesti</rdfs:label>
    <rdfs:label xml:lang="en">required contributions</rdfs:label>
    <owl:versionInfo xml:lang="it">provvisoria - verificare il range</owl:versionInfo>
    <owl:versionInfo xml:lang="en">unstable - check the range</owl:versionInfo>
  </rdf:Description>
  <rdf:Description rdf:about="https://w3id.org/italia/onto/HER/totalExpense">
    <rdf:type rdf:resource="http://www.w3.org/2002/07/owl#DatatypeProperty"/>
    <rdfs:subPropertyOf rdf:resource="https://w3id.org/italia/onto/MU/value"/>
    <rdfs:domain rdf:resource="https://w3id.org/italia/onto/HER/USTATUniversityInterventionExpensesAggregate"/>
    <rdfs:range rdf:resource="http://www.w3.org/2001/XMLSchema#decimal"/>
    <rdfs:comment xml:lang="en">Amount of total expenditure. The values are expressed in EURO. The data relate to the financial year per year (T-1).</rdfs:comment>
    <rdfs:comment xml:lang="it">Importo della spesa totale. I valori sono espressi in EURO. I dati sono relativi all'esercizio finanziario all'anno (T-1).</rdfs:comment>
    <rdfs:isDefinedBy rdf:resource="https://w3id.org/italia/onto/HER"/>
    <rdfs:label xml:lang="it">spese totali</rdfs:label>
    <rdfs:label xml:lang="en">total expense</rdfs:label>
    <owl:versionInfo xml:lang="it">stabile</owl:versionInfo>
    <owl:versionInfo xml:lang="en">stable</owl:versionInfo>
  </rdf:Description>
  <rdf:Description rdf:nodeID="n5bb3bff42afb4ca286d2c3fead9507ddb363">
    <rdf:first rdf:resource="https://w3id.org/italia/onto/HER/USTATTotallyExoneratedStudentsAggregate"/>
    <rdf:rest rdf:resource="http://www.w3.org/1999/02/22-rdf-syntax-ns#nil"/>
  </rdf:Description>
  <rdf:Description rdf:nodeID="n5bb3bff42afb4ca286d2c3fead9507ddb478">
    <rdf:type rdf:resource="http://www.w3.org/2002/07/owl#Restriction"/>
    <owl:onProperty rdf:resource="https://w3id.org/italia/onto/HER/hasParticipationCountry"/>
    <owl:allValuesFrom rdf:resource="https://w3id.org/italia/onto/CLV/Country"/>
  </rdf:Description>
  <rdf:Description rdf:nodeID="n5bb3bff42afb4ca286d2c3fead9507ddb7">
    <rdf:first rdf:resource="https://w3id.org/italia/onto/HER/AACTEligibility"/>
    <rdf:rest rdf:nodeID="n5bb3bff42afb4ca286d2c3fead9507ddb8"/>
  </rdf:Description>
  <rdf:Description rdf:about="https://w3id.org/italia/data/public-organization/agid">
    <rdf:type rdf:resource="http://www.w3.org/2002/07/owl#NamedIndividual"/>
    <rdf:type rdf:resource="http://dati.gov.it/onto/dcatapit#Agent"/>
    <rdf:type rdf:resource="http://xmlns.com/foaf/0.1/Agent"/>
    <ns2:identifier>agid</ns2:identifier>
    <ns5:name xml:lang="it">Agenzia per l'Italia Digitale</ns5:name>
    <ns5:name xml:lang="en">Italian Digital Agency</ns5:name>
  </rdf:Description>
  <rdf:Description rdf:about="https://w3id.org/italia/onto/HER/ECFundingScheme">
    <rdf:type rdf:resource="http://www.w3.org/2002/07/owl#Class"/>
    <rdfs:subClassOf rdf:resource="https://w3id.org/italia/onto/HER/ECClassification"/>
    <rdfs:subClassOf rdf:resource="https://w3id.org/italia/onto/l0/Concept"/>
    <rdfs:comment xml:lang="en">Funding scheme (or "Types of action" in Horizon 2020) are the types of projects funded under a EC Framework Programme. In Horizon 2020, the existing types of action are the following: Research and innovation actions (RIA), Innovation actions (IA), Coordination and support actions (CSA), ERA-NET Cofund actions, European Joint Programme (EJP) Cofund actions, Pre-Commercial Procurement (PCP) actions, Public Procurement of Innovative Solutions (PPI) actions and Prizes.</rdfs:comment>
    <rdfs:comment xml:lang="it">Gli schemi di finanziamento (o "Tipi di azione" in Horizon 2020) sono i tipi di progetti finanziati nell'ambito di un programma quadro CE. In Horizon 2020, i tipi di azione esistenti sono i seguenti: Azioni di ricerca e innovazione (RIA), azioni di innovazione (IA), azioni di coordinamento e sostegno (CSA), azioni Cofund ERA-NET, azioni Cofund del programma comune europeo (EJP), azioni Cofund del programma europeo congiunto (EJP), azioni di appalti pre-commerciali (PCP), azioni di appalti pubblici di soluzioni innovative (PPI) e premi.
</rdfs:comment>
    <rdfs:isDefinedBy rdf:resource="https://w3id.org/italia/onto/HER"/>
    <rdfs:label xml:lang="en">EC Funding Scheme</rdfs:label>
    <rdfs:label xml:lang="it">Piano di finanziamento CE</rdfs:label>
    <owl:versionInfo xml:lang="it">stabile</owl:versionInfo>
    <owl:versionInfo xml:lang="en">stable</owl:versionInfo>
    <ns6:wasDerivedFrom rdf:resource="http://www.w3.org/2004/02/skos/core#Concept"/>
  </rdf:Description>
  <rdf:Description rdf:about="https://w3id.org/italia/onto/HER/ASJC">
    <rdf:type rdf:resource="http://www.w3.org/2002/07/owl#Class"/>
    <rdfs:subClassOf rdf:resource="https://w3id.org/italia/onto/HER/HERClassification"/>
    <rdfs:isDefinedBy rdf:resource="https://w3id.org/italia/onto/HER"/>
    <rdfs:label xml:lang="en">All Science Journal Classification</rdfs:label>
    <rdfs:label xml:lang="it">Classificazione  Scopus</rdfs:label>
    <rdfs:label xml:lang="en">Scopus Classification</rdfs:label>
    <owl:versionInfo xml:lang="it">stabile</owl:versionInfo>
    <owl:versionInfo xml:lang="en">stable</owl:versionInfo>
    <ns6:wasDerivedFrom rdf:resource="http://www.w3.org/2004/02/skos/core#ConceptScheme"/>
    <ns4:controlledVocabulary rdf:resource="https://w3id.org/italia/controlled-vocabulary/classifications-for-universities/all-science-journal"/>
  </rdf:Description>
  <rdf:Description rdf:nodeID="n5bb3bff42afb4ca286d2c3fead9507ddb126">
    <rdf:first rdf:resource="https://w3id.org/italia/onto/HER/USTATEnrolledStudentsAggregate"/>
    <rdf:rest rdf:nodeID="n5bb3bff42afb4ca286d2c3fead9507ddb127"/>
  </rdf:Description>
  <rdf:Description rdf:nodeID="n5bb3bff42afb4ca286d2c3fead9507ddb481">
    <rdf:type rdf:resource="http://www.w3.org/2002/07/owl#Restriction"/>
    <owl:onProperty rdf:resource="https://w3id.org/italia/onto/HER/erasmusplusOrgType"/>
    <owl:maxCardinality rdf:datatype="http://www.w3.org/2001/XMLSchema#nonNegativeInteger">1</owl:maxCardinality>
  </rdf:Description>
  <rdf:Description rdf:nodeID="n5bb3bff42afb4ca286d2c3fead9507ddb50">
    <rdf:type rdf:resource="http://www.w3.org/2002/07/owl#Class"/>
    <owl:unionOf rdf:nodeID="n5bb3bff42afb4ca286d2c3fead9507ddb51"/>
  </rdf:Description>
  <rdf:Description rdf:about="https://w3id.org/italia/onto/HER/includesPPSD">
    <rdf:type rdf:resource="http://www.w3.org/2002/07/owl#DatatypeProperty"/>
    <rdf:type rdf:resource="http://www.w3.org/2002/07/owl#FunctionalProperty"/>
    <rdfs:domain rdf:resource="https://w3id.org/italia/onto/HER/AACTStudy"/>
    <rdfs:range rdf:resource="http://www.w3.org/2001/XMLSchema#boolean"/>
    <rdfs:comment xml:lang="en">Indication that a clinical study that includes a U.S. FDA-regulated device product is a pediatric postmarket surveillance of a device (PPSD) product ordered under section 522 of the Federal Food, Drug, and Cosmetic Act. Select true/false.</rdfs:comment>
    <rdfs:comment xml:lang="it">Indicazione che uno studio clinico che include un prodotto per dispositivi regolamentato dalla FDA statunitense è una sorveglianza pediatrica post-vendita di un prodotto per dispositivi (PPSD) ordinato ai sensi della sezione 522 del Federal Food, Drug, and Cosmetic Act. Selezionare vero/falso.</rdfs:comment>
    <rdfs:isDefinedBy rdf:resource="https://w3id.org/italia/onto/HER"/>
    <rdfs:label xml:lang="it">include sorveglianza pediatrica post-vendita prodotto per dispositivi</rdfs:label>
    <rdfs:label xml:lang="en">includes pediatric postmarket surveillance of a device</rdfs:label>
    <owl:versionInfo xml:lang="it">stabile</owl:versionInfo>
    <owl:versionInfo xml:lang="en">stable</owl:versionInfo>
  </rdf:Description>
  <rdf:Description rdf:nodeID="n5bb3bff42afb4ca286d2c3fead9507ddb490">
    <rdf:type rdf:resource="http://www.w3.org/2002/07/owl#Restriction"/>
    <owl:onProperty rdf:resource="https://w3id.org/italia/onto/HER/abstract"/>
    <owl:maxCardinality rdf:datatype="http://www.w3.org/2001/XMLSchema#nonNegativeInteger">1</owl:maxCardinality>
  </rdf:Description>
  <rdf:Description rdf:nodeID="n5bb3bff42afb4ca286d2c3fead9507ddb137">
    <rdf:type rdf:resource="http://www.w3.org/1999/02/22-rdf-syntax-ns#List"/>
    <rdf:first>None Retained</rdf:first>
    <rdf:rest rdf:nodeID="n5bb3bff42afb4ca286d2c3fead9507ddb138"/>
  </rdf:Description>
  <rdf:Description rdf:nodeID="n5bb3bff42afb4ca286d2c3fead9507ddb483">
    <rdf:type rdf:resource="http://www.w3.org/2002/07/owl#Restriction"/>
    <owl:onProperty rdf:resource="https://w3id.org/italia/onto/HER/hasErasmusplusProjectResult"/>
    <owl:allValuesFrom rdf:resource="https://w3id.org/italia/onto/HER/ErasmusPlusProjectResult"/>
  </rdf:Description>
  <rdf:Description rdf:about="https://w3id.org/italia/onto/HER/CTNPRINOperation">
    <rdf:type rdf:resource="http://www.w3.org/2002/07/owl#Class"/>
    <rdfs:subClassOf rdf:resource="https://w3id.org/italia/onto/l0/Activity"/>
    <rdfs:subClassOf rdf:nodeID="n5bb3bff42afb4ca286d2c3fead9507ddb422"/>
    <rdfs:subClassOf rdf:nodeID="n5bb3bff42afb4ca286d2c3fead9507ddb423"/>
    <rdfs:subClassOf rdf:nodeID="n5bb3bff42afb4ca286d2c3fead9507ddb424"/>
    <rdfs:subClassOf rdf:nodeID="n5bb3bff42afb4ca286d2c3fead9507ddb425"/>
    <rdfs:subClassOf rdf:nodeID="n5bb3bff42afb4ca286d2c3fead9507ddb426"/>
    <rdfs:subClassOf rdf:nodeID="n5bb3bff42afb4ca286d2c3fead9507ddb427"/>
    <rdfs:subClassOf rdf:nodeID="n5bb3bff42afb4ca286d2c3fead9507ddb428"/>
    <rdfs:subClassOf rdf:nodeID="n5bb3bff42afb4ca286d2c3fead9507ddb429"/>
    <rdfs:subClassOf rdf:nodeID="n5bb3bff42afb4ca286d2c3fead9507ddb430"/>
    <rdfs:subClassOf rdf:nodeID="n5bb3bff42afb4ca286d2c3fead9507ddb431"/>
    <rdfs:subClassOf rdf:nodeID="n5bb3bff42afb4ca286d2c3fead9507ddb432"/>
    <rdfs:comment xml:lang="en">Accounting operation, related to Local code project, scope, beneficiary</rdfs:comment>
    <rdfs:comment xml:lang="it">Operazione contabile, relativa a Codice locale progetto, ambito, beneficiario</rdfs:comment>
    <rdfs:isDefinedBy rdf:resource="https://w3id.org/italia/onto/HER"/>
    <rdfs:label xml:lang="en">CTN/PRIN Operation</rdfs:label>
    <rdfs:label xml:lang="it">Operazione CTN/PRIN</rdfs:label>
    <owl:versionInfo xml:lang="it">stabile</owl:versionInfo>
    <owl:versionInfo xml:lang="en">stable</owl:versionInfo>
  </rdf:Description>
  <rdf:Description rdf:about="https://w3id.org/italia/onto/HER/USTATAverageContributionsAggregate">
    <rdf:type rdf:resource="http://www.w3.org/2002/07/owl#Class"/>
    <rdfs:subClassOf rdf:resource="https://w3id.org/italia/onto/HER/StatisticalDataAggregation"/>
    <rdfs:subClassOf rdf:nodeID="n5bb3bff42afb4ca286d2c3fead9507ddb526"/>
    <rdfs:comment xml:lang="en">Information on the average contribution for students enrolled in I and II level degree courses (including single cycle courses) calculated on the basis of the fees actually paid (net of the regional tax for the DSU and stamp duty where applicable) .</rdfs:comment>
    <rdfs:comment xml:lang="it">Informazioni sulla contribuzione media per gli studenti iscritti a corsi di laurea di I e II livello (inclusi i corsi a ciclo unico) calcolata sulla base delle tasse realmente pagate (al netto della tassa regionale per il DSU e dell’imposta di bollo dove previste).</rdfs:comment>
    <rdfs:isDefinedBy rdf:resource="https://w3id.org/italia/onto/HER"/>
    <rdfs:label xml:lang="it">Aggregazione della contribuzione media riportata da USTAT</rdfs:label>
    <rdfs:label xml:lang="en">USTAT Aggregate of Average Contributions</rdfs:label>
    <owl:versionInfo xml:lang="it">stabile</owl:versionInfo>
    <owl:versionInfo xml:lang="en">stable</owl:versionInfo>
  </rdf:Description>
  <rdf:Description rdf:nodeID="n5bb3bff42afb4ca286d2c3fead9507ddb460">
    <rdf:type rdf:resource="http://www.w3.org/2002/07/owl#Restriction"/>
    <owl:onProperty rdf:resource="https://w3id.org/italia/onto/CLV/hasSpatialCoverage"/>
    <owl:allValuesFrom rdf:resource="https://w3id.org/italia/onto/CLV/Feature"/>
  </rdf:Description>
  <rdf:Description rdf:about="https://w3id.org/italia/onto/HER/ERCSubpanel">
    <rdf:type rdf:resource="http://www.w3.org/2002/07/owl#Class"/>
    <rdfs:subClassOf rdf:resource="https://w3id.org/italia/onto/HER/ERCClassification"/>
    <rdfs:comment xml:lang="en">English Version: http://www.unipr.it/sites/default/files/allegatiparagrafo/01-08-2013/settori_erc.pdf</rdfs:comment>
    <rdfs:comment xml:lang="it">Versione in Italiano:
https://it.wikipedia.org/wiki/Settori_ERC</rdfs:comment>
    <rdfs:isDefinedBy rdf:resource="https://w3id.org/italia/onto/HER"/>
    <rdfs:label xml:lang="en">ERC Subpanel</rdfs:label>
    <rdfs:label xml:lang="it">Sotto Pannello ERC</rdfs:label>
    <owl:versionInfo xml:lang="it">stabile</owl:versionInfo>
    <owl:versionInfo xml:lang="en">stable</owl:versionInfo>
    <ns6:wasDerivedFrom rdf:resource="http://www.w3.org/2004/02/skos/core#Concept"/>
    <ns4:controlledVocabulary rdf:resource="https://w3id.org/italia/controlled-vocabulary/classifications-for-her/erc-panel-h2020-fp"/>
  </rdf:Description>
  <rdf:Description rdf:about="https://w3id.org/italia/onto/HER/studyType">
    <rdf:type rdf:resource="http://www.w3.org/2002/07/owl#DatatypeProperty"/>
    <rdfs:domain rdf:resource="https://w3id.org/italia/onto/HER/AACTStudy"/>
    <rdfs:range rdf:resource="http://www.w3.org/2000/01/rdf-schema#Literal"/>
    <rdfs:comment xml:lang="en">Describes the nature of a clinical study. Study types include interventional studies (also called clinical trials), observational studies (including patient registries), and expanded access.</rdfs:comment>
    <rdfs:comment xml:lang="it">Descrive la natura di uno studio clinico. I tipi di studio includono studi interventistici (chiamati anche studi clinici), studi osservazionali (inclusi i registri dei pazienti) e l'accesso esteso.</rdfs:comment>
    <rdfs:isDefinedBy rdf:resource="https://w3id.org/italia/onto/HER"/>
    <rdfs:label xml:lang="en">study type</rdfs:label>
    <rdfs:label xml:lang="it">tipo di studio</rdfs:label>
    <owl:versionInfo xml:lang="it">stabile</owl:versionInfo>
    <owl:versionInfo xml:lang="en">stable</owl:versionInfo>
  </rdf:Description>
  <rdf:Description rdf:about="https://w3id.org/italia/onto/HER/USTATFunctionalArea">
    <rdf:type rdf:resource="http://www.w3.org/2002/07/owl#Class"/>
    <rdfs:subClassOf rdf:resource="https://w3id.org/italia/onto/HER/HERClassification"/>
    <rdfs:comment xml:lang="it">Indica l'area a cui fanno riferimento le funzioni del gruppo di personale tecnico-amministrativo considerato. Rappresenta una delle variabili di disaggregazione dei dati sulle carriere del personale tecnico-amministrativo. Attualmente può assumere i seguenti valori: 01-Dirigenza amministrativa; 02-Amministrativa ed Amministrativa-gestionale; 03-Biblioteche; 04-Servizi generali e tecnici; 05-Socio sanitaria; 06-Tecnica; 07-Area non individuata.</rdfs:comment>
    <rdfs:comment xml:lang="en">It indicates the area to which the functions of the technical-administrative staff group considered refer. Represents one of the variables of disaggregation of the career data of technical-administrative staff. Currently it can take on the following values: 01-Dirigenza amministrativa; 02-Amministrativa ed Amministrativa-gestionale; 03-Biblioteche; 04-Servizi generali e tecnici; 05-Socio sanitaria; 06-Tecnica; 07-Area non individuata.</rdfs:comment>
    <rdfs:isDefinedBy rdf:resource="https://w3id.org/italia/onto/HER"/>
    <rdfs:label xml:lang="it">Area funzionale</rdfs:label>
    <rdfs:label xml:lang="en">Functional Area</rdfs:label>
    <owl:versionInfo xml:lang="it">stabile</owl:versionInfo>
    <owl:versionInfo xml:lang="en">stable</owl:versionInfo>
    <ns6:wasDerivedFrom rdf:resource="http://www.w3.org/2004/02/skos/core#Concept"/>
  </rdf:Description>
  <rdf:Description rdf:about="https://w3id.org/italia/onto/RO/withRole">
    <rdf:type rdf:resource="http://www.w3.org/2002/07/owl#ObjectProperty"/>
  </rdf:Description>
  <rdf:Description rdf:about="https://w3id.org/italia/onto/HER/MIURStudentsByCitizenshipDegreeClassAggregate">
    <rdf:type rdf:resource="http://www.w3.org/2002/07/owl#Class"/>
    <rdfs:subClassOf rdf:resource="https://w3id.org/italia/onto/HER/StatisticalDataAggregation"/>
    <rdfs:comment xml:lang="en">Aggregated data on Italian students filed in the MIUR system, grouped by year, university, citizenship, degree and degree class.</rdfs:comment>
    <rdfs:comment xml:lang="it">Dati aggregati sugli studenti italiani archiviati nel sistema MIUR, raggruppati per anno, università, cittadinanza, laurea e classe di laurea.</rdfs:comment>
    <rdfs:isDefinedBy rdf:resource="https://w3id.org/italia/onto/HER"/>
    <rdfs:label xml:lang="en">Aggregate of Italian Students By Citizenship, Degree and Degree Class</rdfs:label>
    <rdfs:label xml:lang="it">Aggregazione dei studenti italiani per cittadinanza, laurea e classe di laurea</rdfs:label>
    <owl:versionInfo xml:lang="it">stabile</owl:versionInfo>
    <owl:versionInfo xml:lang="en">stable</owl:versionInfo>
  </rdf:Description>
  <rdf:Description rdf:nodeID="n5bb3bff42afb4ca286d2c3fead9507ddb119">
    <rdf:first rdf:resource="https://w3id.org/italia/onto/HER/CTNPRINOperation"/>
    <rdf:rest rdf:nodeID="n5bb3bff42afb4ca286d2c3fead9507ddb120"/>
  </rdf:Description>
  <rdf:Description rdf:about="https://w3id.org/italia/onto/HER/USTATTemporaryStaff">
    <rdf:type rdf:resource="http://www.w3.org/2002/07/owl#Class"/>
    <rdfs:subClassOf rdf:resource="https://w3id.org/italia/onto/COV/Group"/>
    <rdfs:subClassOf rdf:nodeID="n5bb3bff42afb4ca286d2c3fead9507ddb542"/>
    <rdfs:comment xml:lang="it">Personale che ha prestato servizio a tempo determinato negli Enti e negli Uffici per il Diritto allo Studio Universitario - DSU nell'anno di riferimento, aggregato per Regione.</rdfs:comment>
    <rdfs:comment xml:lang="en">Personnel who have served on a temporary basis in the Bodies and Offices for the Right to University Studies - DSU in the year of reference, aggregated by Region.</rdfs:comment>
    <rdfs:isDefinedBy rdf:resource="https://w3id.org/italia/onto/HER"/>
    <rdfs:label xml:lang="it">Personale Determinato</rdfs:label>
    <rdfs:label xml:lang="en">Temporary Staff</rdfs:label>
    <owl:versionInfo xml:lang="it">stabile</owl:versionInfo>
    <owl:versionInfo xml:lang="en">stable</owl:versionInfo>
  </rdf:Description>
  <rdf:Description rdf:about="https://w3id.org/italia/onto/HER/ctnprinInitiativeApprovedCost">
    <rdf:type rdf:resource="http://www.w3.org/2002/07/owl#DatatypeProperty"/>
    <rdfs:subPropertyOf rdf:resource="https://w3id.org/italia/onto/MU/value"/>
    <rdfs:domain rdf:resource="https://w3id.org/italia/onto/HER/CTNPRINInitiative"/>
    <rdfs:range rdf:resource="http://www.w3.org/2001/XMLSchema#decimal"/>
    <rdfs:comment xml:lang="en">Total costs approved after in itinere evaluation compared to the costs reported by the beneficiaries. Calculated as the sum of the homologous 'approvedCost' variable present at the lower aggregation level (approvedCost_operations)</rdfs:comment>
    <rdfs:comment xml:lang="it">Totale dei costi approvati dopo valutazione in itinere rispetto ai costi rendicontati dai beneficiari. Calcolati come somma dell'omologa variabile "approvedCost" presente a livello di aggregazione inferiore (approvedCost_operations)</rdfs:comment>
    <rdfs:isDefinedBy rdf:resource="https://w3id.org/italia/onto/HER"/>
    <rdfs:label xml:lang="en">approved cost of CTN/PRIN initiative</rdfs:label>
    <rdfs:label xml:lang="it">costi approvati per iniziative CTN/PRIN</rdfs:label>
    <owl:versionInfo xml:lang="it">stabile</owl:versionInfo>
    <owl:versionInfo xml:lang="en">stable</owl:versionInfo>
  </rdf:Description>
  <rdf:Description rdf:about="https://w3id.org/italia/onto/HER/USTATExonerationType">
    <rdf:type rdf:resource="http://www.w3.org/2002/07/owl#Class"/>
    <rdfs:subClassOf rdf:resource="https://w3id.org/italia/onto/l0/Characteristic"/>
    <rdfs:comment xml:lang="en">Information on the type of exemption.
In the case of partial exemption, the exemption types are characterised by the following codes/descriptions:

09: Students with a disability of less than 66% (Legislative Decree 68/12 art. 9, c. 7a)
19: Other disability situations not included in the previous ones
15: Other types not included under the above entries

In the case of total exemption, the types of exemption are characterised by the following codes/descriptions:

01: Scholarship recipients (Legislative Decree 68/12 art. 9, c. 2)
02: Eligible non-beneficiaries of scholarships (Legislative Decree 68/12 art. 9, c. 2)
03: Disabled students with disabilities over 66% (Legislative Decree 68/12 art. 9, c. 2)
16: Students who meet the requirements for NO TAX AREA (Law 232/2016, c. 255 and 256) and Beneficiaries of scholarships d.lgs. 68/12
17: Students who meet the requirements for NO TAX AREA (Law 232/2016, c. 255 and 256) and eligibility for a scholarship d.lgs. 68/12
18: Students with requirements for NO TAX AREA (L. 232/2016, c. 255 and 256)
19: Other disability situations not included in the previous ones
20: Doctoral student holder of a PhD scholarship
21: Doctoral student not holding a PhD scholarship (Law 232/2016, c. 262)
15: Other types not included under the above headings</rdfs:comment>
    <rdfs:comment xml:lang="it">Informazioni sulla tipologia di esonero.
Nel caso di esonero parziale, le tipologie di esonero sono caratterizzate dai codici/descrizioni seguenti:

09: Studenti in situazione di disabilità con invalidità inferiore al 66% (d.lgs. 68/12 art. 9, c. 7a)
19: Altre situazioni di disabilità non incluse nelle precedenti
15: Altre tipologie non comprese nelle precedenti voci

Nel caso di esonero totale, le tipologie di esonero sono caratterizzate dai codici/descrizioni seguenti:

01: Beneficiari borse studio (d.lgs. 68/12 art. 9, c. 2)
02: Idonei non beneficiari borse di studio (d.lgs. 68/12 art. 9, c. 2)
03: Studenti in situazione di disabilità con invalidità oltre il 66% (d.lgs. 68/12 art. 9, c. 2)
16: Studenti con compresenza di requisiti per NO TAX AREA (L. 232/2016, c. 255 e 256) e Beneficiari di borsa di studio d.lgs. 68/12
17: Studenti con compresenza di requisiti per NO TAX AREA (L. 232/2016, c. 255 e 256) e Idoneità per borsa di studio d.lgs. 68/12
18: Studenti con requisiti per NO TAX AREA (L. 232/2016, c. 255 e 256)
19: Altre situazioni di disabilità non incluse nelle precedenti
20: Dottorando titolare di borsa di studio di dottorato di ricerca
21: Dottorando non beneficiario di borsa (L. 232/2016, c. 262)
15: Altre tipologie non comprese nelle precedenti voci</rdfs:comment>
    <rdfs:isDefinedBy rdf:resource="https://w3id.org/italia/onto/HER"/>
    <rdfs:label xml:lang="it">Tipo (o classe) di esonero riportata da USTAT</rdfs:label>
    <rdfs:label xml:lang="en">USTAT Reported Exoneration Class</rdfs:label>
    <owl:versionInfo xml:lang="it">stabile</owl:versionInfo>
    <owl:versionInfo xml:lang="en">stable</owl:versionInfo>
  </rdf:Description>
  <rdf:Description rdf:about="https://w3id.org/italia/onto/HER/ecGrantAgreementNo">
    <rdf:type rdf:resource="http://www.w3.org/2002/07/owl#DatatypeProperty"/>
    <rdfs:subPropertyOf rdf:resource="https://w3id.org/italia/onto/l0/identifier"/>
    <rdfs:domain rdf:nodeID="n5bb3bff42afb4ca286d2c3fead9507ddb162"/>
    <rdfs:range rdf:resource="http://www.w3.org/2000/01/rdf-schema#Literal"/>
    <rdfs:comment xml:lang="en">Grant agreement identifier of an EC project.</rdfs:comment>
    <rdfs:comment xml:lang="it">Identificativo dell'accordo di finanziamento di un progetto CE.</rdfs:comment>
    <rdfs:isDefinedBy rdf:resource="https://w3id.org/italia/onto/HER"/>
    <rdfs:label xml:lang="en">ec grant agreement number</rdfs:label>
    <rdfs:label xml:lang="it">identificativo accordo finanziamento CE</rdfs:label>
    <owl:versionInfo xml:lang="it">stabile</owl:versionInfo>
    <owl:versionInfo xml:lang="en">stable</owl:versionInfo>
  </rdf:Description>
  <rdf:Description rdf:nodeID="n5bb3bff42afb4ca286d2c3fead9507ddb52">
    <rdf:first rdf:resource="https://w3id.org/italia/onto/HER/ERCProject"/>
    <rdf:rest rdf:resource="http://www.w3.org/1999/02/22-rdf-syntax-ns#nil"/>
  </rdf:Description>
  <rdf:Description rdf:about="https://w3id.org/italia/onto/HER/hasERCSubpanel">
    <rdf:type rdf:resource="http://www.w3.org/2002/07/owl#ObjectProperty"/>
    <rdfs:subPropertyOf rdf:resource="https://w3id.org/italia/onto/l0/hasTopic"/>
    <rdfs:domain rdf:nodeID="n5bb3bff42afb4ca286d2c3fead9507ddb58"/>
    <rdfs:range rdf:resource="https://w3id.org/italia/onto/HER/ERCSubpanel"/>
    <rdfs:comment xml:lang="en">Property used to specify the second level area/sector of reference (if any) for the CTN/PRIN Operation or CTN/PRIN  Project</rdfs:comment>
    <rdfs:comment xml:lang="it">Proprietà utilizzata per specificare il secondo livello dell'area/settore di riferimento (se esistente) per un'operazione o un progetto CTN/PRIN.</rdfs:comment>
    <rdfs:isDefinedBy rdf:resource="https://w3id.org/italia/onto/HER"/>
    <rdfs:label xml:lang="it">ha sotto pannello ERC</rdfs:label>
    <rdfs:label xml:lang="en">has ERC sub-panel</rdfs:label>
    <owl:versionInfo xml:lang="it">stabile</owl:versionInfo>
    <owl:versionInfo xml:lang="en">stable</owl:versionInfo>
  </rdf:Description>
  <rdf:Description rdf:nodeID="n5bb3bff42afb4ca286d2c3fead9507ddb516">
    <rdf:type rdf:resource="http://www.w3.org/2002/07/owl#Restriction"/>
    <owl:onProperty rdf:resource="https://w3id.org/italia/onto/HER/hasCessationYear"/>
    <owl:maxQualifiedCardinality rdf:datatype="http://www.w3.org/2001/XMLSchema#nonNegativeInteger">1</owl:maxQualifiedCardinality>
    <owl:onClass rdf:resource="https://w3id.org/italia/onto/TI/Year"/>
  </rdf:Description>
  <rdf:Description rdf:about="https://w3id.org/italia/onto/HER/USTATContributionRevenueClass">
    <rdf:type rdf:resource="http://www.w3.org/2002/07/owl#Class"/>
    <rdfs:subClassOf rdf:resource="https://w3id.org/italia/onto/l0/Characteristic"/>
    <rdfs:comment xml:lang="en">Information on the source of the student contribution revenue. In particular, the identifier/extended name shows the code/description of the revenue, respectively, which may consist of the values:
01 : Revenue related to degree courses, master's degree courses, courses of the old system
02 : Revenue related to PhD courses
03 : Revenue related to specialisation courses;
040: Revenue related to first and second level master's courses
041: Revenue related to courses for the purpose of teaching qualification
04a: Revenue related to other course fees
04b: Revenue related to improvement courses
05 : Regional tax for the Right to University Study - DSU (if collected by the university)
06a: Revenue related to state exams, internships and pre-registration tests
07 : Other income not required for registration
08 : Other from students, not constituent revenue.
</rdfs:comment>
    <rdfs:comment xml:lang="it">Informazioni sulla fonte del gettito della contribuzione studentesca. In particolare, l'identificativo/nome esteso riportano il codice/la descrizione del gettito, rispettivamente, e possono essumere i valori:
01 : Gettito relativo a corsi di laurea, corsi di laurea magistrale, corsi del vecchio ordinamento
02 : Gettito relativo a corsi di dottorato
03 : Gettito relativo a corsi di specializzazione
040: Gettito relativo a corsi di master di primo e secondo livello
041: Gettito relativo a corsi finalizzati all'abilitazione all'insegnamento
04a: Gettito relativo ad altri corsi
04b: Gettito relativo a corsi di perfezionamento
05 : Tassa regionale per il DSU (se riscossa da università)
06a: Gettito esami di stato, tirocini e test pre-immatricolazioni
07 : Altre entrate non necessarie per l'iscrizione
08 : Altro da studenti, non costituente gettito</rdfs:comment>
    <rdfs:isDefinedBy rdf:resource="https://w3id.org/italia/onto/HER"/>
    <rdfs:label xml:lang="it">Classe di contribuzione riportata da USTAT</rdfs:label>
    <rdfs:label xml:lang="en">USTAT Reported Contribution Revenue Class</rdfs:label>
    <owl:versionInfo xml:lang="it">stabile</owl:versionInfo>
    <owl:versionInfo xml:lang="en">stable</owl:versionInfo>
  </rdf:Description>
  <rdf:Description rdf:about="https://w3id.org/italia/onto/HER/projectCode">
    <rdf:type rdf:resource="http://www.w3.org/2002/07/owl#DatatypeProperty"/>
    <rdfs:subPropertyOf rdf:resource="https://w3id.org/italia/onto/l0/identifier"/>
    <rdfs:domain rdf:resource="https://w3id.org/italia/onto/Project/PublicInvestmentProject"/>
    <rdfs:range rdf:resource="http://www.w3.org/2000/01/rdf-schema#Literal"/>
    <rdfs:comment xml:lang="en">Identification assigned to the Project to which the operation refers in the Information System of origin. To a single project can be assigned as many operations as there are subjects carrying out the project.
This id allows you to aggregate all the operations that are part of a project.</rdfs:comment>
    <rdfs:comment xml:lang="it">Identificativo assegnato al Progetto a cui si riferisce l'operazione nel Sistema Informatico di provenienza. Ad un unico progetto possono fanno capo tante operazioni quanti sono i soggetti che svolgono il progetto.
Questo id consente di aggregare tutte le operazioni che fanno capo ad un progetto.</rdfs:comment>
    <rdfs:isDefinedBy rdf:resource="https://w3id.org/italia/onto/HER"/>
    <rdfs:label xml:lang="it">codice del progetto</rdfs:label>
    <rdfs:label xml:lang="en">project code</rdfs:label>
    <owl:versionInfo xml:lang="it">provvisoria</owl:versionInfo>
    <owl:versionInfo xml:lang="en">unstable</owl:versionInfo>
  </rdf:Description>
  <rdf:Description rdf:about="https://w3id.org/italia/onto/HER/ecContribution">
    <rdf:type rdf:resource="http://www.w3.org/2002/07/owl#DatatypeProperty"/>
    <rdfs:subPropertyOf rdf:resource="https://w3id.org/italia/onto/MU/value"/>
    <rdfs:domain rdf:nodeID="n5bb3bff42afb4ca286d2c3fead9507ddb159"/>
    <rdfs:range rdf:resource="http://www.w3.org/2001/XMLSchema#decimal"/>
    <rdfs:comment xml:lang="it">Finanziamento concesso dall'Unione Europea. L'importo è espresso in euro.</rdfs:comment>
    <rdfs:comment xml:lang="en">Funding granted by the European Union. The amount is expressed in euros.</rdfs:comment>
    <rdfs:isDefinedBy rdf:resource="https://w3id.org/italia/onto/HER"/>
    <rdfs:label xml:lang="en">EC contribution</rdfs:label>
    <rdfs:label xml:lang="it">contributo CE</rdfs:label>
    <owl:versionInfo xml:lang="it">stabile</owl:versionInfo>
    <owl:versionInfo xml:lang="en">stable</owl:versionInfo>
  </rdf:Description>
  <rdf:Description rdf:about="https://w3id.org/italia/onto/HER/patentApplicationNo">
    <rdf:type rdf:resource="http://www.w3.org/2002/07/owl#DatatypeProperty"/>
    <rdfs:subPropertyOf rdf:resource="https://w3id.org/italia/onto/l0/identifier"/>
    <rdfs:domain rdf:resource="https://w3id.org/italia/onto/HER/Patent"/>
    <rdfs:range rdf:resource="http://www.w3.org/2000/01/rdf-schema#Literal"/>
    <rdfs:comment xml:lang="it">Il numero di identificazione della domanda di brevetto.</rdfs:comment>
    <rdfs:comment xml:lang="en">The identification number of a patent application.</rdfs:comment>
    <rdfs:isDefinedBy rdf:resource="https://w3id.org/italia/onto/HER"/>
    <rdfs:label xml:lang="it">numero richiesta brevetto</rdfs:label>
    <rdfs:label xml:lang="en">patent application number</rdfs:label>
    <owl:versionInfo xml:lang="it">stabile</owl:versionInfo>
    <owl:versionInfo xml:lang="en">stable</owl:versionInfo>
  </rdf:Description>
  <rdf:Description rdf:about="https://w3id.org/italia/onto/HER/ustatCourseType">
    <rdf:type rdf:resource="http://www.w3.org/2002/07/owl#DatatypeProperty"/>
    <rdfs:domain rdf:resource="https://w3id.org/italia/onto/HER/USTATReportedPostgraduateCourse"/>
    <rdfs:range rdf:resource="http://www.w3.org/2000/01/rdf-schema#Literal"/>
    <rdfs:comment xml:lang="en">Name of the postgraduate education course; in this dataset, it can be referred to Postgraduate Schools/Level I Masters/Level II Masters/Research Doctorates.</rdfs:comment>
    <rdfs:comment xml:lang="it">Nome del corso di studio di formazione Post-Laurea; in questo dataset, si può riferire a Scuole di specializzazione/Master di I livello/Master di II livello/Dottorati di ricerca.</rdfs:comment>
    <rdfs:isDefinedBy rdf:resource="https://w3id.org/italia/onto/HER"/>
    <rdfs:label xml:lang="en">course type</rdfs:label>
    <rdfs:label xml:lang="it">tipologia di corso</rdfs:label>
    <owl:versionInfo xml:lang="it">stabile</owl:versionInfo>
    <owl:versionInfo xml:lang="en">stable</owl:versionInfo>
  </rdf:Description>
  <rdf:Description rdf:about="https://w3id.org/italia/onto/HER/hasAACTCondition">
    <rdf:type rdf:resource="http://www.w3.org/2002/07/owl#ObjectProperty"/>
    <rdfs:domain rdf:resource="https://w3id.org/italia/onto/HER/AACTStudy"/>
    <rdfs:range rdf:resource="https://w3id.org/italia/onto/HER/AACTCondition"/>
    <rdfs:comment xml:lang="it">La malattia, il disturbo, la sindrome, la malattia o la lesione che si sta studiando. Su ClinicalTrials.gov, le condizioni possono includere anche altre questioni relative alla salute, come la durata della vita, la qualità della vita e i rischi per la salute.</rdfs:comment>
    <rdfs:comment xml:lang="en">The disease, disorder, syndrome, illness, or injury that is being studied. On ClinicalTrials.gov, conditions may also include other health-related issues, such as lifespan, quality of life, and health risks.</rdfs:comment>
    <rdfs:isDefinedBy rdf:resource="https://w3id.org/italia/onto/HER"/>
    <rdfs:label xml:lang="it">ha condizione AACT</rdfs:label>
    <rdfs:label xml:lang="en">has AACT condition</rdfs:label>
    <owl:versionInfo xml:lang="it">stabile</owl:versionInfo>
    <owl:versionInfo xml:lang="en">stable</owl:versionInfo>
  </rdf:Description>
  <rdf:Description rdf:about="https://w3id.org/italia/onto/HER/AACTInterventionMeshTerm">
    <rdf:type rdf:resource="http://www.w3.org/2002/07/owl#Class"/>
    <rdfs:subClassOf rdf:resource="https://w3id.org/italia/onto/HER/AACTMeshTerm"/>
    <rdfs:comment xml:lang="it">Interventi di studio clinico documentati da NLM's Medical Subject Headings (MeSH) - thesaurus del vocabolario controllato da NLM's Medical Subject Headings (MeSH)</rdfs:comment>
    <rdfs:comment xml:lang="en">clinical study intervention appropriate descriptors from NLM's Medical Subject Headings (MeSH)-controlled vocabulary thesaurus</rdfs:comment>
    <rdfs:isDefinedBy rdf:resource="https://w3id.org/italia/onto/HER"/>
    <rdfs:label xml:lang="en">AACT Intervention Mesh Term</rdfs:label>
    <rdfs:label xml:lang="it">Termine MeSH di Intervento AACT</rdfs:label>
    <owl:versionInfo xml:lang="it">stabile</owl:versionInfo>
    <owl:versionInfo xml:lang="en">stable</owl:versionInfo>
  </rdf:Description>
  <rdf:Description rdf:about="https://w3id.org/italia/onto/HER/Spinoff">
    <rdf:type rdf:resource="http://www.w3.org/2002/07/owl#Class"/>
    <rdfs:subClassOf rdf:resource="https://w3id.org/italia/onto/COV/PrivateOrganization"/>
    <rdfs:subClassOf rdf:nodeID="n5bb3bff42afb4ca286d2c3fead9507ddb513"/>
    <rdfs:subClassOf rdf:nodeID="n5bb3bff42afb4ca286d2c3fead9507ddb514"/>
    <rdfs:subClassOf rdf:nodeID="n5bb3bff42afb4ca286d2c3fead9507ddb515"/>
    <rdfs:subClassOf rdf:nodeID="n5bb3bff42afb4ca286d2c3fead9507ddb516"/>
    <rdfs:subClassOf rdf:nodeID="n5bb3bff42afb4ca286d2c3fead9507ddb517"/>
    <rdfs:subClassOf rdf:nodeID="n5bb3bff42afb4ca286d2c3fead9507ddb518"/>
    <rdfs:subClassOf rdf:nodeID="n5bb3bff42afb4ca286d2c3fead9507ddb519"/>
    <rdfs:subClassOf rdf:nodeID="n5bb3bff42afb4ca286d2c3fead9507ddb520"/>
    <rdfs:subClassOf rdf:nodeID="n5bb3bff42afb4ca286d2c3fead9507ddb521"/>
    <rdfs:subClassOf rdf:nodeID="n5bb3bff42afb4ca286d2c3fead9507ddb522"/>
    <rdfs:subClassOf rdf:nodeID="n5bb3bff42afb4ca286d2c3fead9507ddb523"/>
    <rdfs:subClassOf rdf:nodeID="n5bb3bff42afb4ca286d2c3fead9507ddb524"/>
    <rdfs:comment xml:lang="en">Enterprise created from a pre-existing entity or unit; in this specific dataset are included the spin-offs of public research: adopting the definition of the Netval 2014 report, an "enterprise operating in high-tech sectors constituted by (at least) a university professor/researcher or a doctoral candidate/fellow/student who has carried out multiannual research activities on a specific theme, object of creation of the enterprise itself".The data are obtained from Spin-off Italia, the spin-off database of public research in Italy: https://www.spinoffitalia.it/. As indicated by the website Spin-off Italia (https://www.spinoffitalia.it/?q=about), "The database (Spin-off Italia, Editor's note) is the result of the collaboration between the Centre for Innovation and Entrepreneurship of the Polytechnic University of Marche, NetVal and the Management Institute of the Scuola Superiore Sant'Anna. The database contains information on the companies that the research group considered to associate with the spin-off concept of public research. In particular, in the database it is possible to select the companies that have been accredited as spin-offs by the research institutions of origin".</rdfs:comment>
    <rdfs:comment xml:lang="it">Impresa creata a partire da un ente o un’unità preesistente; in questo specifico dataset vengono inclusi gli spin-off della ricerca pubblica: adottando la definizione del rapporto Netval 2014, una “impresa operante in settori high-tech costituita da (almeno) un professore/ricercatore universitario o da un dottorando/contrattista/studente che abbia effettuato attività di ricerca pluriennale su un tema specifico, oggetto di creazione dell’impresa stessa”. I dati sono ottenuti da Spin-off Italia, il database degli spin-off della ricerca pubblica in Italia: https://www.spinoffitalia.it/. Come indicato dal sito Spin-off Italia (https://www.spinoffitalia.it/?q=about), "Il database (Spin-off Italia, NdR) è frutto della collaborazione fra il Centro per l'Innovazione e l'Imprenditorialità dell'Università Politecnica delle Marche, NetVal e l'Istituto di Management della Scuola Superiore Sant'Anna. Il database contiene informazioni sulle imprese che il gruppo di ricerca ha ritenuto di associare al concetto di spin-off della ricerca pubblica. In particolare, nel database è possibile selezionare le imprese che sono state accreditate come spin-off dagli enti di ricerca di provenienza."</rdfs:comment>
    <rdfs:isDefinedBy rdf:resource="https://w3id.org/italia/onto/HER"/>
    <rdfs:label xml:lang="en">Spinoff</rdfs:label>
    <rdfs:label xml:lang="it">Spinoff</rdfs:label>
    <owl:versionInfo xml:lang="it">stabile</owl:versionInfo>
    <owl:versionInfo xml:lang="en">stable</owl:versionInfo>
  </rdf:Description>
  <rdf:Description rdf:nodeID="n5bb3bff42afb4ca286d2c3fead9507ddb446">
    <rdf:type rdf:resource="http://www.w3.org/2002/07/owl#Restriction"/>
    <owl:onProperty rdf:resource="https://w3id.org/italia/onto/HER/hasECTopic"/>
    <owl:allValuesFrom rdf:resource="https://w3id.org/italia/onto/HER/ECTopic"/>
  </rdf:Description>
  <rdf:Description rdf:nodeID="n5bb3bff42afb4ca286d2c3fead9507ddb140">
    <rdf:type rdf:resource="http://www.w3.org/2002/07/owl#Class"/>
    <owl:unionOf rdf:nodeID="n5bb3bff42afb4ca286d2c3fead9507ddb141"/>
  </rdf:Description>
  <rdf:Description rdf:about="https://w3id.org/italia/onto/HER/resultsFirstSubmittedQCDate">
    <rdf:type rdf:resource="http://www.w3.org/2002/07/owl#DatatypeProperty"/>
    <rdfs:subPropertyOf rdf:resource="https://w3id.org/italia/onto/TI/date"/>
    <rdfs:domain rdf:resource="https://w3id.org/italia/onto/HER/AACTStudy"/>
    <rdfs:range rdf:resource="http://www.w3.org/2001/XMLSchema#date"/>
    <rdfs:comment xml:lang="it">Il suffisso _submitted_qc indica la data di presentazione della versione del record che soddisfa i criteri di controllo della qualità. È comune che ci siano revisioni tra la prima presentazione e la presentazione che soddisfa i criteri qc. Si noti che questa non è la data in cui è stata completata la revisione qc.</rdfs:comment>
    <rdfs:comment xml:lang="en">The _submitted_qc suffix indicates the submission date of the version of the record that met quality control criteria. It is common for there to be revisions between the first submission and the submission that meets qc criteria. Note this is not the date that the qc review was completed.</rdfs:comment>
    <rdfs:isDefinedBy rdf:resource="https://w3id.org/italia/onto/HER"/>
    <rdfs:label xml:lang="en">results first submitted QC date</rdfs:label>
    <rdfs:label xml:lang="it">risultati prima data invio QC</rdfs:label>
    <owl:versionInfo xml:lang="it">stabile</owl:versionInfo>
    <owl:versionInfo xml:lang="en">stable</owl:versionInfo>
  </rdf:Description>
  <rdf:Description rdf:nodeID="n5bb3bff42afb4ca286d2c3fead9507ddb404">
    <rdf:type rdf:resource="http://www.w3.org/2002/07/owl#Restriction"/>
    <owl:onProperty rdf:resource="https://w3id.org/italia/onto/HER/hasCHAFEAParticipant"/>
    <owl:someValuesFrom rdf:resource="https://w3id.org/italia/onto/HER/CHAFEAParticipant"/>
  </rdf:Description>
  <rdf:Description rdf:about="https://w3id.org/italia/onto/CPV/Person">
    <rdf:type rdf:resource="http://www.w3.org/2002/07/owl#Class"/>
    <rdfs:subClassOf rdf:nodeID="n5bb3bff42afb4ca286d2c3fead9507ddb369"/>
  </rdf:Description>
  <rdf:Description rdf:nodeID="n5bb3bff42afb4ca286d2c3fead9507ddb247">
    <rdf:type rdf:resource="http://www.w3.org/2002/07/owl#Class"/>
    <owl:unionOf rdf:nodeID="n5bb3bff42afb4ca286d2c3fead9507ddb248"/>
  </rdf:Description>
  <rdf:Description rdf:about="https://w3id.org/italia/onto/HER/ctnprinAmountReportedCost">
    <rdf:type rdf:resource="http://www.w3.org/2002/07/owl#DatatypeProperty"/>
    <rdfs:subPropertyOf rdf:resource="https://w3id.org/italia/onto/MU/value"/>
    <rdfs:domain rdf:resource="https://w3id.org/italia/onto/HER/CTNPRINAmount"/>
    <rdfs:range rdf:resource="http://www.w3.org/2001/XMLSchema#decimal"/>
    <rdfs:comment xml:lang="en">Cost reported by the beneficiary to which the operation relates by single expense item compared to the eligible costs</rdfs:comment>
    <rdfs:comment xml:lang="it">Costo rendicontato dal beneficiaro a cui fa capo l'operazione per singola voce di spesa rispetto ai costi ammessi</rdfs:comment>
    <rdfs:isDefinedBy rdf:resource="https://w3id.org/italia/onto/HER"/>
    <rdfs:label xml:lang="it">costo rendicontato dell'importo CTN/PRIN</rdfs:label>
    <rdfs:label xml:lang="en">reported cost of CTN/PRIN amount</rdfs:label>
    <owl:versionInfo xml:lang="it">stabile</owl:versionInfo>
    <owl:versionInfo xml:lang="en">stable</owl:versionInfo>
  </rdf:Description>
  <rdf:Description rdf:nodeID="n5bb3bff42afb4ca286d2c3fead9507ddb406">
    <rdf:type rdf:resource="http://www.w3.org/2002/07/owl#Restriction"/>
    <owl:onProperty rdf:resource="https://w3id.org/italia/onto/HER/hasInstrument"/>
    <owl:qualifiedCardinality rdf:datatype="http://www.w3.org/2001/XMLSchema#nonNegativeInteger">1</owl:qualifiedCardinality>
    <owl:onClass rdf:resource="https://w3id.org/italia/onto/HER/CHAFEAInstrument"/>
  </rdf:Description>
  <rdf:Description rdf:nodeID="n5bb3bff42afb4ca286d2c3fead9507ddb166">
    <rdf:first rdf:resource="https://w3id.org/italia/onto/HER/ECProject"/>
    <rdf:rest rdf:nodeID="n5bb3bff42afb4ca286d2c3fead9507ddb167"/>
  </rdf:Description>
  <rdf:Description rdf:about="https://w3id.org/italia/onto/HER/MacroSector">
    <rdf:type rdf:resource="http://www.w3.org/2002/07/owl#Class"/>
    <rdfs:subClassOf rdf:resource="https://w3id.org/italia/onto/HER/AcademicDiscipline"/>
    <rdfs:isDefinedBy rdf:resource="https://w3id.org/italia/onto/HER"/>
    <rdfs:label xml:lang="en">Macro Sector</rdfs:label>
    <rdfs:label xml:lang="it">Macro Settore</rdfs:label>
    <owl:versionInfo xml:lang="it">stabile</owl:versionInfo>
    <owl:versionInfo xml:lang="en">stable</owl:versionInfo>
    <ns6:wasDerivedFrom rdf:resource="http://www.w3.org/2004/02/skos/core#Concept"/>
    <ns4:controlledVocabulary rdf:resource="https://w3id.org/italia/controlled-vocabulary/classifications-for-universities/academic-disciplines"/>
  </rdf:Description>
  <rdf:Description rdf:about="https://w3id.org/italia/onto/HER/hasPrincipalInvestigator">
    <rdf:type rdf:resource="http://www.w3.org/2002/07/owl#ObjectProperty"/>
    <rdfs:domain rdf:resource="https://w3id.org/italia/onto/Project/PublicResearchProject"/>
    <rdfs:range rdf:resource="https://w3id.org/italia/onto/CPV/Person"/>
    <rdfs:comment xml:lang="it">Esaminatore principale del progetto</rdfs:comment>
    <rdfs:comment xml:lang="en">Principal investigator of the project</rdfs:comment>
    <rdfs:isDefinedBy rdf:resource="https://w3id.org/italia/onto/HER"/>
    <rdfs:label xml:lang="it">ha esaminatore principale</rdfs:label>
    <rdfs:label xml:lang="en">has principal investigator</rdfs:label>
    <owl:versionInfo xml:lang="it">provvisoria - verificare la definizione</owl:versionInfo>
    <owl:versionInfo xml:lang="en">unstable</owl:versionInfo>
  </rdf:Description>
  <rdf:Description rdf:nodeID="n5bb3bff42afb4ca286d2c3fead9507ddb469">
    <rdf:type rdf:resource="http://www.w3.org/2002/07/owl#Restriction"/>
    <owl:onProperty rdf:resource="https://w3id.org/italia/onto/HER/status"/>
    <owl:someValuesFrom rdf:resource="http://www.w3.org/2000/01/rdf-schema#Literal"/>
  </rdf:Description>
  <rdf:Description rdf:about="https://w3id.org/italia/onto/HER/forECProject">
    <rdf:type rdf:resource="http://www.w3.org/2002/07/owl#ObjectProperty"/>
    <rdfs:subPropertyOf rdf:resource="https://w3id.org/italia/onto/RO/forEntity"/>
    <rdfs:domain rdf:resource="https://w3id.org/italia/onto/HER/ECParticipant"/>
    <rdfs:range rdf:nodeID="n5bb3bff42afb4ca286d2c3fead9507ddb1"/>
    <rdfs:comment xml:lang="it">Questa proprietà si collega ad un corrispondente progetto della CE.</rdfs:comment>
    <rdfs:comment xml:lang="en">This property links to a corresponding EC project.</rdfs:comment>
    <rdfs:isDefinedBy rdf:resource="https://w3id.org/italia/onto/HER"/>
    <rdfs:label xml:lang="it">ha un progetto CE</rdfs:label>
    <rdfs:label xml:lang="en">has ec project</rdfs:label>
    <owl:versionInfo xml:lang="it">prova</owl:versionInfo>
    <owl:versionInfo xml:lang="en">testing</owl:versionInfo>
  </rdf:Description>
  <rdf:Description rdf:nodeID="n5bb3bff42afb4ca286d2c3fead9507ddb342">
    <rdf:first rdf:resource="https://w3id.org/italia/onto/HER/USTATPostgraduateAggregateOfRegistered"/>
    <rdf:rest rdf:nodeID="n5bb3bff42afb4ca286d2c3fead9507ddb343"/>
  </rdf:Description>
  <rdf:Description rdf:about="https://w3id.org/italia/onto/HER/cycleStartingYear">
    <rdf:type rdf:resource="http://www.w3.org/2002/07/owl#DatatypeProperty"/>
    <rdfs:subPropertyOf rdf:resource="https://w3id.org/italia/onto/TI/year"/>
    <rdfs:domain rdf:resource="https://w3id.org/italia/onto/HER/ItalianPhDCourseByCycle"/>
    <rdfs:range rdf:resource="http://www.w3.org/2001/XMLSchema#gYear"/>
    <rdfs:comment xml:lang="it">L'anno di inizio del ciclo accademico corrispondente.</rdfs:comment>
    <rdfs:comment xml:lang="en">The start year of the corresponding academic cycle.</rdfs:comment>
    <rdfs:isDefinedBy rdf:resource="https://w3id.org/italia/onto/HER"/>
    <rdfs:label xml:lang="it">anno di inizio del ciclo</rdfs:label>
    <rdfs:label xml:lang="en">cycle starting year</rdfs:label>
    <owl:versionInfo xml:lang="it">stabile</owl:versionInfo>
    <owl:versionInfo xml:lang="en">stable</owl:versionInfo>
  </rdf:Description>
  <rdf:Description rdf:about="https://w3id.org/italia/onto/HER/USTATContributionRevenue">
    <rdf:type rdf:resource="http://www.w3.org/2002/07/owl#Class"/>
    <rdfs:subClassOf rdf:resource="https://w3id.org/italia/onto/HER/StatisticalDataAggregation"/>
    <rdfs:subClassOf rdf:nodeID="n5bb3bff42afb4ca286d2c3fead9507ddb528"/>
    <rdfs:comment xml:lang="en">Data on the revenue from the student contribution of the universities, in particular the student contribution and other income from students, the final balance sheet and the established budget. The balance sheet refers to the year (T-1).</rdfs:comment>
    <rdfs:comment xml:lang="it">Dati relativi al gettito della contribuzione studentesca degli atenei, in particolare alla contribuzione studentesca e alle altre entrate provenienti dagli studenti, al conto consuntivo e al bilancio di previsione assestato. Conto consuntivo: riferimento all'anno (T-1).</rdfs:comment>
    <rdfs:isDefinedBy rdf:resource="https://w3id.org/italia/onto/HER"/>
    <rdfs:label xml:lang="it">Aggregazione dei ricavi del contributo riportato da USTAT</rdfs:label>
    <rdfs:label xml:lang="en">USTAT Aggregate of Contribution Revenue</rdfs:label>
    <owl:versionInfo xml:lang="it">stabile</owl:versionInfo>
    <owl:versionInfo xml:lang="en">stable</owl:versionInfo>
  </rdf:Description>
  <rdf:Description rdf:about="https://w3id.org/italia/onto/HER/hasAACTFacility">
    <rdf:type rdf:resource="http://www.w3.org/2002/07/owl#ObjectProperty"/>
    <rdfs:domain rdf:resource="https://w3id.org/italia/onto/HER/AACTStudy"/>
    <rdfs:range rdf:resource="https://w3id.org/italia/onto/HER/AACTFacility"/>
    <rdfs:comment xml:lang="it">conduzione del sito/partecipazione ad uno studio</rdfs:comment>
    <rdfs:comment xml:lang="en">site conducting/participating in a study</rdfs:comment>
    <rdfs:isDefinedBy rdf:resource="https://w3id.org/italia/onto/HER"/>
    <rdfs:label xml:lang="it">ha struttura per sperimentazione clinica</rdfs:label>
    <rdfs:label xml:lang="en">has clinical trial facility</rdfs:label>
    <owl:versionInfo xml:lang="it">provvisoria - da verificare</owl:versionInfo>
    <owl:versionInfo xml:lang="en">unstable - to be verified</owl:versionInfo>
  </rdf:Description>
  <rdf:Description rdf:about="https://w3id.org/italia/onto/HER/hasResearcherSeniorityGrade">
    <rdf:type rdf:resource="http://www.w3.org/2002/07/owl#ObjectProperty"/>
    <rdfs:domain rdf:resource="https://w3id.org/italia/onto/HER/USTATStaffByGender"/>
    <rdfs:range rdf:resource="https://w3id.org/italia/onto/HER/ResearcherSeniorityGrade"/>
    <rdfs:comment xml:lang="it">Codice identificativo della qualifica ricoperta dal personale docente/ricercatore secondo la classificazione del Manuale di Frascati 2015. La corrispondenza tra gradi e qualifica è la seguente: Grade A = Prof. I fascia (ordinario); Grade B = Prof. II fascia (associato); Grade C = Ricercatore a tempo indeterminato e determinato; Grade D = Titolare di assegno di ricerca.</rdfs:comment>
    <rdfs:comment xml:lang="en">Identification code of the qualification held by the teaching staff/researcher according to the classification of the Frascati Manual 2015. The correspondence between grades and qualification is as follows: Grade A = Prof. I category (ordinary); Grade B = Prof. II category (associated); Grade C = Permanent and temporary researcher; Grade D = Holder of research grant.</rdfs:comment>
    <rdfs:isDefinedBy rdf:resource="https://w3id.org/italia/onto/HER"/>
    <rdfs:label xml:lang="it">ha anzianità di servizio del ricercatore</rdfs:label>
    <rdfs:label xml:lang="en">has researcher seniority grade</rdfs:label>
    <owl:versionInfo xml:lang="it">stabile</owl:versionInfo>
    <owl:versionInfo xml:lang="en">stable</owl:versionInfo>
  </rdf:Description>
  <rdf:Description rdf:about="https://w3id.org/italia/onto/HER/ErasmusPlusClassification">
    <rdf:type rdf:resource="http://www.w3.org/2002/07/owl#Class"/>
    <rdfs:subClassOf rdf:resource="https://w3id.org/italia/onto/HER/ECClassification"/>
    <rdfs:comment xml:lang="en">It is used to classify the erasmus plus projects under the European Commission classification.</rdfs:comment>
    <rdfs:comment xml:lang="it">Viene utilizzato per classificare i progetti erasmus plus nella classificazione della Commissione Europea.</rdfs:comment>
    <rdfs:isDefinedBy rdf:resource="https://w3id.org/italia/onto/HER"/>
    <rdfs:label xml:lang="en">Erasmus+ Classification</rdfs:label>
    <rdfs:label xml:lang="it">classificazione Erasmus+</rdfs:label>
    <owl:versionInfo xml:lang="it">stabile</owl:versionInfo>
    <owl:versionInfo xml:lang="en">stable</owl:versionInfo>
    <ns6:wasDerivedFrom rdf:resource="http://www.w3.org/2004/02/skos/core#ConceptScheme"/>
  </rdf:Description>
  <rdf:Description rdf:nodeID="n5bb3bff42afb4ca286d2c3fead9507ddb533">
    <rdf:type rdf:resource="http://www.w3.org/2002/07/owl#Restriction"/>
    <owl:onProperty rdf:resource="https://w3id.org/italia/onto/COV/hasOrganization"/>
    <owl:maxQualifiedCardinality rdf:datatype="http://www.w3.org/2001/XMLSchema#nonNegativeInteger">1</owl:maxQualifiedCardinality>
    <owl:onClass rdf:resource="https://w3id.org/italia/onto/COV/Organization"/>
  </rdf:Description>
  <rdf:Description rdf:about="https://w3id.org/italia/onto/COV/Employment">
    <rdf:type rdf:resource="http://www.w3.org/2002/07/owl#Class"/>
  </rdf:Description>
  <rdf:Description rdf:about="https://w3id.org/italia/onto/HER/MIURStudentsByCitizenshipAggregate">
    <rdf:type rdf:resource="http://www.w3.org/2002/07/owl#Class"/>
    <rdfs:subClassOf rdf:resource="https://w3id.org/italia/onto/HER/StatisticalDataAggregation"/>
    <rdfs:comment xml:lang="en">Aggregated data on Italian students filed in the MIUR system, grouped by year, university and citizenship.</rdfs:comment>
    <rdfs:comment xml:lang="it">Dati aggregati sugli studenti italiani archiviati nel sistema MIUR, raggruppati per anno, università e cittadinanza.</rdfs:comment>
    <rdfs:isDefinedBy rdf:resource="https://w3id.org/italia/onto/HER"/>
    <rdfs:label xml:lang="en">Aggregate of Italian Students By Citizenship</rdfs:label>
    <rdfs:label xml:lang="it">Aggregazione dei studenti italiani per cittadinanza</rdfs:label>
    <owl:versionInfo xml:lang="it">stabile</owl:versionInfo>
    <owl:versionInfo xml:lang="en">stable</owl:versionInfo>
  </rdf:Description>
  <rdf:Description rdf:about="https://w3id.org/italia/onto/HER/removedCountry">
    <rdf:type rdf:resource="http://www.w3.org/2002/07/owl#DatatypeProperty"/>
    <rdf:type rdf:resource="http://www.w3.org/2002/07/owl#FunctionalProperty"/>
    <rdfs:domain rdf:resource="https://w3id.org/italia/onto/HER/CountryInvolvement"/>
    <rdfs:range rdf:resource="http://www.w3.org/2001/XMLSchema#boolean"/>
    <rdfs:comment xml:lang="en">Country where a facility conducting a clinical protocol was removed from study</rdfs:comment>
    <rdfs:comment xml:lang="it">Paese in cui una struttura che conduce un protocollo clinico è stata rimossa dallo studio</rdfs:comment>
    <rdfs:isDefinedBy rdf:resource="https://w3id.org/italia/onto/HER"/>
    <rdfs:label xml:lang="en">country removed</rdfs:label>
    <rdfs:label xml:lang="it">paese rimosso</rdfs:label>
    <owl:versionInfo xml:lang="it">stabile</owl:versionInfo>
    <owl:versionInfo xml:lang="en">stable</owl:versionInfo>
  </rdf:Description>
  <rdf:Description rdf:about="https://w3id.org/italia/onto/HER/sponsorType">
    <rdf:type rdf:resource="http://www.w3.org/2002/07/owl#DatatypeProperty"/>
    <rdfs:domain rdf:resource="https://w3id.org/italia/onto/HER/AACTSponsor"/>
    <rdfs:range rdf:resource="http://www.w3.org/2000/01/rdf-schema#Literal"/>
    <rdfs:comment xml:lang="en">Broad Category of sponsor. They can be: Other, Industry, NIH, US. Fed</rdfs:comment>
    <rdfs:comment xml:lang="it">Tipo di sponsor specificato con una stringa. Possono essere: Altro, Industria, NIH, USA. Fed</rdfs:comment>
    <rdfs:isDefinedBy rdf:resource="https://w3id.org/italia/onto/HER"/>
    <rdfs:label xml:lang="en">sponsor type</rdfs:label>
    <rdfs:label xml:lang="it">tipo di sponsor</rdfs:label>
    <owl:versionInfo xml:lang="it">stabile</owl:versionInfo>
    <owl:versionInfo xml:lang="en">stable</owl:versionInfo>
  </rdf:Description>
  <rdf:Description rdf:nodeID="n5bb3bff42afb4ca286d2c3fead9507ddb548">
    <rdf:type rdf:resource="http://www.w3.org/2002/07/owl#Restriction"/>
    <owl:onProperty rdf:resource="https://w3id.org/italia/onto/HER/hasPrincipalInvestigator"/>
    <owl:maxQualifiedCardinality rdf:datatype="http://www.w3.org/2001/XMLSchema#nonNegativeInteger">1</owl:maxQualifiedCardinality>
    <owl:onClass rdf:resource="https://w3id.org/italia/onto/CPV/Person"/>
  </rdf:Description>
  <rdf:Description rdf:about="https://w3id.org/italia/onto/HER/regionalExpense">
    <rdf:type rdf:resource="http://www.w3.org/2002/07/owl#DatatypeProperty"/>
    <rdfs:domain rdf:resource="https://w3id.org/italia/onto/HER/USTATUniversityInterventionExpensesAggregate"/>
    <rdfs:range rdf:resource="http://www.w3.org/2001/XMLSchema#decimal"/>
    <rdfs:comment xml:lang="en">Amount of expenditure financed with funds from the Region. Data are related to the financial year per year (T-1).</rdfs:comment>
    <rdfs:comment xml:lang="it">Importo della spesa finanziata con fondi della Regione. I dati sono relativi all'esercizio finanziario all'anno (T-1)</rdfs:comment>
    <rdfs:isDefinedBy rdf:resource="https://w3id.org/italia/onto/HER"/>
    <rdfs:label xml:lang="en">regional expense</rdfs:label>
    <rdfs:label xml:lang="it">spese regionali</rdfs:label>
    <owl:versionInfo xml:lang="it">provvisoria - verificare il codominio</owl:versionInfo>
    <owl:versionInfo xml:lang="en">unstable - check the range</owl:versionInfo>
  </rdf:Description>
  <rdf:Description rdf:about="https://w3id.org/italia/onto/HER/ctnprinAmountScope">
    <rdf:type rdf:resource="http://www.w3.org/2002/07/owl#DatatypeProperty"/>
    <rdfs:domain rdf:resource="https://w3id.org/italia/onto/HER/CTNPRINAmount"/>
    <rdfs:range rdf:nodeID="n5bb3bff42afb4ca286d2c3fead9507ddb143"/>
    <rdfs:comment xml:lang="it">Ambito operativo a cui si riferisce l'importo tra quelli previsti dall'iniziativa:
- Ricerca di base
- Ricerca industriale
- Sviluppo
- Formazione</rdfs:comment>
    <rdfs:comment xml:lang="en">Operational scope to which the amount among those foreseen by the initiative refers:
- Basic research
- Industrial research
- Development
- Training</rdfs:comment>
    <rdfs:isDefinedBy rdf:resource="https://w3id.org/italia/onto/HER"/>
    <rdfs:label xml:lang="it">ambito di importo CTN/PRIN</rdfs:label>
    <rdfs:label xml:lang="en">scope of CTN/PRIN amount</rdfs:label>
    <owl:versionInfo xml:lang="it">stabile</owl:versionInfo>
    <owl:versionInfo xml:lang="en">stable</owl:versionInfo>
  </rdf:Description>
  <rdf:Description rdf:about="https://w3id.org/italia/onto/HER/publicationYear">
    <rdf:type rdf:resource="http://www.w3.org/2002/07/owl#DatatypeProperty"/>
    <rdfs:subPropertyOf rdf:resource="https://w3id.org/italia/onto/TI/year"/>
    <rdfs:domain rdf:nodeID="n5bb3bff42afb4ca286d2c3fead9507ddb268"/>
    <rdfs:range rdf:resource="http://www.w3.org/2001/XMLSchema#gYear"/>
    <rdfs:comment xml:lang="it">L'anno di pubblicazione.</rdfs:comment>
    <rdfs:comment xml:lang="en">The year of publication.</rdfs:comment>
    <rdfs:isDefinedBy rdf:resource="https://w3id.org/italia/onto/HER"/>
    <rdfs:label xml:lang="it">anno di pubblicazione</rdfs:label>
    <rdfs:label xml:lang="en">publication year</rdfs:label>
    <owl:versionInfo xml:lang="it">stabile</owl:versionInfo>
    <owl:versionInfo xml:lang="en">stable</owl:versionInfo>
  </rdf:Description>
  <rdf:Description rdf:about="https://w3id.org/italia/onto/HER/leaderName">
    <rdf:type rdf:resource="http://www.w3.org/2002/07/owl#DatatypeProperty"/>
    <rdfs:subPropertyOf rdf:resource="https://w3id.org/italia/onto/l0/name"/>
    <rdfs:domain rdf:resource="https://w3id.org/italia/onto/HER/CHAFEAOutput"/>
    <rdfs:range rdf:resource="http://www.w3.org/2000/01/rdf-schema#Literal"/>
    <rdfs:comment xml:lang="en">Instrument leading Institution</rdfs:comment>
    <rdfs:comment xml:lang="it">Strumento che guida l'istituzione</rdfs:comment>
    <rdfs:isDefinedBy rdf:resource="https://w3id.org/italia/onto/HER"/>
    <rdfs:label xml:lang="en">leader name</rdfs:label>
    <rdfs:label xml:lang="it">nome del capo</rdfs:label>
    <owl:versionInfo xml:lang="it">provvisoria - valutare la possibilità di utilizzare le proprietà di coinvolgimento del progetto.</owl:versionInfo>
    <owl:versionInfo xml:lang="en">unstable</owl:versionInfo>
  </rdf:Description>
  <rdf:Description rdf:nodeID="n5bb3bff42afb4ca286d2c3fead9507ddb425">
    <rdf:type rdf:resource="http://www.w3.org/2002/07/owl#Restriction"/>
    <owl:onProperty rdf:resource="https://w3id.org/italia/onto/HER/ctnprinOperationScope"/>
    <owl:someValuesFrom rdf:resource="http://www.w3.org/2000/01/rdf-schema#Literal"/>
  </rdf:Description>
  <rdf:Description rdf:nodeID="n5bb3bff42afb4ca286d2c3fead9507ddb188">
    <rdf:type rdf:resource="http://www.w3.org/1999/02/22-rdf-syntax-ns#List"/>
    <rdf:first>None (Open Label)</rdf:first>
    <rdf:rest rdf:nodeID="n5bb3bff42afb4ca286d2c3fead9507ddb189"/>
  </rdf:Description>
  <rdf:Description rdf:nodeID="n5bb3bff42afb4ca286d2c3fead9507ddb313">
    <rdf:first rdf:resource="https://w3id.org/italia/onto/HER/USTATInterventionsForStudentsByUniversitiesAggregate"/>
    <rdf:rest rdf:resource="http://www.w3.org/1999/02/22-rdf-syntax-ns#nil"/>
  </rdf:Description>
  <rdf:Description rdf:about="https://w3id.org/italia/onto/HER/hasCTNPRINFinancingFund">
    <rdf:type rdf:resource="http://www.w3.org/2002/07/owl#ObjectProperty"/>
    <rdfs:domain rdf:resource="https://w3id.org/italia/onto/HER/CTNPRINInitiative"/>
    <rdfs:range rdf:resource="https://w3id.org/italia/onto/HER/CTNPRINFinancingFund"/>
    <rdfs:comment xml:lang="it">Collega un'iniziativa al fondo di finanziamento da cui l'iniziativa attinge le sue risorse economiche</rdfs:comment>
    <rdfs:comment xml:lang="en">Connects an initiative to the financing fund from which the initiative draws its economic resources</rdfs:comment>
    <rdfs:isDefinedBy rdf:resource="https://w3id.org/italia/onto/HER"/>
    <rdfs:label xml:lang="en">ha CTN/PRIN financing fund</rdfs:label>
    <rdfs:label xml:lang="it">ha fondo di finanziamento CTN/PRIN</rdfs:label>
    <owl:versionInfo xml:lang="it">provvisoria</owl:versionInfo>
    <owl:versionInfo xml:lang="en">unstable</owl:versionInfo>
  </rdf:Description>
  <rdf:Description rdf:about="https://w3id.org/italia/onto/HER/availableSlot">
    <rdf:type rdf:resource="http://www.w3.org/2002/07/owl#DatatypeProperty"/>
    <rdfs:domain rdf:resource="https://w3id.org/italia/onto/HER/USTATUniversityFacilitiesAggregate"/>
    <rdfs:range rdf:resource="http://www.w3.org/2001/XMLSchema#integer"/>
    <rdfs:comment xml:lang="it">Numero di posti complessivamente disponibili nelle mense e residenze universitarie direttamente gestite dall'istituto all'1/11/(T).
Dalle "Note sul dataset Contribuzione e interventi":
I valori negativi hanno i seguenti significati:
-1: ateneo non rispondente/inadempiente
-2: dato non disponibile
-3: dato non pervenuto
-4: dato incluso in altra voce
-5: dato da definire
-6: dato non rilevabile

Gli spazi vuoti indicano un valore non esistente.</rdfs:comment>
    <rdfs:comment xml:lang="en">Total number of places available in canteens and university residences directly managed by the institute on 1/11/(T).
From "Notes on the dataset Contribution and interventions"":
The negative values have the following meanings
-1: university not responding / non-compliant
-2: data not available
-3: data not received
-4: data included under another heading
-5: data to be defined
-6: data not detectable

Blanks indicate a non-existent value.</rdfs:comment>
    <rdfs:isDefinedBy rdf:resource="https://w3id.org/italia/onto/HER"/>
    <rdfs:label xml:lang="en">available slot</rdfs:label>
    <rdfs:label xml:lang="it">slot disponibile</rdfs:label>
    <owl:versionInfo xml:lang="it">stabile</owl:versionInfo>
    <owl:versionInfo xml:lang="en">stable</owl:versionInfo>
  </rdf:Description>
  <rdf:Description rdf:nodeID="n5bb3bff42afb4ca286d2c3fead9507ddb522">
    <rdf:type rdf:resource="http://www.w3.org/2002/07/owl#Restriction"/>
    <owl:onProperty rdf:resource="https://w3id.org/italia/onto/HER/founderPatent"/>
    <owl:qualifiedCardinality rdf:datatype="http://www.w3.org/2001/XMLSchema#nonNegativeInteger">1</owl:qualifiedCardinality>
    <owl:onDataRange rdf:resource="http://www.w3.org/2001/XMLSchema#boolean"/>
  </rdf:Description>
  <rdf:Description rdf:about="https://w3id.org/italia/onto/HER/aactCriterion">
    <rdf:type rdf:resource="http://www.w3.org/2002/07/owl#DatatypeProperty"/>
    <rdfs:domain rdf:resource="https://w3id.org/italia/onto/HER/AACTEligibility"/>
    <rdfs:range rdf:resource="http://www.w3.org/2000/01/rdf-schema#Literal"/>
    <rdfs:comment xml:lang="it">Criteri di ammissibilità nel contesto delle Aggregated Analysis for clininca trials. I criteri di ammissibilità consistono sia in criteri di inclusione (che sono richiesti per una persona per partecipare allo studio) sia in criteri di esclusione (che impediscono a una persona di partecipare). I tipi di criteri di ammissibilità si riferiscono a stabilire se uno studio accetta volontari sani, se ha requisiti di età o di gruppo d'età o se è limitato dal sesso.</rdfs:comment>
    <rdfs:comment xml:lang="en">Eligibility criteria in the contest of Aggregated Analysis of Clinical Trials (AACT). Eligibility criteria consist of both inclusion criteria (which are required for a person to participate in the study) and exclusion criteria (which prevent a person from participating). Types of eligibility criteria include whether a study accepts healthy volunteers, has age or age group requirements, or is limited by sex.</rdfs:comment>
    <rdfs:isDefinedBy rdf:resource="https://w3id.org/italia/onto/HER"/>
    <rdfs:label xml:lang="en">AACT criterion</rdfs:label>
    <rdfs:label xml:lang="it">Criterio AACT</rdfs:label>
    <owl:versionInfo xml:lang="it">provvisoria - valutare la possibilità di introdurre una classe Criterion allineata con il vocabolario europeo Core Criterion e Core Evidence del programma ISA2</owl:versionInfo>
    <owl:versionInfo xml:lang="en">unstable - evaluate the possibility to have a class Criterion (aligned with Core Criterion and Core Evidence of ISA2 core vocabularies)</owl:versionInfo>
  </rdf:Description>
  <rdf:Description rdf:about="https://w3id.org/italia/onto/HER/DSUCanteenAndAccomodationsAggregate">
    <rdf:type rdf:resource="http://www.w3.org/2002/07/owl#Class"/>
    <rdfs:subClassOf rdf:resource="https://w3id.org/italia/onto/HER/StatisticalDataAggregation"/>
    <rdfs:comment xml:lang="en">Information on accommodation and canteens active at 1/11 of the reference year.</rdfs:comment>
    <rdfs:comment xml:lang="it">Informazioni sui posti alloggio e mense attive all'1/11 dell'anno di riferimento.</rdfs:comment>
    <rdfs:isDefinedBy rdf:resource="https://w3id.org/italia/onto/HER"/>
    <rdfs:label xml:lang="it">Aggregazione degli alloggi e mense riportate da DSU</rdfs:label>
    <rdfs:label xml:lang="en">DSU Aggregate of Canteen And Accommodations</rdfs:label>
    <owl:versionInfo xml:lang="it">stabile</owl:versionInfo>
    <owl:versionInfo xml:lang="en">stable</owl:versionInfo>
  </rdf:Description>
  <rdf:Description rdf:about="https://w3id.org/italia/onto/HER/hasUSTATReportedUniversityFacilityType">
    <rdf:type rdf:resource="http://www.w3.org/2002/07/owl#ObjectProperty"/>
    <rdfs:domain rdf:resource="https://w3id.org/italia/onto/HER/USTATUniversityFacilitiesAggregate"/>
    <rdfs:range rdf:resource="https://w3id.org/italia/onto/HER/USTATReportedUniversityFacilityType"/>
    <rdfs:comment xml:lang="it">Questa proprietà collega l'informazione sulle strutture universitarie (mense e residenze universitarie direttamente gestite dall'istituto) al codice e descrizione della struttura.</rdfs:comment>
    <rdfs:comment xml:lang="en">This property links information on university facilities (canteens and university residences directly managed by the institute) to the code and description of the structure.</rdfs:comment>
    <rdfs:isDefinedBy rdf:resource="https://w3id.org/italia/onto/HER"/>
    <rdfs:label xml:lang="it">ha un tipo di struttura universitaria riportata da USTAT</rdfs:label>
    <rdfs:label xml:lang="en">has USTAT reported university facility type</rdfs:label>
    <owl:versionInfo xml:lang="it">stabile</owl:versionInfo>
    <owl:versionInfo xml:lang="en">stable</owl:versionInfo>
  </rdf:Description>
  <rdf:Description rdf:about="https://w3id.org/italia/onto/HER/averageTaxForPayingStudents">
    <rdf:type rdf:resource="http://www.w3.org/2002/07/owl#DatatypeProperty"/>
    <rdfs:subPropertyOf rdf:resource="https://w3id.org/italia/onto/MU/value"/>
    <rdfs:domain rdf:resource="https://w3id.org/italia/onto/HER/USTATAverageContributionsAggregate"/>
    <rdfs:range rdf:resource="http://www.w3.org/2001/XMLSchema#decimal"/>
    <rdfs:comment xml:lang="en">Average contribution for students enrolled in degree courses, master's degree courses, courses of the old system calculated on the basis of the fees actually paid (net of the regional tax for the Right to University Studies - DSU and stamp duty where applicable), EXCLUDED students totally exempted, students for whom the contribution is not expected or is financed by external bodies. The values are expressed in EURO. The average is calculated considering the central point of each contribution class.</rdfs:comment>
    <rdfs:comment xml:lang="it">Contribuzione media per gli studenti iscritti a corsi di laurea, corsi di laurea magistrale, corsi del vecchio ordinamento calcolata sulla base delle tasse realmente pagate (al netto della tassa regionale per il Diritto allo Studio Universitario - DSU e dell’imposta di bollo dove previste), ESCLUSI gli studenti esonerati totalmente, gli studenti per i quali la contribuzione non è prevista o è finanziata da enti esterni. I valori sono espressi in EURO. La media è calcolata considerando il punto centrale di ciascuna classe di contribuzione.
</rdfs:comment>
    <rdfs:isDefinedBy rdf:resource="https://w3id.org/italia/onto/HER"/>
    <rdfs:label xml:lang="en">average taxes for paying students</rdfs:label>
    <rdfs:label xml:lang="it">spesa media delle tasse per pagare gli studenti</rdfs:label>
    <owl:versionInfo xml:lang="it">provvisoria - controllare codominio</owl:versionInfo>
    <owl:versionInfo xml:lang="en">unstable - check range</owl:versionInfo>
  </rdf:Description>
  <rdf:Description rdf:nodeID="n5bb3bff42afb4ca286d2c3fead9507ddb132">
    <rdf:type rdf:resource="http://www.w3.org/2000/01/rdf-schema#Datatype"/>
    <owl:oneOf rdf:nodeID="n5bb3bff42afb4ca286d2c3fead9507ddb133"/>
  </rdf:Description>
  <rdf:Description rdf:about="https://w3id.org/italia/onto/HER/aactPopulation">
    <rdf:type rdf:resource="http://www.w3.org/2002/07/owl#DatatypeProperty"/>
    <rdfs:domain rdf:resource="https://w3id.org/italia/onto/HER/AACTEligibility"/>
    <rdfs:range rdf:resource="http://www.w3.org/2000/01/rdf-schema#Literal"/>
    <rdfs:comment xml:lang="en">A description of the population from which the groups or cohorts will be selected (for example, primary care clinic, community sample, residents of a certain town).</rdfs:comment>
    <rdfs:comment xml:lang="it">Una descrizione della popolazione da cui saranno selezionati i gruppi (ad esempio, clinica di assistenza primaria, campione della comunità, residenti di una certa città).</rdfs:comment>
    <rdfs:isDefinedBy rdf:resource="https://w3id.org/italia/onto/HER"/>
    <rdfs:label xml:lang="en">AACT population</rdfs:label>
    <rdfs:label xml:lang="it">popolazione AACT</rdfs:label>
    <owl:versionInfo xml:lang="it">stabile</owl:versionInfo>
    <owl:versionInfo xml:lang="en">stable</owl:versionInfo>
  </rdf:Description>
  <rdf:Description rdf:nodeID="n5bb3bff42afb4ca286d2c3fead9507ddb303">
    <rdf:type rdf:resource="http://www.w3.org/2002/07/owl#Class"/>
    <owl:unionOf rdf:nodeID="n5bb3bff42afb4ca286d2c3fead9507ddb304"/>
  </rdf:Description>
  <rdf:Description rdf:about="https://w3id.org/italia/onto/HER/ctnprinOperationIdentifier">
    <rdf:type rdf:resource="http://www.w3.org/2002/07/owl#DatatypeProperty"/>
    <rdfs:subPropertyOf rdf:resource="https://w3id.org/italia/onto/l0/identifier"/>
    <rdfs:domain rdf:resource="https://w3id.org/italia/onto/HER/CTNPRINOperation"/>
    <rdfs:range rdf:resource="http://www.w3.org/2000/01/rdf-schema#Literal"/>
    <rdfs:comment xml:lang="it">ID univoco di una operazione.
E' ottenuto concatenando le seguenti variabili all'origine:
Codice locale progetto +  ambito + CF beneficiario
corrispondenti a: projectCode + scope_operations + fiscalcode_entity</rdfs:comment>
    <rdfs:comment xml:lang="en">Unique ID of an operation.
It is obtained by concatenating the following variables at the origin: "Codice locale progetto +  ambito + CF beneficiario"  corresponding to: projectCode + scope_operations + fiscalcode_entity</rdfs:comment>
    <rdfs:isDefinedBy rdf:resource="https://w3id.org/italia/onto/HER"/>
    <rdfs:label xml:lang="en">CTN/PRIN operation identifier</rdfs:label>
    <rdfs:label xml:lang="it">identificatore operazione CTN/PRIN</rdfs:label>
    <owl:versionInfo xml:lang="it">stabile</owl:versionInfo>
    <owl:versionInfo xml:lang="en">stable</owl:versionInfo>
  </rdf:Description>
  <rdf:Description rdf:nodeID="n5bb3bff42afb4ca286d2c3fead9507ddb519">
    <rdf:type rdf:resource="http://www.w3.org/2002/07/owl#Restriction"/>
    <owl:onProperty rdf:resource="https://w3id.org/italia/onto/HER/additionalInfo"/>
    <owl:allValuesFrom rdf:resource="http://www.w3.org/2000/01/rdf-schema#Literal"/>
  </rdf:Description>
  <rdf:Description rdf:nodeID="n5bb3bff42afb4ca286d2c3fead9507ddb498">
    <rdf:type rdf:resource="http://www.w3.org/2002/07/owl#Restriction"/>
    <owl:onProperty rdf:resource="https://w3id.org/italia/onto/HER/hasPatentPriorityDetail"/>
    <owl:someValuesFrom rdf:resource="https://w3id.org/italia/onto/HER/PatentPriorityDetail"/>
  </rdf:Description>
  <rdf:Description rdf:nodeID="n5bb3bff42afb4ca286d2c3fead9507ddb419">
    <rdf:type rdf:resource="http://www.w3.org/2002/07/owl#Restriction"/>
    <owl:onProperty rdf:resource="https://w3id.org/italia/onto/HER/documentationURL"/>
    <owl:qualifiedCardinality rdf:datatype="http://www.w3.org/2001/XMLSchema#nonNegativeInteger">1</owl:qualifiedCardinality>
    <owl:onDataRange rdf:resource="http://www.w3.org/2001/XMLSchema#anyURI"/>
  </rdf:Description>
  <rdf:Description rdf:about="https://w3id.org/italia/onto/HER/PatentPublicationStage">
    <rdf:type rdf:resource="http://www.w3.org/2002/07/owl#Class"/>
    <rdfs:subClassOf rdf:resource="https://w3id.org/italia/onto/l0/Object"/>
    <rdfs:subClassOf rdf:nodeID="n5bb3bff42afb4ca286d2c3fead9507ddb508"/>
    <rdfs:comment xml:lang="it">La fase in cui è attualmente in corso il processo di pubblicazione dei brevetti.</rdfs:comment>
    <rdfs:comment xml:lang="en">The stage in which the patent publication process is currently on.</rdfs:comment>
    <rdfs:isDefinedBy rdf:resource="https://w3id.org/italia/onto/HER"/>
    <rdfs:label xml:lang="it">Fase di pubblicazione del brevetto</rdfs:label>
    <rdfs:label xml:lang="en">Patent Publication Stage</rdfs:label>
    <owl:versionInfo xml:lang="it">stabile</owl:versionInfo>
    <owl:versionInfo xml:lang="en">stable</owl:versionInfo>
  </rdf:Description>
  <rdf:Description rdf:nodeID="n5bb3bff42afb4ca286d2c3fead9507ddb251">
    <rdf:type rdf:resource="http://www.w3.org/1999/02/22-rdf-syntax-ns#List"/>
    <rdf:first>No</rdf:first>
    <rdf:rest rdf:nodeID="n5bb3bff42afb4ca286d2c3fead9507ddb252"/>
  </rdf:Description>
  <rdf:Description rdf:about="https://w3id.org/italia/onto/HER/DSUInterventionType">
    <rdf:type rdf:resource="http://www.w3.org/2002/07/owl#Class"/>
    <rdfs:subClassOf rdf:resource="https://w3id.org/italia/onto/l0/Characteristic"/>
    <rdfs:subClassOf rdf:nodeID="n5bb3bff42afb4ca286d2c3fead9507ddb436"/>
    <rdfs:subClassOf rdf:nodeID="n5bb3bff42afb4ca286d2c3fead9507ddb437"/>
    <rdfs:comment xml:lang="en">Information (code and description) on interventions in favor of students for the Academic Year (T-1)/(T).</rdfs:comment>
    <rdfs:comment xml:lang="it">Informazioni (codice e descrizione) sugli interventi a favore degli studenti per l'Anno Accademico (T-1)/(T)</rdfs:comment>
    <rdfs:isDefinedBy rdf:resource="https://w3id.org/italia/onto/HER"/>
    <rdfs:label xml:lang="en">DSU Intervention Type</rdfs:label>
    <rdfs:label xml:lang="it">Tipo (o classe) di intervento DSU</rdfs:label>
    <owl:versionInfo xml:lang="it">stabile</owl:versionInfo>
    <owl:versionInfo xml:lang="en">stable</owl:versionInfo>
  </rdf:Description>
  <rdf:Description rdf:nodeID="n5bb3bff42afb4ca286d2c3fead9507ddb80">
    <rdf:first rdf:resource="https://w3id.org/italia/onto/HER/ErasmusPlusParticipant"/>
    <rdf:rest rdf:resource="http://www.w3.org/1999/02/22-rdf-syntax-ns#nil"/>
  </rdf:Description>
  <rdf:Description rdf:about="https://w3id.org/italia/onto/HER/patentPriorityDate">
    <rdf:type rdf:resource="http://www.w3.org/2002/07/owl#DatatypeProperty"/>
    <rdfs:subPropertyOf rdf:resource="https://w3id.org/italia/onto/TI/date"/>
    <rdfs:domain rdf:resource="https://w3id.org/italia/onto/HER/PatentPriorityDetail"/>
    <rdfs:range rdf:resource="http://www.w3.org/2001/XMLSchema#date"/>
    <rdfs:comment xml:lang="it">La data di priorità della domanda di brevetto, corrispondente alla data del primo deposito della domanda</rdfs:comment>
    <rdfs:comment xml:lang="en">The priority date of the patent application, corresponding to the date of the first application filing</rdfs:comment>
    <rdfs:isDefinedBy rdf:resource="https://w3id.org/italia/onto/HER"/>
    <rdfs:label xml:lang="it">date prioritá</rdfs:label>
    <rdfs:label xml:lang="en">priority date</rdfs:label>
    <owl:versionInfo xml:lang="it">stabile</owl:versionInfo>
    <owl:versionInfo xml:lang="en">stable</owl:versionInfo>
  </rdf:Description>
  <rdf:Description rdf:nodeID="n5bb3bff42afb4ca286d2c3fead9507ddb377">
    <rdf:type rdf:resource="http://www.w3.org/2002/07/owl#Restriction"/>
    <owl:onProperty rdf:resource="https://w3id.org/italia/onto/COV/hasOrganization"/>
    <owl:someValuesFrom rdf:resource="https://w3id.org/italia/onto/COV/Organization"/>
  </rdf:Description>
  <rdf:Description rdf:nodeID="n5bb3bff42afb4ca286d2c3fead9507ddb318">
    <rdf:first rdf:resource="https://w3id.org/italia/onto/HER/USTATInterventionExpensesAggregate"/>
    <rdf:rest rdf:nodeID="n5bb3bff42afb4ca286d2c3fead9507ddb319"/>
  </rdf:Description>
  <rdf:Description rdf:nodeID="n5bb3bff42afb4ca286d2c3fead9507ddb371">
    <rdf:type rdf:resource="http://www.w3.org/2002/07/owl#Restriction"/>
    <owl:onProperty rdf:resource="https://w3id.org/italia/onto/HER/allocation"/>
    <owl:maxCardinality rdf:datatype="http://www.w3.org/2001/XMLSchema#nonNegativeInteger">1</owl:maxCardinality>
  </rdf:Description>
  <rdf:Description rdf:about="https://w3id.org/italia/onto/HER/hasECParticipant">
    <rdf:type rdf:resource="http://www.w3.org/2002/07/owl#ObjectProperty"/>
    <rdfs:subPropertyOf rdf:resource="https://w3id.org/italia/onto/RO/hasRiT"/>
    <rdfs:domain rdf:nodeID="n5bb3bff42afb4ca286d2c3fead9507ddb44"/>
    <rdfs:range rdf:resource="https://w3id.org/italia/onto/HER/ECParticipant"/>
    <rdfs:comment xml:lang="it">Questa proprietà collega un progetto CE con uno dei suoi partecipanti.</rdfs:comment>
    <rdfs:comment xml:lang="en">This property connects an EC project with one of its participants.</rdfs:comment>
    <rdfs:isDefinedBy rdf:resource="https://w3id.org/italia/onto/HER"/>
    <rdfs:label xml:lang="it">ha partecipante CE</rdfs:label>
    <rdfs:label xml:lang="en">has EC participant</rdfs:label>
    <owl:versionInfo xml:lang="it">stabile</owl:versionInfo>
    <owl:versionInfo xml:lang="en">stable</owl:versionInfo>
  </rdf:Description>
  <rdf:Description rdf:about="https://w3id.org/italia/onto/HER/PUB">
    <rdf:type rdf:resource="http://www.w3.org/2002/07/owl#NamedIndividual"/>
    <rdf:type rdf:resource="https://w3id.org/italia/onto/HER/ECActivityType"/>
    <rdfs:isDefinedBy rdf:resource="https://w3id.org/italia/onto/HER"/>
    <rdfs:label xml:lang="en">Public bodies (excluding Research Organisations and Secondary or Higher Education Establishments)</rdfs:label>
    <owl:versionInfo xml:lang="it">stabile</owl:versionInfo>
    <owl:versionInfo xml:lang="en">stable</owl:versionInfo>
  </rdf:Description>
  <rdf:Description rdf:about="https://w3id.org/italia/onto/HER/isProducedBy">
    <rdf:type rdf:resource="http://www.w3.org/2002/07/owl#ObjectProperty"/>
    <owl:inverseOf rdf:resource="https://w3id.org/italia/onto/HER/producesPatent"/>
    <rdfs:domain rdf:resource="https://w3id.org/italia/onto/HER/Patent"/>
    <rdfs:range rdf:resource="https://w3id.org/italia/onto/COV/Organization"/>
    <rdfs:comment xml:lang="it">Questa proprietà collega un brevetto con l'organizzazione che lo produce</rdfs:comment>
    <rdfs:comment xml:lang="en">This property connects a patent with the organization that produces it</rdfs:comment>
    <rdfs:isDefinedBy rdf:resource="https://w3id.org/italia/onto/HER"/>
    <rdfs:label xml:lang="it">brevetto prodotto da</rdfs:label>
    <rdfs:label xml:lang="en">patent is produced by</rdfs:label>
    <owl:versionInfo xml:lang="it">stabile</owl:versionInfo>
    <owl:versionInfo xml:lang="en">stable</owl:versionInfo>
  </rdf:Description>
  <rdf:Description rdf:about="https://w3id.org/italia/onto/HER/hasErasmusplusTopic">
    <rdf:type rdf:resource="http://www.w3.org/2002/07/owl#ObjectProperty"/>
    <rdfs:subPropertyOf rdf:resource="https://w3id.org/italia/onto/l0/hasTopic"/>
    <rdfs:domain rdf:resource="https://w3id.org/italia/onto/HER/ErasmusPlusProject"/>
    <rdfs:range rdf:resource="https://w3id.org/italia/onto/HER/ErasmusPlusTopic"/>
    <rdfs:comment xml:lang="en">It is used to link Erasmus+ projects to Topics.</rdfs:comment>
    <rdfs:comment xml:lang="it">Viene utilizzato per collegare i progetti Erasmus+ agli argomenti.</rdfs:comment>
    <rdfs:isDefinedBy rdf:resource="https://w3id.org/italia/onto/HER"/>
    <rdfs:label xml:lang="it">ha argomento Erasmus+</rdfs:label>
    <rdfs:label xml:lang="en">has Erasmus+ topic</rdfs:label>
    <owl:versionInfo xml:lang="it">stabile</owl:versionInfo>
    <owl:versionInfo xml:lang="en">stable</owl:versionInfo>
  </rdf:Description>
  <rdf:Description rdf:about="https://w3id.org/italia/onto/HER/subjectMasked">
    <rdf:type rdf:resource="http://www.w3.org/2002/07/owl#DatatypeProperty"/>
    <rdf:type rdf:resource="http://www.w3.org/2002/07/owl#FunctionalProperty"/>
    <rdfs:domain rdf:resource="https://w3id.org/italia/onto/HER/AACTDesign"/>
    <rdfs:range rdf:resource="http://www.w3.org/2001/XMLSchema#boolean"/>
    <rdfs:comment xml:lang="it">L'obiettivo principale degli interventi che vengono valutati dallo studio clinico. Gli scopi primari sono:
Trattamento: Uno o più interventi sono in fase di valutazione per il trattamento di una malattia, sindrome o condizione.
Prevenzione: Uno o più interventi sono in fase di valutazione per prevenire lo sviluppo di una specifica malattia o condizione di salute.
Diagnostica: Si stanno valutando uno o più interventi per identificare una malattia o una condizione di salute.
Cure di supporto: Uno o più interventi sono valutati per massimizzare il comfort, ridurre al minimo gli effetti collaterali o mitigare il declino della salute o della funzione del partecipante.
Screening: Uno o più interventi sono valutati o esaminati per identificare una condizione, o fattori di rischio per una condizione, in persone che non sono ancora note per avere la condizione o il fattore di rischio.
Ricerca sui servizi sanitari: Uno o più interventi per valutare la fornitura, i processi, la gestione, l'organizzazione o il finanziamento dell'assistenza sanitaria.
Scienza di base: Uno o più interventi per esaminare il meccanismo di base dell'azione (per esempio, la fisiologia o la biomeccanica di un intervento).
Fattibilità del dispositivo: Un intervento di un dispositivo viene valutato in un piccolo trial clinico (generalmente meno di 10 partecipanti) per determinare la fattibilità del prodotto; o un trial clinico per testare un prototipo di dispositivo per verificarne la fattibilità e non gli esiti sanitari. Tali studi sono condotti per confermare la progettazione e le specifiche operative di un dispositivo prima di iniziare una sperimentazione clinica completa.
Altro: Non si applica nessuna delle altre opzioni.</rdfs:comment>
    <rdfs:comment xml:lang="en">Subject is the party or parties involved in the clinical trial who are prevented from having knowledge of the interventions assigned to individual participants.</rdfs:comment>
    <rdfs:isDefinedBy rdf:resource="https://w3id.org/italia/onto/HER"/>
    <rdfs:label xml:lang="en">is subject masked?</rdfs:label>
    <owl:versionInfo xml:lang="it">stabile</owl:versionInfo>
    <owl:versionInfo xml:lang="en">stable</owl:versionInfo>
  </rdf:Description>
  <rdf:Description rdf:nodeID="n5bb3bff42afb4ca286d2c3fead9507ddb39">
    <rdf:first rdf:resource="https://w3id.org/italia/onto/HER/MIURStudentsByDiplomaAggregate"/>
    <rdf:rest rdf:nodeID="n5bb3bff42afb4ca286d2c3fead9507ddb40"/>
  </rdf:Description>
  <rdf:Description rdf:nodeID="n5bb3bff42afb4ca286d2c3fead9507ddb152">
    <rdf:type rdf:resource="http://www.w3.org/2000/01/rdf-schema#Datatype"/>
    <owl:oneOf rdf:nodeID="n5bb3bff42afb4ca286d2c3fead9507ddb153"/>
  </rdf:Description>
  <rdf:Description rdf:about="https://w3id.org/italia/onto/HER/hasDiploma">
    <rdf:type rdf:resource="http://www.w3.org/2002/07/owl#ObjectProperty"/>
    <rdfs:domain rdf:nodeID="n5bb3bff42afb4ca286d2c3fead9507ddb38"/>
    <rdfs:range rdf:resource="https://w3id.org/italia/onto/HER/Diploma"/>
    <rdfs:comment xml:lang="it">Questa proprietà si collega a un diploma accademico.</rdfs:comment>
    <rdfs:comment xml:lang="en">This property links to an academic diploma.</rdfs:comment>
    <rdfs:isDefinedBy rdf:resource="https://w3id.org/italia/onto/HER"/>
    <rdfs:label xml:lang="it">ha  diploma</rdfs:label>
    <rdfs:label xml:lang="en">has diploma</rdfs:label>
    <owl:versionInfo xml:lang="it">stabile</owl:versionInfo>
    <owl:versionInfo xml:lang="en">stable</owl:versionInfo>
  </rdf:Description>
  <rdf:Description rdf:nodeID="n5bb3bff42afb4ca286d2c3fead9507ddb485">
    <rdf:type rdf:resource="http://www.w3.org/2002/07/owl#Restriction"/>
    <owl:onProperty rdf:resource="https://w3id.org/italia/onto/HER/hasEndingDate"/>
    <owl:qualifiedCardinality rdf:datatype="http://www.w3.org/2001/XMLSchema#nonNegativeInteger">1</owl:qualifiedCardinality>
    <owl:onClass rdf:resource="https://w3id.org/italia/onto/TI/TimeInstant"/>
  </rdf:Description>
  <rdf:Description rdf:about="https://w3id.org/italia/onto/HER/hasERCGrantType">
    <rdf:type rdf:resource="http://www.w3.org/2002/07/owl#ObjectProperty"/>
    <rdfs:domain rdf:nodeID="n5bb3bff42afb4ca286d2c3fead9507ddb50"/>
    <rdfs:range rdf:resource="https://w3id.org/italia/onto/HER/ERCGrantType"/>
    <rdfs:comment xml:lang="it">Questa proprietà collega un progetto del CER con il tipo di sovvenzione corrispondente.</rdfs:comment>
    <rdfs:comment xml:lang="en">This property connects an EC or ERC project with the corresponding type of grant.</rdfs:comment>
    <rdfs:isDefinedBy rdf:resource="https://w3id.org/italia/onto/HER"/>
    <rdfs:label xml:lang="it">ha tipo contributo ERC</rdfs:label>
    <rdfs:label xml:lang="en">has ERC grant type</rdfs:label>
    <owl:versionInfo xml:lang="it">stabile</owl:versionInfo>
    <owl:versionInfo xml:lang="en">stable</owl:versionInfo>
  </rdf:Description>
  <rdf:Description rdf:about="https://w3id.org/italia/onto/HER/CTNPRINInitiative">
    <rdf:type rdf:resource="http://www.w3.org/2002/07/owl#Class"/>
    <rdfs:subClassOf rdf:resource="https://w3id.org/italia/onto/l0/Activity"/>
    <rdfs:subClassOf rdf:nodeID="n5bb3bff42afb4ca286d2c3fead9507ddb417"/>
    <rdfs:subClassOf rdf:nodeID="n5bb3bff42afb4ca286d2c3fead9507ddb418"/>
    <rdfs:subClassOf rdf:nodeID="n5bb3bff42afb4ca286d2c3fead9507ddb419"/>
    <rdfs:subClassOf rdf:nodeID="n5bb3bff42afb4ca286d2c3fead9507ddb420"/>
    <rdfs:subClassOf rdf:nodeID="n5bb3bff42afb4ca286d2c3fead9507ddb421"/>
    <rdfs:comment xml:lang="en">An initiative in this context is a funding action that can be associated with a call, a notice, an invitation, a campaign, etc. The data integrated in ToscanaOpenResearch have been obtained in the context of a memorandum of understanding between the Ministry of Education, University and Research and the Tuscan Region, and are related to the initiatives CTN2012, CTN20916 and PRIN 2012, and to projects with at least one beneficiary with legal or operational headquarters in Tuscany.</rdfs:comment>
    <rdfs:comment xml:lang="it">Un'iniziativa in questo contesto è un'azione di finanziamento che può essere associata ad un bando, un avviso, un invito, una campagna, etc. I dati integrati in ToscanaOpenResearch sono stati ottenuti nel contesto di un protocollo di intesa tra il Ministero dell'Istruzione, dell'Università e della Ricerca e la Regione toscana, e sono relativi alle iniziative CTN2012, CTN20916 e PRIN 2012, e a progetti aventi almeno un beneficiario con sede legale o operativa in Toscana.</rdfs:comment>
    <rdfs:isDefinedBy rdf:resource="https://w3id.org/italia/onto/HER"/>
    <rdfs:label xml:lang="en">CTN/PRIN Initiative</rdfs:label>
    <rdfs:label xml:lang="it">iniziativa CTN/PRIN</rdfs:label>
    <owl:versionInfo xml:lang="it">stabile</owl:versionInfo>
    <owl:versionInfo xml:lang="en">stable</owl:versionInfo>
  </rdf:Description>
  <rdf:Description rdf:about="https://w3id.org/italia/onto/HER/hasOperation">
    <rdf:type rdf:resource="http://www.w3.org/2002/07/owl#ObjectProperty"/>
    <rdfs:domain rdf:nodeID="n5bb3bff42afb4ca286d2c3fead9507ddb73"/>
    <rdfs:range rdf:resource="https://w3id.org/italia/onto/HER/CTNPRINOperation"/>
    <rdfs:comment xml:lang="it">Identifica un'operazione contabile. Si veda la proprietà "operationIdentifier" per informazioni sulla definizione.</rdfs:comment>
    <rdfs:comment xml:lang="en">Identifies an accounting transaction. See the "operationIdentifier" property for definition information.</rdfs:comment>
    <rdfs:isDefinedBy rdf:resource="https://w3id.org/italia/onto/HER"/>
    <rdfs:label xml:lang="it">ha operazione CTN/PRIN</rdfs:label>
    <rdfs:label xml:lang="en">has CTN/PRIN operation</rdfs:label>
    <owl:versionInfo xml:lang="it">stabile</owl:versionInfo>
    <owl:versionInfo xml:lang="en">stable</owl:versionInfo>
  </rdf:Description>
  <rdf:Description rdf:nodeID="n5bb3bff42afb4ca286d2c3fead9507ddb15">
    <rdf:first rdf:resource="https://w3id.org/italia/onto/HER/MIURStudentsByDiplomaDegreeDegreeClassAggregate"/>
    <rdf:rest rdf:nodeID="n5bb3bff42afb4ca286d2c3fead9507ddb16"/>
  </rdf:Description>
  <rdf:Description rdf:nodeID="n5bb3bff42afb4ca286d2c3fead9507ddb6">
    <rdf:first rdf:resource="https://w3id.org/italia/onto/HER/AACTDesign"/>
    <rdf:rest rdf:nodeID="n5bb3bff42afb4ca286d2c3fead9507ddb7"/>
  </rdf:Description>
  <rdf:Description rdf:about="https://w3id.org/italia/onto/HER/MIURStudentsByRegionOfResidenceAggregate">
    <rdf:type rdf:resource="http://www.w3.org/2002/07/owl#Class"/>
    <rdfs:subClassOf rdf:resource="https://w3id.org/italia/onto/HER/StatisticalDataAggregation"/>
    <rdfs:subClassOf rdf:nodeID="n5bb3bff42afb4ca286d2c3fead9507ddb496"/>
    <rdfs:comment xml:lang="en">Aggregated data on Italian students filed in the MIUR system, grouped by year, university and Italian region of residence.</rdfs:comment>
    <rdfs:comment xml:lang="it">Dati aggregati sugli studenti italiani archiviati nel sistema MIUR, raggruppati per anno, università e regione di residenza italiana.</rdfs:comment>
    <rdfs:isDefinedBy rdf:resource="https://w3id.org/italia/onto/HER"/>
    <rdfs:label xml:lang="en">Aggregate of Italian Students By Region of Residence</rdfs:label>
    <rdfs:label xml:lang="it">Aggregazione dei studenti italiani per regione di residenza</rdfs:label>
    <owl:versionInfo xml:lang="it">stabile</owl:versionInfo>
    <owl:versionInfo xml:lang="en">stable</owl:versionInfo>
  </rdf:Description>
  <rdf:Description rdf:nodeID="n5bb3bff42afb4ca286d2c3fead9507ddb543">
    <rdf:type rdf:resource="http://www.w3.org/2002/07/owl#Restriction"/>
    <owl:onProperty rdf:resource="https://w3id.org/italia/onto/COV/hasOrganization"/>
    <owl:maxQualifiedCardinality rdf:datatype="http://www.w3.org/2001/XMLSchema#nonNegativeInteger">1</owl:maxQualifiedCardinality>
    <owl:onClass rdf:resource="https://w3id.org/italia/onto/COV/Organization"/>
  </rdf:Description>
  <rdf:Description rdf:about="https://w3id.org/italia/onto/HER/hasEndingDate">
    <rdf:type rdf:resource="http://www.w3.org/2002/07/owl#ObjectProperty"/>
    <rdfs:subPropertyOf rdf:resource="https://w3id.org/italia/onto/TI/hasTemporalEntity"/>
    <rdfs:domain rdf:resource="https://w3id.org/italia/onto/HER/ErasmusPlusProject"/>
    <rdfs:range rdf:resource="https://w3id.org/italia/onto/TI#TimeInstant"/>
    <rdfs:comment xml:lang="it">La proprietà rappresenta la data di fine</rdfs:comment>
    <rdfs:comment xml:lang="en">The property represents the date of ending</rdfs:comment>
    <rdfs:isDefinedBy rdf:resource="https://w3id.org/italia/onto/HER"/>
    <rdfs:label xml:lang="it">ha data di fine</rdfs:label>
    <rdfs:label xml:lang="en">has ending date</rdfs:label>
    <owl:versionInfo xml:lang="it">stabile</owl:versionInfo>
    <owl:versionInfo xml:lang="en">stable</owl:versionInfo>
  </rdf:Description>
  <rdf:Description rdf:nodeID="n5bb3bff42afb4ca286d2c3fead9507ddb328">
    <rdf:type rdf:resource="http://www.w3.org/2002/07/owl#Class"/>
    <owl:unionOf rdf:nodeID="n5bb3bff42afb4ca286d2c3fead9507ddb329"/>
  </rdf:Description>
  <rdf:Description rdf:nodeID="n5bb3bff42afb4ca286d2c3fead9507ddb319">
    <rdf:first rdf:resource="https://w3id.org/italia/onto/HER/USTATInterventionsForStudentsByUniversitiesAggregate"/>
    <rdf:rest rdf:nodeID="n5bb3bff42afb4ca286d2c3fead9507ddb320"/>
  </rdf:Description>
  <rdf:Description rdf:about="https://w3id.org/italia/onto/HER/USTATPostgraduateAggregateOfRegistered">
    <rdf:type rdf:resource="http://www.w3.org/2002/07/owl#Class"/>
    <rdfs:subClassOf rdf:resource="https://w3id.org/italia/onto/HER/StatisticalDataAggregation"/>
    <rdfs:subClassOf rdf:nodeID="n5bb3bff42afb4ca286d2c3fead9507ddb535"/>
    <rdfs:comment xml:lang="it">A partire dal XXXI ciclo, i dati sono desunti dall'Anagrafe Nazionale degli Studenti universitari: in questo caso, l'informazione riportata è relativa agli studenti iscritti per ciclo al primo anno del dottorato di ricerca. Fino al XXX ciclo incluso, la fonte dei dati è la "Rilevazione sull'Istruzione Universititaria", e l'informazione riportata è relativa al numero di studenti vincitori di concorso, a prescindere dal fatto che si siano in seguito iscritti. Fonte dell'informazione: Informazioni sui file relativi ai Dottorati di Ricerca, sito USTAT-MIUR (http://dati.ustat.miur.it/dataset/formazione-post-laurea/resource/fdee4043-0011-43ef-9f44-ef00e484f0d8) e comunciazione dell'Ufficio di Statistica e Studi - settore Università e Ricerca.</rdfs:comment>
    <rdfs:comment xml:lang="en">Starting from the XXXI cycle, the data are derived from the National Register of University Students: in this case, the information reported is related to students enrolled per cycle in the first year of the PhD. Up to and including the XXXth cycle, the data source is the "Universities Education Survey", and the information reported is related to the number of students who have won the exam, regardless of whether they have subsequently enrolled. Source of information: Information on PhD files, USTAT-MIUR website (http://dati.ustat.miur.it/dataset/formazione-post-laurea/resource/fdee4043-0011-43ef-9f44-ef00e484f0d8) and communication from the Office of Statistics and Studies - University and Research sector.</rdfs:comment>
    <rdfs:isDefinedBy rdf:resource="https://w3id.org/italia/onto/HER"/>
    <rdfs:label xml:lang="it">Aggregazione USTAT Postgraduate - Accessi</rdfs:label>
    <rdfs:label xml:lang="en">USTAT Postgraduate Aggregate of Registered</rdfs:label>
    <owl:versionInfo xml:lang="it">stabile</owl:versionInfo>
    <owl:versionInfo xml:lang="en">stable</owl:versionInfo>
  </rdf:Description>
  <rdf:Description rdf:about="https://w3id.org/italia/onto/HER/decreeDate">
    <rdf:type rdf:resource="http://www.w3.org/2002/07/owl#DatatypeProperty"/>
    <rdfs:subPropertyOf rdf:resource="https://w3id.org/italia/onto/TI/date"/>
    <rdfs:domain rdf:resource="https://w3id.org/italia/onto/HER/CTNPRINInitiative"/>
    <rdfs:range rdf:resource="http://www.w3.org/2001/XMLSchema#date"/>
    <rdfs:comment xml:lang="it">Data di emissione del decreto MIUR (Ministero dell'Istruzione, dell'Università e della Ricerca) in cui è pubblicato il bando/avviso che definisce originariamente l'iniziativa in esame</rdfs:comment>
    <rdfs:comment xml:lang="en">Date of issue of the MIUR (Ministry of Education, University and Research) decree in which the call/notice originally defining the initiative in question is published</rdfs:comment>
    <rdfs:isDefinedBy rdf:resource="https://w3id.org/italia/onto/HER"/>
    <rdfs:label xml:lang="it">data decreto</rdfs:label>
    <rdfs:label xml:lang="en">decree date</rdfs:label>
    <owl:versionInfo xml:lang="it">stabile</owl:versionInfo>
    <owl:versionInfo xml:lang="en">stable</owl:versionInfo>
  </rdf:Description>
  <rdf:Description rdf:nodeID="n5bb3bff42afb4ca286d2c3fead9507ddb82">
    <rdf:first rdf:resource="https://w3id.org/italia/onto/HER/MIURStudentsByCitizenshipAggregate"/>
    <rdf:rest rdf:nodeID="n5bb3bff42afb4ca286d2c3fead9507ddb83"/>
  </rdf:Description>
  <rdf:Description rdf:about="https://w3id.org/italia/onto/HER/hasAACTIntervention">
    <rdf:type rdf:resource="http://www.w3.org/2002/07/owl#ObjectProperty"/>
    <rdfs:domain rdf:resource="https://w3id.org/italia/onto/HER/AACTStudy"/>
    <rdfs:range rdf:resource="https://w3id.org/italia/onto/HER/AACTIntervention"/>
    <rdfs:comment xml:lang="en">A process or action that is the focus of a clinical study. Interventions include drugs, medical devices, procedures, vaccines, and other products that are either investigational or already available. Interventions can also include noninvasive approaches, such as education or modifying diet and exercise.</rdfs:comment>
    <rdfs:comment xml:lang="it">Un processo o un'azione che è il fulcro di uno studio clinico. Gli interventi comprendono farmaci, dispositivi medici, procedure, vaccini e altri prodotti che sono in fase di sperimentazione o già disponibili. Gli interventi possono anche includere approcci non invasivi, come l'educazione o la modifica della dieta e dell'esercizio fisico.</rdfs:comment>
    <rdfs:isDefinedBy rdf:resource="https://w3id.org/italia/onto/HER"/>
    <rdfs:label xml:lang="it">ha intervento AACT</rdfs:label>
    <rdfs:label xml:lang="en">has AACT intervention</rdfs:label>
    <owl:versionInfo xml:lang="it">stabile</owl:versionInfo>
    <owl:versionInfo xml:lang="en">stable</owl:versionInfo>
  </rdf:Description>
  <rdf:Description rdf:about="https://w3id.org/italia/onto/HER/hasECTopic">
    <rdf:type rdf:resource="http://www.w3.org/2002/07/owl#ObjectProperty"/>
    <rdfs:subPropertyOf rdf:resource="https://w3id.org/italia/onto/l0/hasTopic"/>
    <rdfs:domain rdf:nodeID="n5bb3bff42afb4ca286d2c3fead9507ddb47"/>
    <rdfs:range rdf:resource="https://w3id.org/italia/onto/HER/ECTopic"/>
    <rdfs:comment xml:lang="it">Questa proprietà collega un progetto CE con l'argomento corrispondente all'interno del suo invito a presentare proposte.</rdfs:comment>
    <rdfs:comment xml:lang="en">This property connects an EC project with the corresponding topic within its call for proposals.</rdfs:comment>
    <rdfs:isDefinedBy rdf:resource="https://w3id.org/italia/onto/HER"/>
    <rdfs:label xml:lang="it">ha argomento CE</rdfs:label>
    <rdfs:label xml:lang="en">has EC topic</rdfs:label>
    <owl:versionInfo xml:lang="it">stabile</owl:versionInfo>
    <owl:versionInfo xml:lang="en">stable</owl:versionInfo>
  </rdf:Description>
  <rdf:Description rdf:about="https://w3id.org/italia/onto/HER/hasAcademicDiscipline">
    <rdf:type rdf:resource="http://www.w3.org/2002/07/owl#ObjectProperty"/>
    <rdfs:domain rdf:resource="http://www.w3.org/2002/07/owl#Thing"/>
    <rdfs:range rdf:resource="https://w3id.org/italia/onto/HER/AcademicDiscipline"/>
    <rdfs:comment xml:lang="it">Questa proprietà consente di collegare qualunque cosa del dominio a discipline accademiche (definite nell'ambito del relativo vocabolario controllato).</rdfs:comment>
    <rdfs:comment xml:lang="en">This property allows one to link any thing of the domain with the academic disciplines (defined in the context of the related controlled vocabulary).</rdfs:comment>
    <rdfs:isDefinedBy rdf:resource="https://w3id.org/italia/onto/HER"/>
    <rdfs:label xml:lang="it">ha discipline accademiche</rdfs:label>
    <rdfs:label xml:lang="en">has Academic Discipline</rdfs:label>
    <owl:versionInfo xml:lang="it">stabile</owl:versionInfo>
    <owl:versionInfo xml:lang="en">stable</owl:versionInfo>
  </rdf:Description>
  <rdf:Description rdf:about="https://w3id.org/italia/onto/HER/hasFORDClassification">
    <rdf:type rdf:resource="http://www.w3.org/2002/07/owl#ObjectProperty"/>
    <rdfs:subPropertyOf rdf:resource="https://w3id.org/italia/onto/l0/hasTopic"/>
    <rdfs:domain rdf:resource="https://w3id.org/italia/onto/HER/USTATStaffByGender"/>
    <rdfs:range rdf:resource="https://w3id.org/italia/onto/HER/FORDClassification"/>
    <rdfs:comment xml:lang="it">Questa proprietà si collega alla classificazione dei Campi di ricerca e sviluppo (FORD) dell'UNESCO.</rdfs:comment>
    <rdfs:comment xml:lang="en">This property links to the UNESCO's Fields of research and development (FORD) classification.</rdfs:comment>
    <rdfs:isDefinedBy rdf:resource="https://w3id.org/italia/onto/HER"/>
    <rdfs:label xml:lang="it">ha una classificazione FORD</rdfs:label>
    <rdfs:label xml:lang="en">has FORD classification</rdfs:label>
    <owl:versionInfo xml:lang="it">stabile</owl:versionInfo>
    <owl:versionInfo xml:lang="en">stable</owl:versionInfo>
  </rdf:Description>
  <rdf:Description rdf:nodeID="n5bb3bff42afb4ca286d2c3fead9507ddb107">
    <rdf:first rdf:resource="https://w3id.org/italia/onto/HER/DSURightToUniversityStudiesAggregate"/>
    <rdf:rest rdf:nodeID="n5bb3bff42afb4ca286d2c3fead9507ddb108"/>
  </rdf:Description>
  <rdf:Description rdf:about="https://w3id.org/italia/onto/HER/AACTMeshTerm">
    <rdf:type rdf:resource="http://www.w3.org/2002/07/owl#Class"/>
    <rdfs:subClassOf rdf:resource="https://w3id.org/italia/onto/l0/Concept"/>
    <rdfs:subClassOf rdf:nodeID="n5bb3bff42afb4ca286d2c3fead9507ddb378"/>
    <rdfs:subClassOf rdf:nodeID="n5bb3bff42afb4ca286d2c3fead9507ddb379"/>
    <rdfs:comment xml:lang="en">descriptors from NLM's Medical Subject Headings (MeSH)-controlled vocabulary thesaurus</rdfs:comment>
    <rdfs:comment xml:lang="it">descrittori del thesaurus del vocabolario controllato dalla NLM "Medical Subject Headings (MeSH)" (MeSH)</rdfs:comment>
    <rdfs:isDefinedBy rdf:resource="https://w3id.org/italia/onto/HER"/>
    <rdfs:label xml:lang="en">Condition/Intervention Mesh Term</rdfs:label>
    <rdfs:label xml:lang="it">Termine Mesh di Condizione/Interventi</rdfs:label>
    <owl:versionInfo xml:lang="it">stabile</owl:versionInfo>
    <owl:versionInfo xml:lang="en">stable</owl:versionInfo>
    <ns6:wasDerivedFrom rdf:resource="http://www.w3.org/2004/02/skos/core#Concept"/>
  </rdf:Description>
  <rdf:Description rdf:about="https://w3id.org/italia/onto/HER/hasUSTATCateenService">
    <rdf:type rdf:resource="http://www.w3.org/2002/07/owl#ObjectProperty"/>
    <rdfs:domain rdf:resource="https://w3id.org/italia/onto/HER/DSUCanteenAndAccomodationsAggregate"/>
    <rdfs:range rdf:resource="https://w3id.org/italia/onto/HER/USTATCanteenServiceClass"/>
    <rdfs:comment xml:lang="it">Questa proprietà collega l'informazione sul totale dei serivizi disponibili alla tipologia di servizio corrispondente.</rdfs:comment>
    <rdfs:comment xml:lang="en">This property links the information on the total number of services available to the corresponding type of service.</rdfs:comment>
    <rdfs:isDefinedBy rdf:resource="https://w3id.org/italia/onto/HER"/>
    <rdfs:label xml:lang="it">ha una classe di servizio ustat</rdfs:label>
    <rdfs:label xml:lang="en">has ustat service class</rdfs:label>
    <owl:versionInfo xml:lang="it">stabile</owl:versionInfo>
    <owl:versionInfo xml:lang="en">stable</owl:versionInfo>
  </rdf:Description>
  <rdf:Description rdf:about="https://w3id.org/italia/onto/HER/hasErasmusplusKeyAction">
    <rdf:type rdf:resource="http://www.w3.org/2002/07/owl#ObjectProperty"/>
    <rdfs:domain rdf:resource="https://w3id.org/italia/onto/HER/ErasmusPlusProject"/>
    <rdfs:range rdf:resource="https://w3id.org/italia/onto/HER/ErasmusPlusKeyAction"/>
    <rdfs:comment xml:lang="en">It is used to link Erasmus+ projects to the key actions.</rdfs:comment>
    <rdfs:comment xml:lang="it">Viene utilizzato per collegare i progetti Erasmus+ alle azioni chiave.</rdfs:comment>
    <rdfs:isDefinedBy rdf:resource="https://w3id.org/italia/onto/HER"/>
    <rdfs:label xml:lang="it">ha azione chiave Erasmus+</rdfs:label>
    <rdfs:label xml:lang="en">has Erasmus+ key action</rdfs:label>
    <owl:versionInfo xml:lang="it">stabile</owl:versionInfo>
    <owl:versionInfo xml:lang="en">stable</owl:versionInfo>
  </rdf:Description>
  <rdf:Description rdf:about="https://w3id.org/italia/onto/HER/definedIn">
    <rdf:type rdf:resource="http://www.w3.org/2002/07/owl#ObjectProperty"/>
    <rdfs:domain rdf:resource="https://w3id.org/italia/onto/HER/AcademicAffiliation"/>
    <rdfs:range rdf:resource="https://w3id.org/italia/onto/COV/Organization"/>
    <rdfs:comment xml:lang="it">Collega l'affiliazione accademica con l'organizzazione corrispondente</rdfs:comment>
    <rdfs:comment xml:lang="en">Connects the academic affiliation with the corresponding organization</rdfs:comment>
    <rdfs:isDefinedBy rdf:resource="https://w3id.org/italia/onto/HER"/>
    <rdfs:label xml:lang="en">defined in</rdfs:label>
    <rdfs:label xml:lang="it">definito in</rdfs:label>
    <owl:versionInfo xml:lang="it">stabile</owl:versionInfo>
    <owl:versionInfo xml:lang="en">stable</owl:versionInfo>
  </rdf:Description>
  <rdf:Description rdf:about="https://w3id.org/italia/onto/HER/cordisRef">
    <rdf:type rdf:resource="http://www.w3.org/2002/07/owl#DatatypeProperty"/>
    <rdfs:subPropertyOf rdf:resource="https://w3id.org/italia/onto/l0/identifier"/>
    <rdfs:domain rdf:nodeID="n5bb3bff42afb4ca286d2c3fead9507ddb140"/>
    <rdfs:range rdf:resource="http://www.w3.org/2000/01/rdf-schema#Literal"/>
    <rdfs:comment xml:lang="it">Numero record di un progetto CE all'interno di CORDIS.</rdfs:comment>
    <rdfs:comment xml:lang="en">Record number of an EC project within CORDIS.</rdfs:comment>
    <rdfs:isDefinedBy rdf:resource="https://w3id.org/italia/onto/HER"/>
    <rdfs:label xml:lang="en">cordis reference number</rdfs:label>
    <rdfs:label xml:lang="it">numero di riferimento cordis</rdfs:label>
    <owl:versionInfo xml:lang="it">stabile</owl:versionInfo>
    <owl:versionInfo xml:lang="en">stable</owl:versionInfo>
  </rdf:Description>
  <rdf:Description rdf:nodeID="n5bb3bff42afb4ca286d2c3fead9507ddb19">
    <rdf:first rdf:resource="https://w3id.org/italia/onto/HER/ItalianPhDCourseByCycle"/>
    <rdf:rest rdf:nodeID="n5bb3bff42afb4ca286d2c3fead9507ddb20"/>
  </rdf:Description>
  <rdf:Description rdf:about="https://w3id.org/italia/onto/HER/USTATPartiallyExoneratedStudentsAggregate">
    <rdf:type rdf:resource="http://www.w3.org/2002/07/owl#Class"/>
    <rdfs:subClassOf rdf:resource="https://w3id.org/italia/onto/HER/StatisticalDataAggregation"/>
    <rdfs:subClassOf rdf:nodeID="n5bb3bff42afb4ca286d2c3fead9507ddb531"/>
    <rdfs:comment xml:lang="en">Data on students with partial exemption of universities.</rdfs:comment>
    <rdfs:comment xml:lang="it">Dati relativi agli studenti con esonero parziale degli atenei</rdfs:comment>
    <rdfs:isDefinedBy rdf:resource="https://w3id.org/italia/onto/HER"/>
    <rdfs:label xml:lang="it">Aggregazione degli studenti parzialmente esonerati riportati da USTAT</rdfs:label>
    <rdfs:label xml:lang="en">USTAT Aggregate of Partially Exonerated Students</rdfs:label>
    <owl:versionInfo xml:lang="it">stabile</owl:versionInfo>
    <owl:versionInfo xml:lang="en">stable</owl:versionInfo>
  </rdf:Description>
  <rdf:Description rdf:nodeID="n5bb3bff42afb4ca286d2c3fead9507ddb402">
    <rdf:type rdf:resource="http://www.w3.org/2002/07/owl#Restriction"/>
    <owl:onProperty rdf:resource="https://w3id.org/italia/onto/l0/name"/>
    <owl:someValuesFrom rdf:resource="http://www.w3.org/2000/01/rdf-schema#Literal"/>
  </rdf:Description>
  <rdf:Description rdf:nodeID="n5bb3bff42afb4ca286d2c3fead9507ddb240">
    <rdf:type rdf:resource="http://www.w3.org/1999/02/22-rdf-syntax-ns#List"/>
    <rdf:first>Ecologic or Community</rdf:first>
    <rdf:rest rdf:nodeID="n5bb3bff42afb4ca286d2c3fead9507ddb241"/>
  </rdf:Description>
  <rdf:Description rdf:nodeID="n5bb3bff42afb4ca286d2c3fead9507ddb502">
    <rdf:type rdf:resource="http://www.w3.org/2002/07/owl#Restriction"/>
    <owl:onProperty rdf:resource="https://w3id.org/italia/onto/HER/patentApplicationDate"/>
    <owl:maxQualifiedCardinality rdf:datatype="http://www.w3.org/2001/XMLSchema#nonNegativeInteger">1</owl:maxQualifiedCardinality>
    <owl:onDataRange rdf:resource="http://www.w3.org/2001/XMLSchema#date"/>
  </rdf:Description>
  <rdf:Description rdf:about="https://w3id.org/italia/onto/HER/hasCHAFEAOutput">
    <rdf:type rdf:resource="http://www.w3.org/2002/07/owl#ObjectProperty"/>
    <rdfs:subPropertyOf rdf:resource="https://w3id.org/italia/onto/HER/hasResult"/>
    <rdfs:domain rdf:resource="https://w3id.org/italia/onto/HER/CHAFEAProject"/>
    <rdfs:range rdf:resource="https://w3id.org/italia/onto/HER/CHAFEAOutput"/>
    <rdfs:comment xml:lang="it">Questa proprietà collega un'attività finanziata con uno dei suoi risultati.</rdfs:comment>
    <rdfs:comment xml:lang="en">This property connects a funded activity with one of its outputs.</rdfs:comment>
    <rdfs:isDefinedBy rdf:resource="https://w3id.org/italia/onto/HER"/>
    <rdfs:label xml:lang="it">ha risultato CHAFEA</rdfs:label>
    <rdfs:label xml:lang="en">has CHAFEA output</rdfs:label>
    <owl:versionInfo xml:lang="it">provvisoria</owl:versionInfo>
    <owl:versionInfo xml:lang="en">unstable</owl:versionInfo>
  </rdf:Description>
  <rdf:Description rdf:nodeID="n5bb3bff42afb4ca286d2c3fead9507ddb61">
    <rdf:type rdf:resource="http://www.w3.org/2002/07/owl#Class"/>
    <owl:unionOf rdf:nodeID="n5bb3bff42afb4ca286d2c3fead9507ddb62"/>
  </rdf:Description>
  <rdf:Description rdf:about="https://w3id.org/italia/onto/HER/ipdURL">
    <rdf:type rdf:resource="http://www.w3.org/2002/07/owl#DatatypeProperty"/>
    <rdfs:subPropertyOf rdf:resource="https://w3id.org/italia/onto/SM/URL"/>
    <rdfs:domain rdf:resource="https://w3id.org/italia/onto/HER/AACTStudy"/>
    <rdfs:range rdf:resource="http://www.w3.org/2001/XMLSchema#anyURI"/>
    <rdfs:comment xml:lang="it">L'indirizzo web, se presente, utilizzato per trovare ulteriori informazioni sul piano di condivisione di IPD.</rdfs:comment>
    <rdfs:comment xml:lang="en">The web address, if any, used to find additional information about the plan to share IPD.</rdfs:comment>
    <rdfs:isDefinedBy rdf:resource="https://w3id.org/italia/onto/HER"/>
    <rdfs:label xml:lang="en">IPD URL</rdfs:label>
    <rdfs:label xml:lang="it">IPD URL</rdfs:label>
    <owl:versionInfo xml:lang="it">stabile</owl:versionInfo>
    <owl:versionInfo xml:lang="en">stable</owl:versionInfo>
  </rdf:Description>
  <rdf:Description rdf:nodeID="n5bb3bff42afb4ca286d2c3fead9507ddb176">
    <rdf:type rdf:resource="http://www.w3.org/1999/02/22-rdf-syntax-ns#List"/>
    <rdf:first>Intermediate</rdf:first>
    <rdf:rest rdf:nodeID="n5bb3bff42afb4ca286d2c3fead9507ddb177"/>
  </rdf:Description>
  <rdf:Description rdf:about="https://w3id.org/italia/onto/HER/averageTaxForTotalEnrolledStudents">
    <rdf:type rdf:resource="http://www.w3.org/2002/07/owl#DatatypeProperty"/>
    <rdfs:subPropertyOf rdf:resource="https://w3id.org/italia/onto/MU/value"/>
    <rdfs:domain rdf:resource="https://w3id.org/italia/onto/HER/USTATAverageContributionsAggregate"/>
    <rdfs:range rdf:resource="http://www.w3.org/2001/XMLSchema#decimal"/>
    <rdfs:comment xml:lang="en">Average contribution for students enrolled in degree courses, master's degree courses, courses of the old system calculated on the basis of the fees actually paid (net of the regional tax for the Right to University Studies - DSU and stamp duty where applicable), INCLUDING students totally exempted, students for whom the contribution is not expected or is financed by external bodies. Values are expressed in EURO. The average is calculated considering the central point of each contribution class.</rdfs:comment>
    <rdfs:comment xml:lang="it">Contribuzione media per gli studenti iscritti a corsi di laurea, corsi di laurea magistrale, corsi del vecchio ordinamento calcolata sulla base delle tasse realmente pagate (al netto della tassa regionale per il DSU e dell’imposta di bollo dove previste), INCLUSI gli studenti esonerati totalmente, gli studenti per i quali la contribuzione non è prevista o è finanziata da enti esterni. I valori sono espressi in EURO. La media è calcolata considerando il punto centrale di ciascuna classe di contribuzione.</rdfs:comment>
    <rdfs:isDefinedBy rdf:resource="https://w3id.org/italia/onto/HER"/>
    <rdfs:label xml:lang="en">average taxes for total enrolled students</rdfs:label>
    <rdfs:label xml:lang="it">spesa media delle tasse per pagare tutti gli studenti iscritti</rdfs:label>
    <owl:versionInfo xml:lang="it">provvisoria - controllare codominio</owl:versionInfo>
    <owl:versionInfo xml:lang="en">unstable - check range</owl:versionInfo>
  </rdf:Description>
  <rdf:Description rdf:nodeID="n5bb3bff42afb4ca286d2c3fead9507ddb536">
    <rdf:type rdf:resource="http://www.w3.org/2002/07/owl#Restriction"/>
    <owl:onProperty rdf:resource="https://w3id.org/italia/onto/HER/ustatCourseType"/>
    <owl:maxCardinality rdf:datatype="http://www.w3.org/2001/XMLSchema#nonNegativeInteger">1</owl:maxCardinality>
  </rdf:Description>
  <rdf:Description rdf:about="https://w3id.org/italia/onto/HER/DSURightToUniversityStudiesAggregate">
    <rdf:type rdf:resource="http://www.w3.org/2002/07/owl#Class"/>
    <rdfs:subClassOf rdf:resource="https://w3id.org/italia/onto/HER/StatisticalDataAggregation"/>
    <rdfs:comment xml:lang="it">Interventi concessi a studenti per ciascun Ateneo/Istituto gestito da ciascun ente per il DSU/ufficio, per l'anno accademico di riferimento.</rdfs:comment>
    <rdfs:comment xml:lang="en">Interventions granted to students for each University/Institute managed by each institution for the Right to University Studies - DSU/Office, for the academic year of reference.</rdfs:comment>
    <rdfs:isDefinedBy rdf:resource="https://w3id.org/italia/onto/HER"/>
    <rdfs:label xml:lang="it">Aggregazione Diritto allo studio universitario riportato da USTAT</rdfs:label>
    <rdfs:label xml:lang="en">DSU Aggregate of Right to University Studies</rdfs:label>
    <owl:versionInfo xml:lang="it">stabile</owl:versionInfo>
    <owl:versionInfo xml:lang="en">stable</owl:versionInfo>
  </rdf:Description>
  <rdf:Description rdf:nodeID="n5bb3bff42afb4ca286d2c3fead9507ddb13">
    <rdf:first rdf:resource="https://w3id.org/italia/onto/HER/MIURStudentsByCitizenshipDegreeDegreeClassAggregate"/>
    <rdf:rest rdf:nodeID="n5bb3bff42afb4ca286d2c3fead9507ddb14"/>
  </rdf:Description>
  <rdf:Description rdf:about="https://w3id.org/italia/onto/HER/Italian">
    <rdf:type rdf:resource="http://www.w3.org/2002/07/owl#NamedIndividual"/>
    <rdf:type rdf:resource="https://w3id.org/italia/onto/HER/ReportedCitizenship"/>
    <rdfs:isDefinedBy rdf:resource="https://w3id.org/italia/onto/HER"/>
    <rdfs:label xml:lang="en">Italian</rdfs:label>
    <rdfs:label xml:lang="it">Italiana</rdfs:label>
    <owl:versionInfo xml:lang="it">stabile</owl:versionInfo>
    <owl:versionInfo xml:lang="en">stable</owl:versionInfo>
  </rdf:Description>
  <rdf:Description rdf:about="https://w3id.org/italia/onto/HER/studiesFDARegulatedDevice">
    <rdf:type rdf:resource="http://www.w3.org/2002/07/owl#DatatypeProperty"/>
    <rdf:type rdf:resource="http://www.w3.org/2002/07/owl#FunctionalProperty"/>
    <rdfs:domain rdf:resource="https://w3id.org/italia/onto/HER/AACTStudy"/>
    <rdfs:range rdf:resource="http://www.w3.org/2001/XMLSchema#boolean"/>
    <rdfs:comment xml:lang="it">Indica se uno studio clinico sta studiando un prodotto per dispositivi soggetti alla sezione 510(k), 515, o 520(m) del Federal Food, Drug, and Cosmetic Act. Selezionare vero/falso.</rdfs:comment>
    <rdfs:comment xml:lang="en">Indication that a clinical study is studying a device product subject to section 510(k), 515, or 520(m) of the Federal Food, Drug, and Cosmetic Act. Select true/false.</rdfs:comment>
    <rdfs:isDefinedBy rdf:resource="https://w3id.org/italia/onto/HER"/>
    <rdfs:label xml:lang="it">studia dispositivo regolamentato da FDA</rdfs:label>
    <rdfs:label xml:lang="en">studies FDA regulated device</rdfs:label>
    <owl:versionInfo xml:lang="it">stabile</owl:versionInfo>
    <owl:versionInfo xml:lang="en">stable</owl:versionInfo>
  </rdf:Description>
  <rdf:Description rdf:about="https://w3id.org/italia/onto/HER/USTATMeasureOfMealsProvided">
    <rdf:type rdf:resource="http://www.w3.org/2002/07/owl#Class"/>
    <rdfs:subClassOf rdf:resource="https://w3id.org/italia/onto/MU/MeasureType"/>
    <rdfs:comment xml:lang="en">Information (code, description and number) on meals provided in the calendar year (T-1). The types are represented by the following codes and descriptions:
11: Meals provided in directly managed canteens
12: Meals provided in indirectly managed canteens
13: Meals provided in contracted catering services
14: Students who use canteens</rdfs:comment>
    <rdfs:comment xml:lang="it">Informazioni (codice, descrizione e numero) sui pasti erogati nell'anno solare (T-1). Le tipologie sono rappresentate dai seguenti codici e descrizioni:
11: Pasti erogati in mense a gestione diretta
12: Pasti erogati in mense a gestione indiretta
13: Pasti erogati in servizi di ristorazione convenzionati
14: Studenti che usufruiscono delle mense</rdfs:comment>
    <rdfs:isDefinedBy rdf:resource="https://w3id.org/italia/onto/HER"/>
    <rdfs:label xml:lang="it">Misura dei pasti forniti riportati da USTAT</rdfs:label>
    <rdfs:label xml:lang="en">USTAT Reported Measure of Meals Provided</rdfs:label>
    <owl:versionInfo xml:lang="it">stabile</owl:versionInfo>
    <owl:versionInfo xml:lang="en">stable</owl:versionInfo>
  </rdf:Description>
  <rdf:Description rdf:about="https://w3id.org/italia/onto/HER/active">
    <rdf:type rdf:resource="http://www.w3.org/2002/07/owl#DatatypeProperty"/>
    <rdf:type rdf:resource="http://www.w3.org/2002/07/owl#FunctionalProperty"/>
    <rdfs:domain rdf:resource="https://w3id.org/italia/onto/HER/Spinoff"/>
    <rdfs:range rdf:resource="http://www.w3.org/2001/XMLSchema#boolean"/>
    <rdfs:comment xml:lang="it">Definisce lo status dello spin-off come riportato nel dataset.</rdfs:comment>
    <rdfs:comment xml:lang="en">It defines the status of the spin-off as reported in the dataset.</rdfs:comment>
    <rdfs:isDefinedBy rdf:resource="https://w3id.org/italia/onto/HER"/>
    <rdfs:label xml:lang="en">active</rdfs:label>
    <rdfs:label xml:lang="it">attivo</rdfs:label>
    <owl:versionInfo xml:lang="it">stabile</owl:versionInfo>
    <owl:versionInfo xml:lang="en">stable</owl:versionInfo>
  </rdf:Description>
  <rdf:Description rdf:nodeID="n5bb3bff42afb4ca286d2c3fead9507ddb395">
    <rdf:type rdf:resource="http://www.w3.org/2002/07/owl#Restriction"/>
    <owl:onProperty rdf:resource="https://w3id.org/italia/onto/HER/verificationDate"/>
    <owl:maxQualifiedCardinality rdf:datatype="http://www.w3.org/2001/XMLSchema#nonNegativeInteger">1</owl:maxQualifiedCardinality>
    <owl:onDataRange rdf:resource="http://www.w3.org/2001/XMLSchema#date"/>
  </rdf:Description>
  <rdf:Description rdf:about="https://w3id.org/italia/onto/HER/MIURStudentsByCitizenshipDegreeDegreeClassAggregate">
    <rdf:type rdf:resource="http://www.w3.org/2002/07/owl#Class"/>
    <rdfs:subClassOf rdf:resource="https://w3id.org/italia/onto/HER/StatisticalDataAggregation"/>
    <rdfs:comment xml:lang="en">Aggregated data on Italian students filed in the MIUR system, grouped by year, university, citizenship and degree class.</rdfs:comment>
    <rdfs:comment xml:lang="it">Dati aggregati sugli studenti italiani archiviati nel sistema MIUR, raggruppati per anno, università, cittadinanza e classe di laurea.</rdfs:comment>
    <rdfs:isDefinedBy rdf:resource="https://w3id.org/italia/onto/HER"/>
    <rdfs:label xml:lang="en">Aggregate of Italian Students By Citizenship and Degree Class</rdfs:label>
    <rdfs:label xml:lang="it">Aggregazione dei studenti italiani per cittadinanza e classe di laurea</rdfs:label>
    <owl:versionInfo xml:lang="it">stabile</owl:versionInfo>
    <owl:versionInfo xml:lang="en">stable</owl:versionInfo>
  </rdf:Description>
  <rdf:Description rdf:nodeID="n5bb3bff42afb4ca286d2c3fead9507ddb106">
    <rdf:type rdf:resource="http://www.w3.org/2002/07/owl#Class"/>
    <owl:unionOf rdf:nodeID="n5bb3bff42afb4ca286d2c3fead9507ddb107"/>
  </rdf:Description>
  <rdf:Description rdf:nodeID="n5bb3bff42afb4ca286d2c3fead9507ddb245">
    <rdf:first rdf:resource="https://w3id.org/italia/onto/HER/PatentPublicationDetail"/>
    <rdf:rest rdf:nodeID="n5bb3bff42afb4ca286d2c3fead9507ddb246"/>
  </rdf:Description>
  <rdf:Description rdf:nodeID="n5bb3bff42afb4ca286d2c3fead9507ddb359">
    <rdf:first rdf:resource="https://w3id.org/italia/onto/HER/USTATEnrolledStudentsAggregate"/>
    <rdf:rest rdf:nodeID="n5bb3bff42afb4ca286d2c3fead9507ddb360"/>
  </rdf:Description>
  <rdf:Description rdf:about="https://w3id.org/italia/onto/l0/Description">
    <rdf:type rdf:resource="http://www.w3.org/2002/07/owl#Class"/>
  </rdf:Description>
  <rdf:Description rdf:about="https://w3id.org/italia/onto/HER/CHAFEAInstrument">
    <rdf:type rdf:resource="http://www.w3.org/2002/07/owl#Class"/>
    <rdfs:subClassOf rdf:resource="https://w3id.org/italia/onto/l0/Concept"/>
    <rdfs:comment xml:lang="it">Tipo di attività finanziata. I tipi sono: Progetti, Conferenza, Azioni congiunte, Sovvenzione di funzionamento, Accordo quadro di partenariato</rdfs:comment>
    <rdfs:comment xml:lang="en">Type of activity funded. Types are: Projects, Conference, Joint Actions, Operating Grant, Framework Partnership Agreement</rdfs:comment>
    <rdfs:isDefinedBy rdf:resource="https://w3id.org/italia/onto/HER"/>
    <rdfs:label xml:lang="en">CHAFEA Instrument</rdfs:label>
    <rdfs:label xml:lang="it">Strumento CHAFEA</rdfs:label>
    <owl:versionInfo xml:lang="it">stabile</owl:versionInfo>
    <owl:versionInfo xml:lang="en">stable</owl:versionInfo>
    <ns6:wasDerivedFrom rdf:resource="http://www.w3.org/2004/02/skos/core#Concept"/>
  </rdf:Description>
  <rdf:Description rdf:nodeID="n5bb3bff42afb4ca286d2c3fead9507ddb156">
    <rdf:type rdf:resource="http://www.w3.org/1999/02/22-rdf-syntax-ns#List"/>
    <rdf:first>R&amp;S</rdf:first>
    <rdf:rest rdf:nodeID="n5bb3bff42afb4ca286d2c3fead9507ddb157"/>
  </rdf:Description>
  <rdf:Description rdf:nodeID="n5bb3bff42afb4ca286d2c3fead9507ddb246">
    <rdf:first rdf:resource="https://w3id.org/italia/onto/HER/PatentPublicationStage"/>
    <rdf:rest rdf:resource="http://www.w3.org/1999/02/22-rdf-syntax-ns#nil"/>
  </rdf:Description>
  <rdf:Description rdf:about="https://w3id.org/italia/onto/HER/timePerspective">
    <rdf:type rdf:resource="http://www.w3.org/2002/07/owl#DatatypeProperty"/>
    <rdfs:domain rdf:resource="https://w3id.org/italia/onto/HER/AACTDesign"/>
    <rdfs:range rdf:nodeID="n5bb3bff42afb4ca286d2c3fead9507ddb284"/>
    <rdfs:comment xml:lang="it">Rapporto temporale tra il periodo di osservazione e il momento dell'iscrizione dei partecipanti. I tipi sono:
Retrospettiva: Osservazione retrospettiva basata su osservazioni raccolte prevalentemente prima della selezione dei soggetti e dell'iscrizione
Prospettiva: Osservazioni periodiche raccolte prevalentemente in seguito all'iscrizione al corso di studi.
Sezione trasversale: Osservazioni o misurazioni effettuate in un unico momento, di solito all'iscrizione del soggetto
Altro: Spiegato nella descrizione dettagliata</rdfs:comment>
    <rdfs:comment xml:lang="en">Temporal relationship of observation period to time of participant enrollment. Types are:
Retrospective: Look back using observations collected predominantly prior to subject selection and enrollment
Prospective: Look forward using periodic observations collected predominantly following subject enrollment
Cross-sectional: Observations or measurements made at a single point in time, usually at subject enrollment
Other: Explain in Detailed Description
</rdfs:comment>
    <rdfs:isDefinedBy rdf:resource="https://w3id.org/italia/onto/HER"/>
    <rdfs:label xml:lang="it">prospettiva temporale</rdfs:label>
    <rdfs:label xml:lang="en">time perspective</rdfs:label>
    <owl:versionInfo xml:lang="it">stabile</owl:versionInfo>
    <owl:versionInfo xml:lang="en">stable</owl:versionInfo>
  </rdf:Description>
  <rdf:Description rdf:about="https://w3id.org/italia/onto/HER/ScientificDisciplinarySector">
    <rdf:type rdf:resource="http://www.w3.org/2002/07/owl#Class"/>
    <rdfs:subClassOf rdf:resource="https://w3id.org/italia/onto/HER/AcademicDiscipline"/>
    <rdfs:isDefinedBy rdf:resource="https://w3id.org/italia/onto/HER"/>
    <rdfs:label xml:lang="it">Settore Scientifico Disciplinare</rdfs:label>
    <rdfs:label xml:lang="en">Sientific Disciplinary Sector</rdfs:label>
    <owl:versionInfo xml:lang="it">stabile</owl:versionInfo>
    <owl:versionInfo xml:lang="en">stable</owl:versionInfo>
    <ns6:wasDerivedFrom rdf:resource="http://www.w3.org/2004/02/skos/core#Concept"/>
    <ns4:controlledVocabulary rdf:resource="https://w3id.org/italia/controlled-vocabulary/classifications-for-universities/academic-disciplines"/>
  </rdf:Description>
  <rdf:Description rdf:about="https://w3id.org/italia/onto/HER/StatisticalDataAggregation">
    <rdf:type rdf:resource="http://www.w3.org/2002/07/owl#Class"/>
    <rdfs:subClassOf rdf:resource="https://w3id.org/italia/onto/l0/Collection"/>
    <rdfs:subClassOf rdf:nodeID="n5bb3bff42afb4ca286d2c3fead9507ddb525"/>
    <rdfs:isDefinedBy rdf:resource="https://w3id.org/italia/onto/HER"/>
    <rdfs:label xml:lang="it">Aggregazione Statistica</rdfs:label>
    <rdfs:label xml:lang="en">Statistical Aggregation</rdfs:label>
    <owl:versionInfo xml:lang="it">provvisoria</owl:versionInfo>
    <owl:versionInfo xml:lang="en">unstable</owl:versionInfo>
  </rdf:Description>
  <rdf:Description rdf:about="https://w3id.org/italia/onto/HER/hasEurekaTechArea">
    <rdf:type rdf:resource="http://www.w3.org/2002/07/owl#ObjectProperty"/>
    <rdfs:subPropertyOf rdf:resource="https://w3id.org/italia/onto/l0/hasTopic"/>
    <rdfs:domain rdf:resource="https://w3id.org/italia/onto/HER/EUREKAProject"/>
    <rdfs:range rdf:resource="https://w3id.org/italia/onto/HER/EUREKATechArea"/>
    <rdfs:comment xml:lang="it">Questa proprietà collega un progetto EUREKA con l'area tecnologica corrispondente.</rdfs:comment>
    <rdfs:comment xml:lang="en">This property connects an EUREKA project with the corresponding tech area.</rdfs:comment>
    <rdfs:isDefinedBy rdf:resource="https://w3id.org/italia/onto/HER"/>
    <rdfs:label xml:lang="it">ha un area tecnica EUREKA</rdfs:label>
    <rdfs:label xml:lang="en">has EUREKA tech area</rdfs:label>
    <owl:versionInfo xml:lang="it">stabile</owl:versionInfo>
    <owl:versionInfo xml:lang="en">stable</owl:versionInfo>
  </rdf:Description>
  <rdf:Description rdf:nodeID="n5bb3bff42afb4ca286d2c3fead9507ddb385">
    <rdf:type rdf:resource="http://www.w3.org/2002/07/owl#Restriction"/>
    <owl:onProperty rdf:resource="https://w3id.org/italia/onto/HER/whyStopped"/>
    <owl:allValuesFrom rdf:resource="http://www.w3.org/2000/01/rdf-schema#Literal"/>
  </rdf:Description>
  <rdf:Description rdf:nodeID="n5bb3bff42afb4ca286d2c3fead9507ddb67">
    <rdf:type rdf:resource="http://www.w3.org/2002/07/owl#Class"/>
    <owl:unionOf rdf:nodeID="n5bb3bff42afb4ca286d2c3fead9507ddb68"/>
  </rdf:Description>
  <rdf:Description rdf:about="https://w3id.org/italia/onto/HER/hasResult">
    <rdf:type rdf:resource="http://www.w3.org/2002/07/owl#ObjectProperty"/>
    <rdfs:domain rdf:resource="http://www.w3.org/2002/07/owl#Thing"/>
    <rdfs:range rdf:resource="https://w3id.org/italia/onto/HER/Result"/>
    <rdfs:comment xml:lang="en">Property that links any thing in the modelled domain to the result or output.</rdfs:comment>
    <rdfs:comment xml:lang="it">Proprietà che collega qualunque cosa nel dominio modellato a un risultato o output.</rdfs:comment>
    <rdfs:isDefinedBy rdf:resource="https://w3id.org/italia/onto/HER"/>
    <rdfs:label xml:lang="it">ha risultato</rdfs:label>
    <rdfs:label xml:lang="en">has result</rdfs:label>
    <owl:versionInfo xml:lang="it">stabile</owl:versionInfo>
    <owl:versionInfo xml:lang="en">stable</owl:versionInfo>
  </rdf:Description>
  <rdf:Description rdf:about="https://w3id.org/italia/onto/HER/refersToProject">
    <rdf:type rdf:resource="http://www.w3.org/2002/07/owl#ObjectProperty"/>
    <rdfs:domain rdf:resource="https://w3id.org/italia/onto/HER/CTNPRINOperation"/>
    <rdfs:range rdf:resource="https://w3id.org/italia/onto/HER/CTNPRINProject"/>
    <rdfs:comment xml:lang="it">Questa proprietà  collega un'operazione CTN/PRIN con il progetto CTN/PRIN di riferimento</rdfs:comment>
    <rdfs:comment xml:lang="en">This property links a CTN/Prin opertion to the reference CTN/PRIN project.</rdfs:comment>
    <rdfs:isDefinedBy rdf:resource="https://w3id.org/italia/onto/HER"/>
    <rdfs:label xml:lang="en">refers to project</rdfs:label>
    <rdfs:label xml:lang="it">si riferisce a progetto</rdfs:label>
    <owl:versionInfo xml:lang="it">provissoria - da verificare</owl:versionInfo>
    <owl:versionInfo xml:lang="en">unstable</owl:versionInfo>
  </rdf:Description>
  <rdf:Description rdf:about="https://w3id.org/italia/onto/HER/PRC">
    <rdf:type rdf:resource="http://www.w3.org/2002/07/owl#NamedIndividual"/>
    <rdf:type rdf:resource="https://w3id.org/italia/onto/HER/ECActivityType"/>
    <rdfs:isDefinedBy rdf:resource="https://w3id.org/italia/onto/HER"/>
    <rdfs:label xml:lang="en">Private for-profit entities (excluding Higher or Secondary Education Establishments)</rdfs:label>
    <owl:versionInfo xml:lang="it">stabile</owl:versionInfo>
    <owl:versionInfo xml:lang="en">stable</owl:versionInfo>
  </rdf:Description>
  <rdf:Description rdf:nodeID="n5bb3bff42afb4ca286d2c3fead9507ddb531">
    <rdf:type rdf:resource="http://www.w3.org/2002/07/owl#Restriction"/>
    <owl:onProperty rdf:resource="https://w3id.org/italia/onto/COV/hasOrganization"/>
    <owl:maxQualifiedCardinality rdf:datatype="http://www.w3.org/2001/XMLSchema#nonNegativeInteger">1</owl:maxQualifiedCardinality>
    <owl:onClass rdf:resource="https://w3id.org/italia/onto/COV/Organization"/>
  </rdf:Description>
  <rdf:Description rdf:about="https://w3id.org/italia/onto/HER/additionalInfo">
    <rdf:type rdf:resource="http://www.w3.org/2002/07/owl#DatatypeProperty"/>
    <rdfs:domain rdf:resource="https://w3id.org/italia/onto/HER/Spinoff"/>
    <rdfs:range rdf:resource="http://www.w3.org/2000/01/rdf-schema#Literal"/>
    <rdfs:comment xml:lang="en">It reports notes and additional information about the spin-off, if any.</rdfs:comment>
    <rdfs:comment xml:lang="it">Riporta delle note e informazioni addizionali sullo spin-off, se presenti.</rdfs:comment>
    <rdfs:isDefinedBy rdf:resource="https://w3id.org/italia/onto/HER"/>
    <rdfs:label xml:lang="en">additional information</rdfs:label>
    <rdfs:label xml:lang="it">informazioni aggiuntive</rdfs:label>
    <owl:versionInfo xml:lang="it">stabile</owl:versionInfo>
    <owl:versionInfo xml:lang="en">stable</owl:versionInfo>
  </rdf:Description>
  <rdf:Description rdf:about="https://w3id.org/italia/onto/HER/ERCProject">
    <rdf:type rdf:resource="http://www.w3.org/2002/07/owl#Class"/>
    <rdfs:subClassOf rdf:resource="https://w3id.org/italia/onto/HER/ECProject"/>
    <rdfs:subClassOf rdf:nodeID="n5bb3bff42afb4ca286d2c3fead9507ddb459"/>
    <rdfs:comment xml:lang="it">Progetto finanziato dal Consiglio Europeo della Ricerca</rdfs:comment>
    <rdfs:comment xml:lang="en">Project funded by the European Research Council</rdfs:comment>
    <rdfs:isDefinedBy rdf:resource="https://w3id.org/italia/onto/HER"/>
    <rdfs:label xml:lang="en">ERC Project</rdfs:label>
    <rdfs:label xml:lang="it">Progetto ERC</rdfs:label>
    <owl:versionInfo xml:lang="it">stabile</owl:versionInfo>
    <owl:versionInfo xml:lang="en">stable</owl:versionInfo>
  </rdf:Description>
  <rdf:Description rdf:nodeID="n5bb3bff42afb4ca286d2c3fead9507ddb378">
    <rdf:type rdf:resource="http://www.w3.org/2002/07/owl#Restriction"/>
    <owl:onProperty rdf:resource="https://w3id.org/italia/onto/l0/identifier"/>
    <owl:allValuesFrom rdf:resource="http://www.w3.org/2000/01/rdf-schema#Literal"/>
  </rdf:Description>
  <rdf:Description rdf:about="http://purl.org/dc/terms/language">
    <rdf:type rdf:resource="http://www.w3.org/2002/07/owl#AnnotationProperty"/>
  </rdf:Description>
  <rdf:Description rdf:nodeID="n5bb3bff42afb4ca286d2c3fead9507ddb343">
    <rdf:first rdf:resource="https://w3id.org/italia/onto/HER/USTATStaffByGender"/>
    <rdf:rest rdf:nodeID="n5bb3bff42afb4ca286d2c3fead9507ddb344"/>
  </rdf:Description>
  <rdf:Description rdf:about="https://w3id.org/italia/onto/HER/hasStudyFirstPostedDate">
    <rdf:type rdf:resource="http://www.w3.org/2002/07/owl#ObjectProperty"/>
    <rdfs:subPropertyOf rdf:resource="https://w3id.org/italia/onto/TI/hasTemporalEntity"/>
    <rdfs:domain rdf:resource="https://w3id.org/italia/onto/HER/AACTStudy"/>
    <rdfs:range rdf:resource="https://w3id.org/italia/onto/TI#TimeInstant"/>
    <rdfs:comment xml:lang="it">La data in cui il record dello studio è stato disponibile per la prima volta su ClinicalTrials.gov. In genere c'è un ritardo di alcuni giorni tra la data in cui lo sponsor dello studio o lo sperimentatore ha presentato la cartella clinica e la prima data di pubblicazione.</rdfs:comment>
    <rdfs:comment xml:lang="en">The date on which the study record was first available on ClinicalTrials.gov. There is typically a delay of a few days between the date the study sponsor or investigator submitted the study record and the first posted date.</rdfs:comment>
    <rdfs:isDefinedBy rdf:resource="https://w3id.org/italia/onto/HER"/>
    <rdfs:label xml:lang="it">ha data inizio studio</rdfs:label>
    <rdfs:label xml:lang="en">has study first posted date</rdfs:label>
    <owl:versionInfo xml:lang="it">prova</owl:versionInfo>
    <owl:versionInfo xml:lang="en">testing</owl:versionInfo>
  </rdf:Description>
  <rdf:Description rdf:nodeID="n5bb3bff42afb4ca286d2c3fead9507ddb110">
    <rdf:first rdf:resource="https://w3id.org/italia/onto/HER/USTATPermanentStaff"/>
    <rdf:rest rdf:nodeID="n5bb3bff42afb4ca286d2c3fead9507ddb111"/>
  </rdf:Description>
  <rdf:Description rdf:about="https://w3id.org/italia/onto/HER/distributedInErasumplusFile">
    <rdf:type rdf:resource="http://www.w3.org/2002/07/owl#ObjectProperty"/>
    <rdfs:domain rdf:resource="https://w3id.org/italia/onto/HER/ErasmusPlusProjectResult"/>
    <rdfs:range rdf:resource="https://w3id.org/italia/onto/HER/ErasmusPlusFile"/>
    <rdfs:comment xml:lang="en">It is used to link the output result of an erasmus plus project to the associated file.</rdfs:comment>
    <rdfs:comment xml:lang="it">Viene utilizzato per collegare il risultato di un progetto erasmus plus al file associato.</rdfs:comment>
    <rdfs:isDefinedBy rdf:resource="https://w3id.org/italia/onto/HER"/>
    <rdfs:label xml:lang="it">distribuito in un file eramsus+</rdfs:label>
    <rdfs:label xml:lang="en">distributed in erasmus+ file</rdfs:label>
    <owl:versionInfo xml:lang="it">stabile</owl:versionInfo>
    <owl:versionInfo xml:lang="en">stable</owl:versionInfo>
  </rdf:Description>
  <rdf:Description rdf:about="https://w3id.org/italia/onto/HER/hasERCPanel">
    <rdf:type rdf:resource="http://www.w3.org/2002/07/owl#ObjectProperty"/>
    <rdfs:subPropertyOf rdf:resource="https://w3id.org/italia/onto/l0/hasTopic"/>
    <rdfs:domain rdf:nodeID="n5bb3bff42afb4ca286d2c3fead9507ddb53"/>
    <rdfs:range rdf:resource="https://w3id.org/italia/onto/HER/ERCPanel"/>
    <rdfs:comment xml:lang="it">Questa proprietà si collega al corrispondente pannello del CER.</rdfs:comment>
    <rdfs:comment xml:lang="en">This property links to the corresponding ERC panel.</rdfs:comment>
    <rdfs:isDefinedBy rdf:resource="https://w3id.org/italia/onto/HER"/>
    <rdfs:label xml:lang="it">ha pannello ERC</rdfs:label>
    <rdfs:label xml:lang="en">has ERC panel</rdfs:label>
    <owl:versionInfo xml:lang="it">stabile</owl:versionInfo>
    <owl:versionInfo xml:lang="en">stable</owl:versionInfo>
  </rdf:Description>
  <rdf:Description rdf:nodeID="n5bb3bff42afb4ca286d2c3fead9507ddb299">
    <rdf:first rdf:resource="https://w3id.org/italia/onto/HER/USTATMealsProvidedAggregate"/>
    <rdf:rest rdf:nodeID="n5bb3bff42afb4ca286d2c3fead9507ddb300"/>
  </rdf:Description>
  <rdf:Description rdf:nodeID="n5bb3bff42afb4ca286d2c3fead9507ddb225">
    <rdf:first rdf:resource="https://w3id.org/italia/onto/HER/MIURStudentsByDiplomaAggregate"/>
    <rdf:rest rdf:nodeID="n5bb3bff42afb4ca286d2c3fead9507ddb226"/>
  </rdf:Description>
  <rdf:Description rdf:about="https://w3id.org/italia/onto/HER/biospecRetention">
    <rdf:type rdf:resource="http://www.w3.org/2002/07/owl#DatatypeProperty"/>
    <rdfs:domain rdf:resource="https://w3id.org/italia/onto/HER/AACTStudy"/>
    <rdfs:range rdf:nodeID="n5bb3bff42afb4ca286d2c3fead9507ddb136"/>
    <rdfs:comment xml:lang="it">Indica se i campioni di materiale dei partecipanti alla ricerca sono conservati in un biorepository. I valori ammessi sono:
Nessuno Conservato: Nessun campione conservato
Campioni con DNA: Campioni conservati, con possibilità di estrazione del DNA da almeno uno dei tipi di campioni conservati (ad esempio, tessuto congelato, sangue intero)
Campioni senza DNA: Campioni conservati, senza possibilità di estrazione del DNA da campioni conservati (ad esempio, tessuto fisso, plasma)</rdfs:comment>
    <rdfs:comment xml:lang="en">Indicate whether samples of material from research participants are retained in a biorepository. They can be:
None Retained: No samples retained
Samples With DNA: Samples retained, with potential for extraction of DNA from at least one of the types of samples retained (e.g., frozen tissue, whole blood)
Samples Without DNA: Samples retained, with no potential for DNA extraction from any retained samples (e.g., fixed tissue, plasma)
</rdfs:comment>
    <rdfs:isDefinedBy rdf:resource="https://w3id.org/italia/onto/HER"/>
    <rdfs:label xml:lang="en">biospec retention</rdfs:label>
    <rdfs:label xml:lang="it">conservazione biospec</rdfs:label>
    <owl:versionInfo xml:lang="it">stabile</owl:versionInfo>
    <owl:versionInfo xml:lang="en">stable</owl:versionInfo>
  </rdf:Description>
  <rdf:Description rdf:about="https://w3id.org/italia/onto/HER/AACTFacility">
    <rdf:type rdf:resource="http://www.w3.org/2002/07/owl#Class"/>
    <rdfs:subClassOf rdf:resource="https://w3id.org/italia/onto/CLV/SpatialObject"/>
    <rdfs:subClassOf rdf:nodeID="n5bb3bff42afb4ca286d2c3fead9507ddb376"/>
    <rdfs:subClassOf rdf:nodeID="n5bb3bff42afb4ca286d2c3fead9507ddb377"/>
    <rdfs:comment xml:lang="it">conduzione del sito/partecipazione ad uno studio</rdfs:comment>
    <rdfs:comment xml:lang="en">site conducting/participating in a study</rdfs:comment>
    <rdfs:isDefinedBy rdf:resource="https://w3id.org/italia/onto/HER"/>
    <rdfs:label xml:lang="en">Facility Clinical Trial</rdfs:label>
    <rdfs:label xml:lang="it">Struttura sperimentazione clinica</rdfs:label>
    <owl:versionInfo xml:lang="it">stabile</owl:versionInfo>
    <owl:versionInfo xml:lang="en">stable</owl:versionInfo>
  </rdf:Description>
  <rdf:Description rdf:about="https://w3id.org/italia/onto/HER/USTATPostgraduateAggregateOfEnrolled">
    <rdf:type rdf:resource="http://www.w3.org/2002/07/owl#Class"/>
    <rdfs:subClassOf rdf:resource="https://w3id.org/italia/onto/HER/StatisticalDataAggregation"/>
    <rdfs:subClassOf rdf:nodeID="n5bb3bff42afb4ca286d2c3fead9507ddb533"/>
    <rdfs:comment xml:lang="en">Information about the students enrolled in [Specialisation Schools / Level I Master / Level II Master / Research Doctorates] by university and by course of study (time series).</rdfs:comment>
    <rdfs:comment xml:lang="it">Informazioni sugli iscritti a [Scuole di specializzazione/Master di I livello/Master di II livello/Dottorati di ricerca] per ateneo e per corso di studio (serie storica).</rdfs:comment>
    <rdfs:isDefinedBy rdf:resource="https://w3id.org/italia/onto/HER"/>
    <rdfs:label xml:lang="it">Aggregazione USTAT Postgraduate - Iscritti</rdfs:label>
    <rdfs:label xml:lang="en">USTAT Postgraduate Aggregate of Enrolled</rdfs:label>
    <owl:versionInfo xml:lang="it">stabile</owl:versionInfo>
    <owl:versionInfo xml:lang="en">stable</owl:versionInfo>
  </rdf:Description>
  <rdf:Description rdf:about="https://w3id.org/italia/onto/HER/hasInitiative">
    <rdf:type rdf:resource="http://www.w3.org/2002/07/owl#ObjectProperty"/>
    <rdfs:domain rdf:nodeID="n5bb3bff42afb4ca286d2c3fead9507ddb70"/>
    <rdfs:range rdf:resource="https://w3id.org/italia/onto/HER/CTNPRINInitiative"/>
    <rdfs:comment xml:lang="en">An initiative may be associated with a call for proposals, a notice, an invitation, a campaign, etc.</rdfs:comment>
    <rdfs:comment xml:lang="it">Un'iniziativa può essere associata ad un bando, un avviso, un invito, una campagna, etc.</rdfs:comment>
    <rdfs:isDefinedBy rdf:resource="https://w3id.org/italia/onto/HER"/>
    <rdfs:label xml:lang="it">ha un'iniziativa CTN/PRIN</rdfs:label>
    <rdfs:label xml:lang="en">has CTN/PRIN initiative</rdfs:label>
    <owl:versionInfo xml:lang="it">stabile</owl:versionInfo>
    <owl:versionInfo xml:lang="en">stable</owl:versionInfo>
  </rdf:Description>
  <rdf:Description rdf:about="https://w3id.org/italia/onto/HER/ISCEDFClassification">
    <rdf:type rdf:resource="http://www.w3.org/2002/07/owl#Class"/>
    <rdfs:subClassOf rdf:resource="https://w3id.org/italia/onto/HER/HERClassification"/>
    <rdfs:comment xml:lang="it">La classificazione internazionale standard dell'istruzione (ISCED) è un quadro per l'assemblaggio, la compilazione e l'analisi di statistiche comparabili a livello transnazionale sull'istruzione. (Fonte: https://unesdoc.unesco.org/ark:/48223/pf0000228085)</rdfs:comment>
    <rdfs:comment xml:lang="en">The International Standard Classification of Education (ISCED) is a framework for assembling, compiling and analysing cross-nationally comparable statistics on education. (Source: https://unesdoc.unesco.org/ark:/48223/pf0000228085)</rdfs:comment>
    <rdfs:isDefinedBy rdf:resource="https://w3id.org/italia/onto/HER"/>
    <rdfs:label xml:lang="it">Classificazione ISCED-F</rdfs:label>
    <rdfs:label xml:lang="en">ISCED-F Classification</rdfs:label>
    <owl:versionInfo xml:lang="it">stabile</owl:versionInfo>
    <owl:versionInfo xml:lang="en">stable</owl:versionInfo>
    <ns6:wasDerivedFrom rdf:resource="http://www.w3.org/2004/02/skos/core#Concept"/>
  </rdf:Description>
  <rdf:Description rdf:about="https://w3id.org/italia/onto/HER/USTATContributionByClass">
    <rdf:type rdf:resource="http://www.w3.org/2002/07/owl#Class"/>
    <rdfs:subClassOf rdf:resource="https://w3id.org/italia/onto/HER/StatisticalDataAggregation"/>
    <rdfs:comment xml:lang="en">Data relating to the contribution classes of university students. Indicates the distribution of students by class of contribution amount per capita, per Academic year (T-1)/(T).</rdfs:comment>
    <rdfs:comment xml:lang="it">Dati relativi alle classi di contribuzione degli studenti universitari. Indica la distribuzione degli studenti per classe di importo della contribuzione pro-capite, per anno Accademico (T-1)/(T)</rdfs:comment>
    <rdfs:isDefinedBy rdf:resource="https://w3id.org/italia/onto/HER"/>
    <rdfs:label xml:lang="it">Aggregazione dei contributi per classe riportati da USTAT</rdfs:label>
    <rdfs:label xml:lang="en">USTAT Aggregate of Contributions By Class</rdfs:label>
    <owl:versionInfo xml:lang="it">stabile</owl:versionInfo>
    <owl:versionInfo xml:lang="en">stable</owl:versionInfo>
  </rdf:Description>
  <rdf:Description rdf:about="https://w3id.org/italia/onto/HER/hasAcademicRole">
    <rdf:type rdf:resource="http://www.w3.org/2002/07/owl#ObjectProperty"/>
    <rdfs:domain rdf:resource="https://w3id.org/italia/onto/HER/ResearcherSeniorityGrade"/>
    <rdfs:range rdf:nodeID="n5bb3bff42afb4ca286d2c3fead9507ddb32"/>
    <rdfs:comment xml:lang="en">Connects a ReseacherSeniorityGrade with the corresponding AcademicRole.</rdfs:comment>
    <rdfs:comment xml:lang="it">Connette un ReseacherSeniorityGrade al corrispondente AcademicRole.</rdfs:comment>
    <rdfs:isDefinedBy rdf:resource="https://w3id.org/italia/onto/HER"/>
    <rdfs:label xml:lang="it">ha ruolo accademico</rdfs:label>
    <rdfs:label xml:lang="en">has academic role</rdfs:label>
    <owl:versionInfo xml:lang="it">stabile</owl:versionInfo>
    <owl:versionInfo xml:lang="en">stable</owl:versionInfo>
  </rdf:Description>
  <rdf:Description rdf:about="https://w3id.org/italia/onto/HER/endingYear">
    <rdf:type rdf:resource="http://www.w3.org/2002/07/owl#DatatypeProperty"/>
    <rdfs:subPropertyOf rdf:resource="https://w3id.org/italia/onto/TI/year"/>
    <rdfs:domain rdf:nodeID="n5bb3bff42afb4ca286d2c3fead9507ddb168"/>
    <rdfs:range rdf:resource="http://www.w3.org/2001/XMLSchema#gYear"/>
    <rdfs:comment xml:lang="en">Ending year of the project</rdfs:comment>
    <rdfs:comment xml:lang="it">Indica l'anno di fine di un progetto</rdfs:comment>
    <rdfs:isDefinedBy rdf:resource="https://w3id.org/italia/onto/HER"/>
    <rdfs:label xml:lang="it">anno di fine</rdfs:label>
    <rdfs:label xml:lang="en">ending year</rdfs:label>
    <owl:versionInfo xml:lang="it">stabile</owl:versionInfo>
    <owl:versionInfo xml:lang="en">stable</owl:versionInfo>
  </rdf:Description>
  <rdf:Description rdf:about="https://w3id.org/italia/onto/HER/grantAgreementNo">
    <rdf:type rdf:resource="http://www.w3.org/2002/07/owl#DatatypeProperty"/>
    <rdfs:subPropertyOf rdf:resource="https://w3id.org/italia/onto/l0/identifier"/>
    <rdfs:range rdf:resource="http://www.w3.org/2000/01/rdf-schema#Literal"/>
    <rdfs:comment xml:lang="en">Grant agreement identifier of an EC project.</rdfs:comment>
    <rdfs:comment xml:lang="it">Identificativo dell'accordo di sovvenzione di un progetto CE.</rdfs:comment>
    <rdfs:isDefinedBy rdf:resource="https://w3id.org/italia/onto/HER"/>
    <rdfs:label xml:lang="en">grant agreement number</rdfs:label>
    <rdfs:label xml:lang="it">numero dell'accordo di sovvenzione</rdfs:label>
    <owl:versionInfo xml:lang="it">provvisoria</owl:versionInfo>
    <owl:versionInfo xml:lang="en">unstable</owl:versionInfo>
  </rdf:Description>
  <rdf:Description rdf:nodeID="n5bb3bff42afb4ca286d2c3fead9507ddb324">
    <rdf:first rdf:resource="https://w3id.org/italia/onto/HER/USTATPostgraduateAggregateOfGraduated"/>
    <rdf:rest rdf:nodeID="n5bb3bff42afb4ca286d2c3fead9507ddb325"/>
  </rdf:Description>
  <rdf:Description rdf:nodeID="n5bb3bff42afb4ca286d2c3fead9507ddb494">
    <rdf:type rdf:resource="http://www.w3.org/2002/07/owl#Restriction"/>
    <owl:onProperty rdf:resource="https://w3id.org/italia/onto/CLV/hasSpatialCoverage"/>
    <owl:someValuesFrom rdf:resource="https://w3id.org/italia/onto/CLV/Province"/>
  </rdf:Description>
  <rdf:Description rdf:nodeID="n5bb3bff42afb4ca286d2c3fead9507ddb147">
    <rdf:type rdf:resource="http://www.w3.org/1999/02/22-rdf-syntax-ns#List"/>
    <rdf:first>Industrial research</rdf:first>
    <rdf:rest rdf:nodeID="n5bb3bff42afb4ca286d2c3fead9507ddb148"/>
  </rdf:Description>
  <rdf:Description rdf:about="https://w3id.org/italia/onto/HER/USTATPostgraduateAggregateOfGraduated">
    <rdf:type rdf:resource="http://www.w3.org/2002/07/owl#Class"/>
    <rdfs:subClassOf rdf:resource="https://w3id.org/italia/onto/HER/StatisticalDataAggregation"/>
    <rdfs:subClassOf rdf:nodeID="n5bb3bff42afb4ca286d2c3fead9507ddb534"/>
    <rdfs:comment xml:lang="en">Information on graduates (of specialization schools, Masters of I and II level, PhDs) by university and by course of study (time series).</rdfs:comment>
    <rdfs:comment xml:lang="it">Informazioni sui diplomati di [Scuole di specializzazione/Master di I livello/Master di II livello/Dottorati di ricerca] per corso di studio.</rdfs:comment>
    <rdfs:isDefinedBy rdf:resource="https://w3id.org/italia/onto/HER"/>
    <rdfs:label xml:lang="it">Aggregazione USTAT Postgraduate - Diplomati</rdfs:label>
    <rdfs:label xml:lang="en">USTAT Postgraduate Aggregate of Graduated</rdfs:label>
    <owl:versionInfo xml:lang="it">stabile</owl:versionInfo>
    <owl:versionInfo xml:lang="en">stable</owl:versionInfo>
  </rdf:Description>
  <rdf:Description rdf:about="https://w3id.org/italia/onto/HER/USTATUniversityInterventionExpensesAggregate">
    <rdf:type rdf:resource="http://www.w3.org/2002/07/owl#Class"/>
    <rdfs:subClassOf rdf:resource="https://w3id.org/italia/onto/HER/StatisticalDataAggregation"/>
    <rdfs:subClassOf rdf:nodeID="n5bb3bff42afb4ca286d2c3fead9507ddb545"/>
    <rdfs:comment xml:lang="en">Data on expenditure on interventions in favour of university students (student loans only).</rdfs:comment>
    <rdfs:comment xml:lang="it">Dati relativi alla spesa per interventi a favore degli studenti degli atenei (solo prestiti a studenti).</rdfs:comment>
    <rdfs:isDefinedBy rdf:resource="https://w3id.org/italia/onto/HER"/>
    <rdfs:label xml:lang="it">Aggregazione delle spese di interventi universitari riportati da USTAT</rdfs:label>
    <rdfs:label xml:lang="en">USTAT Aggregate of University Intervention Expenses</rdfs:label>
    <owl:versionInfo xml:lang="it">stabile</owl:versionInfo>
    <owl:versionInfo xml:lang="en">stable</owl:versionInfo>
  </rdf:Description>
  <rdf:Description rdf:nodeID="n5bb3bff42afb4ca286d2c3fead9507ddb287">
    <rdf:type rdf:resource="http://www.w3.org/1999/02/22-rdf-syntax-ns#List"/>
    <rdf:first>Cross-Sectional, Retrospective</rdf:first>
    <rdf:rest rdf:nodeID="n5bb3bff42afb4ca286d2c3fead9507ddb288"/>
  </rdf:Description>
  <rdf:Description rdf:about="https://w3id.org/italia/onto/HER/hasErasmusplusActionType">
    <rdf:type rdf:resource="http://www.w3.org/2002/07/owl#ObjectProperty"/>
    <rdfs:domain rdf:resource="https://w3id.org/italia/onto/HER/ErasmusPlusProject"/>
    <rdfs:range rdf:resource="https://w3id.org/italia/onto/HER/ErasmusPlusActionType"/>
    <rdfs:comment xml:lang="en">It is used to link Erasmus+ projects to the action types.</rdfs:comment>
    <rdfs:comment xml:lang="it">Viene utilizzato per collegare i progetti Erasmus+ ai tipi di azione.</rdfs:comment>
    <rdfs:isDefinedBy rdf:resource="https://w3id.org/italia/onto/HER"/>
    <rdfs:label xml:lang="it">ha tipologia di azione Erasmus+</rdfs:label>
    <rdfs:label xml:lang="en">has Erasmus+ action type</rdfs:label>
    <owl:versionInfo xml:lang="it">stabile</owl:versionInfo>
    <owl:versionInfo xml:lang="en">stable</owl:versionInfo>
  </rdf:Description>
  <rdf:Description rdf:nodeID="n5bb3bff42afb4ca286d2c3fead9507ddb286">
    <rdf:type rdf:resource="http://www.w3.org/1999/02/22-rdf-syntax-ns#List"/>
    <rdf:first>Cross-Sectional, Prospective</rdf:first>
    <rdf:rest rdf:nodeID="n5bb3bff42afb4ca286d2c3fead9507ddb287"/>
  </rdf:Description>
  <rdf:Description rdf:nodeID="n5bb3bff42afb4ca286d2c3fead9507ddb366">
    <rdf:first rdf:resource="https://w3id.org/italia/onto/HER/ECProject"/>
    <rdf:rest rdf:nodeID="n5bb3bff42afb4ca286d2c3fead9507ddb367"/>
  </rdf:Description>
  <rdf:Description rdf:nodeID="n5bb3bff42afb4ca286d2c3fead9507ddb35">
    <rdf:type rdf:resource="http://www.w3.org/2002/07/owl#Class"/>
    <owl:unionOf rdf:nodeID="n5bb3bff42afb4ca286d2c3fead9507ddb36"/>
  </rdf:Description>
  <rdf:Description rdf:about="https://w3id.org/italia/onto/HER/hasAACTEligibility">
    <rdf:type rdf:resource="http://www.w3.org/2002/07/owl#ObjectProperty"/>
    <rdfs:domain rdf:resource="https://w3id.org/italia/onto/HER/AACTStudy"/>
    <rdfs:range rdf:resource="https://w3id.org/italia/onto/HER/AACTEligibility"/>
    <rdfs:comment xml:lang="it">I requisiti chiave che le persone che vogliono partecipare a uno studio clinico devono soddisfare o le caratteristiche che devono avere.</rdfs:comment>
    <rdfs:comment xml:lang="en">The key requirements that people who want to participate in a clinical study must meet or the characteristics they must have.</rdfs:comment>
    <rdfs:isDefinedBy rdf:resource="https://w3id.org/italia/onto/HER"/>
    <rdfs:label xml:lang="it">ha idoneitá AACT</rdfs:label>
    <rdfs:label xml:lang="en">has AACT eligibility</rdfs:label>
    <owl:versionInfo xml:lang="it">stabile</owl:versionInfo>
    <owl:versionInfo xml:lang="en">stable</owl:versionInfo>
  </rdf:Description>
  <rdf:Description rdf:nodeID="n5bb3bff42afb4ca286d2c3fead9507ddb65">
    <rdf:first rdf:resource="https://w3id.org/italia/onto/HER/ECProject"/>
    <rdf:rest rdf:nodeID="n5bb3bff42afb4ca286d2c3fead9507ddb66"/>
  </rdf:Description>
  <rdf:Description rdf:about="https://w3id.org/italia/onto/HER/EUREKAInstrument">
    <rdf:type rdf:resource="http://www.w3.org/2002/07/owl#Class"/>
    <rdfs:subClassOf rdf:resource="https://w3id.org/italia/onto/HER/HERClassification"/>
    <rdfs:comment xml:lang="en">EUREKA financial instrument. EUREKA instruments are of several kinds, and their choice depends mainly on the type of research project to be developed (Eurostars, Clusters, Network projects and InvestHorizon).</rdfs:comment>
    <rdfs:comment xml:lang="it">Strumento finanziario EUREKA. Gli strumenti EUREKA sono di vario tipo e la loro scelta dipende principalmente dal tipo di progetto di ricerca da sviluppare (Eurostars, Clusters, progetti di rete e InvestHorizon).</rdfs:comment>
    <rdfs:isDefinedBy rdf:resource="https://w3id.org/italia/onto/HER"/>
    <rdfs:label xml:lang="en">EUREKA Instrument</rdfs:label>
    <rdfs:label xml:lang="it">Strumento EUREKA</rdfs:label>
    <owl:versionInfo xml:lang="it">stabile</owl:versionInfo>
    <owl:versionInfo xml:lang="en">stable</owl:versionInfo>
    <ns6:wasDerivedFrom rdf:resource="http://www.w3.org/2004/02/skos/core#Concept"/>
  </rdf:Description>
  <rdf:Description rdf:about="https://w3id.org/italia/onto/HER/AACTCondition">
    <rdf:type rdf:resource="http://www.w3.org/2002/07/owl#Class"/>
    <rdfs:subClassOf rdf:resource="https://w3id.org/italia/onto/l0/Characteristic"/>
    <rdfs:comment xml:lang="it">La malattia, il disturbo, la sindrome, o la lesione che si sta studiando. Su ClinicalTrials.gov, le condizioni possono includere anche altre questioni relative alla salute, come la durata della vita, la qualità della vita e i rischi per la salute. Il nome della condizione può includere lettere maiuscolo o minuscole.</rdfs:comment>
    <rdfs:comment xml:lang="en">The disease, disorder, syndrome, illness, or injury that is being studied. On ClinicalTrials.gov, conditions may also include other health-related issues, such as lifespan, quality of life, and health risks. The name of the condition may include upper or lower case letters.</rdfs:comment>
    <rdfs:isDefinedBy rdf:resource="https://w3id.org/italia/onto/HER"/>
    <rdfs:label xml:lang="en">Condition</rdfs:label>
    <rdfs:label xml:lang="it">Condizione</rdfs:label>
    <owl:versionInfo xml:lang="it">stabile</owl:versionInfo>
    <owl:versionInfo xml:lang="en">stable</owl:versionInfo>
  </rdf:Description>
  <rdf:Description rdf:nodeID="n5bb3bff42afb4ca286d2c3fead9507ddb8">
    <rdf:first rdf:resource="https://w3id.org/italia/onto/HER/AACTMeshTerm"/>
    <rdf:rest rdf:nodeID="n5bb3bff42afb4ca286d2c3fead9507ddb9"/>
  </rdf:Description>
  <rdf:Description rdf:nodeID="n5bb3bff42afb4ca286d2c3fead9507ddb141">
    <rdf:first rdf:resource="https://w3id.org/italia/onto/HER/ECProject"/>
    <rdf:rest rdf:nodeID="n5bb3bff42afb4ca286d2c3fead9507ddb142"/>
  </rdf:Description>
  <rdf:Description rdf:about="https://w3id.org/italia/onto/HER/numberOfProponents">
    <rdf:type rdf:resource="http://www.w3.org/2002/07/owl#DatatypeProperty"/>
    <rdfs:domain rdf:resource="https://w3id.org/italia/onto/HER/CTNPRINInitiative"/>
    <rdfs:range rdf:resource="http://www.w3.org/2001/XMLSchema#int"/>
    <rdfs:comment xml:lang="it">Numero totale di persone giuridiche (soggetti) indicati come proponenti nelle proposte presentate. NB: se un unico soggetto è presente in più proposte viene contato tante volte quante sono le proposte in cui appare</rdfs:comment>
    <rdfs:comment xml:lang="en">Total number of legal persons (entities) indicated as proposers in the proposals submitted. NB: if only one entity is present in more than one proposal, it is counted as many times as there are proposals where it appears</rdfs:comment>
    <rdfs:isDefinedBy rdf:resource="https://w3id.org/italia/onto/HER"/>
    <rdfs:label xml:lang="en">number of proponents</rdfs:label>
    <rdfs:label xml:lang="it">numero di sostenitori</rdfs:label>
    <owl:versionInfo xml:lang="it">stabile</owl:versionInfo>
    <owl:versionInfo xml:lang="en">stable</owl:versionInfo>
  </rdf:Description>
  <rdf:Description rdf:about="https://w3id.org/italia/onto/HER/hasUSTATContributionClass">
    <rdf:type rdf:resource="http://www.w3.org/2002/07/owl#ObjectProperty"/>
    <rdfs:domain rdf:resource="https://w3id.org/italia/onto/HER/USTATContributionByClass"/>
    <rdfs:range rdf:resource="https://w3id.org/italia/onto/HER/USTATContributionClass"/>
    <rdfs:comment xml:lang="en">Code of the university student contribution class. Can take the values:
00: contribution not expected (excluding exemptions)
00a: contribution financed by external bodies
01 : from 0,01 to 100,00 (excluding exemptions)
02 : from 100,01 to 200,00
03 : from 200,01 to 300,00
04 : from 300,01 to 400,00
05 : from 400,01 to 500,00
06 : from 500,01 to 600,00
07 : from 600,01 to 700,00
08 : from 700,01 to 800,00
09 : from 800,01 to 900,00
10 : from 900.01 to 1,000.00
11a: from 1,000.01 to 1,100.00
11b: from 1.100,01 to 1.200,00
11c: from 1.200,01 to 1.300,00
11d: from 1.300,01 to 1.400,00
11e: from 1.400,01 to 1.500,00
12a: from 1.500,01 to 1.600,00
12b: from 1.600,01 to 1.700,00
12c: from 1.700,01 to 1.800,00
12d: from 1.800,01 to 1.900,00
12e: from 1,900.01 to 2,000.00
13 : from 2.000,01 to 2.500,00
14 : from 2,500.01 to 3,000.00
15 : from 3.000,01 to 3.500,00
16 : from 3.500,01 to 4.000,00
17 : from 4.000,01 to 4.500,00
18 : from 4.500,01 to 5.000,00
19 : from 5,000.01 to 6,000.00
20 : from 6,000.01 to 8,000.00
21a: from 8,000.01 to 10,000.00
21b: over 10,000.00</rdfs:comment>
    <rdfs:comment xml:lang="it">Codice della classe di contribuzione degli studenti universitari. Può assumere i valori:
00: contribuzione non prevista (esclusi esoneri)
00a: contribuzione finanziata da enti esterni
01 : da 0,01 a 100,00 (esclusi esoneri)
02 : da 100,01 a 200,00
03 : da 200,01 a 300,00
04 : da 300,01 a 400,00
05 : da 400,01 a 500,00
06 : da 500,01 a 600,00
07 : da 600,01 a 700,00
08 : da 700,01 a 800,00
09 : da 800,01 a 900,00
10 : da 900,01 a 1.000,00
11a: da 1.000,01 a 1.100,00
11b: da 1.100,01 a 1.200,00
11c: da 1.200,01 a 1.300,00
11d: da 1.300,01 a 1.400,00
11e: da 1.400,01 a 1.500,00
12a: da 1.500,01 a 1.600,00
12b: da 1.600,01 a 1.700,00
12c: da 1.700,01 a 1.800,00
12d: da 1.800,01 a 1.900,00
12e: da 1.900,01 a 2.000,00
13 : da 2.000,01 a 2.500,00
14 : da 2.500,01 a 3.000,00
15 : da 3.000,01 a 3.500,00
16 : da 3.500,01 a 4.000,00
17 : da 4.000,01 a 4.500,00
18 : da 4.500,01 a 5.000,00
19 : da 5.000,01 a 6.000,00
20 : da 6.000,01 a 8.000,00
21a: da 8.000,01 a 10.000,00
21b: oltre 10.000,00</rdfs:comment>
    <rdfs:isDefinedBy rdf:resource="https://w3id.org/italia/onto/HER"/>
    <rdfs:label xml:lang="it">ha un contributo per classe</rdfs:label>
    <rdfs:label xml:lang="en">has contribution class</rdfs:label>
    <owl:versionInfo xml:lang="it">stabile</owl:versionInfo>
    <owl:versionInfo xml:lang="en">stable</owl:versionInfo>
  </rdf:Description>
  <rdf:Description rdf:about="https://w3id.org/italia/onto/HER/hasAACTDesign">
    <rdf:type rdf:resource="http://www.w3.org/2002/07/owl#ObjectProperty"/>
    <rdfs:domain rdf:resource="https://w3id.org/italia/onto/HER/AACTStudy"/>
    <rdfs:range rdf:resource="https://w3id.org/italia/onto/HER/AACTDesign"/>
    <rdfs:comment xml:lang="it">I metodi di indagine e le strategie utilizzate nello studio clinico. Una descrizione delle modalità di conduzione dello studio clinico</rdfs:comment>
    <rdfs:comment xml:lang="en">The investigative methods and strategies used in the clinical study. A description of the manner in which the clinical trial will be conducted</rdfs:comment>
    <rdfs:isDefinedBy rdf:resource="https://w3id.org/italia/onto/HER"/>
    <rdfs:label xml:lang="it">ha sviluppo AACT</rdfs:label>
    <rdfs:label xml:lang="en">has AACT design</rdfs:label>
    <owl:versionInfo xml:lang="it">stabile</owl:versionInfo>
    <owl:versionInfo xml:lang="en">stable</owl:versionInfo>
  </rdf:Description>
  <rdf:Description rdf:about="https://w3id.org/italia/onto/HER/leadOrCollaborator">
    <rdf:type rdf:resource="http://www.w3.org/2002/07/owl#DatatypeProperty"/>
    <rdfs:domain rdf:resource="https://w3id.org/italia/onto/HER/AACTSponsor"/>
    <rdfs:range rdf:nodeID="n5bb3bff42afb4ca286d2c3fead9507ddb183"/>
    <rdfs:comment xml:lang="en">If entity is considered to lead the trial or is a Collaborator (ie, other organizationsoproviding support; support may include funding, design, implementation, data analysis or reporting. The responsible party is responsible for confirming all collaborators).</rdfs:comment>
    <rdfs:comment xml:lang="it">Se l'entità è considerata a capo della sperimentazione o è un Collaboratore (cioè un'altra organizzazione che fornisce supporto; il supporto può includere il finanziamento, la progettazione, l'implementazione, l'analisi dei dati o il reporting. Il responsabile è responsabile della conferma di tutti i collaboratori).</rdfs:comment>
    <rdfs:isDefinedBy rdf:resource="https://w3id.org/italia/onto/HER"/>
    <rdfs:label xml:lang="it">capo o collaboratore</rdfs:label>
    <rdfs:label xml:lang="en">lead or collaborator</rdfs:label>
    <owl:versionInfo xml:lang="it">prova</owl:versionInfo>
    <owl:versionInfo xml:lang="en">testing</owl:versionInfo>
  </rdf:Description>
  <rdf:Description rdf:about="https://w3id.org/italia/onto/HER/EUREKAParticipant">
    <rdf:type rdf:resource="http://www.w3.org/2002/07/owl#Class"/>
    <rdfs:subClassOf rdf:resource="https://w3id.org/italia/onto/RO/TimeIndexedRole"/>
    <rdfs:subClassOf rdf:nodeID="n5bb3bff42afb4ca286d2c3fead9507ddb461"/>
    <rdfs:subClassOf rdf:nodeID="n5bb3bff42afb4ca286d2c3fead9507ddb462"/>
    <rdfs:subClassOf rdf:nodeID="n5bb3bff42afb4ca286d2c3fead9507ddb463"/>
    <rdfs:comment xml:lang="it">Partecipanti in progetto EUREKA</rdfs:comment>
    <rdfs:comment xml:lang="en">Participant in a EUREKA project</rdfs:comment>
    <rdfs:isDefinedBy rdf:resource="https://w3id.org/italia/onto/HER"/>
    <rdfs:label xml:lang="en">EUREKA Participant</rdfs:label>
    <rdfs:label xml:lang="it">Partecipante EUREKA</rdfs:label>
    <owl:versionInfo xml:lang="it">stabile</owl:versionInfo>
    <owl:versionInfo xml:lang="en">stable</owl:versionInfo>
  </rdf:Description>
  <rdf:Description rdf:about="https://w3id.org/italia/onto/HER/producesPatent">
    <rdf:type rdf:resource="http://www.w3.org/2002/07/owl#ObjectProperty"/>
    <rdfs:subPropertyOf rdf:resource="https://w3id.org/italia/onto/HER/hasResult"/>
    <rdfs:domain rdf:resource="https://w3id.org/italia/onto/COV/Organization"/>
    <rdfs:range rdf:resource="https://w3id.org/italia/onto/HER/Patent"/>
    <rdfs:comment xml:lang="it">Questa proprietà collega un'organizzazione con un brevetto.</rdfs:comment>
    <rdfs:comment xml:lang="en">This property links an organization with a patent.</rdfs:comment>
    <rdfs:isDefinedBy rdf:resource="https://w3id.org/italia/onto/HER"/>
    <rdfs:label xml:lang="it">brevetto prodotto da</rdfs:label>
    <rdfs:label xml:lang="en">produces patent</rdfs:label>
    <owl:versionInfo xml:lang="it">stabile</owl:versionInfo>
    <owl:versionInfo xml:lang="en">stable</owl:versionInfo>
  </rdf:Description>
  <rdf:Description rdf:about="https://w3id.org/italia/onto/HER/cooperativeClassificationLabel">
    <rdf:type rdf:resource="http://www.w3.org/2002/07/owl#DatatypeProperty"/>
  </rdf:Description>
  <rdf:Description rdf:about="https://w3id.org/italia/onto/HER/ResearcherSeniorityGrade">
    <rdf:type rdf:resource="http://www.w3.org/2002/07/owl#Class"/>
    <rdfs:subClassOf rdf:resource="https://w3id.org/italia/onto/RO/Role"/>
    <rdfs:comment xml:lang="it">La classificazione dell'UNESCO di professionisti impegnati nella concezione o nella creazione di nuove conoscenze (che conducono ricerche e migliorano o sviluppano concetti, teorie, modelli, tecniche di strumentazione, software o metodi operativi) in base ai livelli di anzianità. Si propone di utilizzare la seguente classificazione dei gradi / livelli di anzianità: Categoria A: il singolo voto / posto più alto in cui viene normalmente condotta la ricerca. Esempi: "Direttore della ricerca" o "Professore ordinario" Categoria B: Ricercatori che lavorano in posizioni non più alte della posizione più alta (A) ma più senior rispetto ai neolaureati qualificati (livello ISCED 8). Esempi: "Ricercatore senior" o "Ricercatore principale" o "Professore associato". Categoria C: il primo grado / posto in cui verrebbe normalmente assunto un dottorato di ricerca appena qualificato. Esempi: "Ricercatore" o "Investigatore" o "Ricercatore" o "Dottorando post-dottorato". Categoria D: Studenti di dottorato di livello CITE 8 impegnati come ricercatori o ricercatori che lavorano in posti che normalmente non richiedono un dottorato. Esempi: "dottorandi" o "ricercatori junior" (senza dottorato di ricerca). Anche gli studenti del Master che sono considerati ricercatori rientrerebbero in questa categoria.</rdfs:comment>
    <rdfs:comment xml:lang="en">UNESCO's clasification of professionals engaged in the conception or creation of new knowledge (who conduct research and improve or develop concepts, theories, models, techniques instrumentation, software or operational methods) by the seniority levels. It is proposed to use the following classification of seniority grades/levels: Category A: The single highest grade/post at which research is normally conducted. Examples: "Director of research" or "Full professor" Category B: Researchers working in positions not as senior as top position (A) but more senior than newly qualified doctoral graduates (ISCED level 8). Examples: "Senior researcher" or "Principal investigator" or "Associate professor". Category C: The first grade/post into which a newly qualified doctoral graduate would normally be recruited. Examples: "Researcher" or "Investigator" or "Assistant professor" or "Post-doctoral fellow". Category D: Either doctoral students at the ISCED level 8 who are engaged as researchers, or researchers working in posts that do not normally require a doctorate degree. Examples: "Ph.D. students" or "Junior researchers" (without a Ph.D.). Master’s students who are counted as researchers would also fall under this category.</rdfs:comment>
    <rdfs:isDefinedBy rdf:resource="https://w3id.org/italia/onto/HER"/>
    <rdfs:label xml:lang="it">Anzianità ricercatore</rdfs:label>
    <rdfs:label xml:lang="en">Researcher Seniority Grade</rdfs:label>
    <owl:versionInfo xml:lang="it">stabile</owl:versionInfo>
    <owl:versionInfo xml:lang="en">stable</owl:versionInfo>
  </rdf:Description>
  <rdf:Description rdf:about="https://w3id.org/italia/onto/HER/ctnprinOperationReportedCost">
    <rdf:type rdf:resource="http://www.w3.org/2002/07/owl#DatatypeProperty"/>
    <rdfs:subPropertyOf rdf:resource="https://w3id.org/italia/onto/MU/value"/>
    <rdfs:domain rdf:resource="https://w3id.org/italia/onto/HER/CTNPRINOperation"/>
    <rdfs:range rdf:resource="http://www.w3.org/2001/XMLSchema#decimal"/>
    <rdfs:comment xml:lang="it">Costi rendicontati dal beneficiario a cui fa capo l'operazione rispetto ai costi ammessi. Calcolati come somma dell'omologa variabile "reportedCost" presente a livello di aggregazione inferiore (reportedCost_amounts)</rdfs:comment>
    <rdfs:comment xml:lang="en">Costs reported by the beneficiary to which the operation relates in relation to the eligible costs. Calculated as the sum of the homologous variable 'reportedCost' present at the lower aggregation level (reportedCost_amounts)</rdfs:comment>
    <rdfs:isDefinedBy rdf:resource="https://w3id.org/italia/onto/HER"/>
    <rdfs:label xml:lang="it">costi rendicontati da operazioni CTN/PRIN</rdfs:label>
    <rdfs:label xml:lang="en">reported cost of CTN/PRIN operation</rdfs:label>
    <owl:versionInfo xml:lang="it">stabile</owl:versionInfo>
    <owl:versionInfo xml:lang="en">stable</owl:versionInfo>
  </rdf:Description>
  <rdf:Description rdf:about="https://w3id.org/italia/onto/HER/hasErasmusplusProjectResult">
    <rdf:type rdf:resource="http://www.w3.org/2002/07/owl#ObjectProperty"/>
    <rdfs:subPropertyOf rdf:resource="https://w3id.org/italia/onto/HER/hasResult"/>
    <rdfs:domain rdf:resource="https://w3id.org/italia/onto/HER/ErasmusPlusProject"/>
    <rdfs:range rdf:resource="https://w3id.org/italia/onto/HER/ErasmusPlusProjectResult"/>
    <rdfs:comment xml:lang="en">It is used to link Erasmus+ projects to the output results.</rdfs:comment>
    <rdfs:comment xml:lang="it">Viene utilizzato per collegare i progetti Erasmus+ ai risultati ottenuti.</rdfs:comment>
    <rdfs:isDefinedBy rdf:resource="https://w3id.org/italia/onto/HER"/>
    <rdfs:label xml:lang="it">ha un risultato del progetto Erasmus+</rdfs:label>
    <rdfs:label xml:lang="en">has Erasmus+ project result</rdfs:label>
    <owl:versionInfo xml:lang="it">stabile</owl:versionInfo>
    <owl:versionInfo xml:lang="en">stable</owl:versionInfo>
  </rdf:Description>
  <rdf:Description rdf:nodeID="n5bb3bff42afb4ca286d2c3fead9507ddb75">
    <rdf:first rdf:resource="https://w3id.org/italia/onto/HER/CTNPRINProject"/>
    <rdf:rest rdf:resource="http://www.w3.org/1999/02/22-rdf-syntax-ns#nil"/>
  </rdf:Description>
  <rdf:Description rdf:about="https://w3id.org/italia/onto/HER/REC">
    <rdf:type rdf:resource="http://www.w3.org/2002/07/owl#NamedIndividual"/>
    <rdf:type rdf:resource="https://w3id.org/italia/onto/HER/ECActivityType"/>
    <rdfs:isDefinedBy rdf:resource="https://w3id.org/italia/onto/HER"/>
    <rdfs:label xml:lang="en">Research Organisations</rdfs:label>
    <owl:versionInfo xml:lang="it">stabile</owl:versionInfo>
    <owl:versionInfo xml:lang="en">stable</owl:versionInfo>
  </rdf:Description>
  <rdf:Description rdf:about="https://w3id.org/italia/onto/HER/MIURStudentsByDegreeDegreeClassAggregate">
    <rdf:type rdf:resource="http://www.w3.org/2002/07/owl#Class"/>
    <rdfs:subClassOf rdf:resource="https://w3id.org/italia/onto/HER/StatisticalDataAggregation"/>
    <rdfs:comment xml:lang="en">Aggregated data on Italian students filed in the MIUR system, grouped by year, university, citizenship and degree class.</rdfs:comment>
    <rdfs:comment xml:lang="it">Dati aggregati sugli studenti italiani archiviati nel sistema MIUR, raggruppati per anno, università, cittadinanza e classe di laurea.</rdfs:comment>
    <rdfs:isDefinedBy rdf:resource="https://w3id.org/italia/onto/HER"/>
    <rdfs:label xml:lang="en">Aggregate of Italian Students By Degree and Degree Class</rdfs:label>
    <rdfs:label xml:lang="it">Aggregazione dei studenti italiani per laurea e classe di laurea</rdfs:label>
    <owl:versionInfo xml:lang="it">stabile</owl:versionInfo>
    <owl:versionInfo xml:lang="en">stable</owl:versionInfo>
  </rdf:Description>
  <rdf:Description rdf:about="https://w3id.org/italia/onto/HER/USTATContributionClass">
    <rdf:type rdf:resource="http://www.w3.org/2002/07/owl#Class"/>
    <rdfs:subClassOf rdf:resource="https://w3id.org/italia/onto/l0/Characteristic"/>
    <rdfs:subClassOf rdf:nodeID="n5bb3bff42afb4ca286d2c3fead9507ddb527"/>
    <rdfs:comment xml:lang="en">Data on university student contribution classes.</rdfs:comment>
    <rdfs:comment xml:lang="it">Dati relativi alle classi di contribuzione degli studenti universitari.</rdfs:comment>
    <rdfs:isDefinedBy rdf:resource="https://w3id.org/italia/onto/HER"/>
    <rdfs:label xml:lang="it">Classe di contribuzione USTAT</rdfs:label>
    <rdfs:label xml:lang="en">USTAT Reported Contribution Class</rdfs:label>
    <owl:versionInfo xml:lang="it">stabile</owl:versionInfo>
    <owl:versionInfo xml:lang="en">stable</owl:versionInfo>
  </rdf:Description>
  <rdf:Description rdf:nodeID="n5bb3bff42afb4ca286d2c3fead9507ddb525">
    <rdf:type rdf:resource="http://www.w3.org/2002/07/owl#Restriction"/>
    <owl:onProperty rdf:resource="https://w3id.org/italia/onto/COV/hasOrganization"/>
    <owl:maxQualifiedCardinality rdf:datatype="http://www.w3.org/2001/XMLSchema#nonNegativeInteger">1</owl:maxQualifiedCardinality>
    <owl:onClass rdf:resource="https://w3id.org/italia/onto/COV/Organization"/>
  </rdf:Description>
  <rdf:Description rdf:nodeID="n5bb3bff42afb4ca286d2c3fead9507ddb173">
    <rdf:first rdf:resource="https://w3id.org/italia/onto/HER/ErasmusPlusProject"/>
    <rdf:rest rdf:resource="http://www.w3.org/1999/02/22-rdf-syntax-ns#nil"/>
  </rdf:Description>
  <rdf:Description rdf:about="https://w3id.org/italia/onto/HER/ASJCSupergroup">
    <rdf:type rdf:resource="http://www.w3.org/2002/07/owl#Class"/>
    <rdfs:subClassOf rdf:resource="https://w3id.org/italia/onto/HER/ASJC"/>
    <rdfs:isDefinedBy rdf:resource="https://w3id.org/italia/onto/HER"/>
    <owl:versionInfo xml:lang="it">stabile</owl:versionInfo>
    <owl:versionInfo xml:lang="en">stable</owl:versionInfo>
    <ns6:wasDerivedFrom rdf:resource="http://www.w3.org/2004/02/skos/core#Concept"/>
    <ns4:controlledVocabulary rdf:resource="https://w3id.org/italia/controlled-vocabulary/classifications-for-universities/all-science-journal"/>
  </rdf:Description>
  <rdf:Description rdf:about="https://w3id.org/italia/onto/HER/ctnprinInitiativeCommittedContribution">
    <rdf:type rdf:resource="http://www.w3.org/2002/07/owl#DatatypeProperty"/>
    <rdfs:subPropertyOf rdf:resource="https://w3id.org/italia/onto/MU/value"/>
    <rdfs:domain rdf:resource="https://w3id.org/italia/onto/HER/CTNPRINInitiative"/>
    <rdfs:range rdf:resource="http://www.w3.org/2001/XMLSchema#decimal"/>
    <rdfs:comment xml:lang="en">Total contributions committed by the Ministry on eligible costs following ex-ante evaluation. Calculated as the sum of the homologous variable "committedContribution" present at the lower aggregation level (committedContribution_operations)</rdfs:comment>
    <rdfs:comment xml:lang="it">Totale dei contributi impegnati dal Ministero sui costi ammessi a seguito di valutazione ex-ante. Calcolati come somma dell'omologa variabile "committedContribution" presente a livello di aggregazione inferiore (committedContribution_operations)</rdfs:comment>
    <rdfs:isDefinedBy rdf:resource="https://w3id.org/italia/onto/HER"/>
    <rdfs:label xml:lang="en">committed contribution of CTN/PRIN initiative</rdfs:label>
    <rdfs:label xml:lang="it">contributi impiegati per iniziative CTN/PRIN</rdfs:label>
    <owl:versionInfo xml:lang="it">stabile</owl:versionInfo>
    <owl:versionInfo xml:lang="en">stable</owl:versionInfo>
  </rdf:Description>
  <rdf:Description rdf:nodeID="n5bb3bff42afb4ca286d2c3fead9507ddb135">
    <rdf:type rdf:resource="http://www.w3.org/1999/02/22-rdf-syntax-ns#List"/>
    <rdf:first>Randomized</rdf:first>
    <rdf:rest rdf:resource="http://www.w3.org/1999/02/22-rdf-syntax-ns#nil"/>
  </rdf:Description>
  <rdf:Description rdf:nodeID="n5bb3bff42afb4ca286d2c3fead9507ddb221">
    <rdf:first rdf:resource="https://w3id.org/italia/onto/HER/MIURStudentsByCitizenshipDegreeAggregate"/>
    <rdf:rest rdf:nodeID="n5bb3bff42afb4ca286d2c3fead9507ddb222"/>
  </rdf:Description>
  <rdf:Description rdf:about="https://w3id.org/italia/onto/HER/ECClassification">
    <rdf:type rdf:resource="http://www.w3.org/2002/07/owl#Class"/>
    <rdfs:subClassOf rdf:resource="https://w3id.org/italia/onto/HER/HERClassification"/>
    <rdfs:isDefinedBy rdf:resource="https://w3id.org/italia/onto/HER"/>
    <rdfs:label xml:lang="it">Classificazione CE</rdfs:label>
    <rdfs:label xml:lang="en">EC Classification</rdfs:label>
    <owl:versionInfo xml:lang="it">stabile</owl:versionInfo>
    <owl:versionInfo xml:lang="en">stable</owl:versionInfo>
    <ns6:wasDerivedFrom rdf:resource="http://www.w3.org/2004/02/skos/core#ConceptScheme"/>
  </rdf:Description>
  <rdf:Description rdf:nodeID="n5bb3bff42afb4ca286d2c3fead9507ddb515">
    <rdf:type rdf:resource="http://www.w3.org/2002/07/owl#Restriction"/>
    <owl:onProperty rdf:resource="https://w3id.org/italia/onto/HER/hasFoundationYear"/>
    <owl:qualifiedCardinality rdf:datatype="http://www.w3.org/2001/XMLSchema#nonNegativeInteger">1</owl:qualifiedCardinality>
    <owl:onClass rdf:resource="https://w3id.org/italia/onto/TI/Year"/>
  </rdf:Description>
  <rdf:Description rdf:about="https://w3id.org/italia/onto/HER/founderCapital">
    <rdf:type rdf:resource="http://www.w3.org/2002/07/owl#DatatypeProperty"/>
    <rdfs:domain rdf:resource="https://w3id.org/italia/onto/HER/Spinoff"/>
    <rdfs:range rdf:resource="http://www.w3.org/2000/01/rdf-schema#Literal"/>
    <rdfs:comment xml:lang="it">Indica il capitale dello spin-off al momento della sua fondazione.</rdfs:comment>
    <rdfs:comment xml:lang="en">It indicates the capital of the spin-off at the time of its foundation.</rdfs:comment>
    <rdfs:isDefinedBy rdf:resource="https://w3id.org/italia/onto/HER"/>
    <rdfs:label xml:lang="it">capitale fondatore</rdfs:label>
    <rdfs:label xml:lang="en">founder capital</rdfs:label>
    <owl:versionInfo xml:lang="it">stabile</owl:versionInfo>
    <owl:versionInfo xml:lang="en">stable</owl:versionInfo>
  </rdf:Description>
  <rdf:Description rdf:about="https://w3id.org/italia/onto/HER/ipdAccessCriterion">
    <rdf:type rdf:resource="http://www.w3.org/2002/07/owl#DatatypeProperty"/>
    <rdfs:domain rdf:resource="https://w3id.org/italia/onto/HER/AACTStudy"/>
    <rdfs:range rdf:resource="http://www.w3.org/2000/01/rdf-schema#Literal"/>
    <rdfs:comment xml:lang="en">Describe by what access criteria IPD and any additional supporting information will be shared, including with whom, for what types of analyses, and by what mechanism. Information about who will review requests and criteria for reviewing requests may also be provided.</rdfs:comment>
    <rdfs:comment xml:lang="it">Descrivere in base a quali criteri di accesso IPD ed eventuali informazioni di supporto aggiuntive saranno condivise, anche con chi, per quali tipi di analisi e con quale meccanismo. Possono essere fornite anche informazioni su chi esaminerà le richieste e sui criteri di revisione delle richieste.</rdfs:comment>
    <rdfs:isDefinedBy rdf:resource="https://w3id.org/italia/onto/HER"/>
    <rdfs:label xml:lang="en">IPD access criterion</rdfs:label>
    <rdfs:label xml:lang="it">criterio accesso IPD</rdfs:label>
    <owl:versionInfo xml:lang="it">provvisoria - valutazione dell'introduzione della classe Criterio allineata con il vocabolario europeo Core Criterion e Core Evidence del programma ISA2</owl:versionInfo>
    <owl:versionInfo xml:lang="en">unstable - evalutaion of the possibility to introduce a Criterion class aligned with teh Core Criterion and Core Evidence vocabulary of the ISA2 programme.</owl:versionInfo>
  </rdf:Description>
  <rdf:Description rdf:nodeID="n5bb3bff42afb4ca286d2c3fead9507ddb202">
    <rdf:first rdf:resource="https://w3id.org/italia/onto/HER/MIURStudentsByProvinceOfResidenceDegreeDegreeClassAggregate"/>
    <rdf:rest rdf:nodeID="n5bb3bff42afb4ca286d2c3fead9507ddb203"/>
  </rdf:Description>
  <rdf:Description rdf:about="https://w3id.org/italia/onto/HER/numberOfGraduatedStudents">
    <rdf:type rdf:resource="http://www.w3.org/2002/07/owl#DatatypeProperty"/>
    <rdfs:domain rdf:nodeID="n5bb3bff42afb4ca286d2c3fead9507ddb205"/>
    <rdfs:range rdf:resource="http://www.w3.org/2001/XMLSchema#int"/>
    <rdfs:comment xml:lang="en">Number of students with a degree in the Italian education system.</rdfs:comment>
    <rdfs:comment xml:lang="it">Numero di studenti laureati nel sistema educativo italiano.</rdfs:comment>
    <rdfs:isDefinedBy rdf:resource="https://w3id.org/italia/onto/HER"/>
    <rdfs:label xml:lang="en">number of graduated students</rdfs:label>
    <rdfs:label xml:lang="it">numero di studenti laureati</rdfs:label>
    <owl:versionInfo xml:lang="it">stabile</owl:versionInfo>
    <owl:versionInfo xml:lang="en">stable</owl:versionInfo>
  </rdf:Description>
  <rdf:Description rdf:about="https://w3id.org/italia/onto/HER/totalMaleDoctorateGraduated">
    <rdf:type rdf:resource="http://www.w3.org/2002/07/owl#DatatypeProperty"/>
    <rdfs:subPropertyOf rdf:resource="https://w3id.org/italia/onto/MU/value"/>
    <rdfs:domain rdf:resource="https://w3id.org/italia/onto/HER/USTATStudentsBySexAggregate"/>
    <rdfs:range rdf:resource="http://www.w3.org/2000/01/rdf-schema#Literal"/>
    <rdfs:comment xml:lang="en">Information on men PhDs, disaggregated by gender, university, geographical area, course type and field of education and training (ISCED-F 2013). Data available as of calendar year 2012.</rdfs:comment>
    <rdfs:comment xml:lang="it">Informazioni sui dottori di ricerca di genere maschile, disaggregate per genere, ateneo, area geografica, tipo di corso e field of education and training (ISCED-F 2013). Dati disponibili a partire dall’anno solare 2012.</rdfs:comment>
    <rdfs:isDefinedBy rdf:resource="https://w3id.org/italia/onto/HER"/>
    <rdfs:label xml:lang="en">total male doctorate graduated</rdfs:label>
    <rdfs:label xml:lang="it">totale di laurati ad un dottorato di genere maschile</rdfs:label>
    <owl:versionInfo xml:lang="it">stabile</owl:versionInfo>
    <owl:versionInfo xml:lang="en">stable</owl:versionInfo>
  </rdf:Description>
  <rdf:Description rdf:nodeID="n5bb3bff42afb4ca286d2c3fead9507ddb464">
    <rdf:type rdf:resource="http://www.w3.org/2002/07/owl#Restriction"/>
    <owl:onProperty rdf:resource="https://w3id.org/italia/onto/HER/hasEUREKAParticipant"/>
    <owl:someValuesFrom rdf:resource="https://w3id.org/italia/onto/HER/EUREKAParticipant"/>
  </rdf:Description>
  <rdf:Description rdf:about="https://w3id.org/italia/onto/HER/ctnprinAmountCommittedContribution">
    <rdf:type rdf:resource="http://www.w3.org/2002/07/owl#DatatypeProperty"/>
    <rdfs:subPropertyOf rdf:resource="https://w3id.org/italia/onto/MU/value"/>
    <rdfs:domain rdf:resource="https://w3id.org/italia/onto/HER/CTNPRINAmount"/>
    <rdfs:range rdf:resource="http://www.w3.org/2001/XMLSchema#decimal"/>
    <rdfs:comment xml:lang="en">Contribution committed by the Ministry on the eligible costs per single expense item following ex-ante evaluation</rdfs:comment>
    <rdfs:comment xml:lang="it">Contributo impegnato dal Ministero sui costi ammessi per singola voce di spesa a seguito di valutazione ex-ante</rdfs:comment>
    <rdfs:isDefinedBy rdf:resource="https://w3id.org/italia/onto/HER"/>
    <rdfs:label xml:lang="en">committed contribution of CTN/PRIN amount</rdfs:label>
    <rdfs:label xml:lang="it">contributo impegnato dell'importo CTN/PRIN</rdfs:label>
    <owl:versionInfo xml:lang="it">stabile</owl:versionInfo>
    <owl:versionInfo xml:lang="en">stable</owl:versionInfo>
  </rdf:Description>
  <rdf:Description rdf:nodeID="n5bb3bff42afb4ca286d2c3fead9507ddb27">
    <rdf:first rdf:resource="https://w3id.org/italia/onto/HER/MIURStudentsByDiplomaDegreeDegreeClassAggregate"/>
    <rdf:rest rdf:nodeID="n5bb3bff42afb4ca286d2c3fead9507ddb28"/>
  </rdf:Description>
  <rdf:Description rdf:nodeID="n5bb3bff42afb4ca286d2c3fead9507ddb136">
    <rdf:type rdf:resource="http://www.w3.org/2000/01/rdf-schema#Datatype"/>
    <owl:oneOf rdf:nodeID="n5bb3bff42afb4ca286d2c3fead9507ddb137"/>
  </rdf:Description>
  <rdf:Description rdf:nodeID="n5bb3bff42afb4ca286d2c3fead9507ddb472">
    <rdf:type rdf:resource="http://www.w3.org/2002/07/owl#Restriction"/>
    <owl:onProperty rdf:resource="https://w3id.org/italia/onto/HER/unicsId"/>
    <owl:cardinality rdf:datatype="http://www.w3.org/2001/XMLSchema#nonNegativeInteger">1</owl:cardinality>
  </rdf:Description>
  <rdf:Description rdf:nodeID="n5bb3bff42afb4ca286d2c3fead9507ddb509">
    <rdf:type rdf:resource="http://www.w3.org/2002/07/owl#Restriction"/>
    <owl:onProperty rdf:resource="https://w3id.org/italia/onto/HER/abstract"/>
    <owl:someValuesFrom rdf:resource="http://www.w3.org/2000/01/rdf-schema#Literal"/>
  </rdf:Description>
  <rdf:Description rdf:nodeID="n5bb3bff42afb4ca286d2c3fead9507ddb31">
    <rdf:first rdf:resource="https://w3id.org/italia/onto/HER/MIURStudentsByRegionOfResidenceDegreeDegreeClassAggregate"/>
    <rdf:rest rdf:resource="http://www.w3.org/1999/02/22-rdf-syntax-ns#nil"/>
  </rdf:Description>
  <rdf:Description rdf:nodeID="n5bb3bff42afb4ca286d2c3fead9507ddb122">
    <rdf:type rdf:resource="http://www.w3.org/2002/07/owl#Class"/>
    <owl:unionOf rdf:nodeID="n5bb3bff42afb4ca286d2c3fead9507ddb123"/>
  </rdf:Description>
  <rdf:Description rdf:about="https://w3id.org/italia/onto/HER/ERCGrantType">
    <rdf:type rdf:resource="http://www.w3.org/2002/07/owl#Class"/>
    <rdfs:subClassOf rdf:resource="https://w3id.org/italia/onto/l0/Characteristic"/>
    <rdfs:subClassOf rdf:nodeID="n5bb3bff42afb4ca286d2c3fead9507ddb457"/>
    <rdfs:subClassOf rdf:nodeID="n5bb3bff42afb4ca286d2c3fead9507ddb458"/>
    <rdfs:comment xml:lang="it">Tipo di finanziamento dell'European Research Council - ERC. Le sovvenzioni dell'ERC sono suddivise in 6 tipi: Sovvenzione di avviamento, Sovvenzione per la sinergia, Sovvenzione per il consolidamento, Sovvenzione per il sostegno, Sovvenzione per la prova di un concetto e Sovvenzione per la fase avanzata. Si tratta di contributi finanziari diretti donati dal bilancio del ERC per finanziare le attività.</rdfs:comment>
    <rdfs:comment xml:lang="en">Type of ERC funding. ERC grants are divided in 6 types: Starting Grant, Synergy Grant, Consolidator Grant, Support, Proof of Concept Grant and Advanced Grant. These are direct financial contributions donated from the ERC budget in order to finance activities.</rdfs:comment>
    <rdfs:isDefinedBy rdf:resource="https://w3id.org/italia/onto/HER"/>
    <rdfs:label xml:lang="en">ERC Grant Type</rdfs:label>
    <rdfs:label xml:lang="it">Tipo Contributo ERC</rdfs:label>
    <owl:versionInfo xml:lang="it">stabile</owl:versionInfo>
    <owl:versionInfo xml:lang="en">stable</owl:versionInfo>
  </rdf:Description>
  <rdf:Description rdf:about="https://w3id.org/italia/onto/HER/CHAFEAOutput">
    <rdf:type rdf:resource="http://www.w3.org/2002/07/owl#Class"/>
    <rdfs:subClassOf rdf:resource="https://w3id.org/italia/onto/HER/Result"/>
    <rdfs:subClassOf rdf:nodeID="n5bb3bff42afb4ca286d2c3fead9507ddb399"/>
    <rdfs:comment xml:lang="it">Ouput prodotto da un'attività finanziata. I diversi tipi di output sono: "Dimostratore, pilota, prototipo", "Documento, rapporti...", "Siti web, compilazione di brevetti, video ecc.</rdfs:comment>
    <rdfs:comment xml:lang="en">Ouput produced by a funded activity. The different types of outputs are: "Demonstrator, pilot, prototype", "Document, reports...", "Websites, patent filling, videos etc" and "Other".</rdfs:comment>
    <rdfs:isDefinedBy rdf:resource="https://w3id.org/italia/onto/HER"/>
    <rdfs:label xml:lang="en">CHAFEA Project's Output</rdfs:label>
    <rdfs:label xml:lang="it">Risultato progetto CHAFEA</rdfs:label>
    <owl:versionInfo xml:lang="it">stabile</owl:versionInfo>
    <owl:versionInfo xml:lang="en">stable</owl:versionInfo>
  </rdf:Description>
  <rdf:Description rdf:nodeID="n5bb3bff42afb4ca286d2c3fead9507ddb264">
    <rdf:type rdf:resource="http://www.w3.org/1999/02/22-rdf-syntax-ns#List"/>
    <rdf:first>Treatment</rdf:first>
    <rdf:rest rdf:resource="http://www.w3.org/1999/02/22-rdf-syntax-ns#nil"/>
  </rdf:Description>
  <rdf:Description rdf:nodeID="n5bb3bff42afb4ca286d2c3fead9507ddb172">
    <rdf:first rdf:resource="https://w3id.org/italia/onto/HER/EUREKAProject"/>
    <rdf:rest rdf:nodeID="n5bb3bff42afb4ca286d2c3fead9507ddb173"/>
  </rdf:Description>
  <rdf:Description rdf:about="https://w3id.org/italia/onto/HER/WIPOIPCClass">
    <rdf:type rdf:resource="http://www.w3.org/2002/07/owl#Class"/>
    <rdfs:subClassOf rdf:resource="https://w3id.org/italia/onto/HER/InternationalPatentClassification"/>
    <rdfs:comment xml:lang="en">In each classification symbol, the section (first letter) combined with a two digit number represents the "class".</rdfs:comment>
    <rdfs:comment xml:lang="it">In ogni simbolo di classificazione, la sezione (prima lettera) combinata con un numero di due cifre rappresenta la "classe".</rdfs:comment>
    <rdfs:isDefinedBy rdf:resource="https://w3id.org/italia/onto/HER"/>
    <rdfs:label xml:lang="it">Classe IPC WIPO</rdfs:label>
    <rdfs:label xml:lang="en">WIPO IPC Class</rdfs:label>
    <owl:versionInfo xml:lang="it">stabile</owl:versionInfo>
    <owl:versionInfo xml:lang="en">stable</owl:versionInfo>
    <ns6:wasDerivedFrom rdf:resource="http://www.w3.org/2004/02/skos/core#Concept"/>
  </rdf:Description>
  <rdf:Description rdf:about="https://w3id.org/italia/onto/HER/eurekaOrgType">
    <rdf:type rdf:resource="http://www.w3.org/2002/07/owl#DatatypeProperty"/>
    <rdfs:domain rdf:resource="https://w3id.org/italia/onto/HER/EUREKAParticipant"/>
    <rdfs:range rdf:resource="http://www.w3.org/2000/01/rdf-schema#Literal"/>
    <rdfs:comment xml:lang="it">Tipologia di organizzazione (Istituto di Ricerca, grande impresa, universitá, SME, R&amp;D SME, altro)</rdfs:comment>
    <rdfs:comment xml:lang="en">Type of organization (Research institute, Large company, University, SME, R&amp;D SME, Other)</rdfs:comment>
    <rdfs:isDefinedBy rdf:resource="https://w3id.org/italia/onto/HER"/>
    <rdfs:label xml:lang="en">eureka's organization type</rdfs:label>
    <rdfs:label xml:lang="it">tipologia di organizzazione eureka</rdfs:label>
    <owl:versionInfo xml:lang="it">provvisoria</owl:versionInfo>
    <owl:versionInfo xml:lang="en">unstable</owl:versionInfo>
  </rdf:Description>
  <rdf:Description rdf:about="https://w3id.org/italia/onto/HER/PatentPriorityDetail">
    <rdf:type rdf:resource="http://www.w3.org/2002/07/owl#Class"/>
    <rdfs:subClassOf rdf:resource="https://w3id.org/italia/onto/l0/Description"/>
    <rdfs:subClassOf rdf:nodeID="n5bb3bff42afb4ca286d2c3fead9507ddb503"/>
    <rdfs:subClassOf rdf:nodeID="n5bb3bff42afb4ca286d2c3fead9507ddb504"/>
    <rdfs:comment xml:lang="en">A priority right or right of priority is a time-limited right, triggered by the first filing of an application for a patent. It allows the claimant to file a subsequent application in another country for the same invention as of the date of filing the first application.</rdfs:comment>
    <rdfs:comment xml:lang="it">Un diritto o diritto di priorità prioritario è un diritto limitato nel tempo, innescato dal primo deposito di una domanda di brevetto. Consente al richiedente di presentare una domanda successiva in un altro paese per la stessa invenzione a partire dalla data di deposito della prima domanda.</rdfs:comment>
    <rdfs:isDefinedBy rdf:resource="https://w3id.org/italia/onto/HER"/>
    <rdfs:label xml:lang="it">Dettagli sulla priorità dei brevetti</rdfs:label>
    <rdfs:label xml:lang="en">Patent Priority Details</rdfs:label>
    <owl:versionInfo xml:lang="it">stabile</owl:versionInfo>
    <owl:versionInfo xml:lang="en">stable</owl:versionInfo>
  </rdf:Description>
  <rdf:Description rdf:about="https://w3id.org/italia/onto/HER/forEurekaProject">
    <rdf:type rdf:resource="http://www.w3.org/2002/07/owl#ObjectProperty"/>
    <rdfs:subPropertyOf rdf:resource="https://w3id.org/italia/onto/RO/forEntity"/>
    <rdfs:domain rdf:resource="https://w3id.org/italia/onto/HER/EUREKAParticipant"/>
    <rdfs:range rdf:resource="https://w3id.org/italia/onto/HER/EUREKAProject"/>
    <rdfs:comment xml:lang="it">Questa proprietà collega un partecipante al corrispondente progetto EUREKA.</rdfs:comment>
    <rdfs:comment xml:lang="en">This property connects a participant with the corresponding EUREKA project.</rdfs:comment>
    <rdfs:isDefinedBy rdf:resource="https://w3id.org/italia/onto/HER"/>
    <rdfs:label xml:lang="it">partecipa in progetto eureka</rdfs:label>
    <rdfs:label xml:lang="en">participates in eureka project</rdfs:label>
    <owl:versionInfo xml:lang="it">prova</owl:versionInfo>
    <owl:versionInfo xml:lang="en">testing</owl:versionInfo>
  </rdf:Description>
  <rdf:Description rdf:nodeID="n5bb3bff42afb4ca286d2c3fead9507ddb203">
    <rdf:first rdf:resource="https://w3id.org/italia/onto/HER/MIURStudentsByRegionOfResidenceAggregate"/>
    <rdf:rest rdf:nodeID="n5bb3bff42afb4ca286d2c3fead9507ddb204"/>
  </rdf:Description>
  <rdf:Description rdf:nodeID="n5bb3bff42afb4ca286d2c3fead9507ddb339">
    <rdf:type rdf:resource="http://www.w3.org/2002/07/owl#Class"/>
    <owl:unionOf rdf:nodeID="n5bb3bff42afb4ca286d2c3fead9507ddb340"/>
  </rdf:Description>
  <rdf:Description rdf:about="https://w3id.org/italia/onto/HER/decreeNumber">
    <rdf:type rdf:resource="http://www.w3.org/2002/07/owl#DatatypeProperty"/>
    <rdfs:subPropertyOf rdf:resource="https://w3id.org/italia/onto/l0/identifier"/>
    <rdfs:domain rdf:resource="https://w3id.org/italia/onto/HER/CTNPRINInitiative"/>
    <rdfs:range rdf:resource="http://www.w3.org/2000/01/rdf-schema#Literal"/>
    <rdfs:comment xml:lang="en">Identification number of the MIUR (Ministry of Education, University and Research) decree in which the notice/warning/... which originally defines the initiative in question is published</rdfs:comment>
    <rdfs:comment xml:lang="it">Numero identificativo del decreto MIUR (Ministero dell'Istruzione, dell'Università e della Ricerca) in cui è pubblicato il bando/avviso/... che definisce originariamente l'iniziativa in esame</rdfs:comment>
    <rdfs:isDefinedBy rdf:resource="https://w3id.org/italia/onto/HER"/>
    <rdfs:label xml:lang="en">decree number</rdfs:label>
    <rdfs:label xml:lang="it">numero decreto</rdfs:label>
    <owl:versionInfo xml:lang="it">stabile</owl:versionInfo>
    <owl:versionInfo xml:lang="en">stable</owl:versionInfo>
  </rdf:Description>
  <rdf:Description rdf:nodeID="n5bb3bff42afb4ca286d2c3fead9507ddb155">
    <rdf:type rdf:resource="http://www.w3.org/1999/02/22-rdf-syntax-ns#List"/>
    <rdf:first>R&amp;D</rdf:first>
    <rdf:rest rdf:nodeID="n5bb3bff42afb4ca286d2c3fead9507ddb156"/>
  </rdf:Description>
  <rdf:Description rdf:about="https://w3id.org/italia/onto/HER/AcademicRecruitementField">
    <rdf:type rdf:resource="http://www.w3.org/2002/07/owl#Class"/>
    <rdfs:subClassOf rdf:resource="https://w3id.org/italia/onto/HER/AcademicDiscipline"/>
    <rdfs:isDefinedBy rdf:resource="https://w3id.org/italia/onto/HER"/>
    <owl:versionInfo xml:lang="it">stabile</owl:versionInfo>
    <owl:versionInfo xml:lang="en">stable</owl:versionInfo>
    <ns6:wasDerivedFrom rdf:resource="http://www.w3.org/2004/02/skos/core#Concept"/>
    <ns4:controlledVocabulary rdf:resource="https://w3id.org/italia/controlled-vocabulary/classifications-for-universities/academic-disciplines"/>
  </rdf:Description>
  <rdf:Description rdf:about="https://w3id.org/italia/onto/HER/numberOfEnrolledStudents">
    <rdf:type rdf:resource="http://www.w3.org/2002/07/owl#DatatypeProperty"/>
    <rdfs:domain rdf:nodeID="n5bb3bff42afb4ca286d2c3fead9507ddb192"/>
    <rdfs:range rdf:resource="http://www.w3.org/2001/XMLSchema#int"/>
    <rdfs:comment xml:lang="en">Number of students enrolled in the Italian education system.</rdfs:comment>
    <rdfs:comment xml:lang="it">Numero di studenti iscritti al sistema educativo italiano.</rdfs:comment>
    <rdfs:isDefinedBy rdf:resource="https://w3id.org/italia/onto/HER"/>
    <rdfs:label xml:lang="en">number of enrolled students</rdfs:label>
    <rdfs:label xml:lang="it">numero di studenti iscritti</rdfs:label>
    <owl:versionInfo xml:lang="it">stabile</owl:versionInfo>
    <owl:versionInfo xml:lang="en">stable</owl:versionInfo>
  </rdf:Description>
  <rdf:Description rdf:about="https://w3id.org/italia/onto/COV/PublicOrganization">
    <rdf:type rdf:resource="http://www.w3.org/2002/07/owl#Class"/>
  </rdf:Description>
  <rdf:Description rdf:nodeID="n5bb3bff42afb4ca286d2c3fead9507ddb36">
    <rdf:first rdf:resource="https://w3id.org/italia/onto/HER/AcademicDegree"/>
    <rdf:rest rdf:nodeID="n5bb3bff42afb4ca286d2c3fead9507ddb37"/>
  </rdf:Description>
  <rdf:Description rdf:nodeID="n5bb3bff42afb4ca286d2c3fead9507ddb492">
    <rdf:type rdf:resource="http://www.w3.org/2002/07/owl#Restriction"/>
    <owl:onProperty rdf:resource="https://w3id.org/italia/onto/HER/distributedInErasumplusFile"/>
    <owl:allValuesFrom rdf:resource="https://w3id.org/italia/onto/HER/ErasmusPlusFile"/>
  </rdf:Description>
  <rdf:Description rdf:about="https://w3id.org/italia/data/private-organization/siris">
    <rdf:type rdf:resource="http://www.w3.org/2002/07/owl#NamedIndividual"/>
    <rdf:type rdf:resource="http://dati.gov.it/onto/dcatapit#Agent"/>
    <rdf:type rdf:resource="http://xmlns.com/foaf/0.1/Agent"/>
    <ns2:identifier>siris</ns2:identifier>
    <ns5:name xml:lang="en">SIRIS</ns5:name>
    <ns5:name xml:lang="it">SIRIS</ns5:name>
  </rdf:Description>
  <rdf:Description rdf:about="https://w3id.org/italia/onto/HER/AACTDesign">
    <rdf:type rdf:resource="http://www.w3.org/2002/07/owl#Class"/>
    <rdfs:subClassOf rdf:resource="https://w3id.org/italia/onto/l0/Description"/>
    <rdfs:subClassOf rdf:nodeID="n5bb3bff42afb4ca286d2c3fead9507ddb370"/>
    <rdfs:subClassOf rdf:nodeID="n5bb3bff42afb4ca286d2c3fead9507ddb371"/>
    <rdfs:comment xml:lang="it">I metodi di indagine e le strategie utilizzate nello studio clinico. Una descrizione delle modalità di conduzione dello studio clinico</rdfs:comment>
    <rdfs:comment xml:lang="en">The investigative methods and strategies used in the clinical study. A description of the manner in which the clinical trial will be conducted</rdfs:comment>
    <rdfs:isDefinedBy rdf:resource="https://w3id.org/italia/onto/HER"/>
    <rdfs:label xml:lang="en">AACT Design</rdfs:label>
    <rdfs:label xml:lang="it">Progettazione AACT</rdfs:label>
    <owl:versionInfo xml:lang="it">stabile</owl:versionInfo>
    <owl:versionInfo xml:lang="en">stable</owl:versionInfo>
  </rdf:Description>
  <rdf:Description rdf:nodeID="n5bb3bff42afb4ca286d2c3fead9507ddb350">
    <rdf:first rdf:resource="https://w3id.org/italia/onto/HER/USTATTotallyExoneratedStudentsAggregate"/>
    <rdf:rest rdf:resource="http://www.w3.org/1999/02/22-rdf-syntax-ns#nil"/>
  </rdf:Description>
  <rdf:Description rdf:nodeID="n5bb3bff42afb4ca286d2c3fead9507ddb443">
    <rdf:type rdf:resource="http://www.w3.org/2002/07/owl#Restriction"/>
    <owl:onProperty rdf:resource="https://w3id.org/italia/onto/HER/unicsId"/>
    <owl:cardinality rdf:datatype="http://www.w3.org/2001/XMLSchema#nonNegativeInteger">1</owl:cardinality>
  </rdf:Description>
  <rdf:Description rdf:nodeID="n5bb3bff42afb4ca286d2c3fead9507ddb261">
    <rdf:type rdf:resource="http://www.w3.org/1999/02/22-rdf-syntax-ns#List"/>
    <rdf:first>Prevention</rdf:first>
    <rdf:rest rdf:nodeID="n5bb3bff42afb4ca286d2c3fead9507ddb262"/>
  </rdf:Description>
  <rdf:Description rdf:nodeID="n5bb3bff42afb4ca286d2c3fead9507ddb278">
    <rdf:first rdf:resource="https://w3id.org/italia/onto/HER/EUREKAProject"/>
    <rdf:rest rdf:nodeID="n5bb3bff42afb4ca286d2c3fead9507ddb279"/>
  </rdf:Description>
  <rdf:Description rdf:nodeID="n5bb3bff42afb4ca286d2c3fead9507ddb370">
    <rdf:type rdf:resource="http://www.w3.org/2002/07/owl#Restriction"/>
    <owl:onProperty rdf:resource="https://w3id.org/italia/onto/l0/description"/>
    <owl:someValuesFrom rdf:resource="http://www.w3.org/2000/01/rdf-schema#Literal"/>
  </rdf:Description>
  <rdf:Description rdf:nodeID="n5bb3bff42afb4ca286d2c3fead9507ddb526">
    <rdf:type rdf:resource="http://www.w3.org/2002/07/owl#Restriction"/>
    <owl:onProperty rdf:resource="https://w3id.org/italia/onto/COV/hasOrganization"/>
    <owl:maxQualifiedCardinality rdf:datatype="http://www.w3.org/2001/XMLSchema#nonNegativeInteger">1</owl:maxQualifiedCardinality>
    <owl:onClass rdf:resource="https://w3id.org/italia/onto/COV/Organization"/>
  </rdf:Description>
  <rdf:Description rdf:about="https://w3id.org/italia/onto/HER/initiativeType">
    <rdf:type rdf:resource="http://www.w3.org/2002/07/owl#DatatypeProperty"/>
    <rdfs:domain rdf:resource="https://w3id.org/italia/onto/HER/CTNPRINInitiative"/>
    <rdfs:range rdf:resource="http://www.w3.org/2000/01/rdf-schema#Literal"/>
    <rdfs:comment xml:lang="it">Tipologia dell'iniziativa. La Tipologia di una iniziativa può essere: - Ricerca di base - Ricerca industriale - Diffusione Cultura Scientifica - Antartide - Altro</rdfs:comment>
    <rdfs:comment xml:lang="en">Type of initiative. The typology of an initiative can be: - Basic research - Industrial research - Dissemination of Scientific culture - Antarctica - Other</rdfs:comment>
    <rdfs:isDefinedBy rdf:resource="https://w3id.org/italia/onto/HER"/>
    <rdfs:label xml:lang="en">initiative type</rdfs:label>
    <rdfs:label xml:lang="it">tipi di iniziative</rdfs:label>
    <owl:versionInfo xml:lang="it">provvisoria - controllare i valori controllati della proprietà</owl:versionInfo>
    <owl:versionInfo xml:lang="it">stabile</owl:versionInfo>
    <owl:versionInfo xml:lang="en">stable</owl:versionInfo>
    <owl:versionInfo xml:lang="en">unstable - check the fixed values</owl:versionInfo>
  </rdf:Description>
  <rdf:Description rdf:about="https://w3id.org/italia/onto/HER/birthyear">
    <rdf:type rdf:resource="http://www.w3.org/2002/07/owl#DatatypeProperty"/>
    <rdfs:subPropertyOf rdf:resource="https://w3id.org/italia/onto/TI/year"/>
    <rdfs:domain rdf:resource="https://w3id.org/italia/onto/CPV/Person"/>
    <rdfs:range rdf:resource="http://www.w3.org/2001/XMLSchema#gYear"/>
    <rdfs:comment xml:lang="en">A person's year of birth.</rdfs:comment>
    <rdfs:comment xml:lang="it">L'anno di nascita di una persona.</rdfs:comment>
    <rdfs:isDefinedBy rdf:resource="https://w3id.org/italia/onto/HER"/>
    <rdfs:label xml:lang="it">anno di nascita</rdfs:label>
    <rdfs:label xml:lang="en">birth year</rdfs:label>
    <owl:versionInfo xml:lang="it">provvisoria - valutare di spostare questa proprietà nell'ontologia delle persone CPV</owl:versionInfo>
    <owl:versionInfo xml:lang="en">unstable - evaluate to move this to the Person ontology</owl:versionInfo>
  </rdf:Description>
  <rdf:Description rdf:nodeID="n5bb3bff42afb4ca286d2c3fead9507ddb51">
    <rdf:first rdf:resource="https://w3id.org/italia/onto/HER/ECProject"/>
    <rdf:rest rdf:nodeID="n5bb3bff42afb4ca286d2c3fead9507ddb52"/>
  </rdf:Description>
  <rdf:Description rdf:about="https://w3id.org/italia/onto/HER/CTNPRINProject">
    <rdf:type rdf:resource="http://www.w3.org/2002/07/owl#Class"/>
    <rdfs:subClassOf rdf:resource="https://w3id.org/italia/onto/Project/PublicResearchProject"/>
    <rdfs:comment xml:lang="it">Progetto finanziato da CTN (Cluster Tecnologici Nazionali) o PRIN (Progetti di Ricerca di Interesse Nazionale)</rdfs:comment>
    <rdfs:comment xml:lang="en">Project funded by CTN (Cluster Tecnologici Nazionali) or PRIN (Progetti di Ricerca di Interesse Nazionale)</rdfs:comment>
    <rdfs:isDefinedBy rdf:resource="https://w3id.org/italia/onto/HER"/>
    <rdfs:label xml:lang="en">CTN/PRIN Project</rdfs:label>
    <rdfs:label xml:lang="it">Progetto CTN/PRIN</rdfs:label>
    <owl:versionInfo xml:lang="it">stabile</owl:versionInfo>
    <owl:versionInfo xml:lang="en">stable</owl:versionInfo>
  </rdf:Description>
  <rdf:Description rdf:about="https://w3id.org/italia/onto/HER/hasFoundationYear">
    <rdf:type rdf:resource="http://www.w3.org/2002/07/owl#ObjectProperty"/>
    <rdfs:subPropertyOf rdf:resource="https://w3id.org/italia/onto/TI/hasYear"/>
    <rdfs:domain rdf:resource="https://w3id.org/italia/onto/HER/Spinoff"/>
    <rdfs:range rdf:resource="https://w3id.org/italia/onto/TI/Year"/>
    <rdfs:comment xml:lang="it">Indica l'anno di fondazione dello spin-off.</rdfs:comment>
    <rdfs:comment xml:lang="en">It indicates the year of foundation of the spin-off.</rdfs:comment>
    <rdfs:isDefinedBy rdf:resource="https://w3id.org/italia/onto/HER"/>
    <rdfs:label xml:lang="it">ha anno di fondazione</rdfs:label>
    <rdfs:label xml:lang="en">has foundation year</rdfs:label>
    <owl:versionInfo xml:lang="it">stabile</owl:versionInfo>
    <owl:versionInfo xml:lang="en">stable</owl:versionInfo>
  </rdf:Description>
  <rdf:Description rdf:nodeID="n5bb3bff42afb4ca286d2c3fead9507ddb333">
    <rdf:first rdf:resource="https://w3id.org/italia/onto/HER/USTATPostgraduateAggregateOfEnrolled"/>
    <rdf:rest rdf:nodeID="n5bb3bff42afb4ca286d2c3fead9507ddb334"/>
  </rdf:Description>
  <rdf:Description rdf:about="https://w3id.org/italia/onto/HER/IsPrincipalInvestigatorOf">
    <rdf:type rdf:resource="http://www.w3.org/2002/07/owl#ObjectProperty"/>
    <owl:inverseOf rdf:resource="https://w3id.org/italia/onto/HER/hasPrincipalInvestigator"/>
    <rdfs:domain rdf:resource="https://w3id.org/italia/onto/CPV/Person"/>
    <rdfs:range rdf:resource="https://w3id.org/italia/onto/Project/PublicResearchProject"/>
    <rdfs:comment xml:lang="en">Inverse property of hasPrincipalInvestigator</rdfs:comment>
    <rdfs:comment xml:lang="it">Proprietà inversa di ha esaminatore principale</rdfs:comment>
    <rdfs:isDefinedBy rdf:resource="https://w3id.org/italia/onto/HER"/>
    <rdfs:label xml:lang="en">is principal investigator of</rdfs:label>
    <rdfs:label xml:lang="it">è esaminatore principale di</rdfs:label>
    <owl:versionInfo xml:lang="it">provvisoria - da verificare bene la descrizione</owl:versionInfo>
    <owl:versionInfo xml:lang="en">unstable</owl:versionInfo>
  </rdf:Description>
  <rdf:Description rdf:nodeID="n5bb3bff42afb4ca286d2c3fead9507ddb409">
    <rdf:type rdf:resource="http://www.w3.org/2002/07/owl#Restriction"/>
    <owl:onProperty rdf:resource="https://w3id.org/italia/onto/HER/ecContribution"/>
    <owl:qualifiedCardinality rdf:datatype="http://www.w3.org/2001/XMLSchema#nonNegativeInteger">1</owl:qualifiedCardinality>
    <owl:onDataRange rdf:resource="http://www.w3.org/2001/XMLSchema#decimal"/>
  </rdf:Description>
  <rdf:Description rdf:about="https://w3id.org/italia/onto/HER/ItalianDegree">
    <rdf:type rdf:resource="http://www.w3.org/2002/07/owl#Class"/>
    <rdfs:subClassOf rdf:resource="https://w3id.org/italia/onto/HER/AcademicDegree"/>
    <rdfs:comment xml:lang="en">It is refers to Italian degree qualification that students can award upon successful completion of a course of study in higher education, usually at a college or university.</rdfs:comment>
    <rdfs:comment xml:lang="it">Si riferisce al titolo di studio di laurea italiano che gli studenti possono rilasciare al termine di un corso di studi nell'ambito dell'istruzione superiore, di solito presso un college o un'università.</rdfs:comment>
    <rdfs:isDefinedBy rdf:resource="https://w3id.org/italia/onto/HER"/>
    <rdfs:label xml:lang="en">Italian Degree</rdfs:label>
    <rdfs:label xml:lang="it">Laurea italiana</rdfs:label>
    <owl:versionInfo xml:lang="it">stabile</owl:versionInfo>
    <owl:versionInfo xml:lang="en">stable</owl:versionInfo>
  </rdf:Description>
  <rdf:Description rdf:nodeID="n5bb3bff42afb4ca286d2c3fead9507ddb21">
    <rdf:first rdf:resource="https://w3id.org/italia/onto/HER/MIURStudentsByCitizenshipAggregate"/>
    <rdf:rest rdf:nodeID="n5bb3bff42afb4ca286d2c3fead9507ddb22"/>
  </rdf:Description>
  <rdf:Description rdf:nodeID="n5bb3bff42afb4ca286d2c3fead9507ddb445">
    <rdf:type rdf:resource="http://www.w3.org/2002/07/owl#Restriction"/>
    <owl:onProperty rdf:resource="https://w3id.org/italia/onto/HER/hasECParticipant"/>
    <owl:someValuesFrom rdf:resource="https://w3id.org/italia/onto/HER/ECParticipant"/>
  </rdf:Description>
  <rdf:Description rdf:nodeID="n5bb3bff42afb4ca286d2c3fead9507ddb500">
    <rdf:type rdf:resource="http://www.w3.org/2002/07/owl#Restriction"/>
    <owl:onProperty rdf:resource="https://w3id.org/italia/onto/HER/patentApplicationNo"/>
    <owl:cardinality rdf:datatype="http://www.w3.org/2001/XMLSchema#nonNegativeInteger">1</owl:cardinality>
  </rdf:Description>
  <rdf:Description rdf:about="https://w3id.org/italia/onto/HER/hasCessationYear">
    <rdf:type rdf:resource="http://www.w3.org/2002/07/owl#ObjectProperty"/>
    <rdfs:subPropertyOf rdf:resource="https://w3id.org/italia/onto/TI/hasYear"/>
    <rdfs:domain rdf:resource="https://w3id.org/italia/onto/HER/Spinoff"/>
    <rdfs:range rdf:resource="https://w3id.org/italia/onto/TI/Year"/>
    <rdfs:comment xml:lang="it">Indica l'anno di cessazione dell'attività dello spin-off, se applicabile.</rdfs:comment>
    <rdfs:comment xml:lang="en">It indicates the year of cessation of the spin-off activity, if applicable.</rdfs:comment>
    <rdfs:isDefinedBy rdf:resource="https://w3id.org/italia/onto/HER"/>
    <rdfs:label xml:lang="it">ha anno di cessazione</rdfs:label>
    <rdfs:label xml:lang="en">has cessation year</rdfs:label>
    <owl:versionInfo xml:lang="it">stabile</owl:versionInfo>
    <owl:versionInfo xml:lang="en">stable</owl:versionInfo>
  </rdf:Description>
  <rdf:Description rdf:nodeID="n5bb3bff42afb4ca286d2c3fead9507ddb238">
    <rdf:type rdf:resource="http://www.w3.org/1999/02/22-rdf-syntax-ns#List"/>
    <rdf:first>Defined Population</rdf:first>
    <rdf:rest rdf:nodeID="n5bb3bff42afb4ca286d2c3fead9507ddb239"/>
  </rdf:Description>
  <rdf:Description rdf:nodeID="n5bb3bff42afb4ca286d2c3fead9507ddb120">
    <rdf:first rdf:resource="https://w3id.org/italia/onto/HER/Result"/>
    <rdf:rest rdf:nodeID="n5bb3bff42afb4ca286d2c3fead9507ddb121"/>
  </rdf:Description>
  <rdf:Description rdf:nodeID="n5bb3bff42afb4ca286d2c3fead9507ddb17">
    <rdf:first rdf:resource="https://w3id.org/italia/onto/HER/MIURStudentsByRegionOfResidenceDegreeDegreeClassAggregate"/>
    <rdf:rest rdf:resource="http://www.w3.org/1999/02/22-rdf-syntax-ns#nil"/>
  </rdf:Description>
  <rdf:Description rdf:about="https://w3id.org/italia/onto/HER/hasECFrameworkProgramme">
    <rdf:type rdf:resource="http://www.w3.org/2002/07/owl#ObjectProperty"/>
    <rdfs:domain rdf:nodeID="n5bb3bff42afb4ca286d2c3fead9507ddb41"/>
    <rdfs:range rdf:resource="https://w3id.org/italia/onto/HER/ECFrameworkProgramme"/>
    <rdfs:comment xml:lang="it">Questa proprietà collega un progetto CE con il corrispondente programma quadro.</rdfs:comment>
    <rdfs:comment xml:lang="en">This property links an EC project with the corresponding framework programme.</rdfs:comment>
    <rdfs:isDefinedBy rdf:resource="https://w3id.org/italia/onto/HER"/>
    <rdfs:label xml:lang="it">ha struttura di lavoro CE</rdfs:label>
    <rdfs:label xml:lang="en">has EC framework programme</rdfs:label>
    <owl:versionInfo xml:lang="it">stabile</owl:versionInfo>
    <owl:versionInfo xml:lang="en">stable</owl:versionInfo>
  </rdf:Description>
  <rdf:Description rdf:nodeID="n5bb3bff42afb4ca286d2c3fead9507ddb112">
    <rdf:type rdf:resource="http://www.w3.org/2002/07/owl#Class"/>
    <owl:unionOf rdf:nodeID="n5bb3bff42afb4ca286d2c3fead9507ddb113"/>
  </rdf:Description>
  <rdf:Description rdf:nodeID="n5bb3bff42afb4ca286d2c3fead9507ddb468">
    <rdf:type rdf:resource="http://www.w3.org/2002/07/owl#Restriction"/>
    <owl:onProperty rdf:resource="https://w3id.org/italia/onto/HER/hasEurekaTechArea"/>
    <owl:maxQualifiedCardinality rdf:datatype="http://www.w3.org/2001/XMLSchema#nonNegativeInteger">1</owl:maxQualifiedCardinality>
    <owl:onClass rdf:resource="https://w3id.org/italia/onto/HER/EUREKATechArea"/>
  </rdf:Description>
  <rdf:Description rdf:about="https://w3id.org/italia/onto/HER/AcademicAffiliation">
    <rdf:type rdf:resource="http://www.w3.org/2002/07/owl#Class"/>
    <rdfs:subClassOf rdf:resource="https://w3id.org/italia/onto/COV/Employment"/>
    <rdfs:comment xml:lang="it">Rappresenta l'affiliazione di una persona a un'organizzazione con un determinato ruolo per un periodo di tempo.</rdfs:comment>
    <rdfs:comment xml:lang="en">Represents the affiliation of a person to an organization with a certain role for a period of time.</rdfs:comment>
    <rdfs:isDefinedBy rdf:resource="https://w3id.org/italia/onto/HER"/>
    <rdfs:label xml:lang="en">Academic Affiliation</rdfs:label>
    <rdfs:label xml:lang="it">Affilizazione accademica</rdfs:label>
    <owl:versionInfo xml:lang="it">stabile</owl:versionInfo>
    <owl:versionInfo xml:lang="en">stable</owl:versionInfo>
  </rdf:Description>
  <rdf:Description rdf:nodeID="n5bb3bff42afb4ca286d2c3fead9507ddb289">
    <rdf:type rdf:resource="http://www.w3.org/1999/02/22-rdf-syntax-ns#List"/>
    <rdf:first>Longitudinal</rdf:first>
    <rdf:rest rdf:nodeID="n5bb3bff42afb4ca286d2c3fead9507ddb290"/>
  </rdf:Description>
  <rdf:Description rdf:nodeID="n5bb3bff42afb4ca286d2c3fead9507ddb29">
    <rdf:first rdf:resource="https://w3id.org/italia/onto/HER/MIURStudentsByProvinceOfResidenceDegreeDegreeClassAggregate"/>
    <rdf:rest rdf:nodeID="n5bb3bff42afb4ca286d2c3fead9507ddb30"/>
  </rdf:Description>
  <rdf:Description rdf:nodeID="n5bb3bff42afb4ca286d2c3fead9507ddb473">
    <rdf:type rdf:resource="http://www.w3.org/2002/07/owl#Restriction"/>
    <owl:onProperty rdf:resource="https://w3id.org/italia/onto/HER/endingYear"/>
    <owl:maxQualifiedCardinality rdf:datatype="http://www.w3.org/2001/XMLSchema#nonNegativeInteger">1</owl:maxQualifiedCardinality>
    <owl:onDataRange rdf:resource="http://www.w3.org/2001/XMLSchema#gYear"/>
  </rdf:Description>
  <rdf:Description rdf:nodeID="n5bb3bff42afb4ca286d2c3fead9507ddb331">
    <rdf:first rdf:resource="https://w3id.org/italia/onto/HER/USTATPostgraduateAggregateOfRegistered"/>
    <rdf:rest rdf:resource="http://www.w3.org/1999/02/22-rdf-syntax-ns#nil"/>
  </rdf:Description>
  <rdf:Description rdf:nodeID="n5bb3bff42afb4ca286d2c3fead9507ddb508">
    <rdf:type rdf:resource="http://www.w3.org/2002/07/owl#Restriction"/>
    <owl:onProperty rdf:resource="https://w3id.org/italia/onto/HER/patentKindCode"/>
    <owl:cardinality rdf:datatype="http://www.w3.org/2001/XMLSchema#nonNegativeInteger">1</owl:cardinality>
  </rdf:Description>
  <rdf:Description rdf:about="https://w3id.org/italia/onto/HER/AcademicRole">
    <rdf:type rdf:resource="http://www.w3.org/2002/07/owl#Class"/>
    <rdfs:subClassOf rdf:resource="https://w3id.org/italia/onto/RO/Role"/>
    <rdfs:comment xml:lang="it">Il ruolo che una persona svolge in un'organizzazione accademica.</rdfs:comment>
    <rdfs:comment xml:lang="en">The role a person plays in an academic organization.</rdfs:comment>
    <rdfs:isDefinedBy rdf:resource="https://w3id.org/italia/onto/HER"/>
    <rdfs:label xml:lang="en">Academic role</rdfs:label>
    <rdfs:label xml:lang="it">Ruolo Accademico</rdfs:label>
    <owl:versionInfo xml:lang="it">provvisoria</owl:versionInfo>
    <owl:versionInfo xml:lang="en">unstable</owl:versionInfo>
  </rdf:Description>
  <rdf:Description rdf:about="https://w3id.org/italia/onto/HER/EUREKATechArea">
    <rdf:type rdf:resource="http://www.w3.org/2002/07/owl#Class"/>
    <rdfs:subClassOf rdf:resource="https://w3id.org/italia/onto/HER/HERClassification"/>
    <rdfs:comment xml:lang="it">Area tecnologica EUREKA (Elettronica, IT e tecnologia delle telecomunicazioni; Produzione industriale, materiali e trasporti; Scienze / tecnologie biologiche; Tecnologia per la protezione dell'uomo e dell'ambiente; Tecnologia energetica)</rdfs:comment>
    <rdfs:comment xml:lang="en">EUREKA Tecnological area (Electronics, IT and Telecoms Technology; Industrial Manufacturing, Material and Transport; Biological Sciences / Technologies; Technology for Protecting Man and the Environment; Energy Technology)</rdfs:comment>
    <rdfs:isDefinedBy rdf:resource="https://w3id.org/italia/onto/HER"/>
    <rdfs:label xml:lang="it">Area tecnica EUREKA</rdfs:label>
    <rdfs:label xml:lang="en">EUREKA Tech Area</rdfs:label>
    <owl:versionInfo xml:lang="it">stabile</owl:versionInfo>
    <owl:versionInfo xml:lang="en">stable</owl:versionInfo>
    <ns6:wasDerivedFrom rdf:resource="http://www.w3.org/2004/02/skos/core#Concept"/>
  </rdf:Description>
  <rdf:Description rdf:nodeID="n5bb3bff42afb4ca286d2c3fead9507ddb124">
    <rdf:first rdf:resource="https://w3id.org/italia/onto/HER/USTATAverageContributionsAggregate"/>
    <rdf:rest rdf:nodeID="n5bb3bff42afb4ca286d2c3fead9507ddb125"/>
  </rdf:Description>
  <rdf:Description rdf:about="https://w3id.org/italia/onto/HER/totalForeignMale">
    <rdf:type rdf:resource="http://www.w3.org/2002/07/owl#DatatypeProperty"/>
    <rdfs:subPropertyOf rdf:resource="https://w3id.org/italia/onto/MU/value"/>
    <rdfs:domain rdf:nodeID="n5bb3bff42afb4ca286d2c3fead9507ddb332"/>
    <rdfs:range rdf:resource="http://www.w3.org/2000/01/rdf-schema#Literal"/>
    <rdfs:comment xml:lang="en">Total with respect to the population of men with foreign citizenship of the sample considered.</rdfs:comment>
    <rdfs:comment xml:lang="it">Totale rispetto alla popolazione di sesso maschile e con cittadinanza straniera del campione considerato.</rdfs:comment>
    <rdfs:isDefinedBy rdf:resource="https://w3id.org/italia/onto/HER"/>
    <rdfs:label xml:lang="en">total foreign male</rdfs:label>
    <rdfs:label xml:lang="it">totale di genere maschile straniero</rdfs:label>
    <owl:versionInfo xml:lang="it">stabile</owl:versionInfo>
    <owl:versionInfo xml:lang="en">stable</owl:versionInfo>
  </rdf:Description>
  <rdf:Description rdf:about="https://w3id.org/italia/onto/HER/AACTConditionMeshTerm">
    <rdf:type rdf:resource="http://www.w3.org/2002/07/owl#Class"/>
    <rdfs:subClassOf rdf:resource="https://w3id.org/italia/onto/HER/AACTMeshTerm"/>
    <rdfs:comment xml:lang="it">I nomi della malattia o delle condizioni studiate nello studio clinico, o il focus dello studio clinico. I dati vengono descritti da NLM (Medical Subject Headings - MeSH) - thesaurus del vocabolario controllato o termini da un altro vocabolario, come la Nomenclatura sistematica dei termini medico-clinici (SNOMED CT), che è stato mappato al MeSH all'interno del Metathesaurus Unified Medical Language System (UMLS).

Tradotto con www.DeepL.com/Translator (versione gratuita)</rdfs:comment>
    <rdfs:comment xml:lang="en">The name(s) of the disease(s) or condition(s) studied in the clinical study, or the focus of the clinical study appropriate descriptors from NLM's Medical Subject Headings (MeSH)-controlled vocabulary thesaurus or terms from another vocabulary, such as the Systematized Nomenclature of Medicine—Clinical Terms (SNOMED CT), that has been mapped to MeSH within the Unified Medical Language System (UMLS) Metathesaurus.</rdfs:comment>
    <rdfs:isDefinedBy rdf:resource="https://w3id.org/italia/onto/HER"/>
    <rdfs:label xml:lang="en">Condition Mesh Term</rdfs:label>
    <rdfs:label xml:lang="it">Termine MeSH di Condizione</rdfs:label>
    <owl:versionInfo xml:lang="it">stabile</owl:versionInfo>
    <owl:versionInfo xml:lang="en">stable</owl:versionInfo>
  </rdf:Description>
  <rdf:Description rdf:nodeID="n5bb3bff42afb4ca286d2c3fead9507ddb305">
    <rdf:first rdf:resource="https://w3id.org/italia/onto/HER/USTATContributionByClass"/>
    <rdf:rest rdf:nodeID="n5bb3bff42afb4ca286d2c3fead9507ddb306"/>
  </rdf:Description>
  <rdf:Description rdf:nodeID="n5bb3bff42afb4ca286d2c3fead9507ddb512">
    <rdf:type rdf:resource="http://www.w3.org/2002/07/owl#Restriction"/>
    <owl:onProperty rdf:resource="https://w3id.org/italia/onto/HER/resultType"/>
    <owl:maxCardinality rdf:datatype="http://www.w3.org/2001/XMLSchema#nonNegativeInteger">1</owl:maxCardinality>
  </rdf:Description>
  <rdf:Description rdf:nodeID="n5bb3bff42afb4ca286d2c3fead9507ddb189">
    <rdf:type rdf:resource="http://www.w3.org/1999/02/22-rdf-syntax-ns#List"/>
    <rdf:first>Quadruple</rdf:first>
    <rdf:rest rdf:nodeID="n5bb3bff42afb4ca286d2c3fead9507ddb190"/>
  </rdf:Description>
  <rdf:Description rdf:about="https://w3id.org/italia/onto/HER/USTATReportedPostgraduateCourse">
    <rdf:type rdf:resource="http://www.w3.org/2002/07/owl#Class"/>
    <rdfs:subClassOf rdf:resource="https://w3id.org/italia/onto/l0/Object"/>
    <rdfs:subClassOf rdf:nodeID="n5bb3bff42afb4ca286d2c3fead9507ddb536"/>
    <rdfs:comment xml:lang="it">Corsi di studio di formazione Post-Laurea; in questo dataset, si può riferire a Scuole di specializzazione/Master di I livello/Master di II livello/Dottorati di ricerca.</rdfs:comment>
    <rdfs:comment xml:lang="en">Postgraduate education courses; in this dataset, it can be referred to Specialization Schools / Masters of I Level / Masters of II Level / Research Doctorates.</rdfs:comment>
    <rdfs:isDefinedBy rdf:resource="https://w3id.org/italia/onto/HER"/>
    <rdfs:label xml:lang="it">Corsi di specializzazione riportati da USTAT</rdfs:label>
    <rdfs:label xml:lang="en">USTAT Reported Postgraduate Course</rdfs:label>
    <owl:versionInfo xml:lang="it">stabile</owl:versionInfo>
    <owl:versionInfo xml:lang="en">stable</owl:versionInfo>
  </rdf:Description>
  <rdf:Description rdf:nodeID="n5bb3bff42afb4ca286d2c3fead9507ddb205">
    <rdf:type rdf:resource="http://www.w3.org/2002/07/owl#Class"/>
    <owl:unionOf rdf:nodeID="n5bb3bff42afb4ca286d2c3fead9507ddb206"/>
  </rdf:Description>
  <rdf:Description rdf:about="https://w3id.org/italia/onto/HER/Diploma">
    <rdf:type rdf:resource="http://www.w3.org/2002/07/owl#Class"/>
    <rdfs:subClassOf rdf:resource="https://w3id.org/italia/onto/l0/Object"/>
    <rdfs:comment xml:lang="en">A maturity diploma that can be awarded upon successful completion of secondary education.</rdfs:comment>
    <rdfs:comment xml:lang="it">Un diploma di maturità che può essere rilasciato al termine del ciclo di studi secondari.</rdfs:comment>
    <rdfs:isDefinedBy rdf:resource="https://w3id.org/italia/onto/HER"/>
    <rdfs:label xml:lang="en">Diploma</rdfs:label>
    <rdfs:label xml:lang="it">diploma</rdfs:label>
    <owl:versionInfo xml:lang="it">stabile</owl:versionInfo>
    <owl:versionInfo xml:lang="en">stable</owl:versionInfo>
  </rdf:Description>
  <rdf:Description rdf:about="https://w3id.org/italia/data/distribution/HERAPIT-RDF-XML">
    <rdf:type rdf:resource="http://www.w3.org/2002/07/owl#NamedIndividual"/>
    <rdf:type rdf:resource="https://w3id.org/italia/onto/ADMS/SemanticAssetDistribution"/>
    <ns2:description xml:lang="it">Questa è la distribuzione RDF/XML dell'ontologia della Ricerca Pubblica</ns2:description>
    <ns2:description xml:lang="en">This is the distribution in RDF/XML of the Public Research ontology</ns2:description>
    <ns2:format rdf:resource="http://publications.europa.eu/resource/authority/file-type/RDF_XML"/>
    <ns2:license rdf:resource="https://w3id.org/italia/controlled-vocabulary/licences/A21_CCBY40"/>
    <ns2:title xml:lang="it">Distribuzione RDF/XML ontologia PublicReseach-AP_IT</ns2:title>
    <ns2:title xml:lang="en">RDF/XML distribution of PublicReseach-AP_IT Ontology</ns2:title>
    <ns3:accessURL rdf:resource="https://raw.githubusercontent.com/italia/daf-ontologie-vocabolari-controllati/master/Ontologie/HER/latest"/>
    <ns3:downloadURL rdf:resource="https://raw.githubusercontent.com/italia/daf-ontologie-vocabolari-controllati/master/Ontologie/HER/latest/HER-AP_IT.rdf"/>
  </rdf:Description>
  <rdf:Description rdf:nodeID="n5bb3bff42afb4ca286d2c3fead9507ddb116">
    <rdf:first rdf:resource="https://w3id.org/italia/onto/HER/ItalianPhDCourseByCycle"/>
    <rdf:rest rdf:nodeID="n5bb3bff42afb4ca286d2c3fead9507ddb117"/>
  </rdf:Description>
  <rdf:Description rdf:nodeID="n5bb3bff42afb4ca286d2c3fead9507ddb295">
    <rdf:type rdf:resource="http://www.w3.org/1999/02/22-rdf-syntax-ns#List"/>
    <rdf:first>Retrospective</rdf:first>
    <rdf:rest rdf:nodeID="n5bb3bff42afb4ca286d2c3fead9507ddb296"/>
  </rdf:Description>
  <rdf:Description rdf:nodeID="n5bb3bff42afb4ca286d2c3fead9507ddb501">
    <rdf:type rdf:resource="http://www.w3.org/2002/07/owl#Restriction"/>
    <owl:onProperty rdf:resource="https://w3id.org/italia/onto/HER/patentFamilyCode"/>
    <owl:cardinality rdf:datatype="http://www.w3.org/2001/XMLSchema#nonNegativeInteger">1</owl:cardinality>
  </rdf:Description>
  <rdf:Description rdf:about="https://w3id.org/italia/onto/l0/Topic">
    <rdf:type rdf:resource="http://www.w3.org/2002/07/owl#Class"/>
  </rdf:Description>
  <rdf:Description rdf:nodeID="n5bb3bff42afb4ca286d2c3fead9507ddb338">
    <rdf:first rdf:resource="https://w3id.org/italia/onto/HER/ErasmusPlusProject"/>
    <rdf:rest rdf:resource="http://www.w3.org/1999/02/22-rdf-syntax-ns#nil"/>
  </rdf:Description>
  <rdf:Description rdf:nodeID="n5bb3bff42afb4ca286d2c3fead9507ddb148">
    <rdf:type rdf:resource="http://www.w3.org/1999/02/22-rdf-syntax-ns#List"/>
    <rdf:first>Ricerca di base</rdf:first>
    <rdf:rest rdf:nodeID="n5bb3bff42afb4ca286d2c3fead9507ddb149"/>
  </rdf:Description>
  <rdf:Description rdf:nodeID="n5bb3bff42afb4ca286d2c3fead9507ddb487">
    <rdf:type rdf:resource="http://www.w3.org/2002/07/owl#Restriction"/>
    <owl:onProperty rdf:resource="https://w3id.org/italia/onto/HER/hasErasmusplusKeyAction"/>
    <owl:qualifiedCardinality rdf:datatype="http://www.w3.org/2001/XMLSchema#nonNegativeInteger">1</owl:qualifiedCardinality>
    <owl:onClass rdf:resource="https://w3id.org/italia/onto/HER/ErasmusPlusKeyAction"/>
  </rdf:Description>
  <rdf:Description rdf:nodeID="n5bb3bff42afb4ca286d2c3fead9507ddb306">
    <rdf:first rdf:resource="https://w3id.org/italia/onto/HER/USTATEnrolledStudentsAggregate"/>
    <rdf:rest rdf:nodeID="n5bb3bff42afb4ca286d2c3fead9507ddb307"/>
  </rdf:Description>
  <rdf:Description rdf:nodeID="n5bb3bff42afb4ca286d2c3fead9507ddb139">
    <rdf:type rdf:resource="http://www.w3.org/1999/02/22-rdf-syntax-ns#List"/>
    <rdf:first>Samples Without DNA</rdf:first>
    <rdf:rest rdf:resource="http://www.w3.org/1999/02/22-rdf-syntax-ns#nil"/>
  </rdf:Description>
  <rdf:Description rdf:about="https://w3id.org/italia/onto/HER/hasUSTATFunctionalArea">
    <rdf:type rdf:resource="http://www.w3.org/2002/07/owl#ObjectProperty"/>
    <rdfs:domain rdf:resource="https://w3id.org/italia/onto/HER/USTATTAStaffByGender"/>
    <rdfs:range rdf:resource="https://w3id.org/italia/onto/HER/USTATFunctionalArea"/>
    <rdfs:comment xml:lang="en">It is used to link data on the number of technical-administrative staff by gender and year to the corresponding functional area.</rdfs:comment>
    <rdfs:comment xml:lang="it">Viene utilizzato per collegare i dati sul numero di personale tecnico-amministrativo per genere e per anno all'area funzionale corrispondente.</rdfs:comment>
    <rdfs:isDefinedBy rdf:resource="https://w3id.org/italia/onto/HER"/>
    <rdfs:label xml:lang="it">ha un area funzionale</rdfs:label>
    <rdfs:label xml:lang="en">has functional area</rdfs:label>
    <owl:versionInfo xml:lang="it">stabile</owl:versionInfo>
    <owl:versionInfo xml:lang="en">stable</owl:versionInfo>
  </rdf:Description>
  <rdf:Description rdf:nodeID="n5bb3bff42afb4ca286d2c3fead9507ddb114">
    <rdf:first rdf:resource="https://w3id.org/italia/onto/HER/ItalianAcademicRole"/>
    <rdf:rest rdf:resource="http://www.w3.org/1999/02/22-rdf-syntax-ns#nil"/>
  </rdf:Description>
  <rdf:Description rdf:nodeID="n5bb3bff42afb4ca286d2c3fead9507ddb527">
    <rdf:type rdf:resource="http://www.w3.org/2002/07/owl#Restriction"/>
    <owl:onProperty rdf:resource="https://w3id.org/italia/onto/COV/hasOrganization"/>
    <owl:maxQualifiedCardinality rdf:datatype="http://www.w3.org/2001/XMLSchema#nonNegativeInteger">1</owl:maxQualifiedCardinality>
    <owl:onClass rdf:resource="https://w3id.org/italia/onto/COV/Organization"/>
  </rdf:Description>
  <rdf:Description rdf:nodeID="n5bb3bff42afb4ca286d2c3fead9507ddb275">
    <rdf:first rdf:resource="https://w3id.org/italia/onto/HER/CHAFEAProject"/>
    <rdf:rest rdf:nodeID="n5bb3bff42afb4ca286d2c3fead9507ddb276"/>
  </rdf:Description>
  <rdf:Description rdf:nodeID="n5bb3bff42afb4ca286d2c3fead9507ddb174">
    <rdf:type rdf:resource="http://www.w3.org/2000/01/rdf-schema#Datatype"/>
    <owl:oneOf rdf:nodeID="n5bb3bff42afb4ca286d2c3fead9507ddb175"/>
  </rdf:Description>
  <rdf:Description rdf:nodeID="n5bb3bff42afb4ca286d2c3fead9507ddb373">
    <rdf:type rdf:resource="http://www.w3.org/2002/07/owl#Restriction"/>
    <owl:onProperty rdf:resource="https://w3id.org/italia/onto/HER/aactPopulation"/>
    <owl:allValuesFrom rdf:resource="http://www.w3.org/2000/01/rdf-schema#Literal"/>
  </rdf:Description>
  <rdf:Description rdf:nodeID="n5bb3bff42afb4ca286d2c3fead9507ddb60">
    <rdf:first rdf:resource="https://w3id.org/italia/onto/HER/CTNPRINProject"/>
    <rdf:rest rdf:resource="http://www.w3.org/1999/02/22-rdf-syntax-ns#nil"/>
  </rdf:Description>
  <rdf:Description rdf:nodeID="n5bb3bff42afb4ca286d2c3fead9507ddb292">
    <rdf:type rdf:resource="http://www.w3.org/1999/02/22-rdf-syntax-ns#List"/>
    <rdf:first>Longitudinal, Retrospective/Prospective</rdf:first>
    <rdf:rest rdf:nodeID="n5bb3bff42afb4ca286d2c3fead9507ddb293"/>
  </rdf:Description>
  <rdf:Description rdf:about="https://w3id.org/italia/onto/l0/Object">
    <rdf:type rdf:resource="http://www.w3.org/2002/07/owl#Class"/>
  </rdf:Description>
  <rdf:Description rdf:about="https://w3id.org/italia/onto/HER/USTATReportedHERInstitution">
    <rdf:type rdf:resource="http://www.w3.org/2002/07/owl#Class"/>
    <rdfs:subClassOf rdf:resource="https://w3id.org/italia/onto/COV/PublicOrganization"/>
    <rdfs:comment xml:lang="en">Information (identification code, name, typology) of the Institute under consideration (University, Istituto Alta Formazione Artistica e Musicale - AFAM, Scuola Superiore per Mediatori Linguistici, Other).</rdfs:comment>
    <rdfs:comment xml:lang="it">Informazioni (codice identificativo, nome, tipologia) dell'Istituto in questione (Ateneo, Istituto Alta Formazione Artistica e Musicale - AFAM, Scuola Superiore per Mediatori Linguistici, Altro).</rdfs:comment>
    <rdfs:isDefinedBy rdf:resource="https://w3id.org/italia/onto/HER"/>
    <rdfs:label xml:lang="it">Istituzione HER riportate da USTAT</rdfs:label>
    <rdfs:label xml:lang="en">USTAT Reported HER Institution</rdfs:label>
    <owl:versionInfo xml:lang="it">stabile</owl:versionInfo>
    <owl:versionInfo xml:lang="en">stable</owl:versionInfo>
  </rdf:Description>
  <rdf:Description rdf:about="https://w3id.org/italia/onto/HER/patentPublishedAs">
    <rdf:type rdf:resource="http://www.w3.org/2002/07/owl#DatatypeProperty"/>
    <rdfs:subPropertyOf rdf:resource="https://w3id.org/italia/onto/l0/identifier"/>
    <rdfs:domain rdf:resource="https://w3id.org/italia/onto/HER/Patent"/>
    <rdfs:range rdf:resource="http://www.w3.org/2000/01/rdf-schema#Literal"/>
    <rdfs:comment xml:lang="en">One of the (potentially multiple) publication numbers of a patent.</rdfs:comment>
    <rdfs:comment xml:lang="it">Uno dei numeri di pubblicazione (potenzialmente multipli) di un brevetto.</rdfs:comment>
    <rdfs:isDefinedBy rdf:resource="https://w3id.org/italia/onto/HER"/>
    <rdfs:label xml:lang="it">brevetto pubblicato come</rdfs:label>
    <rdfs:label xml:lang="en">patent published as</rdfs:label>
    <owl:versionInfo xml:lang="it">provvisoria</owl:versionInfo>
    <owl:versionInfo xml:lang="en">unstable</owl:versionInfo>
  </rdf:Description>
  <rdf:Description rdf:nodeID="n5bb3bff42afb4ca286d2c3fead9507ddb534">
    <rdf:type rdf:resource="http://www.w3.org/2002/07/owl#Restriction"/>
    <owl:onProperty rdf:resource="https://w3id.org/italia/onto/COV/hasOrganization"/>
    <owl:maxQualifiedCardinality rdf:datatype="http://www.w3.org/2001/XMLSchema#nonNegativeInteger">1</owl:maxQualifiedCardinality>
    <owl:onClass rdf:resource="https://w3id.org/italia/onto/COV/Organization"/>
  </rdf:Description>
  <rdf:Description rdf:about="https://w3id.org/italia/onto/HER/FORDClassification">
    <rdf:type rdf:resource="http://www.w3.org/2002/07/owl#Class"/>
    <rdfs:subClassOf rdf:resource="https://w3id.org/italia/onto/HER/HERClassification"/>
    <rdfs:comment xml:lang="it">La classificazione Fields of research and development (FORD) viene utilizzata per classificare le unità e le risorse di R&amp;S in base ai campi di indagine, vale a dire ampi domini di conoscenza basati principalmente sul contenuto della materia di R&amp;S. (Fonte: http://uis.unesco.org/en/glossary-term/fields-research-and-development-ford)</rdfs:comment>
    <rdfs:comment xml:lang="en">The Fields of research and development (FORD) classification is used to classify R&amp;D units and resources by fields of enquiry, namely, broad knowledge domains based primarily on the content of the R&amp;D subject matter. (Source: http://uis.unesco.org/en/glossary-term/fields-research-and-development-ford)</rdfs:comment>
    <rdfs:isDefinedBy rdf:resource="https://w3id.org/italia/onto/HER"/>
    <rdfs:label xml:lang="it">Classificazione FORD</rdfs:label>
    <rdfs:label xml:lang="en">FORD Classification</rdfs:label>
    <owl:versionInfo xml:lang="it">stabile</owl:versionInfo>
    <owl:versionInfo xml:lang="en">stable</owl:versionInfo>
    <ns6:wasDerivedFrom rdf:resource="http://www.w3.org/2004/02/skos/core#Concept"/>
    <ns4:controlledVocabulary rdf:resource="https://w3id.org/italia/controlled-vocabulary/classifications-for-her/fields-of-research-development"/>
  </rdf:Description>
  <rdf:Description rdf:nodeID="n5bb3bff42afb4ca286d2c3fead9507ddb33">
    <rdf:first rdf:resource="https://w3id.org/italia/onto/HER/AcademicRole"/>
    <rdf:rest rdf:nodeID="n5bb3bff42afb4ca286d2c3fead9507ddb34"/>
  </rdf:Description>
  <rdf:Description rdf:about="https://w3id.org/italia/onto/HER/ctnprinOperationScope">
    <rdf:type rdf:resource="http://www.w3.org/2002/07/owl#DatatypeProperty"/>
    <rdfs:domain rdf:resource="https://w3id.org/italia/onto/HER/CTNPRINOperation"/>
    <rdfs:range rdf:nodeID="n5bb3bff42afb4ca286d2c3fead9507ddb152"/>
    <rdfs:comment xml:lang="it">Ambito operativo dell'operazione. Può essere:
- R&amp;S
- Formazione
- Ricerca di base</rdfs:comment>
    <rdfs:comment xml:lang="en">Operational scope of the operation. Could be:
- R&amp;D
- Training
- Basic research</rdfs:comment>
    <rdfs:label xml:lang="it">ambito operazione CTN/PRIN</rdfs:label>
    <rdfs:label xml:lang="en">scope of CTN/PRIN operation</rdfs:label>
    <owl:versionInfo xml:lang="it">stabile</owl:versionInfo>
    <owl:versionInfo xml:lang="en">stable</owl:versionInfo>
  </rdf:Description>
  <rdf:Description rdf:about="https://w3id.org/italia/onto/HER/hasCTNPRINAmount">
    <rdf:type rdf:resource="http://www.w3.org/2002/07/owl#ObjectProperty"/>
    <rdfs:domain rdf:resource="https://w3id.org/italia/onto/HER/CTNPRINOperation"/>
    <rdfs:range rdf:resource="https://w3id.org/italia/onto/HER/CTNPRINAmount"/>
    <rdfs:comment xml:lang="it">Questa proprietà collega l'operazione con gli importi.</rdfs:comment>
    <rdfs:comment xml:lang="en">This property links the operation with the amounts.</rdfs:comment>
    <rdfs:isDefinedBy rdf:resource="https://w3id.org/italia/onto/HER"/>
    <rdfs:label xml:lang="it">ha importo riportato da CTN/PRIN</rdfs:label>
    <rdfs:label xml:lang="en">has CTN/PRIN amount</rdfs:label>
    <owl:versionInfo xml:lang="it">provvisoria</owl:versionInfo>
    <owl:versionInfo xml:lang="en">unstable</owl:versionInfo>
  </rdf:Description>
  <rdf:Description rdf:nodeID="n5bb3bff42afb4ca286d2c3fead9507ddb510">
    <rdf:type rdf:resource="http://www.w3.org/2002/07/owl#Restriction"/>
    <owl:onProperty rdf:resource="https://w3id.org/italia/onto/HER/title"/>
    <owl:someValuesFrom rdf:resource="http://www.w3.org/2000/01/rdf-schema#Literal"/>
  </rdf:Description>
  <rdf:Description rdf:nodeID="n5bb3bff42afb4ca286d2c3fead9507ddb217">
    <rdf:first rdf:resource="https://w3id.org/italia/onto/HER/MIURStudentsByRegionOfResidenceDegreeDegreeClassAggregate"/>
    <rdf:rest rdf:resource="http://www.w3.org/1999/02/22-rdf-syntax-ns#nil"/>
  </rdf:Description>
  <rdf:Description rdf:nodeID="n5bb3bff42afb4ca286d2c3fead9507ddb258">
    <rdf:type rdf:resource="http://www.w3.org/1999/02/22-rdf-syntax-ns#List"/>
    <rdf:first>Educational/Counseling/Training</rdf:first>
    <rdf:rest rdf:nodeID="n5bb3bff42afb4ca286d2c3fead9507ddb259"/>
  </rdf:Description>
  <rdf:Description rdf:nodeID="n5bb3bff42afb4ca286d2c3fead9507ddb505">
    <rdf:type rdf:resource="http://www.w3.org/2002/07/owl#Restriction"/>
    <owl:onProperty rdf:resource="https://w3id.org/italia/onto/HER/patentKindCode"/>
    <owl:cardinality rdf:datatype="http://www.w3.org/2001/XMLSchema#nonNegativeInteger">1</owl:cardinality>
  </rdf:Description>
  <rdf:Description rdf:nodeID="n5bb3bff42afb4ca286d2c3fead9507ddb181">
    <rdf:type rdf:resource="http://www.w3.org/1999/02/22-rdf-syntax-ns#List"/>
    <rdf:first>Not yet recruiting</rdf:first>
    <rdf:rest rdf:nodeID="n5bb3bff42afb4ca286d2c3fead9507ddb182"/>
  </rdf:Description>
  <rdf:Description rdf:nodeID="n5bb3bff42afb4ca286d2c3fead9507ddb25">
    <rdf:first rdf:resource="https://w3id.org/italia/onto/HER/MIURStudentsByDegreeDegreeClassAggregate"/>
    <rdf:rest rdf:nodeID="n5bb3bff42afb4ca286d2c3fead9507ddb26"/>
  </rdf:Description>
  <rdf:Description rdf:nodeID="n5bb3bff42afb4ca286d2c3fead9507ddb267">
    <rdf:first rdf:resource="https://w3id.org/italia/onto/HER/Result"/>
    <rdf:rest rdf:resource="http://www.w3.org/1999/02/22-rdf-syntax-ns#nil"/>
  </rdf:Description>
  <rdf:Description rdf:nodeID="n5bb3bff42afb4ca286d2c3fead9507ddb177">
    <rdf:type rdf:resource="http://www.w3.org/1999/02/22-rdf-syntax-ns#List"/>
    <rdf:first>Treatment</rdf:first>
    <rdf:rest rdf:resource="http://www.w3.org/1999/02/22-rdf-syntax-ns#nil"/>
  </rdf:Description>
  <rdf:Description rdf:nodeID="n5bb3bff42afb4ca286d2c3fead9507ddb396">
    <rdf:type rdf:resource="http://www.w3.org/2002/07/owl#Restriction"/>
    <owl:onProperty rdf:resource="https://w3id.org/italia/onto/Project/projectAcronym"/>
    <owl:maxCardinality rdf:datatype="http://www.w3.org/2001/XMLSchema#nonNegativeInteger">1</owl:maxCardinality>
  </rdf:Description>
  <rdf:Description rdf:about="http://www.w3.org/ns/dcat#keyword">
    <rdf:type rdf:resource="http://www.w3.org/2002/07/owl#AnnotationProperty"/>
  </rdf:Description>
  <rdf:Description rdf:nodeID="n5bb3bff42afb4ca286d2c3fead9507ddb283">
    <rdf:first rdf:resource="https://w3id.org/italia/onto/HER/ErasmusPlusProject"/>
    <rdf:rest rdf:resource="http://www.w3.org/1999/02/22-rdf-syntax-ns#nil"/>
  </rdf:Description>
  <rdf:Description rdf:nodeID="n5bb3bff42afb4ca286d2c3fead9507ddb497">
    <rdf:type rdf:resource="http://www.w3.org/2002/07/owl#Restriction"/>
    <owl:onProperty rdf:resource="https://w3id.org/italia/onto/CLV/hasSpatialCoverage"/>
    <owl:someValuesFrom rdf:resource="https://w3id.org/italia/onto/CLV/Region"/>
  </rdf:Description>
  <rdf:Description rdf:nodeID="n5bb3bff42afb4ca286d2c3fead9507ddb528">
    <rdf:type rdf:resource="http://www.w3.org/2002/07/owl#Restriction"/>
    <owl:onProperty rdf:resource="https://w3id.org/italia/onto/COV/hasOrganization"/>
    <owl:maxQualifiedCardinality rdf:datatype="http://www.w3.org/2001/XMLSchema#nonNegativeInteger">1</owl:maxQualifiedCardinality>
    <owl:onClass rdf:resource="https://w3id.org/italia/onto/COV/Organization"/>
  </rdf:Description>
  <rdf:Description rdf:nodeID="n5bb3bff42afb4ca286d2c3fead9507ddb11">
    <rdf:first rdf:resource="https://w3id.org/italia/onto/HER/ISCEDFClassification"/>
    <rdf:rest rdf:nodeID="n5bb3bff42afb4ca286d2c3fead9507ddb12"/>
  </rdf:Description>
  <rdf:Description rdf:nodeID="n5bb3bff42afb4ca286d2c3fead9507ddb397">
    <rdf:type rdf:resource="http://www.w3.org/2002/07/owl#Restriction"/>
    <owl:onProperty rdf:resource="https://w3id.org/italia/onto/l0/name"/>
    <owl:someValuesFrom rdf:resource="http://www.w3.org/2001/XMLSchema#boolean"/>
  </rdf:Description>
  <rdf:Description rdf:nodeID="n5bb3bff42afb4ca286d2c3fead9507ddb10">
    <rdf:type rdf:resource="http://www.w3.org/2002/07/owl#Class"/>
    <owl:unionOf rdf:nodeID="n5bb3bff42afb4ca286d2c3fead9507ddb11"/>
  </rdf:Description>
  <rdf:Description rdf:nodeID="n5bb3bff42afb4ca286d2c3fead9507ddb118">
    <rdf:type rdf:resource="http://www.w3.org/2002/07/owl#Class"/>
    <owl:unionOf rdf:nodeID="n5bb3bff42afb4ca286d2c3fead9507ddb119"/>
  </rdf:Description>
  <rdf:Description rdf:nodeID="n5bb3bff42afb4ca286d2c3fead9507ddb131">
    <rdf:first rdf:resource="https://w3id.org/italia/onto/HER/USTATTotallyExoneratedStudentsAggregate"/>
    <rdf:rest rdf:resource="http://www.w3.org/1999/02/22-rdf-syntax-ns#nil"/>
  </rdf:Description>
  <rdf:Description rdf:nodeID="n5bb3bff42afb4ca286d2c3fead9507ddb374">
    <rdf:type rdf:resource="http://www.w3.org/2002/07/owl#Restriction"/>
    <owl:onProperty rdf:resource="https://w3id.org/italia/onto/HER/aactMaximumAge"/>
    <owl:maxQualifiedCardinality rdf:datatype="http://www.w3.org/2001/XMLSchema#nonNegativeInteger">1</owl:maxQualifiedCardinality>
    <owl:onDataRange rdf:resource="http://www.w3.org/2001/XMLSchema#integer"/>
  </rdf:Description>
  <rdf:Description rdf:nodeID="n5bb3bff42afb4ca286d2c3fead9507ddb242">
    <rdf:type rdf:resource="http://www.w3.org/1999/02/22-rdf-syntax-ns#List"/>
    <rdf:first>Natural History</rdf:first>
    <rdf:rest rdf:nodeID="n5bb3bff42afb4ca286d2c3fead9507ddb243"/>
  </rdf:Description>
  <rdf:Description rdf:nodeID="n5bb3bff42afb4ca286d2c3fead9507ddb436">
    <rdf:type rdf:resource="http://www.w3.org/2002/07/owl#Restriction"/>
    <owl:onProperty rdf:resource="https://w3id.org/italia/onto/l0/description"/>
    <owl:someValuesFrom rdf:resource="http://www.w3.org/2000/01/rdf-schema#Literal"/>
  </rdf:Description>
  <rdf:Description rdf:nodeID="n5bb3bff42afb4ca286d2c3fead9507ddb3">
    <rdf:first rdf:resource="https://w3id.org/italia/onto/HER/ERCProject"/>
    <rdf:rest rdf:resource="http://www.w3.org/1999/02/22-rdf-syntax-ns#nil"/>
  </rdf:Description>
  <rdf:Description rdf:about="https://w3id.org/italia/onto/HER/ItalianPhDCourseByCycle">
    <rdf:type rdf:resource="http://www.w3.org/2002/07/owl#Class"/>
    <rdfs:subClassOf rdf:resource="https://w3id.org/italia/onto/l0/EventOrSituation"/>
    <rdfs:comment xml:lang="it">Rapporti con i corsi di dottorato di ricerca che offre ogni anno.</rdfs:comment>
    <rdfs:comment xml:lang="en">Reified relationship that related an university with the PhD courses it offers each cycle year.</rdfs:comment>
    <rdfs:isDefinedBy rdf:resource="https://w3id.org/italia/onto/HER"/>
    <rdfs:label xml:lang="it">Corsi di PHD italian per ciclo accademico</rdfs:label>
    <rdfs:label xml:lang="en">Italian PhD Course By Academic Cycle</rdfs:label>
    <owl:versionInfo xml:lang="it">stabile</owl:versionInfo>
    <owl:versionInfo xml:lang="en">stable</owl:versionInfo>
  </rdf:Description>
  <rdf:Description rdf:nodeID="n5bb3bff42afb4ca286d2c3fead9507ddb484">
    <rdf:type rdf:resource="http://www.w3.org/2002/07/owl#Restriction"/>
    <owl:onProperty rdf:resource="https://w3id.org/italia/onto/l0/hasTopic"/>
    <owl:allValuesFrom rdf:resource="https://w3id.org/italia/onto/HER/ErasmusPlusTopic"/>
  </rdf:Description>
  <rdf:Description rdf:nodeID="n5bb3bff42afb4ca286d2c3fead9507ddb129">
    <rdf:first rdf:resource="https://w3id.org/italia/onto/HER/USTATPostgraduateAggregateOfEnrolled"/>
    <rdf:rest rdf:nodeID="n5bb3bff42afb4ca286d2c3fead9507ddb130"/>
  </rdf:Description>
  <rdf:Description rdf:nodeID="n5bb3bff42afb4ca286d2c3fead9507ddb5">
    <rdf:first rdf:resource="https://w3id.org/italia/onto/HER/AACTCondition"/>
    <rdf:rest rdf:nodeID="n5bb3bff42afb4ca286d2c3fead9507ddb6"/>
  </rdf:Description>
  <rdf:Description rdf:nodeID="n5bb3bff42afb4ca286d2c3fead9507ddb262">
    <rdf:type rdf:resource="http://www.w3.org/1999/02/22-rdf-syntax-ns#List"/>
    <rdf:first>Screening</rdf:first>
    <rdf:rest rdf:nodeID="n5bb3bff42afb4ca286d2c3fead9507ddb263"/>
  </rdf:Description>
  <rdf:Description rdf:about="https://w3id.org/italia/onto/HER/hasPatentPublicationDetail">
    <rdf:type rdf:resource="http://www.w3.org/2002/07/owl#ObjectProperty"/>
    <rdfs:domain rdf:resource="https://w3id.org/italia/onto/HER/Patent"/>
    <rdfs:range rdf:resource="https://w3id.org/italia/onto/HER/PatentPublicationDetail"/>
    <rdfs:comment xml:lang="it">Questa proprietà collega un brevetto con i suoi dettagli di pubblicazione.</rdfs:comment>
    <rdfs:comment xml:lang="en">This property connects a patent with its publication details.</rdfs:comment>
    <rdfs:isDefinedBy rdf:resource="https://w3id.org/italia/onto/HER"/>
    <rdfs:label xml:lang="it">ha dettagli pubblicazione brevetto</rdfs:label>
    <rdfs:label xml:lang="en">has patent publication details</rdfs:label>
    <owl:versionInfo xml:lang="it">provvisoria</owl:versionInfo>
    <owl:versionInfo xml:lang="en">unstable</owl:versionInfo>
  </rdf:Description>
  <rdf:Description rdf:nodeID="n5bb3bff42afb4ca286d2c3fead9507ddb541">
    <rdf:type rdf:resource="http://www.w3.org/2002/07/owl#Restriction"/>
    <owl:onProperty rdf:resource="https://w3id.org/italia/onto/COV/hasOrganization"/>
    <owl:maxQualifiedCardinality rdf:datatype="http://www.w3.org/2001/XMLSchema#nonNegativeInteger">1</owl:maxQualifiedCardinality>
    <owl:onClass rdf:resource="https://w3id.org/italia/onto/COV/Organization"/>
  </rdf:Description>
  <rdf:Description rdf:nodeID="n5bb3bff42afb4ca286d2c3fead9507ddb175">
    <rdf:type rdf:resource="http://www.w3.org/1999/02/22-rdf-syntax-ns#List"/>
    <rdf:first>Individual</rdf:first>
    <rdf:rest rdf:nodeID="n5bb3bff42afb4ca286d2c3fead9507ddb176"/>
  </rdf:Description>
  <rdf:Description rdf:nodeID="n5bb3bff42afb4ca286d2c3fead9507ddb235">
    <rdf:type rdf:resource="http://www.w3.org/1999/02/22-rdf-syntax-ns#List"/>
    <rdf:first>Case-Crossover</rdf:first>
    <rdf:rest rdf:nodeID="n5bb3bff42afb4ca286d2c3fead9507ddb236"/>
  </rdf:Description>
  <rdf:Description rdf:about="https://w3id.org/italia/onto/HER/investigatorMasked">
    <rdf:type rdf:resource="http://www.w3.org/2002/07/owl#DatatypeProperty"/>
    <rdf:type rdf:resource="http://www.w3.org/2002/07/owl#FunctionalProperty"/>
    <rdfs:domain rdf:resource="https://w3id.org/italia/onto/HER/AACTDesign"/>
    <rdfs:range rdf:resource="http://www.w3.org/2001/XMLSchema#boolean"/>
    <rdfs:comment xml:lang="it">Gli sperimentatori sono le parti coinvolte nello studio clinico che non possono conoscere gli interventi assegnati ai singoli partecipanti.</rdfs:comment>
    <rdfs:comment xml:lang="en">Investigator is the party or parties involved in the clinical trial who are prevented from having knowledge of the interventions assigned to individual participants. True if they are prevented; false if they are not.</rdfs:comment>
    <rdfs:isDefinedBy rdf:resource="https://w3id.org/italia/onto/HER"/>
    <rdfs:label xml:lang="it">esaminatori coinvolti conoscono interventi</rdfs:label>
    <rdfs:label xml:lang="en">investigator masked</rdfs:label>
    <owl:versionInfo xml:lang="it">stabile</owl:versionInfo>
    <owl:versionInfo xml:lang="en">stable</owl:versionInfo>
  </rdf:Description>
  <rdf:Description rdf:nodeID="n5bb3bff42afb4ca286d2c3fead9507ddb479">
    <rdf:type rdf:resource="http://www.w3.org/2002/07/owl#Restriction"/>
    <owl:onProperty rdf:resource="https://w3id.org/italia/onto/l0/name"/>
    <owl:someValuesFrom rdf:resource="http://www.w3.org/2000/01/rdf-schema#Literal"/>
  </rdf:Description>
  <rdf:Description rdf:nodeID="n5bb3bff42afb4ca286d2c3fead9507ddb115">
    <rdf:type rdf:resource="http://www.w3.org/2002/07/owl#Class"/>
    <owl:unionOf rdf:nodeID="n5bb3bff42afb4ca286d2c3fead9507ddb116"/>
  </rdf:Description>
  <rdf:Description rdf:nodeID="n5bb3bff42afb4ca286d2c3fead9507ddb511">
    <rdf:type rdf:resource="http://www.w3.org/2002/07/owl#Restriction"/>
    <owl:onProperty rdf:resource="https://w3id.org/italia/onto/HER/publicationDate"/>
    <owl:qualifiedCardinality rdf:datatype="http://www.w3.org/2001/XMLSchema#nonNegativeInteger">1</owl:qualifiedCardinality>
    <owl:onDataRange rdf:resource="http://www.w3.org/2001/XMLSchema#date"/>
  </rdf:Description>
  <rdf:Description rdf:nodeID="n5bb3bff42afb4ca286d2c3fead9507ddb169">
    <rdf:first rdf:resource="https://w3id.org/italia/onto/HER/CHAFEAProject"/>
    <rdf:rest rdf:nodeID="n5bb3bff42afb4ca286d2c3fead9507ddb170"/>
  </rdf:Description>
  <rdf:Description rdf:nodeID="n5bb3bff42afb4ca286d2c3fead9507ddb347">
    <rdf:first rdf:resource="https://w3id.org/italia/onto/HER/USTATEnrolledStudentsAggregate"/>
    <rdf:rest rdf:nodeID="n5bb3bff42afb4ca286d2c3fead9507ddb348"/>
  </rdf:Description>
  <rdf:Description rdf:nodeID="n5bb3bff42afb4ca286d2c3fead9507ddb499">
    <rdf:type rdf:resource="http://www.w3.org/2002/07/owl#Restriction"/>
    <owl:onProperty rdf:resource="https://w3id.org/italia/onto/HER/hasIPC"/>
    <owl:allValuesFrom rdf:resource="https://w3id.org/italia/onto/HER/InternationalPatentClassification"/>
  </rdf:Description>
  <rdf:Description rdf:nodeID="n5bb3bff42afb4ca286d2c3fead9507ddb450">
    <rdf:type rdf:resource="http://www.w3.org/2002/07/owl#Restriction"/>
    <owl:onProperty rdf:resource="https://w3id.org/italia/onto/HER/hasFundingScheme"/>
    <owl:maxQualifiedCardinality rdf:datatype="http://www.w3.org/2001/XMLSchema#nonNegativeInteger">1</owl:maxQualifiedCardinality>
    <owl:onClass rdf:resource="https://w3id.org/italia/onto/HER/ECFundingScheme"/>
  </rdf:Description>
  <rdf:Description rdf:nodeID="n5bb3bff42afb4ca286d2c3fead9507ddb496">
    <rdf:type rdf:resource="http://www.w3.org/2002/07/owl#Restriction"/>
    <owl:onProperty rdf:resource="https://w3id.org/italia/onto/CLV/hasSpatialCoverage"/>
    <owl:someValuesFrom rdf:resource="https://w3id.org/italia/onto/CLV/Region"/>
  </rdf:Description>
  <rdf:Description rdf:nodeID="n5bb3bff42afb4ca286d2c3fead9507ddb244">
    <rdf:type rdf:resource="http://www.w3.org/2002/07/owl#Class"/>
    <owl:unionOf rdf:nodeID="n5bb3bff42afb4ca286d2c3fead9507ddb245"/>
  </rdf:Description>
  <rdf:Description rdf:about="https://w3id.org/italia/onto/HER/limitationsAndCaveats">
    <rdf:type rdf:resource="http://www.w3.org/2002/07/owl#DatatypeProperty"/>
    <rdfs:domain rdf:resource="https://w3id.org/italia/onto/HER/AACTStudy"/>
    <rdfs:range rdf:resource="http://www.w3.org/2000/01/rdf-schema#Literal"/>
    <rdfs:comment xml:lang="en">Describe significant limitations of the study. Such limitations may include not reaching the target number of participants needed to achieve target power and statistically reliable results or technical problems with measurements leading to unreliable or uninterpretable data.</rdfs:comment>
    <rdfs:comment xml:lang="it">Descrive i limiti significativi dello studio. Tali limitazioni possono includere il mancato raggiungimento del numero di partecipanti necessario per raggiungere il potere target e risultati statisticamente affidabili o problemi tecnici con misurazioni che portano a dati inaffidabili o non interpretabili.</rdfs:comment>
    <rdfs:isDefinedBy rdf:resource="https://w3id.org/italia/onto/HER"/>
    <rdfs:label xml:lang="en">limitations and caveats</rdfs:label>
    <rdfs:label xml:lang="it">limitazioni e avvertimenti</rdfs:label>
    <owl:versionInfo xml:lang="it">stabile</owl:versionInfo>
    <owl:versionInfo xml:lang="en">stable</owl:versionInfo>
  </rdf:Description>
  <rdf:Description rdf:nodeID="n5bb3bff42afb4ca286d2c3fead9507ddb480">
    <rdf:type rdf:resource="http://www.w3.org/2002/07/owl#Restriction"/>
    <owl:onProperty rdf:resource="https://w3id.org/italia/onto/HER/picNumber"/>
    <owl:cardinality rdf:datatype="http://www.w3.org/2001/XMLSchema#nonNegativeInteger">1</owl:cardinality>
  </rdf:Description>
  <rdf:Description rdf:about="https://w3id.org/italia/onto/HER/USTATTotallyExoneratedStudentsAggregate">
    <rdf:type rdf:resource="http://www.w3.org/2002/07/owl#Class"/>
    <rdfs:subClassOf rdf:resource="https://w3id.org/italia/onto/HER/StatisticalDataAggregation"/>
    <rdfs:subClassOf rdf:nodeID="n5bb3bff42afb4ca286d2c3fead9507ddb543"/>
    <rdfs:comment xml:lang="en">Data on totally exempted students by type of exemption. Data referring to the Academic year (T-1)/(T).</rdfs:comment>
    <rdfs:comment xml:lang="it">Dati relativi agli studenti esonerati totalmente per tipologia di esonero. Dati riferiti all'anno Accademico (T-1)/(T).</rdfs:comment>
    <rdfs:isDefinedBy rdf:resource="https://w3id.org/italia/onto/HER"/>
    <rdfs:label xml:lang="it">Aggregazione degli studenti totalmente esonerati riportati da USTAT</rdfs:label>
    <rdfs:label xml:lang="en">USTAT Aggregate of Totally Exonerated Students</rdfs:label>
    <owl:versionInfo xml:lang="it">stabile</owl:versionInfo>
    <owl:versionInfo xml:lang="en">stable</owl:versionInfo>
  </rdf:Description>
  <rdf:Description rdf:nodeID="n5bb3bff42afb4ca286d2c3fead9507ddb398">
    <rdf:type rdf:resource="http://www.w3.org/2002/07/owl#Restriction"/>
    <owl:onProperty rdf:resource="https://w3id.org/italia/onto/l0/name"/>
    <owl:someValuesFrom rdf:resource="http://www.w3.org/2000/01/rdf-schema#Literal"/>
  </rdf:Description>
  <rdf:Description rdf:nodeID="n5bb3bff42afb4ca286d2c3fead9507ddb474">
    <rdf:type rdf:resource="http://www.w3.org/2002/07/owl#Restriction"/>
    <owl:onProperty rdf:resource="https://w3id.org/italia/onto/SM/URL"/>
    <owl:allValuesFrom rdf:resource="http://www.w3.org/2001/XMLSchema#anyURI"/>
  </rdf:Description>
  <rdf:Description rdf:about="https://w3id.org/italia/onto/HER/observationalModel">
    <rdf:type rdf:resource="http://www.w3.org/2002/07/owl#DatatypeProperty"/>
    <rdfs:domain rdf:resource="https://w3id.org/italia/onto/HER/AACTDesign"/>
    <rdfs:range rdf:nodeID="n5bb3bff42afb4ca286d2c3fead9507ddb231"/>
    <rdfs:comment xml:lang="en">Primary strategy for participant identification and follow-up. Types include:
Cohort: Group of individuals, initially defined and composed, with common characteristics (for example, condition, birth year), who are examined or traced over a given time period.
Case-Control: Group of individuals with specific characteristics (for example, conditions or exposures) compared to group(s) with different characteristics, but otherwise similar.
Case-Only: Single group of individuals with specific characteristics.
Case-Crossover: Characteristics of case immediately prior to disease onset (sometimes called the hazard period) compared to characteristics of same case at a prior time (that is, control period).
Ecologic or Community Studies: Geographically defined populations, such as countries or regions within a country, compared on a variety of environmental (for example, air pollution intensity, hours of sunlight) and/or global measures not reducible to individual level characteristics (for example, healthcare system, laws or policies median income, average fat intake, disease rate).
Family-Based: Studies conducted among family members, such as genetic studies within families or twin studies and studies of family environment.
Other: Explain in Detailed Description.
</rdfs:comment>
    <rdfs:comment xml:lang="it">Strategia primaria per l'identificazione dei partecipanti e il follow-up. I tipi includono:
Cohort: Gruppo di individui, inizialmente definiti e composti, con caratteristiche comuni (per esempio, condizione, anno di nascita), che vengono esaminati o tracciati in un determinato periodo di tempo.
Case-Control: Gruppo di individui con caratteristiche specifiche (ad esempio, condizioni o esposizioni) rispetto a gruppi con caratteristiche diverse, ma per il resto simili.
Case-Only: Singolo gruppo di individui con caratteristiche specifiche.
Case-Crossover: Caratteristiche del caso immediatamente prima dell'insorgenza della malattia (talvolta chiamato periodo di pericolo) rispetto alle caratteristiche dello stesso caso in un momento precedente (cioè, periodo di controllo).
Ecologic or Community Studies: Popolazioni geograficamente definite, come paesi o regioni all'interno di un paese, confrontate su una varietà di misure ambientali (ad esempio, intensità dell'inquinamento atmosferico, ore di luce solare) e/o globali non riducibili a caratteristiche di livello individuale (ad esempio, sistema sanitario, leggi o politiche di reddito mediano, assunzione media di grassi, tasso di malattia).
Family-Based: Studi condotti tra i membri della famiglia, come studi genetici all'interno delle famiglie o studi gemelli e studi sull'ambiente familiare.
Altro: Spiegato nella descrizione dettagliata.
</rdfs:comment>
    <rdfs:isDefinedBy rdf:resource="https://w3id.org/italia/onto/HER"/>
    <rdfs:label xml:lang="it">modello osservativo</rdfs:label>
    <rdfs:label xml:lang="en">observational model</rdfs:label>
    <owl:versionInfo xml:lang="it">stabile</owl:versionInfo>
    <owl:versionInfo xml:lang="en">stable</owl:versionInfo>
  </rdf:Description>
  <rdf:Description rdf:nodeID="n5bb3bff42afb4ca286d2c3fead9507ddb466">
    <rdf:type rdf:resource="http://www.w3.org/2002/07/owl#Restriction"/>
    <owl:onProperty rdf:resource="https://w3id.org/italia/onto/HER/hasEurekaCluster"/>
    <owl:maxQualifiedCardinality rdf:datatype="http://www.w3.org/2001/XMLSchema#nonNegativeInteger">1</owl:maxQualifiedCardinality>
    <owl:onClass rdf:resource="https://w3id.org/italia/onto/HER/EUREKACluster"/>
  </rdf:Description>
  <rdf:Description rdf:nodeID="n5bb3bff42afb4ca286d2c3fead9507ddb191">
    <rdf:type rdf:resource="http://www.w3.org/1999/02/22-rdf-syntax-ns#List"/>
    <rdf:first>Triple</rdf:first>
    <rdf:rest rdf:resource="http://www.w3.org/1999/02/22-rdf-syntax-ns#nil"/>
  </rdf:Description>
  <rdf:Description rdf:nodeID="n5bb3bff42afb4ca286d2c3fead9507ddb414">
    <rdf:type rdf:resource="http://www.w3.org/2002/07/owl#Restriction"/>
    <owl:onProperty rdf:resource="https://w3id.org/italia/onto/HER/ctnprinAmountScope"/>
    <owl:maxCardinality rdf:datatype="http://www.w3.org/2001/XMLSchema#nonNegativeInteger">1</owl:maxCardinality>
  </rdf:Description>
  <rdf:Description rdf:nodeID="n5bb3bff42afb4ca286d2c3fead9507ddb442">
    <rdf:type rdf:resource="http://www.w3.org/2002/07/owl#Restriction"/>
    <owl:onProperty rdf:resource="https://w3id.org/italia/onto/HER/rcn"/>
    <owl:cardinality rdf:datatype="http://www.w3.org/2001/XMLSchema#nonNegativeInteger">1</owl:cardinality>
  </rdf:Description>
  <rdf:Description rdf:nodeID="n5bb3bff42afb4ca286d2c3fead9507ddb418">
    <rdf:type rdf:resource="http://www.w3.org/2002/07/owl#Restriction"/>
    <owl:onProperty rdf:resource="https://w3id.org/italia/onto/HER/decreeNumber"/>
    <owl:cardinality rdf:datatype="http://www.w3.org/2001/XMLSchema#nonNegativeInteger">1</owl:cardinality>
  </rdf:Description>
  <rdf:Description rdf:nodeID="n5bb3bff42afb4ca286d2c3fead9507ddb22">
    <rdf:first rdf:resource="https://w3id.org/italia/onto/HER/MIURStudentsByCitizenshipDegreeAggregate"/>
    <rdf:rest rdf:nodeID="n5bb3bff42afb4ca286d2c3fead9507ddb23"/>
  </rdf:Description>
  <rdf:Description rdf:nodeID="n5bb3bff42afb4ca286d2c3fead9507ddb199">
    <rdf:first rdf:resource="https://w3id.org/italia/onto/HER/MIURStudentsByDiplomaAggregate"/>
    <rdf:rest rdf:nodeID="n5bb3bff42afb4ca286d2c3fead9507ddb200"/>
  </rdf:Description>
  <rdf:Description rdf:nodeID="n5bb3bff42afb4ca286d2c3fead9507ddb379">
    <rdf:type rdf:resource="http://www.w3.org/2002/07/owl#Restriction"/>
    <owl:onProperty rdf:resource="https://w3id.org/italia/onto/l0/name"/>
    <owl:allValuesFrom rdf:resource="http://www.w3.org/2000/01/rdf-schema#Literal"/>
  </rdf:Description>
  <rdf:Description rdf:nodeID="n5bb3bff42afb4ca286d2c3fead9507ddb461">
    <rdf:type rdf:resource="http://www.w3.org/2002/07/owl#Restriction"/>
    <owl:onProperty rdf:resource="https://w3id.org/italia/onto/HER/hasParticipationCountry"/>
    <owl:allValuesFrom rdf:resource="https://w3id.org/italia/onto/CLV/Country"/>
  </rdf:Description>
  <rdf:Description rdf:nodeID="n5bb3bff42afb4ca286d2c3fead9507ddb456">
    <rdf:type rdf:resource="http://www.w3.org/2002/07/owl#Restriction"/>
    <owl:onProperty rdf:resource="https://w3id.org/italia/onto/HER/startingYear"/>
    <owl:maxQualifiedCardinality rdf:datatype="http://www.w3.org/2001/XMLSchema#nonNegativeInteger">1</owl:maxQualifiedCardinality>
    <owl:onDataRange rdf:resource="http://www.w3.org/2001/XMLSchema#gYear"/>
  </rdf:Description>
  <rdf:Description rdf:nodeID="n5bb3bff42afb4ca286d2c3fead9507ddb320">
    <rdf:first rdf:resource="https://w3id.org/italia/onto/HER/USTATPartiallyExoneratedStudentsAggregate"/>
    <rdf:rest rdf:nodeID="n5bb3bff42afb4ca286d2c3fead9507ddb321"/>
  </rdf:Description>
  <rdf:Description rdf:nodeID="n5bb3bff42afb4ca286d2c3fead9507ddb503">
    <rdf:type rdf:resource="http://www.w3.org/2002/07/owl#Restriction"/>
    <owl:onProperty rdf:resource="https://w3id.org/italia/onto/HER/patentPriorityDate"/>
    <owl:qualifiedCardinality rdf:datatype="http://www.w3.org/2001/XMLSchema#nonNegativeInteger">1</owl:qualifiedCardinality>
    <owl:onDataRange rdf:resource="http://www.w3.org/2001/XMLSchema#date"/>
  </rdf:Description>
  <rdf:Description rdf:nodeID="n5bb3bff42afb4ca286d2c3fead9507ddb98">
    <rdf:first rdf:resource="https://w3id.org/italia/onto/HER/USTATUniversityInterventionExpensesAggregate"/>
    <rdf:rest rdf:resource="http://www.w3.org/1999/02/22-rdf-syntax-ns#nil"/>
  </rdf:Description>
  <rdf:Description rdf:nodeID="n5bb3bff42afb4ca286d2c3fead9507ddb48">
    <rdf:first rdf:resource="https://w3id.org/italia/onto/HER/ECProject"/>
    <rdf:rest rdf:nodeID="n5bb3bff42afb4ca286d2c3fead9507ddb49"/>
  </rdf:Description>
  <rdf:Description rdf:nodeID="n5bb3bff42afb4ca286d2c3fead9507ddb323">
    <rdf:first rdf:resource="https://w3id.org/italia/onto/HER/USTATPostgraduateAggregateOfEnrolled"/>
    <rdf:rest rdf:nodeID="n5bb3bff42afb4ca286d2c3fead9507ddb324"/>
  </rdf:Description>
  <rdf:Description rdf:nodeID="n5bb3bff42afb4ca286d2c3fead9507ddb103">
    <rdf:first rdf:resource="https://w3id.org/italia/onto/HER/USTATPostgraduateAggregateOfEnrolled"/>
    <rdf:rest rdf:nodeID="n5bb3bff42afb4ca286d2c3fead9507ddb104"/>
  </rdf:Description>
  <rdf:Description rdf:nodeID="n5bb3bff42afb4ca286d2c3fead9507ddb151">
    <rdf:type rdf:resource="http://www.w3.org/1999/02/22-rdf-syntax-ns#List"/>
    <rdf:first>Training</rdf:first>
    <rdf:rest rdf:resource="http://www.w3.org/1999/02/22-rdf-syntax-ns#nil"/>
  </rdf:Description>
  <rdf:Description rdf:nodeID="n5bb3bff42afb4ca286d2c3fead9507ddb71">
    <rdf:first rdf:resource="https://w3id.org/italia/onto/HER/CTNPRINOperation"/>
    <rdf:rest rdf:nodeID="n5bb3bff42afb4ca286d2c3fead9507ddb72"/>
  </rdf:Description>
  <rdf:Description rdf:nodeID="n5bb3bff42afb4ca286d2c3fead9507ddb311">
    <rdf:type rdf:resource="http://www.w3.org/2002/07/owl#Class"/>
    <owl:unionOf rdf:nodeID="n5bb3bff42afb4ca286d2c3fead9507ddb312"/>
  </rdf:Description>
  <rdf:Description rdf:about="https://w3id.org/italia/onto/HER/hasPatentPublicationStage">
    <rdf:type rdf:resource="http://www.w3.org/2002/07/owl#ObjectProperty"/>
    <rdfs:domain rdf:resource="https://w3id.org/italia/onto/HER/PatentPublicationDetail"/>
    <rdfs:range rdf:resource="https://w3id.org/italia/onto/HER/PatentPublicationStage"/>
    <rdfs:comment xml:lang="it">Questa proprietà collega i dettagli della pubblicazione del brevetto con l'attuale fase della pubblicazione.</rdfs:comment>
    <rdfs:comment xml:lang="en">This property connects the publication details of the patent with the current stage of the publication.</rdfs:comment>
    <rdfs:isDefinedBy rdf:resource="https://w3id.org/italia/onto/HER"/>
    <rdfs:label xml:lang="it">ha fase di pubblicazione del brevetto</rdfs:label>
    <rdfs:label xml:lang="en">has patent publication stage</rdfs:label>
    <owl:versionInfo xml:lang="it">stabile</owl:versionInfo>
    <owl:versionInfo xml:lang="en">stable</owl:versionInfo>
  </rdf:Description>
  <rdf:Description rdf:nodeID="n5bb3bff42afb4ca286d2c3fead9507ddb64">
    <rdf:type rdf:resource="http://www.w3.org/2002/07/owl#Class"/>
    <owl:unionOf rdf:nodeID="n5bb3bff42afb4ca286d2c3fead9507ddb65"/>
  </rdf:Description>
  <rdf:Description rdf:nodeID="n5bb3bff42afb4ca286d2c3fead9507ddb457">
    <rdf:type rdf:resource="http://www.w3.org/2002/07/owl#Restriction"/>
    <owl:onProperty rdf:resource="https://w3id.org/italia/onto/l0/description"/>
    <owl:someValuesFrom rdf:resource="http://www.w3.org/2000/01/rdf-schema#Literal"/>
  </rdf:Description>
  <rdf:Description rdf:nodeID="n5bb3bff42afb4ca286d2c3fead9507ddb513">
    <rdf:type rdf:resource="http://www.w3.org/2002/07/owl#Restriction"/>
    <owl:onProperty rdf:resource="https://w3id.org/italia/onto/HER/foundedBy"/>
    <owl:allValuesFrom rdf:resource="https://w3id.org/italia/onto/COV/Organization"/>
  </rdf:Description>
  <rdf:Description rdf:nodeID="n5bb3bff42afb4ca286d2c3fead9507ddb257">
    <rdf:type rdf:resource="http://www.w3.org/1999/02/22-rdf-syntax-ns#List"/>
    <rdf:first>Diagnostic</rdf:first>
    <rdf:rest rdf:nodeID="n5bb3bff42afb4ca286d2c3fead9507ddb258"/>
  </rdf:Description>
  <rdf:Description rdf:nodeID="n5bb3bff42afb4ca286d2c3fead9507ddb101">
    <rdf:first rdf:resource="https://w3id.org/italia/onto/HER/USTATUniversityExpenseClass"/>
    <rdf:rest rdf:resource="http://www.w3.org/1999/02/22-rdf-syntax-ns#nil"/>
  </rdf:Description>
  <rdf:Description rdf:nodeID="n5bb3bff42afb4ca286d2c3fead9507ddb544">
    <rdf:type rdf:resource="http://www.w3.org/2002/07/owl#Restriction"/>
    <owl:onProperty rdf:resource="https://w3id.org/italia/onto/HER/availableSlot"/>
    <owl:maxCardinality rdf:datatype="http://www.w3.org/2001/XMLSchema#nonNegativeInteger">1</owl:maxCardinality>
  </rdf:Description>
  <rdf:Description rdf:nodeID="n5bb3bff42afb4ca286d2c3fead9507ddb495">
    <rdf:type rdf:resource="http://www.w3.org/2002/07/owl#Restriction"/>
    <owl:onProperty rdf:resource="https://w3id.org/italia/onto/CLV/hasSpatialCoverage"/>
    <owl:someValuesFrom rdf:resource="https://w3id.org/italia/onto/CLV/Province"/>
  </rdf:Description>
  <rdf:Description rdf:nodeID="n5bb3bff42afb4ca286d2c3fead9507ddb45">
    <rdf:first rdf:resource="https://w3id.org/italia/onto/HER/ECProject"/>
    <rdf:rest rdf:nodeID="n5bb3bff42afb4ca286d2c3fead9507ddb46"/>
  </rdf:Description>
  <rdf:Description rdf:about="https://w3id.org/italia/onto/HER/eurekaProjectId">
    <rdf:type rdf:resource="http://www.w3.org/2002/07/owl#DatatypeProperty"/>
    <rdfs:subPropertyOf rdf:resource="https://w3id.org/italia/onto/l0/identifier"/>
    <rdfs:domain rdf:resource="https://w3id.org/italia/onto/HER/EUREKAProject"/>
    <rdfs:range rdf:resource="http://www.w3.org/2000/01/rdf-schema#Literal"/>
    <rdfs:comment xml:lang="it">Codice univoco progetto EUREKA</rdfs:comment>
    <rdfs:comment xml:lang="en">EUREKA project unique identifier</rdfs:comment>
    <rdfs:isDefinedBy rdf:resource="https://w3id.org/italia/onto/HER"/>
    <rdfs:label xml:lang="en">EUREKA project ID</rdfs:label>
    <rdfs:label xml:lang="it">ID del progetto EUREKA</rdfs:label>
    <owl:versionInfo xml:lang="it">provvisoria</owl:versionInfo>
    <owl:versionInfo xml:lang="en">unstable</owl:versionInfo>
  </rdf:Description>
  <rdf:Description rdf:nodeID="n5bb3bff42afb4ca286d2c3fead9507ddb408">
    <rdf:type rdf:resource="http://www.w3.org/2002/07/owl#Restriction"/>
    <owl:onProperty rdf:resource="https://w3id.org/italia/onto/l0/hasTopic"/>
    <owl:qualifiedCardinality rdf:datatype="http://www.w3.org/2001/XMLSchema#nonNegativeInteger">1</owl:qualifiedCardinality>
    <owl:onClass rdf:resource="https://w3id.org/italia/onto/HER/CHAFEATopic"/>
  </rdf:Description>
  <rdf:Description rdf:nodeID="n5bb3bff42afb4ca286d2c3fead9507ddb368">
    <rdf:first rdf:resource="https://w3id.org/italia/onto/HER/EUREKAProject"/>
    <rdf:rest rdf:resource="http://www.w3.org/1999/02/22-rdf-syntax-ns#nil"/>
  </rdf:Description>
  <rdf:Description rdf:nodeID="n5bb3bff42afb4ca286d2c3fead9507ddb364">
    <rdf:type rdf:resource="http://www.w3.org/2002/07/owl#Class"/>
    <owl:unionOf rdf:nodeID="n5bb3bff42afb4ca286d2c3fead9507ddb365"/>
  </rdf:Description>
  <rdf:Description rdf:nodeID="n5bb3bff42afb4ca286d2c3fead9507ddb130">
    <rdf:first rdf:resource="https://w3id.org/italia/onto/HER/USTATPostgraduateAggregateOfRegistered"/>
    <rdf:rest rdf:nodeID="n5bb3bff42afb4ca286d2c3fead9507ddb131"/>
  </rdf:Description>
  <rdf:Description rdf:about="https://w3id.org/italia/onto/ADMS/officialURI">
    <rdf:type rdf:resource="http://www.w3.org/2002/07/owl#AnnotationProperty"/>
  </rdf:Description>
  <rdf:Description rdf:about="https://w3id.org/italia/onto/TI#TimeInstant">
    <rdf:type rdf:resource="http://www.w3.org/2002/07/owl#Class"/>
  </rdf:Description>
  <rdf:Description rdf:nodeID="n5bb3bff42afb4ca286d2c3fead9507ddb426">
    <rdf:type rdf:resource="http://www.w3.org/2002/07/owl#Restriction"/>
    <owl:onProperty rdf:resource="https://w3id.org/italia/onto/HER/abstract"/>
    <owl:allValuesFrom rdf:resource="http://www.w3.org/2000/01/rdf-schema#Literal"/>
  </rdf:Description>
  <rdf:Description rdf:nodeID="n5bb3bff42afb4ca286d2c3fead9507ddb403">
    <rdf:type rdf:resource="http://www.w3.org/2002/07/owl#Restriction"/>
    <owl:onProperty rdf:resource="https://w3id.org/italia/onto/l0/identifier"/>
    <owl:cardinality rdf:datatype="http://www.w3.org/2001/XMLSchema#nonNegativeInteger">1</owl:cardinality>
  </rdf:Description>
  <rdf:Description rdf:nodeID="n5bb3bff42afb4ca286d2c3fead9507ddb37">
    <rdf:first rdf:resource="https://w3id.org/italia/onto/HER/ItalianPhDCourseByCycle"/>
    <rdf:rest rdf:resource="http://www.w3.org/1999/02/22-rdf-syntax-ns#nil"/>
  </rdf:Description>
  <rdf:Description rdf:nodeID="n5bb3bff42afb4ca286d2c3fead9507ddb154">
    <rdf:type rdf:resource="http://www.w3.org/1999/02/22-rdf-syntax-ns#List"/>
    <rdf:first>Formazione</rdf:first>
    <rdf:rest rdf:nodeID="n5bb3bff42afb4ca286d2c3fead9507ddb155"/>
  </rdf:Description>
  <rdf:Description rdf:about="https://w3id.org/italia/onto/HER/HERClassification">
    <rdf:type rdf:resource="http://www.w3.org/2002/07/owl#Class"/>
    <rdfs:subClassOf rdf:resource="https://w3id.org/italia/onto/l0/Topic"/>
    <rdfs:isDefinedBy rdf:resource="https://w3id.org/italia/onto/HER"/>
    <rdfs:label xml:lang="it">Classificazione Alta Formazione e Ricerca</rdfs:label>
    <rdfs:label xml:lang="en">HER Classification</rdfs:label>
    <owl:versionInfo xml:lang="it">stabile</owl:versionInfo>
    <owl:versionInfo xml:lang="en">stable</owl:versionInfo>
    <ns6:wasDerivedFrom rdf:resource="http://www.w3.org/2004/02/skos/core#ConceptScheme"/>
  </rdf:Description>
  <rdf:Description rdf:nodeID="n5bb3bff42afb4ca286d2c3fead9507ddb164">
    <rdf:first rdf:resource="https://w3id.org/italia/onto/HER/ERCProject"/>
    <rdf:rest rdf:resource="http://www.w3.org/1999/02/22-rdf-syntax-ns#nil"/>
  </rdf:Description>
  <rdf:Description rdf:about="https://w3id.org/italia/onto/HER/academicYear">
    <rdf:type rdf:resource="http://www.w3.org/2002/07/owl#DatatypeProperty"/>
    <rdfs:subPropertyOf rdf:resource="https://w3id.org/italia/onto/TI/year"/>
    <rdfs:domain rdf:nodeID="n5bb3bff42afb4ca286d2c3fead9507ddb122"/>
    <rdfs:range rdf:resource="http://www.w3.org/2001/XMLSchema#gYear"/>
    <rdfs:comment xml:lang="en">Academic year of reference of the data. The academic year is defined as the period of the year in which a university or other higher education institution carries out its activities in accordance with the regulations in force.</rdfs:comment>
    <rdfs:comment xml:lang="it">Anno Accademico di riferimento dei dati. L'anno accademico viene definito come il periodo dell'anno in cui un'università oppure un altro istituto competente in materia di istruzione superiore svolge la propria attività, in conformità con le normative vigenti.</rdfs:comment>
    <rdfs:isDefinedBy rdf:resource="https://w3id.org/italia/onto/HER"/>
    <rdfs:label xml:lang="en">academic year</rdfs:label>
    <rdfs:label xml:lang="it">anno accademico</rdfs:label>
    <owl:versionInfo xml:lang="it">stabile</owl:versionInfo>
    <owl:versionInfo xml:lang="en">stable</owl:versionInfo>
  </rdf:Description>
  <rdf:Description rdf:nodeID="n5bb3bff42afb4ca286d2c3fead9507ddb296">
    <rdf:type rdf:resource="http://www.w3.org/1999/02/22-rdf-syntax-ns#List"/>
    <rdf:first>Retrospective/Prospective</rdf:first>
    <rdf:rest rdf:resource="http://www.w3.org/1999/02/22-rdf-syntax-ns#nil"/>
  </rdf:Description>
  <rdf:Description rdf:nodeID="n5bb3bff42afb4ca286d2c3fead9507ddb432">
    <rdf:type rdf:resource="http://www.w3.org/2002/07/owl#Restriction"/>
    <owl:onProperty rdf:resource="https://w3id.org/italia/onto/Project/projectAcronym"/>
    <owl:maxCardinality rdf:datatype="http://www.w3.org/2001/XMLSchema#nonNegativeInteger">1</owl:maxCardinality>
  </rdf:Description>
  <rdf:Description rdf:nodeID="n5bb3bff42afb4ca286d2c3fead9507ddb467">
    <rdf:type rdf:resource="http://www.w3.org/2002/07/owl#Restriction"/>
    <owl:onProperty rdf:resource="https://w3id.org/italia/onto/HER/hasEurekaMarketArea"/>
    <owl:maxQualifiedCardinality rdf:datatype="http://www.w3.org/2001/XMLSchema#nonNegativeInteger">1</owl:maxQualifiedCardinality>
    <owl:onClass rdf:resource="https://w3id.org/italia/onto/HER/EUREKAMarketArea"/>
  </rdf:Description>
  <rdf:Description rdf:about="https://w3id.org/italia/onto/COV/Group">
    <rdf:type rdf:resource="http://www.w3.org/2002/07/owl#Class"/>
  </rdf:Description>
  <rdf:Description rdf:nodeID="n5bb3bff42afb4ca286d2c3fead9507ddb380">
    <rdf:type rdf:resource="http://www.w3.org/2002/07/owl#Restriction"/>
    <owl:onProperty rdf:resource="https://w3id.org/italia/onto/HER/sponsorType"/>
    <owl:maxCardinality rdf:datatype="http://www.w3.org/2001/XMLSchema#nonNegativeInteger">1</owl:maxCardinality>
  </rdf:Description>
  <rdf:Description rdf:nodeID="n5bb3bff42afb4ca286d2c3fead9507ddb375">
    <rdf:type rdf:resource="http://www.w3.org/2002/07/owl#Restriction"/>
    <owl:onProperty rdf:resource="https://w3id.org/italia/onto/HER/aactMinimumAge"/>
    <owl:maxQualifiedCardinality rdf:datatype="http://www.w3.org/2001/XMLSchema#nonNegativeInteger">1</owl:maxQualifiedCardinality>
    <owl:onDataRange rdf:resource="http://www.w3.org/2001/XMLSchema#integer"/>
  </rdf:Description>
  <rdf:Description rdf:nodeID="n5bb3bff42afb4ca286d2c3fead9507ddb117">
    <rdf:first rdf:resource="https://w3id.org/italia/onto/HER/USTATPostgraduateAggregateOfRegistered"/>
    <rdf:rest rdf:resource="http://www.w3.org/1999/02/22-rdf-syntax-ns#nil"/>
  </rdf:Description>
  <rdf:Description rdf:nodeID="n5bb3bff42afb4ca286d2c3fead9507ddb228">
    <rdf:first rdf:resource="https://w3id.org/italia/onto/HER/MIURStudentsByProvinceOfResidenceDegreeDegreeClassAggregate"/>
    <rdf:rest rdf:nodeID="n5bb3bff42afb4ca286d2c3fead9507ddb229"/>
  </rdf:Description>
  <rdf:Description rdf:nodeID="n5bb3bff42afb4ca286d2c3fead9507ddb62">
    <rdf:first rdf:resource="https://w3id.org/italia/onto/COV/PublicOrganization"/>
    <rdf:rest rdf:nodeID="n5bb3bff42afb4ca286d2c3fead9507ddb63"/>
  </rdf:Description>
  <rdf:Description rdf:nodeID="n5bb3bff42afb4ca286d2c3fead9507ddb184">
    <rdf:type rdf:resource="http://www.w3.org/1999/02/22-rdf-syntax-ns#List"/>
    <rdf:first>Collaborator</rdf:first>
    <rdf:rest rdf:nodeID="n5bb3bff42afb4ca286d2c3fead9507ddb185"/>
  </rdf:Description>
  <rdf:Description rdf:about="https://w3id.org/italia/onto/ADMS/type">
    <rdf:type rdf:resource="http://www.w3.org/2002/07/owl#AnnotationProperty"/>
  </rdf:Description>
  <rdf:Description rdf:about="https://w3id.org/italia/onto/HER/unicsId">
    <rdf:type rdf:resource="http://www.w3.org/2002/07/owl#DatatypeProperty"/>
    <rdfs:subPropertyOf rdf:resource="https://w3id.org/italia/onto/l0/identifier"/>
    <rdfs:domain rdf:nodeID="n5bb3bff42afb4ca286d2c3fead9507ddb364"/>
    <rdfs:range rdf:resource="http://www.w3.org/2000/01/rdf-schema#Literal"/>
    <rdfs:comment xml:lang="it">Identificativo all'interno della piattaforma UNiCS</rdfs:comment>
    <rdfs:comment xml:lang="en">Identifier in the UNiCS platform.</rdfs:comment>
    <rdfs:isDefinedBy rdf:resource="https://w3id.org/italia/onto/HER"/>
    <rdfs:label xml:lang="it">identificativo in unics</rdfs:label>
    <rdfs:label xml:lang="en">unics identifier</rdfs:label>
    <owl:versionInfo xml:lang="it">stabile</owl:versionInfo>
    <owl:versionInfo xml:lang="en">stable</owl:versionInfo>
  </rdf:Description>
  <rdf:Description rdf:nodeID="n5bb3bff42afb4ca286d2c3fead9507ddb477">
    <rdf:type rdf:resource="http://www.w3.org/2002/07/owl#Restriction"/>
    <owl:onProperty rdf:resource="https://w3id.org/italia/onto/CLV/hasSpatialCoverage"/>
    <owl:allValuesFrom rdf:resource="https://w3id.org/italia/onto/CLV/Feature"/>
  </rdf:Description>
  <rdf:Description rdf:about="https://w3id.org/italia/onto/HER/MIURStudentsByDiplomaAggregate">
    <rdf:type rdf:resource="http://www.w3.org/2002/07/owl#Class"/>
    <rdfs:subClassOf rdf:resource="https://w3id.org/italia/onto/HER/StatisticalDataAggregation"/>
    <rdfs:comment xml:lang="en">Aggregated data on Italian students filed in the MIUR system, grouped by year, university and diploma.</rdfs:comment>
    <rdfs:comment xml:lang="it">Dati aggregati sugli studenti italiani archiviati nel sistema MIUR, raggruppati per anno, università e diploma.</rdfs:comment>
    <rdfs:isDefinedBy rdf:resource="https://w3id.org/italia/onto/HER"/>
    <rdfs:label xml:lang="en">Aggregate of Italian Students By Diploma</rdfs:label>
    <rdfs:label xml:lang="it">Aggregazione dei studenti italiani per diploma</rdfs:label>
    <owl:versionInfo xml:lang="it">stabile</owl:versionInfo>
    <owl:versionInfo xml:lang="en">stable</owl:versionInfo>
  </rdf:Description>
  <rdf:Description rdf:nodeID="n5bb3bff42afb4ca286d2c3fead9507ddb546">
    <rdf:type rdf:resource="http://www.w3.org/2002/07/owl#Restriction"/>
    <owl:onProperty rdf:resource="https://w3id.org/italia/onto/l0/description"/>
    <owl:cardinality rdf:datatype="http://www.w3.org/2001/XMLSchema#nonNegativeInteger">1</owl:cardinality>
  </rdf:Description>
  <rdf:Description rdf:nodeID="n5bb3bff42afb4ca286d2c3fead9507ddb285">
    <rdf:type rdf:resource="http://www.w3.org/1999/02/22-rdf-syntax-ns#List"/>
    <rdf:first>Cross-Sectional</rdf:first>
    <rdf:rest rdf:nodeID="n5bb3bff42afb4ca286d2c3fead9507ddb286"/>
  </rdf:Description>
  <rdf:Description rdf:about="https://w3id.org/italia/onto/ADMS/acronym">
    <rdf:type rdf:resource="http://www.w3.org/2002/07/owl#AnnotationProperty"/>
  </rdf:Description>
  <rdf:Description rdf:nodeID="n5bb3bff42afb4ca286d2c3fead9507ddb524">
    <rdf:type rdf:resource="http://www.w3.org/2002/07/owl#Restriction"/>
    <owl:onProperty rdf:resource="https://w3id.org/italia/onto/HER/innovative"/>
    <owl:qualifiedCardinality rdf:datatype="http://www.w3.org/2001/XMLSchema#nonNegativeInteger">1</owl:qualifiedCardinality>
    <owl:onDataRange rdf:resource="http://www.w3.org/2001/XMLSchema#boolean"/>
  </rdf:Description>
  <rdf:Description rdf:about="https://w3id.org/italia/onto/HER/ErasmusPlusKeyAction">
    <rdf:type rdf:resource="http://www.w3.org/2002/07/owl#Class"/>
    <rdfs:subClassOf rdf:resource="https://w3id.org/italia/onto/HER/ErasmusPlusClassification"/>
    <rdfs:comment xml:lang="en">It refers to the collective name for activities and projects that can be funded under Erasmus+.
There are three Key Action areas which can be summarised as:
- Key Action 1 (Mobility)
- Key Action 2 (Cooperation for Innovation and Exchange of Good Practices)
- Key Action 3 (Support for Policy Reform)</rdfs:comment>
    <rdfs:comment xml:lang="it">Si riferisce al nome collettivo per le attività e i progetti che possono essere finanziati nell'ambito di Erasmus+.
Ci sono tre aree di azione chiave che possono essere riassunte come:
- Azione chiave 1 (Mobilità)
- Azione chiave 2 (Cooperazione per l'innovazione e lo scambio di buone pratiche)
- Azione chiave 3 (Sostegno alla riforma delle politiche)</rdfs:comment>
    <rdfs:isDefinedBy rdf:resource="https://w3id.org/italia/onto/HER"/>
    <rdfs:label xml:lang="it">Azione chiave Erasmus+</rdfs:label>
    <rdfs:label xml:lang="en">Erasmus+ Key Action</rdfs:label>
    <owl:versionInfo xml:lang="it">stabile</owl:versionInfo>
    <owl:versionInfo xml:lang="en">stable</owl:versionInfo>
    <ns6:wasDerivedFrom rdf:resource="http://www.w3.org/2004/02/skos/core#Concept"/>
  </rdf:Description>
  <rdf:Description rdf:nodeID="n5bb3bff42afb4ca286d2c3fead9507ddb317">
    <rdf:first rdf:resource="https://w3id.org/italia/onto/HER/USTATEnrolledStudentsAggregate"/>
    <rdf:rest rdf:nodeID="n5bb3bff42afb4ca286d2c3fead9507ddb318"/>
  </rdf:Description>
  <rdf:Description rdf:nodeID="n5bb3bff42afb4ca286d2c3fead9507ddb355">
    <rdf:first rdf:resource="https://w3id.org/italia/onto/HER/USTATTotallyExoneratedStudentsAggregate"/>
    <rdf:rest rdf:resource="http://www.w3.org/1999/02/22-rdf-syntax-ns#nil"/>
  </rdf:Description>
  <rdf:Description rdf:nodeID="n5bb3bff42afb4ca286d2c3fead9507ddb451">
    <rdf:type rdf:resource="http://www.w3.org/2002/07/owl#Restriction"/>
    <owl:onProperty rdf:resource="https://w3id.org/italia/onto/HER/cordisRef"/>
    <owl:cardinality rdf:datatype="http://www.w3.org/2001/XMLSchema#nonNegativeInteger">1</owl:cardinality>
  </rdf:Description>
  <rdf:Description rdf:nodeID="n5bb3bff42afb4ca286d2c3fead9507ddb219">
    <rdf:first rdf:resource="https://w3id.org/italia/onto/HER/MIURStudentsAggregate"/>
    <rdf:rest rdf:nodeID="n5bb3bff42afb4ca286d2c3fead9507ddb220"/>
  </rdf:Description>
  <rdf:Description rdf:nodeID="n5bb3bff42afb4ca286d2c3fead9507ddb194">
    <rdf:first rdf:resource="https://w3id.org/italia/onto/HER/MIURStudentsByCitizenshipAggregate"/>
    <rdf:rest rdf:nodeID="n5bb3bff42afb4ca286d2c3fead9507ddb195"/>
  </rdf:Description>
  <rdf:Description rdf:nodeID="n5bb3bff42afb4ca286d2c3fead9507ddb269">
    <rdf:first rdf:resource="https://w3id.org/italia/onto/HER/PatentPublicationDetail"/>
    <rdf:rest rdf:nodeID="n5bb3bff42afb4ca286d2c3fead9507ddb270"/>
  </rdf:Description>
  <rdf:Description rdf:nodeID="n5bb3bff42afb4ca286d2c3fead9507ddb26">
    <rdf:first rdf:resource="https://w3id.org/italia/onto/HER/MIURStudentsByDiplomaAggregate"/>
    <rdf:rest rdf:nodeID="n5bb3bff42afb4ca286d2c3fead9507ddb27"/>
  </rdf:Description>
  <rdf:Description rdf:nodeID="n5bb3bff42afb4ca286d2c3fead9507ddb542">
    <rdf:type rdf:resource="http://www.w3.org/2002/07/owl#Restriction"/>
    <owl:onProperty rdf:resource="https://w3id.org/italia/onto/CLV/hasSpatialCoverage"/>
    <owl:allValuesFrom rdf:resource="https://w3id.org/italia/onto/CLV/Feature"/>
  </rdf:Description>
  <rdf:Description rdf:nodeID="n5bb3bff42afb4ca286d2c3fead9507ddb170">
    <rdf:first rdf:resource="https://w3id.org/italia/onto/HER/ECProject"/>
    <rdf:rest rdf:nodeID="n5bb3bff42afb4ca286d2c3fead9507ddb171"/>
  </rdf:Description>
  <rdf:Description rdf:nodeID="n5bb3bff42afb4ca286d2c3fead9507ddb43">
    <rdf:first rdf:resource="https://w3id.org/italia/onto/HER/ERCProject"/>
    <rdf:rest rdf:resource="http://www.w3.org/1999/02/22-rdf-syntax-ns#nil"/>
  </rdf:Description>
  <rdf:Description rdf:nodeID="n5bb3bff42afb4ca286d2c3fead9507ddb259">
    <rdf:type rdf:resource="http://www.w3.org/1999/02/22-rdf-syntax-ns#List"/>
    <rdf:first>Health Services Research</rdf:first>
    <rdf:rest rdf:nodeID="n5bb3bff42afb4ca286d2c3fead9507ddb260"/>
  </rdf:Description>
  <rdf:Description rdf:nodeID="n5bb3bff42afb4ca286d2c3fead9507ddb369">
    <rdf:type rdf:resource="http://www.w3.org/2002/07/owl#Restriction"/>
    <owl:onProperty rdf:resource="https://w3id.org/italia/onto/HER/birthyear"/>
    <owl:maxQualifiedCardinality rdf:datatype="http://www.w3.org/2001/XMLSchema#nonNegativeInteger">1</owl:maxQualifiedCardinality>
    <owl:onDataRange rdf:resource="http://www.w3.org/2001/XMLSchema#gYear"/>
  </rdf:Description>
  <rdf:Description rdf:about="http://www.w3.org/2002/07/owl#maxQualifiedCardinality">
    <rdf:type rdf:resource="http://www.w3.org/2002/07/owl#AnnotationProperty"/>
  </rdf:Description>
  <rdf:Description rdf:nodeID="n5bb3bff42afb4ca286d2c3fead9507ddb243">
    <rdf:type rdf:resource="http://www.w3.org/1999/02/22-rdf-syntax-ns#List"/>
    <rdf:first>Other</rdf:first>
    <rdf:rest rdf:resource="http://www.w3.org/1999/02/22-rdf-syntax-ns#nil"/>
  </rdf:Description>
  <rdf:Description rdf:nodeID="n5bb3bff42afb4ca286d2c3fead9507ddb143">
    <rdf:type rdf:resource="http://www.w3.org/2000/01/rdf-schema#Datatype"/>
    <owl:oneOf rdf:nodeID="n5bb3bff42afb4ca286d2c3fead9507ddb144"/>
  </rdf:Description>
  <rdf:Description rdf:nodeID="n5bb3bff42afb4ca286d2c3fead9507ddb280">
    <rdf:type rdf:resource="http://www.w3.org/2002/07/owl#Class"/>
    <owl:unionOf rdf:nodeID="n5bb3bff42afb4ca286d2c3fead9507ddb281"/>
  </rdf:Description>
  <rdf:Description rdf:nodeID="n5bb3bff42afb4ca286d2c3fead9507ddb68">
    <rdf:first rdf:resource="https://w3id.org/italia/onto/HER/AcademicDegree"/>
    <rdf:rest rdf:nodeID="n5bb3bff42afb4ca286d2c3fead9507ddb69"/>
  </rdf:Description>
  <rdf:Description rdf:nodeID="n5bb3bff42afb4ca286d2c3fead9507ddb237">
    <rdf:type rdf:resource="http://www.w3.org/1999/02/22-rdf-syntax-ns#List"/>
    <rdf:first>Cohort</rdf:first>
    <rdf:rest rdf:nodeID="n5bb3bff42afb4ca286d2c3fead9507ddb238"/>
  </rdf:Description>
  <rdf:Description rdf:nodeID="n5bb3bff42afb4ca286d2c3fead9507ddb547">
    <rdf:type rdf:resource="http://www.w3.org/2002/07/owl#Restriction"/>
    <owl:onProperty rdf:resource="https://w3id.org/italia/onto/l0/identifier"/>
    <owl:cardinality rdf:datatype="http://www.w3.org/2001/XMLSchema#nonNegativeInteger">1</owl:cardinality>
  </rdf:Description>
  <rdf:Description rdf:nodeID="n5bb3bff42afb4ca286d2c3fead9507ddb153">
    <rdf:type rdf:resource="http://www.w3.org/1999/02/22-rdf-syntax-ns#List"/>
    <rdf:first>Basic research</rdf:first>
    <rdf:rest rdf:nodeID="n5bb3bff42afb4ca286d2c3fead9507ddb154"/>
  </rdf:Description>
  <rdf:Description rdf:nodeID="n5bb3bff42afb4ca286d2c3fead9507ddb517">
    <rdf:type rdf:resource="http://www.w3.org/2002/07/owl#Restriction"/>
    <owl:onProperty rdf:resource="https://w3id.org/italia/onto/HER/hasFounderFaculty"/>
    <owl:maxQualifiedCardinality rdf:datatype="http://www.w3.org/2001/XMLSchema#nonNegativeInteger">1</owl:maxQualifiedCardinality>
    <owl:onClass rdf:resource="https://w3id.org/italia/onto/COV/SupportUnit"/>
  </rdf:Description>
  <rdf:Description rdf:nodeID="n5bb3bff42afb4ca286d2c3fead9507ddb271">
    <rdf:type rdf:resource="http://www.w3.org/2000/01/rdf-schema#Datatype"/>
    <owl:oneOf rdf:nodeID="n5bb3bff42afb4ca286d2c3fead9507ddb272"/>
  </rdf:Description>
  <rdf:Description rdf:nodeID="n5bb3bff42afb4ca286d2c3fead9507ddb454">
    <rdf:type rdf:resource="http://www.w3.org/2002/07/owl#Restriction"/>
    <owl:onProperty rdf:resource="https://w3id.org/italia/onto/HER/unicsId"/>
    <owl:cardinality rdf:datatype="http://www.w3.org/2001/XMLSchema#nonNegativeInteger">1</owl:cardinality>
  </rdf:Description>
  <rdf:Description rdf:nodeID="n5bb3bff42afb4ca286d2c3fead9507ddb123">
    <rdf:first rdf:resource="https://w3id.org/italia/onto/HER/DSURightToUniversityStudiesAggregate"/>
    <rdf:rest rdf:nodeID="n5bb3bff42afb4ca286d2c3fead9507ddb124"/>
  </rdf:Description>
  <rdf:Description rdf:nodeID="n5bb3bff42afb4ca286d2c3fead9507ddb239">
    <rdf:type rdf:resource="http://www.w3.org/1999/02/22-rdf-syntax-ns#List"/>
    <rdf:first>Defined Population, Natural History</rdf:first>
    <rdf:rest rdf:nodeID="n5bb3bff42afb4ca286d2c3fead9507ddb240"/>
  </rdf:Description>
  <rdf:Description rdf:nodeID="n5bb3bff42afb4ca286d2c3fead9507ddb358">
    <rdf:first rdf:resource="https://w3id.org/italia/onto/HER/USTATContributionByClass"/>
    <rdf:rest rdf:nodeID="n5bb3bff42afb4ca286d2c3fead9507ddb359"/>
  </rdf:Description>
  <rdf:Description rdf:nodeID="n5bb3bff42afb4ca286d2c3fead9507ddb279">
    <rdf:first rdf:resource="https://w3id.org/italia/onto/HER/ErasmusPlusProject"/>
    <rdf:rest rdf:resource="http://www.w3.org/1999/02/22-rdf-syntax-ns#nil"/>
  </rdf:Description>
  <rdf:Description rdf:nodeID="n5bb3bff42afb4ca286d2c3fead9507ddb427">
    <rdf:type rdf:resource="http://www.w3.org/2002/07/owl#Restriction"/>
    <owl:onProperty rdf:resource="https://w3id.org/italia/onto/HER/admissionDate"/>
    <owl:qualifiedCardinality rdf:datatype="http://www.w3.org/2001/XMLSchema#nonNegativeInteger">1</owl:qualifiedCardinality>
    <owl:onDataRange rdf:resource="http://www.w3.org/2001/XMLSchema#date"/>
  </rdf:Description>
  <rdf:Description rdf:nodeID="n5bb3bff42afb4ca286d2c3fead9507ddb41">
    <rdf:type rdf:resource="http://www.w3.org/2002/07/owl#Class"/>
    <owl:unionOf rdf:nodeID="n5bb3bff42afb4ca286d2c3fead9507ddb42"/>
  </rdf:Description>
  <rdf:Description rdf:nodeID="n5bb3bff42afb4ca286d2c3fead9507ddb162">
    <rdf:type rdf:resource="http://www.w3.org/2002/07/owl#Class"/>
    <owl:unionOf rdf:nodeID="n5bb3bff42afb4ca286d2c3fead9507ddb163"/>
  </rdf:Description>
  <rdf:Description rdf:nodeID="n5bb3bff42afb4ca286d2c3fead9507ddb382">
    <rdf:type rdf:resource="http://www.w3.org/2002/07/owl#Restriction"/>
    <owl:onProperty rdf:resource="https://w3id.org/italia/onto/TI/hasDuration"/>
    <owl:allValuesFrom rdf:resource="https://w3id.org/italia/onto/TI/Duration"/>
  </rdf:Description>
  <rdf:Description rdf:nodeID="n5bb3bff42afb4ca286d2c3fead9507ddb102">
    <rdf:type rdf:resource="http://www.w3.org/2002/07/owl#Class"/>
    <owl:unionOf rdf:nodeID="n5bb3bff42afb4ca286d2c3fead9507ddb103"/>
  </rdf:Description>
  <rdf:Description rdf:nodeID="n5bb3bff42afb4ca286d2c3fead9507ddb76">
    <rdf:type rdf:resource="http://www.w3.org/2002/07/owl#Class"/>
    <owl:unionOf rdf:nodeID="n5bb3bff42afb4ca286d2c3fead9507ddb77"/>
  </rdf:Description>
  <rdf:Description rdf:nodeID="n5bb3bff42afb4ca286d2c3fead9507ddb171">
    <rdf:first rdf:resource="https://w3id.org/italia/onto/HER/ERCProject"/>
    <rdf:rest rdf:nodeID="n5bb3bff42afb4ca286d2c3fead9507ddb172"/>
  </rdf:Description>
  <rdf:Description rdf:nodeID="n5bb3bff42afb4ca286d2c3fead9507ddb182">
    <rdf:type rdf:resource="http://www.w3.org/1999/02/22-rdf-syntax-ns#List"/>
    <rdf:first>Recruiting</rdf:first>
    <rdf:rest rdf:resource="http://www.w3.org/1999/02/22-rdf-syntax-ns#nil"/>
  </rdf:Description>
  <rdf:Description rdf:nodeID="n5bb3bff42afb4ca286d2c3fead9507ddb327">
    <rdf:first rdf:resource="https://w3id.org/italia/onto/HER/USTATTAStaffByGender"/>
    <rdf:rest rdf:resource="http://www.w3.org/1999/02/22-rdf-syntax-ns#nil"/>
  </rdf:Description>
  <rdf:Description rdf:nodeID="n5bb3bff42afb4ca286d2c3fead9507ddb523">
    <rdf:type rdf:resource="http://www.w3.org/2002/07/owl#Restriction"/>
    <owl:onProperty rdf:resource="https://w3id.org/italia/onto/HER/founderShareholding"/>
    <owl:qualifiedCardinality rdf:datatype="http://www.w3.org/2001/XMLSchema#nonNegativeInteger">1</owl:qualifiedCardinality>
    <owl:onDataRange rdf:resource="http://www.w3.org/2001/XMLSchema#decimal"/>
  </rdf:Description>
  <rdf:Description rdf:nodeID="n5bb3bff42afb4ca286d2c3fead9507ddb9">
    <rdf:first rdf:resource="https://w3id.org/italia/onto/HER/CountryInvolvement"/>
    <rdf:rest rdf:resource="http://www.w3.org/1999/02/22-rdf-syntax-ns#nil"/>
  </rdf:Description>
  <rdf:Description rdf:nodeID="n5bb3bff42afb4ca286d2c3fead9507ddb178">
    <rdf:type rdf:resource="http://www.w3.org/2000/01/rdf-schema#Datatype"/>
    <owl:oneOf rdf:nodeID="n5bb3bff42afb4ca286d2c3fead9507ddb179"/>
  </rdf:Description>
  <rdf:Description rdf:nodeID="n5bb3bff42afb4ca286d2c3fead9507ddb72">
    <rdf:first rdf:resource="https://w3id.org/italia/onto/HER/CTNPRINProject"/>
    <rdf:rest rdf:resource="http://www.w3.org/1999/02/22-rdf-syntax-ns#nil"/>
  </rdf:Description>
  <rdf:Description rdf:nodeID="n5bb3bff42afb4ca286d2c3fead9507ddb161">
    <rdf:first rdf:resource="https://w3id.org/italia/onto/HER/ECParticipant"/>
    <rdf:rest rdf:resource="http://www.w3.org/1999/02/22-rdf-syntax-ns#nil"/>
  </rdf:Description>
  <rdf:Description rdf:nodeID="n5bb3bff42afb4ca286d2c3fead9507ddb144">
    <rdf:type rdf:resource="http://www.w3.org/1999/02/22-rdf-syntax-ns#List"/>
    <rdf:first>Basic research</rdf:first>
    <rdf:rest rdf:nodeID="n5bb3bff42afb4ca286d2c3fead9507ddb145"/>
  </rdf:Description>
  <rdf:Description rdf:nodeID="n5bb3bff42afb4ca286d2c3fead9507ddb381">
    <rdf:type rdf:resource="http://www.w3.org/2002/07/owl#Restriction"/>
    <owl:onProperty rdf:resource="https://w3id.org/italia/onto/HER/hasCountryInvolvement"/>
    <owl:someValuesFrom rdf:resource="https://w3id.org/italia/onto/HER/CountryInvolvement"/>
  </rdf:Description>
  <rdf:Description rdf:nodeID="n5bb3bff42afb4ca286d2c3fead9507ddb255">
    <rdf:type rdf:resource="http://www.w3.org/1999/02/22-rdf-syntax-ns#List"/>
    <rdf:first>Basic Science</rdf:first>
    <rdf:rest rdf:nodeID="n5bb3bff42afb4ca286d2c3fead9507ddb256"/>
  </rdf:Description>
  <rdf:Description rdf:nodeID="n5bb3bff42afb4ca286d2c3fead9507ddb220">
    <rdf:first rdf:resource="https://w3id.org/italia/onto/HER/MIURStudentsByCitizenshipAggregate"/>
    <rdf:rest rdf:nodeID="n5bb3bff42afb4ca286d2c3fead9507ddb221"/>
  </rdf:Description>
  <rdf:Description rdf:nodeID="n5bb3bff42afb4ca286d2c3fead9507ddb281">
    <rdf:first rdf:resource="https://w3id.org/italia/onto/HER/AACTFacility"/>
    <rdf:rest rdf:nodeID="n5bb3bff42afb4ca286d2c3fead9507ddb282"/>
  </rdf:Description>
  <rdf:Description rdf:nodeID="n5bb3bff42afb4ca286d2c3fead9507ddb133">
    <rdf:type rdf:resource="http://www.w3.org/1999/02/22-rdf-syntax-ns#List"/>
    <rdf:first>Non-Randomized</rdf:first>
    <rdf:rest rdf:nodeID="n5bb3bff42afb4ca286d2c3fead9507ddb134"/>
  </rdf:Description>
  <rdf:Description rdf:nodeID="n5bb3bff42afb4ca286d2c3fead9507ddb506">
    <rdf:type rdf:resource="http://www.w3.org/2002/07/owl#Restriction"/>
    <owl:onProperty rdf:resource="https://w3id.org/italia/onto/HER/patentPublicationNumber"/>
    <owl:cardinality rdf:datatype="http://www.w3.org/2001/XMLSchema#nonNegativeInteger">1</owl:cardinality>
  </rdf:Description>
  <rdf:Description rdf:nodeID="n5bb3bff42afb4ca286d2c3fead9507ddb58">
    <rdf:type rdf:resource="http://www.w3.org/2002/07/owl#Class"/>
    <owl:unionOf rdf:nodeID="n5bb3bff42afb4ca286d2c3fead9507ddb59"/>
  </rdf:Description>
  <rdf:Description rdf:nodeID="n5bb3bff42afb4ca286d2c3fead9507ddb150">
    <rdf:type rdf:resource="http://www.w3.org/1999/02/22-rdf-syntax-ns#List"/>
    <rdf:first>Sviluppo</rdf:first>
    <rdf:rest rdf:nodeID="n5bb3bff42afb4ca286d2c3fead9507ddb151"/>
  </rdf:Description>
  <rdf:Description rdf:nodeID="n5bb3bff42afb4ca286d2c3fead9507ddb81">
    <rdf:type rdf:resource="http://www.w3.org/2002/07/owl#Class"/>
    <owl:unionOf rdf:nodeID="n5bb3bff42afb4ca286d2c3fead9507ddb82"/>
  </rdf:Description>
  <rdf:Description rdf:about="http://www.w3.org/ns/dcat#theme">
    <rdf:type rdf:resource="http://www.w3.org/2002/07/owl#AnnotationProperty"/>
  </rdf:Description>
  <rdf:Description rdf:nodeID="n5bb3bff42afb4ca286d2c3fead9507ddb332">
    <rdf:type rdf:resource="http://www.w3.org/2002/07/owl#Class"/>
    <owl:unionOf rdf:nodeID="n5bb3bff42afb4ca286d2c3fead9507ddb333"/>
  </rdf:Description>
  <rdf:Description rdf:nodeID="n5bb3bff42afb4ca286d2c3fead9507ddb99">
    <rdf:type rdf:resource="http://www.w3.org/2002/07/owl#Class"/>
    <owl:unionOf rdf:nodeID="n5bb3bff42afb4ca286d2c3fead9507ddb100"/>
  </rdf:Description>
  <rdf:Description rdf:nodeID="n5bb3bff42afb4ca286d2c3fead9507ddb157">
    <rdf:type rdf:resource="http://www.w3.org/1999/02/22-rdf-syntax-ns#List"/>
    <rdf:first>Ricerca di base</rdf:first>
    <rdf:rest rdf:nodeID="n5bb3bff42afb4ca286d2c3fead9507ddb158"/>
  </rdf:Description>
  <rdf:Description rdf:nodeID="n5bb3bff42afb4ca286d2c3fead9507ddb344">
    <rdf:first rdf:resource="https://w3id.org/italia/onto/HER/USTATTAStaffByGender"/>
    <rdf:rest rdf:resource="http://www.w3.org/1999/02/22-rdf-syntax-ns#nil"/>
  </rdf:Description>
  <rdf:Description rdf:nodeID="n5bb3bff42afb4ca286d2c3fead9507ddb87">
    <rdf:first rdf:resource="https://w3id.org/italia/onto/HER/AACTStudy"/>
    <rdf:rest rdf:nodeID="n5bb3bff42afb4ca286d2c3fead9507ddb88"/>
  </rdf:Description>
  <rdf:Description rdf:nodeID="n5bb3bff42afb4ca286d2c3fead9507ddb222">
    <rdf:first rdf:resource="https://w3id.org/italia/onto/HER/MIURStudentsByCitizenshipDegreeClassAggregate"/>
    <rdf:rest rdf:nodeID="n5bb3bff42afb4ca286d2c3fead9507ddb223"/>
  </rdf:Description>
  <rdf:Description rdf:nodeID="n5bb3bff42afb4ca286d2c3fead9507ddb393">
    <rdf:type rdf:resource="http://www.w3.org/2002/07/owl#Restriction"/>
    <owl:onProperty rdf:resource="https://w3id.org/italia/onto/HER/studiesFDARegulatedDevice"/>
    <owl:maxQualifiedCardinality rdf:datatype="http://www.w3.org/2001/XMLSchema#nonNegativeInteger">1</owl:maxQualifiedCardinality>
    <owl:onDataRange rdf:resource="http://www.w3.org/2001/XMLSchema#boolean"/>
  </rdf:Description>
  <rdf:Description rdf:nodeID="n5bb3bff42afb4ca286d2c3fead9507ddb315">
    <rdf:first rdf:resource="https://w3id.org/italia/onto/HER/DSURightToUniversityStudiesAggregate"/>
    <rdf:rest rdf:nodeID="n5bb3bff42afb4ca286d2c3fead9507ddb316"/>
  </rdf:Description>
  <rdf:Description rdf:nodeID="n5bb3bff42afb4ca286d2c3fead9507ddb367">
    <rdf:first rdf:resource="https://w3id.org/italia/onto/HER/ERCProject"/>
    <rdf:rest rdf:nodeID="n5bb3bff42afb4ca286d2c3fead9507ddb368"/>
  </rdf:Description>
  <rdf:Description rdf:nodeID="n5bb3bff42afb4ca286d2c3fead9507ddb69">
    <rdf:first rdf:resource="https://w3id.org/italia/onto/HER/USTATStudentsBySexAggregate"/>
    <rdf:rest rdf:resource="http://www.w3.org/1999/02/22-rdf-syntax-ns#nil"/>
  </rdf:Description>
  <rdf:Description rdf:nodeID="n5bb3bff42afb4ca286d2c3fead9507ddb532">
    <rdf:type rdf:resource="http://www.w3.org/2002/07/owl#Restriction"/>
    <owl:onProperty rdf:resource="https://w3id.org/italia/onto/CLV/hasSpatialCoverage"/>
    <owl:allValuesFrom rdf:resource="https://w3id.org/italia/onto/CLV/Feature"/>
  </rdf:Description>
  <rdf:Description rdf:nodeID="n5bb3bff42afb4ca286d2c3fead9507ddb321">
    <rdf:first rdf:resource="https://w3id.org/italia/onto/HER/USTATTotallyExoneratedStudentsAggregate"/>
    <rdf:rest rdf:resource="http://www.w3.org/1999/02/22-rdf-syntax-ns#nil"/>
  </rdf:Description>
  <rdf:Description rdf:nodeID="n5bb3bff42afb4ca286d2c3fead9507ddb521">
    <rdf:type rdf:resource="http://www.w3.org/2002/07/owl#Restriction"/>
    <owl:onProperty rdf:resource="https://w3id.org/italia/onto/HER/founderCapital"/>
    <owl:qualifiedCardinality rdf:datatype="http://www.w3.org/2001/XMLSchema#nonNegativeInteger">1</owl:qualifiedCardinality>
    <owl:onDataRange rdf:resource="http://www.w3.org/2001/XMLSchema#decimal"/>
  </rdf:Description>
  <rdf:Description rdf:nodeID="n5bb3bff42afb4ca286d2c3fead9507ddb291">
    <rdf:type rdf:resource="http://www.w3.org/1999/02/22-rdf-syntax-ns#List"/>
    <rdf:first>Longitudinal, Retrospective</rdf:first>
    <rdf:rest rdf:nodeID="n5bb3bff42afb4ca286d2c3fead9507ddb292"/>
  </rdf:Description>
  <rdf:Description rdf:nodeID="n5bb3bff42afb4ca286d2c3fead9507ddb482">
    <rdf:type rdf:resource="http://www.w3.org/2002/07/owl#Restriction"/>
    <owl:onProperty rdf:resource="https://w3id.org/italia/onto/HER/hasErasmusPlusParticipant"/>
    <owl:someValuesFrom rdf:resource="https://w3id.org/italia/onto/HER/ErasmusPlusParticipant"/>
  </rdf:Description>
  <rdf:Description rdf:nodeID="n5bb3bff42afb4ca286d2c3fead9507ddb540">
    <rdf:type rdf:resource="http://www.w3.org/2002/07/owl#Restriction"/>
    <owl:onProperty rdf:resource="https://w3id.org/italia/onto/HER/ageClass"/>
    <owl:maxCardinality rdf:datatype="http://www.w3.org/2001/XMLSchema#nonNegativeInteger">1</owl:maxCardinality>
  </rdf:Description>
  <rdf:Description rdf:nodeID="n5bb3bff42afb4ca286d2c3fead9507ddb210">
    <rdf:first rdf:resource="https://w3id.org/italia/onto/HER/MIURStudentsByCitizenshipDegreeDegreeClassAggregate"/>
    <rdf:rest rdf:nodeID="n5bb3bff42afb4ca286d2c3fead9507ddb211"/>
  </rdf:Description>
  <rdf:Description rdf:nodeID="n5bb3bff42afb4ca286d2c3fead9507ddb84">
    <rdf:first rdf:resource="https://w3id.org/italia/onto/HER/MIURStudentsByCitizenshipDegreeClassAggregate"/>
    <rdf:rest rdf:nodeID="n5bb3bff42afb4ca286d2c3fead9507ddb85"/>
  </rdf:Description>
  <rdf:Description rdf:nodeID="n5bb3bff42afb4ca286d2c3fead9507ddb213">
    <rdf:first rdf:resource="https://w3id.org/italia/onto/HER/MIURStudentsByDiplomaDegreeDegreeClassAggregate"/>
    <rdf:rest rdf:nodeID="n5bb3bff42afb4ca286d2c3fead9507ddb214"/>
  </rdf:Description>
  <rdf:Description rdf:nodeID="n5bb3bff42afb4ca286d2c3fead9507ddb352">
    <rdf:first rdf:resource="https://w3id.org/italia/onto/HER/USTATContributionByClass"/>
    <rdf:rest rdf:nodeID="n5bb3bff42afb4ca286d2c3fead9507ddb353"/>
  </rdf:Description>
  <rdf:Description rdf:about="https://w3id.org/italia/onto/ADMS/hasKeyClass">
    <rdf:type rdf:resource="http://www.w3.org/2002/07/owl#AnnotationProperty"/>
  </rdf:Description>
  <rdf:Description rdf:nodeID="n5bb3bff42afb4ca286d2c3fead9507ddb260">
    <rdf:type rdf:resource="http://www.w3.org/1999/02/22-rdf-syntax-ns#List"/>
    <rdf:first>Other</rdf:first>
    <rdf:rest rdf:nodeID="n5bb3bff42afb4ca286d2c3fead9507ddb261"/>
  </rdf:Description>
  <rdf:Description rdf:nodeID="n5bb3bff42afb4ca286d2c3fead9507ddb421">
    <rdf:type rdf:resource="http://www.w3.org/2002/07/owl#Restriction"/>
    <owl:onProperty rdf:resource="https://w3id.org/italia/onto/HER/initiativeType"/>
    <owl:maxCardinality rdf:datatype="http://www.w3.org/2001/XMLSchema#nonNegativeInteger">1</owl:maxCardinality>
  </rdf:Description>
  <rdf:Description rdf:nodeID="n5bb3bff42afb4ca286d2c3fead9507ddb158">
    <rdf:type rdf:resource="http://www.w3.org/1999/02/22-rdf-syntax-ns#List"/>
    <rdf:first>Training</rdf:first>
    <rdf:rest rdf:resource="http://www.w3.org/1999/02/22-rdf-syntax-ns#nil"/>
  </rdf:Description>
  <rdf:Description rdf:nodeID="n5bb3bff42afb4ca286d2c3fead9507ddb128">
    <rdf:first rdf:resource="https://w3id.org/italia/onto/HER/USTATPartiallyExoneratedStudentsAggregate"/>
    <rdf:rest rdf:nodeID="n5bb3bff42afb4ca286d2c3fead9507ddb129"/>
  </rdf:Description>
  <rdf:Description rdf:nodeID="n5bb3bff42afb4ca286d2c3fead9507ddb250">
    <rdf:type rdf:resource="http://www.w3.org/2000/01/rdf-schema#Datatype"/>
    <owl:oneOf rdf:nodeID="n5bb3bff42afb4ca286d2c3fead9507ddb251"/>
  </rdf:Description>
  <rdf:Description rdf:nodeID="n5bb3bff42afb4ca286d2c3fead9507ddb441">
    <rdf:type rdf:resource="http://www.w3.org/2002/07/owl#Restriction"/>
    <owl:onProperty rdf:resource="https://w3id.org/italia/onto/TI/hasYear"/>
    <owl:maxQualifiedCardinality rdf:datatype="http://www.w3.org/2001/XMLSchema#nonNegativeInteger">1</owl:maxQualifiedCardinality>
    <owl:onClass rdf:resource="https://w3id.org/italia/onto/TI/Year"/>
  </rdf:Description>
  <rdf:Description rdf:about="https://w3id.org/italia/onto/ADMS/last">
    <rdf:type rdf:resource="http://www.w3.org/2002/07/owl#AnnotationProperty"/>
  </rdf:Description>
  <rdf:Description rdf:nodeID="n5bb3bff42afb4ca286d2c3fead9507ddb142">
    <rdf:first rdf:resource="https://w3id.org/italia/onto/HER/ERCProject"/>
    <rdf:rest rdf:resource="http://www.w3.org/1999/02/22-rdf-syntax-ns#nil"/>
  </rdf:Description>
  <rdf:Description rdf:nodeID="n5bb3bff42afb4ca286d2c3fead9507ddb549">
    <rdf:type rdf:resource="http://www.w3.org/2002/07/owl#Restriction"/>
    <owl:onProperty rdf:resource="https://w3id.org/italia/onto/HER/abstract"/>
    <owl:allValuesFrom rdf:resource="http://www.w3.org/2000/01/rdf-schema#Literal"/>
  </rdf:Description>
  <rdf:Description rdf:nodeID="n5bb3bff42afb4ca286d2c3fead9507ddb476">
    <rdf:type rdf:resource="http://www.w3.org/2002/07/owl#Restriction"/>
    <owl:onProperty rdf:resource="https://w3id.org/italia/onto/l0/identifier"/>
    <owl:cardinality rdf:datatype="http://www.w3.org/2001/XMLSchema#nonNegativeInteger">1</owl:cardinality>
  </rdf:Description>
  <rdf:Description rdf:nodeID="n5bb3bff42afb4ca286d2c3fead9507ddb53">
    <rdf:type rdf:resource="http://www.w3.org/2002/07/owl#Class"/>
    <owl:unionOf rdf:nodeID="n5bb3bff42afb4ca286d2c3fead9507ddb54"/>
  </rdf:Description>
  <rdf:Description rdf:nodeID="n5bb3bff42afb4ca286d2c3fead9507ddb236">
    <rdf:type rdf:resource="http://www.w3.org/1999/02/22-rdf-syntax-ns#List"/>
    <rdf:first>Case-Only</rdf:first>
    <rdf:rest rdf:nodeID="n5bb3bff42afb4ca286d2c3fead9507ddb237"/>
  </rdf:Description>
  <rdf:Description rdf:nodeID="n5bb3bff42afb4ca286d2c3fead9507ddb159">
    <rdf:type rdf:resource="http://www.w3.org/2002/07/owl#Class"/>
    <owl:unionOf rdf:nodeID="n5bb3bff42afb4ca286d2c3fead9507ddb160"/>
  </rdf:Description>
  <rdf:Description rdf:nodeID="n5bb3bff42afb4ca286d2c3fead9507ddb302">
    <rdf:first rdf:resource="https://w3id.org/italia/onto/HER/USTATUniversityFacilitiesAggregate"/>
    <rdf:rest rdf:resource="http://www.w3.org/1999/02/22-rdf-syntax-ns#nil"/>
  </rdf:Description>
  <rdf:Description rdf:nodeID="n5bb3bff42afb4ca286d2c3fead9507ddb383">
    <rdf:type rdf:resource="http://www.w3.org/2002/07/owl#Restriction"/>
    <owl:onProperty rdf:resource="https://w3id.org/italia/onto/HER/biospecDescription"/>
    <owl:someValuesFrom rdf:resource="http://www.w3.org/2000/01/rdf-schema#Literal"/>
  </rdf:Description>
  <rdf:Description rdf:nodeID="n5bb3bff42afb4ca286d2c3fead9507ddb330">
    <rdf:first rdf:resource="https://w3id.org/italia/onto/HER/USTATPostgraduateAggregateOfGraduated"/>
    <rdf:rest rdf:nodeID="n5bb3bff42afb4ca286d2c3fead9507ddb331"/>
  </rdf:Description>
  <rdf:Description rdf:nodeID="n5bb3bff42afb4ca286d2c3fead9507ddb310">
    <rdf:first rdf:resource="https://w3id.org/italia/onto/HER/USTATTotallyExoneratedStudentsAggregate"/>
    <rdf:rest rdf:resource="http://www.w3.org/1999/02/22-rdf-syntax-ns#nil"/>
  </rdf:Description>
  <rdf:Description rdf:nodeID="n5bb3bff42afb4ca286d2c3fead9507ddb16">
    <rdf:first rdf:resource="https://w3id.org/italia/onto/HER/MIURStudentsByProvinceOfResidenceDegreeDegreeClassAggregate"/>
    <rdf:rest rdf:nodeID="n5bb3bff42afb4ca286d2c3fead9507ddb17"/>
  </rdf:Description>
  <rdf:Description rdf:nodeID="n5bb3bff42afb4ca286d2c3fead9507ddb518">
    <rdf:type rdf:resource="http://www.w3.org/2002/07/owl#Restriction"/>
    <owl:onProperty rdf:resource="https://w3id.org/italia/onto/HER/foundationProjectDescription"/>
    <owl:someValuesFrom rdf:resource="http://www.w3.org/2000/01/rdf-schema#Literal"/>
  </rdf:Description>
  <rdf:Description rdf:about="https://w3id.org/italia/onto/Project/projectAcronym">
    <rdf:type rdf:resource="http://www.w3.org/2002/07/owl#DatatypeProperty"/>
  </rdf:Description>
  <rdf:Description rdf:nodeID="n5bb3bff42afb4ca286d2c3fead9507ddb297">
    <rdf:type rdf:resource="http://www.w3.org/2002/07/owl#Class"/>
    <owl:unionOf rdf:nodeID="n5bb3bff42afb4ca286d2c3fead9507ddb298"/>
  </rdf:Description>
  <rdf:Description rdf:nodeID="n5bb3bff42afb4ca286d2c3fead9507ddb93">
    <rdf:type rdf:resource="http://www.w3.org/2002/07/owl#Class"/>
    <owl:unionOf rdf:nodeID="n5bb3bff42afb4ca286d2c3fead9507ddb94"/>
  </rdf:Description>
  <rdf:Description rdf:about="https://w3id.org/italia/onto/HER/NotItalian">
    <rdf:type rdf:resource="http://www.w3.org/2002/07/owl#NamedIndividual"/>
    <rdf:type rdf:resource="https://w3id.org/italia/onto/HER/ReportedCitizenship"/>
    <rdfs:isDefinedBy rdf:resource="https://w3id.org/italia/onto/HER"/>
    <rdfs:label xml:lang="it">Non Italiana</rdfs:label>
    <rdfs:label xml:lang="en">Not Italian</rdfs:label>
    <owl:versionInfo xml:lang="it">stabile</owl:versionInfo>
    <owl:versionInfo xml:lang="en">stable</owl:versionInfo>
  </rdf:Description>
  <rdf:Description rdf:nodeID="n5bb3bff42afb4ca286d2c3fead9507ddb431">
    <rdf:type rdf:resource="http://www.w3.org/2002/07/owl#Restriction"/>
    <owl:onProperty rdf:resource="https://w3id.org/italia/onto/HER/revoked"/>
    <owl:maxCardinality rdf:datatype="http://www.w3.org/2001/XMLSchema#nonNegativeInteger">1</owl:maxCardinality>
  </rdf:Description>
  <rdf:Description rdf:nodeID="n5bb3bff42afb4ca286d2c3fead9507ddb459">
    <rdf:type rdf:resource="http://www.w3.org/2002/07/owl#Restriction"/>
    <owl:onProperty rdf:resource="https://w3id.org/italia/onto/HER/hasERCGrantType"/>
    <owl:qualifiedCardinality rdf:datatype="http://www.w3.org/2001/XMLSchema#nonNegativeInteger">1</owl:qualifiedCardinality>
    <owl:onClass rdf:resource="https://w3id.org/italia/onto/HER/ERCGrantType"/>
  </rdf:Description>
  <rdf:Description rdf:nodeID="n5bb3bff42afb4ca286d2c3fead9507ddb38">
    <rdf:type rdf:resource="http://www.w3.org/2002/07/owl#Class"/>
    <owl:unionOf rdf:nodeID="n5bb3bff42afb4ca286d2c3fead9507ddb39"/>
  </rdf:Description>
  <rdf:Description rdf:nodeID="n5bb3bff42afb4ca286d2c3fead9507ddb520">
    <rdf:type rdf:resource="http://www.w3.org/2002/07/owl#Restriction"/>
    <owl:onProperty rdf:resource="https://w3id.org/italia/onto/HER/active"/>
    <owl:qualifiedCardinality rdf:datatype="http://www.w3.org/2001/XMLSchema#nonNegativeInteger">1</owl:qualifiedCardinality>
    <owl:onDataRange rdf:resource="http://www.w3.org/2001/XMLSchema#boolean"/>
  </rdf:Description>
  <rdf:Description rdf:nodeID="n5bb3bff42afb4ca286d2c3fead9507ddb274">
    <rdf:type rdf:resource="http://www.w3.org/2002/07/owl#Class"/>
    <owl:unionOf rdf:nodeID="n5bb3bff42afb4ca286d2c3fead9507ddb275"/>
  </rdf:Description>
  <rdf:Description rdf:nodeID="n5bb3bff42afb4ca286d2c3fead9507ddb386">
    <rdf:type rdf:resource="http://www.w3.org/2002/07/owl#Restriction"/>
    <owl:onProperty rdf:resource="https://w3id.org/italia/onto/HER/studyFirstSubmittedDate"/>
    <owl:qualifiedCardinality rdf:datatype="http://www.w3.org/2001/XMLSchema#nonNegativeInteger">1</owl:qualifiedCardinality>
    <owl:onDataRange rdf:resource="http://www.w3.org/2001/XMLSchema#date"/>
  </rdf:Description>
  <rdf:Description rdf:nodeID="n5bb3bff42afb4ca286d2c3fead9507ddb360">
    <rdf:first rdf:resource="https://w3id.org/italia/onto/HER/USTATInterventionExpensesAggregate"/>
    <rdf:rest rdf:nodeID="n5bb3bff42afb4ca286d2c3fead9507ddb361"/>
  </rdf:Description>
  <rdf:Description rdf:nodeID="n5bb3bff42afb4ca286d2c3fead9507ddb149">
    <rdf:type rdf:resource="http://www.w3.org/1999/02/22-rdf-syntax-ns#List"/>
    <rdf:first>Ricerca industriale</rdf:first>
    <rdf:rest rdf:nodeID="n5bb3bff42afb4ca286d2c3fead9507ddb150"/>
  </rdf:Description>
  <rdf:Description rdf:nodeID="n5bb3bff42afb4ca286d2c3fead9507ddb183">
    <rdf:type rdf:resource="http://www.w3.org/2000/01/rdf-schema#Datatype"/>
    <owl:oneOf rdf:nodeID="n5bb3bff42afb4ca286d2c3fead9507ddb184"/>
  </rdf:Description>
  <rdf:Description rdf:nodeID="n5bb3bff42afb4ca286d2c3fead9507ddb198">
    <rdf:first rdf:resource="https://w3id.org/italia/onto/HER/MIURStudentsByDegreeDegreeClassAggregate"/>
    <rdf:rest rdf:nodeID="n5bb3bff42afb4ca286d2c3fead9507ddb199"/>
  </rdf:Description>
  <rdf:Description rdf:nodeID="n5bb3bff42afb4ca286d2c3fead9507ddb18">
    <rdf:type rdf:resource="http://www.w3.org/2002/07/owl#Class"/>
    <owl:unionOf rdf:nodeID="n5bb3bff42afb4ca286d2c3fead9507ddb19"/>
  </rdf:Description>
  <rdf:Description rdf:nodeID="n5bb3bff42afb4ca286d2c3fead9507ddb486">
    <rdf:type rdf:resource="http://www.w3.org/2002/07/owl#Restriction"/>
    <owl:onProperty rdf:resource="https://w3id.org/italia/onto/HER/hasErasmusplusActionType"/>
    <owl:qualifiedCardinality rdf:datatype="http://www.w3.org/2001/XMLSchema#nonNegativeInteger">1</owl:qualifiedCardinality>
    <owl:onClass rdf:resource="https://w3id.org/italia/onto/HER/ErasmusPlusActionType"/>
  </rdf:Description>
  <rdf:Description rdf:about="https://w3id.org/italia/onto/ADMS/hasSemanticAssetDistribution">
    <rdf:type rdf:resource="http://www.w3.org/2002/07/owl#AnnotationProperty"/>
  </rdf:Description>
  <rdf:Description rdf:about="https://w3id.org/italia/onto/ADMS/prefix">
    <rdf:type rdf:resource="http://www.w3.org/2002/07/owl#AnnotationProperty"/>
  </rdf:Description>
  <rdf:Description rdf:nodeID="n5bb3bff42afb4ca286d2c3fead9507ddb550">
    <owl:maxQualifiedCardinality rdf:datatype="http://www.w3.org/2001/XMLSchema#nonNegativeInteger">1</owl:maxQualifiedCardinality>
  </rdf:Description>
  <rdf:Description rdf:nodeID="n5bb3bff42afb4ca286d2c3fead9507ddb207">
    <rdf:first rdf:resource="https://w3id.org/italia/onto/HER/MIURStudentsByCitizenshipAggregate"/>
    <rdf:rest rdf:nodeID="n5bb3bff42afb4ca286d2c3fead9507ddb208"/>
  </rdf:Description>
  <rdf:Description rdf:nodeID="n5bb3bff42afb4ca286d2c3fead9507ddb234">
    <rdf:type rdf:resource="http://www.w3.org/1999/02/22-rdf-syntax-ns#List"/>
    <rdf:first>Case-Control</rdf:first>
    <rdf:rest rdf:nodeID="n5bb3bff42afb4ca286d2c3fead9507ddb235"/>
  </rdf:Description>
  <rdf:Description rdf:nodeID="n5bb3bff42afb4ca286d2c3fead9507ddb206">
    <rdf:first rdf:resource="https://w3id.org/italia/onto/HER/MIURStudentsAggregate"/>
    <rdf:rest rdf:nodeID="n5bb3bff42afb4ca286d2c3fead9507ddb207"/>
  </rdf:Description>
  <rdf:Description rdf:nodeID="n5bb3bff42afb4ca286d2c3fead9507ddb91">
    <rdf:first rdf:resource="https://w3id.org/italia/onto/HER/ECProject"/>
    <rdf:rest rdf:nodeID="n5bb3bff42afb4ca286d2c3fead9507ddb92"/>
  </rdf:Description>
  <rdf:Description rdf:nodeID="n5bb3bff42afb4ca286d2c3fead9507ddb85">
    <rdf:first rdf:resource="https://w3id.org/italia/onto/HER/MIURStudentsByCitizenshipDegreeDegreeClassAggregate"/>
    <rdf:rest rdf:resource="http://www.w3.org/1999/02/22-rdf-syntax-ns#nil"/>
  </rdf:Description>
  <rdf:Description rdf:nodeID="n5bb3bff42afb4ca286d2c3fead9507ddb216">
    <rdf:first rdf:resource="https://w3id.org/italia/onto/HER/MIURStudentsByRegionOfResidenceAggregate"/>
    <rdf:rest rdf:nodeID="n5bb3bff42afb4ca286d2c3fead9507ddb217"/>
  </rdf:Description>
  <rdf:Description rdf:nodeID="n5bb3bff42afb4ca286d2c3fead9507ddb193">
    <rdf:first rdf:resource="https://w3id.org/italia/onto/HER/MIURStudentsAggregate"/>
    <rdf:rest rdf:nodeID="n5bb3bff42afb4ca286d2c3fead9507ddb194"/>
  </rdf:Description>
  <rdf:Description rdf:nodeID="n5bb3bff42afb4ca286d2c3fead9507ddb449">
    <rdf:type rdf:resource="http://www.w3.org/2002/07/owl#Restriction"/>
    <owl:onProperty rdf:resource="https://w3id.org/italia/onto/HER/hasERCPanel"/>
    <owl:maxQualifiedCardinality rdf:datatype="http://www.w3.org/2001/XMLSchema#nonNegativeInteger">1</owl:maxQualifiedCardinality>
    <owl:onClass rdf:resource="https://w3id.org/italia/onto/HER/ERCPanel"/>
  </rdf:Description>
  <rdf:Description rdf:nodeID="n5bb3bff42afb4ca286d2c3fead9507ddb77">
    <rdf:first rdf:resource="https://w3id.org/italia/onto/HER/CHAFEAParticipant"/>
    <rdf:rest rdf:nodeID="n5bb3bff42afb4ca286d2c3fead9507ddb78"/>
  </rdf:Description>
  <rdf:Description rdf:nodeID="n5bb3bff42afb4ca286d2c3fead9507ddb545">
    <rdf:type rdf:resource="http://www.w3.org/2002/07/owl#Restriction"/>
    <owl:onProperty rdf:resource="https://w3id.org/italia/onto/COV/hasOrganization"/>
    <owl:maxQualifiedCardinality rdf:datatype="http://www.w3.org/2001/XMLSchema#nonNegativeInteger">1</owl:maxQualifiedCardinality>
    <owl:onClass rdf:resource="https://w3id.org/italia/onto/COV/Organization"/>
  </rdf:Description>
  <rdf:Description rdf:nodeID="n5bb3bff42afb4ca286d2c3fead9507ddb92">
    <rdf:first rdf:resource="https://w3id.org/italia/onto/HER/ERCProject"/>
    <rdf:rest rdf:resource="http://www.w3.org/1999/02/22-rdf-syntax-ns#nil"/>
  </rdf:Description>
  <rdf:Description rdf:nodeID="n5bb3bff42afb4ca286d2c3fead9507ddb488">
    <rdf:type rdf:resource="http://www.w3.org/2002/07/owl#Restriction"/>
    <owl:onProperty rdf:resource="https://w3id.org/italia/onto/HER/hasStartingDate"/>
    <owl:qualifiedCardinality rdf:datatype="http://www.w3.org/2001/XMLSchema#nonNegativeInteger">1</owl:qualifiedCardinality>
    <owl:onClass rdf:resource="https://w3id.org/italia/onto/TI/TimeInstant"/>
  </rdf:Description>
  <rdf:Description rdf:nodeID="n5bb3bff42afb4ca286d2c3fead9507ddb539">
    <rdf:type rdf:resource="http://www.w3.org/2002/07/owl#Restriction"/>
    <owl:onProperty rdf:resource="https://w3id.org/italia/onto/COV/hasOrganization"/>
    <owl:maxQualifiedCardinality rdf:datatype="http://www.w3.org/2001/XMLSchema#nonNegativeInteger">1</owl:maxQualifiedCardinality>
    <owl:onClass rdf:resource="https://w3id.org/italia/onto/COV/Organization"/>
  </rdf:Description>
  <rdf:Description rdf:nodeID="n5bb3bff42afb4ca286d2c3fead9507ddb63">
    <rdf:first rdf:resource="https://w3id.org/italia/onto/COV/SupportUnit"/>
    <rdf:rest rdf:resource="http://www.w3.org/1999/02/22-rdf-syntax-ns#nil"/>
  </rdf:Description>
  <rdf:Description rdf:nodeID="n5bb3bff42afb4ca286d2c3fead9507ddb276">
    <rdf:first rdf:resource="https://w3id.org/italia/onto/HER/ECProject"/>
    <rdf:rest rdf:nodeID="n5bb3bff42afb4ca286d2c3fead9507ddb277"/>
  </rdf:Description>
  <rdf:Description rdf:nodeID="n5bb3bff42afb4ca286d2c3fead9507ddb424">
    <rdf:type rdf:resource="http://www.w3.org/2002/07/owl#Restriction"/>
    <owl:onProperty rdf:resource="https://w3id.org/italia/onto/HER/refersToProject"/>
    <owl:allValuesFrom rdf:resource="https://w3id.org/italia/onto/HER/CTNPRINProject"/>
  </rdf:Description>
  <rdf:Description rdf:nodeID="n5bb3bff42afb4ca286d2c3fead9507ddb357">
    <rdf:first rdf:resource="https://w3id.org/italia/onto/HER/DSURightToUniversityStudiesAggregate"/>
    <rdf:rest rdf:nodeID="n5bb3bff42afb4ca286d2c3fead9507ddb358"/>
  </rdf:Description>
  <rdf:Description rdf:about="https://w3id.org/italia/onto/Project/PublicInvestmentProject">
    <rdf:type rdf:resource="http://www.w3.org/2002/07/owl#Class"/>
  </rdf:Description>
  <rdf:Description rdf:nodeID="n5bb3bff42afb4ca286d2c3fead9507ddb254">
    <rdf:type rdf:resource="http://www.w3.org/2000/01/rdf-schema#Datatype"/>
    <owl:oneOf rdf:nodeID="n5bb3bff42afb4ca286d2c3fead9507ddb255"/>
  </rdf:Description>
  <rdf:Description rdf:nodeID="n5bb3bff42afb4ca286d2c3fead9507ddb384">
    <rdf:type rdf:resource="http://www.w3.org/2002/07/owl#Restriction"/>
    <owl:onProperty rdf:resource="https://w3id.org/italia/onto/HER/title"/>
    <owl:someValuesFrom rdf:resource="http://www.w3.org/2000/01/rdf-schema#Literal"/>
  </rdf:Description>
  <rdf:Description rdf:nodeID="n5bb3bff42afb4ca286d2c3fead9507ddb351">
    <rdf:type rdf:resource="http://www.w3.org/2002/07/owl#Class"/>
    <owl:unionOf rdf:nodeID="n5bb3bff42afb4ca286d2c3fead9507ddb352"/>
  </rdf:Description>
  <rdf:Description rdf:about="https://w3id.org/italia/onto/POI/PointOfInterest">
    <rdf:type rdf:resource="http://www.w3.org/2002/07/owl#Class"/>
  </rdf:Description>
  <rdf:Description rdf:about="https://w3id.org/italia/onto/SM/URL">
    <rdf:type rdf:resource="http://www.w3.org/2002/07/owl#DatatypeProperty"/>
  </rdf:Description>
  <rdf:Description rdf:nodeID="n5bb3bff42afb4ca286d2c3fead9507ddb407">
    <rdf:type rdf:resource="http://www.w3.org/2002/07/owl#Restriction"/>
    <owl:onProperty rdf:resource="https://w3id.org/italia/onto/TI/hasDuration"/>
    <owl:qualifiedCardinality rdf:datatype="http://www.w3.org/2001/XMLSchema#nonNegativeInteger">1</owl:qualifiedCardinality>
    <owl:onClass rdf:resource="https://w3id.org/italia/onto/TI/Duration"/>
  </rdf:Description>
  <rdf:Description rdf:nodeID="n5bb3bff42afb4ca286d2c3fead9507ddb1">
    <rdf:type rdf:resource="http://www.w3.org/2002/07/owl#Class"/>
    <owl:unionOf rdf:nodeID="n5bb3bff42afb4ca286d2c3fead9507ddb2"/>
  </rdf:Description>
  <rdf:Description rdf:nodeID="n5bb3bff42afb4ca286d2c3fead9507ddb538">
    <rdf:type rdf:resource="http://www.w3.org/2002/07/owl#Restriction"/>
    <owl:onProperty rdf:resource="https://w3id.org/italia/onto/l0/identifier"/>
    <owl:someValuesFrom rdf:resource="http://www.w3.org/2000/01/rdf-schema#Literal"/>
  </rdf:Description>
  <rdf:Description rdf:nodeID="n5bb3bff42afb4ca286d2c3fead9507ddb28">
    <rdf:first rdf:resource="https://w3id.org/italia/onto/HER/MIURStudentsByProvinceOfResidenceAggregate"/>
    <rdf:rest rdf:nodeID="n5bb3bff42afb4ca286d2c3fead9507ddb29"/>
  </rdf:Description>
  <rdf:Description rdf:nodeID="n5bb3bff42afb4ca286d2c3fead9507ddb329">
    <rdf:first rdf:resource="https://w3id.org/italia/onto/HER/USTATPostgraduateAggregateOfEnrolled"/>
    <rdf:rest rdf:nodeID="n5bb3bff42afb4ca286d2c3fead9507ddb330"/>
  </rdf:Description>
  <rdf:Description rdf:nodeID="n5bb3bff42afb4ca286d2c3fead9507ddb12">
    <rdf:first rdf:resource="https://w3id.org/italia/onto/HER/MIURStudentsByCitizenshipDegreeAggregate"/>
    <rdf:rest rdf:nodeID="n5bb3bff42afb4ca286d2c3fead9507ddb13"/>
  </rdf:Description>
  <rdf:Description rdf:nodeID="n5bb3bff42afb4ca286d2c3fead9507ddb192">
    <rdf:type rdf:resource="http://www.w3.org/2002/07/owl#Class"/>
    <owl:unionOf rdf:nodeID="n5bb3bff42afb4ca286d2c3fead9507ddb193"/>
  </rdf:Description>
  <rdf:Description rdf:nodeID="n5bb3bff42afb4ca286d2c3fead9507ddb185">
    <rdf:type rdf:resource="http://www.w3.org/1999/02/22-rdf-syntax-ns#List"/>
    <rdf:first>Lead</rdf:first>
    <rdf:rest rdf:resource="http://www.w3.org/1999/02/22-rdf-syntax-ns#nil"/>
  </rdf:Description>
  <rdf:Description rdf:nodeID="n5bb3bff42afb4ca286d2c3fead9507ddb337">
    <rdf:first rdf:resource="https://w3id.org/italia/onto/HER/EUREKAProject"/>
    <rdf:rest rdf:nodeID="n5bb3bff42afb4ca286d2c3fead9507ddb338"/>
  </rdf:Description>
  <rdf:Description rdf:nodeID="n5bb3bff42afb4ca286d2c3fead9507ddb229">
    <rdf:first rdf:resource="https://w3id.org/italia/onto/HER/MIURStudentsByRegionOfResidenceAggregate"/>
    <rdf:rest rdf:nodeID="n5bb3bff42afb4ca286d2c3fead9507ddb230"/>
  </rdf:Description>
  <rdf:Description rdf:nodeID="n5bb3bff42afb4ca286d2c3fead9507ddb105">
    <rdf:first rdf:resource="https://w3id.org/italia/onto/HER/USTATPostgraduateAggregateOfRegistered"/>
    <rdf:rest rdf:resource="http://www.w3.org/1999/02/22-rdf-syntax-ns#nil"/>
  </rdf:Description>
  <rdf:Description rdf:nodeID="n5bb3bff42afb4ca286d2c3fead9507ddb387">
    <rdf:type rdf:resource="http://www.w3.org/2002/07/owl#Restriction"/>
    <owl:onProperty rdf:resource="https://w3id.org/italia/onto/HER/biospecRetention"/>
    <owl:maxCardinality rdf:datatype="http://www.w3.org/2001/XMLSchema#nonNegativeInteger">1</owl:maxCardinality>
  </rdf:Description>
  <rdf:Description rdf:nodeID="n5bb3bff42afb4ca286d2c3fead9507ddb304">
    <rdf:first rdf:resource="https://w3id.org/italia/onto/HER/DSURightToUniversityStudiesAggregate"/>
    <rdf:rest rdf:nodeID="n5bb3bff42afb4ca286d2c3fead9507ddb305"/>
  </rdf:Description>
  <rdf:Description rdf:nodeID="n5bb3bff42afb4ca286d2c3fead9507ddb376">
    <rdf:type rdf:resource="http://www.w3.org/2002/07/owl#Restriction"/>
    <owl:onProperty rdf:resource="https://w3id.org/italia/onto/CLV/hasAddress"/>
    <owl:someValuesFrom rdf:resource="https://w3id.org/italia/onto/CLV/Address"/>
  </rdf:Description>
  <rdf:Description rdf:nodeID="n5bb3bff42afb4ca286d2c3fead9507ddb197">
    <rdf:first rdf:resource="https://w3id.org/italia/onto/HER/MIURStudentsByCitizenshipDegreeDegreeClassAggregate"/>
    <rdf:rest rdf:nodeID="n5bb3bff42afb4ca286d2c3fead9507ddb198"/>
  </rdf:Description>
  <rdf:Description rdf:nodeID="n5bb3bff42afb4ca286d2c3fead9507ddb97">
    <rdf:first rdf:resource="https://w3id.org/italia/onto/HER/USTATInterventionExpensesAggregate"/>
    <rdf:rest rdf:nodeID="n5bb3bff42afb4ca286d2c3fead9507ddb98"/>
  </rdf:Description>
  <rdf:Description rdf:nodeID="n5bb3bff42afb4ca286d2c3fead9507ddb326">
    <rdf:first rdf:resource="https://w3id.org/italia/onto/HER/USTATStaffByGender"/>
    <rdf:rest rdf:nodeID="n5bb3bff42afb4ca286d2c3fead9507ddb327"/>
  </rdf:Description>
  <rdf:Description rdf:about="https://w3id.org/italia/onto/CPV/hasSex">
    <rdf:type rdf:resource="http://www.w3.org/2002/07/owl#ObjectProperty"/>
  </rdf:Description>
  <rdf:Description rdf:nodeID="n5bb3bff42afb4ca286d2c3fead9507ddb307">
    <rdf:first rdf:resource="https://w3id.org/italia/onto/HER/USTATInterventionExpensesAggregate"/>
    <rdf:rest rdf:nodeID="n5bb3bff42afb4ca286d2c3fead9507ddb308"/>
  </rdf:Description>
  <rdf:Description rdf:nodeID="n5bb3bff42afb4ca286d2c3fead9507ddb165">
    <rdf:type rdf:resource="http://www.w3.org/2002/07/owl#Class"/>
    <owl:unionOf rdf:nodeID="n5bb3bff42afb4ca286d2c3fead9507ddb166"/>
  </rdf:Description>
  <rdf:Description rdf:nodeID="n5bb3bff42afb4ca286d2c3fead9507ddb212">
    <rdf:first rdf:resource="https://w3id.org/italia/onto/HER/MIURStudentsByDiplomaAggregate"/>
    <rdf:rest rdf:nodeID="n5bb3bff42afb4ca286d2c3fead9507ddb213"/>
  </rdf:Description>
  <rdf:Description rdf:nodeID="n5bb3bff42afb4ca286d2c3fead9507ddb322">
    <rdf:type rdf:resource="http://www.w3.org/2002/07/owl#Class"/>
    <owl:unionOf rdf:nodeID="n5bb3bff42afb4ca286d2c3fead9507ddb323"/>
  </rdf:Description>
  <rdf:Description rdf:nodeID="n5bb3bff42afb4ca286d2c3fead9507ddb422">
    <rdf:type rdf:resource="http://www.w3.org/2002/07/owl#Restriction"/>
    <owl:onProperty rdf:resource="https://w3id.org/italia/onto/HER/allocatesFundsTo"/>
    <owl:someValuesFrom rdf:resource="https://w3id.org/italia/onto/HER/CTNPRINEntity"/>
  </rdf:Description>
  <rdf:Description rdf:nodeID="n5bb3bff42afb4ca286d2c3fead9507ddb266">
    <rdf:first rdf:resource="https://w3id.org/italia/onto/HER/PatentPublicationDetail"/>
    <rdf:rest rdf:nodeID="n5bb3bff42afb4ca286d2c3fead9507ddb267"/>
  </rdf:Description>
  <rdf:Description rdf:nodeID="n5bb3bff42afb4ca286d2c3fead9507ddb30">
    <rdf:first rdf:resource="https://w3id.org/italia/onto/HER/MIURStudentsByRegionOfResidenceAggregate"/>
    <rdf:rest rdf:nodeID="n5bb3bff42afb4ca286d2c3fead9507ddb31"/>
  </rdf:Description>
  <rdf:Description rdf:nodeID="n5bb3bff42afb4ca286d2c3fead9507ddb227">
    <rdf:first rdf:resource="https://w3id.org/italia/onto/HER/MIURStudentsByProvinceOfResidenceAggregate"/>
    <rdf:rest rdf:nodeID="n5bb3bff42afb4ca286d2c3fead9507ddb228"/>
  </rdf:Description>
  <rdf:Description rdf:nodeID="n5bb3bff42afb4ca286d2c3fead9507ddb79">
    <rdf:first rdf:resource="https://w3id.org/italia/onto/HER/EUREKAParticipant"/>
    <rdf:rest rdf:nodeID="n5bb3bff42afb4ca286d2c3fead9507ddb80"/>
  </rdf:Description>
  <rdf:Description rdf:nodeID="n5bb3bff42afb4ca286d2c3fead9507ddb429">
    <rdf:type rdf:resource="http://www.w3.org/2002/07/owl#Restriction"/>
    <owl:onProperty rdf:resource="https://w3id.org/italia/onto/HER/transmissionDate"/>
    <owl:qualifiedCardinality rdf:datatype="http://www.w3.org/2001/XMLSchema#nonNegativeInteger">1</owl:qualifiedCardinality>
    <owl:onDataRange rdf:resource="http://www.w3.org/2001/XMLSchema#date"/>
  </rdf:Description>
  <rdf:Description rdf:nodeID="n5bb3bff42afb4ca286d2c3fead9507ddb273">
    <rdf:type rdf:resource="http://www.w3.org/1999/02/22-rdf-syntax-ns#List"/>
    <rdf:first>Probability Sample</rdf:first>
    <rdf:rest rdf:resource="http://www.w3.org/1999/02/22-rdf-syntax-ns#nil"/>
  </rdf:Description>
  <rdf:Description rdf:nodeID="n5bb3bff42afb4ca286d2c3fead9507ddb334">
    <rdf:first rdf:resource="https://w3id.org/italia/onto/HER/USTATPostgraduateAggregateOfGraduated"/>
    <rdf:rest rdf:nodeID="n5bb3bff42afb4ca286d2c3fead9507ddb335"/>
  </rdf:Description>
  <rdf:Description rdf:nodeID="n5bb3bff42afb4ca286d2c3fead9507ddb95">
    <rdf:first rdf:resource="https://w3id.org/italia/onto/HER/USTATTotallyExoneratedStudentsAggregate"/>
    <rdf:rest rdf:resource="http://www.w3.org/1999/02/22-rdf-syntax-ns#nil"/>
  </rdf:Description>
  <rdf:Description rdf:nodeID="n5bb3bff42afb4ca286d2c3fead9507ddb284">
    <rdf:type rdf:resource="http://www.w3.org/2000/01/rdf-schema#Datatype"/>
    <owl:oneOf rdf:nodeID="n5bb3bff42afb4ca286d2c3fead9507ddb285"/>
  </rdf:Description>
  <rdf:Description rdf:nodeID="n5bb3bff42afb4ca286d2c3fead9507ddb489">
    <rdf:type rdf:resource="http://www.w3.org/2002/07/owl#Restriction"/>
    <owl:onProperty rdf:resource="https://w3id.org/italia/onto/HER/status"/>
    <owl:someValuesFrom rdf:resource="http://www.w3.org/2000/01/rdf-schema#Literal"/>
  </rdf:Description>
  <rdf:Description rdf:nodeID="n5bb3bff42afb4ca286d2c3fead9507ddb44">
    <rdf:type rdf:resource="http://www.w3.org/2002/07/owl#Class"/>
    <owl:unionOf rdf:nodeID="n5bb3bff42afb4ca286d2c3fead9507ddb45"/>
  </rdf:Description>
  <rdf:Description rdf:nodeID="n5bb3bff42afb4ca286d2c3fead9507ddb348">
    <rdf:first rdf:resource="https://w3id.org/italia/onto/HER/USTATInterventionsForStudentsByUniversitiesAggregate"/>
    <rdf:rest rdf:nodeID="n5bb3bff42afb4ca286d2c3fead9507ddb349"/>
  </rdf:Description>
  <rdf:Description rdf:about="https://w3id.org/italia/onto/ADMS/hasTask">
    <rdf:type rdf:resource="http://www.w3.org/2002/07/owl#AnnotationProperty"/>
  </rdf:Description>
  <rdf:Description rdf:nodeID="n5bb3bff42afb4ca286d2c3fead9507ddb277">
    <rdf:first rdf:resource="https://w3id.org/italia/onto/HER/ERCProject"/>
    <rdf:rest rdf:nodeID="n5bb3bff42afb4ca286d2c3fead9507ddb278"/>
  </rdf:Description>
  <rdf:Description rdf:nodeID="n5bb3bff42afb4ca286d2c3fead9507ddb294">
    <rdf:type rdf:resource="http://www.w3.org/1999/02/22-rdf-syntax-ns#List"/>
    <rdf:first>Prospective</rdf:first>
    <rdf:rest rdf:nodeID="n5bb3bff42afb4ca286d2c3fead9507ddb295"/>
  </rdf:Description>
  <rdf:Description rdf:nodeID="n5bb3bff42afb4ca286d2c3fead9507ddb231">
    <rdf:type rdf:resource="http://www.w3.org/2000/01/rdf-schema#Datatype"/>
    <owl:oneOf rdf:nodeID="n5bb3bff42afb4ca286d2c3fead9507ddb232"/>
  </rdf:Description>
  <rdf:Description rdf:nodeID="n5bb3bff42afb4ca286d2c3fead9507ddb201">
    <rdf:first rdf:resource="https://w3id.org/italia/onto/HER/MIURStudentsByProvinceOfResidenceAggregate"/>
    <rdf:rest rdf:nodeID="n5bb3bff42afb4ca286d2c3fead9507ddb202"/>
  </rdf:Description>
  <rdf:Description rdf:nodeID="n5bb3bff42afb4ca286d2c3fead9507ddb4">
    <rdf:type rdf:resource="http://www.w3.org/2002/07/owl#Class"/>
    <owl:unionOf rdf:nodeID="n5bb3bff42afb4ca286d2c3fead9507ddb5"/>
  </rdf:Description>
  <rdf:Description rdf:nodeID="n5bb3bff42afb4ca286d2c3fead9507ddb34">
    <rdf:first rdf:resource="https://w3id.org/italia/onto/HER/ItalianAcademicRole"/>
    <rdf:rest rdf:resource="http://www.w3.org/1999/02/22-rdf-syntax-ns#nil"/>
  </rdf:Description>
  <rdf:Description rdf:nodeID="n5bb3bff42afb4ca286d2c3fead9507ddb127">
    <rdf:first rdf:resource="https://w3id.org/italia/onto/HER/USTATInterventionsForStudentsByUniversitiesAggregate"/>
    <rdf:rest rdf:nodeID="n5bb3bff42afb4ca286d2c3fead9507ddb128"/>
  </rdf:Description>
  <rdf:Description rdf:nodeID="n5bb3bff42afb4ca286d2c3fead9507ddb349">
    <rdf:first rdf:resource="https://w3id.org/italia/onto/HER/USTATPartiallyExoneratedStudentsAggregate"/>
    <rdf:rest rdf:nodeID="n5bb3bff42afb4ca286d2c3fead9507ddb350"/>
  </rdf:Description>
  <rdf:Description rdf:nodeID="n5bb3bff42afb4ca286d2c3fead9507ddb300">
    <rdf:first rdf:resource="https://w3id.org/italia/onto/HER/USTATPermanentStaff"/>
    <rdf:rest rdf:nodeID="n5bb3bff42afb4ca286d2c3fead9507ddb301"/>
  </rdf:Description>
  <rdf:Description rdf:nodeID="n5bb3bff42afb4ca286d2c3fead9507ddb265">
    <rdf:type rdf:resource="http://www.w3.org/2002/07/owl#Class"/>
    <owl:unionOf rdf:nodeID="n5bb3bff42afb4ca286d2c3fead9507ddb266"/>
  </rdf:Description>
  <rdf:Description rdf:nodeID="n5bb3bff42afb4ca286d2c3fead9507ddb57">
    <rdf:first rdf:resource="https://w3id.org/italia/onto/HER/ERCProject"/>
    <rdf:rest rdf:resource="http://www.w3.org/1999/02/22-rdf-syntax-ns#nil"/>
  </rdf:Description>
  <rdf:Description rdf:nodeID="n5bb3bff42afb4ca286d2c3fead9507ddb223">
    <rdf:first rdf:resource="https://w3id.org/italia/onto/HER/MIURStudentsByCitizenshipDegreeDegreeClassAggregate"/>
    <rdf:rest rdf:nodeID="n5bb3bff42afb4ca286d2c3fead9507ddb224"/>
  </rdf:Description>
  <rdf:Description rdf:nodeID="n5bb3bff42afb4ca286d2c3fead9507ddb104">
    <rdf:first rdf:resource="https://w3id.org/italia/onto/HER/USTATPostgraduateAggregateOfGraduated"/>
    <rdf:rest rdf:nodeID="n5bb3bff42afb4ca286d2c3fead9507ddb105"/>
  </rdf:Description>
  <rdf:Description rdf:nodeID="n5bb3bff42afb4ca286d2c3fead9507ddb448">
    <rdf:type rdf:resource="http://www.w3.org/2002/07/owl#Restriction"/>
    <owl:onProperty rdf:resource="https://w3id.org/italia/onto/HER/hasECFrameworkProgramme"/>
    <owl:qualifiedCardinality rdf:datatype="http://www.w3.org/2001/XMLSchema#nonNegativeInteger">1</owl:qualifiedCardinality>
    <owl:onClass rdf:resource="https://w3id.org/italia/onto/HER/ECFrameworkProgramme"/>
  </rdf:Description>
  <rdf:Description rdf:nodeID="n5bb3bff42afb4ca286d2c3fead9507ddb249">
    <rdf:first rdf:resource="https://w3id.org/italia/onto/HER/ErasmusPlusParticipant"/>
    <rdf:rest rdf:resource="http://www.w3.org/1999/02/22-rdf-syntax-ns#nil"/>
  </rdf:Description>
  <rdf:Description rdf:nodeID="n5bb3bff42afb4ca286d2c3fead9507ddb168">
    <rdf:type rdf:resource="http://www.w3.org/2002/07/owl#Class"/>
    <owl:unionOf rdf:nodeID="n5bb3bff42afb4ca286d2c3fead9507ddb169"/>
  </rdf:Description>
  <rdf:Description rdf:nodeID="n5bb3bff42afb4ca286d2c3fead9507ddb335">
    <rdf:first rdf:resource="https://w3id.org/italia/onto/HER/USTATPostgraduateAggregateOfRegistered"/>
    <rdf:rest rdf:resource="http://www.w3.org/1999/02/22-rdf-syntax-ns#nil"/>
  </rdf:Description>
  <rdf:Description rdf:about="http://purl.org/dc/terms/accrualPeriodicity">
    <rdf:type rdf:resource="http://www.w3.org/2002/07/owl#AnnotationProperty"/>
  </rdf:Description>
  <rdf:Description rdf:about="https://w3id.org/italia/onto/ADMS/hasFormalityLevel">
    <rdf:type rdf:resource="http://www.w3.org/2002/07/owl#AnnotationProperty"/>
  </rdf:Description>
  <rdf:Description rdf:nodeID="n5bb3bff42afb4ca286d2c3fead9507ddb362">
    <rdf:first rdf:resource="https://w3id.org/italia/onto/HER/USTATPartiallyExoneratedStudentsAggregate"/>
    <rdf:rest rdf:nodeID="n5bb3bff42afb4ca286d2c3fead9507ddb363"/>
  </rdf:Description>
  <rdf:Description rdf:nodeID="n5bb3bff42afb4ca286d2c3fead9507ddb416">
    <rdf:type rdf:resource="http://www.w3.org/2002/07/owl#Restriction"/>
    <owl:onProperty rdf:resource="https://w3id.org/italia/onto/HER/ctnprinAvailableBudget"/>
    <owl:maxCardinality rdf:datatype="http://www.w3.org/2001/XMLSchema#nonNegativeInteger">1</owl:maxCardinality>
  </rdf:Description>
  <rdf:Description rdf:about="https://w3id.org/italia/onto/ADMS/target">
    <rdf:type rdf:resource="http://www.w3.org/2002/07/owl#AnnotationProperty"/>
  </rdf:Description>
  <rdf:Description rdf:nodeID="n5bb3bff42afb4ca286d2c3fead9507ddb204">
    <rdf:first rdf:resource="https://w3id.org/italia/onto/HER/MIURStudentsByRegionOfResidenceDegreeDegreeClassAggregate"/>
    <rdf:rest rdf:resource="http://www.w3.org/1999/02/22-rdf-syntax-ns#nil"/>
  </rdf:Description>
  <rdf:Description rdf:about="https://w3id.org/italia/onto/CPV/familyName">
    <rdf:type rdf:resource="http://www.w3.org/2002/07/owl#DatatypeProperty"/>
  </rdf:Description>
  <rdf:Description rdf:nodeID="n5bb3bff42afb4ca286d2c3fead9507ddb59">
    <rdf:first rdf:resource="https://w3id.org/italia/onto/HER/CTNPRINOperation"/>
    <rdf:rest rdf:nodeID="n5bb3bff42afb4ca286d2c3fead9507ddb60"/>
  </rdf:Description>
  <rdf:Description rdf:about="https://w3id.org/italia/onto/CPV/Sex">
    <rdf:type rdf:resource="http://www.w3.org/2002/07/owl#Class"/>
  </rdf:Description>
  <rdf:Description rdf:about="https://w3id.org/italia/onto/CPV/sexDesc">
    <rdf:type rdf:resource="http://www.w3.org/2002/07/owl#DatatypeProperty"/>
  </rdf:Description>
  <rdf:Description rdf:about="https://w3id.org/italia/onto/COV/PrivateOrganization">
    <rdf:type rdf:resource="http://www.w3.org/2002/07/owl#Class"/>
  </rdf:Description>
  <rdf:Description rdf:about="https://w3id.org/italia/onto/HER/editionLabel">
    <rdf:type rdf:resource="http://www.w3.org/2002/07/owl#DatatypeProperty"/>
  </rdf:Description>
  <rdf:Description rdf:about="https://w3id.org/italia/onto/ADMS/semanticAssetInUse">
    <rdf:type rdf:resource="http://www.w3.org/2002/07/owl#AnnotationProperty"/>
  </rdf:Description>
  <rdf:Description rdf:nodeID="n5bb3bff42afb4ca286d2c3fead9507ddb66">
    <rdf:first rdf:resource="https://w3id.org/italia/onto/HER/ERCProject"/>
    <rdf:rest rdf:resource="http://www.w3.org/1999/02/22-rdf-syntax-ns#nil"/>
  </rdf:Description>
  <rdf:Description rdf:nodeID="n5bb3bff42afb4ca286d2c3fead9507ddb90">
    <rdf:type rdf:resource="http://www.w3.org/2002/07/owl#Class"/>
    <owl:unionOf rdf:nodeID="n5bb3bff42afb4ca286d2c3fead9507ddb91"/>
  </rdf:Description>
  <rdf:Description rdf:nodeID="n5bb3bff42afb4ca286d2c3fead9507ddb14">
    <rdf:first rdf:resource="https://w3id.org/italia/onto/HER/MIURStudentsByDegreeDegreeClassAggregate"/>
    <rdf:rest rdf:nodeID="n5bb3bff42afb4ca286d2c3fead9507ddb15"/>
  </rdf:Description>
  <rdf:Description rdf:about="https://w3id.org/italia/onto/COV/VATnumber">
    <rdf:type rdf:resource="http://www.w3.org/2002/07/owl#DatatypeProperty"/>
  </rdf:Description>
  <rdf:Description rdf:nodeID="n5bb3bff42afb4ca286d2c3fead9507ddb345">
    <rdf:type rdf:resource="http://www.w3.org/2002/07/owl#Class"/>
    <owl:unionOf rdf:nodeID="n5bb3bff42afb4ca286d2c3fead9507ddb346"/>
  </rdf:Description>
  <rdf:Description rdf:nodeID="n5bb3bff42afb4ca286d2c3fead9507ddb241">
    <rdf:type rdf:resource="http://www.w3.org/1999/02/22-rdf-syntax-ns#List"/>
    <rdf:first>Family-Based</rdf:first>
    <rdf:rest rdf:nodeID="n5bb3bff42afb4ca286d2c3fead9507ddb242"/>
  </rdf:Description>
  <rdf:Description rdf:nodeID="n5bb3bff42afb4ca286d2c3fead9507ddb270">
    <rdf:first rdf:resource="https://w3id.org/italia/onto/HER/Result"/>
    <rdf:rest rdf:resource="http://www.w3.org/1999/02/22-rdf-syntax-ns#nil"/>
  </rdf:Description>
  <rdf:Description rdf:nodeID="n5bb3bff42afb4ca286d2c3fead9507ddb23">
    <rdf:first rdf:resource="https://w3id.org/italia/onto/HER/MIURStudentsByCitizenshipDegreeClassAggregate"/>
    <rdf:rest rdf:nodeID="n5bb3bff42afb4ca286d2c3fead9507ddb24"/>
  </rdf:Description>
  <rdf:Description rdf:nodeID="n5bb3bff42afb4ca286d2c3fead9507ddb186">
    <rdf:type rdf:resource="http://www.w3.org/2000/01/rdf-schema#Datatype"/>
    <owl:oneOf rdf:nodeID="n5bb3bff42afb4ca286d2c3fead9507ddb187"/>
  </rdf:Description>
  <rdf:Description rdf:nodeID="n5bb3bff42afb4ca286d2c3fead9507ddb89">
    <rdf:first rdf:resource="https://w3id.org/italia/onto/HER/ErasmusPlusProject"/>
    <rdf:rest rdf:resource="http://www.w3.org/1999/02/22-rdf-syntax-ns#nil"/>
  </rdf:Description>
  <rdf:Description rdf:nodeID="n5bb3bff42afb4ca286d2c3fead9507ddb108">
    <rdf:first rdf:resource="https://w3id.org/italia/onto/HER/USTATInterventionExpensesAggregate"/>
    <rdf:rest rdf:resource="http://www.w3.org/1999/02/22-rdf-syntax-ns#nil"/>
  </rdf:Description>
  <rdf:Description rdf:nodeID="n5bb3bff42afb4ca286d2c3fead9507ddb353">
    <rdf:first rdf:resource="https://w3id.org/italia/onto/HER/USTATInterventionsForStudentsByUniversitiesAggregate"/>
    <rdf:rest rdf:nodeID="n5bb3bff42afb4ca286d2c3fead9507ddb354"/>
  </rdf:Description>
  <rdf:Description rdf:nodeID="n5bb3bff42afb4ca286d2c3fead9507ddb361">
    <rdf:first rdf:resource="https://w3id.org/italia/onto/HER/USTATInterventionsForStudentsByUniversitiesAggregate"/>
    <rdf:rest rdf:nodeID="n5bb3bff42afb4ca286d2c3fead9507ddb362"/>
  </rdf:Description>
  <rdf:Description rdf:about="https://w3id.org/italia/onto/CPV/age">
    <rdf:type rdf:resource="http://www.w3.org/2002/07/owl#DatatypeProperty"/>
  </rdf:Description>
  <rdf:Description rdf:nodeID="n5bb3bff42afb4ca286d2c3fead9507ddb420">
    <rdf:type rdf:resource="http://www.w3.org/2002/07/owl#Restriction"/>
    <owl:onProperty rdf:resource="https://w3id.org/italia/onto/HER/expireDate"/>
    <owl:qualifiedCardinality rdf:datatype="http://www.w3.org/2001/XMLSchema#nonNegativeInteger">1</owl:qualifiedCardinality>
    <owl:onDataRange rdf:resource="http://www.w3.org/2001/XMLSchema#date"/>
  </rdf:Description>
  <rdf:Description rdf:nodeID="n5bb3bff42afb4ca286d2c3fead9507ddb47">
    <rdf:type rdf:resource="http://www.w3.org/2002/07/owl#Class"/>
    <owl:unionOf rdf:nodeID="n5bb3bff42afb4ca286d2c3fead9507ddb48"/>
  </rdf:Description>
  <rdf:Description rdf:nodeID="n5bb3bff42afb4ca286d2c3fead9507ddb40">
    <rdf:first rdf:resource="https://w3id.org/italia/onto/HER/MIURStudentsByDiplomaDegreeDegreeClassAggregate"/>
    <rdf:rest rdf:resource="http://www.w3.org/1999/02/22-rdf-syntax-ns#nil"/>
  </rdf:Description>
  <rdf:Description rdf:nodeID="n5bb3bff42afb4ca286d2c3fead9507ddb32">
    <rdf:type rdf:resource="http://www.w3.org/2002/07/owl#Class"/>
    <owl:unionOf rdf:nodeID="n5bb3bff42afb4ca286d2c3fead9507ddb33"/>
  </rdf:Description>
  <rdf:Description rdf:about="https://w3id.org/italia/onto/RO/forEntity">
    <rdf:type rdf:resource="http://www.w3.org/2002/07/owl#ObjectProperty"/>
  </rdf:Description>
  <rdf:Description rdf:nodeID="n5bb3bff42afb4ca286d2c3fead9507ddb55">
    <rdf:first rdf:resource="https://w3id.org/italia/onto/HER/CTNPRINProject"/>
    <rdf:rest rdf:nodeID="n5bb3bff42afb4ca286d2c3fead9507ddb56"/>
  </rdf:Description>
  <rdf:Description rdf:nodeID="n5bb3bff42afb4ca286d2c3fead9507ddb74">
    <rdf:first rdf:resource="https://w3id.org/italia/onto/HER/CTNPRINAmount"/>
    <rdf:rest rdf:nodeID="n5bb3bff42afb4ca286d2c3fead9507ddb75"/>
  </rdf:Description>
  <rdf:Description rdf:nodeID="n5bb3bff42afb4ca286d2c3fead9507ddb125">
    <rdf:first rdf:resource="https://w3id.org/italia/onto/HER/USTATContributionByClass"/>
    <rdf:rest rdf:nodeID="n5bb3bff42afb4ca286d2c3fead9507ddb126"/>
  </rdf:Description>
  <rdf:Description rdf:about="http://www.w3.org/ns/dcat#contactPoint">
    <rdf:type rdf:resource="http://www.w3.org/2002/07/owl#AnnotationProperty"/>
  </rdf:Description>
  <rdf:Description rdf:nodeID="n5bb3bff42afb4ca286d2c3fead9507ddb160">
    <rdf:first rdf:resource="https://w3id.org/italia/onto/HER/CHAFEAProject"/>
    <rdf:rest rdf:nodeID="n5bb3bff42afb4ca286d2c3fead9507ddb161"/>
  </rdf:Description>
  <rdf:Description rdf:about="https://w3id.org/italia/onto/CPV/givenName">
    <rdf:type rdf:resource="http://www.w3.org/2002/07/owl#DatatypeProperty"/>
  </rdf:Description>
  <rdf:Description rdf:about="https://w3id.org/italia/onto/l0/Collection">
    <rdf:type rdf:resource="http://www.w3.org/2002/07/owl#Class"/>
  </rdf:Description>
  <rdf:Description rdf:about="https://w3id.org/italia/onto/CPV/sexID">
    <rdf:type rdf:resource="http://www.w3.org/2002/07/owl#DatatypeProperty"/>
  </rdf:Description>
  <rdf:Description rdf:nodeID="n5bb3bff42afb4ca286d2c3fead9507ddb78">
    <rdf:first rdf:resource="https://w3id.org/italia/onto/HER/ECParticipant"/>
    <rdf:rest rdf:nodeID="n5bb3bff42afb4ca286d2c3fead9507ddb79"/>
  </rdf:Description>
  <rdf:Description rdf:nodeID="n5bb3bff42afb4ca286d2c3fead9507ddb415">
    <rdf:type rdf:resource="http://www.w3.org/2002/07/owl#Restriction"/>
    <owl:onProperty rdf:resource="https://w3id.org/italia/onto/HER/expenseType"/>
    <owl:maxCardinality rdf:datatype="http://www.w3.org/2001/XMLSchema#nonNegativeInteger">1</owl:maxCardinality>
  </rdf:Description>
  <rdf:Description rdf:about="http://purl.org/dc/terms/rightsHolder">
    <rdf:type rdf:resource="http://www.w3.org/2002/07/owl#AnnotationProperty"/>
  </rdf:Description>
  <rdf:Description rdf:about="https://w3id.org/italia/onto/ADMS/hasOntologyLanguage">
    <rdf:type rdf:resource="http://www.w3.org/2002/07/owl#AnnotationProperty"/>
  </rdf:Description>
  <rdf:Description rdf:about="http://purl.org/dc/terms/publisher">
    <rdf:type rdf:resource="http://www.w3.org/2002/07/owl#AnnotationProperty"/>
  </rdf:Description>
  <rdf:Description rdf:about="https://w3id.org/italia/onto/RO/TimeIndexedRole">
    <rdf:type rdf:resource="http://www.w3.org/2002/07/owl#Class"/>
  </rdf:Description>
  <rdf:Description rdf:about="https://w3id.org/italia/onto/COV/SupportUnit">
    <rdf:type rdf:resource="http://www.w3.org/2002/07/owl#Class"/>
  </rdf:Description>
  <rdf:Description rdf:about="https://w3id.org/italia/onto/l0/hasTopic">
    <rdf:type rdf:resource="http://www.w3.org/2002/07/owl#ObjectProperty"/>
  </rdf:Description>
  <rdf:Description rdf:nodeID="n5bb3bff42afb4ca286d2c3fead9507ddb268">
    <rdf:type rdf:resource="http://www.w3.org/2002/07/owl#Class"/>
    <owl:unionOf rdf:nodeID="n5bb3bff42afb4ca286d2c3fead9507ddb269"/>
  </rdf:Description>
  <rdf:Description rdf:nodeID="n5bb3bff42afb4ca286d2c3fead9507ddb167">
    <rdf:first rdf:resource="https://w3id.org/italia/onto/HER/ERCProject"/>
    <rdf:rest rdf:resource="http://www.w3.org/1999/02/22-rdf-syntax-ns#nil"/>
  </rdf:Description>
  <rdf:Description rdf:nodeID="n5bb3bff42afb4ca286d2c3fead9507ddb341">
    <rdf:first rdf:resource="https://w3id.org/italia/onto/HER/USTATPostgraduateAggregateOfGraduated"/>
    <rdf:rest rdf:nodeID="n5bb3bff42afb4ca286d2c3fead9507ddb342"/>
  </rdf:Description>
  <rdf:Description rdf:about="https://w3id.org/italia/onto/RO/hasRiT">
    <rdf:type rdf:resource="http://www.w3.org/2002/07/owl#ObjectProperty"/>
  </rdf:Description>
  <rdf:Description rdf:about="https://w3id.org/italia/onto/CPV/altName">
    <rdf:type rdf:resource="http://www.w3.org/2002/07/owl#DatatypeProperty"/>
  </rdf:Description>
</rdf:RDF>
