@prefix dct:     <http://purl.org/dc/terms/> .
@prefix adms:    <http://www.w3.org/ns/adms#> .
@prefix rdfs:    <http://www.w3.org/2000/01/rdf-schema#> .
@prefix owl:     <http://www.w3.org/2002/07/owl#> .
@prefix rdf:     <http://www.w3.org/1999/02/22-rdf-syntax-ns#> .
@prefix dc:      <http://purl.org/dc/elements/1.1/> .
@prefix skos:    <http://www.w3.org/2004/02/skos/core#> .
@prefix rtapit:  <https://w3id.org/italia/onto/Route/> .
@prefix xkos:    <http://rdf-vocabulary.ddialliance.org/xkos#> .
@prefix clvapit: <https://w3id.org/italia/onto/CLV/> .
@prefix dcatapit: <http://dati.gov.it/onto/dcatapit#> .
@prefix dcat: <http://www.w3.org/ns/dcat#> .
@prefix foaf: <http://xmlns.com/foaf/0.1/> .
@prefix vcard: <http://www.w3.org/2006/vcard/ns#> .
@prefix xsd: <http://www.w3.org/2001/XMLSchema#> .
@prefix ndc: <https://w3id.org/italia/onto/NDC/> .

skos:ConceptScheme
      a       rdfs:Class .

skos:Concept
      a       rdfs:Class .

rtapit:RouteType
      a       rdfs:Class .

dcatapit:Dataset
      a       rdfs:Class .

dcatapit:Distribution
      a       rdfs:Class .

dcatapit:Standard
      a        rdfs:Class .

dcatapit:Organization
      a        rdfs:Class .

vcard:Organization
      a        rdfs:Class .

vcard:Kind
      a        rdfs:Class .

dcatapit:Agent
      a       rdfs:Class .

foaf:Agent
      a       rdfs:Class .

dct:Standard
      a       rdfs:Class .

skos:prefLabel
      a       rdfs:Property .

skos:notation
      a       rdfs:Property .

skos:inScheme
      a       rdfs:Property .

skos:narrower
	  a 	  rdfs:Property .

skos:broader
	  a		  rdfs:Property .

skos:broaderTransitive
      a 	  rdfs:Property .

skos:narrowerTransitive
      a       rdfs:Property .

skos:definition
	  a		  rdfs:Property .

dct:identifier
	  a       rdfs:Property .

dct:title
    a       rdfs:Property .

dct:type
    a       rdfs:Property .

dct:description
    a       rdfs:Property .

dct:creator
    a       rdfs:Property .

dct:publisher
    a       rdfs:Property .

dct:rightsHolder
    a       rdfs:Property .

dct:conformsTo
    a       rdfs:Property .

dct:subject
    a       rdfs:Property .

dct:accrualPeriodicity
    a       rdfs:Property .

dct:language
    a       rdfs:Property .

dct:format
    a       rdfs:Property .

dct:issued
    a       rdfs:Property .

dct:modified
    a       rdfs:Property .

dct:license
    a       rdfs:Property .


xkos:numberOfLevels
    a     rdfs:Property .

clvapit:hasRankOrder
    a     rdfs:Property .

dcat:theme
    a     rdfs:Property .

dcat:distribution
    a     rdfs:Property .

foaf:name
    a     rdfs:Property .

dcat:keyword
    a     rdfs:Property .

dcat:contactPoint
    a     rdfs:Property .

dcat:accessURL
    a     rdfs:Property .

dcat:downloadURL
    a     rdfs:Property .

owl:versionInfo
    a     rdfs:Property .

adms:representationTechnique
    a     rdfs:Property .

vcard:fn
    a     rdfs:Property .

vcard:hasEmail
    a     rdfs:Property .

ndc:keyConcept
    a     rdfs:Property .

<https://w3id.org/italia/controlled-vocabulary/classifications-for-routes/route-types>
      a       skos:ConceptScheme , adms:Asset , dcatapit:Dataset ;
      dct:title "Route Types Controlled Vocabulary"@en , "Vocabolario controllato dei mezzi di trasporto per itinerari"@it ;
      dct:description "Classification of the types of routes based on the different transportation means. The classification relies on the one provided by GTFS - Google Transit Feed Specification for route_types. The classification also includes the different types of routes that are derived from the Italian Atlas of Paths."@en , "Classificazione dei tipi di itinerari sulla base dei diversi mezzi di trasporto. La classificazione nasce principalmente dalla lista definita all'interno della specifica GTFS - Google Transit Feed Specification per la modellazione dei dati sui trasporti pubblici. La classificazione è tuttavia estesa con ulteriori elementi che derivano dai dati sull'atlante dei cammini italiano (http://www.turismo.beniculturali.it/home-cammini-ditalia/)."@it ;
      rdfs:comment "Classification of the types of routes based on the different transportation means. The classification relies on the one provided by GTFS - Google Transit Feed Specification for route_types. The classification also includes the different types of routes that are derived from the Italian Atlas of Paths."@en , "Classificazione dei tipi di percorso sulla base dei diversi mezzi di trasporto. La classificazione nasce principalmente dalla lista definita all'interno della specifica GTFS - Google Transit Feed Specification per la modellazione dei dati sui trasporti pubblici. La classificazione è tuttavia estesa con ulteriori elementi che derivano dai dati sull'atlante dei cammini italiano (http://www.turismo.beniculturali.it/home-cammini-ditalia/)."@it ;
      rdfs:label "Routes Types Controlled Vocabulary"@en ,  "Vocabolario controllato dei mezzi di trasporto per itinerari"@it ;
      dct:type <http://purl.org/adms/assettype/CodeList> ;
      xkos:numberOfLevels "1";
      ndc:keyConcept "route-types" ;
      adms:representationTechnique <http://purl.org/adms/representationtechnique/SKOS> ;
      dct:identifier "https://w3id.org/italia/controlled-vocabulary/classifications-for-routes/route-types" ;
      dct:rightsHolder <http://spcdata.digitpa.gov.it/browse/page/Amministrazione/agid> ;
      dct:creator <http://spcdata.digitpa.gov.it/browse/page/Amministrazione/agid>  , <http://dati.gov.it/data/resource/Amministrazione/td_PCM> ;
      dct:publisher <http://spcdata.digitpa.gov.it/browse/page/Amministrazione/agid>  ;
      dcat:theme <http://publications.europa.eu/resource/authority/data-theme/EDUC> , <http://publications.europa.eu/resource/authority/data-theme/TRAN> ;
      dct:subject <http://eurovoc.europa.eu/251915> , <http://eurovoc.europa.eu/217826> ;
      dct:conformsTo  <https://w3id.org/italia/data/resource/Standard/SKOS> ;
      dct:language <http://publications.europa.eu/resource/authority/language/ITA> , <http://publications.europa.eu/resource/authority/language/ENG> ;
      dct:accrualPeriodicity <http://publications.europa.eu/resource/authority/frequency/IRREG> ;
      rdfs:isDefinedBy <https://w3id.org/italia/controlled-vocabulary/classifications-for-routes/route-types> ;
      dcat:keyword "Mezzi di trasporto"@it, "Percorsi"@it , "Cammini"@it, "Tipi di Percorso"@it, "Paths"@en , "Routes Types"@en , "Transportation Means"@en ;
      dcat:distribution <https://w3id.org/italia/data/resource/Distribution/RouteType-RDF-Turtle> , <https://w3id.org/italia/data/resource/Distribution/Route-Type-RDF-XML> , <https://w3id.org/italia/data/resource/Distribution/Route-Type-JSON-LD> , <https://w3id.org/italia/data/resource/Distribution/Route-Type-CSV> ,
      <https://w3id.org/italia/data/resource/Distribution/Route-Type-XLSX> ;
      dcat:contactPoint <https://w3id.org/italia/data/resource/ContactPoint/voc_AgID> ;
      skos:hasTopConcept <https://w3id.org/italia/controlled-vocabulary/classifications-for-routes/route-types/0> , <https://w3id.org/italia/controlled-vocabulary/classifications-for-routes/route-types/1> , <https://w3id.org/italia/controlled-vocabulary/classifications-for-routes/route-types/2> , <https://w3id.org/italia/controlled-vocabulary/classifications-for-routes/route-types/3> , <https://w3id.org/italia/controlled-vocabulary/classifications-for-routes/route-types/4> , <https://w3id.org/italia/controlled-vocabulary/classifications-for-routes/route-types/5> , <https://w3id.org/italia/controlled-vocabulary/classifications-for-routes/route-types/6> , <https://w3id.org/italia/controlled-vocabulary/classifications-for-routes/route-types/7> , <https://w3id.org/italia/controlled-vocabulary/classifications-for-routes/route-types/8> , <https://w3id.org/italia/controlled-vocabulary/classifications-for-routes/route-types/9> , <https://w3id.org/italia/controlled-vocabulary/classifications-for-routes/route-types/10> , <https://w3id.org/italia/controlled-vocabulary/classifications-for-routes/route-types/11> , <https://w3id.org/italia/controlled-vocabulary/classifications-for-routes/route-types/12> , <https://w3id.org/italia/controlled-vocabulary/classifications-for-routes/route-types/13> ;
      dct:issued "2018-10-19"^^xsd:date ;
      dct:modified "2018-10-19"^^xsd:date ;
      owl:versionInfo "versione 0.1"@it .

<http://spcdata.digitpa.gov.it/browse/page/Amministrazione/agid>
      a dcatapit:Agent, foaf:Agent ;
      dct:identifier "agid" ;
      foaf:name "Agenzia per l'Italia Digitale"@it , "Italian Digital Agency"@en .

<http://dati.gov.it/data/resource/Amministrazione/td_PCM>
      a dcatapit:Agent, foaf:Agent ;
      dct:identifier "PCM" ;
      foaf:name "Team per la Trasformazione Digitale"@it, "Digital Transformation Team"@en .

<https://w3id.org/italia/data/resource/Standard/SKOS>
      a dcatapit:Standard , dct:Standard ;
      dct:identifier "SKOS" ;
      dct:title "Simple Knowledge Organization System - SKOS" ;
      dct:description "The Simple Knowledge Organization System (SKOS) is a common data model for sharing and linking knowledge organization systems via the Web" .

<https://w3id.org/italia/data/resource/ContactPoint/voc_AgID>
      a	dcatapit:Organization , vcard:Organization, vcard:Kind ;
      vcard:fn		"banche dati e open data" ;
      vcard:hasEmail <mailto:info@dati.gov.it> .

<https://w3id.org/italia/data/resource/Distribution/RouteType-RDF-Turtle>
      a	dcatapit:Distribution  ;
      dct:title				"Distribuzione RDF/Turtle vocabolario controllato tipi di percorso"@it , "RDF/Turtle distribution of the Route types controlled vocabulary"@en ;
      dct:description	"Questa è la distribuzione RDF/Turtle del dataset Linked Open Data del vocabolario controllato sui tipi di percorso"@it , "This is the distribution in RDF/turtle of the Linked Open Dataset of the Route types controlled vocabulary"@en ;
      dct:format 				<http://publications.europa.eu/resource/authority/file-type/RDF_TURTLE> ;
      dct:license <https://w3id.org/italia/controlled-vocabulary/licences/A21_CCBY40> ;
      dcat:downloadURL		<https://raw.githubusercontent.com/italia/daf-ontologie-vocabolari-controllati/master/VocabolariControllati/classifications-for-routes/route-types/route-types.ttl> ;
      dcat:accessURL 			<https://raw.githubusercontent.com/italia/daf-ontologie-vocabolari-controllati/master/VocabolariControllati/classifications-for-routes/route-types> .

<https://w3id.org/italia/data/resource/Distribution/RouteType-RDF-XML>
      a						dcatapit:Distribution  ;
      dct:title				"Distribuzione RDF/XML vocabolario controllato tipi di percorso"@it , "RDF/XML distribution of the Route types controlled vocabulary"@en ;
      dct:description	"Questa è la distribuzione RDF/XML del dataset Linked Open Data del vocabolario controllato sui tipi di percorso"@it , "This is the distribution in RDF/XML of the Linked Open Dataset of the Route types controlled vocabulary "@en ;
      dct:format 				<http://publications.europa.eu/resource/authority/file-type/RDF_XML> ;
      dct:license 			<https://w3id.org/italia/controlled-vocabulary/licences/A21_CCBY40> ;
      dcat:downloadURL		<https://raw.githubusercontent.com/italia/daf-ontologie-vocabolari-controllati/master/VocabolariControllati/classifications-for-routes/route-types/route-types.rdf> ;
      dcat:accessURL 			<https://raw.githubusercontent.com/italia/daf-ontologie-vocabolari-controllati/master/VocabolariControllati/classifications-for-routes/route-types> .

  <https://w3id.org/italia/data/resource/Distribution/RouteType-JSON-LD>
      a						dcatapit:Distribution  ;
      dct:title				"Distribuzione JSON-LD vocabolario controllato categorie tipi di percorso"@it , "JSON-LD distribution of the Route types controlled vocabulary"@en ;
      dct:description	"Questa è la distribuzione JSON-LD del dataset Linked Open Data del vocabolario controllato sui tipi di percorso"@it , "This is the distribution in JSON-LD of the Linked Open Dataset of the Route types controlled vocabulary "@en ;
      dct:format 	<http://publications.europa.eu/resource/authority/file-type/JSON_LD> ;
      dct:license <https://w3id.org/italia/controlled-vocabulary/licences/A21_CCBY40> ;
      dcat:downloadURL		<https://raw.githubusercontent.com/italia/daf-ontologie-vocabolari-controllati/master/VocabolariControllati/classifications-for-routes/route-types/route-types.jsonld> ;
      dcat:accessURL 			<https://raw.githubusercontent.com/italia/daf-ontologie-vocabolari-controllati/master/VocabolariControllati/classifications-for-routes/route-types> .

<https://w3id.org/italia/data/resource/Distribution/RouteType-CSV>
      a						dcatapit:Distribution  ;
      dct:title		"Distribuzione CSV vocabolario controllato categorie tipi di percorso"@it , "CSV distribution of the Route types controlled vocabulary"@en ;
      dct:description	"Questa è la distribuzione CSV del dataset Linked Open Data del vocabolario controllato sui tipi di percorso"@it , "This is the distribution in CSV of the Linked Open Dataset of the Route types controlled vocabulary"@en ;
      dct:format 	<http://publications.europa.eu/resource/authority/file-type/CSV> ;
      dct:license <https://w3id.org/italia/controlled-vocabulary/licences/A21_CCBY40> ;
      dcat:downloadURL		<https://raw.githubusercontent.com/italia/daf-ontologie-vocabolari-controllati/master/VocabolariControllati/classifications-for-routes/route-types/route-types.csv> ;
      dcat:accessURL 			<https://raw.githubusercontent.com/italia/daf-ontologie-vocabolari-controllati/master/VocabolariControllati/classifications-for-routes/route-types> .

<https://w3id.org/italia/data/resource/Distribution/RouteType-XLSX>
      a						dcatapit:Distribution  ;
      dct:title		"Distribuzione XLSX vocabolario controllato sui tipi di percorso"@it , "CSV distribution of the Route Types controlled vocabulary"@en ;
      dct:description	"Questa è la distribuzione XLSX del dataset Linked Open Data del vocabolario controllato sui tipi di percorso"@it , "This is the distribution in XLSX of the Linked Open Dataset of the Route types controlled vocabulary"@en ;
      dct:format 				<http://publications.europa.eu/resource/authority/file-type/XLSX> ;
      dct:license 			<https://w3id.org/italia/controlled-vocabulary/licences/A21_CCBY40> ;
      dcat:downloadURL		<https://raw.githubusercontent.com/italia/daf-ontologie-vocabolari-controllati/master/VocabolariControllati/classifications-for-routes/route-types/route-types.xlsx> ;
      dcat:accessURL 			<https://raw.githubusercontent.com/italia/daf-ontologie-vocabolari-controllati/master/VocabolariControllati/classifications-for-routes/route-types> .

#Definition of the Controlled Vocabulary
 <https://w3id.org/italia/controlled-vocabulary/classifications-for-routes/route-types/0>
 	  a  	skos:Concept , rtapit:RouteType ;
 	  skos:inScheme <https://w3id.org/italia/controlled-vocabulary/classifications-for-routes/route-types> ;
 	  skos:notation "0" ;
 	  dct:identifier "0" ;
    clvapit:hasRankOrder "1" ;
 	  skos:prefLabel "Metropolitana leggera-Tram"@it ;
    skos:prefLabel "Light rail-tram"@en ;
    skos:definition "Qualsiasi sistema di metropolitana leggera o di livello stradale all'interno di un'area metropolitana."@it , "Any light rail or street level system within a metropolitan area."@en .

<https://w3id.org/italia/controlled-vocabulary/classifications-for-routes/route-types/1>
   a  	skos:Concept , rtapit:RouteType ;
   skos:inScheme <https://w3id.org/italia/controlled-vocabulary/classifications-for-routes/route-types> ;
   skos:notation "1" ;
   dct:identifier "1" ;
   clvapit:hasRankOrder "1" ;
   skos:prefLabel "Metropolitana"@it ;
   skos:prefLabel "Metro-Subway"@en ;
   skos:definition "Qualsiasi sistema ferroviario sotterraneo all'interno di un'area metropolitana."@it , "Any underground rail system within a metropolitan area."@en .

<https://w3id.org/italia/controlled-vocabulary/classifications-for-routes/route-types/2>
    a  	skos:Concept , rtapit:RouteType ;
    skos:inScheme <https://w3id.org/italia/controlled-vocabulary/classifications-for-routes/route-types> ;
    skos:notation "2" ;
    dct:identifier "2" ;
    clvapit:hasRankOrder "1" ;
    skos:prefLabel "Ferrovia"@it ;
    skos:prefLabel "Rail"@en ;
    skos:definition "Sistema ferroviario utilizzato per viaggi interurbani o a lunga distanza."@it , "Used for intercity or long-distance travel."@en .

<https://w3id.org/italia/controlled-vocabulary/classifications-for-routes/route-types/3>
    a  	skos:Concept , rtapit:RouteType ;
    skos:inScheme <https://w3id.org/italia/controlled-vocabulary/classifications-for-routes/route-types> ;
    skos:notation "3" ;
    dct:identifier "3" ;
    clvapit:hasRankOrder "1" ;
    skos:prefLabel "Autobus"@it ;
    skos:prefLabel "Bus"@en ;
    skos:definition "Sistema utilizzato per linee di autobus a breve e lunga percorrenza."@it , "Used for short- and long-distance bus routes,"@en .

<https://w3id.org/italia/controlled-vocabulary/classifications-for-routes/route-types/4>
    a  	skos:Concept , rtapit:RouteType ;
    skos:inScheme <https://w3id.org/italia/controlled-vocabulary/classifications-for-routes/route-types> ;
    skos:notation "4" ;
    dct:identifier "4" ;
    clvapit:hasRankOrder "1" ;
    skos:prefLabel "Traghetto"@it ;
    skos:prefLabel "Ferry"@en ;
    skos:definition "Sistema utilizzato per il servizio di navigazione a breve e lunga distanza."@it , "Used for short- and long-distance boat service."@en .

<https://w3id.org/italia/controlled-vocabulary/classifications-for-routes/route-types/5>
    a  	skos:Concept , rtapit:RouteType ;
    skos:inScheme <https://w3id.org/italia/controlled-vocabulary/classifications-for-routes/route-types> ;
    skos:notation "5" ;
    dct:identifier "5" ;
    clvapit:hasRankOrder "1" ;
    skos:prefLabel "Funivia"@it ;
    skos:prefLabel "Cable car"@en ;
    skos:definition "Sistema utilizzato per funivie a livello stradale dove la fune scorre sotto l'auto."@it , "Used for street-level cable cars where the cable runs beneath the car."@en .

<https://w3id.org/italia/controlled-vocabulary/classifications-for-routes/route-types/6>
    a  	skos:Concept , rtapit:RouteType ;
    skos:inScheme <https://w3id.org/italia/controlled-vocabulary/classifications-for-routes/route-types> ;
    skos:notation "6" ;
    dct:identifier "6" ;
    clvapit:hasRankOrder "1" ;
    skos:prefLabel "Funivia sospesa"@it ;
    skos:prefLabel "Suspended cable car"@en ;
    skos:definition "Sistema utilizzata per le funivie aeree dove l'auto è sospesa alla fune"@it , "Typically used for aerial cable cars where the car is suspended from the cable."@en .


<https://w3id.org/italia/controlled-vocabulary/classifications-for-routes/route-types/7>
    a  	skos:Concept , rtapit:RouteType ;
    skos:inScheme <https://w3id.org/italia/controlled-vocabulary/classifications-for-routes/route-types> ;
    skos:notation "7" ;
    dct:identifier "7" ;
    clvapit:hasRankOrder "1" ;
    skos:prefLabel "Funicolare"@it ;
    skos:prefLabel "Funicular"@en ;
    skos:definition "Qualsiasi sistema di binari progettato per pendii ripidi."@it , "Any rail system designed for steep inclines."@en .

<https://w3id.org/italia/controlled-vocabulary/classifications-for-routes/route-types/8>
    a  	skos:Concept , rtapit:RouteType ;
    skos:inScheme <https://w3id.org/italia/controlled-vocabulary/classifications-for-routes/route-types> ;
    skos:notation "8" ;
    dct:identifier "8" ;
    clvapit:hasRankOrder "1" ;
    skos:prefLabel "Bicicletta"@it ;
    skos:prefLabel "Bike"@en .

<https://w3id.org/italia/controlled-vocabulary/classifications-for-routes/route-types/9>
    a  	skos:Concept , rtapit:RouteType ;
    skos:inScheme <https://w3id.org/italia/controlled-vocabulary/classifications-for-routes/route-types> ;
    skos:notation "9" ;
    dct:identifier "9" ;
    clvapit:hasRankOrder "1" ;
    skos:prefLabel "Piedi"@it ;
    skos:prefLabel "Walk"@en .

<https://w3id.org/italia/controlled-vocabulary/classifications-for-routes/route-types/10>
    a  	skos:Concept , rtapit:RouteType ;
    skos:inScheme <https://w3id.org/italia/controlled-vocabulary/classifications-for-routes/route-types> ;
    skos:notation "10" ;
    dct:identifier "10" ;
    clvapit:hasRankOrder "1" ;
    skos:prefLabel "Cavallo"@it ;
    skos:prefLabel "Horseback"@en .

<https://w3id.org/italia/controlled-vocabulary/classifications-for-routes/route-types/11>
    a  	skos:Concept , rtapit:RouteType ;
    skos:inScheme <https://w3id.org/italia/controlled-vocabulary/classifications-for-routes/route-types> ;
    skos:notation "11" ;
    dct:identifier "11" ;
    clvapit:hasRankOrder "1" ;
    skos:prefLabel "Automobile"@it ;
    skos:prefLabel "Car"@en .

<https://w3id.org/italia/controlled-vocabulary/classifications-for-routes/route-types/12>
    a  	skos:Concept , rtapit:RouteType ;
    skos:inScheme <https://w3id.org/italia/controlled-vocabulary/classifications-for-routes/route-types> ;
    skos:notation "12" ;
    dct:identifier "12" ;
    clvapit:hasRankOrder "1" ;
    skos:prefLabel "Camion"@it ;
    skos:prefLabel "Truck"@en .

<https://w3id.org/italia/controlled-vocabulary/classifications-for-routes/route-types/13>
    a  	skos:Concept , rtapit:RouteType ;
    skos:inScheme <https://w3id.org/italia/controlled-vocabulary/classifications-for-routes/route-types> ;
    skos:notation "13" ;
    dct:identifier "13" ;
    clvapit:hasRankOrder "1" ;
    skos:prefLabel "Motocicletta"@it ;
    skos:prefLabel "Motorbike"@en .
