<?xml version="1.0" encoding="utf-8"?>
<rdf:RDF
  xmlns:rdfs="http://www.w3.org/2000/01/rdf-schema#"
  xmlns:dct="http://purl.org/dc/terms/"
  xmlns:dcat="http://www.w3.org/ns/dcat#"
  xmlns:adms="http://www.w3.org/ns/adms#"
  xmlns:dcatapit="http://dati.gov.it/onto/dcatapit#"
  xmlns:vcard="http://www.w3.org/2006/vcard/ns#"
  xmlns:foaf="http://xmlns.com/foaf/0.1/"
  xmlns:owl="http://www.w3.org/2002/07/owl#"
  xmlns:ndc="https://w3id.org/italia/onto/NDC/"
  xmlns:skos="http://www.w3.org/2004/02/skos/core#"
  xmlns:rtapit="https://w3id.org/italia/onto/Route/"
  xmlns:clvapit="https://w3id.org/italia/onto/CLV/"
  xmlns:xkos="http://rdf-vocabulary.ddialliance.org/xkos#"
  xmlns:rdf="http://www.w3.org/1999/02/22-rdf-syntax-ns#"
>
  <skos:ConceptScheme rdf:about="https://w3id.org/italia/controlled-vocabulary/classifications-for-routes/route-types">
    <rdf:type rdf:resource="http://www.w3.org/ns/adms#Asset"/>
    <rdf:type rdf:resource="http://dati.gov.it/onto/dcatapit#Dataset"/>
    <dct:title xml:lang="en">Route Types Controlled Vocabulary</dct:title>
    <dct:title xml:lang="it">Vocabolario controllato dei mezzi di trasporto per itinerari</dct:title>
    <dct:description xml:lang="en">Classification of the types of routes based on the different transportation means. The classification relies on the one provided by GTFS - Google Transit Feed Specification for route_types. The classification also includes the different types of routes that are derived from the Italian Atlas of Paths.</dct:description>
    <dct:description xml:lang="it">Classificazione dei tipi di itinerari sulla base dei diversi mezzi di trasporto. La classificazione nasce principalmente dalla lista definita all'interno della specifica GTFS - Google Transit Feed Specification per la modellazione dei dati sui trasporti pubblici. La classificazione è tuttavia estesa con ulteriori elementi che derivano dai dati sull'atlante dei cammini italiano (http://www.turismo.beniculturali.it/home-cammini-ditalia/).</dct:description>
    <rdfs:comment xml:lang="en">Classification of the types of routes based on the different transportation means. The classification relies on the one provided by GTFS - Google Transit Feed Specification for route_types. The classification also includes the different types of routes that are derived from the Italian Atlas of Paths.</rdfs:comment>
    <rdfs:comment xml:lang="it">Classificazione dei tipi di percorso sulla base dei diversi mezzi di trasporto. La classificazione nasce principalmente dalla lista definita all'interno della specifica GTFS - Google Transit Feed Specification per la modellazione dei dati sui trasporti pubblici. La classificazione è tuttavia estesa con ulteriori elementi che derivano dai dati sull'atlante dei cammini italiano (http://www.turismo.beniculturali.it/home-cammini-ditalia/).</rdfs:comment>
    <rdfs:label xml:lang="en">Routes Types Controlled Vocabulary</rdfs:label>
    <rdfs:label xml:lang="it">Vocabolario controllato dei mezzi di trasporto per itinerari</rdfs:label>
    <dct:type rdf:resource="http://purl.org/adms/assettype/CodeList"/>
    <xkos:numberOfLevels>1</xkos:numberOfLevels>
    <ndc:keyConcept>route-types</ndc:keyConcept>
    <adms:representationTechnique rdf:resource="http://purl.org/adms/representationtechnique/SKOS"/>
    <dct:identifier>https://w3id.org/italia/controlled-vocabulary/classifications-for-routes/route-types</dct:identifier>
    <dct:rightsHolder>
      <dcatapit:Agent rdf:about="http://spcdata.digitpa.gov.it/browse/page/Amministrazione/agid">
        <rdf:type rdf:resource="http://xmlns.com/foaf/0.1/Agent"/>
        <dct:identifier>agid</dct:identifier>
        <foaf:name xml:lang="it">Agenzia per l'Italia Digitale</foaf:name>
        <foaf:name xml:lang="en">Italian Digital Agency</foaf:name>
      </dcatapit:Agent>
    </dct:rightsHolder>
    <dct:creator rdf:resource="http://spcdata.digitpa.gov.it/browse/page/Amministrazione/agid"/>
    <dct:creator>
      <dcatapit:Agent rdf:about="http://dati.gov.it/data/resource/Amministrazione/td_PCM">
        <rdf:type rdf:resource="http://xmlns.com/foaf/0.1/Agent"/>
        <dct:identifier>PCM</dct:identifier>
        <foaf:name xml:lang="it">Team per la Trasformazione Digitale</foaf:name>
        <foaf:name xml:lang="en">Digital Transformation Team</foaf:name>
      </dcatapit:Agent>
    </dct:creator>
    <dct:publisher rdf:resource="http://spcdata.digitpa.gov.it/browse/page/Amministrazione/agid"/>
    <dcat:theme rdf:resource="http://publications.europa.eu/resource/authority/data-theme/EDUC"/>
    <dcat:theme rdf:resource="http://publications.europa.eu/resource/authority/data-theme/TRAN"/>
    <dct:subject rdf:resource="http://eurovoc.europa.eu/251915"/>
    <dct:subject rdf:resource="http://eurovoc.europa.eu/217826"/>
    <dct:conformsTo>
      <dcatapit:Standard rdf:about="https://w3id.org/italia/data/resource/Standard/SKOS">
        <rdf:type rdf:resource="http://purl.org/dc/terms/Standard"/>
        <dct:identifier>SKOS</dct:identifier>
        <dct:title>Simple Knowledge Organization System - SKOS</dct:title>
        <dct:description>The Simple Knowledge Organization System (SKOS) is a common data model for sharing and linking knowledge organization systems via the Web</dct:description>
      </dcatapit:Standard>
    </dct:conformsTo>
    <dct:language rdf:resource="http://publications.europa.eu/resource/authority/language/ITA"/>
    <dct:language rdf:resource="http://publications.europa.eu/resource/authority/language/ENG"/>
    <dct:accrualPeriodicity rdf:resource="http://publications.europa.eu/resource/authority/frequency/IRREG"/>
    <rdfs:isDefinedBy rdf:resource="https://w3id.org/italia/controlled-vocabulary/classifications-for-routes/route-types"/>
    <dcat:keyword xml:lang="it">Mezzi di trasporto</dcat:keyword>
    <dcat:keyword xml:lang="it">Percorsi</dcat:keyword>
    <dcat:keyword xml:lang="it">Cammini</dcat:keyword>
    <dcat:keyword xml:lang="it">Tipi di Percorso</dcat:keyword>
    <dcat:keyword xml:lang="en">Paths</dcat:keyword>
    <dcat:keyword xml:lang="en">Routes Types</dcat:keyword>
    <dcat:keyword xml:lang="en">Transportation Means</dcat:keyword>
    <dcat:distribution>
      <dcatapit:Distribution rdf:about="https://w3id.org/italia/data/resource/Distribution/RouteType-RDF-Turtle">
        <dct:title xml:lang="it">Distribuzione RDF/Turtle vocabolario controllato tipi di percorso</dct:title>
        <dct:title xml:lang="en">RDF/Turtle distribution of the Route types controlled vocabulary</dct:title>
        <dct:description xml:lang="it">Questa è la distribuzione RDF/Turtle del dataset Linked Open Data del vocabolario controllato sui tipi di percorso</dct:description>
        <dct:description xml:lang="en">This is the distribution in RDF/turtle of the Linked Open Dataset of the Route types controlled vocabulary</dct:description>
        <dct:format rdf:resource="http://publications.europa.eu/resource/authority/file-type/RDF_TURTLE"/>
        <dct:license rdf:resource="https://w3id.org/italia/controlled-vocabulary/licences/A21_CCBY40"/>
        <dcat:downloadURL rdf:resource="https://raw.githubusercontent.com/italia/daf-ontologie-vocabolari-controllati/master/VocabolariControllati/classifications-for-routes/route-types/route-types.ttl"/>
        <dcat:accessURL rdf:resource="https://raw.githubusercontent.com/italia/daf-ontologie-vocabolari-controllati/master/VocabolariControllati/classifications-for-routes/route-types"/>
      </dcatapit:Distribution>
    </dcat:distribution>
    <dcat:distribution rdf:resource="https://w3id.org/italia/data/resource/Distribution/Route-Type-RDF-XML"/>
    <dcat:distribution rdf:resource="https://w3id.org/italia/data/resource/Distribution/Route-Type-JSON-LD"/>
    <dcat:distribution rdf:resource="https://w3id.org/italia/data/resource/Distribution/Route-Type-CSV"/>
    <dcat:distribution rdf:resource="https://w3id.org/italia/data/resource/Distribution/Route-Type-XLSX"/>
    <dcat:contactPoint>
      <dcatapit:Organization rdf:about="https://w3id.org/italia/data/resource/ContactPoint/voc_AgID">
        <rdf:type rdf:resource="http://www.w3.org/2006/vcard/ns#Organization"/>
        <rdf:type rdf:resource="http://www.w3.org/2006/vcard/ns#Kind"/>
        <vcard:fn>banche dati e open data</vcard:fn>
        <vcard:hasEmail rdf:resource="mailto:info@dati.gov.it"/>
      </dcatapit:Organization>
    </dcat:contactPoint>
    <skos:hasTopConcept>
      <skos:Concept rdf:about="https://w3id.org/italia/controlled-vocabulary/classifications-for-routes/route-types/0">
        <rdf:type rdf:resource="https://w3id.org/italia/onto/Route/RouteType"/>
        <skos:inScheme rdf:resource="https://w3id.org/italia/controlled-vocabulary/classifications-for-routes/route-types"/>
        <skos:notation>0</skos:notation>
        <dct:identifier>0</dct:identifier>
        <clvapit:hasRankOrder>1</clvapit:hasRankOrder>
        <skos:prefLabel xml:lang="it">Metropolitana leggera-Tram</skos:prefLabel>
        <skos:prefLabel xml:lang="en">Light rail-tram</skos:prefLabel>
        <skos:definition xml:lang="it">Qualsiasi sistema di metropolitana leggera o di livello stradale all'interno di un'area metropolitana.</skos:definition>
        <skos:definition xml:lang="en">Any light rail or street level system within a metropolitan area.</skos:definition>
      </skos:Concept>
    </skos:hasTopConcept>
    <skos:hasTopConcept>
      <skos:Concept rdf:about="https://w3id.org/italia/controlled-vocabulary/classifications-for-routes/route-types/1">
        <rdf:type rdf:resource="https://w3id.org/italia/onto/Route/RouteType"/>
        <skos:inScheme rdf:resource="https://w3id.org/italia/controlled-vocabulary/classifications-for-routes/route-types"/>
        <skos:notation>1</skos:notation>
        <dct:identifier>1</dct:identifier>
        <clvapit:hasRankOrder>1</clvapit:hasRankOrder>
        <skos:prefLabel xml:lang="it">Metropolitana</skos:prefLabel>
        <skos:prefLabel xml:lang="en">Metro-Subway</skos:prefLabel>
        <skos:definition xml:lang="it">Qualsiasi sistema ferroviario sotterraneo all'interno di un'area metropolitana.</skos:definition>
        <skos:definition xml:lang="en">Any underground rail system within a metropolitan area.</skos:definition>
      </skos:Concept>
    </skos:hasTopConcept>
    <skos:hasTopConcept>
      <skos:Concept rdf:about="https://w3id.org/italia/controlled-vocabulary/classifications-for-routes/route-types/2">
        <rdf:type rdf:resource="https://w3id.org/italia/onto/Route/RouteType"/>
        <skos:inScheme rdf:resource="https://w3id.org/italia/controlled-vocabulary/classifications-for-routes/route-types"/>
        <skos:notation>2</skos:notation>
        <dct:identifier>2</dct:identifier>
        <clvapit:hasRankOrder>1</clvapit:hasRankOrder>
        <skos:prefLabel xml:lang="it">Ferrovia</skos:prefLabel>
        <skos:prefLabel xml:lang="en">Rail</skos:prefLabel>
        <skos:definition xml:lang="it">Sistema ferroviario utilizzato per viaggi interurbani o a lunga distanza.</skos:definition>
        <skos:definition xml:lang="en">Used for intercity or long-distance travel.</skos:definition>
      </skos:Concept>
    </skos:hasTopConcept>
    <skos:hasTopConcept>
      <skos:Concept rdf:about="https://w3id.org/italia/controlled-vocabulary/classifications-for-routes/route-types/3">
        <rdf:type rdf:resource="https://w3id.org/italia/onto/Route/RouteType"/>
        <skos:inScheme rdf:resource="https://w3id.org/italia/controlled-vocabulary/classifications-for-routes/route-types"/>
        <skos:notation>3</skos:notation>
        <dct:identifier>3</dct:identifier>
        <clvapit:hasRankOrder>1</clvapit:hasRankOrder>
        <skos:prefLabel xml:lang="it">Autobus</skos:prefLabel>
        <skos:prefLabel xml:lang="en">Bus</skos:prefLabel>
        <skos:definition xml:lang="it">Sistema utilizzato per linee di autobus a breve e lunga percorrenza.</skos:definition>
        <skos:definition xml:lang="en">Used for short- and long-distance bus routes,</skos:definition>
      </skos:Concept>
    </skos:hasTopConcept>
    <skos:hasTopConcept>
      <skos:Concept rdf:about="https://w3id.org/italia/controlled-vocabulary/classifications-for-routes/route-types/4">
        <rdf:type rdf:resource="https://w3id.org/italia/onto/Route/RouteType"/>
        <skos:inScheme rdf:resource="https://w3id.org/italia/controlled-vocabulary/classifications-for-routes/route-types"/>
        <skos:notation>4</skos:notation>
        <dct:identifier>4</dct:identifier>
        <clvapit:hasRankOrder>1</clvapit:hasRankOrder>
        <skos:prefLabel xml:lang="it">Traghetto</skos:prefLabel>
        <skos:prefLabel xml:lang="en">Ferry</skos:prefLabel>
        <skos:definition xml:lang="it">Sistema utilizzato per il servizio di navigazione a breve e lunga distanza.</skos:definition>
        <skos:definition xml:lang="en">Used for short- and long-distance boat service.</skos:definition>
      </skos:Concept>
    </skos:hasTopConcept>
    <skos:hasTopConcept>
      <skos:Concept rdf:about="https://w3id.org/italia/controlled-vocabulary/classifications-for-routes/route-types/5">
        <rdf:type rdf:resource="https://w3id.org/italia/onto/Route/RouteType"/>
        <skos:inScheme rdf:resource="https://w3id.org/italia/controlled-vocabulary/classifications-for-routes/route-types"/>
        <skos:notation>5</skos:notation>
        <dct:identifier>5</dct:identifier>
        <clvapit:hasRankOrder>1</clvapit:hasRankOrder>
        <skos:prefLabel xml:lang="it">Funivia</skos:prefLabel>
        <skos:prefLabel xml:lang="en">Cable car</skos:prefLabel>
        <skos:definition xml:lang="it">Sistema utilizzato per funivie a livello stradale dove la fune scorre sotto l'auto.</skos:definition>
        <skos:definition xml:lang="en">Used for street-level cable cars where the cable runs beneath the car.</skos:definition>
      </skos:Concept>
    </skos:hasTopConcept>
    <skos:hasTopConcept>
      <skos:Concept rdf:about="https://w3id.org/italia/controlled-vocabulary/classifications-for-routes/route-types/6">
        <rdf:type rdf:resource="https://w3id.org/italia/onto/Route/RouteType"/>
        <skos:inScheme rdf:resource="https://w3id.org/italia/controlled-vocabulary/classifications-for-routes/route-types"/>
        <skos:notation>6</skos:notation>
        <dct:identifier>6</dct:identifier>
        <clvapit:hasRankOrder>1</clvapit:hasRankOrder>
        <skos:prefLabel xml:lang="it">Funivia sospesa</skos:prefLabel>
        <skos:prefLabel xml:lang="en">Suspended cable car</skos:prefLabel>
        <skos:definition xml:lang="it">Sistema utilizzata per le funivie aeree dove l'auto è sospesa alla fune</skos:definition>
        <skos:definition xml:lang="en">Typically used for aerial cable cars where the car is suspended from the cable.</skos:definition>
      </skos:Concept>
    </skos:hasTopConcept>
    <skos:hasTopConcept>
      <skos:Concept rdf:about="https://w3id.org/italia/controlled-vocabulary/classifications-for-routes/route-types/7">
        <rdf:type rdf:resource="https://w3id.org/italia/onto/Route/RouteType"/>
        <skos:inScheme rdf:resource="https://w3id.org/italia/controlled-vocabulary/classifications-for-routes/route-types"/>
        <skos:notation>7</skos:notation>
        <dct:identifier>7</dct:identifier>
        <clvapit:hasRankOrder>1</clvapit:hasRankOrder>
        <skos:prefLabel xml:lang="it">Funicolare</skos:prefLabel>
        <skos:prefLabel xml:lang="en">Funicular</skos:prefLabel>
        <skos:definition xml:lang="it">Qualsiasi sistema di binari progettato per pendii ripidi.</skos:definition>
        <skos:definition xml:lang="en">Any rail system designed for steep inclines.</skos:definition>
      </skos:Concept>
    </skos:hasTopConcept>
    <skos:hasTopConcept>
      <skos:Concept rdf:about="https://w3id.org/italia/controlled-vocabulary/classifications-for-routes/route-types/8">
        <rdf:type rdf:resource="https://w3id.org/italia/onto/Route/RouteType"/>
        <skos:inScheme rdf:resource="https://w3id.org/italia/controlled-vocabulary/classifications-for-routes/route-types"/>
        <skos:notation>8</skos:notation>
        <dct:identifier>8</dct:identifier>
        <clvapit:hasRankOrder>1</clvapit:hasRankOrder>
        <skos:prefLabel xml:lang="it">Bicicletta</skos:prefLabel>
        <skos:prefLabel xml:lang="en">Bike</skos:prefLabel>
      </skos:Concept>
    </skos:hasTopConcept>
    <skos:hasTopConcept>
      <skos:Concept rdf:about="https://w3id.org/italia/controlled-vocabulary/classifications-for-routes/route-types/9">
        <rdf:type rdf:resource="https://w3id.org/italia/onto/Route/RouteType"/>
        <skos:inScheme rdf:resource="https://w3id.org/italia/controlled-vocabulary/classifications-for-routes/route-types"/>
        <skos:notation>9</skos:notation>
        <dct:identifier>9</dct:identifier>
        <clvapit:hasRankOrder>1</clvapit:hasRankOrder>
        <skos:prefLabel xml:lang="it">Piedi</skos:prefLabel>
        <skos:prefLabel xml:lang="en">Walk</skos:prefLabel>
      </skos:Concept>
    </skos:hasTopConcept>
    <skos:hasTopConcept>
      <skos:Concept rdf:about="https://w3id.org/italia/controlled-vocabulary/classifications-for-routes/route-types/10">
        <rdf:type rdf:resource="https://w3id.org/italia/onto/Route/RouteType"/>
        <skos:inScheme rdf:resource="https://w3id.org/italia/controlled-vocabulary/classifications-for-routes/route-types"/>
        <skos:notation>10</skos:notation>
        <dct:identifier>10</dct:identifier>
        <clvapit:hasRankOrder>1</clvapit:hasRankOrder>
        <skos:prefLabel xml:lang="it">Cavallo</skos:prefLabel>
        <skos:prefLabel xml:lang="en">Horseback</skos:prefLabel>
      </skos:Concept>
    </skos:hasTopConcept>
    <skos:hasTopConcept>
      <skos:Concept rdf:about="https://w3id.org/italia/controlled-vocabulary/classifications-for-routes/route-types/11">
        <rdf:type rdf:resource="https://w3id.org/italia/onto/Route/RouteType"/>
        <skos:inScheme rdf:resource="https://w3id.org/italia/controlled-vocabulary/classifications-for-routes/route-types"/>
        <skos:notation>11</skos:notation>
        <dct:identifier>11</dct:identifier>
        <clvapit:hasRankOrder>1</clvapit:hasRankOrder>
        <skos:prefLabel xml:lang="it">Automobile</skos:prefLabel>
        <skos:prefLabel xml:lang="en">Car</skos:prefLabel>
      </skos:Concept>
    </skos:hasTopConcept>
    <skos:hasTopConcept>
      <skos:Concept rdf:about="https://w3id.org/italia/controlled-vocabulary/classifications-for-routes/route-types/12">
        <rdf:type rdf:resource="https://w3id.org/italia/onto/Route/RouteType"/>
        <skos:inScheme rdf:resource="https://w3id.org/italia/controlled-vocabulary/classifications-for-routes/route-types"/>
        <skos:notation>12</skos:notation>
        <dct:identifier>12</dct:identifier>
        <clvapit:hasRankOrder>1</clvapit:hasRankOrder>
        <skos:prefLabel xml:lang="it">Camion</skos:prefLabel>
        <skos:prefLabel xml:lang="en">Truck</skos:prefLabel>
      </skos:Concept>
    </skos:hasTopConcept>
    <skos:hasTopConcept>
      <skos:Concept rdf:about="https://w3id.org/italia/controlled-vocabulary/classifications-for-routes/route-types/13">
        <rdf:type rdf:resource="https://w3id.org/italia/onto/Route/RouteType"/>
        <skos:inScheme rdf:resource="https://w3id.org/italia/controlled-vocabulary/classifications-for-routes/route-types"/>
        <skos:notation>13</skos:notation>
        <dct:identifier>13</dct:identifier>
        <clvapit:hasRankOrder>1</clvapit:hasRankOrder>
        <skos:prefLabel xml:lang="it">Motocicletta</skos:prefLabel>
        <skos:prefLabel xml:lang="en">Motorbike</skos:prefLabel>
      </skos:Concept>
    </skos:hasTopConcept>
    <dct:issued rdf:datatype="http://www.w3.org/2001/XMLSchema#date">2018-10-19</dct:issued>
    <dct:modified rdf:datatype="http://www.w3.org/2001/XMLSchema#date">2018-10-19</dct:modified>
    <owl:versionInfo xml:lang="it">versione 0.1</owl:versionInfo>
  </skos:ConceptScheme>
  <rdfs:Property rdf:about="https://w3id.org/italia/onto/NDC/keyConcept"/>
  <rdfs:Property rdf:about="http://purl.org/dc/terms/accrualPeriodicity"/>
  <rdfs:Property rdf:about="http://purl.org/dc/terms/type"/>
  <dcatapit:Distribution rdf:about="https://w3id.org/italia/data/resource/Distribution/RouteType-CSV">
    <dct:title xml:lang="it">Distribuzione CSV vocabolario controllato categorie tipi di percorso</dct:title>
    <dct:title xml:lang="en">CSV distribution of the Route types controlled vocabulary</dct:title>
    <dct:description xml:lang="it">Questa è la distribuzione CSV del dataset Linked Open Data del vocabolario controllato sui tipi di percorso</dct:description>
    <dct:description xml:lang="en">This is the distribution in CSV of the Linked Open Dataset of the Route types controlled vocabulary</dct:description>
    <dct:format rdf:resource="http://publications.europa.eu/resource/authority/file-type/CSV"/>
    <dct:license rdf:resource="https://w3id.org/italia/controlled-vocabulary/licences/A21_CCBY40"/>
    <dcat:downloadURL rdf:resource="https://raw.githubusercontent.com/italia/daf-ontologie-vocabolari-controllati/master/VocabolariControllati/classifications-for-routes/route-types/route-types.csv"/>
    <dcat:accessURL rdf:resource="https://raw.githubusercontent.com/italia/daf-ontologie-vocabolari-controllati/master/VocabolariControllati/classifications-for-routes/route-types"/>
  </dcatapit:Distribution>
  <dcatapit:Distribution rdf:about="https://w3id.org/italia/data/resource/Distribution/RouteType-RDF-XML">
    <dct:title xml:lang="it">Distribuzione RDF/XML vocabolario controllato tipi di percorso</dct:title>
    <dct:title xml:lang="en">RDF/XML distribution of the Route types controlled vocabulary</dct:title>
    <dct:description xml:lang="it">Questa è la distribuzione RDF/XML del dataset Linked Open Data del vocabolario controllato sui tipi di percorso</dct:description>
    <dct:description xml:lang="en">This is the distribution in RDF/XML of the Linked Open Dataset of the Route types controlled vocabulary </dct:description>
    <dct:format rdf:resource="http://publications.europa.eu/resource/authority/file-type/RDF_XML"/>
    <dct:license rdf:resource="https://w3id.org/italia/controlled-vocabulary/licences/A21_CCBY40"/>
    <dcat:downloadURL rdf:resource="https://raw.githubusercontent.com/italia/daf-ontologie-vocabolari-controllati/master/VocabolariControllati/classifications-for-routes/route-types/route-types.rdf"/>
    <dcat:accessURL rdf:resource="https://raw.githubusercontent.com/italia/daf-ontologie-vocabolari-controllati/master/VocabolariControllati/classifications-for-routes/route-types"/>
  </dcatapit:Distribution>
  <dcatapit:Distribution rdf:about="https://w3id.org/italia/data/resource/Distribution/RouteType-XLSX">
    <dct:title xml:lang="it">Distribuzione XLSX vocabolario controllato sui tipi di percorso</dct:title>
    <dct:title xml:lang="en">CSV distribution of the Route Types controlled vocabulary</dct:title>
    <dct:description xml:lang="it">Questa è la distribuzione XLSX del dataset Linked Open Data del vocabolario controllato sui tipi di percorso</dct:description>
    <dct:description xml:lang="en">This is the distribution in XLSX of the Linked Open Dataset of the Route types controlled vocabulary</dct:description>
    <dct:format rdf:resource="http://publications.europa.eu/resource/authority/file-type/XLSX"/>
    <dct:license rdf:resource="https://w3id.org/italia/controlled-vocabulary/licences/A21_CCBY40"/>
    <dcat:downloadURL rdf:resource="https://raw.githubusercontent.com/italia/daf-ontologie-vocabolari-controllati/master/VocabolariControllati/classifications-for-routes/route-types/route-types.xlsx"/>
    <dcat:accessURL rdf:resource="https://raw.githubusercontent.com/italia/daf-ontologie-vocabolari-controllati/master/VocabolariControllati/classifications-for-routes/route-types"/>
  </dcatapit:Distribution>
  <dcatapit:Distribution rdf:about="https://w3id.org/italia/data/resource/Distribution/RouteType-JSON-LD">
    <dct:title xml:lang="it">Distribuzione JSON-LD vocabolario controllato categorie tipi di percorso</dct:title>
    <dct:title xml:lang="en">JSON-LD distribution of the Route types controlled vocabulary</dct:title>
    <dct:description xml:lang="it">Questa è la distribuzione JSON-LD del dataset Linked Open Data del vocabolario controllato sui tipi di percorso</dct:description>
    <dct:description xml:lang="en">This is the distribution in JSON-LD of the Linked Open Dataset of the Route types controlled vocabulary </dct:description>
    <dct:format rdf:resource="http://publications.europa.eu/resource/authority/file-type/JSON_LD"/>
    <dct:license rdf:resource="https://w3id.org/italia/controlled-vocabulary/licences/A21_CCBY40"/>
    <dcat:downloadURL rdf:resource="https://raw.githubusercontent.com/italia/daf-ontologie-vocabolari-controllati/master/VocabolariControllati/classifications-for-routes/route-types/route-types.jsonld"/>
    <dcat:accessURL rdf:resource="https://raw.githubusercontent.com/italia/daf-ontologie-vocabolari-controllati/master/VocabolariControllati/classifications-for-routes/route-types"/>
  </dcatapit:Distribution>
  <rdfs:Property rdf:about="http://purl.org/dc/terms/format"/>
  <rdfs:Property rdf:about="http://www.w3.org/2006/vcard/ns#fn"/>
  <rdfs:Property rdf:about="http://purl.org/dc/terms/publisher"/>
  <rdfs:Property rdf:about="http://www.w3.org/2004/02/skos/core#definition"/>
  <rdfs:Property rdf:about="http://purl.org/dc/terms/description"/>
  <rdfs:Property rdf:about="http://www.w3.org/2002/07/owl#versionInfo"/>
  <rdfs:Property rdf:about="http://xmlns.com/foaf/0.1/name"/>
  <rdfs:Property rdf:about="http://www.w3.org/ns/dcat#contactPoint"/>
  <rdfs:Property rdf:about="http://purl.org/dc/terms/issued"/>
  <rdfs:Property rdf:about="http://www.w3.org/2004/02/skos/core#notation"/>
  <rdfs:Property rdf:about="http://www.w3.org/2004/02/skos/core#broaderTransitive"/>
  <rdfs:Property rdf:about="https://w3id.org/italia/onto/CLV/hasRankOrder"/>
  <rdfs:Property rdf:about="http://www.w3.org/2004/02/skos/core#inScheme"/>
  <rdfs:Property rdf:about="http://www.w3.org/2004/02/skos/core#narrower"/>
  <rdfs:Property rdf:about="http://purl.org/dc/terms/title"/>
  <rdfs:Property rdf:about="http://purl.org/dc/terms/license"/>
  <rdfs:Property rdf:about="http://purl.org/dc/terms/language"/>
  <rdfs:Property rdf:about="http://www.w3.org/ns/dcat#distribution"/>
  <rdfs:Property rdf:about="http://www.w3.org/2004/02/skos/core#narrowerTransitive"/>
  <rdfs:Property rdf:about="http://rdf-vocabulary.ddialliance.org/xkos#numberOfLevels"/>
  <rdfs:Property rdf:about="http://purl.org/dc/terms/conformsTo"/>
  <rdfs:Property rdf:about="http://www.w3.org/2006/vcard/ns#hasEmail"/>
  <rdfs:Property rdf:about="http://www.w3.org/2004/02/skos/core#prefLabel"/>
  <rdfs:Property rdf:about="http://purl.org/dc/terms/identifier"/>
  <rdfs:Property rdf:about="http://purl.org/dc/terms/modified"/>
  <rdfs:Property rdf:about="http://www.w3.org/ns/dcat#accessURL"/>
  <rdfs:Property rdf:about="http://purl.org/dc/terms/rightsHolder"/>
  <rdfs:Property rdf:about="http://www.w3.org/ns/dcat#downloadURL"/>
  <rdfs:Property rdf:about="http://purl.org/dc/terms/creator"/>
  <rdfs:Property rdf:about="http://www.w3.org/ns/dcat#keyword"/>
  <rdfs:Property rdf:about="http://www.w3.org/ns/dcat#theme"/>
  <rdfs:Property rdf:about="http://purl.org/dc/terms/subject"/>
  <rdfs:Property rdf:about="http://www.w3.org/ns/adms#representationTechnique"/>
  <rdfs:Property rdf:about="http://www.w3.org/2004/02/skos/core#broader"/>
  <rdfs:Class rdf:about="http://dati.gov.it/onto/dcatapit#Organization"/>
  <rdfs:Class rdf:about="http://dati.gov.it/onto/dcatapit#Dataset"/>
  <rdfs:Class rdf:about="http://www.w3.org/2004/02/skos/core#ConceptScheme"/>
  <rdfs:Class rdf:about="http://dati.gov.it/onto/dcatapit#Standard"/>
  <rdfs:Class rdf:about="http://xmlns.com/foaf/0.1/Agent"/>
  <rdfs:Class rdf:about="https://w3id.org/italia/onto/Route/RouteType"/>
  <rdfs:Class rdf:about="http://www.w3.org/2004/02/skos/core#Concept"/>
  <rdfs:Class rdf:about="http://dati.gov.it/onto/dcatapit#Agent"/>
  <rdfs:Class rdf:about="http://www.w3.org/2006/vcard/ns#Kind"/>
  <rdfs:Class rdf:about="http://dati.gov.it/onto/dcatapit#Distribution"/>
  <rdfs:Class rdf:about="http://www.w3.org/2006/vcard/ns#Organization"/>
  <rdfs:Class rdf:about="http://purl.org/dc/terms/Standard"/>
</rdf:RDF>
