<rdf:RDF xmlns="https://w3id.org/italia/onto/Transparency/" xmlns:CLV="https://w3id.org/italia/onto/CLV/" xmlns:adms="http://www.w3.org/ns/adms#" xmlns:admsapit="https://w3id.org/italia/onto/ADMS/" xmlns:dc="http://purl.org/dc/elements/1.1/" xmlns:dcat="http://www.w3.org/ns/dcat#" xmlns:dcatapit="http://dati.gov.it/onto/dcatapit#" xmlns:dct="http://purl.org/dc/terms/" xmlns:foaf="http://xmlns.com/foaf/0.1/" xmlns:l0="https://w3id.org/italia/onto/l0/" xmlns:ns="http://www.w3.org/2006/vcard/ns#" xmlns:owl="http://www.w3.org/2002/07/owl#" xmlns:prov="http://www.w3.org/ns/prov#" xmlns:rdf="http://www.w3.org/1999/02/22-rdf-syntax-ns#" xmlns:rdfs="http://www.w3.org/2000/01/rdf-schema#" xmlns:skos="http://www.w3.org/2004/02/skos/core#" xmlns:smapit="https://w3id.org/italia/onto/SM/" xmlns:tiapit="https://w3id.org/italia/onto/TI/" xmlns:xkos="http://rdf-vocabulary.ddialliance.org/xkos#" xmlns:xsd="http://www.w3.org/2001/XMLSchema#" xml:base="https://w3id.org/italia/onto/Transparency/">
    <owl:Ontology rdf:about="https://w3id.org/italia/onto/l0">
        <owl:versionIRI rdf:resource="https://w3id.org/italia/onto/Transparency/0.2"></owl:versionIRI>
        <owl:imports rdf:resource="https://w3id.org/italia/onto/COV"></owl:imports>
        <owl:imports rdf:resource="https://w3id.org/italia/onto/TI"></owl:imports>
        <owl:imports rdf:resource="https://w3id.org/italia/onto/l0"></owl:imports>
        <dct:accrualPeriodicity rdf:resource="http://publications.europa.eu/resource/authority/frequency/IRREG"></dct:accrualPeriodicity>
        <dct:creator rdf:resource="http://spcdata.digitpa.gov.it/Amministrazione/agid"></dct:creator>
        <dct:creator rdf:resource="https://w3id.org/italia/data/organization/private-organization/05481840964"></dct:creator>
        <dct:description rdf:resource="https://w3id.org/italia/onto/Transparency/./latest/img/Transparency-AP_IT.png"></dct:description>
        <dct:description xml:lang="it">Questo è il profilo applicativo italiano dell'Ontologia degli Obblighi della Trasparenza. L'ontologia di OntoPiA implementa le disposizioni in merito all'obbligo di pubblicazione di contenuti informativi nella sezione 'Amministrazione Trasparente' dei siti istituzioonali delle publiche amministrazioni. Questa versione dell'ontologia è in attesa di essere visionata da ANAC.</dct:description>
        <dct:description xml:lang="en">This is the Italian application profile of the Transparency Obligations Ontology. This ontology of OntoPiA implements the dispositions about the publication obligation of informative contents on the section 'Transparent Administration' of the official website of the public administrations. This ontology version is a draft waiting for the ANAC validation.</dct:description>
        <dct:issued rdf:datatype="http://www.w3.org/2001/XMLSchema#date">2019-05-30</dct:issued>
        <dct:language rdf:resource="http://publications.europa.eu/resource/authority/language/ENG"></dct:language>
        <dct:language rdf:resource="http://publications.europa.eu/resource/authority/language/ITA"></dct:language>
        <dct:modified rdf:datatype="http://www.w3.org/2001/XMLSchema#date">2020-04-23</dct:modified>
        <dct:publisher rdf:resource="http://spcdata.digitpa.gov.it/Amministrazione/agid"></dct:publisher>
        <dct:rightsHolder rdf:resource="http://spcdata.digitpa.gov.it/Amministrazione/agid"></dct:rightsHolder>
        <dct:title xml:lang="it">Ontologia dell'Amministrazione Trasparente - profilo applicativo italiano</dct:title>
        <rdfs:comment xml:lang="it">Questo è il profilo applicativo italiano dell'Ontologia degli Obblighi della Trasparenza. L'ontologia di OntoPiA implementa le disposizioni in merito all'obbligo di pubblicazione di contenuti informativi nella sezione 'Amministrazione Trasparente' dei siti istituzionali delle publiche amministrazioni. Questa versione dell'ontologia è in attesa di essere visionata da ANAC.</rdfs:comment>
        <rdfs:comment xml:lang="en">This is the Italian application profile of the Transparency Obligations Ontology. This ontology of OntoPiA implements the dispositions about the publication obligation of informative contents on the section 'Transparent Administration' of the official website of the public administrations. This ontology version is a draft waiting for the ANAC validation.</rdfs:comment>
        <rdfs:isDefinedBy rdf:resource="https://w3id.org/italia/onto/Transparency"></rdfs:isDefinedBy>
        <rdfs:label xml:lang="it">Ontologia degli Obblighi della Trasparenza - profilo applicativo italiano</rdfs:label>
        <rdfs:label xml:lang="en">Transparency Obligations Ontology - Italian application profile</rdfs:label>
        <owl:versionInfo xml:lang="it">La presente versione dell'ontologia è un draft in attesa di revisone da parte di ANAC.</owl:versionInfo>
        <owl:versionInfo xml:lang="en">version 0.2 - added property appliesToOrganization which replaces appliesToPA, added property exceprionObligationNote, updated TransparencyObligation and TransparencySubjct modifing restrictions and stating skos:Concept derivation, stating disjoint among TransparencyArchiveActivity and TransparencyUpdateActivity.</owl:versionInfo>
        <owl:versionInfo xml:lang="it">version 0.2 - aggiunta proprietà appliesToOrganization che sostituisce appliesToPA, aggiunta proprietà exceprionObligationNote, aggiornati TransparencyObligation e TransparencySubjct modificando le restrizioni e dichiarando che deriva da skos:Concept, aggiunto disjoint tra TransparencyArchiveActivity e TransparencyUpdateActivity</owl:versionInfo>
        <dcat:contactPoint rdf:resource="http://dati.gov.it/data/resource/ContactPoint/voc_AgID"></dcat:contactPoint>
        <dcat:keyword xml:lang="en">transparency</dcat:keyword>
        <dcat:keyword xml:lang="en">transparency for public administration</dcat:keyword>
        <dcat:keyword xml:lang="it">trasparenza</dcat:keyword>
        <dcat:keyword xml:lang="it">trasparenza PA</dcat:keyword>
        <dcat:keyword xml:lang="it">trasparenza pa</dcat:keyword>
        <dcat:keyword xml:lang="it">trasparenza pubblica amministrazione</dcat:keyword>
        <dcat:theme rdf:resource="http://publications.europa.eu/resource/authority/data-theme/GOVE"></dcat:theme>
        <dcat:theme rdf:resource="http://publications.europa.eu/resource/authority/data-theme/TECH"></dcat:theme>
        <admsapit:acronym>Transparency-AP_IT</admsapit:acronym>
        <admsapit:hasFormalityLevel rdf:resource="https://w3id.org/italia/onto/ADMS/Formal"></admsapit:hasFormalityLevel>
        <admsapit:hasOntologyLanguage rdf:resource="https://w3id.org/italia/onto/ADMS/OWL"></admsapit:hasOntologyLanguage>
        <admsapit:hasSemanticAssetDistribution rdf:resource="https://w3id.org/italia/data/distribution/TRAPIT-JSON-LD"></admsapit:hasSemanticAssetDistribution>
        <admsapit:hasSemanticAssetDistribution rdf:resource="https://w3id.org/italia/data/distribution/TRAPIT-RDF-TURTLE"></admsapit:hasSemanticAssetDistribution>
        <admsapit:hasSemanticAssetDistribution rdf:resource="https://w3id.org/italia/data/distribution/TRAPIT-RDF-XML"></admsapit:hasSemanticAssetDistribution>
        <admsapit:hasTask rdf:resource="https://w3id.org/italia/onto/ADMS/AnnotationTask"></admsapit:hasTask>
        <admsapit:hasTask rdf:resource="https://w3id.org/italia/onto/ADMS/QueryFormulationTask"></admsapit:hasTask>
        <admsapit:hasTask rdf:resource="https://w3id.org/italia/onto/ADMS/SearchTask"></admsapit:hasTask>
        <admsapit:last rdf:resource="https://w3id.org/italia/onto/Transparency/0.1"></admsapit:last>
        <admsapit:officialURI rdf:datatype="http://www.w3.org/2001/XMLSchema#anyURI">https://w3id.org/italia/onto/Transparency</admsapit:officialURI>
        <admsapit:prefix>trapit</admsapit:prefix>
        <admsapit:semanticAssetInUse rdf:resource="https://w3id.org/italia/data/project/DAF"></admsapit:semanticAssetInUse>
        <admsapit:semanticAssetInUse rdf:resource="https://w3id.org/italia/data/project/OntoPiA"></admsapit:semanticAssetInUse>
        <admsapit:status>draft</admsapit:status>
        <admsapit:target xml:lang="it">Cittadini</admsapit:target>
        <admsapit:target xml:lang="it">Pubbliche amministrazioni</admsapit:target>
        <admsapit:type rdf:resource="https://w3id.org/italia/onto/ADMS/DomainOntology"></admsapit:type>
    </owl:Ontology>
    


    <!-- 
    ///////////////////////////////////////////////////////////////////////////////////////
    //
    // Annotation properties
    //
    ///////////////////////////////////////////////////////////////////////////////////////
     -->

    


    <!-- http://www.w3.org/2000/01/rdf-schema#labels -->

    <owl:AnnotationProperty rdf:about="http://www.w3.org/2000/01/rdf-schema#labels"></owl:AnnotationProperty>
    


    <!-- 
    ///////////////////////////////////////////////////////////////////////////////////////
    //
    // Datatypes
    //
    ///////////////////////////////////////////////////////////////////////////////////////
     -->

    


    <!-- http://www.w3.org/2001/XMLSchema#date -->

    <rdfs:Datatype rdf:about="http://www.w3.org/2001/XMLSchema#date"></rdfs:Datatype>
    


    <!-- http://www.w3.org/2001/XMLSchema#time -->

    <rdfs:Datatype rdf:about="http://www.w3.org/2001/XMLSchema#time"></rdfs:Datatype>
    


    <!-- 
    ///////////////////////////////////////////////////////////////////////////////////////
    //
    // Object Properties
    //
    ///////////////////////////////////////////////////////////////////////////////////////
     -->

    


    <!-- https://w3id.org/italia/onto/Transparency/appliesToOrganization -->

    <owl:ObjectProperty rdf:about="https://w3id.org/italia/onto/Transparency/appliesToOrganization">
        <owl:inverseOf rdf:resource="https://w3id.org/italia/onto/Transparency/obligedToEnforce"></owl:inverseOf>
        <rdfs:domain rdf:resource="https://w3id.org/italia/onto/Transparency/TransparencyObligation"></rdfs:domain>
        <rdfs:range>
            <owl:Class>
                <owl:unionOf rdf:parseType="Collection">
                    <rdf:Description rdf:about="https://w3id.org/italia/onto/COV/Organization"></rdf:Description>
                    <rdf:Description rdf:about="https://w3id.org/italia/onto/COV/PublicOrganizationCategory"></rdf:Description>
                </owl:unionOf>
            </owl:Class>
        </rdfs:range>
        <rdfs:comment xml:lang="it">Questa proprietà lega un obbligo di trasparenza all'organizzazione o a alla tipologia di pubblica amministrazione a cui si applica.</rdfs:comment>
        <rdfs:comment xml:lang="en">This property links a transparency obligation to a organization or a public administration category to whom is applied.</rdfs:comment>
        <rdfs:isDefinedBy rdf:resource="https://w3id.org/italia/onto/Transparency"></rdfs:isDefinedBy>
        <rdfs:label xml:lang="en">applies to organization</rdfs:label>
        <rdfs:label xml:lang="it">si applica all'organizzazione</rdfs:label>
        <owl:versionInfo xml:lang="it">stabile - proprietà aggiunta nella versione 0.2, sostituisce la proprietà appliesToPA</owl:versionInfo>
        <owl:versionInfo xml:lang="en">stable  - property added to version 0.2, it replaces the property appliesToPA</owl:versionInfo>
    </owl:ObjectProperty>
    


    <!-- https://w3id.org/italia/onto/Transparency/definesUpdateFrequency -->

    <owl:ObjectProperty rdf:about="https://w3id.org/italia/onto/Transparency/definesUpdateFrequency">
        <rdfs:domain rdf:resource="https://w3id.org/italia/onto/Transparency/TransparencyObligation"></rdfs:domain>
        <rdfs:range rdf:resource="https://w3id.org/italia/onto/Transparency/UpdateFrequency"></rdfs:range>
        <rdfs:comment xml:lang="it">Questa proprietà collega un obbligo di trasparenza alla frequenza di aggiornamento da esso definita.</rdfs:comment>
        <rdfs:comment xml:lang="en">This property links a transparency obligation to the update frequency which it defines.</rdfs:comment>
        <rdfs:isDefinedBy rdf:resource="https://w3id.org/italia/onto/Transparency"></rdfs:isDefinedBy>
        <rdfs:label xml:lang="en">defines update frequency</rdfs:label>
        <rdfs:label xml:lang="it">definisce frequenza di aggiornamento</rdfs:label>
        <owl:versionInfo xml:lang="it">stabile</owl:versionInfo>
        <owl:versionInfo xml:lang="en">stable</owl:versionInfo>
    </owl:ObjectProperty>
    


    <!-- https://w3id.org/italia/onto/Transparency/generatedBy -->

    <owl:ObjectProperty rdf:about="https://w3id.org/italia/onto/Transparency/generatedBy">
        <owl:inverseOf rdf:resource="https://w3id.org/italia/onto/Transparency/generatesResource"></owl:inverseOf>
        <rdfs:domain rdf:resource="https://w3id.org/italia/onto/Transparency/TransparencyResource"></rdfs:domain>
        <rdfs:range rdf:resource="https://w3id.org/italia/onto/Transparency/TransparencyActivity"></rdfs:range>
        <rdfs:comment xml:lang="it">Questa proprità lega una risorsa all'attività che la genera.</rdfs:comment>
        <rdfs:comment xml:lang="en">This property links a transparency resource to the activity from which is generated by.</rdfs:comment>
        <rdfs:isDefinedBy rdf:resource="https://w3id.org/italia/onto/Transparency"></rdfs:isDefinedBy>
        <rdfs:label xml:lang="en">generated by</rdfs:label>
        <rdfs:label xml:lang="it">generato da</rdfs:label>
        <owl:versionInfo xml:lang="it">stabile</owl:versionInfo>
        <owl:versionInfo xml:lang="en">stable</owl:versionInfo>
    </owl:ObjectProperty>
    


    <!-- https://w3id.org/italia/onto/Transparency/generatesResource -->

    <owl:ObjectProperty rdf:about="https://w3id.org/italia/onto/Transparency/generatesResource">
        <rdfs:domain rdf:resource="https://w3id.org/italia/onto/Transparency/TransparencyActivity"></rdfs:domain>
        <rdfs:range rdf:resource="https://w3id.org/italia/onto/Transparency/TransparencyResource"></rdfs:range>
        <rdfs:comment xml:lang="it">Questa proprietà lega un'attività della trasparenza alla risorsa generata come risultato dell'attività.</rdfs:comment>
        <rdfs:comment xml:lang="en">This property links a transparency activity to the resource generated as outcome of it.</rdfs:comment>
        <rdfs:isDefinedBy rdf:resource="https://w3id.org/italia/onto/Transparency"></rdfs:isDefinedBy>
        <rdfs:label xml:lang="en">generates resource</rdfs:label>
        <rdfs:label xml:lang="it">produce risorsa</rdfs:label>
        <owl:versionInfo xml:lang="it">stabile</owl:versionInfo>
        <owl:versionInfo xml:lang="en">stable</owl:versionInfo>
    </owl:ObjectProperty>
    


    <!-- https://w3id.org/italia/onto/Transparency/hasAllowedFormat -->

    <owl:ObjectProperty rdf:about="https://w3id.org/italia/onto/Transparency/hasAllowedFormat">
        <rdfs:domain rdf:resource="https://w3id.org/italia/onto/Transparency/TransparencyResource"></rdfs:domain>
        <rdfs:range rdf:resource="https://w3id.org/italia/onto/Transparency/Format"></rdfs:range>
        <rdfs:comment xml:lang="it">Questa proprità lega una risorsa della trasparenza al formato definito per la pubblicazione</rdfs:comment>
        <rdfs:comment xml:lang="en">This property links a transparency resource to the allowed format defined for publication.</rdfs:comment>
        <rdfs:isDefinedBy rdf:resource="https://w3id.org/italia/onto/Transparency"></rdfs:isDefinedBy>
        <rdfs:label xml:lang="it">da pubblicare nel formato</rdfs:label>
        <rdfs:label xml:lang="en">has allowed format</rdfs:label>
        <owl:versionInfo xml:lang="it">stabile</owl:versionInfo>
        <owl:versionInfo xml:lang="en">stable</owl:versionInfo>
    </owl:ObjectProperty>
    


    <!-- https://w3id.org/italia/onto/Transparency/hasTransparencyActivityTypology -->

    <owl:ObjectProperty rdf:about="https://w3id.org/italia/onto/Transparency/hasTransparencyActivityTypology">
        <rdfs:domain rdf:resource="https://w3id.org/italia/onto/Transparency/TransparencyActivity"></rdfs:domain>
        <rdfs:range rdf:resource="https://w3id.org/italia/onto/Transparency/TransparencyActivityTypology"></rdfs:range>
        <rdfs:comment xml:lang="it">Questa proprietà lega una attività della trasparenza alla sua tipologia.</rdfs:comment>
        <rdfs:comment xml:lang="en">This property links a transparency activity to its typology.</rdfs:comment>
        <rdfs:isDefinedBy rdf:resource="https://w3id.org/italia/onto/Transparency"></rdfs:isDefinedBy>
        <rdfs:label xml:lang="it">ha tipologia di attività della trasparenza</rdfs:label>
        <rdfs:label xml:lang="en">has transparency activity typology</rdfs:label>
        <owl:versionInfo xml:lang="it">stabile</owl:versionInfo>
        <owl:versionInfo xml:lang="en">stable</owl:versionInfo>
    </owl:ObjectProperty>
    


    <!-- https://w3id.org/italia/onto/Transparency/hasTransparencyStatus -->

    <owl:ObjectProperty rdf:about="https://w3id.org/italia/onto/Transparency/hasTransparencyStatus">
        <rdfs:domain rdf:resource="https://w3id.org/italia/onto/Transparency/TransparencyObligation"></rdfs:domain>
        <rdfs:range rdf:resource="https://w3id.org/italia/onto/Transparency/TransparencyObligationStatus"></rdfs:range>
        <rdfs:comment xml:lang="it">Questa proprietà lega un obbligo di trasparenza al suo stato attuale.</rdfs:comment>
        <rdfs:comment xml:lang="en">This property links a transparency obligation to its current status.</rdfs:comment>
        <rdfs:isDefinedBy rdf:resource="https://w3id.org/italia/onto/Transparency"></rdfs:isDefinedBy>
        <rdfs:label xml:lang="it">ha stato trasparenza</rdfs:label>
        <rdfs:label xml:lang="en">has transparency status</rdfs:label>
        <owl:versionInfo xml:lang="it">stabile</owl:versionInfo>
        <owl:versionInfo xml:lang="en">stable</owl:versionInfo>
    </owl:ObjectProperty>
    


    <!-- https://w3id.org/italia/onto/Transparency/hasTransparencySubject -->

    <owl:ObjectProperty rdf:about="https://w3id.org/italia/onto/Transparency/hasTransparencySubject">
        <rdfs:domain rdf:resource="https://w3id.org/italia/onto/Transparency/TransparencyObligation"></rdfs:domain>
        <rdfs:range rdf:resource="https://w3id.org/italia/onto/Transparency/TransparencySubject"></rdfs:range>
        <rdfs:comment xml:lang="it">Questa proprietà lega un obbligo di trasparenza ai temi che lo caratterizzano.</rdfs:comment>
        <rdfs:comment xml:lang="en">This property links a transparency obligation to the related subjects.</rdfs:comment>
        <rdfs:isDefinedBy rdf:resource="https://w3id.org/italia/onto/Transparency"></rdfs:isDefinedBy>
        <rdfs:label xml:lang="it">ha soggetto della trasparenza</rdfs:label>
        <rdfs:label xml:lang="it">ha tema della trasparenza</rdfs:label>
        <rdfs:label xml:lang="en">has transparency subject</rdfs:label>
        <rdfs:label xml:lang="en">has transparency theme</rdfs:label>
        <owl:versionInfo xml:lang="it">stabile</owl:versionInfo>
        <owl:versionInfo xml:lang="en">stable</owl:versionInfo>
    </owl:ObjectProperty>
    


    <!-- https://w3id.org/italia/onto/Transparency/isClassifiedBy -->

    <owl:ObjectProperty rdf:about="https://w3id.org/italia/onto/Transparency/isClassifiedBy">
        <rdfs:domain rdf:resource="https://w3id.org/italia/onto/Transparency/TransparencyObligation"></rdfs:domain>
        <rdfs:range rdf:resource="https://w3id.org/italia/onto/Transparency/TransparencyDataTypology"></rdfs:range>
        <rdfs:comment xml:lang="it">Questa proprietà lega un obbligo di trasparenza alla relativa tipologia. Le voci sono controllate della tassonomia https://w3id.org/italia/controlled-vocabulary/classifications-for-transparency/transparency-titulus</rdfs:comment>
        <rdfs:comment xml:lang="en">This property links a transparency obligation to the corresponding data typology. The values are controlled by the taxonomy  https://w3id.org/italia/controlled-vocabulary/classifications-for-transparency/transparency-titulus </rdfs:comment>
        <rdfs:isDefinedBy rdf:resource="https://w3id.org/italia/onto/Transparency"></rdfs:isDefinedBy>
        <rdfs:labels xml:lang="en">is classified by</rdfs:labels>
        <rdfs:labels xml:lang="it">è classificato da</rdfs:labels>
        <owl:versionInfo xml:lang="it">stabile</owl:versionInfo>
        <owl:versionInfo xml:lang="en">stable</owl:versionInfo>
    </owl:ObjectProperty>
    


    <!-- https://w3id.org/italia/onto/Transparency/isPerformedByAgent -->

    <owl:ObjectProperty rdf:about="https://w3id.org/italia/onto/Transparency/isPerformedByAgent">
        <rdfs:domain rdf:resource="https://w3id.org/italia/onto/Transparency/TransparencyActivity"></rdfs:domain>
        <rdfs:range rdf:resource="https://w3id.org/italia/onto/l0/Agent"></rdfs:range>
        <rdfs:comment xml:lang="it">Questa proprietà lega una attività al soggetto che la esegue.</rdfs:comment>
        <rdfs:comment xml:lang="en">This property links a transparency activity to the agent that performs it.</rdfs:comment>
        <rdfs:isDefinedBy rdf:resource="https://w3id.org/italia/onto/Transparency"></rdfs:isDefinedBy>
        <rdfs:label xml:lang="en">is performed by</rdfs:label>
        <rdfs:label xml:lang="it">è eseguita da</rdfs:label>
        <owl:versionInfo xml:lang="it">stabile</owl:versionInfo>
        <owl:versionInfo xml:lang="en">stable</owl:versionInfo>
    </owl:ObjectProperty>
    


    <!-- https://w3id.org/italia/onto/Transparency/isVersionOf -->

    <owl:ObjectProperty rdf:about="https://w3id.org/italia/onto/Transparency/isVersionOf">
        <rdfs:domain rdf:resource="https://w3id.org/italia/onto/Transparency/TransparencyResource"></rdfs:domain>
        <rdfs:range rdf:resource="https://w3id.org/italia/onto/Transparency/TransparencyResource"></rdfs:range>
        <rdfs:comment xml:lang="it">Questa proprietà lega una risorsa ad una sua versione.</rdfs:comment>
        <rdfs:comment xml:lang="en">This property links a transparency resource to its other version.</rdfs:comment>
        <rdfs:isDefinedBy rdf:resource="https://w3id.org/italia/onto/Transparency"></rdfs:isDefinedBy>
        <rdfs:label xml:lang="en">version of</rdfs:label>
        <rdfs:label xml:lang="it">versione di</rdfs:label>
        <owl:versionInfo xml:lang="it">stabile</owl:versionInfo>
        <owl:versionInfo xml:lang="en">stable</owl:versionInfo>
    </owl:ObjectProperty>
    


    <!-- https://w3id.org/italia/onto/Transparency/mustBeUptodatedWithin -->

    <owl:ObjectProperty rdf:about="https://w3id.org/italia/onto/Transparency/mustBeUptodatedWithin">
        <rdfs:domain rdf:resource="https://w3id.org/italia/onto/Transparency/TransparencyResource"></rdfs:domain>
        <rdfs:range rdf:resource="https://w3id.org/italia/onto/Transparency/UpdateFrequency"></rdfs:range>
        <rdfs:comment xml:lang="it">Questa proprietà collega una risorsa della trasparenza alla frequenza con cui deve addiornamento.</rdfs:comment>
        <rdfs:comment xml:lang="en">This property links a transparency resource to the prescribed update frequency.</rdfs:comment>
        <rdfs:isDefinedBy rdf:resource="https://w3id.org/italia/onto/Transparency"></rdfs:isDefinedBy>
        <rdfs:label xml:lang="it">deve essere aggiornata entro</rdfs:label>
        <rdfs:label xml:lang="en">must be update within</rdfs:label>
        <owl:versionInfo xml:lang="it">stabile</owl:versionInfo>
        <owl:versionInfo xml:lang="en">stable</owl:versionInfo>
    </owl:ObjectProperty>
    


    <!-- https://w3id.org/italia/onto/Transparency/obligedToEnforce -->

    <owl:ObjectProperty rdf:about="https://w3id.org/italia/onto/Transparency/obligedToEnforce">
        <rdfs:domain>
            <owl:Class>
                <owl:unionOf rdf:parseType="Collection">
                    <rdf:Description rdf:about="https://w3id.org/italia/onto/COV/Organization"></rdf:Description>
                    <rdf:Description rdf:about="https://w3id.org/italia/onto/COV/PublicOrganizationCategory"></rdf:Description>
                </owl:unionOf>
            </owl:Class>
        </rdfs:domain>
        <rdfs:range rdf:resource="https://w3id.org/italia/onto/Transparency/TransparencyObligation"></rdfs:range>
        <rdfs:comment xml:lang="it">Questa proprietà lega una organizzazione o una tipologia di pubblica amministrazione agli obblighi di trasparenza che è obbligata a rispettare.</rdfs:comment>
        <rdfs:comment xml:lang="en">This property links a organization or a public administration category to the transparecy obligations which is obliged to enforce.</rdfs:comment>
        <rdfs:isDefinedBy rdf:resource="https://w3id.org/italia/onto/Transparency"></rdfs:isDefinedBy>
        <rdfs:label xml:lang="it">obbligata a rispettare l'obbligo</rdfs:label>
        <rdfs:label xml:lang="en">obliged to enforce obligation</rdfs:label>
        <owl:versionInfo xml:lang="it">stabile - modificata nella versione 0.2</owl:versionInfo>
        <owl:versionInfo xml:lang="en">stable - modified in version 0.2</owl:versionInfo>
    </owl:ObjectProperty>
    


    <!-- https://w3id.org/italia/onto/Transparency/performsTransparencyActivity -->

    <owl:ObjectProperty rdf:about="https://w3id.org/italia/onto/Transparency/performsTransparencyActivity">
        <rdfs:domain rdf:resource="https://w3id.org/italia/onto/l0/Agent"></rdfs:domain>
        <rdfs:range rdf:resource="https://w3id.org/italia/onto/Transparency/TransparencyActivity"></rdfs:range>
        <rdfs:comment xml:lang="it">Questa proprietà lega una attività al soggetto che la esegue.</rdfs:comment>
        <rdfs:comment xml:lang="en">This property links a transparency activity to the agent that performs it.</rdfs:comment>
        <rdfs:isDefinedBy rdf:resource="https://w3id.org/italia/onto/Transparency"></rdfs:isDefinedBy>
        <rdfs:label xml:lang="it">esegue attività della trasparenza</rdfs:label>
        <rdfs:label xml:lang="en">performs transparency activity</rdfs:label>
        <owl:versionInfo xml:lang="it">stabile</owl:versionInfo>
        <owl:versionInfo xml:lang="en">stable</owl:versionInfo>
    </owl:ObjectProperty>
    


    <!-- https://w3id.org/italia/onto/Transparency/refersToTransparencyEntity -->

    <owl:ObjectProperty rdf:about="https://w3id.org/italia/onto/Transparency/refersToTransparencyEntity">
        <rdfs:domain rdf:resource="https://w3id.org/italia/onto/Transparency/TransparencyResource"></rdfs:domain>
        <rdfs:range>
            <owl:Class>
                <owl:unionOf rdf:parseType="Collection">
                    <rdf:Description rdf:about="https://w3id.org/italia/onto/l0/Activity"></rdf:Description>
                    <rdf:Description rdf:about="https://w3id.org/italia/onto/l0/Object"></rdf:Description>
                </owl:unionOf>
            </owl:Class>
        </rdfs:range>
        <rdfs:comment xml:lang="it">Questa proprità lega una risorsa della trasparenza alle entità ad essa collegata</rdfs:comment>
        <rdfs:comment xml:lang="en">This property links a transparency resource to the related entities.</rdfs:comment>
        <rdfs:isDefinedBy rdf:resource="https://w3id.org/italia/onto/Transparency"></rdfs:isDefinedBy>
        <rdfs:label xml:lang="en">refers to transparency entity</rdfs:label>
        <rdfs:label xml:lang="it">si riferisce a entità</rdfs:label>
        <owl:versionInfo xml:lang="it">stabile</owl:versionInfo>
        <owl:versionInfo xml:lang="en">stable</owl:versionInfo>
    </owl:ObjectProperty>
    


    <!-- https://w3id.org/italia/onto/Transparency/refersToTransparencySubject -->

    <owl:ObjectProperty rdf:about="https://w3id.org/italia/onto/Transparency/refersToTransparencySubject">
        <rdfs:domain>
            <owl:Class>
                <owl:unionOf rdf:parseType="Collection">
                    <rdf:Description rdf:about="https://w3id.org/italia/onto/l0/Activity"></rdf:Description>
                    <rdf:Description rdf:about="https://w3id.org/italia/onto/l0/Object"></rdf:Description>
                </owl:unionOf>
            </owl:Class>
        </rdfs:domain>
        <rdfs:range rdf:resource="https://w3id.org/italia/onto/Transparency/TransparencySubject"></rdfs:range>
        <rdfs:comment xml:lang="it">Questa proprità lega una entità ai soggetti della trasparenza.</rdfs:comment>
        <rdfs:comment xml:lang="en">This property links an entity to the transparency subjects.</rdfs:comment>
        <rdfs:isDefinedBy rdf:resource="https://w3id.org/italia/onto/Transparency"></rdfs:isDefinedBy>
        <rdfs:label xml:lang="en">refers to transparency subject</rdfs:label>
        <rdfs:label xml:lang="it">si riferisce a soggetto</rdfs:label>
        <owl:versionInfo xml:lang="it">stabile</owl:versionInfo>
        <owl:versionInfo xml:lang="en">stable</owl:versionInfo>
    </owl:ObjectProperty>
    


    <!-- https://w3id.org/italia/onto/Transparency/subTransparencyObligationOf -->

    <owl:ObjectProperty rdf:about="https://w3id.org/italia/onto/Transparency/subTransparencyObligationOf">
        <owl:inverseOf rdf:resource="https://w3id.org/italia/onto/Transparency/superTransparencyObligationOf"></owl:inverseOf>
        <rdfs:domain rdf:resource="https://w3id.org/italia/onto/Transparency/TransparencyObligation"></rdfs:domain>
        <rdfs:range rdf:resource="https://w3id.org/italia/onto/Transparency/TransparencyObligation"></rdfs:range>
        <rdfs:comment xml:lang="it">Questa proprietà lega un obbligo di trasparenza ad un obbligo di cui fa parte.</rdfs:comment>
        <rdfs:comment xml:lang="en">This property links a transparency obligation to a transparency obligation of which is part of.</rdfs:comment>
        <rdfs:isDefinedBy rdf:resource="https://w3id.org/italia/onto/Transparency"></rdfs:isDefinedBy>
        <rdfs:label xml:lang="it">sotto-obbligo di trasparenza di</rdfs:label>
        <rdfs:label xml:lang="en">sub-transparency obligation of</rdfs:label>
        <owl:versionInfo xml:lang="it">stabile</owl:versionInfo>
        <owl:versionInfo xml:lang="en">stable</owl:versionInfo>
    </owl:ObjectProperty>
    


    <!-- https://w3id.org/italia/onto/Transparency/superTransparencyObligationOf -->

    <owl:ObjectProperty rdf:about="https://w3id.org/italia/onto/Transparency/superTransparencyObligationOf">
        <rdfs:domain rdf:resource="https://w3id.org/italia/onto/Transparency/TransparencyObligation"></rdfs:domain>
        <rdfs:range rdf:resource="https://w3id.org/italia/onto/Transparency/TransparencyObligation"></rdfs:range>
        <rdfs:comment xml:lang="it">Questa proprietà lega un obbligo di trasparenza ad un obbligo di cui è composto.</rdfs:comment>
        <rdfs:comment xml:lang="en">This property links a transparency obligation to a transparency obligation of which is composed by.</rdfs:comment>
        <rdfs:isDefinedBy rdf:resource="https://w3id.org/italia/onto/Transparency"></rdfs:isDefinedBy>
        <rdfs:label xml:lang="it">super-obbligo di trasparenza di</rdfs:label>
        <rdfs:label xml:lang="en">super-transparency obligation of</rdfs:label>
        <owl:versionInfo xml:lang="it">stabile</owl:versionInfo>
        <owl:versionInfo xml:lang="en">stable</owl:versionInfo>
    </owl:ObjectProperty>
    


    <!-- https://w3id.org/italia/onto/Transparency/triggeredBy -->

    <owl:ObjectProperty rdf:about="https://w3id.org/italia/onto/Transparency/triggeredBy">
        <owl:inverseOf rdf:resource="https://w3id.org/italia/onto/Transparency/triggers"></owl:inverseOf>
        <rdfs:domain rdf:resource="https://w3id.org/italia/onto/Transparency/TransparencyActivity"></rdfs:domain>
        <rdfs:range rdf:resource="https://w3id.org/italia/onto/Transparency/TransparencyObligation"></rdfs:range>
        <rdfs:comment xml:lang="it">Questa proprietà lega un obbligo di trasparenza all'attività che attiva.</rdfs:comment>
        <rdfs:comment xml:lang="en">This property links a trasparency obbligation to the activty triggered by it.</rdfs:comment>
        <rdfs:isDefinedBy rdf:resource="https://w3id.org/italia/onto/Transparency"></rdfs:isDefinedBy>
        <rdfs:label xml:lang="it">attivato da</rdfs:label>
        <rdfs:label xml:lang="en">triggered by</rdfs:label>
        <owl:versionInfo xml:lang="it">stabile</owl:versionInfo>
        <owl:versionInfo xml:lang="en">stable</owl:versionInfo>
    </owl:ObjectProperty>
    


    <!-- https://w3id.org/italia/onto/Transparency/triggers -->

    <owl:ObjectProperty rdf:about="https://w3id.org/italia/onto/Transparency/triggers">
        <rdfs:domain rdf:resource="https://w3id.org/italia/onto/Transparency/TransparencyObligation"></rdfs:domain>
        <rdfs:range rdf:resource="https://w3id.org/italia/onto/Transparency/TransparencyActivity"></rdfs:range>
        <rdfs:comment xml:lang="it">Questa proprietà lega un obbligo di trasparenza all'attività che attiva.</rdfs:comment>
        <rdfs:comment xml:lang="en">This property links a trasparency obbligation to the activty triggered by it.</rdfs:comment>
        <rdfs:isDefinedBy rdf:resource="https://w3id.org/italia/onto/Transparency"></rdfs:isDefinedBy>
        <rdfs:label xml:lang="it">attiva</rdfs:label>
        <rdfs:label xml:lang="en">triggers</rdfs:label>
        <owl:versionInfo xml:lang="it">stabile</owl:versionInfo>
        <owl:versionInfo xml:lang="en">stable</owl:versionInfo>
    </owl:ObjectProperty>
    


    <!-- 
    ///////////////////////////////////////////////////////////////////////////////////////
    //
    // Data properties
    //
    ///////////////////////////////////////////////////////////////////////////////////////
     -->

    


    <!-- https://w3id.org/italia/onto/Transparency/accessURL -->

    <owl:DatatypeProperty rdf:about="https://w3id.org/italia/onto/Transparency/accessURL">
        <rdfs:subPropertyOf rdf:resource="https://w3id.org/italia/onto/SM/URL"></rdfs:subPropertyOf>
        <rdfs:domain rdf:resource="https://w3id.org/italia/onto/Transparency/TransparencyResource"></rdfs:domain>
        <rdfs:range rdf:resource="http://www.w3.org/2001/XMLSchema#anyURI"></rdfs:range>
        <rdfs:comment xml:lang="it">Questa URL definisce l'indirizzo di accesso e reperimento del contenuto informativo.</rdfs:comment>
        <rdfs:comment xml:lang="en">This URL defines the access address of the informative content.</rdfs:comment>
        <rdfs:isDefinedBy rdf:resource="https://w3id.org/italia/onto/Transparency"></rdfs:isDefinedBy>
        <rdfs:label xml:lang="it">URL di accesso alla risorsa</rdfs:label>
        <rdfs:label xml:lang="en">access URL</rdfs:label>
        <owl:versionInfo xml:lang="it">stabile</owl:versionInfo>
        <owl:versionInfo xml:lang="en">stable</owl:versionInfo>
    </owl:DatatypeProperty>
    


    <!-- https://w3id.org/italia/onto/Transparency/downloadURL -->

    <owl:DatatypeProperty rdf:about="https://w3id.org/italia/onto/Transparency/downloadURL">
        <rdfs:subPropertyOf rdf:resource="https://w3id.org/italia/onto/SM/URL"></rdfs:subPropertyOf>
        <rdfs:domain rdf:resource="https://w3id.org/italia/onto/Transparency/TransparencyResource"></rdfs:domain>
        <rdfs:range rdf:resource="http://www.w3.org/2001/XMLSchema#anyURI"></rdfs:range>
        <rdfs:comment xml:lang="it">Questa URL definisce l'indirizzo di download del contenuto informativo.</rdfs:comment>
        <rdfs:comment xml:lang="en">This URL defines the download adress of the informative content.</rdfs:comment>
        <rdfs:isDefinedBy rdf:resource="https://w3id.org/italia/onto/Transparency"></rdfs:isDefinedBy>
        <rdfs:label xml:lang="it">URL di download del contenuto</rdfs:label>
        <rdfs:label xml:lang="en">download URL</rdfs:label>
        <owl:versionInfo xml:lang="it">stabile</owl:versionInfo>
        <owl:versionInfo xml:lang="en">stable</owl:versionInfo>
    </owl:DatatypeProperty>
    


    <!-- https://w3id.org/italia/onto/Transparency/exceptionObligationNote -->

    <owl:DatatypeProperty rdf:about="https://w3id.org/italia/onto/Transparency/exceptionObligationNote">
        <rdfs:subPropertyOf rdf:resource="https://w3id.org/italia/onto/l0/description"></rdfs:subPropertyOf>
        <rdfs:domain rdf:resource="https://w3id.org/italia/onto/Transparency/TransparencyObligation"></rdfs:domain>
        <rdfs:range rdf:resource="http://www.w3.org/2000/01/rdf-schema#Literal"></rdfs:range>
        <rdfs:comment xml:lang="it">Questa proprietà ha lo scopo di specificare le eccezzioni in merito all'applicazione dell'obbligo di trasparenza ad una organizzazione o tipologia di amministrazione.</rdfs:comment>
        <rdfs:comment xml:lang="en">This property is used to describe the exceptions related to the application of a transparency obbligation to a organization or an administration category.</rdfs:comment>
        <rdfs:isDefinedBy rdf:resource="https://w3id.org/italia/onto/Transparency"></rdfs:isDefinedBy>
        <rdfs:label xml:lang="en">exception obligation note</rdfs:label>
        <rdfs:label xml:lang="it">nota di eccezzione dell'obbligo</rdfs:label>
        <owl:versionInfo xml:lang="it">stabile - introdotta nella versione 0.2</owl:versionInfo>
        <owl:versionInfo xml:lang="en">stable - added to version 0.2</owl:versionInfo>
    </owl:DatatypeProperty>
    


    <!-- https://w3id.org/italia/onto/Transparency/regulationReference -->

    <owl:DatatypeProperty rdf:about="https://w3id.org/italia/onto/Transparency/regulationReference">
        <rdfs:domain rdf:resource="https://w3id.org/italia/onto/Transparency/TransparencyObligation"></rdfs:domain>
        <rdfs:range rdf:resource="http://www.w3.org/2000/01/rdf-schema#Literal"></rdfs:range>
        <rdfs:comment xml:lang="it">Questa proprietà lega un obbligo di trasparenza al riferimento normativo da cui deriva.</rdfs:comment>
        <rdfs:comment xml:lang="en">This property links a transparency obligation to the law that defines it.</rdfs:comment>
        <rdfs:isDefinedBy rdf:resource="https://w3id.org/italia/onto/Transparency"></rdfs:isDefinedBy>
        <rdfs:label xml:lang="en">normative reference</rdfs:label>
        <rdfs:label xml:lang="it">riferimento normativo</rdfs:label>
        <owl:versionInfo xml:lang="it">stabile</owl:versionInfo>
        <owl:versionInfo xml:lang="en">stable</owl:versionInfo>
    </owl:DatatypeProperty>
    


    <!-- 
    ///////////////////////////////////////////////////////////////////////////////////////
    //
    // Classes
    //
    ///////////////////////////////////////////////////////////////////////////////////////
     -->

    


    <!-- https://w3id.org/italia/onto/Transparency/Format -->

    <owl:Class rdf:about="https://w3id.org/italia/onto/Transparency/Format">
        <rdfs:subClassOf rdf:resource="https://w3id.org/italia/onto/l0/Characteristic"></rdfs:subClassOf>
        <rdfs:comment xml:lang="it">Questa classe indica il formato di una risorsa</rdfs:comment>
        <rdfs:comment xml:lang="en">This class represents the format of a resource.</rdfs:comment>
        <rdfs:isDefinedBy rdf:resource="https://w3id.org/italia/onto/Transparency"></rdfs:isDefinedBy>
        <rdfs:label xml:lang="en">Format</rdfs:label>
        <rdfs:label xml:lang="it">Formato</rdfs:label>
        <owl:versionInfo xml:lang="it">stabile</owl:versionInfo>
        <owl:versionInfo xml:lang="en">stable</owl:versionInfo>
    </owl:Class>
    


    <!-- https://w3id.org/italia/onto/Transparency/TransparencyActivity -->

    <owl:Class rdf:about="https://w3id.org/italia/onto/Transparency/TransparencyActivity">
        <rdfs:subClassOf rdf:resource="https://w3id.org/italia/onto/l0/Activity"></rdfs:subClassOf>
        <rdfs:subClassOf>
            <owl:Restriction>
                <owl:onProperty rdf:resource="https://w3id.org/italia/onto/Transparency/generatesResource"></owl:onProperty>
                <owl:someValuesFrom rdf:resource="https://w3id.org/italia/onto/Transparency/TransparencyResource"></owl:someValuesFrom>
            </owl:Restriction>
        </rdfs:subClassOf>
        <rdfs:subClassOf>
            <owl:Restriction>
                <owl:onProperty rdf:resource="https://w3id.org/italia/onto/Transparency/hasTransparencyActivityTypology"></owl:onProperty>
                <owl:someValuesFrom rdf:resource="https://w3id.org/italia/onto/Transparency/TransparencyActivityTypology"></owl:someValuesFrom>
            </owl:Restriction>
        </rdfs:subClassOf>
        <rdfs:subClassOf>
            <owl:Restriction>
                <owl:onProperty rdf:resource="https://w3id.org/italia/onto/Transparency/isPerformedByAgent"></owl:onProperty>
                <owl:qualifiedCardinality rdf:datatype="http://www.w3.org/2001/XMLSchema#nonNegativeInteger">1</owl:qualifiedCardinality>
                <owl:onClass rdf:resource="https://w3id.org/italia/onto/l0/Agent"></owl:onClass>
            </owl:Restriction>
        </rdfs:subClassOf>
        <rdfs:subClassOf>
            <owl:Restriction>
                <owl:onProperty rdf:resource="https://w3id.org/italia/onto/TI/date"></owl:onProperty>
                <owl:qualifiedCardinality rdf:datatype="http://www.w3.org/2001/XMLSchema#nonNegativeInteger">1</owl:qualifiedCardinality>
                <owl:onDataRange>
                    <rdfs:Datatype>
                        <owl:unionOf rdf:parseType="Collection">
                            <rdf:Description rdf:about="http://www.w3.org/2001/XMLSchema#date"></rdf:Description>
                            <rdf:Description rdf:about="http://www.w3.org/2001/XMLSchema#dateTime"></rdf:Description>
                        </owl:unionOf>
                    </rdfs:Datatype>
                </owl:onDataRange>
            </owl:Restriction>
        </rdfs:subClassOf>
        <rdfs:comment xml:lang="it">Questa classe rappresenta un'attività di trasparenza come conseguenza di un obbligo di trasparenza.</rdfs:comment>
        <rdfs:comment xml:lang="en">This class represents a trasparency activity as an effect of a transparency obbligation. For example pubblication, update,...</rdfs:comment>
        <rdfs:isDefinedBy rdf:resource="https://w3id.org/italia/onto/Transparency"></rdfs:isDefinedBy>
        <rdfs:label xml:lang="it">Attività di trasparenza.</rdfs:label>
        <rdfs:label xml:lang="en">Transparency activity</rdfs:label>
        <owl:versionInfo xml:lang="it">stabile</owl:versionInfo>
        <owl:versionInfo xml:lang="en">stable</owl:versionInfo>
    </owl:Class>
    


    <!-- https://w3id.org/italia/onto/Transparency/TransparencyActivityTypology -->

    <owl:Class rdf:about="https://w3id.org/italia/onto/Transparency/TransparencyActivityTypology">
        <rdfs:subClassOf rdf:resource="https://w3id.org/italia/onto/l0/Characteristic"></rdfs:subClassOf>
        <rdfs:comment xml:lang="it">Questa classe indica la tipologia di attività della trasparenza.</rdfs:comment>
        <rdfs:comment xml:lang="en">This class represents the transparency activity typology.</rdfs:comment>
        <rdfs:isDefinedBy rdf:resource="https://w3id.org/italia/onto/Transparency"></rdfs:isDefinedBy>
        <rdfs:label xml:lang="it">Tipologia di attività della trasparenza</rdfs:label>
        <rdfs:label xml:lang="en">Transparency activity typology</rdfs:label>
        <owl:versionInfo xml:lang="it">stabile</owl:versionInfo>
        <owl:versionInfo xml:lang="en">stable</owl:versionInfo>
    </owl:Class>
    


    <!-- https://w3id.org/italia/onto/Transparency/TransparencyArchiveActivity -->

    <owl:Class rdf:about="https://w3id.org/italia/onto/Transparency/TransparencyArchiveActivity">
        <owl:equivalentClass>
            <owl:Restriction>
                <owl:onProperty rdf:resource="https://w3id.org/italia/onto/Transparency/hasTransparencyActivityTypology"></owl:onProperty>
                <owl:hasValue rdf:resource="https://w3id.org/italia/onto/Transparency/TransparencyArchiveActivity"></owl:hasValue>
            </owl:Restriction>
        </owl:equivalentClass>
        <rdfs:subClassOf rdf:resource="https://w3id.org/italia/onto/Transparency/TransparencyActivity"></rdfs:subClassOf>
        <owl:disjointWith rdf:resource="https://w3id.org/italia/onto/Transparency/TransparencyPublicationActivity"></owl:disjointWith>
        <owl:disjointWith rdf:resource="https://w3id.org/italia/onto/Transparency/TransparencyUpdateActivity"></owl:disjointWith>
    </owl:Class>
    


    <!-- https://w3id.org/italia/onto/Transparency/TransparencyDataTypology -->

    <owl:Class rdf:about="https://w3id.org/italia/onto/Transparency/TransparencyDataTypology">
        <rdfs:subClassOf rdf:resource="https://w3id.org/italia/onto/l0/Characteristic"></rdfs:subClassOf>
        <rdfs:comment xml:lang="it">Questa classe rappresenta la tipologia di dati della trasparenza: i valori sono controllati dal vocabolario relativo, e determinano l'attuale strutturazione delle sezioni e sotto-sezioni dell'"Amministrazione Trasparente" dei siti web della PA come previsto dalla normativa di settore (d.lgs 33/2013 e s.m.i).</rdfs:comment>
        <rdfs:comment xml:lang="en">This class represents the typology of transparency data: the values are defined by a specific vocabulary, and are used to organize contents inside the current transparency section structure for the websites of the Italian Public Administrations, as defined by the legislation (d.lgs 33/2013 e s.m.i).</rdfs:comment>
        <rdfs:isDefinedBy rdf:resource="https://w3id.org/italia/onto/Transparency"></rdfs:isDefinedBy>
        <rdfs:label xml:lang="it">Tipologia dato della trasparenza</rdfs:label>
        <rdfs:label xml:lang="en">Transparency data typology</rdfs:label>
        <owl:versionInfo xml:lang="it">stabile</owl:versionInfo>
        <owl:versionInfo xml:lang="en">stable</owl:versionInfo>
        <l0:controlledVocabulary rdf:resource="https://w3id.org/italia/controlled-vocabulary/classifications-for-transparency/transparency-titulus"></l0:controlledVocabulary>
    </owl:Class>
    


    <!-- https://w3id.org/italia/onto/Transparency/TransparencyObligation -->

    <owl:Class rdf:about="https://w3id.org/italia/onto/Transparency/TransparencyObligation">
        <rdfs:subClassOf rdf:resource="https://w3id.org/italia/onto/l0/Description"></rdfs:subClassOf>
        <rdfs:subClassOf>
            <owl:Restriction>
                <owl:onProperty rdf:resource="https://w3id.org/italia/onto/TI/atTime"></owl:onProperty>
                <owl:allValuesFrom rdf:resource="https://w3id.org/italia/onto/TI/TimeInterval"></owl:allValuesFrom>
            </owl:Restriction>
        </rdfs:subClassOf>
        <rdfs:subClassOf>
            <owl:Restriction>
                <owl:onProperty rdf:resource="https://w3id.org/italia/onto/Transparency/appliesToOrganization"></owl:onProperty>
                <owl:minQualifiedCardinality rdf:datatype="http://www.w3.org/2001/XMLSchema#nonNegativeInteger">1</owl:minQualifiedCardinality>
                <owl:onClass>
                    <owl:Class>
                        <owl:unionOf rdf:parseType="Collection">
                            <rdf:Description rdf:about="https://w3id.org/italia/onto/COV/Organization"></rdf:Description>
                            <rdf:Description rdf:about="https://w3id.org/italia/onto/COV/PublicOrganizationCategory"></rdf:Description>
                        </owl:unionOf>
                    </owl:Class>
                </owl:onClass>
            </owl:Restriction>
        </rdfs:subClassOf>
        <rdfs:subClassOf>
            <owl:Restriction>
                <owl:onProperty rdf:resource="https://w3id.org/italia/onto/Transparency/isClassifiedBy"></owl:onProperty>
                <owl:minQualifiedCardinality rdf:datatype="http://www.w3.org/2001/XMLSchema#nonNegativeInteger">1</owl:minQualifiedCardinality>
                <owl:onClass rdf:resource="https://w3id.org/italia/onto/Transparency/TransparencyDataTypology"></owl:onClass>
            </owl:Restriction>
        </rdfs:subClassOf>
        <rdfs:subClassOf>
            <owl:Restriction>
                <owl:onProperty rdf:resource="https://w3id.org/italia/onto/Transparency/hasTransparencyStatus"></owl:onProperty>
                <owl:qualifiedCardinality rdf:datatype="http://www.w3.org/2001/XMLSchema#nonNegativeInteger">1</owl:qualifiedCardinality>
                <owl:onClass rdf:resource="https://w3id.org/italia/onto/Transparency/TransparencyObligationStatus"></owl:onClass>
            </owl:Restriction>
        </rdfs:subClassOf>
        <rdfs:subClassOf>
            <owl:Restriction>
                <owl:onProperty rdf:resource="https://w3id.org/italia/onto/Transparency/regulationReference"></owl:onProperty>
                <owl:someValuesFrom rdf:resource="http://www.w3.org/2000/01/rdf-schema#Literal"></owl:someValuesFrom>
            </owl:Restriction>
        </rdfs:subClassOf>
        <rdfs:comment xml:lang="it">Questa classe rappresenta gli obblighi di trasparenza definiti dalla normativa di riferimento a cui devono sottostare le Pubbliche Amministrazioni.</rdfs:comment>
        <rdfs:comment xml:lang="en">This class represents the transparency obligation for Public Administrations, according to the transparency norms.</rdfs:comment>
        <rdfs:isDefinedBy rdf:resource="https://w3id.org/italia/onto/Transparency"></rdfs:isDefinedBy>
        <rdfs:label xml:lang="it">Obbligo di trasparenza</rdfs:label>
        <rdfs:label xml:lang="en">Transparency Obligation</rdfs:label>
        <owl:versionInfo xml:lang="it">stabile - modificato nella versione 0.2, rimuovendo le restriction su l0:description e l0:name e aggiungendo che la classe deriva da skos:Concept, aggiungendo restriction su :appliesToOrganization, :hasTransparencyStatus.</owl:versionInfo>
        <owl:versionInfo xml:lang="en">stable - modified in version 0.2, removing therestrictions on l0:description and l0:name and adding that the class derives from skos:Concept, adding restriction on :appliesToOrganization, :hasTransparencyStatus.</owl:versionInfo>
        <prov:wasDerivedFrom rdf:resource="http://www.w3.org/2004/02/skos/core#Concept"></prov:wasDerivedFrom>
        <l0:controlledVocabulary rdf:resource="https://w3id.org/italia/controlled-vocabulary/classifications-for-transparency/transparency-obligation"></l0:controlledVocabulary>
    </owl:Class>
    


    <!-- https://w3id.org/italia/onto/Transparency/TransparencyObligationStatus -->

    <owl:Class rdf:about="https://w3id.org/italia/onto/Transparency/TransparencyObligationStatus">
        <rdfs:subClassOf rdf:resource="https://w3id.org/italia/onto/l0/Characteristic"></rdfs:subClassOf>
        <rdfs:comment xml:lang="it">Questa classe rappresenta lo stato dell'obbligo di trasparenza. Per esempio vigente, decaduto,...</rdfs:comment>
        <rdfs:comment xml:lang="en">This class represents the transparency obbligation status. Ex: in force, deprecated,...</rdfs:comment>
        <rdfs:isDefinedBy rdf:resource="https://w3id.org/italia/onto/Transparency"></rdfs:isDefinedBy>
        <rdfs:label xml:lang="it">Stato dell'obbligo di trasparenza.</rdfs:label>
        <rdfs:label xml:lang="en">Transparency obbligation status</rdfs:label>
        <owl:versionInfo xml:lang="it">stabile</owl:versionInfo>
        <owl:versionInfo xml:lang="en">stable</owl:versionInfo>
    </owl:Class>
    


    <!-- https://w3id.org/italia/onto/Transparency/TransparencyPublicationActivity -->

    <owl:Class rdf:about="https://w3id.org/italia/onto/Transparency/TransparencyPublicationActivity">
        <owl:equivalentClass>
            <owl:Restriction>
                <owl:onProperty rdf:resource="https://w3id.org/italia/onto/Transparency/hasTransparencyActivityTypology"></owl:onProperty>
                <owl:hasValue rdf:resource="https://w3id.org/italia/onto/Transparency/TransparencyPublicationActivity"></owl:hasValue>
            </owl:Restriction>
        </owl:equivalentClass>
        <rdfs:subClassOf rdf:resource="https://w3id.org/italia/onto/Transparency/TransparencyActivity"></rdfs:subClassOf>
        <owl:disjointWith rdf:resource="https://w3id.org/italia/onto/Transparency/TransparencyUpdateActivity"></owl:disjointWith>
    </owl:Class>
    


    <!-- https://w3id.org/italia/onto/Transparency/TransparencyResource -->

    <owl:Class rdf:about="https://w3id.org/italia/onto/Transparency/TransparencyResource">
        <rdfs:subClassOf rdf:resource="https://w3id.org/italia/onto/l0/Object"></rdfs:subClassOf>
        <rdfs:subClassOf>
            <owl:Restriction>
                <owl:onProperty rdf:resource="https://w3id.org/italia/onto/Transparency/refersToTransparencyEntity"></owl:onProperty>
                <owl:someValuesFrom>
                    <owl:Class>
                        <owl:unionOf rdf:parseType="Collection">
                            <rdf:Description rdf:about="https://w3id.org/italia/onto/l0/Activity"></rdf:Description>
                            <rdf:Description rdf:about="https://w3id.org/italia/onto/l0/Object"></rdf:Description>
                        </owl:unionOf>
                    </owl:Class>
                </owl:someValuesFrom>
            </owl:Restriction>
        </rdfs:subClassOf>
        <rdfs:subClassOf>
            <owl:Restriction>
                <owl:onProperty rdf:resource="https://w3id.org/italia/onto/l0/name"></owl:onProperty>
                <owl:someValuesFrom rdf:resource="http://www.w3.org/2000/01/rdf-schema#Literal"></owl:someValuesFrom>
            </owl:Restriction>
        </rdfs:subClassOf>
        <rdfs:subClassOf>
            <owl:Restriction>
                <owl:onProperty rdf:resource="https://w3id.org/italia/onto/Transparency/accessURL"></owl:onProperty>
                <owl:qualifiedCardinality rdf:datatype="http://www.w3.org/2001/XMLSchema#nonNegativeInteger">1</owl:qualifiedCardinality>
                <owl:onDataRange rdf:resource="http://www.w3.org/2001/XMLSchema#anyURI"></owl:onDataRange>
            </owl:Restriction>
        </rdfs:subClassOf>
        <rdfs:subClassOf>
            <owl:Restriction>
                <owl:onProperty rdf:resource="https://w3id.org/italia/onto/TI/modified"></owl:onProperty>
                <owl:maxQualifiedCardinality rdf:datatype="http://www.w3.org/2001/XMLSchema#nonNegativeInteger">1</owl:maxQualifiedCardinality>
                <owl:onDataRange>
                    <rdfs:Datatype>
                        <owl:unionOf rdf:parseType="Collection">
                            <rdf:Description rdf:about="http://www.w3.org/2001/XMLSchema#date"></rdf:Description>
                            <rdf:Description rdf:about="http://www.w3.org/2001/XMLSchema#dateTime"></rdf:Description>
                            <rdf:Description rdf:about="http://www.w3.org/2001/XMLSchema#time"></rdf:Description>
                        </owl:unionOf>
                    </rdfs:Datatype>
                </owl:onDataRange>
            </owl:Restriction>
        </rdfs:subClassOf>
        <rdfs:comment xml:lang="it">Questa classe rappresenta i documenti, le informazioni e i dati oggetto di pubblicazione nei siti istituzionali delle pubbliche amministrazioni.</rdfs:comment>
        <rdfs:comment xml:lang="en">This class represents documents, informazions and data object of publication on the official website of the public administrations.</rdfs:comment>
        <rdfs:isDefinedBy rdf:resource="https://w3id.org/italia/onto/Transparency"></rdfs:isDefinedBy>
        <rdfs:label xml:lang="it">Risorsa di trasparenza</rdfs:label>
        <rdfs:label xml:lang="en">Transparency resource</rdfs:label>
        <owl:versionInfo xml:lang="it">stabile</owl:versionInfo>
        <owl:versionInfo xml:lang="en">stable</owl:versionInfo>
    </owl:Class>
    


    <!-- https://w3id.org/italia/onto/Transparency/TransparencySubject -->

    <owl:Class rdf:about="https://w3id.org/italia/onto/Transparency/TransparencySubject">
        <rdfs:subClassOf rdf:resource="https://w3id.org/italia/onto/l0/Concept"></rdfs:subClassOf>
        <rdfs:comment xml:lang="it">Questa classe rappresenta un soggetto (tema) collegato a un obbligo di trasparenza. Fa riferimento alla colonna 'contenuto dell'obbligo' dell'allegato alla guida ANAC.</rdfs:comment>
        <rdfs:comment xml:lang="en">This class represents a subject releted to a transparency obbligation. It's related to the 'contenuto dell'obbligo' column of the ANAC guideline attachment.</rdfs:comment>
        <rdfs:isDefinedBy rdf:resource="https://w3id.org/italia/onto/Transparency"></rdfs:isDefinedBy>
        <rdfs:label xml:lang="it">Soggetto della trasparenza</rdfs:label>
        <rdfs:label xml:lang="en">Transparency subject</rdfs:label>
        <owl:versionInfo xml:lang="it">stabile - modificato nella versione 0.2, rimuovendo le restriction su l0:description e l0:name e aggiungendo che la classe deriva da skos:Concept, aggiuingendo collegamento con il vocabolario transparency-subject.</owl:versionInfo>
        <owl:versionInfo xml:lang="en">stable - modified in version 0.2, removing therestrictions on l0:description and l0:name and adding that the class derives from skos:Concept, adding link to transparency-subject vocabulary.</owl:versionInfo>
        <prov:wasDerivedFrom rdf:resource="http://www.w3.org/2004/02/skos/core#Concept"></prov:wasDerivedFrom>
        <l0:controlledVocabulary rdf:resource="https://w3id.org/italia/controlled-vocabulary/classifications-for-transparency/transparency-subject"></l0:controlledVocabulary>
    </owl:Class>
    


    <!-- https://w3id.org/italia/onto/Transparency/TransparencyUpdateActivity -->

    <owl:Class rdf:about="https://w3id.org/italia/onto/Transparency/TransparencyUpdateActivity">
        <owl:equivalentClass>
            <owl:Restriction>
                <owl:onProperty rdf:resource="https://w3id.org/italia/onto/Transparency/hasTransparencyActivityTypology"></owl:onProperty>
                <owl:hasValue rdf:resource="https://w3id.org/italia/onto/Transparency/TransparencyUpdateActivity"></owl:hasValue>
            </owl:Restriction>
        </owl:equivalentClass>
        <rdfs:subClassOf rdf:resource="https://w3id.org/italia/onto/Transparency/TransparencyActivity"></rdfs:subClassOf>
    </owl:Class>
    


    <!-- https://w3id.org/italia/onto/Transparency/UpdateFrequency -->

    <owl:Class rdf:about="https://w3id.org/italia/onto/Transparency/UpdateFrequency">
        <rdfs:subClassOf rdf:resource="https://w3id.org/italia/onto/l0/Characteristic"></rdfs:subClassOf>
        <rdfs:comment xml:lang="it">Questa classe la frequenza di aggiornamento di una risorsa così come indicato dall'obbligo ti trasaprenza.</rdfs:comment>
        <rdfs:comment xml:lang="en">This class represents the update frequency as prescribed by the transparency obbligation.</rdfs:comment>
        <rdfs:isDefinedBy rdf:resource="https://w3id.org/italia/onto/Transparency"></rdfs:isDefinedBy>
        <rdfs:label xml:lang="it">Frequenza di aggiornamento</rdfs:label>
        <rdfs:label xml:lang="en">Update frequency</rdfs:label>
        <owl:versionInfo xml:lang="it">stabile</owl:versionInfo>
        <owl:versionInfo xml:lang="en">stable</owl:versionInfo>
    </owl:Class>
    


    <!-- https://w3id.org/italia/onto/l0/Activity -->

    <owl:Class rdf:about="https://w3id.org/italia/onto/l0/Activity"></owl:Class>
    


    <!-- https://w3id.org/italia/onto/l0/Concept -->

    <owl:Class rdf:about="https://w3id.org/italia/onto/l0/Concept"></owl:Class>
    


    <!-- 
    ///////////////////////////////////////////////////////////////////////////////////////
    //
    // Individuals
    //
    ///////////////////////////////////////////////////////////////////////////////////////
     -->

    


    <!-- http://spcdata.digitpa.gov.it/Amministrazione/agid -->

    <owl:NamedIndividual rdf:about="http://spcdata.digitpa.gov.it/Amministrazione/agid">
        <rdf:type rdf:resource="http://dati.gov.it/onto/dcatapit#Agent"></rdf:type>
        <rdf:type rdf:resource="http://xmlns.com/foaf/0.1/Agent"></rdf:type>
        <dct:identifier>agid</dct:identifier>
        <foaf:name xml:lang="it">Agenzia per l'Italia Digitale</foaf:name>
        <foaf:name xml:lang="en">Italian Digital Agency</foaf:name>
    </owl:NamedIndividual>
    


    <!-- https://w3id.org/italia/data/distribution/TRAPIT-JSON-LD -->

    <owl:NamedIndividual rdf:about="https://w3id.org/italia/data/distribution/TRAPIT-JSON-LD">
        <rdf:type rdf:resource="https://w3id.org/italia/onto/ADMS/SemanticAssetDistribution"></rdf:type>
        <dct:description xml:lang="it">Questa è la distribuzione JSON-LD dell'Ontologia degli Obblighi della Trasparenza</dct:description>
        <dct:description xml:lang="en">This is the distribution in JSON-LD of the Transparency Obligations Ontology</dct:description>
        <dct:format rdf:resource="http://publications.europa.eu/resource/authority/file-type/JSON_LD"></dct:format>
        <dct:license rdf:resource="https://w3id.org/italia/controlled-vocabulary/licences/A21_CCBY40"></dct:license>
        <dct:title xml:lang="it">Distribuzione JSON-LD ontologia Transparency-AP_IT</dct:title>
        <dct:title xml:lang="en">JSON-LD distribution of Transparency-AP_IT Ontology</dct:title>
        <dcat:accessURL rdf:resource="https://raw.githubusercontent.com/italia/daf-ontologie-vocabolari-controllati/master/Ontologie/Transparency/latest"></dcat:accessURL>
        <dcat:downloadURL rdf:resource="https://raw.githubusercontent.com/italia/daf-ontologie-vocabolari-controllati/master/Ontologie/Transparency/Transparency-AP_IT.jsonld"></dcat:downloadURL>
    </owl:NamedIndividual>
    


    <!-- https://w3id.org/italia/data/distribution/TRAPIT-RDF-TURTLE -->

    <owl:NamedIndividual rdf:about="https://w3id.org/italia/data/distribution/TRAPIT-RDF-TURTLE">
        <rdf:type rdf:resource="https://w3id.org/italia/onto/ADMS/SemanticAssetDistribution"></rdf:type>
        <dct:description xml:lang="it">Questa è la distribuzione RDF/Turtle dell'Ontologia degli Obblighi della Trasparenza</dct:description>
        <dct:description xml:lang="en">This is the distribution in RDF/Turtle of the Transparency Obligations Ontology</dct:description>
        <dct:format rdf:resource="http://publications.europa.eu/resource/authority/file-type/RDF_TURTLE"></dct:format>
        <dct:license rdf:resource="https://w3id.org/italia/controlled-vocabulary/licences/A21_CCBY40"></dct:license>
        <dct:title xml:lang="it">Distribuzione RDF/Turtle ontologia Transparency-AP_IT</dct:title>
        <dct:title xml:lang="en">RDF/Turtle distribution of Transparency-AP_IT Ontology</dct:title>
        <dcat:accessURL rdf:resource="https://raw.githubusercontent.com/italia/daf-ontologie-vocabolari-controllati/master/Ontologie/Transparency/latest"></dcat:accessURL>
        <dcat:downloadURL rdf:resource="https://raw.githubusercontent.com/italia/daf-ontologie-vocabolari-controllati/master/Ontologie/Transparency/Transparency-AP_IT.ttl"></dcat:downloadURL>
    </owl:NamedIndividual>
    


    <!-- https://w3id.org/italia/data/distribution/TRAPIT-RDF-XML -->

    <owl:NamedIndividual rdf:about="https://w3id.org/italia/data/distribution/TRAPIT-RDF-XML">
        <rdf:type rdf:resource="https://w3id.org/italia/onto/ADMS/SemanticAssetDistribution"></rdf:type>
        <dct:description xml:lang="it">Questa è la distribuzione RDF/XML dell'Ontologia degli Obblighi della Trasparenza</dct:description>
        <dct:description xml:lang="en">This is the distribution in RDF/XML of the Transparency Obligations Ontology</dct:description>
        <dct:format rdf:resource="http://publications.europa.eu/resource/authority/file-type/RDF_XML"></dct:format>
        <dct:license rdf:resource="https://w3id.org/italia/controlled-vocabulary/licences/A21_CCBY40"></dct:license>
        <dct:title xml:lang="it">Distribuzione RDF/XML ontologia Transparency-AP_IT</dct:title>
        <dct:title xml:lang="en">RDF/XML distribution of Transparency-AP_IT Ontology</dct:title>
        <dcat:accessURL rdf:resource="https://raw.githubusercontent.com/italia/daf-ontologie-vocabolari-controllati/master/Ontologie/Transparency/latest"></dcat:accessURL>
        <dcat:downloadURL rdf:resource="https://raw.githubusercontent.com/italia/daf-ontologie-vocabolari-controllati/master/Ontologie/Transparency/Transparency-AP_IT.rdf"></dcat:downloadURL>
    </owl:NamedIndividual>
    


    <!-- https://w3id.org/italia/data/organization/private-organization/05481840964 -->

    <owl:NamedIndividual rdf:about="https://w3id.org/italia/data/organization/private-organization/05481840964">
        <rdf:type rdf:resource="http://dati.gov.it/onto/dcatapit#Agent"></rdf:type>
        <rdf:type rdf:resource="http://xmlns.com/foaf/0.1/Agent"></rdf:type>
        <dct:identifier>05481840964</dct:identifier>
        <foaf:name xml:lang="it">Almawave Srl</foaf:name>
    </owl:NamedIndividual>
    


    <!-- https://w3id.org/italia/onto/Transparency -->

    <owl:NamedIndividual rdf:about="https://w3id.org/italia/onto/Transparency">
        <rdf:type rdf:resource="https://w3id.org/italia/onto/ADMS/SemanticAsset"></rdf:type>
    </owl:NamedIndividual>
    


    <!-- https://w3id.org/italia/onto/Transparency/Deprecated -->

    <owl:NamedIndividual rdf:about="https://w3id.org/italia/onto/Transparency/Deprecated">
        <rdf:type rdf:resource="https://w3id.org/italia/onto/Transparency/TransparencyObligationStatus"></rdf:type>
        <l0:description xml:lang="it">Questo individuo rappresenta lo stato decaduto di un obbligo di trasparenza</l0:description>
        <l0:description xml:lang="en">This individual represents the status deprecated of a transparency obbligation</l0:description>
        <rdfs:isDefinedBy rdf:resource="https://w3id.org/italia/onto/Transparency"></rdfs:isDefinedBy>
        <rdfs:label xml:lang="it">decaduto</rdfs:label>
        <rdfs:label xml:lang="en">deprecated</rdfs:label>
        <owl:versionInfo xml:lang="it">stabile</owl:versionInfo>
        <owl:versionInfo xml:lang="en">stable</owl:versionInfo>
    </owl:NamedIndividual>
    


    <!-- https://w3id.org/italia/onto/Transparency/InForce -->

    <owl:NamedIndividual rdf:about="https://w3id.org/italia/onto/Transparency/InForce">
        <rdf:type rdf:resource="https://w3id.org/italia/onto/Transparency/TransparencyObligationStatus"></rdf:type>
        <l0:description xml:lang="it">Questo individuo rappresenta lo stato vigente di un obbligo di trasparenza</l0:description>
        <l0:description xml:lang="en">This individual represents the status in force of a transparency obbligation</l0:description>
        <rdfs:isDefinedBy rdf:resource="https://w3id.org/italia/onto/Transparency"></rdfs:isDefinedBy>
        <rdfs:label xml:lang="en">in force</rdfs:label>
        <rdfs:label xml:lang="it">vigente</rdfs:label>
        <owl:versionInfo xml:lang="it">stabile</owl:versionInfo>
        <owl:versionInfo xml:lang="en">stable</owl:versionInfo>
    </owl:NamedIndividual>
    


    <!-- https://w3id.org/italia/onto/Transparency/TransparencyArchiveActivity -->

    <owl:NamedIndividual rdf:about="https://w3id.org/italia/onto/Transparency/TransparencyArchiveActivity">
        <rdf:type rdf:resource="https://w3id.org/italia/onto/Transparency/TransparencyActivityTypology"></rdf:type>
        <l0:description xml:lang="it">Questo individuo rappresenta l'attività di storicizzazione attivata da un obbligo di trasparenza.</l0:description>
        <l0:description xml:lang="en">This individual represents the archive activity triggered by a transparency obligation.</l0:description>
    </owl:NamedIndividual>
    


    <!-- https://w3id.org/italia/onto/Transparency/TransparencyPublicationActivity -->

    <owl:NamedIndividual rdf:about="https://w3id.org/italia/onto/Transparency/TransparencyPublicationActivity">
        <rdf:type rdf:resource="https://w3id.org/italia/onto/Transparency/TransparencyActivityTypology"></rdf:type>
        <l0:description xml:lang="it">Questo individuo rappresenta l'attività di pubblicazione attivata da un obbligo di trasparenza.</l0:description>
        <l0:description xml:lang="en">This individual represents the publication activity triggered by a transparency obligation.</l0:description>
    </owl:NamedIndividual>
    


    <!-- https://w3id.org/italia/onto/Transparency/TransparencyUpdateActivity -->

    <owl:NamedIndividual rdf:about="https://w3id.org/italia/onto/Transparency/TransparencyUpdateActivity">
        <rdf:type rdf:resource="https://w3id.org/italia/onto/Transparency/TransparencyActivityTypology"></rdf:type>
        <l0:description xml:lang="it">Questo individuo rappresenta l'attività di aggiornamento attivata da un obbligo di trasparenza.</l0:description>
        <l0:description xml:lang="en">This individual represents the update activity triggered by a transparency obligation.</l0:description>
    </owl:NamedIndividual>
    


    <!-- 
    ///////////////////////////////////////////////////////////////////////////////////////
    //
    // Annotations
    //
    ///////////////////////////////////////////////////////////////////////////////////////
     -->

    <rdf:Description rdf:about="https://w3id.org/italia/onto/Transparency/TransparencyArchiveActivity">
        <rdfs:comment xml:lang="en">This class represents an archive activity as an effect of a transparency obbligation.</rdfs:comment>
        <rdfs:isDefinedBy rdf:resource="https://w3id.org/italia/onto/Transparency"></rdfs:isDefinedBy>
        <rdfs:label xml:lang="it">storicizzazione</rdfs:label>
        <owl:versionInfo xml:lang="it">stabile</owl:versionInfo>
        <owl:versionInfo xml:lang="en">stable</owl:versionInfo>
        <rdfs:comment xml:lang="it">Questa classe rappresenta un'attività di storicizzazione come conseguenza di un obbligo di trasparenza.</rdfs:comment>
        <rdfs:label xml:lang="it">archive</rdfs:label>
        <rdfs:label xml:lang="it">Attività di trasparenza: Storicizzazione.</rdfs:label>
        <rdfs:label xml:lang="en">Transparency activity: Archive.</rdfs:label>
    </rdf:Description>
    <rdf:Description rdf:about="https://w3id.org/italia/onto/Transparency/TransparencyPublicationActivity">
        <rdfs:comment xml:lang="it">Questa classe rappresenta un'attività di pubblicazione come conseguenza di un obbligo di trasparenza.</rdfs:comment>
        <owl:versionInfo xml:lang="it">stabile</owl:versionInfo>
        <rdfs:isDefinedBy rdf:resource="https://w3id.org/italia/onto/Transparency"></rdfs:isDefinedBy>
        <rdfs:label xml:lang="it">publication</rdfs:label>
        <rdfs:label xml:lang="it">Attività di trasparenza: Pubblicazione.</rdfs:label>
        <owl:versionInfo xml:lang="en">stable</owl:versionInfo>
        <rdfs:label xml:lang="en">Transparency activity: Publication.</rdfs:label>
        <rdfs:label xml:lang="en">Transparency activity: Publication</rdfs:label>
        <rdfs:comment xml:lang="en">This class represents a publication activity as an effect of a transparency obbligation.</rdfs:comment>
        <rdfs:label xml:lang="it">pubblicazione</rdfs:label>
    </rdf:Description>
    <rdf:Description rdf:about="https://w3id.org/italia/onto/Transparency/TransparencyUpdateActivity">
        <rdfs:isDefinedBy rdf:resource="https://w3id.org/italia/onto/Transparency"></rdfs:isDefinedBy>
        <owl:versionInfo xml:lang="en">stable</owl:versionInfo>
        <rdfs:label xml:lang="it">aggiornamento</rdfs:label>
        <rdfs:label xml:lang="it">Attività di trasparenza: Aggiornamento.</rdfs:label>
        <rdfs:label xml:lang="en">Transparency activity: Update.</rdfs:label>
        <rdfs:label xml:lang="it">update</rdfs:label>
        <rdfs:comment xml:lang="it">Questa classe rappresenta un'attività di aggiornamento come conseguenza di un obbligo di trasparenza.</rdfs:comment>
        <owl:versionInfo xml:lang="it">stabile</owl:versionInfo>
        <rdfs:comment xml:lang="en">This class represents an update activity as an effect of a transparency obbligation.</rdfs:comment>
    </rdf:Description>
</rdf:RDF>
<!-- Generated by the OWL API (version 4.5.9.2019-02-01T07:24:44Z) https://github.com/owlcs/owlapi -->