<rdf:RDF xmlns="https://w3id.org/italia/onto/CPV/" xmlns:CLV="https://w3id.org/italia/onto/CLV/" xmlns:admsapit="https://w3id.org/italia/onto/ADMS/" xmlns:dcat="http://www.w3.org/ns/dcat#" xmlns:dct="http://purl.org/dc/terms/" xmlns:foaf="http://xmlns.com/foaf/0.1/" xmlns:l0="https://w3id.org/italia/onto/l0/" xmlns:owl="http://www.w3.org/2002/07/owl#" xmlns:prov="http://www.w3.org/ns/prov#" xmlns:rdf="http://www.w3.org/1999/02/22-rdf-syntax-ns#" xmlns:rdfs="http://www.w3.org/2000/01/rdf-schema#" xmlns:vcard="http://www.w3.org/2006/vcard/ns#" xmlns:xsd="http://www.w3.org/2001/XMLSchema#" xml:base="https://w3id.org/italia/onto/CPV/">
    <owl:Ontology rdf:about="https://w3id.org/italia/onto/CPV">
        <owl:versionIRI rdf:resource="https://w3id.org/italia/onto/CPV/0.7"></owl:versionIRI>
        <owl:imports rdf:resource="https://w3id.org/italia/onto/CLV"></owl:imports>
        <owl:imports rdf:resource="https://w3id.org/italia/onto/TI"></owl:imports>
        <owl:imports rdf:resource="https://w3id.org/italia/onto/l0"></owl:imports>
        <dct:accrualPeriodicity rdf:resource="http://publications.europa.eu/resource/authority/frequency/IRREG"></dct:accrualPeriodicity>
        <dct:creator rdf:resource="http://spcdata.digitpa.gov.it/browse/page/Amministrazione/ISTAT"></dct:creator>
        <dct:creator rdf:resource="http://spcdata.digitpa.gov.it/browse/page/Amministrazione/agid"></dct:creator>
        <dct:description xml:lang="it">Questa è l'ontologia del profilo applicativo italiano sulle persone.</dct:description>
        <dct:description xml:lang="en">This is the ontology of the Italian application profile for Persons</dct:description>
        <dct:identifier>https://w3id.org/italia/onto/CPV</dct:identifier>
        <dct:issued rdf:datatype="http://www.w3.org/2001/XMLSchema#date">2017-07-19</dct:issued>
        <dct:language rdf:resource="http://publications.europa.eu/resource/authority/language/ENG"></dct:language>
        <dct:language rdf:resource="http://publications.europa.eu/resource/authority/language/ITA"></dct:language>
        <dct:modified rdf:datatype="http://www.w3.org/2001/XMLSchema#date">2020-04-27</dct:modified>
        <dct:publisher rdf:resource="http://spcdata.digitpa.gov.it/browse/page/Amministrazione/agid"></dct:publisher>
        <dct:rightsHolder rdf:resource="http://spcdata.digitpa.gov.it/browse/page/Amministrazione/ISTAT"></dct:rightsHolder>
        <dct:title xml:lang="en">CPV-AP_IT - Core Person Vocabulary Italian Application Profile - Person Ontology</dct:title>
        <dct:title xml:lang="it">CPV-AP_IT: Core Person Vocabulary - profilo applicativo italiano - Ontologia delle persone</dct:title>
        <rdfs:comment xml:lang="it">Questa è l'ontologia del profilo applicativo italiano sulle persone.</rdfs:comment>
        <rdfs:comment xml:lang="en">This is the ontology of the Italian application profile for Persons</rdfs:comment>
        <rdfs:isDefinedBy rdf:resource="https://w3id.org/italia/onto/CPV"></rdfs:isDefinedBy>
        <rdfs:label xml:lang="it">Ontologia delle persone (individui)</rdfs:label>
        <rdfs:label xml:lang="en">Person ontology</rdfs:label>
        <owl:versionInfo xml:lang="en">Version 0.7 - updated on 27th April 2020 - fixed a few typo in the lang it for two classes 'Education Level' and 'Family' and in a word fogio instead of foglio; updated on 17th of July - deleted subclassOf ParentalRelationship for FamilySheetHolder and added the reference to the controlled vocabulary for ParentalRelationshipType. Renamed ParentalRelationship in ParentalRelationshipType</owl:versionInfo>
        <owl:versionInfo xml:lang="it">Versione 0.7 - aggiornata il 27 Aprile 2020 - corretti due typo sulla lingua it per due classi 'Grado di Istruzione' e a'Famiglia' e nella parola 'fogio'; aggiornata il 17 Luglio 2019 - tolto il riferimento di sotto classe di Relazione Parentale per l'Intestatario di foglio di famiglia. Aggiunto il riferimento al vocabolario controllato relativo per il concetto di ParentalRelationshipType ( Tipo Relazione Parentale). Rinominata classe ParentalRelationship in ParentalRelationshipType</owl:versionInfo>
        <dcat:contactPoint rdf:resource="https://w3id.org/italia/data/contact-point/onto-agid"></dcat:contactPoint>
        <dcat:keyword xml:lang="it">famiglia</dcat:keyword>
        <dcat:keyword xml:lang="it">persona</dcat:keyword>
        <dcat:keyword xml:lang="it">persone</dcat:keyword>
        <dcat:keyword xml:lang="it">residenza</dcat:keyword>
        <dcat:theme rdf:resource="http://publications.europa.eu/resource/authority/data-theme/SOCI"></dcat:theme>
        <prov:wasDerivedFrom rdf:resource="https://w3id.org/italia/onto/CPV/0.6"></prov:wasDerivedFrom>
        <admsapit:acronym>CPV-AP_IT</admsapit:acronym>
        <admsapit:hasContributor rdf:resource="https://w3id.org/italia/data/organization/support-unit/cnr-Z6HZEH/stlab"></admsapit:hasContributor>
        <admsapit:hasFormalityLevel rdf:resource="https://w3id.org/italia/onto/ADMS/Formal"></admsapit:hasFormalityLevel>
        <admsapit:hasKeyClass rdf:resource="https://w3id.org/italia/onto/CPV/Person"></admsapit:hasKeyClass>
        <admsapit:hasKeyClass rdf:resource="https://w3id.org/italia/onto/CPV/RegisteredFamily"></admsapit:hasKeyClass>
        <admsapit:hasKeyClass rdf:resource="https://w3id.org/italia/onto/CPV/ResidenceInTime"></admsapit:hasKeyClass>
        <admsapit:hasOntologyLanguage rdf:resource="https://w3id.org/italia/onto/ADMS/OWL"></admsapit:hasOntologyLanguage>
        <admsapit:hasSemanticAssetDistribution rdf:resource="https://w3id.org/italia/data/distribution/CPVAPIT-JSON-LD"></admsapit:hasSemanticAssetDistribution>
        <admsapit:hasSemanticAssetDistribution rdf:resource="https://w3id.org/italia/data/distribution/CPVAPIT-RDF-TURTLE"></admsapit:hasSemanticAssetDistribution>
        <admsapit:hasSemanticAssetDistribution rdf:resource="https://w3id.org/italia/data/distribution/CPVAPIT-RDF-XML"></admsapit:hasSemanticAssetDistribution>
        <admsapit:hasTask rdf:resource="https://w3id.org/italia/onto/ADMS/AnnotationTask"></admsapit:hasTask>
        <admsapit:hasTask rdf:resource="https://w3id.org/italia/onto/ADMS/QueryFormulationTask"></admsapit:hasTask>
        <admsapit:last rdf:resource="https://w3id.org/italia/onto/CPV/0.7"></admsapit:last>
        <admsapit:officialURI rdf:datatype="http://www.w3.org/2001/XMLSchema#anyURI">https://w3id.org/italia/onto/CPV</admsapit:officialURI>
        <admsapit:prefix>cpvapit</admsapit:prefix>
        <admsapit:prev rdf:resource="https://w3id.org/italia/onto/CPV/0.6"></admsapit:prev>
        <admsapit:semanticAssetInUse rdf:resource="https://w3id.org/italia/data/project/DAF"></admsapit:semanticAssetInUse>
        <admsapit:semanticAssetInUse rdf:resource="https://w3id.org/italia/data/project/OntoPiA"></admsapit:semanticAssetInUse>
        <admsapit:status>catalogued</admsapit:status>
        <admsapit:status>published</admsapit:status>
        <admsapit:target>Imprese</admsapit:target>
        <admsapit:target>Pubbliche Amministrazioni</admsapit:target>
        <admsapit:type rdf:resource="https://w3id.org/italia/onto/ADMS/CoreOntology"></admsapit:type>
    </owl:Ontology>



    <!--
    ///////////////////////////////////////////////////////////////////////////////////////
    //
    // Annotation properties
    //
    ///////////////////////////////////////////////////////////////////////////////////////
     -->




    <!-- http://purl.org/dc/terms/description -->

    <owl:AnnotationProperty rdf:about="http://purl.org/dc/terms/description"></owl:AnnotationProperty>



    <!-- http://purl.org/dc/terms/format -->

    <owl:AnnotationProperty rdf:about="http://purl.org/dc/terms/format"></owl:AnnotationProperty>



    <!-- http://purl.org/dc/terms/identifier -->

    <owl:AnnotationProperty rdf:about="http://purl.org/dc/terms/identifier"></owl:AnnotationProperty>



    <!-- http://purl.org/dc/terms/license -->

    <owl:AnnotationProperty rdf:about="http://purl.org/dc/terms/license"></owl:AnnotationProperty>



    <!-- http://purl.org/dc/terms/title -->

    <owl:AnnotationProperty rdf:about="http://purl.org/dc/terms/title"></owl:AnnotationProperty>



    <!-- http://www.w3.org/2006/vcard/ns#fn -->

    <owl:AnnotationProperty rdf:about="http://www.w3.org/2006/vcard/ns#fn"></owl:AnnotationProperty>



    <!-- http://www.w3.org/2006/vcard/ns#hasEmail -->

    <owl:AnnotationProperty rdf:about="http://www.w3.org/2006/vcard/ns#hasEmail"></owl:AnnotationProperty>



    <!-- http://www.w3.org/ns/dcat#accessURL -->

    <owl:AnnotationProperty rdf:about="http://www.w3.org/ns/dcat#accessURL"></owl:AnnotationProperty>



    <!-- http://www.w3.org/ns/dcat#downloadURL -->

    <owl:AnnotationProperty rdf:about="http://www.w3.org/ns/dcat#downloadURL"></owl:AnnotationProperty>



    <!-- http://xmlns.com/foaf/0.1/name -->

    <owl:AnnotationProperty rdf:about="http://xmlns.com/foaf/0.1/name"></owl:AnnotationProperty>



    <!-- https://w3id.org/italia/onto/l0/controlledVocabulary -->

    <owl:AnnotationProperty rdf:about="https://w3id.org/italia/onto/l0/controlledVocabulary"></owl:AnnotationProperty>



    <!--
    ///////////////////////////////////////////////////////////////////////////////////////
    //
    // Datatypes
    //
    ///////////////////////////////////////////////////////////////////////////////////////
     -->




    <!-- http://www.w3.org/2001/XMLSchema#date -->

    <rdfs:Datatype rdf:about="http://www.w3.org/2001/XMLSchema#date"></rdfs:Datatype>



    <!--
    ///////////////////////////////////////////////////////////////////////////////////////
    //
    // Object Properties
    //
    ///////////////////////////////////////////////////////////////////////////////////////
     -->




    <!-- https://w3id.org/italia/onto/CLV/hasAddress -->

    <owl:ObjectProperty rdf:about="https://w3id.org/italia/onto/CLV/hasAddress"></owl:ObjectProperty>



    <!-- https://w3id.org/italia/onto/CPV/belongsToFamily -->

    <owl:ObjectProperty rdf:about="https://w3id.org/italia/onto/CPV/belongsToFamily">
        <rdfs:domain rdf:resource="https://w3id.org/italia/onto/CPV/Resident"></rdfs:domain>
        <rdfs:range rdf:resource="https://w3id.org/italia/onto/CPV/Family"></rdfs:range>
        <rdfs:comment xml:lang="it">La relazione che lega una persona residente in un paese a una famiglia</rdfs:comment>
        <rdfs:comment xml:lang="en">The relationship that links a person who is resident in a country to a family</rdfs:comment>
        <rdfs:isDefinedBy rdf:resource="https://w3id.org/italia/onto/CPV"></rdfs:isDefinedBy>
        <rdfs:label xml:lang="it">appartiene a famiglia</rdfs:label>
        <rdfs:label xml:lang="en">belongs to family</rdfs:label>
        <owl:versionInfo xml:lang="it">provvisoria</owl:versionInfo>
        <owl:versionInfo xml:lang="en">unstable</owl:versionInfo>
    </owl:ObjectProperty>



    <!-- https://w3id.org/italia/onto/CPV/hasBirthPlace -->

    <owl:ObjectProperty rdf:about="https://w3id.org/italia/onto/CPV/hasBirthPlace">
        <owl:inverseOf rdf:resource="https://w3id.org/italia/onto/CPV/isBirthPlaceOf"></owl:inverseOf>
        <rdfs:domain rdf:resource="https://w3id.org/italia/onto/CPV/Person"></rdfs:domain>
        <rdfs:range rdf:resource="https://w3id.org/italia/onto/l0/Location"></rdfs:range>
        <rdfs:comment xml:lang="it">La relazione che permette di asserire che una persona è nata in un certo luogo.</rdfs:comment>
        <rdfs:comment xml:lang="en">The relation asserts that a person has a certain place of birth.</rdfs:comment>
        <rdfs:isDefinedBy rdf:resource="https://w3id.org/italia/onto/CPV"></rdfs:isDefinedBy>
        <rdfs:label xml:lang="en">birth place</rdfs:label>
        <rdfs:label xml:lang="it">luogo di nascita</rdfs:label>
        <owl:versionInfo xml:lang="it">stabile</owl:versionInfo>
        <owl:versionInfo xml:lang="en">stable</owl:versionInfo>
    </owl:ObjectProperty>



    <!-- https://w3id.org/italia/onto/CPV/hasCitizenship -->

    <owl:ObjectProperty rdf:about="https://w3id.org/italia/onto/CPV/hasCitizenship">
        <rdfs:domain rdf:resource="https://w3id.org/italia/onto/CPV/Person"></rdfs:domain>
        <rdfs:range rdf:resource="https://w3id.org/italia/onto/l0/Location"></rdfs:range>
        <rdfs:comment xml:lang="it">La relazione che lega una persona alla sua cittadinanza (ex. cittadinanza italiana).</rdfs:comment>
        <rdfs:comment xml:lang="en">The relation that links a person to its citizenship (e.g. Italian)</rdfs:comment>
        <rdfs:isDefinedBy rdf:resource="https://w3id.org/italia/onto/CPV"></rdfs:isDefinedBy>
        <rdfs:label xml:lang="en">citizenship</rdfs:label>
        <rdfs:label xml:lang="it">ha cittadinanza</rdfs:label>
        <owl:versionInfo xml:lang="it">stabile</owl:versionInfo>
        <owl:versionInfo xml:lang="en">stable</owl:versionInfo>
    </owl:ObjectProperty>



    <!-- https://w3id.org/italia/onto/CPV/hasCurrentResidence -->

    <owl:ObjectProperty rdf:about="https://w3id.org/italia/onto/CPV/hasCurrentResidence">
        <owl:inverseOf rdf:resource="https://w3id.org/italia/onto/CPV/isCurrentResidenceOf"></owl:inverseOf>
        <rdfs:domain rdf:resource="https://w3id.org/italia/onto/CPV/Resident"></rdfs:domain>
        <rdfs:range rdf:resource="https://w3id.org/italia/onto/CLV/Address"></rdfs:range>
        <rdfs:comment xml:lang="it">Relazione che lega una persona residente in un paese al proprio luogo di residenza Rappresenta la residenza corrente della persona</rdfs:comment>
        <rdfs:comment xml:lang="en">The relation that links a person who is resident in a country to his/her location of residence. It is the current residence of the person.</rdfs:comment>
        <rdfs:isDefinedBy rdf:resource="https://w3id.org/italia/onto/CPV"></rdfs:isDefinedBy>
        <rdfs:label xml:lang="it">ha residenza attuale</rdfs:label>
        <rdfs:label xml:lang="en">has current residence</rdfs:label>
        <owl:versionInfo xml:lang="it">stabile</owl:versionInfo>
        <owl:versionInfo xml:lang="en">stable</owl:versionInfo>
    </owl:ObjectProperty>



    <!-- https://w3id.org/italia/onto/CPV/hasDeathPlace -->

    <owl:ObjectProperty rdf:about="https://w3id.org/italia/onto/CPV/hasDeathPlace">
        <owl:inverseOf rdf:resource="https://w3id.org/italia/onto/CPV/isDeathPlaceOf"></owl:inverseOf>
        <rdfs:domain rdf:resource="https://w3id.org/italia/onto/CPV/Dead"></rdfs:domain>
        <rdfs:range rdf:resource="https://w3id.org/italia/onto/l0/Location"></rdfs:range>
        <rdfs:comment xml:lang="it">La relazione che lega una persona morta al luogo di morte.</rdfs:comment>
        <rdfs:comment xml:lang="en">The relation that links a person who is dead to its place of death.</rdfs:comment>
        <rdfs:isDefinedBy rdf:resource="https://w3id.org/italia/onto/CPV"></rdfs:isDefinedBy>
        <rdfs:label xml:lang="en">death place</rdfs:label>
        <rdfs:label xml:lang="it">luogo di morte</rdfs:label>
        <owl:versionInfo xml:lang="it">stabile</owl:versionInfo>
        <owl:versionInfo xml:lang="en">unstable</owl:versionInfo>
    </owl:ObjectProperty>



    <!-- https://w3id.org/italia/onto/CPV/hasLevelOfEducation -->

    <owl:ObjectProperty rdf:about="https://w3id.org/italia/onto/CPV/hasLevelOfEducation">
        <rdfs:domain rdf:resource="https://w3id.org/italia/onto/CPV/Alive"></rdfs:domain>
        <rdfs:range rdf:resource="https://w3id.org/italia/onto/CPV/EducationLevel"></rdfs:range>
        <rdfs:comment xml:lang="it">La relazione che lega una persona in vita al suo grado di istruzione</rdfs:comment>
        <rdfs:comment xml:lang="en">The relation that links an alive person to his/her education level</rdfs:comment>
        <rdfs:isDefinedBy rdf:resource="https://w3id.org/italia/onto/CPV"></rdfs:isDefinedBy>
        <rdfs:label xml:lang="it">ha grado di istruzione</rdfs:label>
        <rdfs:label xml:lang="en">has level of education</rdfs:label>
        <owl:versionInfo xml:lang="it">stabile</owl:versionInfo>
        <owl:versionInfo xml:lang="en">stable</owl:versionInfo>
    </owl:ObjectProperty>



    <!-- https://w3id.org/italia/onto/CPV/hasParentalRelationshipWith -->

    <owl:ObjectProperty rdf:about="https://w3id.org/italia/onto/CPV/hasParentalRelationshipWith">
        <rdfs:subPropertyOf rdf:resource="https://w3id.org/italia/onto/CPV/hasRelationshipWith"></rdfs:subPropertyOf>
        <rdfs:domain rdf:resource="https://w3id.org/italia/onto/CPV/Person"></rdfs:domain>
        <rdfs:range rdf:resource="https://w3id.org/italia/onto/CPV/Person"></rdfs:range>
        <rdfs:comment xml:lang="en">A parental relationship between two persons.</rdfs:comment>
        <rdfs:comment xml:lang="it">Una relazione di parentela tra due persone.</rdfs:comment>
        <rdfs:isDefinedBy rdf:resource="https://w3id.org/italia/onto/CPV"></rdfs:isDefinedBy>
        <rdfs:label xml:lang="it">ha relazione parentale con</rdfs:label>
        <rdfs:label xml:lang="en">has parental relationship with</rdfs:label>
        <owl:versionInfo xml:lang="it">stabile</owl:versionInfo>
        <owl:versionInfo xml:lang="en">stable</owl:versionInfo>
    </owl:ObjectProperty>



    <!-- https://w3id.org/italia/onto/CPV/hasPersonTitle -->

    <owl:ObjectProperty rdf:about="https://w3id.org/italia/onto/CPV/hasPersonTitle">
        <rdfs:domain rdf:resource="https://w3id.org/italia/onto/CPV/Person"></rdfs:domain>
        <rdfs:range rdf:resource="https://w3id.org/italia/onto/CPV/PersonTitle"></rdfs:range>
        <rdfs:comment xml:lang="it">Connette una persona ad un suo titolo.</rdfs:comment>
        <rdfs:comment xml:lang="en">It links a person to his/her title.</rdfs:comment>
        <rdfs:isDefinedBy rdf:resource="https://w3id.org/italia/onto/CPV"></rdfs:isDefinedBy>
        <rdfs:label xml:lang="it">ha titolo</rdfs:label>
        <rdfs:label xml:lang="en">has title</rdfs:label>
        <admsapit:status xml:lang="it">instabile</admsapit:status>
        <admsapit:status xml:lang="en">unstable</admsapit:status>
    </owl:ObjectProperty>



    <!-- https://w3id.org/italia/onto/CPV/hasRelationshipWith -->

    <owl:ObjectProperty rdf:about="https://w3id.org/italia/onto/CPV/hasRelationshipWith">
        <rdfs:domain rdf:resource="https://w3id.org/italia/onto/CPV/Person"></rdfs:domain>
        <rdfs:range rdf:resource="https://w3id.org/italia/onto/CPV/Person"></rdfs:range>
        <rdfs:comment xml:lang="en">Any relationship between people.</rdfs:comment>
        <rdfs:comment xml:lang="it">Qualsiasi relazione tra persone.</rdfs:comment>
        <rdfs:isDefinedBy rdf:resource="https://w3id.org/italia/onto/CPV"></rdfs:isDefinedBy>
        <rdfs:label xml:lang="it">ha relazione con</rdfs:label>
        <rdfs:label xml:lang="en">has relationship with</rdfs:label>
        <owl:versionInfo xml:lang="it">stabile</owl:versionInfo>
        <owl:versionInfo xml:lang="en">stable</owl:versionInfo>
    </owl:ObjectProperty>



    <!-- https://w3id.org/italia/onto/CPV/hasResidenceInTime -->

    <owl:ObjectProperty rdf:about="https://w3id.org/italia/onto/CPV/hasResidenceInTime">
        <owl:inverseOf rdf:resource="https://w3id.org/italia/onto/CPV/isResidenceInTimeOf"></owl:inverseOf>
        <rdfs:domain rdf:resource="https://w3id.org/italia/onto/CPV/Person"></rdfs:domain>
        <rdfs:range rdf:resource="https://w3id.org/italia/onto/CPV/ResidenceInTime"></rdfs:range>
        <rdfs:comment xml:lang="en">Property that links a person to his/her residence in time</rdfs:comment>
        <rdfs:comment xml:lang="it">Proprietà che lega una persona allo storico della sua residenza (lega quindi la persona alla relazione ennaria residenza nel tempo)</rdfs:comment>
        <rdfs:isDefinedBy rdf:resource="https://w3id.org/italia/onto/CPV"></rdfs:isDefinedBy>
        <rdfs:label xml:lang="it">ha stato residenza (ha residenza nel tempo)</rdfs:label>
        <rdfs:label xml:lang="en">has residence in time</rdfs:label>
        <owl:versionInfo xml:lang="it">provvisoria</owl:versionInfo>
        <owl:versionInfo xml:lang="en">unstable</owl:versionInfo>
    </owl:ObjectProperty>



    <!-- https://w3id.org/italia/onto/CPV/hasSex -->

    <owl:ObjectProperty rdf:about="https://w3id.org/italia/onto/CPV/hasSex">
        <rdfs:domain rdf:resource="https://w3id.org/italia/onto/CPV/Person"></rdfs:domain>
        <rdfs:range rdf:resource="https://w3id.org/italia/onto/CPV/Sex"></rdfs:range>
        <rdfs:comment xml:lang="it">La relazione che lega una persona al suo sesso</rdfs:comment>
        <rdfs:comment xml:lang="en">The relation that links a person to his/her sex</rdfs:comment>
        <rdfs:isDefinedBy rdf:resource="https://w3id.org/italia/onto/CPV"></rdfs:isDefinedBy>
        <rdfs:label xml:lang="it">ha sesso</rdfs:label>
        <rdfs:label xml:lang="en">has sex</rdfs:label>
        <owl:versionInfo xml:lang="it">stabile</owl:versionInfo>
        <owl:versionInfo xml:lang="en">stable</owl:versionInfo>
    </owl:ObjectProperty>



    <!-- https://w3id.org/italia/onto/CPV/inRegisteredFamily -->

    <owl:ObjectProperty rdf:about="https://w3id.org/italia/onto/CPV/inRegisteredFamily">
        <rdfs:domain rdf:resource="https://w3id.org/italia/onto/CPV/ParentalRelationshipType"></rdfs:domain>
        <rdfs:range rdf:resource="https://w3id.org/italia/onto/CPV/RegisteredFamily"></rdfs:range>
        <rdfs:comment xml:lang="it">Relazione che lega un tipo di relazione parentale con la relativa famiglia anagrafica</rdfs:comment>
        <rdfs:comment xml:lang="en">The relation that links the different types of Parental Relationship to the related Registered Family</rdfs:comment>
        <rdfs:isDefinedBy rdf:resource="https://w3id.org/italia/onto/CPV"></rdfs:isDefinedBy>
        <rdfs:label xml:lang="it">in famiglia anagrafica</rdfs:label>
        <rdfs:label xml:lang="en">in registered family</rdfs:label>
        <owl:versionInfo xml:lang="it">stabile</owl:versionInfo>
        <owl:versionInfo xml:lang="en">stable</owl:versionInfo>
    </owl:ObjectProperty>



    <!-- https://w3id.org/italia/onto/CPV/isBirthPlaceOf -->

    <owl:ObjectProperty rdf:about="https://w3id.org/italia/onto/CPV/isBirthPlaceOf">
        <rdfs:domain rdf:resource="https://w3id.org/italia/onto/l0/Location"></rdfs:domain>
        <rdfs:range rdf:resource="https://w3id.org/italia/onto/CPV/Person"></rdfs:range>
        <rdfs:comment xml:lang="it">La relazione tra un luogo ed una persona dove il luogo è il luogo di nascit della persona oggetto della relazione.</rdfs:comment>
        <rdfs:comment xml:lang="en">The relation between a place and a person. The relation asserts that a place is the place of birth of the person object of the relation.</rdfs:comment>
        <rdfs:isDefinedBy rdf:resource="https://w3id.org/italia/onto/CPV"></rdfs:isDefinedBy>
        <rdfs:label xml:lang="en">is birth place of</rdfs:label>
        <rdfs:label xml:lang="it">è luogo di nascita di</rdfs:label>
        <owl:versionInfo xml:lang="it">stabile</owl:versionInfo>
        <owl:versionInfo xml:lang="en">stable</owl:versionInfo>
    </owl:ObjectProperty>



    <!-- https://w3id.org/italia/onto/CPV/isChildOf -->

    <owl:ObjectProperty rdf:about="https://w3id.org/italia/onto/CPV/isChildOf">
        <rdfs:subPropertyOf rdf:resource="https://w3id.org/italia/onto/CPV/hasParentalRelationshipWith"></rdfs:subPropertyOf>
        <owl:inverseOf rdf:resource="https://w3id.org/italia/onto/CPV/isParentOf"></owl:inverseOf>
        <rdfs:domain rdf:resource="https://w3id.org/italia/onto/CPV/Person"></rdfs:domain>
        <rdfs:range rdf:resource="https://w3id.org/italia/onto/CPV/Person"></rdfs:range>
    </owl:ObjectProperty>



    <!-- https://w3id.org/italia/onto/CPV/isConsortOf -->

    <owl:ObjectProperty rdf:about="https://w3id.org/italia/onto/CPV/isConsortOf">
        <rdfs:subPropertyOf rdf:resource="https://w3id.org/italia/onto/CPV/hasParentalRelationshipWith"></rdfs:subPropertyOf>
        <rdfs:domain rdf:resource="https://w3id.org/italia/onto/CPV/Person"></rdfs:domain>
        <rdfs:range rdf:resource="https://w3id.org/italia/onto/CPV/Person"></rdfs:range>
    </owl:ObjectProperty>



    <!-- https://w3id.org/italia/onto/CPV/isCurrentResidenceOf -->

    <owl:ObjectProperty rdf:about="https://w3id.org/italia/onto/CPV/isCurrentResidenceOf">
        <rdfs:domain rdf:resource="https://w3id.org/italia/onto/CLV/Address"></rdfs:domain>
        <rdfs:range rdf:resource="https://w3id.org/italia/onto/CPV/Resident"></rdfs:range>
        <rdfs:comment xml:lang="it">Relazione inversa che lega una persona residente in un paese al proprio luogo di residenza Rappresenta la residenza corrente della persona</rdfs:comment>
        <rdfs:comment xml:lang="en">The inverse relation that links a person who is resident in a country to his/her location of residence. It is the current residence of the person.</rdfs:comment>
        <rdfs:label xml:lang="en">is current residence of</rdfs:label>
        <rdfs:label xml:lang="it">è residenza attuale di</rdfs:label>
    </owl:ObjectProperty>



    <!-- https://w3id.org/italia/onto/CPV/isDeathPlaceOf -->

    <owl:ObjectProperty rdf:about="https://w3id.org/italia/onto/CPV/isDeathPlaceOf">
        <rdfs:domain rdf:resource="https://w3id.org/italia/onto/l0/Location"></rdfs:domain>
        <rdfs:range rdf:resource="https://w3id.org/italia/onto/CPV/Dead"></rdfs:range>
        <rdfs:comment xml:lang="it">La proprietà per associare un luogo di morte (i.e. una località) alla persona morta.</rdfs:comment>
        <rdfs:comment xml:lang="en">The property to link the death place (i.e. a location) to a person</rdfs:comment>
        <rdfs:isDefinedBy rdf:resource="https://w3id.org/italia/onto/CPV"></rdfs:isDefinedBy>
        <rdfs:label xml:lang="en">death place of</rdfs:label>
        <rdfs:label xml:lang="it">è luogo di morte di</rdfs:label>
        <owl:versionInfo xml:lang="it">stabile</owl:versionInfo>
        <owl:versionInfo xml:lang="en">stable</owl:versionInfo>
    </owl:ObjectProperty>



    <!-- https://w3id.org/italia/onto/CPV/isFamilySheetHolderOf -->

    <owl:ObjectProperty rdf:about="https://w3id.org/italia/onto/CPV/isFamilySheetHolderOf">
        <rdfs:subPropertyOf rdf:resource="https://w3id.org/italia/onto/CPV/hasParentalRelationshipWith"></rdfs:subPropertyOf>
        <rdfs:domain rdf:resource="https://w3id.org/italia/onto/CPV/FamilySheetHolder"></rdfs:domain>
        <rdfs:range rdf:resource="https://w3id.org/italia/onto/CPV/Person"></rdfs:range>
    </owl:ObjectProperty>



    <!-- https://w3id.org/italia/onto/CPV/isGrandChildOf -->

    <owl:ObjectProperty rdf:about="https://w3id.org/italia/onto/CPV/isGrandChildOf">
        <rdfs:subPropertyOf rdf:resource="https://w3id.org/italia/onto/CPV/hasParentalRelationshipWith"></rdfs:subPropertyOf>
        <owl:inverseOf rdf:resource="https://w3id.org/italia/onto/CPV/isGrandFatherOf"></owl:inverseOf>
        <rdfs:domain rdf:resource="https://w3id.org/italia/onto/CPV/Person"></rdfs:domain>
        <rdfs:range rdf:resource="https://w3id.org/italia/onto/CPV/Person"></rdfs:range>
    </owl:ObjectProperty>



    <!-- https://w3id.org/italia/onto/CPV/isGrandFatherOf -->

    <owl:ObjectProperty rdf:about="https://w3id.org/italia/onto/CPV/isGrandFatherOf">
        <rdfs:subPropertyOf rdf:resource="https://w3id.org/italia/onto/CPV/hasParentalRelationshipWith"></rdfs:subPropertyOf>
        <rdfs:domain rdf:resource="https://w3id.org/italia/onto/CPV/Person"></rdfs:domain>
        <rdfs:range rdf:resource="https://w3id.org/italia/onto/CPV/Person"></rdfs:range>
    </owl:ObjectProperty>



    <!-- https://w3id.org/italia/onto/CPV/isNephewOf -->

    <owl:ObjectProperty rdf:about="https://w3id.org/italia/onto/CPV/isNephewOf">
        <rdfs:subPropertyOf rdf:resource="https://w3id.org/italia/onto/CPV/hasParentalRelationshipWith"></rdfs:subPropertyOf>
        <owl:inverseOf rdf:resource="https://w3id.org/italia/onto/CPV/isUncleOf"></owl:inverseOf>
        <rdfs:domain rdf:resource="https://w3id.org/italia/onto/CPV/Person"></rdfs:domain>
        <rdfs:range rdf:resource="https://w3id.org/italia/onto/CPV/Person"></rdfs:range>
    </owl:ObjectProperty>



    <!-- https://w3id.org/italia/onto/CPV/isParentOf -->

    <owl:ObjectProperty rdf:about="https://w3id.org/italia/onto/CPV/isParentOf">
        <rdfs:subPropertyOf rdf:resource="https://w3id.org/italia/onto/CPV/hasParentalRelationshipWith"></rdfs:subPropertyOf>
        <rdfs:domain rdf:resource="https://w3id.org/italia/onto/CPV/Person"></rdfs:domain>
        <rdfs:range rdf:resource="https://w3id.org/italia/onto/CPV/Person"></rdfs:range>
    </owl:ObjectProperty>



    <!-- https://w3id.org/italia/onto/CPV/isResidenceInTimeOf -->

    <owl:ObjectProperty rdf:about="https://w3id.org/italia/onto/CPV/isResidenceInTimeOf">
        <rdfs:domain rdf:resource="https://w3id.org/italia/onto/CPV/ResidenceInTime"></rdfs:domain>
        <rdfs:range rdf:resource="https://w3id.org/italia/onto/CPV/Person"></rdfs:range>
        <rdfs:comment xml:lang="en">Inverse property of "has residence in time" which links residence in time with the person</rdfs:comment>
        <rdfs:comment xml:lang="it">Proprietà inversa di "ha residenza nel tempo (ha stato residenza)" che collega il concetto di residenza nel tempo con la persona.</rdfs:comment>
        <rdfs:isDefinedBy rdf:resource="https://w3id.org/italia/onto/CPV"></rdfs:isDefinedBy>
        <rdfs:label xml:lang="en">is residence in time of</rdfs:label>
        <rdfs:label xml:lang="it">è stato residenza di (è residenza nel tempo di)</rdfs:label>
        <owl:versionInfo xml:lang="it">provvisoria</owl:versionInfo>
        <owl:versionInfo xml:lang="en">unstable</owl:versionInfo>
    </owl:ObjectProperty>



    <!-- https://w3id.org/italia/onto/CPV/isResidenceOf -->

    <owl:ObjectProperty rdf:about="https://w3id.org/italia/onto/CPV/isResidenceOf">
        <owl:inverseOf rdf:resource="https://w3id.org/italia/onto/CPV/residentIn"></owl:inverseOf>
    </owl:ObjectProperty>



    <!-- https://w3id.org/italia/onto/CPV/isUncleOf -->

    <owl:ObjectProperty rdf:about="https://w3id.org/italia/onto/CPV/isUncleOf">
        <rdfs:subPropertyOf rdf:resource="https://w3id.org/italia/onto/CPV/hasParentalRelationshipWith"></rdfs:subPropertyOf>
        <rdfs:domain rdf:resource="https://w3id.org/italia/onto/CPV/Person"></rdfs:domain>
        <rdfs:range rdf:resource="https://w3id.org/italia/onto/CPV/Person"></rdfs:range>
    </owl:ObjectProperty>



    <!-- https://w3id.org/italia/onto/CPV/knows -->

    <owl:ObjectProperty rdf:about="https://w3id.org/italia/onto/CPV/knows">
        <rdfs:subPropertyOf rdf:resource="https://w3id.org/italia/onto/CPV/hasRelationshipWith"></rdfs:subPropertyOf>
        <rdf:type rdf:resource="http://www.w3.org/2002/07/owl#SymmetricProperty"></rdf:type>
        <rdfs:domain rdf:resource="https://w3id.org/italia/onto/CPV/Person"></rdfs:domain>
        <rdfs:range rdf:resource="https://w3id.org/italia/onto/CPV/Person"></rdfs:range>
        <rdfs:comment xml:lang="it">La relazione di conoscenza che intercorre tra due persone. Ex. 'Mario Rossi' conosce 'Paolo Neri'.</rdfs:comment>
        <rdfs:comment xml:lang="en">The relationship of knowledge between two people. E.g. 'John White' knows 'Bob Black'.</rdfs:comment>
        <rdfs:isDefinedBy rdf:resource="https://w3id.org/italia/onto/CPV"></rdfs:isDefinedBy>
        <rdfs:label xml:lang="it">conosce</rdfs:label>
        <rdfs:label xml:lang="en">knows</rdfs:label>
        <owl:versionInfo xml:lang="it">stabile</owl:versionInfo>
        <owl:versionInfo xml:lang="en">stable</owl:versionInfo>
    </owl:ObjectProperty>



    <!-- https://w3id.org/italia/onto/CPV/residenceInLocation -->

    <owl:ObjectProperty rdf:about="https://w3id.org/italia/onto/CPV/residenceInLocation">
        <rdfs:domain rdf:resource="https://w3id.org/italia/onto/CPV/ResidenceInTime"></rdfs:domain>
        <rdfs:range rdf:resource="https://w3id.org/italia/onto/l0/Location"></rdfs:range>
        <rdfs:comment xml:lang="en">Property that links the residence in time (the n-ray relationship) to the location of the residence.</rdfs:comment>
        <rdfs:comment xml:lang="it">Proprietà che lega la residenza nel tempo (lo storico della residenza attraverso la definizione della relazione ennaria) al luogo della residenza.</rdfs:comment>
        <rdfs:isDefinedBy rdf:resource="https://w3id.org/italia/onto/CPV"></rdfs:isDefinedBy>
        <rdfs:label xml:lang="en">residence in location</rdfs:label>
        <rdfs:label xml:lang="it">residenza in luogo</rdfs:label>
        <owl:versionInfo xml:lang="it">provvisoria</owl:versionInfo>
        <owl:versionInfo xml:lang="en">unstable</owl:versionInfo>
    </owl:ObjectProperty>



    <!-- https://w3id.org/italia/onto/CPV/residentIn -->

    <owl:ObjectProperty rdf:about="https://w3id.org/italia/onto/CPV/residentIn">
        <rdfs:domain rdf:resource="https://w3id.org/italia/onto/CPV/Person"></rdfs:domain>
        <rdfs:range rdf:resource="https://w3id.org/italia/onto/CLV/Address"></rdfs:range>
        <owl:propertyChainAxiom rdf:parseType="Collection">
            <rdf:Description rdf:about="https://w3id.org/italia/onto/CPV/hasResidenceInTime"></rdf:Description>
            <rdf:Description rdf:about="https://w3id.org/italia/onto/CPV/residenceInLocation"></rdf:Description>
        </owl:propertyChainAxiom>
        <rdfs:comment xml:lang="it">Questa proprietà rappresenta la residenza espressa come relazione binaria tra una persona ed un indirizzo.</rdfs:comment>
        <rdfs:comment xml:lang="en">This property represents the residence expressed as binary relation between a person and an address.</rdfs:comment>
        <rdfs:label xml:lang="en">resident in</rdfs:label>
        <rdfs:label xml:lang="it">residente in</rdfs:label>
    </owl:ObjectProperty>



    <!--
    ///////////////////////////////////////////////////////////////////////////////////////
    //
    // Data properties
    //
    ///////////////////////////////////////////////////////////////////////////////////////
     -->




    <!-- https://w3id.org/italia/onto/CPV/age -->

    <owl:DatatypeProperty rdf:about="https://w3id.org/italia/onto/CPV/age">
        <rdfs:domain rdf:resource="https://w3id.org/italia/onto/CPV/Alive"></rdfs:domain>
        <rdfs:range rdf:resource="http://www.w3.org/2001/XMLSchema#integer"></rdfs:range>
        <rdfs:comment xml:lang="it">L'età della persona naturale. Es: 64</rdfs:comment>
        <rdfs:comment xml:lang="en">The age of the natural person</rdfs:comment>
        <rdfs:isDefinedBy rdf:resource="https://w3id.org/italia/onto/CPV"></rdfs:isDefinedBy>
        <rdfs:label xml:lang="en">age</rdfs:label>
        <rdfs:label xml:lang="it">età</rdfs:label>
        <owl:versionInfo xml:lang="it">stabile</owl:versionInfo>
        <owl:versionInfo xml:lang="en">stable</owl:versionInfo>
    </owl:DatatypeProperty>



    <!-- https://w3id.org/italia/onto/CPV/ageWhenDead -->

    <owl:DatatypeProperty rdf:about="https://w3id.org/italia/onto/CPV/ageWhenDead">
        <rdfs:subPropertyOf rdf:resource="https://w3id.org/italia/onto/CPV/age"></rdfs:subPropertyOf>
        <rdfs:domain rdf:resource="https://w3id.org/italia/onto/CPV/Dead"></rdfs:domain>
        <rdfs:range rdf:resource="http://www.w3.org/2001/XMLSchema#integer"></rdfs:range>
        <rdfs:comment xml:lang="it">L'età della persona naturale rielvata al momento del decesso.</rdfs:comment>
        <rdfs:comment xml:lang="en">The age of the natural person observed at the time of death</rdfs:comment>
        <rdfs:isDefinedBy rdf:resource="https://w3id.org/italia/onto/CPV"></rdfs:isDefinedBy>
        <rdfs:label xml:lang="en">age when dead</rdfs:label>
        <rdfs:label xml:lang="it">età al decesso</rdfs:label>
        <owl:versionInfo xml:lang="it">stabile</owl:versionInfo>
        <owl:versionInfo xml:lang="en">stable</owl:versionInfo>
    </owl:DatatypeProperty>



    <!-- https://w3id.org/italia/onto/CPV/altName -->

    <owl:DatatypeProperty rdf:about="https://w3id.org/italia/onto/CPV/altName">
        <rdfs:subPropertyOf rdf:resource="https://w3id.org/italia/onto/l0/name"></rdfs:subPropertyOf>
        <rdfs:domain rdf:resource="https://w3id.org/italia/onto/CPV/Person"></rdfs:domain>
        <rdfs:range rdf:resource="http://www.w3.org/2001/XMLSchema#string"></rdfs:range>
        <rdfs:comment xml:lang="en">The alternative name or middle name of a person. E.g., Anne is the middle name of "Mary Anne Clark".</rdfs:comment>
        <rdfs:comment xml:lang="it">il nome alternativo o secondo nome di una persona. Per esempio Anne è il secondo nome di "Mary Anne Clarke".</rdfs:comment>
        <rdfs:isDefinedBy rdf:resource="https://w3id.org/italia/onto/CPV"></rdfs:isDefinedBy>
        <rdfs:label xml:lang="en">alternative name</rdfs:label>
        <rdfs:label xml:lang="it">nome alternativo (secondo nome)</rdfs:label>
        <owl:versionInfo xml:lang="it">provvisoria</owl:versionInfo>
        <owl:versionInfo xml:lang="en">unstable</owl:versionInfo>
    </owl:DatatypeProperty>



    <!-- https://w3id.org/italia/onto/CPV/dateOfBirth -->

    <owl:DatatypeProperty rdf:about="https://w3id.org/italia/onto/CPV/dateOfBirth">
        <rdf:type rdf:resource="http://www.w3.org/2002/07/owl#FunctionalProperty"></rdf:type>
        <rdfs:domain rdf:resource="https://w3id.org/italia/onto/CPV/Person"></rdfs:domain>
        <rdfs:range rdf:resource="http://www.w3.org/2001/XMLSchema#dateTime"></rdfs:range>
        <rdfs:comment xml:lang="it">La data di nascita della persona naturale</rdfs:comment>
        <rdfs:comment xml:lang="en">The date of birth of the natural person</rdfs:comment>
        <rdfs:isDefinedBy rdf:resource="https://w3id.org/italia/onto/CPV"></rdfs:isDefinedBy>
        <rdfs:label xml:lang="it">data di nascita</rdfs:label>
        <rdfs:label xml:lang="en">date of birth</rdfs:label>
        <owl:versionInfo xml:lang="it">stabile</owl:versionInfo>
        <owl:versionInfo xml:lang="en">stable</owl:versionInfo>
    </owl:DatatypeProperty>



    <!-- https://w3id.org/italia/onto/CPV/dateOfDeath -->

    <owl:DatatypeProperty rdf:about="https://w3id.org/italia/onto/CPV/dateOfDeath">
        <rdf:type rdf:resource="http://www.w3.org/2002/07/owl#FunctionalProperty"></rdf:type>
        <rdfs:domain rdf:resource="https://w3id.org/italia/onto/CPV/Dead"></rdfs:domain>
        <rdfs:range rdf:resource="http://www.w3.org/2001/XMLSchema#dateTime"></rdfs:range>
        <rdfs:comment xml:lang="it">La data di morte della persona naturale. Es: 2002-10-04</rdfs:comment>
        <rdfs:comment xml:lang="en">The date of birth of the natural person</rdfs:comment>
        <rdfs:isDefinedBy rdf:resource="https://w3id.org/italia/onto/CPV"></rdfs:isDefinedBy>
        <rdfs:label xml:lang="it">data di morte</rdfs:label>
        <rdfs:label xml:lang="en">date of death</rdfs:label>
        <owl:versionInfo xml:lang="it">stabile</owl:versionInfo>
        <owl:versionInfo xml:lang="en">stable</owl:versionInfo>
    </owl:DatatypeProperty>



    <!-- https://w3id.org/italia/onto/CPV/educationLevelDesc -->

    <owl:DatatypeProperty rdf:about="https://w3id.org/italia/onto/CPV/educationLevelDesc">
        <rdfs:subPropertyOf rdf:resource="https://w3id.org/italia/onto/l0/description"></rdfs:subPropertyOf>
        <rdfs:domain rdf:resource="https://w3id.org/italia/onto/CPV/EducationLevel"></rdfs:domain>
        <rdfs:range rdf:resource="http://www.w3.org/2000/01/rdf-schema#Literal"></rdfs:range>
        <rdfs:comment xml:lang="en">Property used to represent the education level as defined in the related controlled vocabulary EducationLevel https://w3id.org/italia/controlled-vocabulary/classifications-for-people/education-level</rdfs:comment>
        <rdfs:comment xml:lang="it">Proprietà utilizzata per rappresentare il grado di istruzione come definito nel relativo vocabolario controllato EducationLevel https://w3id.org/italia/controlled-vocabulary/classifications-for-people/education-level</rdfs:comment>
        <rdfs:isDefinedBy rdf:resource="https://w3id.org/italia/onto/CPV"></rdfs:isDefinedBy>
        <rdfs:label xml:lang="it">descrizione grado di istruzione</rdfs:label>
        <rdfs:label xml:lang="en">education level description</rdfs:label>
        <owl:versionInfo xml:lang="it">stabile</owl:versionInfo>
        <owl:versionInfo xml:lang="en">stable</owl:versionInfo>
        <l0:controlledVocabulary rdf:resource="https://w3id.org/italia/controlled-vocabulary/classifications-for-people/education-level"></l0:controlledVocabulary>
    </owl:DatatypeProperty>



    <!-- https://w3id.org/italia/onto/CPV/educationLevelID -->

    <owl:DatatypeProperty rdf:about="https://w3id.org/italia/onto/CPV/educationLevelID">
        <rdfs:subPropertyOf rdf:resource="https://w3id.org/italia/onto/l0/identifier"></rdfs:subPropertyOf>
        <rdf:type rdf:resource="http://www.w3.org/2002/07/owl#FunctionalProperty"></rdf:type>
        <rdfs:domain rdf:resource="https://w3id.org/italia/onto/CPV/EducationLevel"></rdfs:domain>
        <rdfs:range rdf:resource="http://www.w3.org/2000/01/rdf-schema#Literal"></rdfs:range>
        <rdfs:comment xml:lang="en">Unique code used to identify the education level in the controlled vocabulary EducationLevel https://w3id.org/italia/controlled-vocabulary/classifications-for-people/education-level</rdfs:comment>
        <rdfs:comment xml:lang="it">codice univoco che identifica il grado di istruzione nel vocabolario controllato EducationLevel https://w3id.org/italia/controlled-vocabulary/classifications-for-people/education-level</rdfs:comment>
        <rdfs:isDefinedBy rdf:resource="https://w3id.org/italia/onto/CPV"></rdfs:isDefinedBy>
        <rdfs:label xml:lang="it">codice grado di istruzione</rdfs:label>
        <rdfs:label xml:lang="en">education level identifier</rdfs:label>
        <owl:versionInfo xml:lang="it">stabile</owl:versionInfo>
        <owl:versionInfo xml:lang="en">stable</owl:versionInfo>
        <l0:controlledVocabulary rdf:resource="https://w3id.org/italia/controlled-vocabulary/classifications-for-people/education-level"></l0:controlledVocabulary>
    </owl:DatatypeProperty>



    <!-- https://w3id.org/italia/onto/CPV/familyName -->

    <owl:DatatypeProperty rdf:about="https://w3id.org/italia/onto/CPV/familyName">
        <rdfs:subPropertyOf rdf:resource="https://w3id.org/italia/onto/l0/name"></rdfs:subPropertyOf>
        <rdfs:domain rdf:resource="https://w3id.org/italia/onto/CPV/Person"></rdfs:domain>
        <rdfs:range rdf:resource="http://www.w3.org/2001/XMLSchema#string"></rdfs:range>
        <rdfs:comment xml:lang="it">Il cognome di una persona. Ex. 'Rossi' è il cognome della persona 'Mario Rossi'</rdfs:comment>
        <rdfs:comment xml:lang="en">The family name of a person. E.g. 'Rossi' is the family name of the person 'Mario Rossi'.</rdfs:comment>
        <rdfs:isDefinedBy rdf:resource="https://w3id.org/italia/onto/CPV"></rdfs:isDefinedBy>
        <rdfs:label xml:lang="it">cognome</rdfs:label>
        <rdfs:label xml:lang="en">family name</rdfs:label>
        <owl:versionInfo xml:lang="it">stabile</owl:versionInfo>
        <owl:versionInfo xml:lang="en">stable</owl:versionInfo>
    </owl:DatatypeProperty>



    <!-- https://w3id.org/italia/onto/CPV/givenName -->

    <owl:DatatypeProperty rdf:about="https://w3id.org/italia/onto/CPV/givenName">
        <rdfs:subPropertyOf rdf:resource="https://w3id.org/italia/onto/l0/name"></rdfs:subPropertyOf>
        <rdfs:domain rdf:resource="https://w3id.org/italia/onto/CPV/Person"></rdfs:domain>
        <rdfs:range rdf:resource="http://www.w3.org/2001/XMLSchema#string"></rdfs:range>
        <rdfs:comment xml:lang="it">Il nome di una persona. Ex. 'Mario' è il nome della persona 'Mario Rossi'.</rdfs:comment>
        <rdfs:comment xml:lang="en">The given name of a person. E.g. 'Mario' is the given name of the person 'Mario Rossi'.</rdfs:comment>
        <rdfs:isDefinedBy rdf:resource="https://w3id.org/italia/onto/CPV"></rdfs:isDefinedBy>
        <rdfs:label xml:lang="en">given name</rdfs:label>
        <rdfs:label xml:lang="it">nome proprio</rdfs:label>
        <owl:versionInfo xml:lang="it">stabile</owl:versionInfo>
        <owl:versionInfo xml:lang="en">stable</owl:versionInfo>
    </owl:DatatypeProperty>



    <!-- https://w3id.org/italia/onto/CPV/numberRegFamilyComponents -->

    <owl:DatatypeProperty rdf:about="https://w3id.org/italia/onto/CPV/numberRegFamilyComponents">
        <rdfs:domain rdf:resource="https://w3id.org/italia/onto/CPV/RegisteredFamily"></rdfs:domain>
        <rdfs:range rdf:resource="http://www.w3.org/2001/XMLSchema#integer"></rdfs:range>
        <rdfs:comment xml:lang="it">Il numero di persone che compongono la famiglia anagrafica</rdfs:comment>
        <rdfs:comment xml:lang="en">The number of people who forms the registered family</rdfs:comment>
        <rdfs:isDefinedBy rdf:resource="https://w3id.org/italia/onto/CPV"></rdfs:isDefinedBy>
        <rdfs:label xml:lang="en">number of components in registered family</rdfs:label>
        <rdfs:label xml:lang="it">numero componenti famiglia anagrafica</rdfs:label>
        <owl:versionInfo xml:lang="it">stabile</owl:versionInfo>
        <owl:versionInfo xml:lang="en">stable</owl:versionInfo>
    </owl:DatatypeProperty>



    <!-- https://w3id.org/italia/onto/CPV/personID -->

    <owl:DatatypeProperty rdf:about="https://w3id.org/italia/onto/CPV/personID">
        <rdfs:subPropertyOf rdf:resource="https://w3id.org/italia/onto/l0/identifier"></rdfs:subPropertyOf>
        <rdf:type rdf:resource="http://www.w3.org/2002/07/owl#FunctionalProperty"></rdf:type>
        <rdfs:domain rdf:resource="https://w3id.org/italia/onto/CPV/Person"></rdfs:domain>
        <rdfs:range rdf:resource="http://www.w3.org/2001/XMLSchema#string"></rdfs:range>
        <rdfs:comment xml:lang="it">E' un codice univoco associato a una persona. Potrebbe essere per esempio il codice individuo attribuito dall'ISTAT per la gestione dei dati nei propri registri interni.</rdfs:comment>
        <rdfs:comment xml:lang="en">Unique identifier of a person. For instance it maybe a unique code associated by ISTAT (Italian Institute of Statistics) in its internal systems.</rdfs:comment>
        <rdfs:isDefinedBy rdf:resource="https://w3id.org/italia/onto/CPV"></rdfs:isDefinedBy>
        <rdfs:label xml:lang="it">codice persona</rdfs:label>
        <rdfs:label xml:lang="en">person identifier</rdfs:label>
        <owl:versionInfo xml:lang="it">stabile</owl:versionInfo>
        <owl:versionInfo xml:lang="en">stable</owl:versionInfo>
    </owl:DatatypeProperty>



    <!-- https://w3id.org/italia/onto/CPV/registeredFamilyID -->

    <owl:DatatypeProperty rdf:about="https://w3id.org/italia/onto/CPV/registeredFamilyID">
        <rdfs:subPropertyOf rdf:resource="https://w3id.org/italia/onto/l0/identifier"></rdfs:subPropertyOf>
        <rdf:type rdf:resource="http://www.w3.org/2002/07/owl#FunctionalProperty"></rdf:type>
        <rdfs:domain rdf:resource="https://w3id.org/italia/onto/CPV/RegisteredFamily"></rdfs:domain>
        <rdfs:range rdf:resource="http://www.w3.org/2000/01/rdf-schema#Literal"></rdfs:range>
        <rdfs:comment xml:lang="it">Identificativo univoco della famiglia anagrafica</rdfs:comment>
        <rdfs:comment xml:lang="en">Unique identifier of the registered family</rdfs:comment>
        <rdfs:comment xml:lang="en">registered family identifier</rdfs:comment>
        <rdfs:isDefinedBy rdf:resource="https://w3id.org/italia/onto/CPV"></rdfs:isDefinedBy>
        <rdfs:label xml:lang="it">codice famiglia anagrafica</rdfs:label>
        <owl:versionInfo xml:lang="it">stabile</owl:versionInfo>
        <owl:versionInfo xml:lang="en">stable</owl:versionInfo>
    </owl:DatatypeProperty>



    <!-- https://w3id.org/italia/onto/CPV/sexDesc -->

    <owl:DatatypeProperty rdf:about="https://w3id.org/italia/onto/CPV/sexDesc">
        <rdfs:subPropertyOf rdf:resource="https://w3id.org/italia/onto/l0/description"></rdfs:subPropertyOf>
        <rdfs:domain rdf:resource="https://w3id.org/italia/onto/CPV/Sex"></rdfs:domain>
        <rdfs:range rdf:resource="http://www.w3.org/2000/01/rdf-schema#Literal"></rdfs:range>
        <rdfs:comment xml:lang="en">Property used to represent the sex as defined in the related Sex controlled vocabulary  https://w3id.org/italia/controlled-vocabulary/classifications-for-people/sex</rdfs:comment>
        <rdfs:comment xml:lang="it">Proprietà utilizzata per rappresentare il sesso di una persona come definito nel vocabolario controllato sul sesso: https://w3id.org/italia/controlled-vocabulary/classifications-for-people/sex</rdfs:comment>
        <rdfs:isDefinedBy rdf:resource="https://w3id.org/italia/onto/CPV"></rdfs:isDefinedBy>
        <rdfs:label xml:lang="it">descrizione sesso</rdfs:label>
        <rdfs:label xml:lang="en">sex description</rdfs:label>
        <owl:versionInfo xml:lang="it">stabile</owl:versionInfo>
        <owl:versionInfo xml:lang="en">stable</owl:versionInfo>
        <l0:controlledVocabulary rdf:resource="https://w3id.org/italia/controlled-vocabulary/classifications-for-people/sex"></l0:controlledVocabulary>
    </owl:DatatypeProperty>



    <!-- https://w3id.org/italia/onto/CPV/sexID -->

    <owl:DatatypeProperty rdf:about="https://w3id.org/italia/onto/CPV/sexID">
        <rdfs:subPropertyOf rdf:resource="https://w3id.org/italia/onto/l0/identifier"></rdfs:subPropertyOf>
        <rdf:type rdf:resource="http://www.w3.org/2002/07/owl#FunctionalProperty"></rdf:type>
        <rdfs:domain rdf:resource="https://w3id.org/italia/onto/CPV/Sex"></rdfs:domain>
        <rdfs:range rdf:resource="http://www.w3.org/2000/01/rdf-schema#Literal"></rdfs:range>
        <rdfs:comment xml:lang="it">Codice della voce del vocabolario controllato sul sesso  https://w3id.org/italia/controlled-vocabulary/classifications-for-people/sex. Esso assume i valori "M" e "F".</rdfs:comment>
        <rdfs:comment xml:lang="en">Sex code used in the sex controlled vocabulary https://w3id.org/italia/controlled-vocabulary/classifications-for-people/sex. It assumes the values "F" and "M".</rdfs:comment>
        <rdfs:isDefinedBy rdf:resource="https://w3id.org/italia/onto/CPV"></rdfs:isDefinedBy>
        <rdfs:label xml:lang="it">codice sesso</rdfs:label>
        <rdfs:label xml:lang="en">sex identifier</rdfs:label>
        <owl:versionInfo xml:lang="it">stabile</owl:versionInfo>
        <owl:versionInfo xml:lang="en">stable</owl:versionInfo>
        <l0:controlledVocabulary rdf:resource="https://w3id.org/italia/controlled-vocabulary/classifications-for-people/sex"></l0:controlledVocabulary>
    </owl:DatatypeProperty>



    <!-- https://w3id.org/italia/onto/CPV/taxCode -->

    <owl:DatatypeProperty rdf:about="https://w3id.org/italia/onto/CPV/taxCode">
        <rdfs:subPropertyOf rdf:resource="https://w3id.org/italia/onto/l0/identifier"></rdfs:subPropertyOf>
        <rdfs:domain rdf:resource="https://w3id.org/italia/onto/CPV/Person"></rdfs:domain>
        <rdfs:range rdf:resource="http://www.w3.org/2000/01/rdf-schema#Literal"></rdfs:range>
        <rdfs:comment xml:lang="it">Il codice fiscale di  una persona.</rdfs:comment>
        <rdfs:comment xml:lang="en">The tax code of a person.</rdfs:comment>
        <rdfs:isDefinedBy rdf:resource="https://w3id.org/italia/onto/CPV"></rdfs:isDefinedBy>
        <rdfs:label xml:lang="it">codice fiscale</rdfs:label>
        <rdfs:label xml:lang="en">tax code</rdfs:label>
        <owl:versionInfo xml:lang="it">stabile</owl:versionInfo>
        <owl:versionInfo xml:lang="en">stable</owl:versionInfo>
    </owl:DatatypeProperty>



    <!-- https://w3id.org/italia/onto/l0/description -->

    <owl:DatatypeProperty rdf:about="https://w3id.org/italia/onto/l0/description">
        <rdfs:isDefinedBy rdf:resource="https://w3id.org/italia/onto/l0/"></rdfs:isDefinedBy>
    </owl:DatatypeProperty>



    <!-- https://w3id.org/italia/onto/l0/identifier -->

    <owl:DatatypeProperty rdf:about="https://w3id.org/italia/onto/l0/identifier">
        <rdfs:isDefinedBy rdf:resource="https://w3id.org/italia/onto/l0/"></rdfs:isDefinedBy>
    </owl:DatatypeProperty>



    <!-- https://w3id.org/italia/onto/l0/name -->

    <owl:DatatypeProperty rdf:about="https://w3id.org/italia/onto/l0/name">
        <rdfs:isDefinedBy rdf:resource="https://w3id.org/italia/onto/l0/"></rdfs:isDefinedBy>
    </owl:DatatypeProperty>



    <!--
    ///////////////////////////////////////////////////////////////////////////////////////
    //
    // Classes
    //
    ///////////////////////////////////////////////////////////////////////////////////////
     -->




    <!-- http://dati.gov.it/onto/dcatapit#Agent -->

    <owl:Class rdf:about="http://dati.gov.it/onto/dcatapit#Agent"></owl:Class>



    <!-- http://dati.gov.it/onto/dcatapit#Organization -->

    <owl:Class rdf:about="http://dati.gov.it/onto/dcatapit#Organization"></owl:Class>



    <!-- http://www.w3.org/2006/vcard/ns#Kind -->

    <owl:Class rdf:about="http://www.w3.org/2006/vcard/ns#Kind"></owl:Class>



    <!-- http://www.w3.org/2006/vcard/ns#Organization -->

    <owl:Class rdf:about="http://www.w3.org/2006/vcard/ns#Organization"></owl:Class>



    <!-- http://xmlns.com/foaf/0.1/Agent -->

    <owl:Class rdf:about="http://xmlns.com/foaf/0.1/Agent"></owl:Class>



    <!-- https://w3id.org/italia/onto/ADMS/Project -->

    <owl:Class rdf:about="https://w3id.org/italia/onto/ADMS/Project"></owl:Class>



    <!-- https://w3id.org/italia/onto/ADMS/SemanticAsset -->

    <owl:Class rdf:about="https://w3id.org/italia/onto/ADMS/SemanticAsset"></owl:Class>



    <!-- https://w3id.org/italia/onto/ADMS/SemanticAssetDistribution -->

    <owl:Class rdf:about="https://w3id.org/italia/onto/ADMS/SemanticAssetDistribution"></owl:Class>



    <!-- https://w3id.org/italia/onto/CLV/Address -->

    <owl:Class rdf:about="https://w3id.org/italia/onto/CLV/Address"></owl:Class>



    <!-- https://w3id.org/italia/onto/CPV/Alive -->

    <owl:Class rdf:about="https://w3id.org/italia/onto/CPV/Alive">
        <rdfs:subClassOf rdf:resource="https://w3id.org/italia/onto/CPV/Person"></rdfs:subClassOf>
        <rdfs:subClassOf>
            <owl:Restriction>
                <owl:onProperty rdf:resource="https://w3id.org/italia/onto/CPV/hasLevelOfEducation"></owl:onProperty>
                <owl:maxQualifiedCardinality rdf:datatype="http://www.w3.org/2001/XMLSchema#nonNegativeInteger">1</owl:maxQualifiedCardinality>
                <owl:onClass rdf:resource="https://w3id.org/italia/onto/CPV/EducationLevel"></owl:onClass>
            </owl:Restriction>
        </rdfs:subClassOf>
        <rdfs:subClassOf>
            <owl:Restriction>
                <owl:onProperty rdf:resource="https://w3id.org/italia/onto/CPV/age"></owl:onProperty>
                <owl:maxQualifiedCardinality rdf:datatype="http://www.w3.org/2001/XMLSchema#nonNegativeInteger">1</owl:maxQualifiedCardinality>
                <owl:onDataRange rdf:resource="http://www.w3.org/2001/XMLSchema#integer"></owl:onDataRange>
            </owl:Restriction>
        </rdfs:subClassOf>
        <owl:disjointWith rdf:resource="https://w3id.org/italia/onto/CPV/Dead"></owl:disjointWith>
        <rdfs:comment xml:lang="en">An alive person</rdfs:comment>
        <rdfs:comment xml:lang="it">Una persona in vita</rdfs:comment>
        <rdfs:isDefinedBy rdf:resource="https://w3id.org/italia/onto/CPV"></rdfs:isDefinedBy>
        <rdfs:label xml:lang="en">Alive Person</rdfs:label>
        <rdfs:label xml:lang="it">Persona in Vita</rdfs:label>
        <owl:versionInfo xml:lang="it">stabile</owl:versionInfo>
        <owl:versionInfo xml:lang="en">stable</owl:versionInfo>
    </owl:Class>



    <!-- https://w3id.org/italia/onto/CPV/BornDead -->

    <owl:Class rdf:about="https://w3id.org/italia/onto/CPV/BornDead">
        <rdfs:subClassOf rdf:resource="https://w3id.org/italia/onto/CPV/Dead"></rdfs:subClassOf>
        <rdfs:comment xml:lang="en">A natural person who was born dead</rdfs:comment>
        <rdfs:comment xml:lang="it">Una persona naturale che è nata morta</rdfs:comment>
        <rdfs:isDefinedBy rdf:resource="https://w3id.org/italia/onto/CPV"></rdfs:isDefinedBy>
        <rdfs:label xml:lang="en">Born Dead Person</rdfs:label>
        <rdfs:label xml:lang="it">Persona Nata Morta</rdfs:label>
        <owl:versionInfo xml:lang="it">stabile</owl:versionInfo>
        <owl:versionInfo xml:lang="en">stable</owl:versionInfo>
    </owl:Class>



    <!-- https://w3id.org/italia/onto/CPV/Dead -->

    <owl:Class rdf:about="https://w3id.org/italia/onto/CPV/Dead">
        <rdfs:subClassOf rdf:resource="https://w3id.org/italia/onto/CPV/Person"></rdfs:subClassOf>
        <rdfs:subClassOf>
            <owl:Restriction>
                <owl:onProperty rdf:resource="https://w3id.org/italia/onto/CPV/hasDeathPlace"></owl:onProperty>
                <owl:maxQualifiedCardinality rdf:datatype="http://www.w3.org/2001/XMLSchema#nonNegativeInteger">1</owl:maxQualifiedCardinality>
                <owl:onClass rdf:resource="https://w3id.org/italia/onto/l0/Location"></owl:onClass>
            </owl:Restriction>
        </rdfs:subClassOf>
        <rdfs:subClassOf>
            <owl:Restriction>
                <owl:onProperty rdf:resource="https://w3id.org/italia/onto/CPV/ageWhenDead"></owl:onProperty>
                <owl:maxQualifiedCardinality rdf:datatype="http://www.w3.org/2001/XMLSchema#nonNegativeInteger">1</owl:maxQualifiedCardinality>
                <owl:onDataRange rdf:resource="http://www.w3.org/2001/XMLSchema#integer"></owl:onDataRange>
            </owl:Restriction>
        </rdfs:subClassOf>
        <rdfs:comment xml:lang="en">A dead natural person</rdfs:comment>
        <rdfs:comment xml:lang="it">Una persona naturale morta</rdfs:comment>
        <rdfs:isDefinedBy rdf:resource="https://w3id.org/italia/onto/CPV"></rdfs:isDefinedBy>
        <rdfs:label xml:lang="en">Dead Person</rdfs:label>
        <rdfs:label xml:lang="it">Persona Morta</rdfs:label>
        <owl:versionInfo xml:lang="it">stabile</owl:versionInfo>
        <owl:versionInfo xml:lang="en">stable</owl:versionInfo>
    </owl:Class>



    <!-- https://w3id.org/italia/onto/CPV/EducationLevel -->

    <owl:Class rdf:about="https://w3id.org/italia/onto/CPV/EducationLevel">
        <rdfs:subClassOf rdf:resource="https://w3id.org/italia/onto/l0/Characteristic"></rdfs:subClassOf>
        <rdfs:subClassOf>
            <owl:Restriction>
                <owl:onProperty rdf:resource="https://w3id.org/italia/onto/CPV/educationLevelDesc"></owl:onProperty>
                <owl:someValuesFrom rdf:resource="http://www.w3.org/2000/01/rdf-schema#Literal"></owl:someValuesFrom>
            </owl:Restriction>
        </rdfs:subClassOf>
        <rdfs:subClassOf>
            <owl:Restriction>
                <owl:onProperty rdf:resource="https://w3id.org/italia/onto/CPV/educationLevelID"></owl:onProperty>
                <owl:cardinality rdf:datatype="http://www.w3.org/2001/XMLSchema#nonNegativeInteger">1</owl:cardinality>
            </owl:Restriction>
        </rdfs:subClassOf>
        <rdfs:comment xml:lang="it">Questa classe rappresenta il grado di istruzione della persona. Le istanze di questa classe sono definite nel relativo vocabolario controllato EducationLevel https://w3id.org/italia/controlled-vocabulary/classifications-for-people/education-level</rdfs:comment>
        <rdfs:comment xml:lang="en">This class represents the level of education of a person. The individuals of this class are defined in the related controlled vocabulary EducationLevel https://w3id.org/italia/controlled-vocabulary/classifications-for-people/education-level</rdfs:comment>
        <rdfs:isDefinedBy rdf:resource="https://w3id.org/italia/onto/CPV"></rdfs:isDefinedBy>
        <rdfs:label xml:lang="en">Education Level</rdfs:label>
        <rdfs:label xml:lang="it">Grado di Istruzione</rdfs:label>
        <owl:versionInfo xml:lang="it">stabile</owl:versionInfo>
        <owl:versionInfo xml:lang="en">stable</owl:versionInfo>
        <l0:controlledVocabulary rdf:resource="https://w3id.org/italia/controlled-vocabulary/classifications-for-people/education-level"></l0:controlledVocabulary>
    </owl:Class>



    <!-- https://w3id.org/italia/onto/CPV/Family -->

    <owl:Class rdf:about="https://w3id.org/italia/onto/CPV/Family">
        <rdfs:subClassOf rdf:resource="https://w3id.org/italia/onto/l0/Agent"></rdfs:subClassOf>
        <rdfs:comment xml:lang="en">A human community generally formed by people tied together by a relationship of coexistence, of kinship, of affinity, which constitutes the fundamental element of every society, since it is aimed, in its processes and relations, at the perpetuation of the species through reproduction.</rdfs:comment>
        <rdfs:comment xml:lang="it">In senso ampio, comunità umana, diversamente caratterizzata nelle varie situazioni storiche e geografiche, ma in genere formata da persone legate fra loro da un rapporto di convivenza, di parentela, di affinità, che costituisce l’elemento fondamentale di ogni società, essendo essa finalizzata, nei suoi processi e nelle sue relazioni, alla perpetuazione della specie mediante la riproduzione.</rdfs:comment>
        <rdfs:isDefinedBy rdf:resource="https://w3id.org/italia/onto/CPV"></rdfs:isDefinedBy>
        <rdfs:label xml:lang="it">Famiglia</rdfs:label>
        <rdfs:label xml:lang="en">Family</rdfs:label>
        <owl:versionInfo xml:lang="it">stabile</owl:versionInfo>
        <owl:versionInfo xml:lang="en">stable</owl:versionInfo>
    </owl:Class>



    <!-- https://w3id.org/italia/onto/CPV/FamilySheetHolder -->

    <owl:Class rdf:about="https://w3id.org/italia/onto/CPV/FamilySheetHolder">
        <rdfs:subClassOf rdf:resource="https://w3id.org/italia/onto/CPV/Person"></rdfs:subClassOf>
        <rdfs:comment xml:lang="it">Questa classe rappresenta l'intestatario del foglio di famiglia. Per intestatario del foglio di famiglia si intende la persona cui è intestata la scheda di famiglia in anagrafe.</rdfs:comment>
        <rdfs:comment xml:lang="en">This class represents the holder of the family sheet. The holder of the family sheet is defined as the person to whom the family in the civil register is headed.</rdfs:comment>
        <rdfs:isDefinedBy rdf:resource="https://w3id.org/italia/onto/CPV"></rdfs:isDefinedBy>
        <rdfs:label xml:lang="en">Family Sheet Holder</rdfs:label>
        <rdfs:label xml:lang="it">Intestatario Foglio di Famiglia</rdfs:label>
        <owl:versionInfo xml:lang="it">stabile</owl:versionInfo>
        <owl:versionInfo xml:lang="en">stable</owl:versionInfo>
    </owl:Class>



    <!-- https://w3id.org/italia/onto/CPV/Female -->

    <owl:Class rdf:about="https://w3id.org/italia/onto/CPV/Female">
        <rdfs:subClassOf rdf:resource="https://w3id.org/italia/onto/CPV/Person"></rdfs:subClassOf>
        <owl:disjointWith rdf:resource="https://w3id.org/italia/onto/CPV/Male"></owl:disjointWith>
        <rdfs:isDefinedBy rdf:resource="https://w3id.org/italia/onto/CPV"></rdfs:isDefinedBy>
        <rdfs:label xml:lang="en">Female</rdfs:label>
        <rdfs:label xml:lang="it">Femmina</rdfs:label>
        <rdfs:comment xml:lang="en">A natural person of sex Female</rdfs:comment>
        <rdfs:comment xml:lang="it">Una persona naturale di sesso femminile</rdfs:comment>
        <owl:versionInfo xml:lang="it">stabile</owl:versionInfo>
        <owl:versionInfo xml:lang="en">stable</owl:versionInfo>
    </owl:Class>



    <!-- https://w3id.org/italia/onto/CPV/ForeignCitizen -->

    <owl:Class rdf:about="https://w3id.org/italia/onto/CPV/ForeignCitizen">
        <rdfs:subClassOf rdf:resource="https://w3id.org/italia/onto/CPV/Alive"></rdfs:subClassOf>
        <rdfs:comment xml:lang="en">A natural person who owns a foreign nationality</rdfs:comment>
        <rdfs:comment xml:lang="it">Una persona naturale che ha cittadinanza straniera</rdfs:comment>
        <rdfs:isDefinedBy rdf:resource="https://w3id.org/italia/onto/CPV"></rdfs:isDefinedBy>
        <rdfs:label xml:lang="it">Cittadino Straniero</rdfs:label>
        <rdfs:label xml:lang="en">Foreign Citizen</rdfs:label>
        <owl:versionInfo xml:lang="it">stabile</owl:versionInfo>
        <owl:versionInfo xml:lang="en">stable</owl:versionInfo>
    </owl:Class>



    <!-- https://w3id.org/italia/onto/CPV/ItalianCitizen -->

    <owl:Class rdf:about="https://w3id.org/italia/onto/CPV/ItalianCitizen">
        <rdfs:subClassOf rdf:resource="https://w3id.org/italia/onto/CPV/Alive"></rdfs:subClassOf>
        <rdfs:comment xml:lang="en">A natural person who owns an Italian nationality</rdfs:comment>
        <rdfs:comment xml:lang="it">Una persona naturale che possiede la cittadinanza italiana</rdfs:comment>
        <rdfs:isDefinedBy rdf:resource="https://w3id.org/italia/onto/CPV"></rdfs:isDefinedBy>
        <rdfs:label xml:lang="it">Cittadino Italiano</rdfs:label>
        <rdfs:label xml:lang="en">Italian Citizen</rdfs:label>
        <owl:versionInfo xml:lang="it">stabile</owl:versionInfo>
        <owl:versionInfo xml:lang="en">stable</owl:versionInfo>
    </owl:Class>



    <!-- https://w3id.org/italia/onto/CPV/Male -->

    <owl:Class rdf:about="https://w3id.org/italia/onto/CPV/Male">
        <rdfs:subClassOf rdf:resource="https://w3id.org/italia/onto/CPV/Person"></rdfs:subClassOf>
        <rdfs:isDefinedBy rdf:resource="https://w3id.org/italia/onto/CPV"></rdfs:isDefinedBy>
        <rdfs:label xml:lang="en">Male</rdfs:label>
        <rdfs:label xml:lang="it">Maschio</rdfs:label>
        <rdfs:comment xml:lang="en">A natural person with sex Male</rdfs:comment>
        <rdfs:comment xml:lang="it">Una persona naturale di sesso maschile</rdfs:comment>
        <owl:versionInfo xml:lang="it">stabile</owl:versionInfo>
        <owl:versionInfo xml:lang="en">stable</owl:versionInfo>
    </owl:Class>



    <!-- https://w3id.org/italia/onto/CPV/NotResident -->

    <owl:Class rdf:about="https://w3id.org/italia/onto/CPV/NotResident">
        <rdfs:subClassOf rdf:resource="https://w3id.org/italia/onto/CPV/Person"></rdfs:subClassOf>
        <owl:disjointWith rdf:resource="https://w3id.org/italia/onto/CPV/Resident"></owl:disjointWith>
        <rdfs:comment xml:lang="en">A natural person who is not resident in the country.</rdfs:comment>
        <rdfs:comment xml:lang="it">Una persona naturale non residenze nel Paese.</rdfs:comment>
        <rdfs:isDefinedBy rdf:resource="https://w3id.org/italia/onto/CPV"></rdfs:isDefinedBy>
        <rdfs:label xml:lang="en">Not Resident Person</rdfs:label>
        <rdfs:label xml:lang="it">Persona non Residente</rdfs:label>
        <owl:versionInfo xml:lang="it">stabile</owl:versionInfo>
        <owl:versionInfo xml:lang="en">stable</owl:versionInfo>
    </owl:Class>



    <!-- https://w3id.org/italia/onto/CPV/ParentalRelationshipType -->

    <owl:Class rdf:about="https://w3id.org/italia/onto/CPV/ParentalRelationshipType">
        <rdfs:subClassOf rdf:resource="https://w3id.org/italia/onto/l0/Description"></rdfs:subClassOf>
        <rdfs:comment xml:lang="it">La classe rappresenta i diversi tipi di relazioni parentali. Per esempio l'intestatario della scheda di famiglia in anagrafe è un tipo di relazione parentale così come il coniuge (o convivente) dell'intestatario, il figlio  dell'intestatario e coniuge convivente, il fratello/sorella dell'intestatario.</rdfs:comment>
        <rdfs:comment xml:lang="en">The class represents the different types of parental relationships</rdfs:comment>
        <rdfs:isDefinedBy rdf:resource="https://w3id.org/italia/onto/CPV"></rdfs:isDefinedBy>
        <rdfs:label xml:lang="en">Parental Relationship Type</rdfs:label>
        <rdfs:label xml:lang="it">Tipo Relazione Parentale</rdfs:label>
        <owl:versionInfo xml:lang="it">stabile</owl:versionInfo>
        <owl:versionInfo xml:lang="en">stable</owl:versionInfo>
        <l0:controlledVocabulary rdf:resource="https://w3id.org/italia/controlled-vocabulary/classifications-for-people/parental-relationship-types"></l0:controlledVocabulary>
    </owl:Class>



    <!-- https://w3id.org/italia/onto/CPV/Person -->

    <owl:Class rdf:about="https://w3id.org/italia/onto/CPV/Person">
        <rdfs:subClassOf rdf:resource="https://w3id.org/italia/onto/l0/Agent"></rdfs:subClassOf>
        <rdfs:subClassOf>
            <owl:Restriction>
                <owl:onProperty rdf:resource="https://w3id.org/italia/onto/CLV/hasAddress"></owl:onProperty>
                <owl:allValuesFrom rdf:resource="https://w3id.org/italia/onto/CLV/Address"></owl:allValuesFrom>
            </owl:Restriction>
        </rdfs:subClassOf>
        <rdfs:subClassOf>
            <owl:Restriction>
                <owl:onProperty rdf:resource="https://w3id.org/italia/onto/CPV/hasParentalRelationshipWith"></owl:onProperty>
                <owl:allValuesFrom rdf:resource="https://w3id.org/italia/onto/CPV/Person"></owl:allValuesFrom>
            </owl:Restriction>
        </rdfs:subClassOf>
        <rdfs:subClassOf>
            <owl:Restriction>
                <owl:onProperty rdf:resource="https://w3id.org/italia/onto/CPV/hasPersonTitle"></owl:onProperty>
                <owl:allValuesFrom rdf:resource="https://w3id.org/italia/onto/CPV/PersonTitle"></owl:allValuesFrom>
            </owl:Restriction>
        </rdfs:subClassOf>
        <rdfs:subClassOf>
            <owl:Restriction>
                <owl:onProperty rdf:resource="https://w3id.org/italia/onto/CPV/hasRelationshipWith"></owl:onProperty>
                <owl:allValuesFrom rdf:resource="https://w3id.org/italia/onto/CPV/Person"></owl:allValuesFrom>
            </owl:Restriction>
        </rdfs:subClassOf>
        <rdfs:subClassOf>
            <owl:Restriction>
                <owl:onProperty rdf:resource="https://w3id.org/italia/onto/CPV/hasResidenceInTime"></owl:onProperty>
                <owl:allValuesFrom rdf:resource="https://w3id.org/italia/onto/CPV/ResidenceInTime"></owl:allValuesFrom>
            </owl:Restriction>
        </rdfs:subClassOf>
        <rdfs:subClassOf>
            <owl:Restriction>
                <owl:onProperty rdf:resource="https://w3id.org/italia/onto/CPV/residentIn"></owl:onProperty>
                <owl:allValuesFrom rdf:resource="https://w3id.org/italia/onto/CLV/Address"></owl:allValuesFrom>
            </owl:Restriction>
        </rdfs:subClassOf>
        <rdfs:subClassOf>
            <owl:Restriction>
                <owl:onProperty rdf:resource="https://w3id.org/italia/onto/CPV/hasBirthPlace"></owl:onProperty>
                <owl:qualifiedCardinality rdf:datatype="http://www.w3.org/2001/XMLSchema#nonNegativeInteger">1</owl:qualifiedCardinality>
                <owl:onClass rdf:resource="https://w3id.org/italia/onto/l0/Location"></owl:onClass>
            </owl:Restriction>
        </rdfs:subClassOf>
        <rdfs:subClassOf>
            <owl:Restriction>
                <owl:onProperty rdf:resource="https://w3id.org/italia/onto/CPV/hasSex"></owl:onProperty>
                <owl:qualifiedCardinality rdf:datatype="http://www.w3.org/2001/XMLSchema#nonNegativeInteger">1</owl:qualifiedCardinality>
                <owl:onClass rdf:resource="https://w3id.org/italia/onto/CPV/Sex"></owl:onClass>
            </owl:Restriction>
        </rdfs:subClassOf>
        <rdfs:subClassOf>
            <owl:Restriction>
                <owl:onProperty rdf:resource="https://w3id.org/italia/onto/CPV/dateOfBirth"></owl:onProperty>
                <owl:qualifiedCardinality rdf:datatype="http://www.w3.org/2001/XMLSchema#nonNegativeInteger">1</owl:qualifiedCardinality>
                <owl:onDataRange rdf:resource="http://www.w3.org/2001/XMLSchema#dateTime"></owl:onDataRange>
            </owl:Restriction>
        </rdfs:subClassOf>
        <rdfs:subClassOf>
            <owl:Restriction>
                <owl:onProperty rdf:resource="https://w3id.org/italia/onto/CPV/personID"></owl:onProperty>
                <owl:qualifiedCardinality rdf:datatype="http://www.w3.org/2001/XMLSchema#nonNegativeInteger">1</owl:qualifiedCardinality>
                <owl:onDataRange rdf:resource="http://www.w3.org/2001/XMLSchema#string"></owl:onDataRange>
            </owl:Restriction>
        </rdfs:subClassOf>
        <rdfs:subClassOf>
            <owl:Restriction>
                <owl:onProperty rdf:resource="https://w3id.org/italia/onto/CPV/altName"></owl:onProperty>
                <owl:maxQualifiedCardinality rdf:datatype="http://www.w3.org/2001/XMLSchema#nonNegativeInteger">1</owl:maxQualifiedCardinality>
                <owl:onDataRange rdf:resource="http://www.w3.org/2001/XMLSchema#string"></owl:onDataRange>
            </owl:Restriction>
        </rdfs:subClassOf>
        <rdfs:subClassOf>
            <owl:Restriction>
                <owl:onProperty rdf:resource="https://w3id.org/italia/onto/CPV/familyName"></owl:onProperty>
                <owl:maxQualifiedCardinality rdf:datatype="http://www.w3.org/2001/XMLSchema#nonNegativeInteger">1</owl:maxQualifiedCardinality>
                <owl:onDataRange rdf:resource="http://www.w3.org/2001/XMLSchema#string"></owl:onDataRange>
            </owl:Restriction>
        </rdfs:subClassOf>
        <rdfs:subClassOf>
            <owl:Restriction>
                <owl:onProperty rdf:resource="https://w3id.org/italia/onto/CPV/givenName"></owl:onProperty>
                <owl:maxQualifiedCardinality rdf:datatype="http://www.w3.org/2001/XMLSchema#nonNegativeInteger">1</owl:maxQualifiedCardinality>
                <owl:onDataRange rdf:resource="http://www.w3.org/2001/XMLSchema#string"></owl:onDataRange>
            </owl:Restriction>
        </rdfs:subClassOf>
        <rdfs:subClassOf>
            <owl:Restriction>
                <owl:onProperty rdf:resource="https://w3id.org/italia/onto/CPV/taxCode"></owl:onProperty>
                <owl:maxCardinality rdf:datatype="http://www.w3.org/2001/XMLSchema#nonNegativeInteger">1</owl:maxCardinality>
            </owl:Restriction>
        </rdfs:subClassOf>
        <rdfs:comment xml:lang="en">A natural person</rdfs:comment>
        <rdfs:comment xml:lang="it">Una persona naturale</rdfs:comment>
        <rdfs:isDefinedBy rdf:resource="https://w3id.org/italia/onto/CPV"></rdfs:isDefinedBy>
        <rdfs:label xml:lang="en">Person</rdfs:label>
        <rdfs:label xml:lang="it">Persona</rdfs:label>
        <owl:versionInfo xml:lang="it">stabile</owl:versionInfo>
        <owl:versionInfo xml:lang="en">stable</owl:versionInfo>
    </owl:Class>



    <!-- https://w3id.org/italia/onto/CPV/PersonTitle -->

    <owl:Class rdf:about="https://w3id.org/italia/onto/CPV/PersonTitle">
        <rdfs:subClassOf rdf:resource="https://w3id.org/italia/onto/l0/Characteristic"></rdfs:subClassOf>
        <rdfs:comment xml:lang="en">A title is a word used before or after a person's name (e.g. Mr., Mrs. etc.)</rdfs:comment>
        <rdfs:comment xml:lang="it">Un titolo è una parola usata prima o dopo il nome di una persona (e.g. Sig. Dott., Avv.).</rdfs:comment>
        <rdfs:isDefinedBy rdf:resource="https://w3id.org/italia/onto/CPV"></rdfs:isDefinedBy>
        <rdfs:label xml:lang="en">Person Title</rdfs:label>
        <rdfs:label xml:lang="it">Titolo Persona</rdfs:label>
        <owl:versionInfo xml:lang="it">instabile</owl:versionInfo>
        <owl:versionInfo xml:lang="en">unstable</owl:versionInfo>
        <l0:controlledVocabulary rdf:resource="https://w3id.org/italia/controlled-vocabulary/classifications-for-people/person-title"></l0:controlledVocabulary>
    </owl:Class>



    <!-- https://w3id.org/italia/onto/CPV/RegisteredFamily -->

    <owl:Class rdf:about="https://w3id.org/italia/onto/CPV/RegisteredFamily">
        <rdfs:subClassOf rdf:resource="https://w3id.org/italia/onto/CPV/Family"></rdfs:subClassOf>
        <rdfs:subClassOf>
            <owl:Restriction>
                <owl:onProperty rdf:resource="https://w3id.org/italia/onto/CPV/registeredFamilyID"></owl:onProperty>
                <owl:cardinality rdf:datatype="http://www.w3.org/2001/XMLSchema#nonNegativeInteger">1</owl:cardinality>
            </owl:Restriction>
        </rdfs:subClassOf>
        <rdfs:subClassOf>
            <owl:Restriction>
                <owl:onProperty rdf:resource="https://w3id.org/italia/onto/CPV/numberRegFamilyComponents"></owl:onProperty>
                <owl:maxQualifiedCardinality rdf:datatype="http://www.w3.org/2001/XMLSchema#nonNegativeInteger">1</owl:maxQualifiedCardinality>
                <owl:onDataRange rdf:resource="http://www.w3.org/2001/XMLSchema#integer"></owl:onDataRange>
            </owl:Restriction>
        </rdfs:subClassOf>
        <rdfs:comment xml:lang="it">E' un insieme di persone legate da vincoli di matrimonio, parentela, affinità, adozione, tutela o da vincoli affettivi. I membri devono coabitare e avere dimora abituale nello stesso Comune (articolo 4 del Decreto del Presidente della Repubblica 30/05/1989, n. 223)</rdfs:comment>
        <rdfs:comment xml:lang="en">It is a group of people tied together by relationships of marriage, kinship, affinity, adoption, protection or affection. The members must live and be habitually resident in the same municipality (Article 4 of Italian Presidential Decree 30/05/1989, n. 223)</rdfs:comment>
        <rdfs:label xml:lang="it">Famiglia Anagrafica</rdfs:label>
        <rdfs:label xml:lang="en">Registered Family</rdfs:label>
        <owl:versionInfo rdf:resource="https://w3id.org/italia/onto/CPV"></owl:versionInfo>
        <owl:versionInfo xml:lang="it">stabile</owl:versionInfo>
        <owl:versionInfo xml:lang="en">stable</owl:versionInfo>
    </owl:Class>



    <!-- https://w3id.org/italia/onto/CPV/ResidenceInTime -->

    <owl:Class rdf:about="https://w3id.org/italia/onto/CPV/ResidenceInTime">
        <rdfs:subClassOf rdf:resource="https://w3id.org/italia/onto/TI/TimeIndexedEvent"></rdfs:subClassOf>
        <rdfs:subClassOf>
            <owl:Restriction>
                <owl:onProperty rdf:resource="https://w3id.org/italia/onto/CPV/residenceInLocation"></owl:onProperty>
                <owl:qualifiedCardinality rdf:datatype="http://www.w3.org/2001/XMLSchema#nonNegativeInteger">1</owl:qualifiedCardinality>
                <owl:onClass rdf:resource="https://w3id.org/italia/onto/CLV/Address"></owl:onClass>
            </owl:Restriction>
        </rdfs:subClassOf>
        <rdfs:subClassOf>
            <owl:Restriction>
                <owl:onProperty rdf:resource="https://w3id.org/italia/onto/CPV/isResidenceInTimeOf"></owl:onProperty>
                <owl:maxQualifiedCardinality rdf:datatype="http://www.w3.org/2001/XMLSchema#nonNegativeInteger">1</owl:maxQualifiedCardinality>
                <owl:onClass rdf:resource="https://w3id.org/italia/onto/CPV/Person"></owl:onClass>
            </owl:Restriction>
        </rdfs:subClassOf>
        <rdfs:comment xml:lang="it">Questa classe rappresenta una relazione ennaria tra diversi concetti del dominio, in particolare con una persona residente in un paese, il luogo di residenza e il periodo temporale. E' utilizzata per gestire lo storico delle residenze delle persone. Essa è sottoclasse di 'TimeIndexedEvent' definita nell'ontologia del tempo della rete di ontologie OntoPiA e pertanto eredita la relazione con l'intervallo temporale.</rdfs:comment>
        <rdfs:comment xml:lang="en">This class represents the n-ary relationship between a resident, the location of residence and the time. It is specifically subclass of the TimeIndexedEvent defined in the time ontology of OntoPiA network from which it inherits the relationship with the time interval</rdfs:comment>
        <rdfs:isDefinedBy rdf:resource="https://w3id.org/italia/onto/CPV"></rdfs:isDefinedBy>
        <rdfs:label xml:lang="en">Residence in Time</rdfs:label>
        <rdfs:label xml:lang="it">Residenza nel tempo (storica)</rdfs:label>
        <owl:versionInfo xml:lang="it">provvisoria</owl:versionInfo>
        <owl:versionInfo xml:lang="en">unstable</owl:versionInfo>
    </owl:Class>



    <!-- https://w3id.org/italia/onto/CPV/Resident -->

    <owl:Class rdf:about="https://w3id.org/italia/onto/CPV/Resident">
        <rdfs:subClassOf rdf:resource="https://w3id.org/italia/onto/CPV/Alive"></rdfs:subClassOf>
        <rdfs:subClassOf>
            <owl:Restriction>
                <owl:onProperty rdf:resource="https://w3id.org/italia/onto/CPV/belongsToFamily"></owl:onProperty>
                <owl:allValuesFrom rdf:resource="https://w3id.org/italia/onto/CPV/Family"></owl:allValuesFrom>
            </owl:Restriction>
        </rdfs:subClassOf>
        <rdfs:subClassOf>
            <owl:Restriction>
                <owl:onProperty rdf:resource="https://w3id.org/italia/onto/CPV/hasCurrentResidence"></owl:onProperty>
                <owl:qualifiedCardinality rdf:datatype="http://www.w3.org/2001/XMLSchema#nonNegativeInteger">1</owl:qualifiedCardinality>
                <owl:onClass rdf:resource="https://w3id.org/italia/onto/l0/Location"></owl:onClass>
            </owl:Restriction>
        </rdfs:subClassOf>
        <rdfs:comment xml:lang="en">A natural person who is resident in the country</rdfs:comment>
        <rdfs:comment xml:lang="it">Una persona naturale residente nel Paese.</rdfs:comment>
        <rdfs:isDefinedBy rdf:resource="https://w3id.org/italia/onto/CPV"></rdfs:isDefinedBy>
        <rdfs:label xml:lang="en">Resident</rdfs:label>
        <rdfs:label xml:lang="it">Residente</rdfs:label>
        <owl:versionInfo xml:lang="it">stabile</owl:versionInfo>
        <owl:versionInfo xml:lang="en">stable</owl:versionInfo>
    </owl:Class>



    <!-- https://w3id.org/italia/onto/CPV/Sex -->

    <owl:Class rdf:about="https://w3id.org/italia/onto/CPV/Sex">
        <rdfs:subClassOf rdf:resource="https://w3id.org/italia/onto/l0/Characteristic"></rdfs:subClassOf>
        <rdfs:subClassOf>
            <owl:Restriction>
                <owl:onProperty rdf:resource="https://w3id.org/italia/onto/CPV/sexDesc"></owl:onProperty>
                <owl:someValuesFrom rdf:resource="http://www.w3.org/2001/XMLSchema#string"></owl:someValuesFrom>
            </owl:Restriction>
        </rdfs:subClassOf>
        <rdfs:subClassOf>
            <owl:Restriction>
                <owl:onProperty rdf:resource="https://w3id.org/italia/onto/CPV/sexID"></owl:onProperty>
                <owl:cardinality rdf:datatype="http://www.w3.org/2001/XMLSchema#nonNegativeInteger">1</owl:cardinality>
            </owl:Restriction>
        </rdfs:subClassOf>
        <rdfs:comment xml:lang="it">Questa classe rappresenta il sesso della persona. Le istanze della classe sono definite nel relativo vocabolario controllato sul sesso https://w3id.org/italia/controlled-vocabulary/classifications-for-people/sex</rdfs:comment>
        <rdfs:comment xml:lang="en">This class represents the sex of the person. The instances of the class are defined in the related sex controlled vocabulary https://w3id.org/italia/controlled-vocabulary/classifications-for-people/sex</rdfs:comment>
        <rdfs:isDefinedBy rdf:resource="https://w3id.org/italia/onto/CPV"></rdfs:isDefinedBy>
        <rdfs:label xml:lang="it">Sesso</rdfs:label>
        <rdfs:label xml:lang="en">Sex</rdfs:label>
        <owl:versionInfo xml:lang="it">stabile</owl:versionInfo>
        <owl:versionInfo xml:lang="en">stable</owl:versionInfo>
        <l0:controlledVocabulary rdf:resource="https://w3id.org/italia/controlled-vocabulary/classifications-for-people/sex"></l0:controlledVocabulary>
    </owl:Class>



    <!-- https://w3id.org/italia/onto/CPV/Stateless -->

    <owl:Class rdf:about="https://w3id.org/italia/onto/CPV/Stateless">
        <rdfs:subClassOf rdf:resource="https://w3id.org/italia/onto/CPV/Alive"></rdfs:subClassOf>
        <owl:disjointWith>
            <owl:Class>
                <owl:unionOf rdf:parseType="Collection">
                    <rdf:Description rdf:about="https://w3id.org/italia/onto/CPV/ForeignCitizen"></rdf:Description>
                    <rdf:Description rdf:about="https://w3id.org/italia/onto/CPV/ItalianCitizen"></rdf:Description>
                </owl:unionOf>
            </owl:Class>
        </owl:disjointWith>
        <rdfs:comment xml:lang="en">A natural person who emigrated abroad, who has no nationality, because he or she does not have the nationality of origin and does not possess another one.</rdfs:comment>
        <rdfs:comment xml:lang="it">Una persona naturale emigrata all'estero, che non ha alcuna cittadinanza, perché priva di quella di origine e non in possesso di un'altra</rdfs:comment>
        <rdfs:isDefinedBy rdf:resource="https://w3id.org/italia/onto/CPV"></rdfs:isDefinedBy>
        <rdfs:label xml:lang="it">Apolide</rdfs:label>
        <rdfs:label xml:lang="en">Stateless Person</rdfs:label>
        <owl:versionInfo xml:lang="it">stabile</owl:versionInfo>
        <owl:versionInfo xml:lang="en">stable</owl:versionInfo>
    </owl:Class>



    <!--
    ///////////////////////////////////////////////////////////////////////////////////////
    //
    // Individuals
    //
    ///////////////////////////////////////////////////////////////////////////////////////
     -->




    <!-- http://spcdata.digitpa.gov.it/browse/page/Amministrazione/ISTAT -->

    <owl:NamedIndividual rdf:about="http://spcdata.digitpa.gov.it/browse/page/Amministrazione/ISTAT">
        <rdf:type rdf:resource="http://dati.gov.it/onto/dcatapit#Agent"></rdf:type>
        <rdf:type rdf:resource="http://xmlns.com/foaf/0.1/Agent"></rdf:type>
        <dct:identifier>ISTAT</dct:identifier>
        <foaf:name xml:lang="it">Istituto Nazionale di Statistica - ISTAT</foaf:name>
        <foaf:name xml:lang="en">Italian National Institute of Statistics - ISTAT</foaf:name>
    </owl:NamedIndividual>



    <!-- http://spcdata.digitpa.gov.it/browse/page/Amministrazione/agid -->

    <owl:NamedIndividual rdf:about="http://spcdata.digitpa.gov.it/browse/page/Amministrazione/agid">
        <rdf:type rdf:resource="http://dati.gov.it/onto/dcatapit#Agent"></rdf:type>
        <rdf:type rdf:resource="http://xmlns.com/foaf/0.1/Agent"></rdf:type>
        <dct:identifier>agid</dct:identifier>
        <foaf:name xml:lang="it">Agenzia per l'Italia Digitale</foaf:name>
        <foaf:name xml:lang="en">Italian Digital Agency</foaf:name>
    </owl:NamedIndividual>



    <!-- https://w3id.org/italia/controlled-vocabulary/classifications-for-people/parental-relationship-types/1 -->

    <owl:NamedIndividual rdf:about="https://w3id.org/italia/controlled-vocabulary/classifications-for-people/parental-relationship-types/1">
        <owl:sameAs rdf:resource="https://w3id.org/italia/onto/CPV/isFamilySheetHolderOf"></owl:sameAs>
    </owl:NamedIndividual>



    <!-- https://w3id.org/italia/controlled-vocabulary/classifications-for-people/parental-relationship-types/10 -->

    <owl:NamedIndividual rdf:about="https://w3id.org/italia/controlled-vocabulary/classifications-for-people/parental-relationship-types/10">
        <owl:sameAs rdf:resource="https://w3id.org/italia/onto/CPV/isNephewOf"></owl:sameAs>
    </owl:NamedIndividual>



    <!-- https://w3id.org/italia/controlled-vocabulary/classifications-for-people/parental-relationship-types/11 -->

    <owl:NamedIndividual rdf:about="https://w3id.org/italia/controlled-vocabulary/classifications-for-people/parental-relationship-types/11">
        <owl:sameAs rdf:resource="https://w3id.org/italia/onto/CPV/isUncleOf"></owl:sameAs>
    </owl:NamedIndividual>



    <!-- https://w3id.org/italia/controlled-vocabulary/classifications-for-people/parental-relationship-types/2 -->

    <owl:NamedIndividual rdf:about="https://w3id.org/italia/controlled-vocabulary/classifications-for-people/parental-relationship-types/2">
        <owl:sameAs rdf:resource="https://w3id.org/italia/onto/CPV/isConsortOf"></owl:sameAs>
    </owl:NamedIndividual>



    <!-- https://w3id.org/italia/controlled-vocabulary/classifications-for-people/parental-relationship-types/3 -->

    <owl:NamedIndividual rdf:about="https://w3id.org/italia/controlled-vocabulary/classifications-for-people/parental-relationship-types/3">
        <owl:sameAs rdf:resource="https://w3id.org/italia/onto/CPV/isChildOf"></owl:sameAs>
    </owl:NamedIndividual>



    <!-- https://w3id.org/italia/controlled-vocabulary/classifications-for-people/parental-relationship-types/4 -->

    <owl:NamedIndividual rdf:about="https://w3id.org/italia/controlled-vocabulary/classifications-for-people/parental-relationship-types/4">
        <owl:sameAs rdf:resource="https://w3id.org/italia/onto/CPV/isGrandChildOf"></owl:sameAs>
    </owl:NamedIndividual>



    <!-- https://w3id.org/italia/controlled-vocabulary/classifications-for-people/parental-relationship-types/6 -->

    <owl:NamedIndividual rdf:about="https://w3id.org/italia/controlled-vocabulary/classifications-for-people/parental-relationship-types/6">
        <owl:sameAs rdf:resource="https://w3id.org/italia/onto/CPV/isParentOf"></owl:sameAs>
    </owl:NamedIndividual>



    <!-- https://w3id.org/italia/controlled-vocabulary/classifications-for-people/parental-relationship-types/7 -->

    <owl:NamedIndividual rdf:about="https://w3id.org/italia/controlled-vocabulary/classifications-for-people/parental-relationship-types/7">
        <owl:sameAs rdf:resource="https://w3id.org/italia/onto/CPV/isGrandFatherOf"></owl:sameAs>
    </owl:NamedIndividual>



    <!-- https://w3id.org/italia/data/contact-point/onto-agid -->

    <owl:NamedIndividual rdf:about="https://w3id.org/italia/data/contact-point/onto-agid">
        <rdf:type rdf:resource="http://dati.gov.it/onto/dcatapit#Organization"></rdf:type>
        <rdf:type rdf:resource="http://www.w3.org/2006/vcard/ns#Kind"></rdf:type>
        <rdf:type rdf:resource="http://www.w3.org/2006/vcard/ns#Organization"></rdf:type>
        <vcard:fn>banche dati e open data</vcard:fn>
        <vcard:hasEmail rdf:resource="mailto:info@dati.gov.it"></vcard:hasEmail>
    </owl:NamedIndividual>



    <!-- https://w3id.org/italia/data/distribution/CPVAPIT-JSON-LD -->

    <owl:NamedIndividual rdf:about="https://w3id.org/italia/data/distribution/CPVAPIT-JSON-LD">
        <rdf:type rdf:resource="https://w3id.org/italia/onto/ADMS/SemanticAssetDistribution"></rdf:type>
        <dct:description xml:lang="it">Questa è la distribuzione JSON-LD dell'ontologia delle Persone</dct:description>
        <dct:description xml:lang="en">This is the distribution in JSON-LD of the persons ontology</dct:description>
        <dct:format rdf:resource="http://publications.europa.eu/resource/authority/file-type/JSON_LD"></dct:format>
        <dct:license rdf:resource="https://w3id.org/italia/controlled-vocabulary/licences/A21_CCBY40"></dct:license>
        <dct:title xml:lang="it">Distribuzione JSON-LD ontologia CPV-AP_IT</dct:title>
        <dct:title xml:lang="en">JSON-LD distribution of CPV-AP_IT Ontology</dct:title>
        <dcat:accessURL rdf:resource="https://raw.githubusercontent.com/italia/daf-ontologie-vocabolari-controllati/master/Ontologie/CPV/latest"></dcat:accessURL>
        <dcat:downloadURL rdf:resource="https://raw.githubusercontent.com/italia/daf-ontologie-vocabolari-controllati/master/Ontologie/CPV/latest/CPV-AP_IT.jsonld"></dcat:downloadURL>
    </owl:NamedIndividual>



    <!-- https://w3id.org/italia/data/distribution/CPVAPIT-RDF-TURTLE -->

    <owl:NamedIndividual rdf:about="https://w3id.org/italia/data/distribution/CPVAPIT-RDF-TURTLE">
        <rdf:type rdf:resource="https://w3id.org/italia/onto/ADMS/SemanticAssetDistribution"></rdf:type>
        <dct:description xml:lang="it">Questa è la distribuzione RDF/Turtle dell'ontologia delle persone</dct:description>
        <dct:description xml:lang="en">This is the distribution in RDF/turtle of the persons ontology</dct:description>
        <dct:format rdf:resource="http://publications.europa.eu/resource/authority/file-type/RDF_TURTLE"></dct:format>
        <dct:license rdf:resource="https://w3id.org/italia/controlled-vocabulary/licences/A21_CCBY40"></dct:license>
        <dct:title xml:lang="it">Distribuzione RDF/Turtle ontologia CPV-AP_IT</dct:title>
        <dct:title xml:lang="en">RDF/Turtle distribution of CPV-AP_IT Ontology</dct:title>
        <dcat:accessURL rdf:resource="https://raw.githubusercontent.com/italia/daf-ontologie-vocabolari-controllati/master/Ontologie/CPV/latest"></dcat:accessURL>
        <dcat:downloadURL rdf:resource="https://raw.githubusercontent.com/italia/daf-ontologie-vocabolari-controllati/master/Ontologie/CPV/latest/CPV-AP_IT.ttl"></dcat:downloadURL>
    </owl:NamedIndividual>



    <!-- https://w3id.org/italia/data/distribution/CPVAPIT-RDF-XML -->

    <owl:NamedIndividual rdf:about="https://w3id.org/italia/data/distribution/CPVAPIT-RDF-XML">
        <rdf:type rdf:resource="https://w3id.org/italia/onto/ADMS/SemanticAssetDistribution"></rdf:type>
        <dct:description xml:lang="it">Questa è la distribuzione RDF/XML dell'ontologia delle persone</dct:description>
        <dct:description xml:lang="en">This is the distribution in RDF/XML of the persons ontology</dct:description>
        <dct:format rdf:resource="http://publications.europa.eu/resource/authority/file-type/RDF_XML"></dct:format>
        <dct:license rdf:resource="https://w3id.org/italia/controlled-vocabulary/licences/A21_CCBY40"></dct:license>
        <dct:title xml:lang="it">Distribuzione RDF/XML ontologia CPV-AP_IT</dct:title>
        <dct:title xml:lang="en">RDF/XML distribution of CPV-AP_IT Ontology</dct:title>
        <dcat:accessURL rdf:resource="https://raw.githubusercontent.com/italia/daf-ontologie-vocabolari-controllati/master/Ontologie/CPV/latest"></dcat:accessURL>
        <dcat:downloadURL rdf:resource="https://raw.githubusercontent.com/italia/daf-ontologie-vocabolari-controllati/master/Ontologie/CPV/latest/CPV-AP_IT.rdf"></dcat:downloadURL>
    </owl:NamedIndividual>



    <!-- https://w3id.org/italia/data/organization/support-unit/cnr-Z6HZEH/stlab -->

    <owl:NamedIndividual rdf:about="https://w3id.org/italia/data/organization/support-unit/cnr-Z6HZEH/stlab">
        <rdf:type rdf:resource="http://dati.gov.it/onto/dcatapit#Agent"></rdf:type>
        <rdf:type rdf:resource="http://xmlns.com/foaf/0.1/Agent"></rdf:type>
        <dct:identifier>cnr - Z6HZEH - STLab</dct:identifier>
        <foaf:name xml:lang="en">Institute of Cognitive Sciences and Technologies of the Italian Research Council (CNR) - Semantic Technology Laboratory (STLab)</foaf:name>
        <foaf:name xml:lang="it">Istituto di Scienze e Tecnologie della Cognizione del CNR - Semantic Technology Lab (STLab)</foaf:name>
    </owl:NamedIndividual>



    <!-- https://w3id.org/italia/data/project/DAF -->

    <owl:NamedIndividual rdf:about="https://w3id.org/italia/data/project/DAF">
        <rdf:type rdf:resource="https://w3id.org/italia/onto/ADMS/Project"></rdf:type>
        <l0:name xml:lang="it">Data &amp; Analytics Framework</l0:name>
    </owl:NamedIndividual>



    <!-- https://w3id.org/italia/data/project/OntoPiA -->

    <owl:NamedIndividual rdf:about="https://w3id.org/italia/data/project/OntoPiA">
        <rdf:type rdf:resource="https://w3id.org/italia/onto/ADMS/Project"></rdf:type>
        <l0:name xml:lang="it">OntoPiA - la rete di ontologie della pubblica amministrazione italiana</l0:name>
    </owl:NamedIndividual>



    <!-- https://w3id.org/italia/onto/CPV -->

    <owl:NamedIndividual rdf:about="https://w3id.org/italia/onto/CPV">
        <rdf:type rdf:resource="https://w3id.org/italia/onto/ADMS/SemanticAsset"></rdf:type>
    </owl:NamedIndividual>



    <!-- https://w3id.org/italia/onto/CPV/isChildOf -->

    <owl:NamedIndividual rdf:about="https://w3id.org/italia/onto/CPV/isChildOf">
        <rdf:type rdf:resource="https://w3id.org/italia/onto/CPV/ParentalRelationshipType"></rdf:type>
    </owl:NamedIndividual>



    <!-- https://w3id.org/italia/onto/CPV/isConsortOf -->

    <owl:NamedIndividual rdf:about="https://w3id.org/italia/onto/CPV/isConsortOf">
        <rdf:type rdf:resource="https://w3id.org/italia/onto/CPV/ParentalRelationshipType"></rdf:type>
    </owl:NamedIndividual>



    <!-- https://w3id.org/italia/onto/CPV/isFamilySheetHolderOf -->

    <owl:NamedIndividual rdf:about="https://w3id.org/italia/onto/CPV/isFamilySheetHolderOf">
        <rdf:type rdf:resource="https://w3id.org/italia/onto/CPV/ParentalRelationshipType"></rdf:type>
    </owl:NamedIndividual>



    <!-- https://w3id.org/italia/onto/CPV/isGrandChildOf -->

    <owl:NamedIndividual rdf:about="https://w3id.org/italia/onto/CPV/isGrandChildOf">
        <rdf:type rdf:resource="https://w3id.org/italia/onto/CPV/ParentalRelationshipType"></rdf:type>
    </owl:NamedIndividual>



    <!-- https://w3id.org/italia/onto/CPV/isGrandFatherOf -->

    <owl:NamedIndividual rdf:about="https://w3id.org/italia/onto/CPV/isGrandFatherOf">
        <rdf:type rdf:resource="https://w3id.org/italia/onto/CPV/ParentalRelationshipType"></rdf:type>
    </owl:NamedIndividual>



    <!-- https://w3id.org/italia/onto/CPV/isNephewOf -->

    <owl:NamedIndividual rdf:about="https://w3id.org/italia/onto/CPV/isNephewOf">
        <rdf:type rdf:resource="https://w3id.org/italia/onto/CPV/ParentalRelationshipType"></rdf:type>
    </owl:NamedIndividual>



    <!-- https://w3id.org/italia/onto/CPV/isParentOf -->

    <owl:NamedIndividual rdf:about="https://w3id.org/italia/onto/CPV/isParentOf">
        <rdf:type rdf:resource="https://w3id.org/italia/onto/CPV/ParentalRelationshipType"></rdf:type>
    </owl:NamedIndividual>



    <!-- https://w3id.org/italia/onto/CPV/isUncleOf -->

    <owl:NamedIndividual rdf:about="https://w3id.org/italia/onto/CPV/isUncleOf">
        <rdf:type rdf:resource="https://w3id.org/italia/onto/CPV/ParentalRelationshipType"></rdf:type>
    </owl:NamedIndividual>



    <!--
    ///////////////////////////////////////////////////////////////////////////////////////
    //
    // Annotations
    //
    ///////////////////////////////////////////////////////////////////////////////////////
     -->

    <rdf:Description rdf:about="https://w3id.org/italia/onto/CPV/isChildOf">
        <rdfs:isDefinedBy rdf:resource="https://w3id.org/italia/onto/CPV"></rdfs:isDefinedBy>
        <rdfs:comment xml:lang="it">La relazione figlio-padre (ex. Mario è figlio di Carlo).</rdfs:comment>
        <rdfs:comment xml:lang="en">The relation child-parent (e.g. John is the son of Peter).</rdfs:comment>
        <owl:versionInfo xml:lang="en">stable</owl:versionInfo>
        <owl:versionInfo xml:lang="it">stabile</owl:versionInfo>
        <rdfs:label xml:lang="it">figlio di</rdfs:label>
        <rdfs:label xml:lang="en">child of</rdfs:label>
    </rdf:Description>
    <rdf:Description rdf:about="https://w3id.org/italia/onto/CPV/isConsortOf">
        <rdfs:comment xml:lang="it">La relazione di matrimonio tra due persone.</rdfs:comment>
        <owl:versionInfo xml:lang="en">stable</owl:versionInfo>
        <rdfs:label xml:lang="en">is consort of</rdfs:label>
        <rdfs:comment xml:lang="en">The marriage relation between persons</rdfs:comment>
        <owl:versionInfo xml:lang="it">stabile</owl:versionInfo>
        <rdfs:label xml:lang="it">è coniuge di</rdfs:label>
        <rdfs:isDefinedBy rdf:resource="https://w3id.org/italia/onto/CPV"></rdfs:isDefinedBy>
    </rdf:Description>
    <rdf:Description rdf:about="https://w3id.org/italia/onto/CPV/isFamilySheetHolderOf">
        <rdfs:comment xml:lang="it">Proprietà che lega l'intestatario del foglio di famiglia a una persona</rdfs:comment>
        <rdfs:comment xml:lang="en">Property that links the family sheet holder to a person of the family</rdfs:comment>
        <rdfs:isDefinedBy rdf:resource="https://w3id.org/italia/onto/CPV"></rdfs:isDefinedBy>
        <owl:versionInfo xml:lang="en">unstable</owl:versionInfo>
        <rdfs:label xml:lang="en">intestatario foglio di famiglia di</rdfs:label>
        <owl:versionInfo xml:lang="it">provvisoria</owl:versionInfo>
        <rdfs:label xml:lang="en">family sheet holder of</rdfs:label>
    </rdf:Description>
    <rdf:Description rdf:about="https://w3id.org/italia/onto/CPV/isGrandChildOf">
        <rdfs:isDefinedBy rdf:resource="https://w3id.org/italia/onto/CPV"></rdfs:isDefinedBy>
        <rdfs:comment xml:lang="en">It represents the parental relationship grandchild-grandfather</rdfs:comment>
        <rdfs:label xml:lang="it">è nipote lato nonni di</rdfs:label>
        <rdfs:label xml:lang="en">is granchild of</rdfs:label>
        <owl:versionInfo xml:lang="en">unstable</owl:versionInfo>
        <rdfs:comment xml:lang="it">Rappresenta la relazione di parentela nipote-nonno</rdfs:comment>
        <owl:versionInfo xml:lang="it">provvisoria</owl:versionInfo>
    </rdf:Description>
    <rdf:Description rdf:about="https://w3id.org/italia/onto/CPV/isGrandFatherOf">
        <rdfs:comment xml:lang="en">The grandfathership relation</rdfs:comment>
        <owl:versionInfo xml:lang="it">stabile</owl:versionInfo>
        <rdfs:isDefinedBy rdf:resource="https://w3id.org/italia/onto/CPV"></rdfs:isDefinedBy>
        <owl:versionInfo xml:lang="en">stable</owl:versionInfo>
        <rdfs:comment xml:lang="it">La relazione parentale tra nonno-nipote</rdfs:comment>
        <rdfs:label xml:lang="it">è nonno di</rdfs:label>
        <rdfs:label xml:lang="en">is grandfather of</rdfs:label>
    </rdf:Description>
    <rdf:Description rdf:about="https://w3id.org/italia/onto/CPV/isNephewOf">
        <rdfs:comment xml:lang="en">The nephew relation between a newphew and an uncle.</rdfs:comment>
        <rdfs:isDefinedBy rdf:resource="https://w3id.org/italia/onto/CPV"></rdfs:isDefinedBy>
        <rdfs:label xml:lang="it">è nipote lato zii di</rdfs:label>
        <rdfs:comment xml:lang="it">La relazione di parentela tra un nipote ed uno zio.</rdfs:comment>
        <owl:versionInfo xml:lang="it">provvisoria</owl:versionInfo>
        <owl:versionInfo xml:lang="en">unstable</owl:versionInfo>
        <rdfs:label xml:lang="en">is nephew of</rdfs:label>
    </rdf:Description>
    <rdf:Description rdf:about="https://w3id.org/italia/onto/CPV/isParentOf">
        <rdfs:comment xml:lang="it">La relazione padre-figlio.</rdfs:comment>
        <owl:versionInfo xml:lang="en">stable</owl:versionInfo>
        <rdfs:comment xml:lang="en">The parent-child relationship.</rdfs:comment>
        <rdfs:label xml:lang="en">is parent of</rdfs:label>
        <rdfs:isDefinedBy rdf:resource="https://w3id.org/italia/onto/CPV"></rdfs:isDefinedBy>
        <rdfs:label xml:lang="it">è genitore di</rdfs:label>
        <owl:versionInfo xml:lang="it">stabile</owl:versionInfo>
    </rdf:Description>
    <rdf:Description rdf:about="https://w3id.org/italia/onto/CPV/isUncleOf">
        <owl:versionInfo xml:lang="it">provvisoria</owl:versionInfo>
        <rdfs:comment xml:lang="it">La relazione di parentela tra zio e nipote.</rdfs:comment>
        <owl:versionInfo xml:lang="en">unstable</owl:versionInfo>
        <rdfs:comment xml:lang="en">The uncleship relation.</rdfs:comment>
        <rdfs:isDefinedBy rdf:resource="https://w3id.org/italia/onto/CPV"></rdfs:isDefinedBy>
        <rdfs:label xml:lang="it">è zio di</rdfs:label>
        <rdfs:label xml:lang="en">is uncle of</rdfs:label>
    </rdf:Description>
</rdf:RDF>
<!-- Generated by the OWL API (version 4.5.9.2019-02-01T07:24:44Z) https://github.com/owlcs/owlapi -->