@prefix :      <http://contrattipubblici.org/csi/> .
@prefix l0:    <http://dati.gov.it/onto/l0/> .
@prefix owl:   <http://www.w3.org/2002/07/owl#> .
@prefix xsd:   <http://www.w3.org/2001/XMLSchema#> .
@prefix rdfs:  <http://www.w3.org/2000/01/rdf-schema#> .

:subcontratctExpected
        a             owl:DatatypeProperty ;
        rdfs:comment  "The property that determines if a subcontract if expected in the Contract."@en , "La proprietà che determina se nel contratto è previsto un subappalto."@it ;
        rdfs:domain   :Contract ;
        rdfs:label    "subcontract expected"@en , "previsto subappalto"@it ;
        rdfs:range    xsd:boolean .

:Threshold  a         owl:Class ;
        rdfs:comment  "La classe che rappresenta la soglia di prezzo di un Contratto."@it , "The class that represents the price threshold of a contract."@en ;
        rdfs:label    "Threshold"@en , "Soglia"@it .

:municipalityCode  rdfs:comment  "La proprietà che dermina il codice identificativo del comune (codice Istat)."@it , "The property that determines the municipality code (codice Istat)."@en ;
        rdfs:domain   :BusinessEntity , :Location ;
        rdfs:label    "Municipality identifier code"@en , "Codice identificativo del Comune"@it ;
        rdfs:range    xsd:string .

:netAmount  rdfs:comment  "La proprietà che determina l'ammontare netto del pagamento."@it , "The property that determines the net amount of the payment."@en ;
        rdfs:domain   :Bill ;
        rdfs:label    "net amount"@en , "ammontare netto"@it ;
        rdfs:range    xsd:float .

:publicationDate  a   owl:DatatypeProperty ;
        rdfs:comment  "The property that determines the publication date of the Announcement or the Lot."@en , "La proprietà che indica la data di pubblicazione del Bando/Avviso. o del Lotto"@it ;
        rdfs:domain   :Lot , :Announcement ;
        rdfs:label    "publication date"@en , "data pubblicazione"@it ;
        rdfs:range    xsd:date .

<http://contrattipubblici/csi/agreedPrice>
        a             owl:DatatypeProperty ;
        rdfs:comment  "The Property that determines the price agreed for the Contract or the Announcement."@en , "La proprietà che determina il prezzo concordato per il Contratto o per il Bando."@it ;
        rdfs:domain   :Announcement , :Contract ;
        rdfs:label    "Agreed price"@en , "Prezzo concordato"@it ;
        rdfs:range    xsd:float .

:variationType  rdfs:comment  "The property that determines contract variation type."@en , "La proprietà che determina il tipo di variante del contratto."@it ;
        rdfs:domain   :Variant ;
        rdfs:label    "variation type"@en , "tipo variante"@it ;
        rdfs:range    xsd:string .

:announcementType  a  owl:ObjectProperty ;
        rdfs:comment  "La proprietà che indica il tipo di bando."@it , "La proprietà che definisce un criterio di valutazione dell'offerta."@it , "The property that determines the announcement type."@en , "Property for setting a criterion for tender evaluation."@en ;
        rdfs:domain   :Announcement ;
        rdfs:label    "has award criterion"@en , "ha tipo bando"@it , "ha tipo di aggiudicazione"@it , "has type announcement"@en ;
        rdfs:range    :announcementType , :AnnouncementType .

:hasReason  a         owl:ObjectProperty ;
        rdfs:comment  "The property that links the contract variation and the related motivation."@en , "La proprietà che collega la variante del contratto alla relativa motivazione."@it ;
        rdfs:domain   :Variant ;
        rdfs:label    "has motivation"@it , "ha motivazione"@it ;
        rdfs:range    :VariantReason .

:validityEndDate  a   owl:DatatypeProperty ;
        rdfs:comment  "The property that determines the validity end date of a Threshold."@en , "La proprietà che determina la data di cessazionedi validità della Soglia comunitaria."@it ;
        rdfs:domain   :Threshold ;
        rdfs:label    "Data termine validita."@it , "Validity end date."@en ;
        rdfs:range    xsd:date .

:contractingAuthority
        a             owl:ObjectProperty ;
        rdfs:comment  "Institution which issues a public contract, receives tenders to the contract and chooses a suitable supplier on the base of the conditions given by the contract."@en , "La proprietà che indica l'istituzione che emette il contratto pubblico, riceve le offerte e sceglie il fornitore idoneo sulla base delle condizioni definite dal contratto."@it ;
        rdfs:domain   :Lot ;
        rdfs:label    "contracting Authority"@en , "stazione appaltante"@it ;
        rdfs:range    :BusinessEntity .

:estimatedAmount  rdfs:comment  "La proprietà che detemina limporto di denaro presunto relativo ad un Subappalto."@it , "The property that determines the estimated amount of money of a subcontract."@en ;
        rdfs:domain   :SubContract ;
        rdfs:label    "Estimated Amount"@it , "importo Presunto"@it ;
        rdfs:range    xsd:float .

:ProcedureType  a     owl:Class ;
        rdfs:comment  "La  Classe che rappresenta la procedura di scelta del contraente."@it , "The class that represents the type of procedure."@en ;
        rdfs:label    "Procedure Type"@en , "Procedura di Scelta del Contraente"@it .

:actualEndDate  a     owl:DatatypeProperty ;
        rdfs:comment  "Questa proprietà indica la data di effettiva realizzazione del contratto pubblico"@it , "Property for actual end date of public contract's realization."@en ;
        rdfs:domain   :Contract ;
        rdfs:label    "Property for actual end date of public contract's realization."@en , "Data effettiva termine lavoro"@it ;
        rdfs:range    xsd:date .

:contractEndDate  a   owl:DatatypeProperty ;
        rdfs:comment  "Questa proprietà determina la fine dei lavori dichiarata nel contratto."@it , "The property that determines the end date declared in the Contract."@en ;
        rdfs:domain   :Contract ;
        rdfs:label    "Contract end Date"@en , "data fine Contrattuale"@it ;
        rdfs:range    xsd:float .

:hasVariant  a        owl:ObjectProperty ;
        rdfs:comment  "The property that determines the contract variation."@en , "La proprietà che determina la variazione del contratto."@it ;
        rdfs:domain   :Contract ;
        rdfs:label    "has variation"@en , "ha variante"@it ;
        rdfs:range    :Variant .

:awardedTender  a     owl:ObjectProperty ;
        rdfs:comment  "Property for awarded tender submitted by a bidder."@en , "La proprietà che indica l'offerta aggiudicataria presentata da un offerente."@it ;
        rdfs:domain   :Contract ;
        rdfs:label    "has awarded tender"@en , "ha offerta aggiudicataria"@it ;
        rdfs:range    <http://purl.org/procurement/public-contracts#Tender> .

:procedureType  a     owl:ObjectProperty ;
        rdfs:comment  "Type of procedure of a public contract specifies a procedure which is applied to publish information about the contract and choose a supplier."@en , "La proprietà che specifica i criteri applicati per la pubblicazione di un lotto e per la scelta di un contraente."@it ;
        rdfs:domain   :Announcement , :Lot ;
        rdfs:label    "has type of procedure"@en , "ha scelta contraente"@it ;
        rdfs:range    :ProcedureType .

:Contract  a          owl:Class ;
        rdfs:comment  "Una istanza di questa classe rappresenta un contratto realizzato tra una stazione appaltante e un fornitore."@it , "An instance of this class is an abstract information entity about a realized contract between a contracting authority and their supplier."@en ;
        rdfs:label    "Contratto"@it , "Contract"@en .

:payment  rdfs:domain  :Contract ;
        rdfs:range   :Conto .

:CPVsoap  rdfs:domain  :Contract ;
        rdfs:range   :Cpv .

:additionalDays  rdfs:comment  "Questa proprietà indica i giorni aggiuntivi necessari per la variante."@it , "The property that determines additional days needed in the variation."@en ;
        rdfs:domain   :Variant ;
        rdfs:label    "additional days"@en , "giorni aggiuntivi"@it ;
        rdfs:range    xsd:float .

:Variant  a           owl:Class ;
        rdfs:comment  "La classe che rappresenta la variazione di un contratto."@it , "The class that represents a contract variation."@en ;
        rdfs:label    "Variant"@en , "Variante"@it .

:Tender  a            owl:Class ;
        rdfs:comment  "Una istanza di questa classe rappresenta una offerta relativa ad un lotto."@it , "An instance of this class rapresents a tender of a lot"@en ;
        rdfs:label    "Offerta"@it , "Tender"@en .

:LegalNature  a                  owl:Class ;
        rdfs:comment             "La classe che rappresenta la natura legale di una Business Entity."@it , "The class that represents the legal nature of a Business Entity."@en ;
        rdfs:label               "Legal Nature"@en , "Natura Giuridica"@it ;
        l0:controlledVocabulary  <http://dati.gov.it/onto/controlledvocabulary/CommonProcurementVocabulary> .

:bidder  rdfs:comment  "Questa proprietà rappresenta l'offerente di una offerta."@it , "This property represents the bidder of a Tender"@en ;
        rdfs:domain   :Tender ;
        rdfs:label    "Offerente"@it , "bidder"@en ;
        rdfs:range    :BusinessEntity .

:specialSector  a     owl:DatatypeProperty ;
        rdfs:comment  "La proprietà che determina se un contratto appartiene a uno dei settori speciali definiti dal DLGS 163/2006 Art3."@it , "The property that determines wheter or not the Contract belongs to with a sector  that is considered special by DLGS 163/2006 Art3."@en ;
        rdfs:domain   :Soglia , :Contract ;
        rdfs:label    "special sector"@en , "settore speciale"@it ;
        rdfs:range    xsd:boolean .

:actualPrice  a       owl:DatatypeProperty ;
        rdfs:comment  "La proprietà che determina la somma di denaro che non è ribassabile relativa ad un Lotto."@it , "The property that determines the final amount of money to be paid"@en ;
        rdfs:domain   :Contract ;
        rdfs:label    "Actual price"@it , "Importo conto finale"@it ;
        rdfs:range    xsd:float .

:AnnouncementOutcome  a  owl:Class ;
        rdfs:comment  "The class that represents the type final state of the announcement."@en , "La classe che rappresenta l'esito di un bando/avviso."@it ;
        rdfs:label    "Announcement Outcome"@en , "Esito del Bando"@it .

:Cpv    a                        owl:Class ;
        rdfs:comment             "Una istanza di questa classe rappresenta la classificazione di un lotto secondo il Common Procurement Vocabulary"@it , "This class rapresents the lot classification with the Common Procurement Vocabulary"@en ;
        rdfs:label               "Common Procurement Vocabulary"@it , "Common Procurement Vocabulary"@en ;
        l0:controlledVocabulary  <http://dati.gov.it/onto/controlledvocabulary/CommonProcurementVocabulary> .

:CPVsimog  rdfs:domain  :Contract ;
        rdfs:range   :Cpv .

:MotivazioneVariante  a  owl:Class ;
        rdfs:comment  "The class that represents the motivation of the variation of the contract."@en ;
        rdfs:label    "MotivazioneVariante" .

:CPV    rdfs:comment  "CPV (Common Procurement Vocabulary) code describing the main object of a public contract."@en ;
        rdfs:domain   :subappalto , :Lot ;
        rdfs:label    "CPV" ;
        rdfs:range    :Cpv .

:codNat  rdfs:domain  :BusinessEntity ;
        rdfs:range   :NatGiuridica .

:reductionPercentage  a  owl:DatatypeProperty ;
        rdfs:comment  "The property that determines the declared percentage of price cut."@en , "La proprietà che determina la percentuale dichiarata di ribasso."@it ;
        rdfs:domain   :Contract ;
        rdfs:label    "reduction percentage"@en , "percentuale di ribasso"@it ;
        rdfs:range    xsd:float .

:winDate  a           owl:DatatypeProperty ;
        rdfs:comment  "Property for date of contract award to a bidder."@en , "Proprietà che indica la data di aggiudicazione di un contratto a un offerente"@it ;
        rdfs:domain   :Announcement ;
        rdfs:label    "data di aggiudicazione"@it , "win date"@en ;
        rdfs:range    xsd:date .

l0:controlledVocabulary
        a       owl:AnnotationProperty .

:Location  a          owl:Class ;
        rdfs:comment  "Una istanza di questa classe prappresenta una localizzazione"@it , "An instance of this class rapresents a  Location"@en ;
        rdfs:label    "Localizzazione"@it , "Location"@en .

:startDate  a         owl:DatatypeProperty ;
        rdfs:comment  "La proprietà che determina la data di inzio dei lavori."@en , "The property that detemins the beginning date."@en ;
        rdfs:domain   :Threshold , :Lot ;
        rdfs:label    "Start Date"@en , "Data di inizio"@it ;
        rdfs:range    xsd:date .

:NUTS   rdfs:comment             "La proprietà che determina il codice nut."@it , "The property that determines the NUTS code."@en ;
        rdfs:domain              :Location ;
        rdfs:label               "NUTS"@it , "NUTS"@en ;
        rdfs:range               xsd:string ;
        l0:controlledVocabulary  <http://dati.gov.it/onto/controlledvocabulary/NUTS> .

:AnnouncementType  a  owl:Class ;
        rdfs:comment  "The class that represents the announcement type."@en , "La classe che rappresenta il tipo di bando/avviso."@it ;
        rdfs:label    "Announcement Type "@en , "Tipopolgia del Bando"@it .

:contractType  a      owl:ObjectProperty ;
        rdfs:comment  "The property for declaring the type of contract (work service or supply)."@en , "La proprietà che indica il tipo di contratto."@it ;
        rdfs:domain   :Soglia , :Contract ;
        rdfs:label    "has type of contract"@en , "ha tipo di contratto"@it ;
        rdfs:range    :ProcedureType .

:expireDate  a        owl:DatatypeProperty ;
        rdfs:comment  "The property that determines the expire date."@en , "Proprietà che determina la data di scadenza del Bando/Avviso."@it ;
        rdfs:domain   :Announcement ;
        rdfs:label    "expire date"@it , "expire date"@en ;
        rdfs:range    xsd:date .

:Bill   a             owl:Class ;
        rdfs:comment  "Una istanza di questa classe rappresenta il conto associato ad  una contratto."@en , "The class that represents the Bill associated to a contract"@en ;
        rdfs:label    "Bill"@en .

:auctionBaseAmount  a  owl:DatatypeProperty ;
        rdfs:comment  "The property that determines the auction base amount."@en , "La proprietà che determina l'importo base dell'asta."@it ;
        rdfs:domain   :Contract ;
        rdfs:label    "auction base amount"@en , "importo base asta"@it ;
        rdfs:range    xsd:float .

:frameworkAgreement  a  owl:ObjectProperty ;
        rdfs:comment  "The property that determines the type of award of the announcement."@en , "La proprietà che determina il tipo di aggiudicazione del bando."@it ;
        rdfs:domain   :Contract ;
        rdfs:label    "type of Award"@en , "tipo di Aggiudicazione"@it ;
        rdfs:range    :FrameworkAgreement .

:Announcement  a      owl:Class ;
        rdfs:comment  "The class that represents an announcement of one or more lots. That is either a notice or an announcement."@en , "La classe che rappresenta un tipo di annuncio di uno o più lotti, sia esso un bando o un avviso."@it ;
        rdfs:label    "Announcement"@en , "Bando/Avviso"@it .

:importoProgetto  a   owl:DatatypeProperty ;
        rdfs:comment  "The property that determines the planning cost of the Contract."@en , "La proprietà che determina l'importo per il progetto del contratto."@it ;
        rdfs:domain   :Contract ;
        rdfs:label    "planning cost"@en , "importo progetto"@it ;
        rdfs:range    xsd:float .

:safetyAmount  a      owl:DatatypeProperty ;
        rdfs:comment  "The property that determines the amount of money to be spent for safety reason as stated in the lot or in the Announcement."@en , "La proprietà che determina l'importo dedicato alla sicurezza stabilito nel lotto oppure nel bando"@it ;
        rdfs:domain   :Announcement , :Lot ;
        rdfs:label    "safety amount"@en , "importo sicurezza"@it ;
        rdfs:range    xsd:float .

:hasAnnouncement  a   owl:ObjectProperty ;
        rdfs:comment  "The property that determines if the related contract belongs to an announcement."@en , "La proprietà che indica se il contratto appartiene a un bando."@it ;
        rdfs:domain   :Lot ;
        rdfs:label    "has announcement"@en , "ha bando"@it ;
        rdfs:range    xsd:string , :Announcement .

:nonDiscountableSum  a  owl:DatatypeProperty ;
        rdfs:comment  "La proprietà che determina la somma di nenaro che non è ribassabile relativa ad un Lotto."@it , "The property that determines the amount of the starting price that is not lowerable."@en ;
        rdfs:domain   :Lot ;
        rdfs:label    "Sum of non-discountable money"@en , "Somma non ribassabile"@it ;
        rdfs:range    xsd:float .

:FrameworkAgreement  a  owl:Class ;
        rdfs:comment  "The class that represents the award type."@en ;
        rdfs:label    "Framework Agreement"@en , "Tipo di Aggiudicazione"@it .

:TipContratto  a      owl:Class ;
        rdfs:comment  "The class that represents the type of the contract (work service or supply)."@en ;
        rdfs:label    "TipContratto" .

:estimatedEndDate  a  owl:DatatypeProperty ;
        rdfs:comment  "La proprietà che determina la data  stimata di fine lavori."@en , "The property that detemins the estimated end Date."@en ;
        rdfs:domain   :Contract ;
        rdfs:label    "Estimated End Date"@en , "Data stimata di fine lavori"@it ;
        rdfs:range    xsd:date .

:hasSubcontractor  a  owl:ObjectProperty ;
        rdfs:comment  "The property that determines the business entity that sign the subcontract."@en , "The property che indica la business entity che sottoscrive il subappalto."@it ;
        rdfs:domain   :Subcontract ;
        rdfs:label    "has subcontractor"@en , "ha subappaltatrice"@it ;
        rdfs:range    :BusinessEntity .

:BusinessEntity  a    owl:Class ;
        rdfs:comment  "Una istance di questa classe rappresenta una entità commerciale che fa o cerca una particolare offerta. Questa può essere una persona fisica o una persona giuridica."@it , "An instance of this class represents the legal agent making (or seeking) a particular offering. This can be a legal body or a person."@en ;
        rdfs:label    "BusinessEntity"@en , "Entità commerciale"@it .

:Subcontract  a       owl:Class ;
        rdfs:comment  "An instance of this class represents a subcontract."@en , "Una istanza di questa classe rappresenta un subcontratto."@it ;
        rdfs:label    "Subcontract"@en , "Subappalto"@it .

:Lot    a             owl:Class ;
        rdfs:comment  "Una istanza di questa classe rappresenta un contratto pubblico."@it , "An instance of this class is an abstract information entity about a public contract. It consists of all currently known information about a contract, e.g., a contracting authority, services or supplies which shall be purchased, and contract conditions (e.g., important dates, expected price, etc.). It also informs about tenders received from particular bidders and about an accepted tender. If the contract has already been realized it also informs about an actual price of realization, etc."@en ;
        rdfs:label    "Lotto"@it , "Lot"@en .

:identifiers  a       owl:DatatypeProperty ;
        rdfs:comment  "La proprietà che determina l'identificativo."@it , "The property that determines the identifier."@en ;
        rdfs:domain   :BusinessEntity , :Cpv , :Contract ;
        rdfs:label    "Identifier"@en , "Identificativo"@it ;
        rdfs:range    xsd:string .
