@prefix owl: <http://www.w3.org/2002/07/owl#> .
@prefix rdfs: <http://www.w3.org/2000/01/rdf-schema#> .
@prefix gr: <http://purl.org/goodrelations/v1#> .
@prefix xsd: <http://www.w3.org/2001/XMLSchema#> .


#################################################################
#    Object Properties
#################################################################


<http://contrattipubblici.org/csi/frameworkAgreement>
  rdfs:domain <http://purl.org/procurement/public-contracts#Contract> ;
  rdfs:range <http://contrattipubblici.org/csi/FrameworkAgreement> ;
  rdfs:label "tipo di Aggiudicazione"@it ;
  rdfs:comment "The property that determines the type of award of the announcement."@en ;
  owl:equivalentProperty <http://purl.org/procurement/public-contracts#frameworkAgreement> .

csi:payment   rdfs:domain csi:Contract ;
  rdfs:range <http://contrattipubblici.org/csi/Conto> .


<http://contrattipubblici.org/csi/CPV>
  rdfs:domain <http://purl.org/procurement/public-contracts#Contract>, <http://contrattipubblici.org/csi/subappalto> ;
  rdfs:range <http://contrattipubblici.org/csi/Cpv> ;
  rdfs:label "CPV" ;
  rdfs:comment "CPV (Common Procurement Vocabulary) code describing the main object of a public contract."@en ;
  owl:equivalentProperty <http://purl.org/procurement/public-contracts#mainObject> .

<http://contrattipubblici.org/csi/CPVsoap>
  rdfs:domain <http://purl.org/procurement/public-contracts#Contract> ;
  rdfs:range <http://contrattipubblici.org/csi/Cpv> .

<http://contrattipubblici.org/csi/CPVsimog>
  rdfs:domain <http://purl.org/procurement/public-contracts#Contract> ;
  rdfs:range <http://contrattipubblici.org/csi/Cpv> .

<http://purl.org/procurement/public-contracts#contractingAutority>
  rdfs:domain <http://purl.org/procurement/public-contracts#Contract> ;
  rdfs:range gr:BusinessEntity .

<http://contrattipubblici.org/csi/haBando>
  rdfs:domain <http://purl.org/procurement/public-contracts#Contract> ;
  rdfs:range <http://contrattipubblici.org/csi/Bando>, xsd:string ;
  rdfs:label "haBando" ;
  rdfs:comment "The property that determines if the related contract belongs to an announcement."@en .


<http://contrattipubblici.org/csi/opera>
  rdfs:domain <http://purl.org/procurement/public-contracts#Contract> ;
  rdfs:range <http://contrattipubblici.org/csi/Opera> ;
  rdfs:label "opera" ;
  rdfs:comment "The property that link the contract with the related 'Opera'."@en .

<http://contrattipubblici.org/csi/tipContratto>
  rdfs:domain <http://purl.org/procurement/public-contracts#Contract>, <http://contrattipubblici.org/csi/Soglia> ;
  rdfs:range <http://contrattipubblici.org/csi/TipContratto> ;
  rdfs:label "tipContratto" ;
  rdfs:comment "The property for declaring the type of contract (work service or supply)."@en .

<http://contrattipubblici.org/csi/sceltaContr>
  rdfs:domain <http://purl.org/procurement/public-contracts#Contract>, <http://contrattipubblici.org/csi/Bando> ;
  rdfs:range <http://contrattipubblici.org/csi/SceltaContraente> ;
  rdfs:label "sceltaContr" ;
  owl:equivalentProperty <http://purl.org/procurement/public-contracts#procedureType> .

<http://purl.org/procurement/public-contracts#awardedTender>
  rdfs:domain <http://purl.org/procurement/public-contracts#Contract> ;
  rdfs:range <http://purl.org/procurement/public-contracts#Tender> .

<http://contrattipubblici.org/csi/haVariante>
  rdfs:domain <http://purl.org/procurement/public-contracts#Contract> ;
  rdfs:range <http://contrattipubblici.org/csi/Variante> ;
  rdfs:label "haVariante" ;
  rdfs:comment "The property that determines the contract variation."@en .


<http://contrattipubblici.org/csi/tipBando>
  rdfs:domain <http://contrattipubblici.org/csi/Bando> ;
  rdfs:range <http://contrattipubblici.org/csi/TipBando> ;
  rdfs:label "tipBando" ;
  rdfs:comment "The property that determines the announcement type."@en .

<http://contrattipubblici.org/csi/tipAggiudicazione>
  rdfs:domain <http://contrattipubblici.org/csi/Bando> ;
  rdfs:range <http://contrattipubblici.org/csi/TipAggiudicazione> ;
  rdfs:label "tipAggiudicazione" ;
  owl:equivalentProperty <http://purl.org/procurement/public-contracts#awardCriterion> .


  
#################################################################
#    Data properties
#################################################################
 
 

<http://contrattipubblici/csi/agreedPrice>
   rdfs:label "Prezzo concordato"@it ;
   rdfs:label "Agreed Price"@en ;
  rdfs:comment "The property that determines the type of award of the announcement."@en ;
  rdfs:comment "La proprietà che determina il prezzo concordato per il lotto."@en ;
  rdfs:domain csi:Contract ;
  rdfs:range xsd:float .

<http://contrattipubblici.org/csi/nonDiscountableSum>
  rdfs:domain csi:Contract ;
  rdfs:range xsd:float ;
  rdfs:label "Somma non ribassabile"@it ;
    rdfs:label "Sum of non-discountable money"@en ;
  rdfs:comment "The property that determines the amount of the starting price that is not lowerable."@en ;
  rdfs:comment "La proprietà che determina la somma di nenaro che non è ribassabile relativa ad un Lotto."@it .

<http://contrattipubblici.org/csi/actualPrice>
  rdfs:domain <http://purl.org/procurement/public-contracts#Contract> ;
  rdfs:range xsd:float ;
  rdfs:label "importoconto finale"@it ;
  rdfs:label "Actual Price"@it ;
rdfs:comment "The property that determines the final amount of money to be paid"@en ;
  rdfs:comment "La proprietà che determina la somma di nenaro che non è ribassabile relativa ad un Lotto."@it .

csi:date   rdfs:domain csi:Contract, <http://contrattipubblici.org/csi/Conto> ;
  rdfs:range xsd:date ;
   rdfs:label "Prezzo concordato"@it ;
   rdfs:label "Agreed Price"@en ;
  rdfs:comment "The property that determines the type of award of the announcement."@en ;
  rdfs:comment "La proprietà che determina il prezzo concordato per il lotto."@en ;

<http://contrattipubblici.org/csi/percRibasso>
  rdfs:domain <http://purl.org/procurement/public-contracts#Contract> ;
  rdfs:range xsd:float ;
  rdfs:label "percRibasso" ;
  rdfs:comment "The property that determines the declared percentage of price cut."@en .
 

<http://purl.org/procurement/public-contracts#startDate>
  rdfs:domain <http://purl.org/procurement/public-contracts#Contract>, <http://contrattipubblici.org/csi/Soglia> ;
  rdfs:range xsd:date .

<http://purl.org/procurement/public-contracts#estimatedEndDate>
  rdfs:domain <http://purl.org/procurement/public-contracts#Contract> ;
  rdfs:range xsd:date .

<http://contrattipubblici.org/csi/dataFineContrattuale>
  rdfs:domain <http://purl.org/procurement/public-contracts#Contract> ;
  rdfs:range xsd:float ;
  rdfs:label "dataFineContrattuale" ;
  rdfs:comment "The property that determines the end date declared in the Contract."@en .

<http://contrattipubblici.org/csi/importoProgetto>
  rdfs:domain <http://purl.org/procurement/public-contracts#Contract> ;
  rdfs:range xsd:float ;
  rdfs:label "importoProgetto" ;
  rdfs:comment "The property that determines the planning cost of the Contract."@en .

<http://contrattipubblici.org/csi/settoreSpeciale>
  rdfs:domain <http://purl.org/procurement/public-contracts#Contract>, <http://contrattipubblici.org/csi/Soglia> ;
  rdfs:range xsd:string ;
  rdfs:label "settoreSpeciale" ;
  rdfs:comment "The property that determines if the Contract deal with an area that is considered special by DLGS 163/2006 Art3."@en, "The property that determines whether or not the contract belong to a special sector."@en .

<http://contrattipubblici.org/csi/previstoSubappalto>
  rdfs:domain <http://purl.org/procurement/public-contracts#Contract> ;
  rdfs:range xsd:string ;
  rdfs:label "previstoSubappalto" ;
  rdfs:comment "The property that determines if a subcontract if expected in the Contract."@en .
  
<http://contrattipubblici.org/csi/ID>
  rdfs:domain <http://purl.org/procurement/public-contracts#Contract> ;
  rdfs:range xsd:int .

<http://purl.org/dc/terms#identifier>
  rdfs:domain <http://purl.org/procurement/public-contracts#Contract>, <http://contrattipubblici.org/csi/Cpv> ;
  rdfs:range xsd:string .
  
<http://contrattipubblici.org/csi/importoBaseAsta>
  rdfs:domain <http://purl.org/procurement/public-contracts#Contract> ;
  rdfs:range xsd:float ;
  rdfs:label "importoBaseAsta" ;
  rdfs:comment "The property that determines the auction base amount."@en .

<http://contrattipubblici.org/csi/congruenzaCPV>
  rdfs:domain <http://purl.org/procurement/public-contracts#Contract> ;
  rdfs:range xsd:float ;
  rdfs:label "congruenzaCPV" ;
  rdfs:comment "The property that determines if the declared CPV code is compatible with the declared contract type (work service or supply)."@en .
  
<http://contrattipubblici.org/csi/importoSicurezza>
  rdfs:domain <http://purl.org/procurement/public-contracts#Contract>, <http://contrattipubblici.org/csi/Bando> ;
  rdfs:range xsd:float ;
  rdfs:label "importoSicurezza" ;
  rdfs:comment "The property that determines the amount of money to be spent for safety reason in the contract."@en, "The property that determines the amount of money to be spent for security reason in the announcement."@en .

<http://contrattipubblici.org/csi/importoAggiudicazione>
  rdfs:domain <http://contrattipubblici.org/csi/Bando> ;
  rdfs:range xsd:float ;
  rdfs:label "importoAggiudicazione" ;
  owl:equivalentProperty <http://purl.org/procurement/public-contracts#agreedPrice> .

<http://contrattipubblici.org/csi/pubDate>
  rdfs:domain <http://contrattipubblici.org/csi/Bando> ;
  rdfs:range xsd:date ;
  rdfs:label "pubDate" ;
  rdfs:comment "The property that determines the publication date."@en .

<http://contrattipubblici.org/csi/winDate>
  rdfs:domain <http://contrattipubblici.org/csi/Bando> ;
  rdfs:range xsd:date ;
  rdfs:label "winDate" ;
  owl:equivalentProperty <http://purl.org/procurement/public-contracts#awardDate> .

<http://contrattipubblici.org/csi/expireDate>
  rdfs:domain <http://contrattipubblici.org/csi/Bando> ;
  rdfs:range xsd:date ;
  rdfs:label "expireDate" ;
  rdfs:comment "The property that determines the expire date."@en .

  <http://contrattipubblici.org/csi/validityEndDate> rdf:type owl:DatatypeProperty ;
  rdfs:domain <http://contrattipubblici.org/csi/Threshold> ;
  rdfs:range xsd:date;
  rdfs:comment "La proprietà che determina la data di cessazionedi validità della soglia comunitaria."@it ,
 "The property that determines the validity end date of a threshold." @en ;
  rdfs:label "Validity end date."@en ;
 rdfs:label "Data termine validita."@it .

  <http://contrattipubblici.org/csi/actualEndDate> rdf:type owl:DatatypeProperty ;
  rdfs:domain csi:Contract ;
  rdfs:range xsd:date ;
    rdfs:comment "Property for actual end date of public contract's realization."@en ,
   "Questa proprietà indica la data di effettiva realizzazione del contratto pubblico"@it ;
rdfs:label "Data effettiva termine lavoro"@it , 
 "Property for actual end date of public contract's realization."@en .



#################################################################
#    Classes
#################################################################

<http://purl.org/procurement/public-contracts#Contract> a owl:Class ;
rdfs:label "Contract" .

# XXX toglierei il domain di rdfs:label

<http://contrattipubblici.org/csi/Bando>
  a owl:Class ;
  rdfs:label "Bando" ;
  rdfs:comment "The class  that represents announcements."@en .

<http://contrattipubblici.org/csi/TipBando>
  a owl:Class ;
  rdfs:label "TipBando" ;
  rdfs:comment "The class that represents the announcement type."@en .

<http://contrattipubblici.org/csi/SceltaContraente>
  a owl:Class ;
  rdfs:label "SceltaContraente" ;
  rdfs:comment "The class that represents the type of procedure."@en .

<http://contrattipubblici.org/csi/MotivazioneVariante>
  a owl:Class ;
  rdfs:label "MotivazioneVariante" ;
  rdfs:comment "The class that represents the motivation of the variation of the contract."@en .

<http://contrattipubblici.org/csi/FrameworkAgreement>
  a owl:Class ;
  rdfs:label "Tipo di Aggiudicazione"@it ;
  rdfs:label "Framework Agreement"@en ;
  rdfs:comment "The class that represents the award type."@en .

<http://contrattipubblici.org/csi/TipContratto>
  a owl:Class ;
  rdfs:label "TipContratto" ;
  rdfs:comment "The class that represents the type of the contract (work service or supply)."@en .

<http://contrattipubblici.org/csi/EsitoBando>
  a owl:Class ;
  rdfs:label "EsitoBando" ;
  rdfs:comment "The class that represents the type final state of the announcement."@en .

<http://contrattipubblici.org/csi/NatGiuridica>
  a owl:Class ;
  rdfs:label "NatGiuridica" ;
  rdfs:comment "The class that represents the type of legal corporate entity."@en .

<http://contrattipubblici.org/csi/Cpv>
  a owl:Class ;
  rdfs:label "Cpv" ;
  rdfs:comment "The class that represents the Common Procurement Classification entity."@en .

<http://contrattipubblici.org/csi/Opera>
  a owl:Class ;
  rdfs:label "Opera" ;
  rdfs:comment "The class that represents the group of announcement called Opera."@en .

<http://contrattipubblici.org/csi/CUP>
  rdfs:domain <http://contrattipubblici.org/csi/Opera> ;
  rdfs:range xsd:string ;
  rdfs:label "CUP" ;
  rdfs:comment "The property that determines the cup (codice unico di procedura) code."@en .

<http://contrattipubblici.org/csi/Conto>
  a owl:Class ;
  rdfs:label "Conto" ;
  rdfs:comment "The class that represents the payment of a Contract"@en .

<http://reference.data.gov.uk/def/payment#netAmount>
  rdfs:domain <http://contrattipubblici.org/csi/Conto> ;
  rdfs:range xsd:float .

<http://purl.org/procurement/public-contracts#Tender> a owl:Class .
<http://purl.org/procurement/public-contracts#bidder>
  rdfs:domain <http://purl.org/procurement/public-contracts#Tender> ;
  rdfs:range gr:BusinessEntity .

<http://contrattipubblici.org/csi/Localizzazione>
  a owl:Class ;
  rdfs:label "Localizzazione" ;
  rdfs:comment "The class that represents the Localization of a Contract (pc:Contract), an announcement (csi:Bando) or an Opera (csi:Opera)"@en .

<http://contrattipubblici.org/csi/ciComune>
  rdfs:domain <http://contrattipubblici.org/csi/Localizzazione>, gr:BusinessEntity ;
  rdfs:label "ciComune" ;
  rdfs:comment "The property that determines the municipality code (codice Istat)."@en ;
  rdfs:range xsd:string .

<http://contrattipubblici.org/csi/NUTS>
  rdfs:domain <http://contrattipubblici.org/csi/Localizzazione> ;
  rdfs:label "NUTS" ;
  rdfs:comment "The property that determines the NUTS code."@en ;
  rdfs:range xsd:string .

<http://contrattipubblici.org/csi/Programmazione>
  a owl:Class ;
  rdfs:label "Programmazione" ;
  rdfs:comment "The class that represents the group of csi:Opera that belongs to the same 'programmazione'."@en .

<http://contrattipubblici.org/csi/haOpera>
  rdfs:domain <http://contrattipubblici.org/csi/Programmazione> ;
  rdfs:label "haOpera" ;
  rdfs:comment "The property that determines the relation of csi:Opera and csi:Programmazione."@en ;
  rdfs:range <http://contrattipubblici.org/csi/Opera> .

<http://contrattipubblici.org/csi/Subappalto>
  a owl:Class ;
  rdfs:label "Subappalto" ;
  rdfs:comment "The class that represents a subcontract."@en .

<http://contrattipubblici.org/csi/importoPresunto>
  rdfs:domain <http://contrattipubblici.org/csi/subappalto> ;
  rdfs:label "importoPresunto" ;
  rdfs:comment "The property that determines the estimated amount of money."@en ;
  rdfs:range xsd:float .

<http://contrattipubblici.org/csi/haSubappaltatrice>
  rdfs:domain <http://contrattipubblici.org/csi/subappalto> ;
  rdfs:range gr:BusinessEntity ;
  rdfs:label "haSubappaltatrice" ;
  rdfs:comment "The property that determines the business entity that sign the subcontract."@en .

<http://contrattipubblici.org/csi/Threshold>
  a owl:Class ;
  rdfs:label "Soglia"@it ;
  rdfs:label "Threshold"@en ;
  rdfs:comment "The class that represents the price threshold of a contract."@en .
  rdfs:comment "La classe che rappresenta la soglia di prezzo di un Contratto."@it .


gr:BusinessEntity a owl:Class .
<http://purl.org/dc/terms#identifiers>
  rdfs:domain gr:BusinessEntity ;
  rdfs:range xsd:string .

<http://contrattipubblici.org/csi/codNat>
  rdfs:domain gr:BusinessEntity ;
  rdfs:range <http://contrattipubblici.org/csi/NatGiuridica> .

<http://contrattipubblici.org/csi/Variante>
  a owl:Class ;
  rdfs:label "Variante" ;
  rdfs:comment "The class that represents a contract variation."@en .

<http://contrattipubblici.org/csi/haMotivazione>
  rdfs:domain <http://contrattipubblici.org/csi/Variante> ;
  rdfs:range <http://contrattipubblici.org/csi/MotivazioneVariante> ;
  rdfs:label "haMotivazione" ;
  rdfs:comment "The property that links the contract variation and the related motivation."@en .

<http://contrattipubblici.org/csi/variationType>
  rdfs:domain <http://contrattipubblici.org/csi/Variante> ;
  rdfs:range xsd:string ;
  rdfs:label "tipo variante" @it ,
  "variation type" @en ;
  rdfs:comment "The property that determines contract variation type."@en .

<http://contrattipubblici.org/csi/additionalDays>
  rdfs:domain <http://contrattipubblici.org/csi/Variante> ;
  rdfs:range xsd:float ;
  rdfs:label "giorni aggiuntivi" @it ;
  rdfs:label "additional days" @en ;
  rdfs:comment "The property that determines additional days needed in the variation."@en .
  rdfs:comment "Questa proprietà indica i giorni aggiuntivi necessari per la variante." @it.

