<rdf:RDF xmlns="https://w3id.org/italia/onto/SM/" xmlns:CLV="https://w3id.org/italia/onto/CLV/" xmlns:admsapit="https://w3id.org/italia/onto/ADMS/" xmlns:covapit="https://w3id.org/italia/onto/COV/" xmlns:dc="http://purl.org/dc/elements/1.1/" xmlns:dcat="http://www.w3.org/ns/dcat#" xmlns:dcatapit="http://dati.gov.it/onto/dcatapit#" xmlns:dct="http://purl.org/dc/terms/" xmlns:foaf="http://xmlns.com/foaf/0.1/" xmlns:l0="https://w3id.org/italia/onto/l0/" xmlns:owl="http://www.w3.org/2002/07/owl#" xmlns:prov="http://www.w3.org/ns/prov#" xmlns:rdf="http://www.w3.org/1999/02/22-rdf-syntax-ns#" xmlns:rdfs="http://www.w3.org/2000/01/rdf-schema#" xmlns:skos="http://www.w3.org/2004/02/skos/core#" xmlns:vcard="http://www.w3.org/2006/vcard/ns#" xmlns:xsd="http://www.w3.org/2001/XMLSchema#" xml:base="https://w3id.org/italia/onto/SM/">
    <owl:Ontology rdf:about="https://w3id.org/italia/onto/SM">
        <owl:versionIRI rdf:resource="https://w3id.org/italia/onto/SM/0.7"></owl:versionIRI>
        <owl:imports rdf:resource="https://w3id.org/italia/onto/AccessCondition"></owl:imports>
        <owl:imports rdf:resource="https://w3id.org/italia/onto/POI"></owl:imports>
        <owl:imports rdf:resource="https://w3id.org/italia/onto/l0"></owl:imports>
        <dct:accrualPeriodicity rdf:resource="http://publications.europa.eu/resource/authority/frequency/IRREG"></dct:accrualPeriodicity>
        <dct:creator rdf:resource="http://spcdata.digitpa.gov.it/browse/page/Amministrazione/agid"></dct:creator>
        <dct:creator rdf:resource="https://w3id.org/italia/data/organization/support-unit/cnr-Z6HZEH/stlab"></dct:creator>
        <dct:description xml:lang="it">L'ontologia per i social media, i punti di contatto e internet. Questa ontologia permette di rappresentare social network, account, post, review, rating, indirizzi email, loghi, , punti di contatto, ecc...</dct:description>
        <dct:description xml:lang="en">The ontology for Social Media, contacts and internet. This ontology allows to represents social networks, account, email addresses, logos, points of contact etc.</dct:description>
        <dct:identifier>https://w3id.org/italia/onto/SM</dct:identifier>
        <dct:issued rdf:datatype="http://www.w3.org/2001/XMLSchema#date">2017-09-29</dct:issued>
        <dct:language rdf:resource="http://publications.europa.eu/resource/authority/language/ENG"></dct:language>
        <dct:language rdf:resource="http://publications.europa.eu/resource/authority/language/ITA"></dct:language>
        <dct:modified rdf:datatype="http://www.w3.org/2001/XMLSchema#date">2019-04-24</dct:modified>
        <dct:publisher rdf:resource="http://spcdata.digitpa.gov.it/browse/page/Amministrazione/agid"></dct:publisher>
        <dct:rightsHolder rdf:resource="http://spcdata.digitpa.gov.it/browse/page/Amministrazione/agid"></dct:rightsHolder>
        <dct:title xml:lang="it">Ontologia per i social media / contatti e internet - Profilo applicativo italiano</dct:title>
        <dct:title xml:lang="en">Social Media / Contact and Internet ontology - Italian Application Profile</dct:title>
        <rdfs:comment xml:lang="it">L'ontologia per i social media, i punti di contatto e internet. Questa ontologia permette di rappresentare social network, account, post, review, rating, indirizzi email, loghi, punti di contatto, ecc...</rdfs:comment>
        <rdfs:comment xml:lang="en">The ontology for Social Media contact and internet. This ontology allows to represents social networks, account, email addresses, logos, points of contact, etc.</rdfs:comment>
        <rdfs:label xml:lang="it">Ontologia per i social media / contatti e Internet</rdfs:label>
        <rdfs:label xml:lang="en">Social Media / Contact and Internet ontology</rdfs:label>
        <owl:versionInfo xml:lang="en">Version 0.7 - change of super class of TelephoneType and EmailType; New title of the ontology; Introduction of Contact Point generic class specialized in Physical and Online Contact Point. Introduction of the object property available that connects a contact point with access conditions. Changed the restrictions in UserAccount </owl:versionInfo>
        <owl:versionInfo xml:lang="it">Versione 0.7 - cambiata la super classe per TelephoneType e EmailType; cambiato il titolo dell'ontologia; introduzione del concetto di punto di contatto specializzato in fisico e online. Introduzione della proprietà disponibilità che collega un punto di contatto con le condizioni di accesso. Cambiate alcune restrizione per l'Account utente</owl:versionInfo>
        <dcat:contactPoint rdf:resource="https://w3id.org/italia/data/contact-point/onto-agid"></dcat:contactPoint>
        <dcat:keyword xml:lang="it">internet</dcat:keyword>
        <dcat:keyword xml:lang="it">post</dcat:keyword>
        <dcat:keyword xml:lang="it">punto di contatto</dcat:keyword>
        <dcat:keyword xml:lang="it">recensioni</dcat:keyword>
        <dcat:keyword xml:lang="it">social media</dcat:keyword>
        <dcat:theme rdf:resource="http://publications.europa.eu/resource/authority/data-theme/TECH"></dcat:theme>
        <prov:wasDerivedFrom rdf:resource="https://w3id.org/italia/onto/SM/0.6"></prov:wasDerivedFrom>
        <admsapit:acronym>SM-AP_IT</admsapit:acronym>
        <admsapit:hasContributor rdf:resource="https://w3id.org/italia/data/organization/public-organization/td"></admsapit:hasContributor>
        <admsapit:hasFormalityLevel rdf:resource="https://w3id.org/italia/onto/ADMS/Formal"></admsapit:hasFormalityLevel>
        <admsapit:hasKeyClass rdf:resource="https://w3id.org/italia/onto/SM/Email"></admsapit:hasKeyClass>
        <admsapit:hasKeyClass rdf:resource="https://w3id.org/italia/onto/SM/OnlineContactPoint"></admsapit:hasKeyClass>
        <admsapit:hasKeyClass rdf:resource="https://w3id.org/italia/onto/SM/Post"></admsapit:hasKeyClass>
        <admsapit:hasKeyClass rdf:resource="https://w3id.org/italia/onto/SM/SocialMedia"></admsapit:hasKeyClass>
        <admsapit:hasKeyClass rdf:resource="https://w3id.org/italia/onto/SM/WebSite"></admsapit:hasKeyClass>
        <admsapit:hasOntologyLanguage rdf:resource="https://w3id.org/italia/onto/ADMS/OWL"></admsapit:hasOntologyLanguage>
        <admsapit:hasSemanticAssetDistribution rdf:resource="https://w3id.org/italia/data/distribution/SMAPIT-JSON-LD"></admsapit:hasSemanticAssetDistribution>
        <admsapit:hasSemanticAssetDistribution rdf:resource="https://w3id.org/italia/data/distribution/SMAPIT-RDF-TURTLE"></admsapit:hasSemanticAssetDistribution>
        <admsapit:hasSemanticAssetDistribution rdf:resource="https://w3id.org/italia/data/distribution/SMAPIT-RDF-XML"></admsapit:hasSemanticAssetDistribution>
        <admsapit:hasTask rdf:resource="https://w3id.org/italia/onto/ADMS/AnnotationTask"></admsapit:hasTask>
        <admsapit:hasTask rdf:resource="https://w3id.org/italia/onto/ADMS/QueryFormulationTask"></admsapit:hasTask>
        <admsapit:hasTask rdf:resource="https://w3id.org/italia/onto/ADMS/SearchTask"></admsapit:hasTask>
        <admsapit:last rdf:resource="https://w3id.org/italia/onto/SM/0.7"></admsapit:last>
        <admsapit:officialURI rdf:datatype="http://www.w3.org/2001/XMLSchema#anyURI">https://w3id.org/italia/onto/SM</admsapit:officialURI>
        <admsapit:prefix>smapit</admsapit:prefix>
        <admsapit:prev rdf:resource="https://w3id.org/italia/onto/SM/0.6"></admsapit:prev>
        <admsapit:semanticAssetInUse rdf:resource="https://w3id.org/italia/data/project/DAF"></admsapit:semanticAssetInUse>
        <admsapit:semanticAssetInUse rdf:resource="https://w3id.org/italia/data/project/OntoPiA"></admsapit:semanticAssetInUse>
        <admsapit:status>catalogued</admsapit:status>
        <admsapit:status>published</admsapit:status>
        <admsapit:target>Cittadini</admsapit:target>
        <admsapit:target>Imprese</admsapit:target>
        <admsapit:target>Pubbliche Amministrazioni</admsapit:target>
        <admsapit:type rdf:resource="https://w3id.org/italia/onto/ADMS/ServiceOntology"></admsapit:type>
    </owl:Ontology>



    <!--
    ///////////////////////////////////////////////////////////////////////////////////////
    //
    // Annotation properties
    //
    ///////////////////////////////////////////////////////////////////////////////////////
     -->




    <!-- http://purl.org/dc/terms/description -->

    <owl:AnnotationProperty rdf:about="http://purl.org/dc/terms/description"></owl:AnnotationProperty>



    <!-- http://purl.org/dc/terms/format -->

    <owl:AnnotationProperty rdf:about="http://purl.org/dc/terms/format"></owl:AnnotationProperty>



    <!-- http://purl.org/dc/terms/identifier -->

    <owl:AnnotationProperty rdf:about="http://purl.org/dc/terms/identifier"></owl:AnnotationProperty>



    <!-- http://purl.org/dc/terms/license -->

    <owl:AnnotationProperty rdf:about="http://purl.org/dc/terms/license"></owl:AnnotationProperty>



    <!-- http://purl.org/dc/terms/title -->

    <owl:AnnotationProperty rdf:about="http://purl.org/dc/terms/title"></owl:AnnotationProperty>



    <!-- http://www.w3.org/2006/vcard/ns#fn -->

    <owl:AnnotationProperty rdf:about="http://www.w3.org/2006/vcard/ns#fn"></owl:AnnotationProperty>



    <!-- http://www.w3.org/2006/vcard/ns#hasEmail -->

    <owl:AnnotationProperty rdf:about="http://www.w3.org/2006/vcard/ns#hasEmail"></owl:AnnotationProperty>



    <!-- http://www.w3.org/ns/dcat#accessURL -->

    <owl:AnnotationProperty rdf:about="http://www.w3.org/ns/dcat#accessURL"></owl:AnnotationProperty>



    <!-- http://www.w3.org/ns/dcat#downloadURL -->

    <owl:AnnotationProperty rdf:about="http://www.w3.org/ns/dcat#downloadURL"></owl:AnnotationProperty>



    <!-- http://www.w3.org/ns/prov#wasDerivedFrom -->

    <owl:AnnotationProperty rdf:about="http://www.w3.org/ns/prov#wasDerivedFrom"></owl:AnnotationProperty>



    <!-- http://www.w3.org/ns/prov#wasInfluencedBy -->

    <owl:AnnotationProperty rdf:about="http://www.w3.org/ns/prov#wasInfluencedBy"></owl:AnnotationProperty>



    <!-- http://xmlns.com/foaf/0.1/name -->

    <owl:AnnotationProperty rdf:about="http://xmlns.com/foaf/0.1/name"></owl:AnnotationProperty>



    <!-- https://w3id.org/italia/onto/ADMS/prev -->

    <owl:AnnotationProperty rdf:about="https://w3id.org/italia/onto/ADMS/prev"></owl:AnnotationProperty>



    <!-- https://w3id.org/italia/onto/ADMS/status -->

    <owl:AnnotationProperty rdf:about="https://w3id.org/italia/onto/ADMS/status"></owl:AnnotationProperty>



    <!--
    ///////////////////////////////////////////////////////////////////////////////////////
    //
    // Object Properties
    //
    ///////////////////////////////////////////////////////////////////////////////////////
     -->




    <!-- https://w3id.org/italia/onto/SM#hasReview -->

    <owl:ObjectProperty rdf:about="https://w3id.org/italia/onto/SM/hasReview">
        <rdfs:domain rdf:resource="http://www.w3.org/2002/07/owl#Thing"></rdfs:domain>
        <rdfs:range rdf:resource="https://w3id.org/italia/onto/SM/Review"></rdfs:range>
        <rdfs:comment xml:lang="en">Property that links a thing of the modelled domain to a review</rdfs:comment>
        <rdfs:comment xml:lang="it">Proprietà che collega qualsiasi cosa del dominio modellato a una recensione</rdfs:comment>
        <rdfs:isDefinedBy rdf:resource="https://w3id.org/italia/onto/SM"></rdfs:isDefinedBy>
        <rdfs:label xml:lang="it">ha recensione</rdfs:label>
        <rdfs:label xml:lang="en">has review</rdfs:label>
        <owl:versionInfo xml:lang="it">stabile</owl:versionInfo>
        <owl:versionInfo xml:lang="en">stable</owl:versionInfo>
    </owl:ObjectProperty>



    <!-- https://w3id.org/italia/onto/SM/available -->

    <owl:ObjectProperty rdf:about="https://w3id.org/italia/onto/SM/available">
        <rdfs:domain rdf:resource="https://w3id.org/italia/onto/SM/ContactPoint"></rdfs:domain>
        <rdfs:range rdf:resource="https://w3id.org/italia/onto/AccessCondition/AccessCondition"></rdfs:range>
        <rdfs:comment xml:lang="en">Property used to represent the availability of a contact point. It is through this property that is possibile to express opening hours of a specific contact point</rdfs:comment>
        <rdfs:comment xml:lang="it">Proprietà utilizzata per rappresentare la disponibilità del punto di contatto. E' attraverso questa proprietà che possono essere specificati gli orari di apertura del punto di contatto.</rdfs:comment>
        <rdfs:isDefinedBy rdf:resource="https://w3id.org/italia/onto/SM"></rdfs:isDefinedBy>
        <rdfs:label xml:lang="en">contact point available</rdfs:label>
        <rdfs:label xml:lang="it">punto di contatto disponibile</rdfs:label>
        <owl:versionInfo xml:lang="it">stabile</owl:versionInfo>
        <owl:versionInfo xml:lang="en">stable</owl:versionInfo>
    </owl:ObjectProperty>



    <!-- https://w3id.org/italia/onto/SM/hasCertifiedEmail -->

    <owl:ObjectProperty rdf:about="https://w3id.org/italia/onto/SM/hasCertifiedEmail">
        <rdfs:subPropertyOf rdf:resource="https://w3id.org/italia/onto/SM/hasEmail"></rdfs:subPropertyOf>
    </owl:ObjectProperty>



    <!-- https://w3id.org/italia/onto/SM/hasContactPoint -->

    <owl:ObjectProperty rdf:about="https://w3id.org/italia/onto/SM/hasContactPoint">
        <rdfs:domain rdf:resource="http://www.w3.org/2002/07/owl#Thing"></rdfs:domain>
        <rdfs:range rdf:resource="https://w3id.org/italia/onto/SM/ContactPoint"></rdfs:range>
        <rdfs:comment xml:lang="en">Property that allows one to specify a contact point for a thing.</rdfs:comment>
        <rdfs:comment xml:lang="it">Proprietà che consente di specificare un punto di contatto associato a una cosa del dominio modellato.</rdfs:comment>
        <rdfs:isDefinedBy rdf:resource="https://w3id.org/italia/onto/SM"></rdfs:isDefinedBy>
        <rdfs:label xml:lang="it">ha punto di contatto</rdfs:label>
        <rdfs:label xml:lang="en">has contact point</rdfs:label>
        <owl:versionInfo xml:lang="it">stabile</owl:versionInfo>
        <owl:versionInfo xml:lang="en">stable</owl:versionInfo>
    </owl:ObjectProperty>



    <!-- https://w3id.org/italia/onto/SM/hasCreator -->

    <owl:ObjectProperty rdf:about="https://w3id.org/italia/onto/SM/hasCreator">
        <rdfs:subPropertyOf rdf:resource="http://www.w3.org/2002/07/owl#topObjectProperty"></rdfs:subPropertyOf>
        <owl:inverseOf rdf:resource="https://w3id.org/italia/onto/SM/isCreatorOf"></owl:inverseOf>
        <rdfs:domain rdf:resource="https://w3id.org/italia/onto/SM/Post"></rdfs:domain>
        <rdfs:range rdf:resource="https://w3id.org/italia/onto/SM/UserAccount"></rdfs:range>
        <rdfs:comment xml:lang="it">Questa proprietà asserisce che un post è stato creato da un certo account utente.</rdfs:comment>
        <rdfs:comment xml:lang="en">This property states that a post has been created by a certain user account.</rdfs:comment>
        <rdfs:isDefinedBy rdf:resource="https://w3id.org/italia/onto/SM"></rdfs:isDefinedBy>
        <rdfs:label xml:lang="it">ha autore</rdfs:label>
        <rdfs:label xml:lang="en">has creator</rdfs:label>
        <prov:wasInfluencedBy rdf:resource="http://rdfs.org/sioc/ns"></prov:wasInfluencedBy>
    </owl:ObjectProperty>



    <!-- https://w3id.org/italia/onto/SM/hasEmail -->

    <owl:ObjectProperty rdf:about="https://w3id.org/italia/onto/SM/hasEmail">
        <owl:inverseOf rdf:resource="https://w3id.org/italia/onto/SM/isEmailOf"></owl:inverseOf>
        <rdfs:domain rdf:resource="https://w3id.org/italia/onto/SM/OnlineContactPoint"></rdfs:domain>
        <rdfs:range rdf:resource="https://w3id.org/italia/onto/SM/Email"></rdfs:range>
        <rdfs:comment xml:lang="it">Questa proprietà collega un punto di contatto online con uno o più indirizzi email di vario tipo.</rdfs:comment>
        <rdfs:comment xml:lang="en">This property links an online contact  point with one or more email addresses of various types.</rdfs:comment>
        <rdfs:isDefinedBy rdf:resource="https://w3id.org/italia/onto/SM"></rdfs:isDefinedBy>
        <rdfs:label xml:lang="it">ha email</rdfs:label>
        <rdfs:label xml:lang="en">has email</rdfs:label>
    </owl:ObjectProperty>



    <!-- https://w3id.org/italia/onto/SM/hasEmailType -->

    <owl:ObjectProperty rdf:about="https://w3id.org/italia/onto/SM/hasEmailType">
        <owl:inverseOf rdf:resource="https://w3id.org/italia/onto/SM/isEmailTypeOf"></owl:inverseOf>
        <rdf:type rdf:resource="http://www.w3.org/2002/07/owl#FunctionalProperty"></rdf:type>
        <rdfs:domain rdf:resource="https://w3id.org/italia/onto/SM/Email"></rdfs:domain>
        <rdfs:range rdf:resource="https://w3id.org/italia/onto/SM/EmailType"></rdfs:range>
        <rdfs:comment xml:lang="it">Questa proprietà collega l'email al suo tipo.</rdfs:comment>
        <rdfs:comment xml:lang="en">This property links the Email to its type.</rdfs:comment>
        <rdfs:isDefinedBy rdf:resource="https://w3id.org/italia/onto/SM"></rdfs:isDefinedBy>
        <rdfs:label xml:lang="it">ha tipo email</rdfs:label>
        <rdfs:label xml:lang="en">has email type</rdfs:label>
    </owl:ObjectProperty>



    <!-- https://w3id.org/italia/onto/SM/hasImage -->

    <owl:ObjectProperty rdf:about="https://w3id.org/italia/onto/SM/hasImage">
        <owl:inverseOf rdf:resource="https://w3id.org/italia/onto/SM/isImageOf"></owl:inverseOf>
        <rdfs:domain rdf:resource="http://www.w3.org/2002/07/owl#Thing"></rdfs:domain>
        <rdfs:range rdf:resource="https://w3id.org/italia/onto/SM/Image"></rdfs:range>
        <rdfs:comment xml:lang="it">Questa proprietà collega qualsiasi cosa ad un'immagine.</rdfs:comment>
        <rdfs:comment xml:lang="en">This property links anything to an image.</rdfs:comment>
        <rdfs:isDefinedBy rdf:resource="https://w3id.org/italia/onto/SM"></rdfs:isDefinedBy>
        <rdfs:label xml:lang="it">ha immagine</rdfs:label>
        <rdfs:label xml:lang="en">has image</rdfs:label>
    </owl:ObjectProperty>



    <!-- https://w3id.org/italia/onto/SM/hasOnlineContactPoint -->

    <owl:ObjectProperty rdf:about="https://w3id.org/italia/onto/SM/hasOnlineContactPoint">
        <rdfs:subPropertyOf rdf:resource="https://w3id.org/italia/onto/SM/hasContactPoint"></rdfs:subPropertyOf>
        <owl:inverseOf rdf:resource="https://w3id.org/italia/onto/SM/isOnlineContactPointOf"></owl:inverseOf>
        <rdfs:domain rdf:resource="http://www.w3.org/2002/07/owl#Thing"></rdfs:domain>
        <rdfs:range rdf:resource="https://w3id.org/italia/onto/SM/OnlineContactPoint"></rdfs:range>
        <rdfs:comment xml:lang="it">Questa proprietà lega qualsiasi cosa del dominio modellato a un punto di contatto online.</rdfs:comment>
        <rdfs:comment xml:lang="en">This property links any thing of the domain being modelled with the online contact point.</rdfs:comment>
        <rdfs:label xml:lang="it">ha punto di contatto online</rdfs:label>
        <rdfs:label xml:lang="en">has online contact point</rdfs:label>
        <owl:versionInfo xml:lang="it">stabile</owl:versionInfo>
    </owl:ObjectProperty>



    <!-- https://w3id.org/italia/onto/SM/hasPhysicalContactPoint -->

    <owl:ObjectProperty rdf:about="https://w3id.org/italia/onto/SM/hasPhysicalContactPoint">
        <rdfs:subPropertyOf rdf:resource="https://w3id.org/italia/onto/SM/hasContactPoint"></rdfs:subPropertyOf>
        <rdfs:domain rdf:resource="http://www.w3.org/2002/07/owl#Thing"></rdfs:domain>
        <rdfs:range rdf:resource="https://w3id.org/italia/onto/SM/PhysicalContactPoint"></rdfs:range>
        <rdfs:comment xml:lang="en">Property used to associate a physical contact point to any thing.</rdfs:comment>
        <rdfs:comment xml:lang="it">Proprietà utilizzata per associare un contatto fisico a una qualunque cosa del dominio modellato</rdfs:comment>
        <rdfs:isDefinedBy rdf:resource="https://w3id.org/italia/onto/SM"></rdfs:isDefinedBy>
        <rdfs:label xml:lang="it">ha punto di contatto fisico</rdfs:label>
        <rdfs:label xml:lang="en">has physical contact point</rdfs:label>
        <owl:versionInfo xml:lang="it">stabile</owl:versionInfo>
        <owl:versionInfo xml:lang="en">stable</owl:versionInfo>
    </owl:ObjectProperty>



    <!-- https://w3id.org/italia/onto/SM/hasRating -->

    <owl:ObjectProperty rdf:about="https://w3id.org/italia/onto/SM/hasRating">
        <rdfs:domain rdf:resource="http://www.w3.org/2002/07/owl#Thing"></rdfs:domain>
        <rdfs:range rdf:resource="https://w3id.org/italia/onto/SM/Rating"></rdfs:range>
        <rdfs:comment xml:lang="en">Property that links anything to a possible rating.</rdfs:comment>
        <rdfs:comment xml:lang="it">Proprietà che collega qualsiasi cosa a una possibile valutazione generale.</rdfs:comment>
        <rdfs:isDefinedBy rdf:resource="https://w3id.org/italia/onto/SM"></rdfs:isDefinedBy>
        <rdfs:label xml:lang="it">ha valutazione</rdfs:label>
        <rdfs:label xml:lang="en">has rating</rdfs:label>
        <owl:versionInfo xml:lang="it">stabile</owl:versionInfo>
        <owl:versionInfo xml:lang="en">stable</owl:versionInfo>
    </owl:ObjectProperty>



    <!-- https://w3id.org/italia/onto/SM/hasReply -->

    <owl:ObjectProperty rdf:about="https://w3id.org/italia/onto/SM/hasReply">
        <rdfs:subPropertyOf rdf:resource="http://www.w3.org/2002/07/owl#topObjectProperty"></rdfs:subPropertyOf>
        <owl:inverseOf rdf:resource="https://w3id.org/italia/onto/SM/isReplyOf"></owl:inverseOf>
        <rdfs:domain rdf:resource="https://w3id.org/italia/onto/SM/Post"></rdfs:domain>
        <rdfs:range rdf:resource="https://w3id.org/italia/onto/SM/Post"></rdfs:range>
        <rdfs:comment xml:lang="it">La proprietà 'ha risposta' permette di dire che un post ha una risposta, ovvero, permette di creare thread di post ed organizzarla in una struttura ad albero.</rdfs:comment>
        <rdfs:comment xml:lang="en">This property links an Item to other follow-up content Items made on the same topic. Use of this property can result in a single branch of replies from the original Item, or in a tree-like structure with branches forking at different Items along the way.</rdfs:comment>
        <rdfs:isDefinedBy rdf:resource="https://w3id.org/italia/onto/SM"></rdfs:isDefinedBy>
        <rdfs:label xml:lang="it">ha risposta</rdfs:label>
        <rdfs:label xml:lang="en">has reply</rdfs:label>
        <prov:wasInfluencedBy rdf:resource="http://rdfs.org/sioc/ns#has_reply"></prov:wasInfluencedBy>
    </owl:ObjectProperty>



    <!-- https://w3id.org/italia/onto/SM/hasTelephone -->

    <owl:ObjectProperty rdf:about="https://w3id.org/italia/onto/SM/hasTelephone">
        <owl:inverseOf rdf:resource="https://w3id.org/italia/onto/SM/isTelephoneOf"></owl:inverseOf>
        <rdfs:domain rdf:resource="https://w3id.org/italia/onto/SM/OnlineContactPoint"></rdfs:domain>
        <rdfs:range rdf:resource="https://w3id.org/italia/onto/SM/Telephone"></rdfs:range>
        <rdfs:comment xml:lang="it">Questa proprietà collega un punto di contatto online con il telefono.</rdfs:comment>
        <rdfs:comment xml:lang="en">This property links the online contact point with the telephone element</rdfs:comment>
        <rdfs:isDefinedBy rdf:resource="https://w3id.org/italia/onto/SM"></rdfs:isDefinedBy>
        <rdfs:label xml:lang="it">ha telefono</rdfs:label>
        <rdfs:label xml:lang="en">has telephone</rdfs:label>
        <owl:versionInfo xml:lang="it">stabile</owl:versionInfo>
        <owl:versionInfo xml:lang="en">stable</owl:versionInfo>
    </owl:ObjectProperty>



    <!-- https://w3id.org/italia/onto/SM/hasTelephoneType -->

    <owl:ObjectProperty rdf:about="https://w3id.org/italia/onto/SM/hasTelephoneType">
        <owl:inverseOf rdf:resource="https://w3id.org/italia/onto/SM/isTelephoneTypeOf"></owl:inverseOf>
        <rdf:type rdf:resource="http://www.w3.org/2002/07/owl#FunctionalProperty"></rdf:type>
        <rdfs:domain rdf:resource="https://w3id.org/italia/onto/SM/Telephone"></rdfs:domain>
        <rdfs:range rdf:resource="https://w3id.org/italia/onto/SM/TelephoneType"></rdfs:range>
        <rdfs:comment xml:lang="it">Questa proprietà lega un telefono al suo tipo (voce, fax).</rdfs:comment>
        <rdfs:comment xml:lang="en">This property links the Telephone to its type (voice, fax)</rdfs:comment>
        <rdfs:isDefinedBy rdf:resource="https://w3id.org/italia/onto/SM"></rdfs:isDefinedBy>
        <rdfs:label xml:lang="it">ha tipo di telefono</rdfs:label>
        <rdfs:label xml:lang="en">has telephone type</rdfs:label>
        <owl:versionInfo xml:lang="it">stabile</owl:versionInfo>
        <owl:versionInfo xml:lang="en">stable</owl:versionInfo>
    </owl:ObjectProperty>



    <!-- https://w3id.org/italia/onto/SM/hasUserAccount -->

    <owl:ObjectProperty rdf:about="https://w3id.org/italia/onto/SM/hasUserAccount">
        <rdfs:subPropertyOf rdf:resource="http://www.w3.org/2002/07/owl#topObjectProperty"></rdfs:subPropertyOf>
        <owl:inverseOf rdf:resource="https://w3id.org/italia/onto/SM/isUserAccountOf"></owl:inverseOf>
        <rdfs:domain rdf:resource="https://w3id.org/italia/onto/SM/OnlineContactPoint"></rdfs:domain>
        <rdfs:range rdf:resource="https://w3id.org/italia/onto/SM/UserAccount"></rdfs:range>
        <rdfs:comment xml:lang="it">Questa proprietà collega un punto di contatto online al suo account utente.</rdfs:comment>
        <rdfs:comment xml:lang="en">This property links an online contactPoint to its user account.</rdfs:comment>
        <rdfs:isDefinedBy rdf:resource="https://w3id.org/italia/onto/SM"></rdfs:isDefinedBy>
        <rdfs:label xml:lang="it">ha account utente</rdfs:label>
        <rdfs:label xml:lang="en">has user account</rdfs:label>
    </owl:ObjectProperty>



    <!-- https://w3id.org/italia/onto/SM/hasWebSite -->

    <owl:ObjectProperty rdf:about="https://w3id.org/italia/onto/SM/hasWebSite">
        <owl:inverseOf rdf:resource="https://w3id.org/italia/onto/SM/isWebSiteOf"></owl:inverseOf>
        <rdfs:domain rdf:resource="http://www.w3.org/2002/07/owl#Thing"></rdfs:domain>
        <rdfs:range rdf:resource="https://w3id.org/italia/onto/SM/WebSite"></rdfs:range>
        <rdfs:comment xml:lang="en">Relation between anything and its web site.</rdfs:comment>
        <rdfs:comment xml:lang="it">Relazione tra una qualsiasi entità e la sua pagina Web.</rdfs:comment>
        <rdfs:isDefinedBy rdf:resource="https://w3id.org/italia/onto/SM"></rdfs:isDefinedBy>
        <rdfs:label xml:lang="it">ha pagina Web</rdfs:label>
        <rdfs:label xml:lang="en">has Web site</rdfs:label>
    </owl:ObjectProperty>



    <!-- https://w3id.org/italia/onto/SM/isAccountIssuedBy -->

    <owl:ObjectProperty rdf:about="https://w3id.org/italia/onto/SM/isAccountIssuedBy">
        <owl:inverseOf rdf:resource="https://w3id.org/italia/onto/SM/issuesAccount"></owl:inverseOf>
        <rdfs:domain rdf:resource="https://w3id.org/italia/onto/SM/UserAccount"></rdfs:domain>
        <rdfs:range rdf:resource="https://w3id.org/italia/onto/SM/SocialMedia"></rdfs:range>
        <rdfs:comment xml:lang="it">Questa proprietà rappresenta la relazione tra un social media e gli account utenti che sono stati rilasciati su tale media.</rdfs:comment>
        <rdfs:comment xml:lang="en">This property represents the relation between a social media and the user account issued by such a social media.</rdfs:comment>
        <rdfs:isDefinedBy rdf:resource="https://w3id.org/italia/onto/SM"></rdfs:isDefinedBy>
        <rdfs:label xml:lang="en">is account issued by</rdfs:label>
        <rdfs:label xml:lang="it">è account rilasciato da</rdfs:label>
    </owl:ObjectProperty>



    <!-- https://w3id.org/italia/onto/SM/isCreatorOf -->

    <owl:ObjectProperty rdf:about="https://w3id.org/italia/onto/SM/isCreatorOf">
        <rdfs:domain rdf:resource="https://w3id.org/italia/onto/SM/UserAccount"></rdfs:domain>
        <rdfs:range rdf:resource="https://w3id.org/italia/onto/SM/Post"></rdfs:range>
        <rdfs:comment xml:lang="it">La relazione che permette di asserire che un account utente ha creato un certo post.</rdfs:comment>
        <rdfs:comment xml:lang="en">The fact that a user account creates a post.</rdfs:comment>
        <rdfs:isDefinedBy rdf:resource="https://w3id.org/italia/onto/SM"></rdfs:isDefinedBy>
        <rdfs:label xml:lang="en">is creator of</rdfs:label>
        <rdfs:label xml:lang="it">è autore di</rdfs:label>
        <prov:wasInfluencedBy rdf:resource="http://rdfs.org/sioc/ns"></prov:wasInfluencedBy>
    </owl:ObjectProperty>



    <!-- https://w3id.org/italia/onto/SM/isEmailOf -->

    <owl:ObjectProperty rdf:about="https://w3id.org/italia/onto/SM/isEmailOf">
        <rdfs:subPropertyOf rdf:resource="http://www.w3.org/2002/07/owl#topObjectProperty"></rdfs:subPropertyOf>
        <rdfs:domain rdf:resource="https://w3id.org/italia/onto/SM/Email"></rdfs:domain>
        <rdfs:range rdf:resource="https://w3id.org/italia/onto/SM/OnlineContactPoint"></rdfs:range>
        <rdfs:comment xml:lang="en">Inverse Property of "has email".</rdfs:comment>
        <rdfs:comment xml:lang="it">Proprietà inversa di "ha email".</rdfs:comment>
        <rdfs:isDefinedBy rdf:resource="https://w3id.org/italia/onto/SM"></rdfs:isDefinedBy>
        <rdfs:label xml:lang="en">is email of</rdfs:label>
        <rdfs:label xml:lang="it">è email di</rdfs:label>
        <owl:versionInfo xml:lang="it">stabile</owl:versionInfo>
        <owl:versionInfo xml:lang="en">stable</owl:versionInfo>
    </owl:ObjectProperty>



    <!-- https://w3id.org/italia/onto/SM/isEmailTypeOf -->

    <owl:ObjectProperty rdf:about="https://w3id.org/italia/onto/SM/isEmailTypeOf">
        <rdfs:domain rdf:resource="https://w3id.org/italia/onto/SM/EmailType"></rdfs:domain>
        <rdfs:range rdf:resource="https://w3id.org/italia/onto/SM/Email"></rdfs:range>
        <rdfs:comment xml:lang="en">Inverse property of has email type. Hence, this property links an email type to an email.</rdfs:comment>
        <rdfs:comment xml:lang="it">Proprietà inversa di 'ha tipo di email'. Di conseguenza, questa proprietà collega un individuo della classe 'Tipo di email' ad un individuo della classe 'Email'.</rdfs:comment>
        <rdfs:isDefinedBy rdf:resource="https://w3id.org/italia/onto/SM"></rdfs:isDefinedBy>
        <rdfs:label xml:lang="en">is email type of</rdfs:label>
        <rdfs:label xml:lang="it">è tipo di email di</rdfs:label>
    </owl:ObjectProperty>



    <!-- https://w3id.org/italia/onto/SM/isImageOf -->

    <owl:ObjectProperty rdf:about="https://w3id.org/italia/onto/SM/isImageOf">
        <rdfs:domain rdf:resource="https://w3id.org/italia/onto/SM/Image"></rdfs:domain>
        <rdfs:range rdf:resource="http://www.w3.org/2002/07/owl#Thing"></rdfs:range>
        <rdfs:comment xml:lang="it">Questa proprietà collega un'immagine a qualsiasi cosa. E' la proprietà inversa di 'ha immagine'.</rdfs:comment>
        <rdfs:comment xml:lang="en">This property links an image to anything. It is defined as the inverse property of 'has image'.</rdfs:comment>
        <rdfs:isDefinedBy rdf:resource="https://w3id.org/italia/onto/SM"></rdfs:isDefinedBy>
        <rdfs:label xml:lang="en">is image of</rdfs:label>
        <rdfs:label xml:lang="it">è immagine di</rdfs:label>
    </owl:ObjectProperty>



    <!-- https://w3id.org/italia/onto/SM/isOnlineContactPointOf -->

    <owl:ObjectProperty rdf:about="https://w3id.org/italia/onto/SM/isOnlineContactPointOf">
        <rdfs:domain rdf:resource="https://w3id.org/italia/onto/SM/OnlineContactPoint"></rdfs:domain>
        <rdfs:range rdf:resource="http://www.w3.org/2002/07/owl#Thing"></rdfs:range>
        <rdfs:comment xml:lang="it">Questa proprietà è l'inversa di "ha punto di contatto online" e collega un punto di contatto online con qualsiasi cosa del dominio modellato.</rdfs:comment>
        <rdfs:comment xml:lang="en">This property is the inverse one for "has online contact point" and links an online contact point to any thing of the modelled domain.</rdfs:comment>
        <rdfs:isDefinedBy rdf:resource="https://w3id.org/italia/onto/SM"></rdfs:isDefinedBy>
        <rdfs:label xml:lang="en">is online contact point of</rdfs:label>
        <rdfs:label xml:lang="it">è punto di contatto online di</rdfs:label>
        <owl:versionInfo xml:lang="it">stabile</owl:versionInfo>
        <owl:versionInfo xml:lang="en">stable</owl:versionInfo>
    </owl:ObjectProperty>



    <!-- https://w3id.org/italia/onto/SM/isReplyOf -->

    <owl:ObjectProperty rdf:about="https://w3id.org/italia/onto/SM/isReplyOf">
        <rdfs:domain rdf:resource="https://w3id.org/italia/onto/SM/Post"></rdfs:domain>
        <rdfs:range rdf:resource="https://w3id.org/italia/onto/SM/Post"></rdfs:range>
        <rdfs:comment xml:lang="it">La proprietà 'è risposta di' permette di asserire che un certo post è la risposta ad un altro post.</rdfs:comment>
        <rdfs:comment xml:lang="en">The property 'is reply of' asserts that a given post is the answer to another post.</rdfs:comment>
        <rdfs:isDefinedBy rdf:resource="https://w3id.org/italia/onto/SM"></rdfs:isDefinedBy>
        <rdfs:label xml:lang="en">is reply of</rdfs:label>
        <rdfs:label xml:lang="it">è risposta di</rdfs:label>
        <prov:wasInfluencedBy rdf:resource="http://rdfs.org/sioc/ns#reply_of"></prov:wasInfluencedBy>
    </owl:ObjectProperty>



    <!-- https://w3id.org/italia/onto/SM/isTelephoneOf -->

    <owl:ObjectProperty rdf:about="https://w3id.org/italia/onto/SM/isTelephoneOf">
        <rdfs:domain rdf:resource="https://w3id.org/italia/onto/SM/Telephone"></rdfs:domain>
        <rdfs:range rdf:resource="https://w3id.org/italia/onto/SM/OnlineContactPoint"></rdfs:range>
        <rdfs:comment xml:lang="en">Inverse property of "has telephone".</rdfs:comment>
        <rdfs:comment xml:lang="it">Proprietà inversa di "ha telefono"</rdfs:comment>
        <rdfs:isDefinedBy rdf:resource="https://w3id.org/italia/onto/SM"></rdfs:isDefinedBy>
        <rdfs:label xml:lang="en">is telephone of</rdfs:label>
        <rdfs:label xml:lang="it">è telefono di</rdfs:label>
        <owl:versionInfo xml:lang="it">stabile</owl:versionInfo>
        <owl:versionInfo xml:lang="en">stable</owl:versionInfo>
    </owl:ObjectProperty>



    <!-- https://w3id.org/italia/onto/SM/isTelephoneTypeOf -->

    <owl:ObjectProperty rdf:about="https://w3id.org/italia/onto/SM/isTelephoneTypeOf">
        <rdfs:domain rdf:resource="https://w3id.org/italia/onto/SM/TelephoneType"></rdfs:domain>
        <rdfs:range rdf:resource="https://w3id.org/italia/onto/SM/Telephone"></rdfs:range>
        <rdfs:comment xml:lang="en">Inverse property of "has telephone type".</rdfs:comment>
        <rdfs:comment xml:lang="it">Proprietà inversa di "ha tipo di telefono".</rdfs:comment>
        <rdfs:isDefinedBy rdf:resource="https://w3id.org/italia/onto/SM"></rdfs:isDefinedBy>
        <rdfs:label xml:lang="en">is telephone type of</rdfs:label>
        <rdfs:label xml:lang="it">è tipo di telefono di</rdfs:label>
        <owl:versionInfo xml:lang="it">stabile</owl:versionInfo>
        <owl:versionInfo xml:lang="en">stable</owl:versionInfo>
    </owl:ObjectProperty>



    <!-- https://w3id.org/italia/onto/SM/isUserAccountOf -->

    <owl:ObjectProperty rdf:about="https://w3id.org/italia/onto/SM/isUserAccountOf">
        <rdfs:domain rdf:resource="https://w3id.org/italia/onto/SM/UserAccount"></rdfs:domain>
        <rdfs:range rdf:resource="https://w3id.org/italia/onto/SM/OnlineContactPoint"></rdfs:range>
        <rdfs:comment xml:lang="it">Questa proprietà collega un account utente al suo proprietario, che è un istanza di agente. E' la proprietà inversa di 'ha account utente'.</rdfs:comment>
        <rdfs:comment xml:lang="en">This property links a user account to its owner, which, in turn, is an agent. This property is the inverse of 'has user account'.</rdfs:comment>
        <rdfs:isDefinedBy rdf:resource="https://w3id.org/italia/onto/SM"></rdfs:isDefinedBy>
        <rdfs:label xml:lang="en">is user account of</rdfs:label>
        <rdfs:label xml:lang="it">è account utente di</rdfs:label>
    </owl:ObjectProperty>



    <!-- https://w3id.org/italia/onto/SM/isWebSiteOf -->

    <owl:ObjectProperty rdf:about="https://w3id.org/italia/onto/SM/isWebSiteOf">
        <rdfs:domain rdf:resource="https://w3id.org/italia/onto/SM/WebSite"></rdfs:domain>
        <rdfs:range rdf:resource="http://www.w3.org/2002/07/owl#Thing"></rdfs:range>
        <rdfs:comment xml:lang="en">Relation between a Web site and the entity this Web site is associated with. This property is the inverse of 'has Web site'.</rdfs:comment>
        <rdfs:comment xml:lang="it">Relazione tra un sito Web e l'entità a cui il sito Web è associato. Questa proprietà è l'inversa di 'ha sito Web'.</rdfs:comment>
        <rdfs:isDefinedBy rdf:resource="https://w3id.org/italia/onto/SM"></rdfs:isDefinedBy>
        <rdfs:label xml:lang="en">is Web site of</rdfs:label>
        <rdfs:label xml:lang="it">è sito Web di</rdfs:label>
    </owl:ObjectProperty>



    <!-- https://w3id.org/italia/onto/SM/issuesAccount -->

    <owl:ObjectProperty rdf:about="https://w3id.org/italia/onto/SM/issuesAccount">
        <rdfs:domain rdf:resource="https://w3id.org/italia/onto/SM/SocialMedia"></rdfs:domain>
        <rdfs:range rdf:resource="https://w3id.org/italia/onto/SM/UserAccount"></rdfs:range>
        <rdfs:comment xml:lang="it">Questa proprietà rappresenta il rilascio di un account utente da parte di un social media.</rdfs:comment>
        <rdfs:comment xml:lang="en">This property means that a Social Media issues a user account.</rdfs:comment>
        <rdfs:isDefinedBy rdf:resource="https://w3id.org/italia/onto/SM"></rdfs:isDefinedBy>
        <rdfs:label xml:lang="en">issues account</rdfs:label>
        <rdfs:label xml:lang="it">rilascia account</rdfs:label>
    </owl:ObjectProperty>



    <!--
    ///////////////////////////////////////////////////////////////////////////////////////
    //
    // Data properties
    //
    ///////////////////////////////////////////////////////////////////////////////////////
     -->




    <!-- https://w3id.org/italia/onto/SM/URL -->

    <owl:DatatypeProperty rdf:about="https://w3id.org/italia/onto/SM/URL">
        <rdfs:domain rdf:resource="http://www.w3.org/2002/07/owl#Thing"></rdfs:domain>
        <rdfs:range rdf:resource="http://www.w3.org/2001/XMLSchema#anyURI"></rdfs:range>
        <rdfs:comment xml:lang="it">Questa proprietà rappresenta un URL di una qualsiasi cosa del dominio modellato.</rdfs:comment>
        <rdfs:comment xml:lang="en">This property represents a general URL associated with any thing of the modelled domain.</rdfs:comment>
        <rdfs:label xml:lang="en">URL</rdfs:label>
        <rdfs:label xml:lang="it">URL</rdfs:label>
        <owl:versionInfo xml:lang="it">provvisoria</owl:versionInfo>
        <owl:versionInfo xml:lang="en">unstable</owl:versionInfo>
    </owl:DatatypeProperty>



    <!-- https://w3id.org/italia/onto/SM/bestUserRating -->

    <owl:DatatypeProperty rdf:about="https://w3id.org/italia/onto/SM/bestUserRating">
        <rdfs:subPropertyOf rdf:resource="https://w3id.org/italia/onto/SM/userRating"></rdfs:subPropertyOf>
        <rdfs:domain rdf:resource="https://w3id.org/italia/onto/SM/Rating"></rdfs:domain>
        <rdfs:range rdf:resource="http://www.w3.org/2000/01/rdf-schema#Literal"></rdfs:range>
        <rdfs:comment xml:lang="en">Among all  user rating scores it represents the best one</rdfs:comment>
        <rdfs:comment xml:lang="it">Tra tutte le valutazioni  rappresenta la migliore</rdfs:comment>
        <rdfs:isDefinedBy rdf:resource="https://w3id.org/italia/onto/SM"></rdfs:isDefinedBy>
        <rdfs:label xml:lang="en">best user rating</rdfs:label>
        <rdfs:label xml:lang="it">miglior valutazione utente</rdfs:label>
        <owl:versionInfo xml:lang="it">stabile</owl:versionInfo>
        <owl:versionInfo xml:lang="en">stable</owl:versionInfo>
    </owl:DatatypeProperty>



    <!-- https://w3id.org/italia/onto/SM/emailAddress -->

    <owl:DatatypeProperty rdf:about="https://w3id.org/italia/onto/SM/emailAddress">
        <rdf:type rdf:resource="http://www.w3.org/2002/07/owl#FunctionalProperty"></rdf:type>
        <rdfs:domain rdf:resource="https://w3id.org/italia/onto/SM/Email"></rdfs:domain>
        <rdfs:range rdf:resource="http://www.w3.org/2001/XMLSchema#anyURI"></rdfs:range>
        <rdfs:comment xml:lang="it">Questa proprietà rappresenta l'indirizzo email che deve essere espresso nella forma mailto:XX@YY.ZZ</rdfs:comment>
        <rdfs:comment xml:lang="en">This property represents the email address expressed as mailto:XX@YY.ZZ</rdfs:comment>
        <rdfs:isDefinedBy rdf:resource="https://w3id.org/italia/onto/SM"></rdfs:isDefinedBy>
        <rdfs:label xml:lang="en">email address</rdfs:label>
        <rdfs:label xml:lang="it">indirizzo email</rdfs:label>
    </owl:DatatypeProperty>



    <!-- https://w3id.org/italia/onto/SM/postContent -->

    <owl:DatatypeProperty rdf:about="https://w3id.org/italia/onto/SM/postContent">
        <rdfs:domain rdf:resource="https://w3id.org/italia/onto/SM/Post"></rdfs:domain>
        <rdfs:range rdf:resource="http://www.w3.org/2000/01/rdf-schema#Literal"></rdfs:range>
        <rdfs:comment xml:lang="it">Il contenuto di un post.</rdfs:comment>
        <rdfs:comment xml:lang="en">The content of a post.</rdfs:comment>
        <rdfs:isDefinedBy rdf:resource="https://w3id.org/italia/onto/SM"></rdfs:isDefinedBy>
        <rdfs:label xml:lang="it">contenuto del post</rdfs:label>
        <rdfs:label xml:lang="en">post content</rdfs:label>
    </owl:DatatypeProperty>



    <!-- https://w3id.org/italia/onto/SM/reviewAspect -->

    <owl:DatatypeProperty rdf:about="https://w3id.org/italia/onto/SM/reviewAspect">
        <rdfs:domain rdf:resource="https://w3id.org/italia/onto/SM/Review"></rdfs:domain>
        <rdfs:range rdf:resource="http://www.w3.org/2000/01/rdf-schema#Literal"></rdfs:range>
        <rdfs:comment xml:lang="it">L'aspetto sul quale si focalizza la recensione. Esempio: stanza per una struttura ricettiva, servizi offerti dall'evento pubblico, ecc.</rdfs:comment>
        <rdfs:comment xml:lang="en">The aspect on which the review focusses.</rdfs:comment>
        <rdfs:isDefinedBy rdf:resource="https://w3id.org/italia/onto/SM"></rdfs:isDefinedBy>
        <rdfs:label xml:lang="it">aspetto della recensione</rdfs:label>
        <rdfs:label xml:lang="en">review aspect</rdfs:label>
        <owl:versionInfo xml:lang="it">stabile</owl:versionInfo>
        <owl:versionInfo xml:lang="en">stable</owl:versionInfo>
    </owl:DatatypeProperty>



    <!-- https://w3id.org/italia/onto/SM/socialMediaName -->

    <owl:DatatypeProperty rdf:about="https://w3id.org/italia/onto/SM/socialMediaName">
        <rdfs:subPropertyOf rdf:resource="https://w3id.org/italia/onto/l0/name"></rdfs:subPropertyOf>
        <rdf:type rdf:resource="http://www.w3.org/2002/07/owl#FunctionalProperty"></rdf:type>
        <rdfs:domain rdf:resource="https://w3id.org/italia/onto/SM/SocialMedia"></rdfs:domain>
        <rdfs:range rdf:resource="http://www.w3.org/2000/01/rdf-schema#Literal"></rdfs:range>
        <rdfs:comment xml:lang="it">Il nome associato con un individuo che rappresenta un social media.</rdfs:comment>
        <rdfs:comment xml:lang="en">The name associated with a social media entity.</rdfs:comment>
        <rdfs:isDefinedBy rdf:resource="https://w3id.org/italia/onto/SM"></rdfs:isDefinedBy>
        <rdfs:label xml:lang="it">nome di social media</rdfs:label>
        <rdfs:label xml:lang="en">social media name</rdfs:label>
    </owl:DatatypeProperty>



    <!-- https://w3id.org/italia/onto/SM/telephoneNumber -->

    <owl:DatatypeProperty rdf:about="https://w3id.org/italia/onto/SM/telephoneNumber">
        <rdf:type rdf:resource="http://www.w3.org/2002/07/owl#FunctionalProperty"></rdf:type>
        <rdfs:domain rdf:resource="https://w3id.org/italia/onto/SM/Telephone"></rdfs:domain>
        <rdfs:range rdf:resource="http://www.w3.org/2000/01/rdf-schema#Literal"></rdfs:range>
        <rdfs:comment xml:lang="it">Questa proprietà consente di rappresentare il numero di telefono.</rdfs:comment>
        <rdfs:comment xml:lang="en">This property represents the telephone number</rdfs:comment>
        <rdfs:isDefinedBy rdf:resource="https://w3id.org/italia/onto/SM"></rdfs:isDefinedBy>
        <rdfs:label xml:lang="it">numero di telefono</rdfs:label>
        <rdfs:label xml:lang="en">telephone number</rdfs:label>
        <owl:versionInfo xml:lang="it">stabile</owl:versionInfo>
        <owl:versionInfo xml:lang="en">stable</owl:versionInfo>
    </owl:DatatypeProperty>



    <!-- https://w3id.org/italia/onto/SM/userAccountName -->

    <owl:DatatypeProperty rdf:about="https://w3id.org/italia/onto/SM/userAccountName">
        <rdfs:subPropertyOf rdf:resource="https://w3id.org/italia/onto/l0/name"></rdfs:subPropertyOf>
        <rdfs:domain rdf:resource="https://w3id.org/italia/onto/SM/UserAccount"></rdfs:domain>
        <rdfs:range rdf:resource="http://www.w3.org/2001/XMLSchema#string"></rdfs:range>
        <rdfs:comment xml:lang="it">Questa proprietà collega un account utente al suo nome (un letterale).</rdfs:comment>
        <rdfs:comment xml:lang="en">This property links a user account to its name (i.e. a literal).</rdfs:comment>
        <rdfs:isDefinedBy rdf:resource="https://w3id.org/italia/onto/SM"></rdfs:isDefinedBy>
        <rdfs:label xml:lang="it">nome dell'account utente</rdfs:label>
        <rdfs:label xml:lang="en">user account name</rdfs:label>
    </owl:DatatypeProperty>



    <!-- https://w3id.org/italia/onto/SM/userRating -->

    <owl:DatatypeProperty rdf:about="https://w3id.org/italia/onto/SM/userRating">
        <rdfs:domain rdf:resource="https://w3id.org/italia/onto/SM/Rating"></rdfs:domain>
        <rdfs:range rdf:resource="http://www.w3.org/2000/01/rdf-schema#Literal"></rdfs:range>
        <rdfs:comment xml:lang="it">Questa proprietà rappresenta una valutazione dell'utente espressa come 1,2,3,4,5 oppure ogni altro tipo di valutazione associata a una recensione.</rdfs:comment>
        <rdfs:comment xml:lang="en">This property represents a user evaluation/rating expressed as 1,2,3,4,5 or any other type of rating associated with a review.</rdfs:comment>
        <rdfs:isDefinedBy rdf:resource="https://w3id.org/italia/onto/SM"></rdfs:isDefinedBy>
        <rdfs:label xml:lang="en">user rating</rdfs:label>
        <rdfs:label xml:lang="it">valutazione utente</rdfs:label>
        <owl:versionInfo xml:lang="it">stabile</owl:versionInfo>
        <owl:versionInfo xml:lang="en">stable</owl:versionInfo>
    </owl:DatatypeProperty>



    <!-- https://w3id.org/italia/onto/SM/worstUserRating -->

    <owl:DatatypeProperty rdf:about="https://w3id.org/italia/onto/SM/worstUserRating">
        <rdfs:subPropertyOf rdf:resource="https://w3id.org/italia/onto/SM/userRating"></rdfs:subPropertyOf>
        <rdfs:domain rdf:resource="https://w3id.org/italia/onto/SM/Rating"></rdfs:domain>
        <rdfs:range rdf:resource="http://www.w3.org/2000/01/rdf-schema#Literal"></rdfs:range>
        <rdfs:comment xml:lang="en">Among all the rating associated with a thing of the modelled domain, it represents the worst rating.</rdfs:comment>
        <rdfs:comment xml:lang="it">Tra tutte le valutazioni rispetto a una cosa del dominio da modellare, rappresenta la peggior valutazione.</rdfs:comment>
        <rdfs:isDefinedBy rdf:resource="https://w3id.org/italia/onto/SM"></rdfs:isDefinedBy>
        <rdfs:label xml:lang="it">peggior valutazione utente</rdfs:label>
        <rdfs:label xml:lang="en">worst user rating</rdfs:label>
        <owl:versionInfo xml:lang="it">stabile</owl:versionInfo>
        <owl:versionInfo xml:lang="en">stable</owl:versionInfo>
    </owl:DatatypeProperty>



    <!-- https://w3id.org/italia/onto/l0/name -->

    <owl:DatatypeProperty rdf:about="https://w3id.org/italia/onto/l0/name"></owl:DatatypeProperty>



    <!--
    ///////////////////////////////////////////////////////////////////////////////////////
    //
    // Classes
    //
    ///////////////////////////////////////////////////////////////////////////////////////
     -->




    <!-- http://dati.gov.it/onto/dcatapit#Agent -->

    <owl:Class rdf:about="http://dati.gov.it/onto/dcatapit#Agent"></owl:Class>



    <!-- http://dati.gov.it/onto/dcatapit#Organization -->

    <owl:Class rdf:about="http://dati.gov.it/onto/dcatapit#Organization"></owl:Class>



    <!-- http://www.w3.org/2006/vcard/ns#Kind -->

    <owl:Class rdf:about="http://www.w3.org/2006/vcard/ns#Kind"></owl:Class>



    <!-- http://www.w3.org/2006/vcard/ns#Organization -->

    <owl:Class rdf:about="http://www.w3.org/2006/vcard/ns#Organization"></owl:Class>



    <!-- http://xmlns.com/foaf/0.1/Agent -->

    <owl:Class rdf:about="http://xmlns.com/foaf/0.1/Agent"></owl:Class>



    <!-- https://w3id.org/italia/onto/ADMS/Project -->

    <owl:Class rdf:about="https://w3id.org/italia/onto/ADMS/Project"></owl:Class>



    <!-- https://w3id.org/italia/onto/ADMS/SemanticAsset -->

    <owl:Class rdf:about="https://w3id.org/italia/onto/ADMS/SemanticAsset"></owl:Class>



    <!-- https://w3id.org/italia/onto/ADMS/SemanticAssetDistribution -->

    <owl:Class rdf:about="https://w3id.org/italia/onto/ADMS/SemanticAssetDistribution"></owl:Class>



    <!-- https://w3id.org/italia/onto/SM/ContactPoint -->

    <owl:Class rdf:about="https://w3id.org/italia/onto/SM/ContactPoint">
        <rdfs:subClassOf rdf:resource="https://w3id.org/italia/onto/l0/Object"></rdfs:subClassOf>
        <rdfs:comment xml:lang="en">A contact point that can be physical or available online</rdfs:comment>
        <rdfs:comment xml:lang="it">Un punto di contatto che può essere fisico o disponibile online</rdfs:comment>
        <rdfs:isDefinedBy rdf:resource="https://w3id.org/italia/onto/SM"></rdfs:isDefinedBy>
        <rdfs:label xml:lang="en">Contact Point</rdfs:label>
        <rdfs:label xml:lang="it">Punto di Contatto</rdfs:label>
        <owl:versionInfo xml:lang="it">stabile</owl:versionInfo>
        <owl:versionInfo xml:lang="en">stable</owl:versionInfo>
    </owl:Class>



    <!-- https://w3id.org/italia/onto/SM/Email -->

    <owl:Class rdf:about="https://w3id.org/italia/onto/SM/Email">
        <rdfs:subClassOf rdf:resource="https://w3id.org/italia/onto/l0/Object"></rdfs:subClassOf>
        <rdfs:subClassOf>
            <owl:Restriction>
                <owl:onProperty rdf:resource="https://w3id.org/italia/onto/SM/hasEmailType"></owl:onProperty>
                <owl:qualifiedCardinality rdf:datatype="http://www.w3.org/2001/XMLSchema#nonNegativeInteger">1</owl:qualifiedCardinality>
                <owl:onClass rdf:resource="https://w3id.org/italia/onto/SM/EmailType"></owl:onClass>
            </owl:Restriction>
        </rdfs:subClassOf>
        <rdfs:subClassOf>
            <owl:Restriction>
                <owl:onProperty rdf:resource="https://w3id.org/italia/onto/SM/isEmailOf"></owl:onProperty>
                <owl:qualifiedCardinality rdf:datatype="http://www.w3.org/2001/XMLSchema#nonNegativeInteger">1</owl:qualifiedCardinality>
                <owl:onClass rdf:resource="https://w3id.org/italia/onto/SM/OnlineContactPoint"></owl:onClass>
            </owl:Restriction>
        </rdfs:subClassOf>
        <rdfs:subClassOf>
            <owl:Restriction>
                <owl:onProperty rdf:resource="https://w3id.org/italia/onto/SM/emailAddress"></owl:onProperty>
                <owl:qualifiedCardinality rdf:datatype="http://www.w3.org/2001/XMLSchema#nonNegativeInteger">1</owl:qualifiedCardinality>
                <owl:onDataRange rdf:resource="http://www.w3.org/2001/XMLSchema#anyURI"></owl:onDataRange>
            </owl:Restriction>
        </rdfs:subClassOf>
        <rdfs:comment xml:lang="it">Questa classe rappresenta l'indirizzo email del punto di contatto di un'organizzazione. La classe è collegata al tipo di email. Nell'ambito itailano si identificano due tipi principali di email, la PEC e l'email tradizionale.</rdfs:comment>
        <rdfs:comment xml:lang="en">This class represents the Email address of the contact point of an organization. The class is linked to the type of email that can be specified. In the Italian context we identify two types of Emails; namely, Certified Electronic Email and Traditional Email addresses.</rdfs:comment>
        <rdfs:isDefinedBy rdf:resource="https://w3id.org/italia/onto/SM"></rdfs:isDefinedBy>
        <rdfs:label xml:lang="en">Email</rdfs:label>
        <rdfs:label xml:lang="it">Email</rdfs:label>
        <prov:wasInfluencedBy rdf:resource="http://www.w3.org/2006/vcard/ns#Email"></prov:wasInfluencedBy>
    </owl:Class>



    <!-- https://w3id.org/italia/onto/SM/EmailType -->

    <owl:Class rdf:about="https://w3id.org/italia/onto/SM/EmailType">
        <rdfs:subClassOf rdf:resource="https://w3id.org/italia/onto/l0/Concept"></rdfs:subClassOf>
        <rdfs:subClassOf>
            <owl:Restriction>
                <owl:onProperty rdf:resource="https://w3id.org/italia/onto/SM/isEmailTypeOf"></owl:onProperty>
                <owl:allValuesFrom rdf:resource="https://w3id.org/italia/onto/SM/Email"></owl:allValuesFrom>
            </owl:Restriction>
        </rdfs:subClassOf>
        <rdfs:comment xml:lang="it">Questa classe rappresenta i tipo di email e può assumere due valori come definiti nel vocabolario controllato dei canali di erogazione dei servizi (https://w3id.org/italia/controlled-vocabulary/classifications-for-public-services/channel). Nello specifico le istanze di questa classe sono: https://w3id.org/italia/controlled-vocabulary/classifications-for-public-services/channel/042 (Email tradizionale) e https://w3id.org/italia/controlled-vocabulary/classifications-for-public-services/channel/041 (PEC).</rdfs:comment>
        <rdfs:comment xml:lang="en">This class represents the type of email. It can assume two values that are defined in the Channel controlled vocabulary https://w3id.org/italia/controlled-vocabulary/classifications-for-public-services/channel. In particular, the istances of this class are https://w3id.org/italia/controlled-vocabulary/classifications-for-public-services/channel/041 (Certified Electronic Mail) and https://w3id.org/italia/controlled-vocabulary/classifications-for-public-services/channel/042 (E-mail).</rdfs:comment>
        <rdfs:isDefinedBy rdf:resource="https://w3id.org/italia/onto/SM"></rdfs:isDefinedBy>
        <rdfs:label xml:lang="en">Email Type</rdfs:label>
        <rdfs:label xml:lang="it">Tipo di email</rdfs:label>
        <owl:versionInfo xml:lang="it">stabile</owl:versionInfo>
        <owl:versionInfo xml:lang="en">stable</owl:versionInfo>
    </owl:Class>



    <!-- https://w3id.org/italia/onto/SM/Image -->

    <owl:Class rdf:about="https://w3id.org/italia/onto/SM/Image">
        <rdfs:subClassOf rdf:resource="https://w3id.org/italia/onto/l0/Object"></rdfs:subClassOf>
        <rdfs:comment xml:lang="it">Questa classe rappresenta le immagini (ex. loghi).</rdfs:comment>
        <rdfs:comment xml:lang="en">This class represents images.</rdfs:comment>
        <rdfs:isDefinedBy rdf:resource="https://w3id.org/italia/onto/SM"></rdfs:isDefinedBy>
        <rdfs:label xml:lang="en">Image</rdfs:label>
        <rdfs:label xml:lang="it">Immagine</rdfs:label>
        <prov:wasInfluencedBy rdf:resource="http://schema.org/ImageObject"></prov:wasInfluencedBy>
        <prov:wasInfluencedBy rdf:resource="http://xmlns.com/foaf/0.1/Image"></prov:wasInfluencedBy>
    </owl:Class>



    <!-- https://w3id.org/italia/onto/SM/OnlineContactPoint -->

    <owl:Class rdf:about="https://w3id.org/italia/onto/SM/OnlineContactPoint">
        <rdfs:subClassOf rdf:resource="https://w3id.org/italia/onto/SM/ContactPoint"></rdfs:subClassOf>
        <rdfs:subClassOf>
            <owl:Restriction>
                <owl:onProperty rdf:resource="https://w3id.org/italia/onto/SM/hasEmail"></owl:onProperty>
                <owl:someValuesFrom rdf:resource="https://w3id.org/italia/onto/SM/Email"></owl:someValuesFrom>
            </owl:Restriction>
        </rdfs:subClassOf>
        <rdfs:subClassOf>
            <owl:Restriction>
                <owl:onProperty rdf:resource="https://w3id.org/italia/onto/SM/hasTelephone"></owl:onProperty>
                <owl:allValuesFrom rdf:resource="https://w3id.org/italia/onto/SM/Telephone"></owl:allValuesFrom>
            </owl:Restriction>
        </rdfs:subClassOf>
        <rdfs:subClassOf>
            <owl:Restriction>
                <owl:onProperty rdf:resource="https://w3id.org/italia/onto/SM/hasUserAccount"></owl:onProperty>
                <owl:allValuesFrom rdf:resource="https://w3id.org/italia/onto/SM/UserAccount"></owl:allValuesFrom>
            </owl:Restriction>
        </rdfs:subClassOf>
        <rdfs:subClassOf>
            <owl:Restriction>
                <owl:onProperty rdf:resource="https://w3id.org/italia/onto/SM/hasWebSite"></owl:onProperty>
                <owl:allValuesFrom rdf:resource="https://w3id.org/italia/onto/SM/WebSite"></owl:allValuesFrom>
            </owl:Restriction>
        </rdfs:subClassOf>
        <owl:disjointWith rdf:resource="https://w3id.org/italia/onto/SM/PhysicalContactPoint"></owl:disjointWith>
        <rdfs:comment xml:lang="it">Questa classe rappresenta un punto di contatto online. Essa raggruppa un insieme di tipi di canali di contatto online come account di social network, email, siti web, ecc.</rdfs:comment>
        <rdfs:comment xml:lang="en">This class represents an online contact point; that is, an object that groups a set of types of online (social) media channels such as email, social network contacts, web site, ecc.</rdfs:comment>
        <rdfs:isDefinedBy rdf:resource="https://w3id.org/italia/onto/SM"></rdfs:isDefinedBy>
        <rdfs:label xml:lang="en">Online Contact Point</rdfs:label>
        <rdfs:label xml:lang="it">Punto di Contatto Online</rdfs:label>
        <owl:versionInfo xml:lang="it">stabile</owl:versionInfo>
        <owl:versionInfo xml:lang="en">stable</owl:versionInfo>
        <prov:wasInfluencedBy rdf:resource="http://schema.org/ContactPoint"></prov:wasInfluencedBy>
    </owl:Class>



    <!-- https://w3id.org/italia/onto/SM/PhysicalContactPoint -->

    <owl:Class rdf:about="https://w3id.org/italia/onto/SM/PhysicalContactPoint">
        <rdfs:subClassOf rdf:resource="https://w3id.org/italia/onto/POI/PointOfInterest"></rdfs:subClassOf>
        <rdfs:subClassOf rdf:resource="https://w3id.org/italia/onto/SM/ContactPoint"></rdfs:subClassOf>
        <rdfs:comment xml:lang="it">Questa classe rappresenta un punto di contatto fisico come per esempio un box informazioni, un punto turistico, una biglietteria, un ufficio, ecc. Può essere considerato un punto di interesse.</rdfs:comment>
        <rdfs:comment xml:lang="en">This class rapresents a physical contact point such as a ticket office, an office, a tourtist point</rdfs:comment>
        <rdfs:label xml:lang="en">Physical Contact Point</rdfs:label>
        <rdfs:label xml:lang="it">Punto di Contatto Fisico</rdfs:label>
        <owl:versionInfo rdf:resource="https://w3id.org/italia/onto/SM"></owl:versionInfo>
        <owl:versionInfo xml:lang="it">provvisoria</owl:versionInfo>
        <owl:versionInfo xml:lang="en">unstable</owl:versionInfo>
    </owl:Class>



    <!-- https://w3id.org/italia/onto/SM/Post -->

    <owl:Class rdf:about="https://w3id.org/italia/onto/SM/Post">
        <rdfs:subClassOf rdf:resource="https://w3id.org/italia/onto/l0/Object"></rdfs:subClassOf>
        <rdfs:subClassOf>
            <owl:Restriction>
                <owl:onProperty rdf:resource="https://w3id.org/italia/onto/SM/hasCreator"></owl:onProperty>
                <owl:qualifiedCardinality rdf:datatype="http://www.w3.org/2001/XMLSchema#nonNegativeInteger">1</owl:qualifiedCardinality>
                <owl:onClass rdf:resource="https://w3id.org/italia/onto/SM/UserAccount"></owl:onClass>
            </owl:Restriction>
        </rdfs:subClassOf>
        <rdfs:subClassOf>
            <owl:Restriction>
                <owl:onProperty rdf:resource="https://w3id.org/italia/onto/SM/postContent"></owl:onProperty>
                <owl:cardinality rdf:datatype="http://www.w3.org/2001/XMLSchema#nonNegativeInteger">1</owl:cardinality>
            </owl:Restriction>
        </rdfs:subClassOf>
        <rdfs:comment xml:lang="en">A post on a social media.</rdfs:comment>
        <rdfs:comment xml:lang="it">Un post su un social media.</rdfs:comment>
        <rdfs:isDefinedBy rdf:resource="https://w3id.org/italia/onto/SM"></rdfs:isDefinedBy>
        <rdfs:label xml:lang="en">Post</rdfs:label>
        <rdfs:label xml:lang="it">Post</rdfs:label>
        <prov:wasInfluencedBy rdf:resource="http://rdfs.org/sioc/ns#Post"></prov:wasInfluencedBy>
        <prov:wasInfluencedBy rdf:resource="http://schema.org/SocialMediaPosting"></prov:wasInfluencedBy>
    </owl:Class>



    <!-- https://w3id.org/italia/onto/SM/Rating -->

    <owl:Class rdf:about="https://w3id.org/italia/onto/SM/Rating">
        <rdfs:subClassOf rdf:resource="https://w3id.org/italia/onto/l0/Description"></rdfs:subClassOf>
        <rdfs:subClassOf>
            <owl:Restriction>
                <owl:onProperty rdf:resource="https://w3id.org/italia/onto/SM/bestUserRating"></owl:onProperty>
                <owl:allValuesFrom rdf:resource="http://www.w3.org/2000/01/rdf-schema#Literal"></owl:allValuesFrom>
            </owl:Restriction>
        </rdfs:subClassOf>
        <rdfs:subClassOf>
            <owl:Restriction>
                <owl:onProperty rdf:resource="https://w3id.org/italia/onto/SM/worstUserRating"></owl:onProperty>
                <owl:allValuesFrom rdf:resource="http://www.w3.org/2000/01/rdf-schema#Literal"></owl:allValuesFrom>
            </owl:Restriction>
        </rdfs:subClassOf>
        <rdfs:subClassOf>
            <owl:Restriction>
                <owl:onProperty rdf:resource="https://w3id.org/italia/onto/SM/userRating"></owl:onProperty>
                <owl:cardinality rdf:datatype="http://www.w3.org/2001/XMLSchema#nonNegativeInteger">1</owl:cardinality>
            </owl:Restriction>
        </rdfs:subClassOf>
        <rdfs:comment xml:lang="it">Gli individui della classe rappresentano una valutazione degli utenti rispetto a una determinata cosa del dominio da modellare. Essa può assumere valori quali per esempio 1, 2, 3... oppure positivo, negativo, ecc.</rdfs:comment>
        <rdfs:comment xml:lang="en">The individuals of this class represent an evaluation which may assume values such as "1", "2", etc.</rdfs:comment>
        <rdfs:isDefinedBy rdf:resource="https://w3id.org/italia/onto/SM"></rdfs:isDefinedBy>
        <rdfs:label xml:lang="en">Rating</rdfs:label>
        <rdfs:label xml:lang="it">Valutazione</rdfs:label>
        <owl:versionInfo xml:lang="it">stabile</owl:versionInfo>
        <owl:versionInfo xml:lang="en">stable</owl:versionInfo>
        <prov:wasDerivedFrom rdf:resource="https://schema.org/Rating"></prov:wasDerivedFrom>
    </owl:Class>



    <!-- https://w3id.org/italia/onto/SM/Review -->

    <owl:Class rdf:about="https://w3id.org/italia/onto/SM/Review">
        <rdfs:subClassOf rdf:resource="https://w3id.org/italia/onto/SM/Post"></rdfs:subClassOf>
        <rdfs:subClassOf>
            <owl:Restriction>
                <owl:onProperty rdf:resource="https://w3id.org/italia/onto/SM/hasRating"></owl:onProperty>
                <owl:allValuesFrom rdf:resource="https://w3id.org/italia/onto/SM/Rating"></owl:allValuesFrom>
            </owl:Restriction>
        </rdfs:subClassOf>
        <rdfs:subClassOf>
            <owl:Restriction>
                <owl:onProperty rdf:resource="https://w3id.org/italia/onto/SM/reviewAspect"></owl:onProperty>
                <owl:allValuesFrom rdf:resource="http://www.w3.org/2000/01/rdf-schema#Literal"></owl:allValuesFrom>
            </owl:Restriction>
        </rdfs:subClassOf>
        <rdfs:comment xml:lang="it">Gli individui di questa classe rapprensetano particolari tipi di Post che sono recensioni (esempio: recensioni di strutture ricettive, recensioni di eventi pubblici, ecc.)</rdfs:comment>
        <rdfs:comment xml:lang="en">Individuals of this class represent specific types of posts that are review (examples include review for accommodation facilities, review for public events, etc.)</rdfs:comment>
        <rdfs:isDefinedBy rdf:resource="https://w3id.org/italia/onto/SM"></rdfs:isDefinedBy>
        <rdfs:label xml:lang="it">Recensione</rdfs:label>
        <rdfs:label xml:lang="en">Review</rdfs:label>
        <owl:versionInfo xml:lang="it">stabile</owl:versionInfo>
        <owl:versionInfo xml:lang="en">stable</owl:versionInfo>
        <prov:wasDerivedFrom rdf:resource="https://schema.org/Review"></prov:wasDerivedFrom>
    </owl:Class>



    <!-- https://w3id.org/italia/onto/SM/SocialMedia -->

    <owl:Class rdf:about="https://w3id.org/italia/onto/SM/SocialMedia">
        <rdfs:subClassOf rdf:resource="https://w3id.org/italia/onto/l0/Object"></rdfs:subClassOf>
        <rdfs:subClassOf>
            <owl:Restriction>
                <owl:onProperty rdf:resource="https://w3id.org/italia/onto/SM/socialMediaName"></owl:onProperty>
                <owl:cardinality rdf:datatype="http://www.w3.org/2001/XMLSchema#nonNegativeInteger">1</owl:cardinality>
            </owl:Restriction>
        </rdfs:subClassOf>
        <rdfs:comment xml:lang="it">Questa  classe rappresenta un social media come, ad esempio, un social network (ex. Facebook, Twitter, ecc...).</rdfs:comment>
        <rdfs:comment xml:lang="en">This class represents a social media like a social network (e.g. Facebook, Twitter, etc.).</rdfs:comment>
        <rdfs:isDefinedBy rdf:resource="https://w3id.org/italia/onto/SM"></rdfs:isDefinedBy>
        <rdfs:label xml:lang="en">Social media</rdfs:label>
        <rdfs:label xml:lang="it">Social media</rdfs:label>
    </owl:Class>



    <!-- https://w3id.org/italia/onto/SM/Telephone -->

    <owl:Class rdf:about="https://w3id.org/italia/onto/SM/Telephone">
        <rdfs:subClassOf rdf:resource="https://w3id.org/italia/onto/l0/Object"></rdfs:subClassOf>
        <rdfs:subClassOf>
            <owl:Restriction>
                <owl:onProperty rdf:resource="https://w3id.org/italia/onto/SM/hasTelephoneType"></owl:onProperty>
                <owl:qualifiedCardinality rdf:datatype="http://www.w3.org/2001/XMLSchema#nonNegativeInteger">1</owl:qualifiedCardinality>
                <owl:onClass rdf:resource="https://w3id.org/italia/onto/SM/TelephoneType"></owl:onClass>
            </owl:Restriction>
        </rdfs:subClassOf>
        <rdfs:subClassOf>
            <owl:Restriction>
                <owl:onProperty rdf:resource="https://w3id.org/italia/onto/SM/isTelephoneOf"></owl:onProperty>
                <owl:qualifiedCardinality rdf:datatype="http://www.w3.org/2001/XMLSchema#nonNegativeInteger">1</owl:qualifiedCardinality>
                <owl:onClass rdf:resource="https://w3id.org/italia/onto/SM/OnlineContactPoint"></owl:onClass>
            </owl:Restriction>
        </rdfs:subClassOf>
        <rdfs:subClassOf>
            <owl:Restriction>
                <owl:onProperty rdf:resource="https://w3id.org/italia/onto/SM/telephoneNumber"></owl:onProperty>
                <owl:cardinality rdf:datatype="http://www.w3.org/2001/XMLSchema#nonNegativeInteger">1</owl:cardinality>
            </owl:Restriction>
        </rdfs:subClassOf>
        <rdfs:comment xml:lang="it">Questa classe rappresenta un telefono che a sua volta è caratterizzato da un tipo (Voce, Fax) e da un numero.</rdfs:comment>
        <rdfs:comment xml:lang="en">This class represents the Telephone that is characterized by a type (Voice, Fax) and a telephone number.</rdfs:comment>
        <rdfs:isDefinedBy rdf:resource="https://w3id.org/italia/onto/SM"></rdfs:isDefinedBy>
        <rdfs:label xml:lang="it">Telefono</rdfs:label>
        <rdfs:label xml:lang="en">Telephone</rdfs:label>
        <prov:wasInfluencedBy rdf:resource="http://www.w3.org/2006/vcard/ns#TelephoneType"></prov:wasInfluencedBy>
    </owl:Class>



    <!-- https://w3id.org/italia/onto/SM/TelephoneType -->

    <owl:Class rdf:about="https://w3id.org/italia/onto/SM/TelephoneType">
        <rdfs:subClassOf rdf:resource="https://w3id.org/italia/onto/l0/Concept"></rdfs:subClassOf>
        <rdfs:subClassOf>
            <owl:Restriction>
                <owl:onProperty rdf:resource="https://w3id.org/italia/onto/SM/isTelephoneTypeOf"></owl:onProperty>
                <owl:allValuesFrom rdf:resource="https://w3id.org/italia/onto/SM/Telephone"></owl:allValuesFrom>
            </owl:Restriction>
        </rdfs:subClassOf>
        <rdfs:comment xml:lang="it">Questa classe rappresenta il tipo di telefono. I valori di questa classe sono quelli del vocabolario controllato https://w3id.org/italia/controlled-vocabulary/classifications-for-public-services/channel e in particolare sono i valori finali della categoria https://w3id.org/italia/controlled-vocabulary/classifications-for-public-services/channel/03 (telefono) e quindi i seguenti https://w3id.org/italia/controlled-vocabulary/classifications-for-public-services/channel/031 (Numero Dedicato - Voce), hhttps://w3id.org/italia/controlled-vocabulary/classifications-for-public-services/channel/032 (Call Center), https://w3id.org/italia/controlled-vocabulary/classifications-for-public-services/channel/033 (Fax)</rdfs:comment>
        <rdfs:comment xml:lang="en">This class represents the type of Telephone. The value of this class are those defined in the controlled vocabulary https://w3id.org/italia/controlled-vocabulary/classifications-for-public-services/channel and in particular the final values of the category telephone (https://w3id.org/italia/controlled-vocabulary/classifications-for-public-services/channel/03) that are the following: https://w3id.org/italia/controlled-vocabulary/classifications-for-public-services/channel/031 (Voice) https://w3id.org/italia/controlled-vocabulary/classifications-for-public-services/channel/032 (Call Center)  https://w3id.org/italia/controlled-vocabulary/classifications-for-public-services/channel/033 (Fax)</rdfs:comment>
        <rdfs:isDefinedBy rdf:resource="https://w3id.org/italia/onto/SM"></rdfs:isDefinedBy>
        <rdfs:label xml:lang="en">Telephone Type</rdfs:label>
        <rdfs:label xml:lang="it">Tipo di Telefono</rdfs:label>
        <owl:versionInfo xml:lang="it">stabile</owl:versionInfo>
        <owl:versionInfo xml:lang="en">stable</owl:versionInfo>
        <prov:wasInfluencedBy rdf:resource="http://www.w3.org/2006/vcard/ns#TelephoneType"></prov:wasInfluencedBy>
    </owl:Class>



    <!-- https://w3id.org/italia/onto/SM/UserAccount -->

    <owl:Class rdf:about="https://w3id.org/italia/onto/SM/UserAccount">
        <rdfs:subClassOf rdf:resource="https://w3id.org/italia/onto/l0/Object"></rdfs:subClassOf>
        <rdfs:subClassOf>
            <owl:Restriction>
                <owl:onProperty rdf:resource="https://w3id.org/italia/onto/SM/isAccountIssuedBy"></owl:onProperty>
                <owl:qualifiedCardinality rdf:datatype="http://www.w3.org/2001/XMLSchema#nonNegativeInteger">1</owl:qualifiedCardinality>
                <owl:onClass rdf:resource="https://w3id.org/italia/onto/SM/SocialMedia"></owl:onClass>
            </owl:Restriction>
        </rdfs:subClassOf>
        <rdfs:subClassOf>
            <owl:Restriction>
                <owl:onProperty rdf:resource="https://w3id.org/italia/onto/SM/isUserAccountOf"></owl:onProperty>
                <owl:qualifiedCardinality rdf:datatype="http://www.w3.org/2001/XMLSchema#nonNegativeInteger">1</owl:qualifiedCardinality>
                <owl:onClass rdf:resource="https://w3id.org/italia/onto/SM/OnlineContactPoint"></owl:onClass>
            </owl:Restriction>
        </rdfs:subClassOf>
        <rdfs:subClassOf>
            <owl:Restriction>
                <owl:onProperty rdf:resource="https://w3id.org/italia/onto/SM/URL"></owl:onProperty>
                <owl:maxQualifiedCardinality rdf:datatype="http://www.w3.org/2001/XMLSchema#nonNegativeInteger">1</owl:maxQualifiedCardinality>
                <owl:onDataRange rdf:resource="http://www.w3.org/2001/XMLSchema#anyURI"></owl:onDataRange>
            </owl:Restriction>
        </rdfs:subClassOf>
        <rdfs:subClassOf>
            <owl:Restriction>
                <owl:onProperty rdf:resource="https://w3id.org/italia/onto/SM/userAccountName"></owl:onProperty>
                <owl:maxQualifiedCardinality rdf:datatype="http://www.w3.org/2001/XMLSchema#nonNegativeInteger">1</owl:maxQualifiedCardinality>
                <owl:onDataRange rdf:resource="http://www.w3.org/2001/XMLSchema#string"></owl:onDataRange>
            </owl:Restriction>
        </rdfs:subClassOf>
        <rdfs:comment xml:lang="it">Questa classe rappresenta un account come quello che può possedere un utente su un social network.</rdfs:comment>
        <rdfs:comment xml:lang="en">This class represents a user account, such as the account owned by a person on a social network.</rdfs:comment>
        <rdfs:isDefinedBy rdf:resource="https://w3id.org/italia/onto/SM"></rdfs:isDefinedBy>
        <rdfs:label xml:lang="it">Account utente</rdfs:label>
        <rdfs:label xml:lang="en">User account</rdfs:label>
        <prov:wasInfluencedBy rdf:resource="http://rdfs.org/sioc/ns#"></prov:wasInfluencedBy>
        <prov:wasInfluencedBy rdf:resource="http://xmlns.com/foaf/0.1/OnlineAccount"></prov:wasInfluencedBy>
    </owl:Class>



    <!-- https://w3id.org/italia/onto/SM/WebSite -->

    <owl:Class rdf:about="https://w3id.org/italia/onto/SM/WebSite">
        <rdfs:subClassOf rdf:resource="https://w3id.org/italia/onto/l0/Object"></rdfs:subClassOf>
        <rdfs:subClassOf>
            <owl:Restriction>
                <owl:onProperty rdf:resource="https://w3id.org/italia/onto/SM/isWebSiteOf"></owl:onProperty>
                <owl:qualifiedCardinality rdf:datatype="http://www.w3.org/2001/XMLSchema#nonNegativeInteger">1</owl:qualifiedCardinality>
                <owl:onClass rdf:resource="https://w3id.org/italia/onto/SM/OnlineContactPoint"></owl:onClass>
            </owl:Restriction>
        </rdfs:subClassOf>
        <rdfs:comment xml:lang="it">Questa classe rappresenta il sito web di riferimento dell'organizzazione.</rdfs:comment>
        <rdfs:comment xml:lang="en">This class represents the web site of refernce of the organization.</rdfs:comment>
        <rdfs:isDefinedBy rdf:resource="https://w3id.org/italia/onto/SM"></rdfs:isDefinedBy>
        <rdfs:label xml:lang="it">Sito Web</rdfs:label>
        <rdfs:label xml:lang="en">Web site</rdfs:label>
        <prov:wasInfluencedBy rdf:resource="http://schema.org/WebSite"></prov:wasInfluencedBy>
        <prov:wasInfluencedBy rdf:resource="http://xmlns.com/foaf/0.1/Document"></prov:wasInfluencedBy>
    </owl:Class>



    <!-- https://w3id.org/italia/onto/l0/Characteristic -->

    <owl:Class rdf:about="https://w3id.org/italia/onto/l0/Characteristic"></owl:Class>



    <!-- https://w3id.org/italia/onto/l0/Concept -->

    <owl:Class rdf:about="https://w3id.org/italia/onto/l0/Concept"></owl:Class>



    <!-- https://w3id.org/italia/onto/l0/Description -->

    <owl:Class rdf:about="https://w3id.org/italia/onto/l0/Description"></owl:Class>



    <!-- https://w3id.org/italia/onto/l0/Object -->

    <owl:Class rdf:about="https://w3id.org/italia/onto/l0/Object"></owl:Class>



    <!--
    ///////////////////////////////////////////////////////////////////////////////////////
    //
    // Individuals
    //
    ///////////////////////////////////////////////////////////////////////////////////////
     -->




    <!-- http://spcdata.digitpa.gov.it/browse/page/Amministrazione/agid -->

    <owl:NamedIndividual rdf:about="http://spcdata.digitpa.gov.it/browse/page/Amministrazione/agid">
        <rdf:type rdf:resource="http://dati.gov.it/onto/dcatapit#Agent"></rdf:type>
        <rdf:type rdf:resource="http://xmlns.com/foaf/0.1/Agent"></rdf:type>
        <dct:identifier>agid</dct:identifier>
        <foaf:name xml:lang="it">Agenzia per l'Italia Digitale</foaf:name>
        <foaf:name xml:lang="en">Italian Digital Agency</foaf:name>
    </owl:NamedIndividual>



    <!-- https://w3id.org/italia/data/contact-point/onto-agid -->

    <owl:NamedIndividual rdf:about="https://w3id.org/italia/data/contact-point/onto-agid">
        <rdf:type rdf:resource="http://www.w3.org/2006/vcard/ns#Kind"></rdf:type>
        <rdf:type rdf:resource="http://www.w3.org/2006/vcard/ns#Organization"></rdf:type>
        <vcard:fn>banche dati e open data</vcard:fn>
        <vcard:hasEmail rdf:resource="mailto:info@dati.gov.it"></vcard:hasEmail>
    </owl:NamedIndividual>



    <!-- https://w3id.org/italia/data/distribution/SMAPIT-JSON-LD -->

    <owl:NamedIndividual rdf:about="https://w3id.org/italia/data/distribution/SMAPIT-JSON-LD">
        <rdf:type rdf:resource="https://w3id.org/italia/onto/ADMS/SemanticAssetDistribution"></rdf:type>
        <dct:description xml:lang="it">Questa è la distribuzione JSON-LD dell'ontologia dei social media - Internet</dct:description>
        <dct:description xml:lang="en">This is the distribution in JSON-LD of the social media - Internet ontology</dct:description>
        <dct:format rdf:resource="http://publications.europa.eu/resource/authority/file-type/JSON_LD"></dct:format>
        <dct:license rdf:resource="https://w3id.org/italia/controlled-vocabulary/licences/A21_CCBY40"></dct:license>
        <dct:title xml:lang="it">Distribuzione JSON-LD ontologia SM-AP_IT</dct:title>
        <dct:title xml:lang="en">JSON-LD distribution of SM-AP_IT Ontology</dct:title>
        <dcat:accessURL rdf:resource="https://raw.githubusercontent.com/italia/daf-ontologie-vocabolari-controllati/master/Ontologie/SM/latest"></dcat:accessURL>
        <dcat:downloadURL rdf:resource="https://raw.githubusercontent.com/italia/daf-ontologie-vocabolari-controllati/master/Ontologie/SM/latest/SM-AP_IT.jsonld"></dcat:downloadURL>
    </owl:NamedIndividual>



    <!-- https://w3id.org/italia/data/distribution/SMAPIT-RDF-TURTLE -->

    <owl:NamedIndividual rdf:about="https://w3id.org/italia/data/distribution/SMAPIT-RDF-TURTLE">
        <rdf:type rdf:resource="https://w3id.org/italia/onto/ADMS/SemanticAssetDistribution"></rdf:type>
        <dct:description xml:lang="it">Questa è la distribuzione RDF/Turtle dell'ontologia dei social media - Internet</dct:description>
        <dct:description xml:lang="en">This is the distribution in RDF/turtle of the social media - Internet ontology</dct:description>
        <dct:format rdf:resource="http://publications.europa.eu/resource/authority/file-type/RDF_TURTLE"></dct:format>
        <dct:license rdf:resource="https://w3id.org/italia/controlled-vocabulary/licences/A21_CCBY40"></dct:license>
        <dct:title xml:lang="it">Distribuzione RDF/Turtle ontologia SM-AP_IT</dct:title>
        <dct:title xml:lang="en">RDF/Turtle distribution of SM-AP_IT Ontology</dct:title>
        <dcat:accessURL rdf:resource="https://raw.githubusercontent.com/italia/daf-ontologie-vocabolari-controllati/master/Ontologie/SM/latest"></dcat:accessURL>
        <dcat:downloadURL rdf:resource="https://raw.githubusercontent.com/italia/daf-ontologie-vocabolari-controllati/master/Ontologie/SM/latest/SM-AP_IT.ttl"></dcat:downloadURL>
    </owl:NamedIndividual>



    <!-- https://w3id.org/italia/data/distribution/SMAPIT-RDF-XML -->

    <owl:NamedIndividual rdf:about="https://w3id.org/italia/data/distribution/SMAPIT-RDF-XML">
        <rdf:type rdf:resource="https://w3id.org/italia/onto/ADMS/SemanticAssetDistribution"></rdf:type>
        <dct:description xml:lang="it">Questa è la distribuzione RDF/XML dell'ontologia dei social media - Internet</dct:description>
        <dct:description xml:lang="en">This is the distribution in RDF/XML of the social media - Internet ontology</dct:description>
        <dct:format rdf:resource="http://publications.europa.eu/resource/authority/file-type/RDF_XML"></dct:format>
        <dct:license rdf:resource="https://w3id.org/italia/controlled-vocabulary/licences/A21_CCBY40"></dct:license>
        <dct:title xml:lang="it">Distribuzione RDF/XML ontologia SM-AP_IT</dct:title>
        <dct:title xml:lang="en">RDF/XML distribution of SM-AP_IT Ontology</dct:title>
        <dcat:accessURL rdf:resource="https://raw.githubusercontent.com/italia/daf-ontologie-vocabolari-controllati/master/Ontologie/SM/latest"></dcat:accessURL>
        <dcat:downloadURL rdf:resource="https://raw.githubusercontent.com/italia/daf-ontologie-vocabolari-controllati/master/Ontologie/SM/latest/SM-AP_IT.rdf"></dcat:downloadURL>
    </owl:NamedIndividual>



    <!-- https://w3id.org/italia/data/organization/public-organization/td -->

    <owl:NamedIndividual rdf:about="https://w3id.org/italia/data/organization/public-organization/td">
        <rdf:type rdf:resource="http://dati.gov.it/onto/dcatapit#Agent"></rdf:type>
        <rdf:type rdf:resource="http://xmlns.com/foaf/0.1/Agent"></rdf:type>
        <dct:identifier>TD</dct:identifier>
        <foaf:name xml:lang="en">Digital Transformation Team</foaf:name>
        <foaf:name xml:lang="it">Team per la Trasformazione Digitale</foaf:name>
    </owl:NamedIndividual>



    <!-- https://w3id.org/italia/data/organization/support-unit/cnr-Z6HZEH/stlab -->

    <owl:NamedIndividual rdf:about="https://w3id.org/italia/data/organization/support-unit/cnr-Z6HZEH/stlab">
        <l0:name xml:lang="en">Institute of Cognitive Sciences and Technologies of the Italian Research Council (CNR) - Semantic Technology Laboratory (STLab)</l0:name>
        <l0:name xml:lang="it">Istituto di Scienze e Tecnologie della Cognizione del CNR - Semantic Technology Lab (STLab)</l0:name>
        <dct:identifier>cnr - Z6HZEH - STLab</dct:identifier>
    </owl:NamedIndividual>



    <!-- https://w3id.org/italia/data/project/DAF -->

    <owl:NamedIndividual rdf:about="https://w3id.org/italia/data/project/DAF">
        <rdf:type rdf:resource="https://w3id.org/italia/onto/ADMS/Project"></rdf:type>
        <l0:name xml:lang="it">Data &amp; Analytics Framework</l0:name>
    </owl:NamedIndividual>



    <!-- https://w3id.org/italia/data/project/OntoPiA -->

    <owl:NamedIndividual rdf:about="https://w3id.org/italia/data/project/OntoPiA">
        <rdf:type rdf:resource="https://w3id.org/italia/onto/ADMS/Project"></rdf:type>
        <l0:name xml:lang="it">OntoPiA - la rete di ontologie della pubblica amministrazione italiana</l0:name>
    </owl:NamedIndividual>



    <!-- https://w3id.org/italia/onto/SM -->

    <owl:NamedIndividual rdf:about="https://w3id.org/italia/onto/SM">
        <rdf:type rdf:resource="https://w3id.org/italia/onto/ADMS/SemanticAsset"></rdf:type>
    </owl:NamedIndividual>



    <!-- https://w3id.org/italia/onto/SM/PEC -->

    <owl:NamedIndividual rdf:about="https://w3id.org/italia/onto/SM/PEC"></owl:NamedIndividual>



    <!-- https://w3id.org/italia/onto/SM/TraditionalEmail -->

    <owl:NamedIndividual rdf:about="https://w3id.org/italia/onto/SM/TraditionalEmail"></owl:NamedIndividual>
</rdf:RDF>
<!-- Generated by the OWL API (version 4.5.9.2019-02-01T07:24:44Z) https://github.com/owlcs/owlapi -->